<?xml version="1.0"?>
<rdf:RDF xmlns:pns="http://data.press.net/ontology/stuff/" xmlns:dcterms="http://purl.org/dc/terms/" xmlns:pne="http://data.press.net/ontology/event/" xmlns:foaf="http://xmlns.com/foaf/0.1/" xmlns:vs="http://www.w3.org/2003/06/sw-vocab-status/ns#" xmlns:owl="http://www.w3.org/2002/07/owl#" xmlns:xsd="http://www.w3.org/2001/XMLSchema#" xmlns:rdfs="http://www.w3.org/2000/01/rdf-schema#" xmlns:rdf="http://www.w3.org/1999/02/22-rdf-syntax-ns#" xmlns:event="http://purl.org/NET/c4dm/event.owl#">
    <owl:Ontology rdf:about="http://data.press.net/ontology/event/">
        <dcterms:title xml:lang="en">SNaP Event Ontology</dcterms:title>
        <dcterms:created rdf:datatype="http://www.w3.org/2001/XMLSchema#date">2011-07-28</dcterms:created>
        <dcterms:modified rdf:datatype="http://www.w3.org/2001/XMLSchema#date">2012-04-20</dcterms:modified>
        <dcterms:license rdf:resource="http://creativecommons.org/licenses/by-nd/3.0/" />
        <rdfs:comment xml:lang="en">The Event Ontology models news-worthy events and their relationship to news assets and stuff (simple entities) in the world.</rdfs:comment>
        <foaf:maker>
            <foaf:Person rdf:about="http://uk.linkedin.com/in/jarredmcginnis">
                <foaf:name>Jarred McGinnis</foaf:name>
            </foaf:Person>
        </foaf:maker>
        <foaf:maker>
            <foaf:Person rdf:about="http://uk.linkedin.com/in/paulwilton">
                <foaf:name>Paul Wilton</foaf:name>
            </foaf:Person>
        </foaf:maker>
        <foaf:maker>
            <foaf:Person rdf:about="http://uk.linkedin.com/in/pauliharman">
                <foaf:name>Paul Harman</foaf:name>
            </foaf:Person>
        </foaf:maker>
        <owl:versionInfo rdf:datatype="http://www.w3.org/2001/XMLSchema#string">0.5.0</owl:versionInfo>
    </owl:Ontology>
    <owl:Class rdf:about="http://data.press.net/ontology/event/Event">
        <rdfs:subClassOf rdf:resource="http://purl.org/NET/c4dm/event.owl#Event" />
        <rdfs:subClassOf rdf:resource="http://data.press.net/ontology/stuff/Stuff" />
        <rdfs:label xml:lang="en">Generic Event Class</rdfs:label>
        <rdfs:comment xml:lang="en">Generic Event Class, a subclass of event:Event. The Event class also subclasses pnt:Stuff as it is a Compound domain entity, this inheritance means news assets can be tagged with Events</rdfs:comment>
        <rdfs:isDefinedBy rdf:resource="http://data.press.net/ontology/event/" />
        <vs:term_status>testing</vs:term_status>
    </owl:Class>
    <owl:TransitiveProperty rdf:about="http://data.press.net/ontology/event/subEventOf">
        <rdfs:domain rdf:resource="http://data.press.net/ontology/event/Event" />
        <rdfs:range rdf:resource="http://data.press.net/ontology/event/Event" />
        <rdfs:label xml:lang="en">Transitive Property defining a parent-child relationship between events</rdfs:label>
        <rdfs:comment xml:lang="en">Transitive Property defining a parent-child relationship between events. Event Y is a sub event of Event X</rdfs:comment>
        <rdfs:isDefinedBy rdf:resource="http://data.press.net/ontology/event/" />
        <vs:term_status>testing</vs:term_status>
    </owl:TransitiveProperty>
    <owl:DatatypeProperty rdf:about="http://data.press.net/ontology/event/title">
        <rdfs:subPropertyOf rdf:resource="http://purl.org/dc/terms/title" />
        <rdfs:subPropertyOf rdf:resource="http://data.press.net/ontology/stuff/label" />
        <rdfs:domain rdf:resource="http://data.press.net/ontology/event/Event" />
        <rdfs:range rdf:resource="http://www.w3.org/2001/XMLSchema#string" />
        <rdfs:label xml:lang="en">An Event title</rdfs:label>
        <rdfs:comment xml:lang="en">Property for expressing an event title. Datatype is String</rdfs:comment>
        <rdfs:isDefinedBy rdf:resource="http://data.press.net/ontology/event/" />
        <vs:term_status>testing</vs:term_status>
    </owl:DatatypeProperty>
    <owl:DatatypeProperty rdf:about="http://data.press.net/ontology/event/summary">
        <rdfs:subPropertyOf rdf:resource="http://purl.org/dc/terms/abstract" />
        <rdfs:subPropertyOf rdf:resource="http://data.press.net/ontology/stuff/comment" />
        <rdfs:domain rdf:resource="http://data.press.net/ontology/event/Event" />
        <rdfs:range rdf:resource="http://www.w3.org/2001/XMLSchema#string" />
        <rdfs:label xml:lang="en">An Event summary</rdfs:label>
        <rdfs:comment xml:lang="en">Property for expressing an event summary. Datatype is String</rdfs:comment>
        <rdfs:isDefinedBy rdf:resource="http://data.press.net/ontology/event/" />
        <vs:term_status>testing</vs:term_status>
    </owl:DatatypeProperty>
    <owl:ObjectProperty rdf:about="http://data.press.net/ontology/event/theme">
        <rdfs:subPropertyOf rdf:resource="http://data.press.net/ontology/stuff/notablyAssociatedWith" />
        <rdfs:domain rdf:resource="http://data.press.net/ontology/event/Event" />
        <rdfs:range rdf:resource="http://data.press.net/ontology/stuff/Intangible" />
        <rdfs:label xml:lang="en">Associates an Event with an intangible theme</rdfs:label>
        <rdfs:comment xml:lang="en">Property for expressing the theme of an event, its range is pns:Intangible</rdfs:comment>
        <rdfs:isDefinedBy rdf:resource="http://data.press.net/ontology/event/" />
        <vs:term_status>testing</vs:term_status>
    </owl:ObjectProperty>
</rdf:RDF>