<?xml version="1.0" encoding="utf-8"?>
<?xml-stylesheet href="./ns-schema.xsl" type="text/xsl" media="screen"?>
<!DOCTYPE rdf:RDF [
 <!ENTITY rdfs  'http://www.w3.org/2000/01/rdf-schema#'>
 <!ENTITY owl  'http://www.w3.org/2002/07/owl#'>
 <!ENTITY whois  'http://www.kanzaki.com/ns/whois'>
 <!ENTITY foaf  'http://xmlns.com/foaf/0.1/'>
 <!ENTITY geo 'http://www.w3.org/2003/01/geo/wgs84_pos#'>
 <!ENTITY cal 'http://www.w3.org/2002/12/cal/icaltzd#'>
]>
<rdf:RDF
  xmlns:rdf="http://www.w3.org/1999/02/22-rdf-syntax-ns#"
  xmlns:rdfs="&rdfs;"
  xmlns:foaf="&foaf;"
  xmlns:owl="&owl;"
  xmlns:ex="http://purl.org/net/ns/ex#"
  xmlns="&whois;#"
  xmlns:ont="http://purl.org/net/ns/ontology-annot#"
  xml:base="&whois;"
  >

 <owl:Ontology rdf:about="">
  <owl:imports rdf:resource="http://www.kanzaki.com/ns/dliser.rdf"/>
  <rdfs:label>Who&apos;s who description vocabulary</rdfs:label>
  <rdfs:comment>An experimental vocabulary to describe a person&apos;s profile/history. Properties 'whois:stage' describe one&apos;s stage of life (whois:Stage). Similar to Ian Davis&apos; BIO: vocab, however, while BIO: describes events on specific dates, this vocabulary uses whois:since/whois:until so that it can describe a period of time. This also includes such properties as career or honor to be used as a personal resume. Examples included in this document. </rdfs:comment>
  <rdfs:comment xml:lang="ja">プロフィールを記述するための実験ボキャブラリ。Ian DavisのBIO: vocabと似ていますが、BIO:がEventという単位を基本に特定の日を記述するのに対し、こちらはライフサイクルのステージという概念で期間も記述できるようにしています。career, honorといったプロパティは、履歴メタデータの記述にも使えます。</rdfs:comment>
  <ont:created>2003-07-08</ont:created>
  <ont:modified>2012-09-16</ont:modified>
  <owl:versionInfo>Version 0.5.4. added whois:publication.</owl:versionInfo>
  <ont:creator>
   <foaf:Person rdf:about="urn:pin:MK705">
    <foaf:name xml:lang="ja">神崎正英</foaf:name>
    <rdfs:seeAlso rdf:resource="http://www.kanzaki.com/info/webwho.rdf"/>
   </foaf:Person>
  </ont:creator>
 </owl:Ontology>

<!-- ==== Class definitions ==== -->

 <owl:Class rdf:ID="Place">
  <rdfs:label>Place</rdfs:label>
  <rdfs:comment>A place -- this can be the domain of both contact: vocab and geo: vocab.</rdfs:comment>
  <rdfs:comment xml:lang="ja">場所を表すクラス</rdfs:comment>
  <rdfs:subClassOf rdf:resource="&geo;SpatialThing"/>
  <rdfs:isDefinedBy rdf:resource=""/>
 </owl:Class>

 <owl:Class rdf:ID="Stage">
  <rdfs:label>Stage</rdfs:label>
  <rdfs:comment>A stage of life. A distinct time period in a sequence of one&apos;s life cycle.</rdfs:comment>
  <rdfs:comment xml:lang="ja">人生のあるステージ。人のライフサイクルの中での、はっきりと区切られる一時期</rdfs:comment>
  <rdfs:isDefinedBy rdf:resource=""/>
 </owl:Class>

 <owl:Class rdf:ID="Education">
  <rdfs:label>Educaton (stage)</rdfs:label>
  <rdfs:comment>A period of education in one&apos;s academic career, as a stage of life. NOT an activity of learning.</rdfs:comment>
  <rdfs:comment xml:lang="ja">ライフステージ中での、学業期間。学歴を表す</rdfs:comment>
  <rdfs:subClassOf rdf:resource="#Stage"/>
  <rdfs:isDefinedBy rdf:resource=""/>
 </owl:Class>

 <owl:Class rdf:ID="Job">
  <rdfs:label>Job (stage)</rdfs:label>
  <rdfs:comment>A period of job in one&apos;s professional career, as a stage of life. NOT an activity of working.</rdfs:comment>
  <rdfs:comment xml:lang="ja">ライフステージ中でのある職業の期間。職歴を表す</rdfs:comment>
  <rdfs:subClassOf rdf:resource="#Stage"/>
  <rdfs:isDefinedBy rdf:resource=""/>
 </owl:Class>



<!-- ==== Property definitions ==== -->
<!-- Properties to describe a Person -->
 <owl:ObjectProperty rdf:ID="description">
  <rdfs:label>Description</rdfs:label>
  <rdfs:comment>General description of a person&apos;s activities. Use to describe something that does not fit into a Stage.</rdfs:comment>
  <rdfs:comment xml:lang="ja">人の活動の一般的な記述。stage、career、planの上位プロパティ。一つのステージに収まらない事項を記述するためにも使える</rdfs:comment>
  <rdfs:domain rdf:resource="&foaf;Person"/>
  <rdfs:range rdf:resource="&owl;Thing"/>
  <rdfs:isDefinedBy rdf:resource=""/>
 </owl:ObjectProperty>

 <owl:ObjectProperty rdf:ID="stage">
  <rdfs:label>Stage</rdfs:label>
  <rdfs:comment>Describes an aspect of one&apos;s personal history. <!-- no more a super property of career.--></rdfs:comment>
  <rdfs:comment xml:lang="ja">人の履歴のにおけるある切り口を記述する</rdfs:comment>
  <rdfs:subPropertyOf rdf:resource="#description"/>
  <rdfs:range rdf:resource="#Stage"/>
  <!-- <rdfs:range rdf:resource="rdfs:Resource"/> -->
  <rdfs:isDefinedBy rdf:resource=""/>
 </owl:ObjectProperty>

 <owl:ObjectProperty rdf:ID="career">
  <rdfs:label>Career</rdfs:label>
  <rdfs:comment>A job, education or any achievement in one&apos;s life, which can be specific to a stage of life (object = #Stage) or in general (object = any).</rdfs:comment>
  <rdfs:comment xml:lang="ja">人生における職業、教育、業績などを記述する</rdfs:comment>
  <rdfs:subPropertyOf rdf:resource="#description"/>
  <rdfs:isDefinedBy rdf:resource=""/>
 </owl:ObjectProperty>

 <owl:ObjectProperty rdf:ID="academicCareer">
  <rdfs:label>Academic Career</rdfs:label>
  <rdfs:comment>an educational career in one&apos;s personal history.</rdfs:comment>
  <rdfs:subPropertyOf rdf:resource="#career"/>
  <rdfs:comment xml:lang="ja">学歴を記述する。careerのサブプロパティ</rdfs:comment>
  <rdfs:range rdf:resource="#Education"/>
  <rdfs:isDefinedBy rdf:resource=""/>
 </owl:ObjectProperty>

 <owl:ObjectProperty rdf:ID="professionalCareer">
  <rdfs:label>Professional Career</rdfs:label>
  <rdfs:comment>a professional or business career in one&apos;s personal history.</rdfs:comment>
  <rdfs:comment xml:lang="ja">職歴を記述する。careerのサブプロパティ</rdfs:comment>
  <rdfs:subPropertyOf rdf:resource="#career"/>
  <rdfs:range rdf:resource="#Job"/>
  <rdfs:isDefinedBy rdf:resource=""/>
 </owl:ObjectProperty>

 <owl:ObjectProperty rdf:ID="achievement">
  <rdfs:label>Achievement</rdfs:label>
  <rdfs:comment>a one&apos;s achievement in general. Note you can use foaf:pastProject for a specific achievement.</rdfs:comment>
  <rdfs:comment xml:lang="ja">業績を記述する。careerのサブプロパティ</rdfs:comment>
  <rdfs:subPropertyOf rdf:resource="#career"/>
  <rdfs:isDefinedBy rdf:resource=""/>
 </owl:ObjectProperty>

 <owl:ObjectProperty rdf:ID="honor">
  <rdfs:label>Honor</rdfs:label>
  <rdfs:comment>an honor that one has been rewarded.</rdfs:comment>
  <rdfs:comment xml:lang="ja">顕彰歴を記述する。careerのサブプロパティ</rdfs:comment>
  <rdfs:subPropertyOf rdf:resource="#career"/>
  <rdfs:isDefinedBy rdf:resource=""/>
 </owl:ObjectProperty>

 <owl:ObjectProperty rdf:ID="publication">
  <rdfs:label>Publication</rdfs:label>
  <rdfs:comment>a one&apos;s publication in general. Note foaf:publications describes publication list page.</rdfs:comment>
  <rdfs:comment xml:lang="ja">出版物、論文を記述する。descriptionのサブプロパティ</rdfs:comment>
  <rdfs:subPropertyOf rdf:resource="#description"/>
  <rdfs:isDefinedBy rdf:resource=""/>
 </owl:ObjectProperty>




 <owl:ObjectProperty rdf:ID="where">
  <rdfs:label>Where</rdfs:label>
  <rdfs:comment>Place which relates to a stage of life. The range is whois:Place to have structured description. Use bio:place for literal value</rdfs:comment>
  <rdfs:comment xml:lang="ja">あるステージの場所を記述する</rdfs:comment>
  <rdfs:domain rdf:resource="#Stage"/>
  <rdfs:range rdf:resource="#Place"/>
  <rdfs:isDefinedBy rdf:resource=""/>
 </owl:ObjectProperty>

 <owl:DatatypeProperty rdf:ID="place">
  <rdfs:label>Place</rdfs:label>
  <rdfs:comment>Place which relates to a stage of life. Literal version of 'where'. ":x whois:place 'y'." implies ":x whois:where [rdfs:label 'y'].".</rdfs:comment>
  <rdfs:comment xml:lang="ja">あるステージの場所をリテラルとして記述する</rdfs:comment>
  <rdfs:domain rdf:resource="#Stage"/>
  <rdfs:isDefinedBy rdf:resource=""/>
 </owl:DatatypeProperty>

 <owl:ObjectProperty rdf:ID="what">
  <rdfs:label>What</rdfs:label>
  <rdfs:comment>Specifies a topic in a stage of life. The range is owl:Thing to have structured description. Use dc:description for literal description, or dc:subject for keywords.</rdfs:comment>
  <rdfs:comment xml:lang="ja">あるステージを特徴付けるトピックを記述する（目的語はリテラルではないことに注意）</rdfs:comment>
  <rdfs:subPropertyOf rdf:resource="&foaf;topic"/>
  <rdfs:domain rdf:resource="#Stage"/>
  <rdfs:range rdf:resource="&owl;Thing"/>
  <rdfs:isDefinedBy rdf:resource=""/>
 </owl:ObjectProperty>

 <owl:DatatypeProperty rdf:ID="when">
  <rdfs:label>When</rdfs:label>
  <rdfs:comment>date/time which is related to a stage of life. Super property of since and until. W3C-DTF format value is assumed (i.e. can be yyyy, yyyy-mm, yyyy-mm-dd etc).</rdfs:comment>
  <rdfs:comment xml:lang="ja">あるステージの時期を記述するための上位プロパティ</rdfs:comment>
  <rdfs:domain rdf:resource="#Stage"/>
  <rdfs:range rdf:resource="&rdfs;Literal"/>
  <rdfs:isDefinedBy rdf:resource=""/>
 </owl:DatatypeProperty>

 <owl:DatatypeProperty rdf:ID="since">
  <rdfs:label>Since</rdfs:label>
  <rdfs:comment>date when a stage of life started. </rdfs:comment>
  <rdfs:comment xml:lang="ja">あるステージが始まったときを記述する。whenのサブプロパティ</rdfs:comment>
  <rdfs:subPropertyOf rdf:resource="#when"/>
  <rdfs:subPropertyOf rdf:resource="&cal;dtstart"/>
  <rdfs:isDefinedBy rdf:resource=""/>
 </owl:DatatypeProperty>

 <owl:DatatypeProperty rdf:ID="until">
  <rdfs:label>Until</rdfs:label>
  <rdfs:comment>date when a stage of life ended.</rdfs:comment>
  <rdfs:comment xml:lang="ja">あるステージが終わったときを記述する。whenのサブプロパティ</rdfs:comment>
  <rdfs:subPropertyOf rdf:resource="#when"/>
  <rdfs:subPropertyOf rdf:resource="&cal;dtend"/>
  <rdfs:isDefinedBy rdf:resource=""/>
 </owl:DatatypeProperty>

 <owl:DatatypeProperty rdf:ID="born">
  <rdfs:label>Born</rdfs:label>
  <rdfs:comment>One&apos;s birthday. This can be used in place of 'whois:since' where the 'whois:Stage' is one&apos;s first stage.</rdfs:comment>
  <rdfs:comment xml:lang="ja">誕生日を記述する。sinceのサブプロパティ（人生の最初のステージの始まり）</rdfs:comment>
  <rdfs:subPropertyOf rdf:resource="#since"/>
  <rdfs:isDefinedBy rdf:resource=""/>
 </owl:DatatypeProperty>


 <owl:ObjectProperty rdf:ID="plan">
  <rdfs:label>Plan</rdfs:label>
  <rdfs:comment>General description of a person&apos;s future activities. Note past activity can be described with #career.</rdfs:comment>
  <rdfs:comment xml:lang="ja">人の将来の活動予定を記述する</rdfs:comment>
  <rdfs:subPropertyOf rdf:resource="#description"/>
  <rdfs:isDefinedBy rdf:resource=""/>
 </owl:ObjectProperty>







<!-- ==== External names ==== -->
 <owl:Class rdf:about="&geo;SpatialThing"/>
 <owl:ObjectProperty rdf:about="&foaf;topic"/>
 <owl:DatatypeProperty rdf:about="&cal;dtstart"/>
 <owl:DatatypeProperty rdf:about="&cal;dtend"/>


<!-- ==== Examples ==== -->
<ex:Example>
 <rdfs:comment>Simple, unstructured description. Class tags 'whois:Stage' are omitted by using rdf:parseType='Resource', and 'whois:place' property is used instead of 'whois:where' to have literal values). Note the 'whois:born' (instead of 'whois:since') implies (the omitted 'whois:Stage' is) one&apos;s first stage of life, and the stage without 'whois:until' denotes the current phase.</rdfs:comment>
 <rdfs:comment xml:lang="ja">最もシンプルな例（rdf:parseType='Resource'を用いて'whois:Stage'も省略）。場所を単なるリテラルとするためにwhois:placeを用いている。whois:bornを持つwhois:Stageは出身地での人生の最初のステージを示す。また、whois:untilのないwhois:Stageは現在のステージ。</rdfs:comment>
 <!--http://internetalchemy.org/vocab/bio/0.1/-->
 <ex:image rdf:resource="http://www.kanzaki.com/works/2007/misc/whois-vocab-sample1.png"/> <ex:pfx>whois:</ex:pfx>
 <ex:code><![CDATA[
<foaf:Person>
 <foaf:name>Masahide Kanzaki</foaf:name>
 <whois:stage rdf:parseType='Resource'>
  <whois:place>Tokyo, Japan</whois:place>
  <whois:since>1982</whois:since>
 </whois:stage>
 <whois:stage rdf:parseType='Resource'>
  <whois:place>Suzuka, Mie, Japan</whois:place>
  <whois:born>1960</whois:born>
  <whois:until>1978</whois:until>
 </whois:stage>
</foaf:Person>
 ]]></ex:code>
 <ex:exampleOf rdf:resource=""/>
</ex:Example>

<ex:Example>
 <rdfs:comment>A structured description of a stage of one&apos;s life. Note properties from contact: and geo: vocabulary can be used with whois:Place.</rdfs:comment>
 <rdfs:comment xml:lang="ja">whois:where、whois:whatの内容にほかの語彙を含む構造的な記述を利用した例。</rdfs:comment>
 <ex:code><![CDATA[
<whois:stage>
 <whois:Stage>
  <whois:since>1987</whois:since>
  <whois:until>1989</whois:until>
  <whois:where>
   <whois:Place geo:lat="40.794" geo:long="-73.972">
    <contact:country>U.S.A.</contact:country>
    <contact:city>New York</contact:city>
   </whois:Place>
  </whois:where>
  <whois:what>
   <wn:School>
    <foaf:homepage rdf:resource="http://www.columbia.edu/cu/business/"/>
   </wn:School>
  </whois:what>
 </whois:Stage>
</whois:stage>
 ]]></ex:code>
 <ex:exampleOf rdf:resource=""/>
</ex:Example>

<ex:Example>
 <rdfs:comment>Combined with other FOAF vocabularies, we can make a personal resume as a metadata. A career can be described with 'whois:career' property + 'whois:Education' or 'whois:Job' class, or sub properties 'whois:academicCareer' and 'whois:professionalCareer' that denote appropriate classes as range.</rdfs:comment>
 <rdfs:comment xml:lang="ja">'whois:career'プロパティと'whois:Education', 'whois:Job'クラスを使って、履歴メタデータを記述する例。これらはサブプロパティ'whois:academicCareer'および'whois:professionalCareer'によってクラスを暗黙的に示すこともできる。</rdfs:comment>
 <ex:code><![CDATA[
<foaf:Person>
 <foaf:name>Masahide Kanzaki</foaf:name>
 <foaf:homepage rdf:resource="http://www.kanzaki.com/"/>
 <whois:stage whois:born="1960" rdfs:label="Suzuka, Mie, Japan"/>
 <whois:career>
  <whois:Education>
   <rdfs:label>Columbia Business School</rdfs:label>
   <whois:since>1987</whois:since>
   <whois:until>1989</whois:until>
  </whois:Education>
 </whois:career>
 <whois:career>
  <whois:Job>
   <rdfs:label>A virtual corporation</rdfs:label>
   <whois:since>1989</whois:since>
   <whois:until>2002</whois:until>
  </whois:Job>
 </whois:career>
 <whois:professionalCareer rdf:parseType="Resource">
  <rdfs:label>Keio University</rdfs:label>
  <whois:since>2003</whois:since>
 </whois:professionalCareer>
</foaf:Person>
 ]]></ex:code>
 <ex:exampleOf rdf:resource=""/>
</ex:Example>

</rdf:RDF>

