<?xml version="1.0"?>


<!DOCTYPE rdf:RDF [
    <!ENTITY dc "http://purl.org/dc/terms/" >
    <!ENTITY vann "http://purl.org/vocab/vann/" >
    <!ENTITY geo "http://geovocab.org/spatial#" >
    <!ENTITY cc "http://creativecommons.org/ns#" >
    <!ENTITY owl "http://www.w3.org/2002/07/owl#" >
    <!ENTITY voaf "http://purl.org/vocommons/voaf#" >
    <!ENTITY cidoc-crm "http://erlangen-crm.org/current/" >
    <!ENTITY xsd "http://www.w3.org/2001/XMLSchema#" >
    <!ENTITY skos "http://www.w3.org/2004/02/skos/core#" >
    <!ENTITY rdfs "http://www.w3.org/2000/01/rdf-schema#" >
    <!ENTITY rdf "http://www.w3.org/1999/02/22-rdf-syntax-ns#" >
]>


<rdf:RDF xmlns="http://lawd.info/ontology/"
     xml:base="http://lawd.info/ontology/"
     xmlns:dc="http://purl.org/dc/terms/"
     xmlns:geo="http://geovocab.org/spatial#"
     xmlns:vann="http://purl.org/vocab/vann/"
     xmlns:voaf="http://purl.org/vocommons/voaf#"
     xmlns:rdfs="http://www.w3.org/2000/01/rdf-schema#"
     xmlns:owl="http://www.w3.org/2002/07/owl#"
     xmlns:xsd="http://www.w3.org/2001/XMLSchema#"
     xmlns:rdf="http://www.w3.org/1999/02/22-rdf-syntax-ns#"
     xmlns:cidoc-crm="http://erlangen-crm.org/current/"
     xmlns:skos="http://www.w3.org/2004/02/skos/core#"
     xmlns:cc="http://creativecommons.org/ns#">
    <owl:Ontology rdf:about="http://lawd.info/ontology/">
        <dc:title>Linking Ancient World Data Ontology</dc:title>
        <vann:preferredNamespacePrefix>lawd</vann:preferredNamespacePrefix>
        <dc:issued>2013-03-28</dc:issued>
        <vann:preferredNamespaceUri>http://lawd.info/ontology/</vann:preferredNamespaceUri>
        <dc:rights>Copyright © 2013 Hugh A. Cayless</dc:rights>
        <dc:modified>2014-09-03</dc:modified>
        <dc:description>The goal of LAWD is to fill in the cracks between the data used and published by projects with a focus on the ancient world and the standard Linked Data vocablary schemes, like Dublin Core, the Open Annotation Collaboration, and CIDOC-CRM.</dc:description>
        <cc:license rdf:resource="http://creativecommons.org/license/by/3.0/"/>
        <owl:imports rdf:resource="http://erlangen-crm.org/current/"/>
        <owl:versionIRI rdf:resource="http://lawd.info/ontology/1.0/"/>
        <owl:imports rdf:resource="http://purl.org/ontology/olo/core#"/>
        <owl:imports rdf:resource="http://www.w3.org/2004/02/skos/core"/>
        <owl:imports rdf:resource="http://www.w3.org/ns/oa#"/>
        <owl:imports rdf:resource="http://www.w3.org/ns/prov-o#"/>
    </owl:Ontology>
    


    <!-- 
    ///////////////////////////////////////////////////////////////////////////////////////
    //
    // Object Properties
    //
    ///////////////////////////////////////////////////////////////////////////////////////
     -->

    


    <!-- http://lawd.info/ontology/conjunctOf -->

    <owl:ObjectProperty rdf:about="http://lawd.info/ontology/conjunctOf">
        <rdf:type rdf:resource="&owl;SymmetricProperty"/>
        <rdfs:comment xml:lang="en">Indicates that a piece of evidence (any subclass of lawd:EvidentiaryItem) is joined to another—for example because they co-occur.</rdfs:comment>
        <rdfs:range rdf:resource="http://lawd.info/ontology/EvidentiaryItem"/>
        <rdfs:domain rdf:resource="http://lawd.info/ontology/EvidentiaryItem"/>
    </owl:ObjectProperty>
    


    <!-- http://lawd.info/ontology/embodies -->

    <owl:ObjectProperty rdf:about="http://lawd.info/ontology/embodies">
        <rdfs:comment xml:lang="en">The relationship between a Written Work and the abstract Conceptual Work it embodies. For example, the OCT text of Homer&apos;s Iliad&apos;s relationship to the idea of Homer&apos;s Iliad.</rdfs:comment>
        <rdfs:range rdf:resource="http://lawd.info/ontology/ConceptualWork"/>
        <rdfs:domain rdf:resource="http://lawd.info/ontology/WrittenWork"/>
    </owl:ObjectProperty>
    


    <!-- http://lawd.info/ontology/foundAt -->

    <owl:ObjectProperty rdf:about="http://lawd.info/ontology/foundAt">
        <rdfs:comment xml:lang="en">The place where an artifact was discovered.</rdfs:comment>
        <rdfs:range rdf:resource="http://lawd.info/ontology/Place"/>
        <rdfs:subPropertyOf rdf:resource="http://lawd.info/ontology/where"/>
    </owl:ObjectProperty>
    


    <!-- http://lawd.info/ontology/hasAttestation -->

    <owl:ObjectProperty rdf:about="http://lawd.info/ontology/hasAttestation">
        <rdfs:comment xml:lang="en">Indicates a lawd:Attestation providing evidence for a name, etc.</rdfs:comment>
        <rdfs:range rdf:resource="http://lawd.info/ontology/Attestation"/>
    </owl:ObjectProperty>
    


    <!-- http://lawd.info/ontology/hasCitation -->

    <owl:ObjectProperty rdf:about="http://lawd.info/ontology/hasCitation">
        <rdfs:comment xml:lang="en">Indicates a Citation that contains the source for a lawd:Attestation</rdfs:comment>
        <rdfs:range rdf:resource="http://lawd.info/ontology/Citation"/>
        <rdfs:domain rdf:resource="http://lawd.info/ontology/EvidentiaryItem"/>
    </owl:ObjectProperty>
    


    <!-- http://lawd.info/ontology/hasName -->

    <owl:ObjectProperty rdf:about="http://lawd.info/ontology/hasName">
        <rdfs:comment xml:lang="en">Indicates that (e.g.) a Person or Place has a lawd:Name that is the range of the property.</rdfs:comment>
        <rdfs:range rdf:resource="http://lawd.info/ontology/Name"/>
    </owl:ObjectProperty>
    


    <!-- http://lawd.info/ontology/origin -->

    <owl:ObjectProperty rdf:about="http://lawd.info/ontology/origin">
        <rdfs:comment xml:lang="en">The place where an artifact originated.</rdfs:comment>
        <rdfs:range rdf:resource="http://lawd.info/ontology/Place"/>
        <rdfs:subPropertyOf rdf:resource="http://lawd.info/ontology/where"/>
    </owl:ObjectProperty>
    


    <!-- http://lawd.info/ontology/readingType -->

    <owl:ObjectProperty rdf:about="http://lawd.info/ontology/readingType">
        <rdfs:range rdf:resource="http://lawd.info/ontology/Reading"/>
    </owl:ObjectProperty>
    


    <!-- http://lawd.info/ontology/representedBy -->

    <owl:ObjectProperty rdf:about="http://lawd.info/ontology/representedBy">
        <owl:deprecated xml:lang="en">Will be removed in a future release.</owl:deprecated>
        <rdfs:range rdf:resource="http://lawd.info/ontology/Citation"/>
        <rdfs:domain rdf:resource="http://lawd.info/ontology/WrittenWork"/>
    </owl:ObjectProperty>
    


    <!-- http://lawd.info/ontology/represents -->

    <owl:ObjectProperty rdf:about="http://lawd.info/ontology/represents">
        <rdfs:comment xml:lang="en">Describes the relationship between a Citation or Siglum and the
      Written Work it indicates.</rdfs:comment>
        <rdfs:domain rdf:resource="http://lawd.info/ontology/Citation"/>
        <rdfs:range rdf:resource="http://lawd.info/ontology/WrittenWork"/>
        <owl:inverseOf rdf:resource="http://lawd.info/ontology/representedBy"/>
    </owl:ObjectProperty>
    


    <!-- http://lawd.info/ontology/responsibleAgent -->

    <owl:ObjectProperty rdf:about="http://lawd.info/ontology/responsibleAgent">
        <rdfs:comment xml:lang="en">Connects a work of any type to the person, group, or insitution
      responsible for the creation of the work.</rdfs:comment>
        <rdfs:range rdf:resource="http://lawd.info/ontology/Agent"/>
        <owl:inverseOf rdf:resource="http://lawd.info/ontology/responsibleFor"/>
    </owl:ObjectProperty>
    


    <!-- http://lawd.info/ontology/responsibleFor -->

    <owl:ObjectProperty rdf:about="http://lawd.info/ontology/responsibleFor">
        <rdfs:comment xml:lang="en">Connects any kind of author or creator to the work he/she/it is responsible for creating or contributing to. The author may be anonymous or fictional.</rdfs:comment>
        <rdfs:domain rdf:resource="http://lawd.info/ontology/Agent"/>
    </owl:ObjectProperty>
    


    <!-- http://lawd.info/ontology/reuseFrom -->

    <owl:ObjectProperty rdf:about="http://lawd.info/ontology/reuseFrom">
        <rdfs:comment xml:lang="en">Links an instance of text reuse to a citation of the work from which the text came.</rdfs:comment>
        <rdfs:range rdf:resource="http://lawd.info/ontology/Citation"/>
        <rdfs:domain rdf:resource="http://lawd.info/ontology/TextReuse"/>
    </owl:ObjectProperty>
    


    <!-- http://lawd.info/ontology/reuseIn -->

    <owl:ObjectProperty rdf:about="http://lawd.info/ontology/reuseIn">
        <rdfs:comment xml:lang="en">Links an instance of text reuse to a citation of the work in which the reuse appears.</rdfs:comment>
        <rdfs:range rdf:resource="http://lawd.info/ontology/Citation"/>
        <rdfs:domain rdf:resource="http://lawd.info/ontology/TextReuse"/>
    </owl:ObjectProperty>
    


    <!-- http://lawd.info/ontology/where -->

    <owl:ObjectProperty rdf:about="http://lawd.info/ontology/where">
        <rdfs:comment xml:lang="en">Generic location relation. Useful when the nature of the related place 
            (e.g. origin, findspot) is not clear.</rdfs:comment>
        <rdfs:range rdf:resource="http://lawd.info/ontology/Place"/>
    </owl:ObjectProperty>
    


    <!-- http://lawd.info/ontology/witness -->

    <owl:ObjectProperty rdf:about="http://lawd.info/ontology/witness">
        <rdfs:comment xml:lang="en">(Experimental) Connects an item in a collation to the witness it derives from.</rdfs:comment>
        <rdfs:domain rdf:resource="http://lawd.info/ontology/CollationItem"/>
        <rdfs:range rdf:resource="http://lawd.info/ontology/Siglum"/>
    </owl:ObjectProperty>
    


    <!-- 
    ///////////////////////////////////////////////////////////////////////////////////////
    //
    // Data properties
    //
    ///////////////////////////////////////////////////////////////////////////////////////
     -->

    


    <!-- http://lawd.info/ontology/abbreviation -->

    <owl:DatatypeProperty rdf:about="http://lawd.info/ontology/abbreviation">
        <rdfs:comment xml:lang="en">A label representing an abbreviated form of a name or title, e.g. of
      an author or work. E.g. Homer -&gt; Hom.; Odyssey -&gt; Od.;</rdfs:comment>
    </owl:DatatypeProperty>
    


    <!-- http://lawd.info/ontology/primaryForm -->

    <owl:DatatypeProperty rdf:about="http://lawd.info/ontology/primaryForm">
        <rdfs:comment xml:lang="en">Indicates the primary form of a lawd:Name</rdfs:comment>
        <rdfs:domain rdf:resource="http://lawd.info/ontology/Name"/>
    </owl:DatatypeProperty>
    


    <!-- http://lawd.info/ontology/variantForm -->

    <owl:DatatypeProperty rdf:about="http://lawd.info/ontology/variantForm">
        <rdfs:comment xml:lang="en">Indicates a variant form of a lawd:Name</rdfs:comment>
        <rdfs:domain rdf:resource="http://lawd.info/ontology/Name"/>
        <rdfs:subPropertyOf rdf:resource="&owl;topDataProperty"/>
    </owl:DatatypeProperty>
    


    <!-- 
    ///////////////////////////////////////////////////////////////////////////////////////
    //
    // Classes
    //
    ///////////////////////////////////////////////////////////////////////////////////////
     -->

    


    <!-- http://erlangen-crm.org/current/E21_Person -->

    <rdf:Description rdf:about="&cidoc-crm;E21_Person">
        <owl:equivalentClass rdf:resource="http://lawd.info/ontology/Person"/>
    </rdf:Description>
    


    <!-- http://erlangen-crm.org/current/E27_Site -->

    <rdf:Description rdf:about="&cidoc-crm;E27_Site">
        <owl:equivalentClass rdf:resource="http://lawd.info/ontology/Place"/>
    </rdf:Description>
    


    <!-- http://erlangen-crm.org/current/E33_Linguistic_Object -->

    <rdf:Description rdf:about="&cidoc-crm;E33_Linguistic_Object">
        <owl:equivalentClass rdf:resource="http://lawd.info/ontology/WrittenWork"/>
    </rdf:Description>
    


    <!-- http://geovocab.org/spatial#Feature -->

    <owl:Class rdf:about="&geo;Feature">
        <owl:equivalentClass rdf:resource="http://lawd.info/ontology/Place"/>
    </owl:Class>
    


    <!-- http://lawd.info/ontology/Agent -->

    <owl:Class rdf:about="http://lawd.info/ontology/Agent">
        <owl:equivalentClass rdf:resource="http://www.w3.org/ns/prov#Agent"/>
        <rdfs:comment xml:lang="en">An Agent is an abstract entity which has agency or is considered capable of acting in some way. Current subclasses include Deities and Persons.</rdfs:comment>
    </owl:Class>
    


    <!-- http://lawd.info/ontology/AssembledWork -->

    <owl:Class rdf:about="http://lawd.info/ontology/AssembledWork">
        <rdfs:subClassOf rdf:resource="http://lawd.info/ontology/WrittenWork"/>
        <rdfs:comment xml:lang="en">A Written Work that collects together more than one Written Work.
      Manuscripts are often AssembledWorks.</rdfs:comment>
    </owl:Class>
    


    <!-- http://lawd.info/ontology/Attestation -->

    <owl:Class rdf:about="http://lawd.info/ontology/Attestation">
        <rdfs:subClassOf rdf:resource="http://lawd.info/ontology/EvidentiaryItem"/>
        <rdfs:comment xml:lang="en">An Attestation models a piece of evidence for something in a text (e.g. the mention of a person in a document). Typically it is the conjunction of a Citation and an entity like a name or person.</rdfs:comment>
    </owl:Class>
    


    <!-- http://lawd.info/ontology/Citation -->

    <owl:Class rdf:about="http://lawd.info/ontology/Citation">
        <rdfs:comment xml:lang="en">A Citation models a bibliographic reference as a resource.</rdfs:comment>
    </owl:Class>
    


    <!-- http://lawd.info/ontology/CollationItem -->

    <owl:Class rdf:about="http://lawd.info/ontology/CollationItem">
        <rdfs:comment>(Experimental) Part of a collation of witnesses to a text.</rdfs:comment>
    </owl:Class>
    


    <!-- http://lawd.info/ontology/ConceptualWork -->

    <owl:Class rdf:about="http://lawd.info/ontology/ConceptualWork">
        <rdfs:comment xml:lang="en">A Conceptual Work groups together one or more Written Works which
      have the same intellectual source. E.g. The Iliad, as opposed to a particular manuscript witness or edition of the Iliad.</rdfs:comment>
    </owl:Class>
    


    <!-- http://lawd.info/ontology/Deity -->

    <owl:Class rdf:about="http://lawd.info/ontology/Deity">
        <rdfs:subClassOf rdf:resource="http://lawd.info/ontology/Agent"/>
        <rdfs:comment>Any divine Agent.</rdfs:comment>
    </owl:Class>
    


    <!-- http://lawd.info/ontology/Edition -->

    <owl:Class rdf:about="http://lawd.info/ontology/Edition">
        <rdfs:subClassOf rdf:resource="http://lawd.info/ontology/WrittenWork"/>
        <rdfs:comment xml:lang="en">A published (whether officially or not) Written Work that relies on
      one or more Written Works as sources</rdfs:comment>
    </owl:Class>
    


    <!-- http://lawd.info/ontology/EditorialComment -->

    <owl:Class rdf:about="http://lawd.info/ontology/EditorialComment">
        <rdfs:subClassOf rdf:resource="http://lawd.info/ontology/CollationItem"/>
    </owl:Class>
    


    <!-- http://lawd.info/ontology/EvidentiaryItem -->

    <owl:Class rdf:about="http://lawd.info/ontology/EvidentiaryItem">
        <rdfs:subClassOf rdf:resource="http://lawd.info/ontology/Observation"/>
        <rdfs:comment xml:lang="en">Superclass for types of evidence that support assertions.</rdfs:comment>
    </owl:Class>
    


    <!-- http://lawd.info/ontology/Group -->

    <owl:Class rdf:about="http://lawd.info/ontology/Group">
        <rdfs:subClassOf rdf:resource="http://lawd.info/ontology/Agent"/>
        <rdfs:comment>Any group of Agents referred to as a single entity.</rdfs:comment>
    </owl:Class>
    


    <!-- http://lawd.info/ontology/Hand -->

    <owl:Class rdf:about="http://lawd.info/ontology/Hand">
        <rdfs:subClassOf rdf:resource="http://lawd.info/ontology/WrittenWork"/>
        <rdfs:comment xml:lang="en">A portion of a Written Work in a distinct hand. Written Works may
      consist of one or more hands.</rdfs:comment>
    </owl:Class>
    


    <!-- http://lawd.info/ontology/MythologicalCreature -->

    <owl:Class rdf:about="http://lawd.info/ontology/MythologicalCreature">
        <rdfs:subClassOf rdf:resource="http://lawd.info/ontology/Agent"/>
        <rdfs:comment>Class for non-human, non-divine Agents, e.g. Polyphemus or Medusa.</rdfs:comment>
        <owl:deprecated xml:lang="en">Will be removed in a future release.</owl:deprecated>
    </owl:Class>
    


    <!-- http://lawd.info/ontology/Name -->

    <owl:Class rdf:about="http://lawd.info/ontology/Name">
        <rdfs:comment xml:lang="en">A name is a resource providing a name for some thing. It may be specialized with subclasses like PersonalName or PlaceName</rdfs:comment>
    </owl:Class>
    


    <!-- http://lawd.info/ontology/Observation -->

    <owl:Class rdf:about="http://lawd.info/ontology/Observation">
        <rdfs:label>Observation</rdfs:label>
        <owl:equivalentClass>
            <owl:Restriction>
                <owl:onProperty rdf:resource="http://www.w3.org/ns/prov#qualifiedAssociation"/>
                <owl:someValuesFrom rdf:resource="http://lawd.info/ontology/ObserverRoleAssociation"/>
            </owl:Restriction>
        </owl:equivalentClass>
        <rdfs:subClassOf rdf:resource="http://www.w3.org/ns/prov#Activity"/>
        <rdfs:comment xml:lang="en">An Observation is a scholarly assertion based on looking at evidence. An Observation might state, for example, that an entity provides evidence for the existence of a person or that a text quotes from another text.</rdfs:comment>
    </owl:Class>
    


    <!-- http://lawd.info/ontology/ObserverRoleAssociation -->

    <owl:Class rdf:about="http://lawd.info/ontology/ObserverRoleAssociation">
        <rdfs:label>Observer Role Association</rdfs:label>
        <owl:equivalentClass>
            <owl:Restriction>
                <owl:onProperty rdf:resource="http://www.w3.org/ns/prov#hadRole"/>
                <owl:hasValue rdf:resource="http://lawd.info/ontology/observerRole"/>
            </owl:Restriction>
        </owl:equivalentClass>
        <rdfs:subClassOf rdf:resource="http://www.w3.org/ns/prov#Association"/>
        <rdfs:comment>An instance of lawd:ObserverRoleAssociation characterizes a prov:Agent&apos;s association to a prov:Activity as serving in a lawd:observer role.</rdfs:comment>
    </owl:Class>
    


    <!-- http://lawd.info/ontology/Person -->

    <owl:Class rdf:about="http://lawd.info/ontology/Person">
        <rdfs:subClassOf rdf:resource="http://lawd.info/ontology/Agent"/>
        <rdfs:comment>Any person, whether historical, mythological, or fictional</rdfs:comment>
    </owl:Class>
    


    <!-- http://lawd.info/ontology/PersonalName -->

    <owl:Class rdf:about="http://lawd.info/ontology/PersonalName">
        <rdfs:subClassOf rdf:resource="http://lawd.info/ontology/Name"/>
        <rdfs:comment xml:lang="en">A name belonging to a lawd:Person</rdfs:comment>
    </owl:Class>
    


    <!-- http://lawd.info/ontology/Place -->

    <owl:Class rdf:about="http://lawd.info/ontology/Place">
        <rdfs:comment xml:lang="en">Any conceivable place, such as a town, a mountain, or the site of a building.</rdfs:comment>
    </owl:Class>
    


    <!-- http://lawd.info/ontology/PlaceName -->

    <owl:Class rdf:about="http://lawd.info/ontology/PlaceName">
        <rdfs:subClassOf rdf:resource="http://lawd.info/ontology/Name"/>
        <rdfs:comment xml:lang="en">The name of a lawd:Place</rdfs:comment>
    </owl:Class>
    


    <!-- http://lawd.info/ontology/Reading -->

    <owl:Class rdf:about="http://lawd.info/ontology/Reading">
        <rdfs:subClassOf rdf:resource="&skos;Concept"/>
        <rdfs:comment xml:lang="en">(Experimental) The superclass for members of the readingScheme concept scheme. A Reading is a word, phrase, or larger chunk of text from a witness (or any observation of variance concerning the text, such as an omission or interpolation).</rdfs:comment>
    </owl:Class>
    


    <!-- http://lawd.info/ontology/Reference -->

    <owl:Class rdf:about="http://lawd.info/ontology/Reference">
        <rdfs:subClassOf rdf:resource="http://lawd.info/ontology/CollationItem"/>
    </owl:Class>
    


    <!-- http://lawd.info/ontology/Sigla -->

    <owl:Class rdf:about="http://lawd.info/ontology/Sigla">
        <rdfs:subClassOf rdf:resource="http://purl.org/ontology/olo/core#OrderedList"/>
        <rdfs:comment xml:lang="en">An ordered collection that maps Written Works used as sources for an
      Edition to symbols used to represent them in the context of that Edition.</rdfs:comment>
    </owl:Class>
    


    <!-- http://lawd.info/ontology/Siglum -->

    <owl:Class rdf:about="http://lawd.info/ontology/Siglum">
        <rdfs:subClassOf rdf:resource="http://lawd.info/ontology/Citation"/>
        <rdfs:comment xml:lang="en">A Siglum represents a witness (a Written Work of some kind) and
      associates it with a symbol used to represent that work in the context of an
      Edition.</rdfs:comment>
    </owl:Class>
    


    <!-- http://lawd.info/ontology/TextPart -->

    <owl:Class rdf:about="http://lawd.info/ontology/TextPart">
        <rdfs:subClassOf rdf:resource="http://lawd.info/ontology/WrittenWork"/>
        <rdfs:comment xml:lang="en">Any portion of a larger WrittenWork.</rdfs:comment>
    </owl:Class>
    


    <!-- http://lawd.info/ontology/TextReuse -->

    <owl:Class rdf:about="http://lawd.info/ontology/TextReuse">
        <rdfs:subClassOf rdf:resource="http://lawd.info/ontology/Observation"/>
        <rdfs:comment xml:lang="en">A WrittenWork (or portion thereof) that quotes, translates, summarizes, or otherwise re-uses another WrittenWork.</rdfs:comment>
    </owl:Class>
    


    <!-- http://lawd.info/ontology/Translation -->

    <owl:Class rdf:about="http://lawd.info/ontology/Translation">
        <rdfs:subClassOf rdf:resource="http://lawd.info/ontology/WrittenWork"/>
        <rdfs:comment xml:lang="en">A Written Work that translates one or more other Written Works that embody the same Conceptual Work.</rdfs:comment>
    </owl:Class>
    


    <!-- http://lawd.info/ontology/WrittenWork -->

    <owl:Class rdf:about="http://lawd.info/ontology/WrittenWork">
        <rdfs:comment xml:lang="en">A written work, whether extant or not. May be considered to embody a Conceptual Work.</rdfs:comment>
    </owl:Class>
    


    <!-- http://purl.org/vocommons/voaf#Vocabulary -->

    <owl:Class rdf:about="&voaf;Vocabulary"/>
    


    <!-- http://www.w3.org/ns/prov#Agent -->

    <rdf:Description rdf:about="http://www.w3.org/ns/prov#Agent"/>
    


    <!-- 
    ///////////////////////////////////////////////////////////////////////////////////////
    //
    // Individuals
    //
    ///////////////////////////////////////////////////////////////////////////////////////
     -->

    


    <!-- http://lawd.info/ontology/ -->

    <owl:NamedIndividual rdf:about="http://lawd.info/ontology/">
        <rdf:type rdf:resource="&voaf;Vocabulary"/>
    </owl:NamedIndividual>
    


    <!-- http://lawd.info/ontology/addition -->

    <owl:NamedIndividual rdf:about="http://lawd.info/ontology/addition">
        <rdf:type rdf:resource="http://lawd.info/ontology/Reading"/>
        <skos:inScheme rdf:resource="http://lawd.info/ontology/readingScheme"/>
        <skos:broader rdf:resource="http://lawd.info/ontology/variant"/>
    </owl:NamedIndividual>
    


    <!-- http://lawd.info/ontology/agreement -->

    <owl:NamedIndividual rdf:about="http://lawd.info/ontology/agreement">
        <rdf:type rdf:resource="http://lawd.info/ontology/Reading"/>
        <skos:inScheme rdf:resource="http://lawd.info/ontology/readingScheme"/>
    </owl:NamedIndividual>
    


    <!-- http://lawd.info/ontology/collation -->

    <owl:NamedIndividual rdf:about="http://lawd.info/ontology/collation">
        <rdf:type rdf:resource="http://www.w3.org/ns/oa#Motivation"/>
        <rdfs:comment xml:lang="en">a Motivation that represents the addition of a critical apparatus
      comment upon a text</rdfs:comment>
        <skos:broader rdf:resource="http://www.w3.org/ns/oa#commenting"/>
    </owl:NamedIndividual>
    


    <!-- http://lawd.info/ontology/conjecture -->

    <owl:NamedIndividual rdf:about="http://lawd.info/ontology/conjecture">
        <rdf:type rdf:resource="http://lawd.info/ontology/Reading"/>
        <skos:inScheme rdf:resource="http://lawd.info/ontology/readingScheme"/>
    </owl:NamedIndividual>
    


    <!-- http://lawd.info/ontology/correction -->

    <owl:NamedIndividual rdf:about="http://lawd.info/ontology/correction">
        <rdf:type rdf:resource="http://lawd.info/ontology/Reading"/>
        <skos:broader rdf:resource="http://lawd.info/ontology/intervention"/>
        <skos:inScheme rdf:resource="http://lawd.info/ontology/readingScheme"/>
    </owl:NamedIndividual>
    


    <!-- http://lawd.info/ontology/deletion -->

    <owl:NamedIndividual rdf:about="http://lawd.info/ontology/deletion">
        <rdf:type rdf:resource="http://lawd.info/ontology/Reading"/>
        <skos:broader rdf:resource="http://lawd.info/ontology/intervention"/>
        <skos:inScheme rdf:resource="http://lawd.info/ontology/readingScheme"/>
    </owl:NamedIndividual>
    


    <!-- http://lawd.info/ontology/interpolation -->

    <owl:NamedIndividual rdf:about="http://lawd.info/ontology/interpolation">
        <rdf:type rdf:resource="http://lawd.info/ontology/Reading"/>
        <skos:inScheme rdf:resource="http://lawd.info/ontology/readingScheme"/>
        <skos:broader rdf:resource="http://lawd.info/ontology/variant"/>
    </owl:NamedIndividual>
    


    <!-- http://lawd.info/ontology/intervention -->

    <owl:NamedIndividual rdf:about="http://lawd.info/ontology/intervention">
        <rdf:type rdf:resource="http://lawd.info/ontology/Reading"/>
        <skos:inScheme rdf:resource="http://lawd.info/ontology/readingScheme"/>
        <skos:broader rdf:resource="http://lawd.info/ontology/variant"/>
    </owl:NamedIndividual>
    


    <!-- http://lawd.info/ontology/observerRole -->

    <owl:NamedIndividual rdf:about="http://lawd.info/ontology/observerRole">
        <rdf:type rdf:resource="http://www.w3.org/ns/prov#Role"/>
        <rdfs:label>observer role</rdfs:label>
        <rdfs:comment>The role of justifying a claim by appealing  to observed evidence.</rdfs:comment>
    </owl:NamedIndividual>
    


    <!-- http://lawd.info/ontology/omission -->

    <owl:NamedIndividual rdf:about="http://lawd.info/ontology/omission">
        <rdf:type rdf:resource="http://lawd.info/ontology/Reading"/>
        <skos:inScheme rdf:resource="http://lawd.info/ontology/readingScheme"/>
        <skos:broader rdf:resource="http://lawd.info/ontology/variant"/>
    </owl:NamedIndividual>
    


    <!-- http://lawd.info/ontology/readingScheme -->

    <owl:NamedIndividual rdf:about="http://lawd.info/ontology/readingScheme">
        <rdfs:comment xml:lang="en">(Experimental) The SKOS scheme for classifying types of lawd:Reading.</rdfs:comment>
    </owl:NamedIndividual>
    


    <!-- http://lawd.info/ontology/transposition -->

    <owl:NamedIndividual rdf:about="http://lawd.info/ontology/transposition">
        <rdf:type rdf:resource="http://lawd.info/ontology/Reading"/>
        <skos:inScheme rdf:resource="http://lawd.info/ontology/readingScheme"/>
        <skos:broader rdf:resource="http://lawd.info/ontology/variant"/>
    </owl:NamedIndividual>
    


    <!-- http://lawd.info/ontology/uncertainReading -->

    <owl:NamedIndividual rdf:about="http://lawd.info/ontology/uncertainReading">
        <rdf:type rdf:resource="http://lawd.info/ontology/Reading"/>
        <skos:inScheme rdf:resource="http://lawd.info/ontology/readingScheme"/>
    </owl:NamedIndividual>
    


    <!-- http://lawd.info/ontology/variant -->

    <owl:NamedIndividual rdf:about="http://lawd.info/ontology/variant">
        <rdf:type rdf:resource="http://lawd.info/ontology/Reading"/>
        <skos:inScheme rdf:resource="http://lawd.info/ontology/readingScheme"/>
    </owl:NamedIndividual>
</rdf:RDF>



<!-- Generated by the OWL API (version 3.4.2) http://owlapi.sourceforge.net -->

