<?xml version="1.0"?>
<rdf:RDF xmlns="http://w3id.org/medred/medred#"
     xml:base="http://w3id.org/medred/medred"
     xmlns:rdf="http://www.w3.org/1999/02/22-rdf-syntax-ns#"
     xmlns:terms="http://purl.org/dc/terms/"
     xmlns:owl="http://www.w3.org/2002/07/owl#"
     xmlns:discovery="http://rdf-vocabulary.ddialliance.org/discovery#"
     xmlns:xml="http://www.w3.org/XML/1998/namespace"
     xmlns:xsd="http://www.w3.org/2001/XMLSchema#"
     xmlns:rdfs="http://www.w3.org/2000/01/rdf-schema#"
     xmlns:vann="http://purl.org/vocab/vann/"
     xmlns:prov="http://www.w3.org/ns/prov#"
     xmlns:dc="http://purl.org/dc/elements/1.1/">
    <owl:Ontology rdf:about="http://w3id.org/medred/medred#">
        <owl:imports rdf:resource="http://purl.org/net/p-plan#"/>
        <owl:imports rdf:resource="http://rdf-vocabulary.ddialliance.org/discovery"/>
        <dc:publisher rdf:resource="http://aislab.hevs.ch/"/>
        <terms:creator rdf:resource="http://w3id.org/people/jpcik/me"/>
        <terms:description xml:lang="fr">Cette ontologie a été conçue pour representer des Instruments pour l&apos;aquisition de données cliniques, dans le contexte du projet MedRed project (https://www.hevs.ch/en/rad-institutes/institute-of-information-systems/projects/medical-research-data-acquisition-platform-14092)</terms:description>
        <terms:description xml:lang="es">Esta ontología has sido diseñada para representar Instrumentos de captura de datos clínicos, dentro del contexto del proyecto MedRed (https://www.hevs.ch/en/rad-institutes/institute-of-information-systems/projects/medical-research-data-acquisition-platform-14092)</terms:description>
        <terms:description xml:lang="en">This ontology aims to model generic Medical Data Acquisition Instruments, which can be interoperable across different clinical data management systems. The ontology is developed in the context of the MedRed project (https://www.hevs.ch/en/rad-institutes/institute-of-information-systems/projects/medical-research-data-acquisition-platform-14092)</terms:description>
        <terms:issued rdf:datatype="http://www.w3.org/2001/XMLSchema#date">2017-04-01</terms:issued>
        <terms:license rdf:resource="https://creativecommons.org/licenses/by/4.0/"/>
        <terms:modified rdf:datatype="http://www.w3.org/2001/XMLSchema#date">2017-04-25</terms:modified>
        <terms:publisher rdf:resource="http://w3id.org/hes-so/aislab"/>
        <terms:rights rdf:datatype="http://www.w3.org/2001/XMLSchema#string">Copyright © 2017 HES-SO Valais-Wallis</terms:rights>
        <terms:title xml:lang="fr">MedRed ontologie: modèle d&apos;aquisition de données cliniques</terms:title>
        <terms:title xml:lang="en">MedRed ontology: clinical data acquisition model</terms:title>
        <terms:title xml:lang="es">Ontología MedRed: modelo de adquisición de datos clínicos</terms:title>
        <vann:preferredNamespacePrefix rdf:datatype="http://www.w3.org/2001/XMLSchema#string">medred</vann:preferredNamespacePrefix>
        <vann:preferredNamespaceUri rdf:datatype="http://www.w3.org/2001/XMLSchema#string">http://w3id.org/medred/medred#</vann:preferredNamespaceUri>
        <rdfs:comment xml:lang="fr">Cette ontologie a été conçue pour representer des Instruments pour l&apos;aquisition de données cliniques, dans le contexte du projet MedRed project (https://www.hevs.ch/en/rad-institutes/institute-of-information-systems/projects/medical-research-data-acquisition-platform-14092)</rdfs:comment>
        <rdfs:comment xml:lang="es">Esta ontología has sido diseñada para representar Instrumentos de captura de datos clínicos, dentro del contexto del proyecto MedRed (https://www.hevs.ch/en/rad-institutes/institute-of-information-systems/projects/medical-research-data-acquisition-platform-14092)</rdfs:comment>
        <rdfs:comment xml:lang="en">This ontology aims to model generic Medical Data Acquisition Instruments, which can be interoperable across different clinical data management systems. The ontology is developed in the context of the MedRed project (https://www.hevs.ch/en/rad-institutes/institute-of-information-systems/projects/medical-research-data-acquisition-platform-14092)</rdfs:comment>
        <owl:versionInfo rdf:datatype="http://www.w3.org/2001/XMLSchema#string">0.0.1</owl:versionInfo>
    </owl:Ontology>
    


    <!-- 
    ///////////////////////////////////////////////////////////////////////////////////////
    //
    // Object Properties
    //
    ///////////////////////////////////////////////////////////////////////////////////////
     -->


    


    <!-- http://w3id.org/medred/medred#dataType -->


    <owl:ObjectProperty rdf:about="http://w3id.org/medred/medred#dataType">
        <rdfs:subPropertyOf rdf:resource="http://www.w3.org/2002/07/owl#topObjectProperty"/>
        <rdfs:domain rdf:resource="http://purl.org/net/p-plan#Variable"/>
        <rdfs:range rdf:resource="http://www.w3.org/2000/01/rdf-schema#Datatype"/>
        <rdfs:comment xml:lang="en">The dataType estalbishes a relationship between a Variable and the datatype of its data item</rdfs:comment>
        <rdfs:isDefinedBy rdf:resource="http://w3id.org/medred/medred#"/>
        <rdfs:label xml:lang="en">dataType</rdfs:label>
    </owl:ObjectProperty>
    


    <!-- http://w3id.org/medred/medred#hasArms -->


    <owl:ObjectProperty rdf:about="http://w3id.org/medred/medred#hasArms">
        <rdfs:domain rdf:resource="http://w3id.org/medred/medred#Study"/>
        <rdfs:range rdf:resource="http://w3id.org/medred/medred#ArmList"/>
        <rdfs:comment xml:lang="en">A relation between a Study and a list of its different Arms</rdfs:comment>
        <rdfs:isDefinedBy rdf:resource="http://w3id.org/medred/medred#"/>
        <rdfs:label xml:lang="en">hasArms</rdfs:label>
        <rdfs:seeAlso rdf:resource="http://w3id.org/medred/medred#Arm"/>
        <rdfs:seeAlso rdf:resource="http://w3id.org/medred/medred#Study"/>
    </owl:ObjectProperty>
    


    <!-- http://w3id.org/medred/medred#hasChoices -->


    <owl:ObjectProperty rdf:about="http://w3id.org/medred/medred#hasChoices">
        <rdfs:domain rdf:resource="http://w3id.org/medred/medred#Question"/>
        <rdfs:range rdf:resource="http://w3id.org/medred/medred#ChoiceList"/>
        <rdfs:comment xml:lang="en">A relation between an Instrument question, and the list of possible Choice elements</rdfs:comment>
        <rdfs:isDefinedBy rdf:resource="http://w3id.org/medred/medred#"/>
        <rdfs:label xml:lang="en">hasChoices</rdfs:label>
        <rdfs:seeAlso rdf:resource="http://w3id.org/medred/medred#Choice"/>
    </owl:ObjectProperty>
    


    <!-- http://w3id.org/medred/medred#hasInstruments -->


    <owl:ObjectProperty rdf:about="http://w3id.org/medred/medred#hasInstruments">
        <rdfs:domain rdf:resource="http://w3id.org/medred/medred#Study"/>
        <rdfs:range rdf:resource="http://w3id.org/medred/medred#InstrumentList"/>
        <rdfs:comment xml:lang="en">The instrument establishes a relationship between a Study and a list of Instruments</rdfs:comment>
        <rdfs:isDefinedBy rdf:resource="http://w3id.org/medred/medred#"/>
        <rdfs:label xml:lang="en">hasInstruments</rdfs:label>
        <rdfs:seeAlso rdf:resource="http://w3id.org/medred/medred#Instrument"/>
    </owl:ObjectProperty>
    


    <!-- http://w3id.org/medred/medred#includedInStudy -->


    <owl:ObjectProperty rdf:about="http://w3id.org/medred/medred#includedInStudy">
        <rdfs:domain>
            <owl:Class>
                <owl:unionOf rdf:parseType="Collection">
                    <rdf:Description rdf:about="http://w3id.org/medred/medred#Arm"/>
                    <rdf:Description rdf:about="http://w3id.org/medred/medred#Instrument"/>
                </owl:unionOf>
            </owl:Class>
        </rdfs:domain>
        <rdfs:range rdf:resource="http://w3id.org/medred/medred#Study"/>
        <rdfs:comment xml:lang="en">It establishes a relationship between an Arm or Instrument, and a Study</rdfs:comment>
        <rdfs:isDefinedBy rdf:resource="http://w3id.org/medred/medred#"/>
        <rdfs:label xml:lang="en">includedInStudy</rdfs:label>
        <rdfs:seeAlso rdf:resource="http://w3id.org/medred/medred#Arm"/>
        <rdfs:seeAlso rdf:resource="http://w3id.org/medred/medred#Instrument"/>
        <rdfs:seeAlso rdf:resource="http://w3id.org/medred/medred#Study"/>
    </owl:ObjectProperty>
    


    <!-- http://w3id.org/medred/medred#includesEvents -->


    <owl:ObjectProperty rdf:about="http://w3id.org/medred/medred#includesEvents">
        <rdfs:domain>
            <owl:Class>
                <owl:unionOf rdf:parseType="Collection">
                    <rdf:Description rdf:about="http://w3id.org/medred/medred#Arm"/>
                    <rdf:Description rdf:about="http://w3id.org/medred/medred#Study"/>
                </owl:unionOf>
            </owl:Class>
        </rdfs:domain>
        <rdfs:range rdf:resource="http://w3id.org/medred/medred#EventList"/>
        <rdfs:comment xml:lang="en">A relation between an Arm or Study, and the list of its events</rdfs:comment>
        <rdfs:isDefinedBy rdf:resource="http://w3id.org/medred/medred#"/>
        <rdfs:label xml:lang="en">includesEvents</rdfs:label>
        <rdfs:seeAlso rdf:resource="http://w3id.org/medred/medred#Arm"/>
        <rdfs:seeAlso rdf:resource="http://w3id.org/medred/medred#StudyEvent"/>
    </owl:ObjectProperty>
    


    <!-- http://w3id.org/medred/medred#includesInstrument -->


    <owl:ObjectProperty rdf:about="http://w3id.org/medred/medred#includesInstrument">
        <rdfs:domain rdf:resource="http://w3id.org/medred/medred#StudyEvent"/>
        <rdfs:range rdf:resource="http://w3id.org/medred/medred#Instrument"/>
        <rdfs:comment xml:lang="en">A relation between an StudyEvent, and an Instrument it includes</rdfs:comment>
        <rdfs:isDefinedBy rdf:resource="http://w3id.org/medred/medred#"/>
        <rdfs:label xml:lang="en">includesInstrument</rdfs:label>
        <rdfs:seeAlso rdf:resource="http://w3id.org/medred/medred#Instrument"/>
        <rdfs:seeAlso rdf:resource="http://w3id.org/medred/medred#StudyEvent"/>
    </owl:ObjectProperty>
    


    <!-- http://w3id.org/medred/medred#isEventOfArm -->


    <owl:ObjectProperty rdf:about="http://w3id.org/medred/medred#isEventOfArm">
        <rdfs:domain rdf:resource="http://w3id.org/medred/medred#StudyEvent"/>
        <rdfs:range rdf:resource="http://w3id.org/medred/medred#Arm"/>
        <rdfs:comment xml:lang="en">It establishes a relationship between a StudyEvent, and an Arm</rdfs:comment>
        <rdfs:isDefinedBy rdf:resource="http://w3id.org/medred/medred#"/>
        <rdfs:label xml:lang="en">isEventOfArm</rdfs:label>
        <rdfs:seeAlso rdf:resource="http://w3id.org/medred/medred#Arm"/>
        <rdfs:seeAlso rdf:resource="http://w3id.org/medred/medred#StudyEvent"/>
    </owl:ObjectProperty>
    


    <!-- http://w3id.org/medred/medred#isItemOfInstrument -->


    <owl:ObjectProperty rdf:about="http://w3id.org/medred/medred#isItemOfInstrument">
        <rdfs:subPropertyOf rdf:resource="http://purl.org/net/p-plan#isStepOfPlan"/>
        <rdfs:domain rdf:resource="http://w3id.org/medred/medred#Item"/>
        <rdfs:range rdf:resource="http://w3id.org/medred/medred#Instrument"/>
        <rdfs:comment xml:lang="en">It establishes a relationship between an Item and an Instrument</rdfs:comment>
        <rdfs:isDefinedBy rdf:resource="http://w3id.org/medred/medred#"/>
        <rdfs:label xml:lang="en">isItemofInstrument</rdfs:label>
        <rdfs:seeAlso rdf:resource="http://w3id.org/medred/medred#Instrument"/>
        <rdfs:seeAlso rdf:resource="http://w3id.org/medred/medred#Item"/>
    </owl:ObjectProperty>
    


    <!-- http://w3id.org/medred/medred#isItemOfSection -->


    <owl:ObjectProperty rdf:about="http://w3id.org/medred/medred#isItemOfSection">
        <rdfs:subPropertyOf rdf:resource="http://purl.org/net/p-plan#isStepOfPlan"/>
        <rdfs:domain rdf:resource="http://w3id.org/medred/medred#Item"/>
        <rdfs:range rdf:resource="http://w3id.org/medred/medred#Section"/>
        <rdfs:comment xml:lang="en">It establishes a relationship between an Item and a Section</rdfs:comment>
        <rdfs:isDefinedBy rdf:resource="http://w3id.org/medred/medred#"/>
        <rdfs:label xml:lang="en">isItemofSection</rdfs:label>
        <rdfs:seeAlso rdf:resource="http://w3id.org/medred/medred#Item"/>
        <rdfs:seeAlso rdf:resource="http://w3id.org/medred/medred#Section"/>
    </owl:ObjectProperty>
    


    <!-- http://w3id.org/medred/medred#items -->


    <owl:ObjectProperty rdf:about="http://w3id.org/medred/medred#items">
        <rdfs:domain>
            <owl:Class>
                <owl:unionOf rdf:parseType="Collection">
                    <rdf:Description rdf:about="http://w3id.org/medred/medred#Instrument"/>
                    <rdf:Description rdf:about="http://w3id.org/medred/medred#Item"/>
                </owl:unionOf>
            </owl:Class>
        </rdfs:domain>
        <rdfs:range rdf:resource="http://w3id.org/medred/medred#ItemList"/>
        <rdfs:comment xml:lang="en">The items property represents a relationship between an Instrument and its constitutent ItemList</rdfs:comment>
        <rdfs:isDefinedBy rdf:resource="http://w3id.org/medred/medred#"/>
        <rdfs:label xml:lang="en">items</rdfs:label>
        <rdfs:seeAlso rdf:resource="http://w3id.org/medred/medred#ItemList"/>
    </owl:ObjectProperty>
    


    <!-- http://w3id.org/medred/medred#validationShape -->


    <owl:ObjectProperty rdf:about="http://w3id.org/medred/medred#validationShape">
        <rdfs:domain rdf:resource="http://w3id.org/medred/medred#Item"/>
        <rdfs:range rdf:resource="http://www.w3.org/ns/shacl#PropertyShape"/>
        <rdfs:comment xml:lang="en">It establishes a relationship between an Item, and a PropertyShape, which defines the type of validation expected for the Observations made for the Item.</rdfs:comment>
        <rdfs:isDefinedBy rdf:resource="http://w3id.org/medred/medred#"/>
        <rdfs:label xml:lang="en">validationShape</rdfs:label>
        <rdfs:seeAlso rdf:resource="http://w3id.org/medred/medred#Item"/>
        <rdfs:seeAlso rdf:resource="http://www.w3.org/ns/shacl#PropertyShape"/>
    </owl:ObjectProperty>
    


    <!-- http://www.w3.org/1999/02/22-rdf-syntax-ns#first -->


    <owl:ObjectProperty rdf:about="http://www.w3.org/1999/02/22-rdf-syntax-ns#first"/>
    


    <!-- http://www.w3.org/1999/02/22-rdf-syntax-ns#rest -->


    <owl:ObjectProperty rdf:about="http://www.w3.org/1999/02/22-rdf-syntax-ns#rest"/>
    


    <!-- 
    ///////////////////////////////////////////////////////////////////////////////////////
    //
    // Data properties
    //
    ///////////////////////////////////////////////////////////////////////////////////////
     -->


    


    <!-- http://purl.org/dc/terms/title -->


    <owl:DatatypeProperty rdf:about="http://purl.org/dc/terms/title"/>
    


    <!-- http://w3id.org/medred/medred#calculation -->


    <owl:DatatypeProperty rdf:about="http://w3id.org/medred/medred#calculation">
        <rdfs:domain rdf:resource="http://w3id.org/medred/medred#Operation"/>
        <rdfs:range rdf:resource="http://www.w3.org/2000/01/rdf-schema#Literal"/>
        <rdfs:comment xml:lang="en">It indicates the definition of a calculation or a computation on an Operation item, over input variables.</rdfs:comment>
        <rdfs:isDefinedBy rdf:resource="http://w3id.org/medred/medred#"/>
        <rdfs:label xml:lang="en">calculation</rdfs:label>
        <rdfs:seeAlso rdf:resource="http://w3id.org/medred/medred#Operation"/>
    </owl:DatatypeProperty>
    


    <!-- http://w3id.org/medred/medred#dataValue -->


    <owl:DatatypeProperty rdf:about="http://w3id.org/medred/medred#dataValue">
        <rdfs:domain rdf:resource="http://w3id.org/medred/medred#Observation"/>
        <rdfs:range rdf:resource="http://www.w3.org/2000/01/rdf-schema#Literal"/>
        <rdfs:comment xml:lang="en">It establishes a value of a data element related to a given Observation</rdfs:comment>
        <rdfs:isDefinedBy rdf:resource="http://w3id.org/medred/medred#"/>
        <rdfs:label xml:lang="en">dataValue</rdfs:label>
    </owl:DatatypeProperty>
    


    <!-- http://w3id.org/medred/medred#hasValue -->


    <owl:DatatypeProperty rdf:about="http://w3id.org/medred/medred#hasValue">
        <rdfs:domain rdf:resource="http://w3id.org/medred/medred#Choice"/>
        <rdfs:range rdf:resource="http://www.w3.org/2000/01/rdf-schema#Literal"/>
        <rdfs:comment xml:lang="en">It establishes a value for a given Choice element.</rdfs:comment>
        <rdfs:isDefinedBy rdf:resource="http://w3id.org/medred/medred#"/>
        <rdfs:label xml:lang="en">hasValue</rdfs:label>
    </owl:DatatypeProperty>
    


    <!-- http://w3id.org/medred/medred#studyName -->


    <owl:DatatypeProperty rdf:about="http://w3id.org/medred/medred#studyName">
        <rdfs:subPropertyOf rdf:resource="http://purl.org/dc/terms/title"/>
        <rdfs:domain rdf:resource="http://w3id.org/medred/medred#Study"/>
        <rdfs:range rdf:resource="http://www.w3.org/2001/XMLSchema#string"/>
        <rdfs:comment xml:lang="en">It establishes a value for the name of the study</rdfs:comment>
        <rdfs:isDefinedBy rdf:resource="http://w3id.org/medred/medred#"/>
        <rdfs:label xml:lang="en">studyName</rdfs:label>
    </owl:DatatypeProperty>
    


    <!-- http://w3id.org/medred/medred#varName -->


    <owl:DatatypeProperty rdf:about="http://w3id.org/medred/medred#varName">
        <rdfs:domain rdf:resource="http://purl.org/net/p-plan#Variable"/>
        <rdfs:range rdf:resource="http://www.w3.org/2001/XMLSchema#string"/>
        <rdfs:comment xml:lang="en">It establishes a value for the name of a Variable</rdfs:comment>
        <rdfs:isDefinedBy rdf:resource="http://w3id.org/medred/medred#"/>
        <rdfs:label xml:lang="en">varName</rdfs:label>
    </owl:DatatypeProperty>
    


    <!-- 
    ///////////////////////////////////////////////////////////////////////////////////////
    //
    // Classes
    //
    ///////////////////////////////////////////////////////////////////////////////////////
     -->


    


    <!-- http://purl.org/vocommons/voaf#Vocabulary -->


    <owl:Class rdf:about="http://purl.org/vocommons/voaf#Vocabulary"/>
    


    <!-- http://w3id.org/medred/medred#Arm -->


    <owl:Class rdf:about="http://w3id.org/medred/medred#Arm">
        <rdfs:subClassOf rdf:resource="http://purl.org/net/p-plan#Plan"/>
        <owl:disjointWith rdf:resource="http://w3id.org/medred/medred#Instrument"/>
        <rdfs:comment xml:lang="en">An Arm is branching of a study that corresponds to a particular set of conditions, typically used to compare different behaviours, patterns or steps within the same study. Different Arms typically will have different sets of Instruments applied over time.</rdfs:comment>
        <rdfs:isDefinedBy rdf:resource="http://w3id.org/medred/medred#"/>
        <rdfs:label xml:lang="en">Arm</rdfs:label>
        <rdfs:seeAlso rdf:resource="http://w3id.org/medred/medred#Instrument"/>
        <rdfs:seeAlso rdf:resource="http://w3id.org/medred/medred#Study"/>
    </owl:Class>
    


    <!-- http://w3id.org/medred/medred#ArmList -->


    <owl:Class rdf:about="http://w3id.org/medred/medred#ArmList">
        <rdfs:subClassOf rdf:resource="http://www.w3.org/1999/02/22-rdf-syntax-ns#List"/>
        <rdfs:comment xml:lang="en">A ArmList is an ordered sequence of Arms, for a given study.</rdfs:comment>
        <rdfs:isDefinedBy rdf:resource="http://w3id.org/medred/medred#"/>
        <rdfs:label xml:lang="en">ArmList</rdfs:label>
        <rdfs:seeAlso rdf:resource="http://w3id.org/medred/medred#Arm"/>
        <rdfs:seeAlso rdf:resource="http://w3id.org/medred/medred#Study"/>
    </owl:Class>
    


    <!-- http://w3id.org/medred/medred#CaseReportForm -->


    <owl:Class rdf:about="http://w3id.org/medred/medred#CaseReportForm">
        <rdfs:subClassOf rdf:resource="http://w3id.org/medred/medred#Instrument"/>
        <rdfs:comment xml:lang="en">A CaseReportForm is a tool used for a clinical study to collect data from each participating subject</rdfs:comment>
        <rdfs:isDefinedBy rdf:resource="http://w3id.org/medred/medred#"/>
        <rdfs:label xml:lang="en">CaseReportForm</rdfs:label>
    </owl:Class>
    


    <!-- http://w3id.org/medred/medred#Choice -->


    <owl:Class rdf:about="http://w3id.org/medred/medred#Choice">
        <rdfs:comment xml:lang="en">Each Choice corresponds to a possible answer to a given Question</rdfs:comment>
        <rdfs:isDefinedBy rdf:resource="http://w3id.org/medred/medred#"/>
        <rdfs:label xml:lang="en">Choice</rdfs:label>
        <rdfs:seeAlso rdf:resource="http://w3id.org/medred/medred#ChoiceList"/>
    </owl:Class>
    


    <!-- http://w3id.org/medred/medred#ChoiceList -->


    <owl:Class rdf:about="http://w3id.org/medred/medred#ChoiceList">
        <owl:equivalentClass>
            <owl:Restriction>
                <owl:onProperty>
                    <rdf:Description>
                        <owl:inverseOf rdf:resource="http://w3id.org/medred/medred#hasChoices"/>
                    </rdf:Description>
                </owl:onProperty>
                <owl:someValuesFrom rdf:resource="http://w3id.org/medred/medred#Question"/>
            </owl:Restriction>
        </owl:equivalentClass>
        <rdfs:subClassOf rdf:resource="http://www.w3.org/1999/02/22-rdf-syntax-ns#List"/>
        <rdfs:comment xml:lang="en">The ChoiceList corresponds to a list of Choice items for a given Question</rdfs:comment>
        <rdfs:isDefinedBy rdf:resource="http://w3id.org/medred/medred#"/>
        <rdfs:label xml:lang="en">ChoiceList</rdfs:label>
    </owl:Class>
    


    <!-- http://w3id.org/medred/medred#EventList -->


    <owl:Class rdf:about="http://w3id.org/medred/medred#EventList">
        <rdfs:subClassOf rdf:resource="http://www.w3.org/1999/02/22-rdf-syntax-ns#List"/>
        <rdfs:comment xml:lang="en">An EventList is an ordered list of Event elements for a study that is carried out over a long period of time.</rdfs:comment>
        <rdfs:isDefinedBy rdf:resource="http://w3id.org/medred/medred#"/>
        <rdfs:label xml:lang="en">EventList</rdfs:label>
        <rdfs:seeAlso rdf:resource="http://w3id.org/medred/medred#Event"/>
        <rdfs:seeAlso rdf:resource="http://w3id.org/medred/medred#Study"/>
    </owl:Class>
    


    <!-- http://w3id.org/medred/medred#Information -->


    <owl:Class rdf:about="http://w3id.org/medred/medred#Information">
        <rdfs:subClassOf rdf:resource="http://w3id.org/medred/medred#Item"/>
        <rdfs:comment xml:lang="en">Information corresponds to an instrument item that holds an information for the subject</rdfs:comment>
        <rdfs:isDefinedBy rdf:resource="http://w3id.org/medred/medred#"/>
        <rdfs:label xml:lang="en">Information</rdfs:label>
    </owl:Class>
    


    <!-- http://w3id.org/medred/medred#Instrument -->


    <owl:Class rdf:about="http://w3id.org/medred/medred#Instrument">
        <rdfs:subClassOf rdf:resource="http://rdf-vocabulary.ddialliance.org/discovery#Instrument"/>
        <rdfs:subClassOf rdf:resource="http://www.w3.org/ns/prov#Plan"/>
        <owl:disjointWith rdf:resource="http://w3id.org/medred/medred#Observation"/>
        <rdfs:comment xml:lang="en">An Instrument represents a data acquisition tool for a medical study, e.g. a questionnaire, survey, assessment, etc.</rdfs:comment>
        <rdfs:isDefinedBy rdf:resource="http://w3id.org/medred/medred#"/>
        <rdfs:label xml:lang="en">Instrument</rdfs:label>
    </owl:Class>
    


    <!-- http://w3id.org/medred/medred#InstrumentList -->


    <owl:Class rdf:about="http://w3id.org/medred/medred#InstrumentList">
        <rdfs:subClassOf rdf:resource="http://www.w3.org/1999/02/22-rdf-syntax-ns#List"/>
        <rdfs:comment xml:lang="en">An InstrumentList is an ordered sequence of Instruments, for a given study.</rdfs:comment>
        <rdfs:isDefinedBy rdf:resource="http://w3id.org/medred/medred#"/>
        <rdfs:label xml:lang="en">InstrumentList</rdfs:label>
        <rdfs:seeAlso rdf:resource="http://w3id.org/medred/medred#Instrument"/>
        <rdfs:seeAlso rdf:resource="http://w3id.org/medred/medred#Study"/>
    </owl:Class>
    


    <!-- http://w3id.org/medred/medred#Item -->


    <owl:Class rdf:about="http://w3id.org/medred/medred#Item">
        <rdfs:subClassOf rdf:resource="http://purl.org/net/p-plan#Step"/>
        <rdfs:subClassOf>
            <owl:Restriction>
                <owl:onProperty rdf:resource="http://purl.org/dc/terms/title"/>
                <owl:someValuesFrom rdf:resource="http://www.w3.org/2001/XMLSchema#string"/>
            </owl:Restriction>
        </rdfs:subClassOf>
        <rdfs:comment xml:lang="en">An Item is a step of an Instrument</rdfs:comment>
        <rdfs:isDefinedBy rdf:resource="http://w3id.org/medred/medred#"/>
        <rdfs:label xml:lang="en">Item</rdfs:label>
    </owl:Class>
    


    <!-- http://w3id.org/medred/medred#ItemList -->


    <owl:Class rdf:about="http://w3id.org/medred/medred#ItemList">
        <rdfs:subClassOf rdf:resource="http://www.w3.org/1999/02/22-rdf-syntax-ns#List"/>
        <rdfs:comment xml:lang="en">The ItemList is a list of Item elements</rdfs:comment>
        <rdfs:isDefinedBy rdf:resource="http://w3id.org/medred/medred#"/>
        <rdfs:label xml:lang="en">ItemList</rdfs:label>
    </owl:Class>
    


    <!-- http://w3id.org/medred/medred#LongitudinalStudy -->


    <owl:Class rdf:about="http://w3id.org/medred/medred#LongitudinalStudy">
        <rdfs:subClassOf rdf:resource="http://w3id.org/medred/medred#Study"/>
        <rdfs:comment xml:lang="en">A LongitudinalStudy is a study that invloves the repeated observation of data and variables over a period of time</rdfs:comment>
        <rdfs:isDefinedBy rdf:resource="http://w3id.org/medred/medred#"/>
        <rdfs:label xml:lang="en">LongitudinalStudy</rdfs:label>
        <rdfs:seeAlso rdf:resource="http://rdf-vocabulary.ddialliance.org/discovery#Study"/>
        <rdfs:seeAlso rdf:resource="http://w3id.org/medred/medred#Study"/>
    </owl:Class>
    


    <!-- http://w3id.org/medred/medred#Observation -->


    <owl:Class rdf:about="http://w3id.org/medred/medred#Observation">
        <rdfs:subClassOf rdf:resource="http://purl.org/net/p-plan#Entity"/>
        <rdfs:comment xml:lang="en">An Observation is a clinical data element corresponding to an Item in the scope of an Instrument. Observations may include answers to questions, recordings related to a variable, computations effectuated, etc.</rdfs:comment>
        <rdfs:isDefinedBy rdf:resource="http://w3id.org/medred/medred#"/>
        <rdfs:label xml:lang="en">Observation</rdfs:label>
        <rdfs:seeAlso rdf:resource="http://w3id.org/medred/medred#Instrument"/>
        <rdfs:seeAlso rdf:resource="http://w3id.org/medred/medred#Item"/>
    </owl:Class>
    


    <!-- http://w3id.org/medred/medred#Operation -->


    <owl:Class rdf:about="http://w3id.org/medred/medred#Operation">
        <rdfs:subClassOf rdf:resource="http://w3id.org/medred/medred#Item"/>
        <rdfs:comment xml:lang="en">An Operation is an Instrument item that results of a computation, or generated form other items</rdfs:comment>
        <rdfs:isDefinedBy rdf:resource="http://w3id.org/medred/medred#"/>
        <rdfs:label xml:lang="en">Operation</rdfs:label>
    </owl:Class>
    


    <!-- http://w3id.org/medred/medred#Question -->


    <owl:Class rdf:about="http://w3id.org/medred/medred#Question">
        <rdfs:subClassOf rdf:resource="http://rdf-vocabulary.ddialliance.org/discovery#Question"/>
        <rdfs:subClassOf rdf:resource="http://w3id.org/medred/medred#Item"/>
        <rdfs:comment xml:lang="en">A Question is an Instrument item consisting of an inquiry or query to a subject</rdfs:comment>
        <rdfs:isDefinedBy rdf:resource="http://w3id.org/medred/medred#"/>
        <rdfs:label xml:lang="en">Question</rdfs:label>
    </owl:Class>
    


    <!-- http://w3id.org/medred/medred#Questionnaire -->


    <owl:Class rdf:about="http://w3id.org/medred/medred#Questionnaire">
        <rdfs:subClassOf rdf:resource="http://w3id.org/medred/medred#Instrument"/>
        <rdfs:comment xml:lang="en">A Questionnaire is an Instrument that consists fo different questions made to the subject</rdfs:comment>
        <rdfs:isDefinedBy rdf:resource="http://w3id.org/medred/medred#"/>
        <rdfs:label xml:lang="en">Questionnaire</rdfs:label>
    </owl:Class>
    


    <!-- http://w3id.org/medred/medred#Section -->


    <owl:Class rdf:about="http://w3id.org/medred/medred#Section">
        <rdfs:subClassOf rdf:resource="http://purl.org/net/p-plan#MultiStep"/>
        <rdfs:subClassOf rdf:resource="http://w3id.org/medred/medred#Item"/>
        <rdfs:comment xml:lang="en">A Section is an Instrument item that regroups a subset of Items</rdfs:comment>
        <rdfs:isDefinedBy rdf:resource="http://w3id.org/medred/medred#"/>
        <rdfs:label xml:lang="en">Section</rdfs:label>
    </owl:Class>
    


    <!-- http://w3id.org/medred/medred#Study -->


    <owl:Class rdf:about="http://w3id.org/medred/medred#Study">
        <rdfs:subClassOf rdf:resource="http://rdf-vocabulary.ddialliance.org/discovery#Study"/>
        <rdfs:subClassOf rdf:resource="http://www.w3.org/ns/prov#Entity"/>
        <rdfs:comment xml:lang="en">A Study is a medical research investigation composed of several instruments</rdfs:comment>
        <rdfs:isDefinedBy rdf:resource="http://w3id.org/medred/medred#"/>
        <rdfs:label xml:lang="en">Study</rdfs:label>
        <rdfs:seeAlso rdf:resource="http://rdf-vocabulary.ddialliance.org/discovery#Study"/>
    </owl:Class>
    


    <!-- http://w3id.org/medred/medred#StudyEvent -->


    <owl:Class rdf:about="http://w3id.org/medred/medred#StudyEvent">
        <rdfs:subClassOf rdf:resource="http://purl.org/net/p-plan#Entity"/>
        <rdfs:comment xml:lang="en">A StudyEvent is a planned event within a study (e.g. longitudinal), which will occur at a given time point, and will include a subset of the planned instruments.</rdfs:comment>
        <rdfs:isDefinedBy rdf:resource="http://w3id.org/medred/medred#"/>
        <rdfs:label xml:lang="en">StudyEvent</rdfs:label>
        <rdfs:seeAlso rdf:resource="http://rdf-vocabulary.ddialliance.org/discovery#Study"/>
        <rdfs:seeAlso rdf:resource="http://w3id.org/medred/medred#Study"/>
    </owl:Class>
    


    <!-- http://www.w3.org/1999/02/22-rdf-syntax-ns#List -->


    <owl:Class rdf:about="http://www.w3.org/1999/02/22-rdf-syntax-ns#List"/>
    


    <!-- http://www.w3.org/2000/01/rdf-schema#Datatype -->


    <owl:Class rdf:about="http://www.w3.org/2000/01/rdf-schema#Datatype"/>
    


    <!-- http://www.w3.org/ns/shacl#PropertyShape -->


    <owl:Class rdf:about="http://www.w3.org/ns/shacl#PropertyShape"/>
    


    <!-- 
    ///////////////////////////////////////////////////////////////////////////////////////
    //
    // Individuals
    //
    ///////////////////////////////////////////////////////////////////////////////////////
     -->


    


    <!-- http://w3id.org/medred/medred# -->


    <owl:NamedIndividual rdf:about="http://w3id.org/medred/medred#">
        <rdf:type rdf:resource="http://purl.org/vocommons/voaf#Vocabulary"/>
    </owl:NamedIndividual>
    


    <!-- http://www.w3.org/1999/02/22-rdf-syntax-ns#nil -->


    <owl:NamedIndividual rdf:about="http://www.w3.org/1999/02/22-rdf-syntax-ns#nil"/>
</rdf:RDF>



<!-- Generated by the OWL API (version 5.1.0) https://github.com/owlcs/owlapi/ -->


