<?xml version="1.0"?>
<rdf:RDF xmlns:dcterms="http://purl.org/dc/terms/" xmlns:pnc="http://data.press.net/ontology/classification/" xmlns:foaf="http://xmlns.com/foaf/0.1/" xmlns:vs="http://www.w3.org/2003/06/sw-vocab-status/ns#" xmlns:owl="http://www.w3.org/2002/07/owl#" xmlns:xsd="http://www.w3.org/2001/XMLSchema#" xmlns:rdfs="http://www.w3.org/2000/01/rdf-schema#" xmlns:rdf="http://www.w3.org/1999/02/22-rdf-syntax-ns#" xmlns:psys="http://proton.semanticweb.org/protonsys#">
    <owl:Ontology rdf:about="http://data.press.net/ontology/classification/">
        <dcterms:title xml:lang="en">SNaP Classification Ontology</dcterms:title>
        <dcterms:created rdf:datatype="http://www.w3.org/2001/XMLSchema#date">2011-07-28</dcterms:created>
        <dcterms:modified rdf:datatype="http://www.w3.org/2001/XMLSchema#date">2012-09-25</dcterms:modified>
        <dcterms:license rdf:resource="http://creativecommons.org/licenses/by-nd/3.0/" />
        <rdfs:comment xml:lang="en">The Classification Ontology allows assets to be holistically classified using a controlled vocabulary or taxonomy.</rdfs:comment>
        <foaf:maker>
            <foaf:Person rdf:about="http://uk.linkedin.com/in/paulwilton">
                <foaf:name>Paul Wilton</foaf:name>
            </foaf:Person>
        </foaf:maker>
        <foaf:maker>
            <foaf:Person rdf:about="http://uk.linkedin.com/in/jarredmcginnis">
                <foaf:name>Jarred McGinnis</foaf:name>
            </foaf:Person>
        </foaf:maker>
        <foaf:maker>
            <foaf:Person rdf:about="http://uk.linkedin.com/in/pauliharman">
                <foaf:name>Paul Harman</foaf:name>
            </foaf:Person>
        </foaf:maker>
        <owl:versionInfo rdf:datatype="http://www.w3.org/2001/XMLSchema#string">0.2.2</owl:versionInfo>
    </owl:Ontology>
    <owl:Class rdf:about="http://data.press.net/ontology/classification/Classification">
        <rdfs:label xml:lang="en">Generic Classification Class.</rdfs:label>
        <rdfs:comment xml:lang="en">Generic Classification Class. Vocabulary instances would be of this type.</rdfs:comment>
        <rdfs:isDefinedBy rdf:resource="http://data.press.net/ontology/classification/" />
        <vs:term_status>testing</vs:term_status>
    </owl:Class>
    <owl:ObjectProperty rdf:about="http://data.press.net/ontology/classification/isClassifiedBy">
        <rdfs:subPropertyOf rdf:resource="http://purl.org/dc/terms/subject" />
        <psys:transitiveOver>
            <owl:TransitiveProperty rdf:about="http://data.press.net/ontology/classification/subClassificationOf">
                <rdfs:domain rdf:resource="http://data.press.net/ontology/classification/Classification" />
                <rdfs:range rdf:resource="http://data.press.net/ontology/classification/Classification" />
                <rdfs:label xml:lang="en">Parent-child transitive relationship between Classifications.</rdfs:label>
                <rdfs:comment xml:lang="en">Transitive property that allows classifications to be related to parent classifications</rdfs:comment>
                <rdfs:isDefinedBy rdf:resource="http://data.press.net/ontology/classification/" />
                <vs:term_status>testing</vs:term_status>
            </owl:TransitiveProperty>
        </psys:transitiveOver>
        <rdfs:domain>
            <owl:Class rdf:about="http://data.press.net/ontology/classification/Classifiable">
                <rdfs:label xml:lang="en">Generic Classifiable Class</rdfs:label>
                <rdfs:comment xml:lang="en">Generic Classifiable Class - inheriting from this makes the descendant Classifiable by a Classification</rdfs:comment>
                <rdfs:isDefinedBy rdf:resource="http://data.press.net/ontology/classification/" />
                <vs:term_status>testing</vs:term_status>
            </owl:Class>
        </rdfs:domain>
        <rdfs:range rdf:resource="http://data.press.net/ontology/classification/Classification" />
        <rdfs:label xml:lang="en">Property that associates Classifications with Classifiables. A subPropertyOf dcterms:subject</rdfs:label>
        <rdfs:comment xml:lang="en">Property that associates Classifications with Classifiables.  e.g. &lt;MyAsset&gt; isClassifiedBy &lt;SomeClassification&gt;</rdfs:comment>
        <rdfs:isDefinedBy rdf:resource="http://data.press.net/ontology/classification/" />
        <vs:term_status>testing</vs:term_status>
    </owl:ObjectProperty>
</rdf:RDF>