<?xml version="1.0" encoding="utf-8"?>
<rdf:RDF xmlns:adms="http://www.w3.org/ns/adms#"
   xmlns:cc="http://creativecommons.org/ns#"
   xmlns:dbpedia="http://dbpedia.org/ontology/"
   xmlns:dcam="http://purl.org/dc/dcam/"
   xmlns:dcterms="http://purl.org/dc/terms/"
   xmlns:foaf="http://xmlns.com/foaf/0.1/"
   xmlns:geo="http://www.w3.org/2003/01/geo/wgs84_pos#"
   xmlns:gn="http://www.geonames.org/ontology#"
   xmlns:gsp="http://www.opengis.net/ont/geosparql#"
   xmlns:ic="http://ontology.eil.utoronto.ca/icontact.owl#"
   xmlns:juso="http://rdfs.co/juso/"
   xmlns:lgdo="http://linkedgeodata.org/ontology/"
   xmlns:locn="http://www.w3.org/ns/locn#"
   xmlns:ngeo="http://geovocab.org/geometry#"
   xmlns:org="http://www.w3.org/ns/org#"
   xmlns:owl="http://www.w3.org/2002/07/owl#"
   xmlns:rdf="http://www.w3.org/1999/02/22-rdf-syntax-ns#"
   xmlns:rdfs="http://www.w3.org/2000/01/rdf-schema#"
   xmlns:schema="http://schema.org/"
   xmlns:skos="http://www.w3.org/2004/02/skos/core#"
   xmlns:spatial="http://geovocab.org/spatial#"
   xmlns:status="http://www.w3.org/2003/06/sw-vocab-status/ns#"
   xmlns:vann="http://purl.org/vocab/vann/"
   xmlns:vcard="http://www.w3.org/2006/vcard/ns#"
   xmlns:voaf="http://purl.org/vocommons/voaf#"
   xmlns:xsd="http://www.w3.org/2001/XMLSchema#">
  <foaf:Person rdf:about="http://jayg.me/">
    <owl:sameAs rdf:resource="http://listinc.kr/id/member/jgkim"/>
    <org:memberOf rdf:resource="http://listinc.kr/id/listinc"/>
    <foaf:homepage rdf:resource="http://jayg.org/"/>
    <foaf:mbox_sha1sum>f03421e94730da58e8943d3a1d2c4c6b02898e14</foaf:mbox_sha1sum>
    <foaf:name xml:lang="en">James G. Kim</foaf:name>
    <foaf:name xml:lang="ko">김보람</foaf:name>
  </foaf:Person>
  <rdf:Description rdf:about="http://linkedgeodata.org/ontology/Place">
    <rdfs:subClassOf rdf:resource="http://rdfs.co/juso/SpatialThing"/>
  </rdf:Description>
  <foaf:Organization rdf:about="http://listinc.kr/id/listinc">
    <rdf:type rdf:resource="http://www.w3.org/ns/org#Organization"/>
    <foaf:homepage rdf:resource="http://li-st.com/"/>
    <foaf:homepage rdf:resource="http://listinc.kr/"/>
    <foaf:mbox_sha1sum>de068365487dd2da1f2e88f1eaad0217bff79b40</foaf:mbox_sha1sum>
    <foaf:member rdf:resource="http://listinc.kr/id/member/jgkim"/>
    <foaf:name xml:lang="en">LiST Inc.</foaf:name>
    <foaf:name xml:lang="ko">주식회사 리스트</foaf:name>
  </foaf:Organization>
  <rdf:Description rdf:about="http://ontology.eil.utoronto.ca/icontact.owl#hasPostalCode">
    <owl:propertyChainAxiom>
      <rdf:Description>
        <rdf:first rdf:resource="http://rdfs.co/juso/postal_code"/>
        <rdf:rest>
          <rdf:Description>
            <rdf:first rdf:resource="http://www.w3.org/1999/02/22-rdf-syntax-ns#value"/>
            <rdf:rest rdf:resource="http://www.w3.org/1999/02/22-rdf-syntax-ns#nil"/>
          </rdf:Description>
        </rdf:rest>
      </rdf:Description>
    </owl:propertyChainAxiom>
  </rdf:Description>
  <rdf:Description rdf:about="http://ontology.eil.utoronto.ca/icontact.owl#hasState">
    <rdfs:subPropertyOf rdf:resource="http://rdfs.co/juso/first_level_administrative_division"/>
  </rdf:Description>
  <rdf:Description rdf:about="http://ontology.eil.utoronto.ca/icontact.owl#hasStreetNumber">
    <rdfs:subPropertyOf rdf:resource="http://rdfs.co/juso/thoroughfare_address"/>
  </rdf:Description>
  <rdf:Description rdf:about="http://purl.org/dc/terms/Location">
    <rdfs:subClassOf rdf:resource="http://rdfs.co/juso/SpatialThing"/>
  </rdf:Description>
  <owl:Ontology rdf:about="http://rdfs.co/juso/0.1.2">
    <cc:license rdf:resource="http://creativecommons.org/licenses/by/4.0/"/>
    <dcterms:creator rdf:resource="http://jayg.me/"/>
    <dcterms:description xml:lang="en">
    Juso Ontology is a Web vocabulary for describing geographical addresses and
    features.
    </dcterms:description>
    <dcterms:hasFormat rdf:resource="http://rdfs.co/juso/0.1.2/html"/>
    <dcterms:hasFormat rdf:resource="http://rdfs.co/juso/0.1.2/rdf"/>
    <dcterms:hasFormat rdf:resource="http://rdfs.co/juso/0.1.2/ttl"/>
    <dcterms:identifier>http://rdfs.co/juso/0.1.2</dcterms:identifier>
    <dcterms:isVersionOf rdf:resource="http://rdfs.co/juso/"/>
    <dcterms:issued rdf:datatype="http://www.w3.org/2001/XMLSchema#date">2015-10-02+09:00</dcterms:issued>
    <dcterms:modified rdf:datatype="http://www.w3.org/2001/XMLSchema#date">2015-12-30+09:00</dcterms:modified>
    <dcterms:publisher rdf:resource="http://listinc.kr/id/listinc"/>
    <dcterms:replaces rdf:resource="http://rdfs.co/juso/0.1.1"/>
    <dcterms:rights>Copyright © 2015 LiST Inc. Some Rights Reserved.</dcterms:rights>
    <dcterms:title xml:lang="en">Juso Ontology</dcterms:title>
    <dcterms:title xml:lang="ko">주소 온톨로지</dcterms:title>
    <dcterms:type rdf:resource="http://purl.org/adms/assettype/Ontology"/>
    <vann:example>
      <rdf:Description>
        <rdfs:comment rdf:datatype="http://www.w3.org/1999/02/22-rdf-syntax-ns#HTML">
    &lt;pre&gt;&lt;code&gt;_:YangyongBldg a juso:Feature ;
  juso:name "Yangyong Building"@en , "양용빌딩"@ko ;
  juso:geometry &amp;lt;http://geohash.org/wydjrzg6ece9&amp;gt; .

_:LiSTInc a juso:SpatialThing , foaf:Organization ;
  juso:name "LiST Inc."@en , "주식회사 리스트"@ko ;
  juso:within _:YangyongBldg ;
  juso:historical_address [
    a juso:Address ;
    juso:full_address
      "대한민국 서울특별시 영등포구 당산동 121-17 양용빌딩 9층 150-040"@ko ,
      "9th Floor, Yangyong Building, 121-17, Dangsan-dong, Yeongdeungpo-gu, Seoul, 150-040, South Korea"@en ;
    juso:country &amp;lt;http://sws.geonames.org/1835841/&amp;gt; ;
    juso:first_level_administrative_division &amp;lt;http://sws.geonames.org/1835847/&amp;gt; ;
    juso:second_level_administrative_division &amp;lt;http://sws.geonames.org/1832536/&amp;gt; ;
    juso:third_level_administrative_division &amp;lt;http://sws.geonames.org/8692617/&amp;gt; ;
    juso:locator _:YangyongBldg ;
    juso:locator_address "9층"@ko , "9th Floor"@en ;
    juso:postal_code [
      a juso:PostalCode ;
      rdf:value "150-040"
    ]
  ] ;
  juso:address [
    a juso:Address ;
    juso:full_address
      "대한민국 서울특별시 영등포구 버드나루로19길 3 (당산동) 양용빌딩 9층 07229"@ko ,
      "9th Floor, Yangyong Building, 3, Beodeunaru-ro 19-gil, Yeongdeungpo-gu, Seoul, 07229, South Korea"@en ;
    juso:country &amp;lt;http://sws.geonames.org/1835841/&amp;gt; ;
    juso:first_level_administrative_division &amp;lt;http://sws.geonames.org/1835847/&amp;gt; ;
    juso:second_level_administrative_division &amp;lt;http://sws.geonames.org/1832536/&amp;gt; ;
    juso:third_level_administrative_division &amp;lt;http://sws.geonames.org/8692617/&amp;gt; ;
    juso:thoroughfare [
      a juso:Street ;
      juso:name "Beodeunaru-ro 19-gil"@en , "버드나루로19길"@ko ;
      juso:parent &amp;lt;http://sws.geonames.org/8692617/&amp;gt;
    ] ;
    juso:thoroughfare_address "3" ;
    juso:locator _:YangyongBldg ;
    juso:locator_address "9층"@ko , "9th Floor"@en ;
    juso:postal_code [
      a juso:PostalCode ;
      rdf:value "07229"
    ]
  ] .&lt;/code&gt;&lt;/pre&gt;
    </rdfs:comment>
        <rdfs:label xml:lang="en">LiST Inc.</rdfs:label>
      </rdf:Description>
    </vann:example>
    <vann:preferredNamespacePrefix>juso</vann:preferredNamespacePrefix>
    <vann:preferredNamespaceUri>http://rdfs.co/juso/</vann:preferredNamespaceUri>
    <vann:termGroup rdf:resource="http://rdfs.co/juso/AddressGroup"/>
    <vann:termGroup rdf:resource="http://rdfs.co/juso/CoreGroup"/>
    <vann:termGroup rdf:resource="http://rdfs.co/juso/PoliticalDivisionGroup"/>
    <rdf:type rdf:resource="http://creativecommons.org/ns#Work"/>
    <rdf:type rdf:resource="http://purl.org/vocommons/voaf#Vocabulary"/>
    <rdf:type rdf:resource="http://www.w3.org/ns/adms#SemanticAsset"/>
    <rdfs:comment rdf:datatype="http://www.w3.org/1999/02/22-rdf-syntax-ns#HTML">
    &lt;div&gt;
      The master version of this vocabulary is maintained in &lt;a
      href="https://github.com/listinc/juso-ontology"&gt;the GitHub repository&lt;/a&gt;
      so others can contribute edits and improvements.
    &lt;/div&gt;
    </rdfs:comment>
    <rdfs:comment xml:lang="en">
    Most of the descriptions given here are from Wikipedia or from the related
    ontologies and vocabularies.
    </rdfs:comment>
    <rdfs:comment xml:lang="ko">
    There is an extension to this ontology with some country-specific terms for
    &lt;a href="http://rdfs.co/juso/kr/"&gt;South Korea&lt;/a&gt;.
    </rdfs:comment>
    <rdfs:seeAlso rdf:resource="https://github.com/listinc/juso-ontology"/>
    <owl:versionInfo>0.1.2</owl:versionInfo>
    <skos:changeNote>
      <rdf:Description>
        <dcterms:creator rdf:resource="http://jayg.me/"/>
        <dcterms:date rdf:datatype="http://www.w3.org/2001/XMLSchema#date">2015-10-07+09:00</dcterms:date>
        <rdf:value xml:lang="en">
      Fixed the wrong use of rdf:XMLLiteral
      </rdf:value>
      </rdf:Description>
    </skos:changeNote>
    <skos:historyNote>
      <rdf:Description>
        <dcterms:creator rdf:resource="http://jayg.me/"/>
        <dcterms:date rdf:datatype="http://www.w3.org/2001/XMLSchema#date">2015-11-10+09:00</dcterms:date>
        <rdf:value xml:lang="en">
      Added juso:Point, juso:wgs84_lat, juso:wgs84_long,
      juso:itrf2000_lat, and juso:itrf2000_long
      </rdf:value>
      </rdf:Description>
    </skos:historyNote>
    <skos:historyNote>
      <rdf:Description>
        <dcterms:creator rdf:resource="http://jayg.me/"/>
        <dcterms:date rdf:datatype="http://www.w3.org/2001/XMLSchema#date">2015-12-30+09:00</dcterms:date>
        <rdf:value xml:lang="en">
      Added juso:official_name, juso:alternate_name, juso:short_name
      </rdf:value>
      </rdf:Description>
    </skos:historyNote>
    <adms:status rdf:resource="http://purl.org/adms/status/UnderDevelopment"/>
  </owl:Ontology>
  <rdf:Description rdf:about="http://rdfs.co/juso/0.1.2/html">
    <dcterms:format>
      <dcterms:MediaType>
        <dcam:memberOf rdf:resource="http://purl.org/dc/terms/IMT"/>
        <rdf:value>text/html</rdf:value>
        <rdfs:label xml:lang="en">HTML</rdfs:label>
        <rdfs:seeAlso rdf:resource="http://www.iana.org/assignments/media-types/text/html"/>
        <owl:sameAs rdf:resource="https://w3id.org/spar/mediatype/text/html"/>
      </dcterms:MediaType>
    </dcterms:format>
  </rdf:Description>
  <rdf:Description rdf:about="http://rdfs.co/juso/0.1.2/rdf">
    <dcterms:format>
      <dcterms:MediaType>
        <dcam:memberOf rdf:resource="http://purl.org/dc/terms/IMT"/>
        <rdf:value>application/rdf+xml</rdf:value>
        <rdfs:label xml:lang="en">RDF/XML</rdfs:label>
        <rdfs:seeAlso rdf:resource="http://www.iana.org/assignments/media-types/application/rdf+xml"/>
        <owl:sameAs rdf:resource="https://w3id.org/spar/mediatype/application/rdf%2Bxml"/>
      </dcterms:MediaType>
    </dcterms:format>
  </rdf:Description>
  <rdf:Description rdf:about="http://rdfs.co/juso/0.1.2/ttl">
    <dcterms:format>
      <dcterms:MediaType>
        <dcam:memberOf rdf:resource="http://purl.org/dc/terms/IMT"/>
        <rdf:value>text/turtle</rdf:value>
        <rdfs:label xml:lang="en">Turtle</rdfs:label>
        <rdfs:seeAlso rdf:resource="http://www.iana.org/assignments/media-types/text/turtle"/>
        <owl:sameAs rdf:resource="https://w3id.org/spar/mediatype/text/turtle"/>
      </dcterms:MediaType>
    </dcterms:format>
  </rdf:Description>
  <owl:Class rdf:about="http://rdfs.co/juso/Address">
    <dcterms:issued rdf:datatype="http://www.w3.org/2001/XMLSchema#date">2015-10-02+09:00</dcterms:issued>
    <dcterms:modified rdf:datatype="http://www.w3.org/2001/XMLSchema#date">2015-10-02+09:00</dcterms:modified>
    <rdfs:isDefinedBy rdf:resource="http://rdfs.co/juso/"/>
    <rdfs:seeAlso rdf:resource="https://en.wikipedia.org/wiki/Address_(geography)"/>
    <owl:sameAs rdf:resource="http://ontology.eil.utoronto.ca/icontact.owl#Address"/>
    <owl:sameAs rdf:resource="http://www.w3.org/ns/locn#Address"/>
    <status:term_status xml:lang="en">testing</status:term_status>
    <skos:altLabel xml:lang="en">Geographical Address</skos:altLabel>
    <skos:altLabel xml:lang="en">Postal Address</skos:altLabel>
    <skos:definition xml:lang="en">
    An address is a collection of information, presented in a mostly fixed
    format, used for describing the location of a building, apartment, or other
    structure or a plot of land, generally using political boundaries and
    street names as references, along with other identifiers such as house or
    apartment numbers. Some addresses also contain special codes to aid routing
    of mail and packages, such as a ZIP code or post code.
    </skos:definition>
    <skos:prefLabel xml:lang="en">Address</skos:prefLabel>
    <skos:prefLabel xml:lang="ko">주소</skos:prefLabel>
  </owl:Class>
  <rdf:Bag rdf:about="http://rdfs.co/juso/AddressGroup">
    <rdf:_1 rdf:resource="http://rdfs.co/juso/full_address"/>
    <rdf:_10 rdf:resource="http://rdfs.co/juso/thoroughfare"/>
    <rdf:_11 rdf:resource="http://rdfs.co/juso/thoroughfare_address"/>
    <rdf:_12 rdf:resource="http://rdfs.co/juso/locator"/>
    <rdf:_13 rdf:resource="http://rdfs.co/juso/locator_address"/>
    <rdf:_14 rdf:resource="http://rdfs.co/juso/po_box"/>
    <rdf:_15 rdf:resource="http://rdfs.co/juso/PostalCode"/>
    <rdf:_16 rdf:resource="http://rdfs.co/juso/postal_code"/>
    <rdf:_2 rdf:resource="http://rdfs.co/juso/country"/>
    <rdf:_3 rdf:resource="http://rdfs.co/juso/first_level_administrative_division"/>
    <rdf:_4 rdf:resource="http://rdfs.co/juso/second_level_administrative_division"/>
    <rdf:_5 rdf:resource="http://rdfs.co/juso/third_level_administrative_division"/>
    <rdf:_6 rdf:resource="http://rdfs.co/juso/fourth_level_administrative_division"/>
    <rdf:_7 rdf:resource="http://rdfs.co/juso/fifth_level_administrative_division"/>
    <rdf:_8 rdf:resource="http://rdfs.co/juso/Thoroughfare"/>
    <rdf:_9 rdf:resource="http://rdfs.co/juso/Street"/>
    <rdfs:comment xml:lang="en">
    These classes and properties are used to describe addresses.
    </rdfs:comment>
    <rdfs:label xml:lang="en">Address Terms</rdfs:label>
  </rdf:Bag>
  <owl:Class rdf:about="http://rdfs.co/juso/AdministrativeDivision">
    <dcterms:issued rdf:datatype="http://www.w3.org/2001/XMLSchema#date">2015-10-02+09:00</dcterms:issued>
    <dcterms:modified rdf:datatype="http://www.w3.org/2001/XMLSchema#date">2015-10-02+09:00</dcterms:modified>
    <rdfs:isDefinedBy rdf:resource="http://rdfs.co/juso/"/>
    <rdfs:seeAlso rdf:resource="http://www.geonames.org/ontology#A.ADMD"/>
    <rdfs:seeAlso rdf:resource="https://en.wikipedia.org/wiki/Administrative_division"/>
    <rdfs:subClassOf rdf:resource="http://rdfs.co/juso/PoliticalDivision"/>
    <status:term_status xml:lang="en">unstable</status:term_status>
    <skos:altLabel xml:lang="en">Administrative Entity</skos:altLabel>
    <skos:altLabel xml:lang="en">Administrative Unit</skos:altLabel>
    <skos:altLabel xml:lang="en">Country Subdivision</skos:altLabel>
    <skos:altLabel xml:lang="en">Geopolitical Division</skos:altLabel>
    <skos:altLabel xml:lang="en">Subnational Entity</skos:altLabel>
    <skos:definition xml:lang="en">
    An administrative division is a portion of a country or other region
    delineated for the purpose of administration. Administrative divisions are
    each granted a certain degree of autonomy and are usually required to
    manage themselves through their own local governments.
    </skos:definition>
    <skos:prefLabel xml:lang="en">Administrative Division</skos:prefLabel>
  </owl:Class>
  <owl:Class rdf:about="http://rdfs.co/juso/CapitalDistrict">
    <dcterms:issued rdf:datatype="http://www.w3.org/2001/XMLSchema#date">2015-10-02+09:00</dcterms:issued>
    <dcterms:modified rdf:datatype="http://www.w3.org/2001/XMLSchema#date">2015-10-02+09:00</dcterms:modified>
    <rdfs:isDefinedBy rdf:resource="http://rdfs.co/juso/"/>
    <rdfs:seeAlso rdf:resource="https://en.wikipedia.org/wiki/Capital_districts_and_territories"/>
    <rdfs:subClassOf rdf:resource="http://rdfs.co/juso/AdministrativeDivision"/>
    <status:term_status xml:lang="en">unstable</status:term_status>
    <skos:altLabel xml:lang="en">Capital Territory</skos:altLabel>
    <skos:definition xml:lang="en">
    A capital district or capital territory is normally a specially designated
    administrative division where a country's seat of government is located.
    </skos:definition>
    <skos:prefLabel xml:lang="en">Capital District</skos:prefLabel>
  </owl:Class>
  <owl:Class rdf:about="http://rdfs.co/juso/City">
    <dcterms:issued rdf:datatype="http://www.w3.org/2001/XMLSchema#date">2015-10-02+09:00</dcterms:issued>
    <dcterms:modified rdf:datatype="http://www.w3.org/2001/XMLSchema#date">2015-10-02+09:00</dcterms:modified>
    <rdfs:isDefinedBy rdf:resource="http://rdfs.co/juso/"/>
    <rdfs:seeAlso rdf:resource="https://en.wikipedia.org/wiki/City"/>
    <rdfs:subClassOf rdf:resource="http://rdfs.co/juso/AdministrativeDivision"/>
    <rdfs:subClassOf rdf:resource="http://schema.org/City"/>
    <owl:sameAs rdf:resource="http://dbpedia.org/ontology/City"/>
    <owl:sameAs rdf:resource="http://linkedgeodata.org/ontology/City"/>
    <status:term_status xml:lang="en">unstable</status:term_status>
    <skos:definition xml:lang="en">
    A city is a large and permanent human settlement. Although there is no
    agreement on how a city is distinguished from a town in general English
    language meanings, many cities have a particular administrative, legal, or
    historical status based on local law.
    </skos:definition>
    <skos:prefLabel xml:lang="en">City</skos:prefLabel>
    <skos:prefLabel xml:lang="ja">市</skos:prefLabel>
    <skos:prefLabel xml:lang="ko">시</skos:prefLabel>
  </owl:Class>
  <owl:Class rdf:about="http://rdfs.co/juso/ConsolidatedCityCounty">
    <dcterms:issued rdf:datatype="http://www.w3.org/2001/XMLSchema#date">2015-10-02+09:00</dcterms:issued>
    <dcterms:modified rdf:datatype="http://www.w3.org/2001/XMLSchema#date">2015-10-02+09:00</dcterms:modified>
    <rdfs:isDefinedBy rdf:resource="http://rdfs.co/juso/"/>
    <rdfs:seeAlso rdf:resource="https://en.wikipedia.org/wiki/Consolidated_city-county"/>
    <rdfs:subClassOf rdf:resource="http://rdfs.co/juso/City"/>
    <rdfs:subClassOf rdf:resource="http://rdfs.co/juso/County"/>
    <status:term_status xml:lang="en">unstable</status:term_status>
    <skos:definition xml:lang="en">
    A consolidated city-county is a city and county that have been merged into
    one unified jurisdiction. As such it is simultaneously a city, which is a
    municipal corporation, and a county, which is an administrative division of
    a state. It has the powers and responsibilities of both types of entities.
    </skos:definition>
    <skos:prefLabel xml:lang="en">Consolidated City-county</skos:prefLabel>
  </owl:Class>
  <rdf:Bag rdf:about="http://rdfs.co/juso/CoreGroup">
    <rdf:_1 rdf:resource="http://rdfs.co/juso/SpatialThing"/>
    <rdf:_10 rdf:resource="http://rdfs.co/juso/within"/>
    <rdf:_11 rdf:resource="http://rdfs.co/juso/endonym"/>
    <rdf:_12 rdf:resource="http://rdfs.co/juso/exonym"/>
    <rdf:_13 rdf:resource="http://rdfs.co/juso/geometry"/>
    <rdf:_14 rdf:resource="http://rdfs.co/juso/address"/>
    <rdf:_15 rdf:resource="http://rdfs.co/juso/historical_address"/>
    <rdf:_2 rdf:resource="http://rdfs.co/juso/Feature"/>
    <rdf:_3 rdf:resource="http://rdfs.co/juso/Geometry"/>
    <rdf:_4 rdf:resource="http://rdfs.co/juso/Point"/>
    <rdf:_5 rdf:resource="http://rdfs.co/juso/Address"/>
    <rdf:_6 rdf:resource="http://rdfs.co/juso/name"/>
    <rdf:_7 rdf:resource="http://rdfs.co/juso/official_name"/>
    <rdf:_8 rdf:resource="http://rdfs.co/juso/alternate_name"/>
    <rdf:_9 rdf:resource="http://rdfs.co/juso/short_name"/>
    <rdfs:comment xml:lang="en">
    These classes and properties form the core of Juso Ontology. They describe
    fundamental characteristics of geography in relatively broad terms.
    </rdfs:comment>
    <rdfs:label xml:lang="en">Core Terms</rdfs:label>
  </rdf:Bag>
  <owl:Class rdf:about="http://rdfs.co/juso/Country">
    <dcterms:issued rdf:datatype="http://www.w3.org/2001/XMLSchema#date">2015-10-02+09:00</dcterms:issued>
    <dcterms:modified rdf:datatype="http://www.w3.org/2001/XMLSchema#date">2015-10-02+09:00</dcterms:modified>
    <rdfs:isDefinedBy rdf:resource="http://rdfs.co/juso/"/>
    <rdfs:seeAlso rdf:resource="https://en.wikipedia.org/wiki/Country"/>
    <rdfs:subClassOf rdf:resource="http://rdfs.co/juso/PoliticalDivision"/>
    <owl:sameAs rdf:resource="http://dbpedia.org/ontology/Country"/>
    <owl:sameAs rdf:resource="http://linkedgeodata.org/ontology/Country"/>
    <owl:sameAs rdf:resource="http://schema.org/Country"/>
    <status:term_status xml:lang="en">unstable</status:term_status>
    <skos:altLabel xml:lang="ja">国家</skos:altLabel>
    <skos:altLabel xml:lang="ko">국가</skos:altLabel>
    <skos:definition xml:lang="en">
    A country is a region that is identified as a distinct entity in political
    geography. A country may be an independent sovereign state or one that is
    occupied by another state, as a non-sovereign or formerly sovereign
    political division, or a geographic region associated with sets of
    previously independent or differently associated people with distinct
    political characteristics.
    </skos:definition>
    <skos:prefLabel xml:lang="en">Country</skos:prefLabel>
    <skos:prefLabel xml:lang="ja">国</skos:prefLabel>
    <skos:prefLabel xml:lang="ko">나라</skos:prefLabel>
  </owl:Class>
  <owl:Class rdf:about="http://rdfs.co/juso/County">
    <dcterms:issued rdf:datatype="http://www.w3.org/2001/XMLSchema#date">2015-10-02+09:00</dcterms:issued>
    <dcterms:modified rdf:datatype="http://www.w3.org/2001/XMLSchema#date">2015-10-02+09:00</dcterms:modified>
    <rdfs:isDefinedBy rdf:resource="http://rdfs.co/juso/"/>
    <rdfs:seeAlso rdf:resource="https://en.wikipedia.org/wiki/County"/>
    <rdfs:subClassOf rdf:resource="http://rdfs.co/juso/AdministrativeDivision"/>
    <owl:sameAs rdf:resource="http://linkedgeodata.org/ontology/County"/>
    <status:term_status xml:lang="en">unstable</status:term_status>
    <skos:altLabel xml:lang="en-US">Cnty.</skos:altLabel>
    <skos:altLabel xml:lang="en-GB">Co.</skos:altLabel>
    <skos:definition xml:lang="en">
    A county is a geographical region of a country used for administrative or
    other purposes, in certain modern nations.
    </skos:definition>
    <skos:prefLabel xml:lang="en">County</skos:prefLabel>
    <skos:prefLabel xml:lang="ko">군</skos:prefLabel>
  </owl:Class>
  <owl:Class rdf:about="http://rdfs.co/juso/District">
    <dcterms:issued rdf:datatype="http://www.w3.org/2001/XMLSchema#date">2015-10-02+09:00</dcterms:issued>
    <dcterms:modified rdf:datatype="http://www.w3.org/2001/XMLSchema#date">2015-10-02+09:00</dcterms:modified>
    <rdfs:isDefinedBy rdf:resource="http://rdfs.co/juso/"/>
    <rdfs:seeAlso rdf:resource="https://en.wikipedia.org/wiki/District"/>
    <rdfs:subClassOf rdf:resource="http://rdfs.co/juso/AdministrativeDivision"/>
    <owl:sameAs rdf:resource="http://dbpedia.org/ontology/District"/>
    <status:term_status xml:lang="en">unstable</status:term_status>
    <skos:definition xml:lang="en">
    A district is a type of administrative division that, in some countries, is
    managed by local government. Across the world, areas known as "districts"
    vary greatly in size, spanning entire regions or counties, several
    municipalities, subdivisions of municipalities, school district, or
    political district.
    </skos:definition>
    <skos:prefLabel xml:lang="en">District</skos:prefLabel>
    <skos:prefLabel xml:lang="ko">구</skos:prefLabel>
  </owl:Class>
  <owl:Class rdf:about="http://rdfs.co/juso/Feature">
    <dcterms:issued rdf:datatype="http://www.w3.org/2001/XMLSchema#date">2015-10-02+09:00</dcterms:issued>
    <dcterms:modified rdf:datatype="http://www.w3.org/2001/XMLSchema#date">2015-10-02+09:00</dcterms:modified>
    <rdfs:isDefinedBy rdf:resource="http://rdfs.co/juso/"/>
    <rdfs:seeAlso rdf:resource="https://en.wikipedia.org/wiki/Geographical_feature"/>
    <rdfs:subClassOf rdf:resource="http://rdfs.co/juso/SpatialThing"/>
    <rdfs:subClassOf rdf:resource="http://www.opengis.net/ont/geosparql#Feature"/>
    <owl:disjointWith rdf:resource="http://rdfs.co/juso/Geometry"/>
    <owl:equivalentClass rdf:resource="http://www.geonames.org/ontology#Feature"/>
    <owl:sameAs rdf:resource="http://geovocab.org/spatial#Feature"/>
    <status:term_status xml:lang="en">unstable</status:term_status>
    <skos:altLabel xml:lang="en">Feature</skos:altLabel>
    <skos:definition xml:lang="en">
    Geographical features are man-made or naturally-created features associated
    with a location relative to the Earth.
    </skos:definition>
    <skos:prefLabel xml:lang="en">Geographical Feature</skos:prefLabel>
  </owl:Class>
  <owl:Class rdf:about="http://rdfs.co/juso/FederatedState">
    <dcterms:issued rdf:datatype="http://www.w3.org/2001/XMLSchema#date">2015-10-02+09:00</dcterms:issued>
    <dcterms:modified rdf:datatype="http://www.w3.org/2001/XMLSchema#date">2015-10-02+09:00</dcterms:modified>
    <rdfs:isDefinedBy rdf:resource="http://rdfs.co/juso/"/>
    <rdfs:seeAlso rdf:resource="https://en.wikipedia.org/wiki/Federated_state"/>
    <rdfs:subClassOf rdf:resource="http://dbpedia.org/ontology/State"/>
    <rdfs:subClassOf rdf:resource="http://linkedgeodata.org/ontology/State"/>
    <rdfs:subClassOf rdf:resource="http://rdfs.co/juso/AdministrativeDivision"/>
    <rdfs:subClassOf rdf:resource="http://schema.org/State"/>
    <status:term_status xml:lang="en">unstable</status:term_status>
    <skos:altLabel xml:lang="en">State</skos:altLabel>
    <skos:altLabel xml:lang="ko">주</skos:altLabel>
    <skos:definition xml:lang="en">
    A federated state is a territorial and constitutional community forming
    part of a federal union (federation) such as the United States and
    Australia.
    </skos:definition>
    <skos:prefLabel xml:lang="en">Federated State</skos:prefLabel>
    <skos:prefLabel xml:lang="ko">연방주</skos:prefLabel>
  </owl:Class>
  <owl:Class rdf:about="http://rdfs.co/juso/FifthLevelAdministrativeDivision">
    <dcterms:issued rdf:datatype="http://www.w3.org/2001/XMLSchema#date">2015-10-02+09:00</dcterms:issued>
    <dcterms:modified rdf:datatype="http://www.w3.org/2001/XMLSchema#date">2015-10-02+09:00</dcterms:modified>
    <rdfs:isDefinedBy rdf:resource="http://rdfs.co/juso/"/>
    <rdfs:seeAlso rdf:resource="http://www.geonames.org/ontology#A.ADM5"/>
    <rdfs:subClassOf rdf:resource="http://rdfs.co/juso/AdministrativeDivision"/>
    <status:term_status xml:lang="en">unstable</status:term_status>
    <skos:altLabel xml:lang="en">Fifth Administrative Level</skos:altLabel>
    <skos:altLabel xml:lang="en">Fifth-order Administrative Division</skos:altLabel>
    <skos:definition xml:lang="en">
    A subdivision of a fourth-level administrative division.
    </skos:definition>
    <skos:prefLabel xml:lang="en">Fifth-level Administrative Division</skos:prefLabel>
  </owl:Class>
  <owl:Class rdf:about="http://rdfs.co/juso/FirstLevelAdministrativeDivision">
    <dcterms:issued rdf:datatype="http://www.w3.org/2001/XMLSchema#date">2015-10-02+09:00</dcterms:issued>
    <dcterms:modified rdf:datatype="http://www.w3.org/2001/XMLSchema#date">2015-10-02+09:00</dcterms:modified>
    <rdfs:isDefinedBy rdf:resource="http://rdfs.co/juso/"/>
    <rdfs:seeAlso rdf:resource="http://www.geonames.org/ontology#A.ADM1"/>
    <rdfs:subClassOf rdf:resource="http://rdfs.co/juso/AdministrativeDivision"/>
    <status:term_status xml:lang="en">unstable</status:term_status>
    <skos:altLabel xml:lang="en">First Administrative Level</skos:altLabel>
    <skos:altLabel xml:lang="en">First-order Administrative Division</skos:altLabel>
    <skos:definition xml:lang="en">
    A primary administrative division of a country, such as a state in the
    United States.
    </skos:definition>
    <skos:prefLabel xml:lang="en">First-level Administrative Division</skos:prefLabel>
  </owl:Class>
  <owl:Class rdf:about="http://rdfs.co/juso/FourthLevelAdministrativeDivision">
    <dcterms:issued rdf:datatype="http://www.w3.org/2001/XMLSchema#date">2015-10-02+09:00</dcterms:issued>
    <dcterms:modified rdf:datatype="http://www.w3.org/2001/XMLSchema#date">2015-10-02+09:00</dcterms:modified>
    <rdfs:isDefinedBy rdf:resource="http://rdfs.co/juso/"/>
    <rdfs:seeAlso rdf:resource="http://www.geonames.org/ontology#A.ADM4"/>
    <rdfs:subClassOf rdf:resource="http://rdfs.co/juso/AdministrativeDivision"/>
    <status:term_status xml:lang="en">unstable</status:term_status>
    <skos:altLabel xml:lang="en">Fourth Administrative Level</skos:altLabel>
    <skos:altLabel xml:lang="en">Fourth-order Administrative Division</skos:altLabel>
    <skos:definition xml:lang="en">
    A subdivision of a third-level administrative division.
    </skos:definition>
    <skos:prefLabel xml:lang="en">Fourth-level Administrative Division</skos:prefLabel>
  </owl:Class>
  <owl:Class rdf:about="http://rdfs.co/juso/Geometry">
    <dcterms:issued rdf:datatype="http://www.w3.org/2001/XMLSchema#date">2015-10-02+09:00</dcterms:issued>
    <dcterms:modified rdf:datatype="http://www.w3.org/2001/XMLSchema#date">2015-10-02+09:00</dcterms:modified>
    <rdfs:isDefinedBy rdf:resource="http://rdfs.co/juso/"/>
    <rdfs:seeAlso rdf:resource="https://en.wikipedia.org/wiki/Geometry"/>
    <rdfs:subClassOf rdf:resource="http://rdfs.co/juso/SpatialThing"/>
    <owl:disjointWith rdf:resource="http://rdfs.co/juso/Feature"/>
    <owl:sameAs rdf:resource="http://geovocab.org/geometry#Geometry"/>
    <owl:sameAs rdf:resource="http://www.opengis.net/ont/geosparql#Geometry"/>
    <owl:sameAs rdf:resource="http://www.w3.org/ns/locn#Geometry"/>
    <status:term_status xml:lang="en">unstable</status:term_status>
    <skos:definition xml:lang="en">
    Geometry provides "the means for the quantitative description, by means of
    coordinates and mathematical functions, of the spatial characteristics of
    features, including dimension, position, size, shape, and orientation", as
    defined in ISO 19107.
    </skos:definition>
    <skos:prefLabel xml:lang="en">Geometry</skos:prefLabel>
    <skos:prefLabel xml:lang="ko">기하</skos:prefLabel>
  </owl:Class>
  <owl:Class rdf:about="http://rdfs.co/juso/Hamlet">
    <dcterms:issued rdf:datatype="http://www.w3.org/2001/XMLSchema#date">2015-10-02+09:00</dcterms:issued>
    <dcterms:modified rdf:datatype="http://www.w3.org/2001/XMLSchema#date">2015-10-02+09:00</dcterms:modified>
    <rdfs:isDefinedBy rdf:resource="http://rdfs.co/juso/"/>
    <rdfs:seeAlso rdf:resource="https://en.wikipedia.org/wiki/Hamlet_(place)"/>
    <rdfs:subClassOf rdf:resource="http://rdfs.co/juso/AdministrativeDivision"/>
    <owl:sameAs rdf:resource="http://linkedgeodata.org/ontology/Hamlet"/>
    <status:term_status xml:lang="en">unstable</status:term_status>
    <skos:definition xml:lang="en">
    A hamlet is a type of settlement. The definition of hamlet varies by
    country. It usually refers to a small settlement, with a small population
    that is usually under 100, in a rural area, or a component of a larger
    settlement or municipality. Hamlets are typically unincorporated
    communities.
    </skos:definition>
    <skos:prefLabel xml:lang="en">Hamlet</skos:prefLabel>
  </owl:Class>
  <owl:Class rdf:about="http://rdfs.co/juso/Municipality">
    <dcterms:issued rdf:datatype="http://www.w3.org/2001/XMLSchema#date">2015-10-02+09:00</dcterms:issued>
    <dcterms:modified rdf:datatype="http://www.w3.org/2001/XMLSchema#date">2015-10-02+09:00</dcterms:modified>
    <rdfs:isDefinedBy rdf:resource="http://rdfs.co/juso/"/>
    <rdfs:seeAlso rdf:resource="https://en.wikipedia.org/wiki/Municipality"/>
    <rdfs:subClassOf rdf:resource="http://rdfs.co/juso/AdministrativeDivision"/>
    <owl:sameAs rdf:resource="http://dbpedia.org/ontology/Municipality"/>
    <owl:sameAs rdf:resource="http://linkedgeodata.org/ontology/Municipality"/>
    <status:term_status xml:lang="en">unstable</status:term_status>
    <skos:definition xml:lang="en">
    A municipality is usually an urban administrative division having corporate
    status and usually powers of self-government or jurisdiction.
    </skos:definition>
    <skos:prefLabel xml:lang="en">Municipality</skos:prefLabel>
  </owl:Class>
  <owl:Class rdf:about="http://rdfs.co/juso/Neighborhood">
    <dcterms:issued rdf:datatype="http://www.w3.org/2001/XMLSchema#date">2015-10-02+09:00</dcterms:issued>
    <dcterms:modified rdf:datatype="http://www.w3.org/2001/XMLSchema#date">2015-10-02+09:00</dcterms:modified>
    <rdfs:isDefinedBy rdf:resource="http://rdfs.co/juso/"/>
    <rdfs:seeAlso rdf:resource="https://en.wikipedia.org/wiki/Neighbourhood"/>
    <rdfs:subClassOf rdf:resource="http://rdfs.co/juso/AdministrativeDivision"/>
    <status:term_status xml:lang="en">unstable</status:term_status>
    <skos:definition xml:lang="en">
    A neighborhood, or neighbourhood, is a geographically localised community
    within a larger city, town, suburb or rural area.
    </skos:definition>
    <skos:prefLabel xml:lang="en-US">Neighborhood</skos:prefLabel>
    <skos:prefLabel xml:lang="en-GB">Neighbourhood</skos:prefLabel>
    <skos:prefLabel xml:lang="ko">동</skos:prefLabel>
  </owl:Class>
  <owl:Class rdf:about="http://rdfs.co/juso/Parish">
    <dcterms:issued rdf:datatype="http://www.w3.org/2001/XMLSchema#date">2015-10-02+09:00</dcterms:issued>
    <dcterms:modified rdf:datatype="http://www.w3.org/2001/XMLSchema#date">2015-10-02+09:00</dcterms:modified>
    <rdfs:isDefinedBy rdf:resource="http://rdfs.co/juso/"/>
    <rdfs:seeAlso rdf:resource="https://en.wikipedia.org/wiki/Parish_(administrative_division)"/>
    <rdfs:subClassOf rdf:resource="http://rdfs.co/juso/AdministrativeDivision"/>
    <status:term_status xml:lang="en">unstable</status:term_status>
    <skos:altLabel xml:lang="en-GB">Civil Parish</skos:altLabel>
    <skos:definition xml:lang="en">
    A parish is an administrative division used by several countries. In parts
    of the British Isles it is known as a civil parish to distinguish it from
    the ecclesiastical parish.
    </skos:definition>
    <skos:prefLabel xml:lang="en">Parish</skos:prefLabel>
  </owl:Class>
  <owl:Class rdf:about="http://rdfs.co/juso/Point">
    <dcterms:issued rdf:datatype="http://www.w3.org/2001/XMLSchema#date">2015-11-10+09:00</dcterms:issued>
    <dcterms:modified rdf:datatype="http://www.w3.org/2001/XMLSchema#date">2015-11-10+09:00</dcterms:modified>
    <rdfs:isDefinedBy rdf:resource="http://rdfs.co/juso/"/>
    <rdfs:seeAlso rdf:resource="https://en.wikipedia.org/wiki/Point_(geometry)"/>
    <rdfs:subClassOf rdf:resource="http://rdfs.co/juso/Geometry"/>
    <owl:sameAs rdf:resource="http://www.w3.org/2003/01/geo/wgs84_pos#Point"/>
    <status:term_status xml:lang="en">unstable</status:term_status>
    <skos:definition xml:lang="en">
    A point is a geographical point on the surface of the Earth, typically
    described using a coordinate system relative to the Earth, such as WGS84.
  </skos:definition>
    <skos:prefLabel xml:lang="en">Point</skos:prefLabel>
    <skos:prefLabel xml:lang="ko">점</skos:prefLabel>
  </owl:Class>
  <owl:Class rdf:about="http://rdfs.co/juso/PoliticalDivision">
    <dcterms:issued rdf:datatype="http://www.w3.org/2001/XMLSchema#date">2015-10-02+09:00</dcterms:issued>
    <dcterms:modified rdf:datatype="http://www.w3.org/2001/XMLSchema#date">2015-10-02+09:00</dcterms:modified>
    <rdfs:isDefinedBy rdf:resource="http://rdfs.co/juso/"/>
    <rdfs:seeAlso rdf:resource="https://en.wikipedia.org/wiki/Political_division"/>
    <rdfs:subClassOf rdf:resource="http://rdfs.co/juso/Feature"/>
    <owl:equivalentClass rdf:resource="http://schema.org/AdministrativeArea"/>
    <status:term_status xml:lang="en">unstable</status:term_status>
    <skos:definition xml:lang="en">
    A political division is a geographic region accepted to be in the
    jurisdiction of a particular governmental entity. The particular government
    entity varies as each organizes its operations by further divisions
    (subdivisions of the state) to further its tasks and satisfy its
    responsibilities.
    </skos:definition>
    <skos:prefLabel xml:lang="en">Political Division</skos:prefLabel>
  </owl:Class>
  <rdf:Bag rdf:about="http://rdfs.co/juso/PoliticalDivisionGroup">
    <rdf:_1 rdf:resource="http://rdfs.co/juso/PoliticalDivision"/>
    <rdf:_10 rdf:resource="http://rdfs.co/juso/Province"/>
    <rdf:_11 rdf:resource="http://rdfs.co/juso/County"/>
    <rdf:_12 rdf:resource="http://rdfs.co/juso/Parish"/>
    <rdf:_13 rdf:resource="http://rdfs.co/juso/Borough"/>
    <rdf:_14 rdf:resource="http://rdfs.co/juso/CapitalDistrict"/>
    <rdf:_15 rdf:resource="http://rdfs.co/juso/City"/>
    <rdf:_16 rdf:resource="http://rdfs.co/juso/ConsolidatedCityCounty"/>
    <rdf:_17 rdf:resource="http://rdfs.co/juso/Municipality"/>
    <rdf:_18 rdf:resource="http://rdfs.co/juso/District"/>
    <rdf:_19 rdf:resource="http://rdfs.co/juso/Town"/>
    <rdf:_2 rdf:resource="http://rdfs.co/juso/Country"/>
    <rdf:_20 rdf:resource="http://rdfs.co/juso/Township"/>
    <rdf:_21 rdf:resource="http://rdfs.co/juso/Neighborhood"/>
    <rdf:_22 rdf:resource="http://rdfs.co/juso/Village"/>
    <rdf:_23 rdf:resource="http://rdfs.co/juso/Hamlet"/>
    <rdf:_24 rdf:resource="http://rdfs.co/juso/political_division"/>
    <rdf:_25 rdf:resource="http://rdfs.co/juso/parent"/>
    <rdf:_3 rdf:resource="http://rdfs.co/juso/AdministrativeDivision"/>
    <rdf:_4 rdf:resource="http://rdfs.co/juso/FirstLevelAdministrativeDivision"/>
    <rdf:_5 rdf:resource="http://rdfs.co/juso/SecondLevelAdministrativeDivision"/>
    <rdf:_6 rdf:resource="http://rdfs.co/juso/ThirdLevelAdministrativeDivision"/>
    <rdf:_7 rdf:resource="http://rdfs.co/juso/FourthLevelAdministrativeDivision"/>
    <rdf:_8 rdf:resource="http://rdfs.co/juso/FifthLevelAdministrativeDivision"/>
    <rdf:_9 rdf:resource="http://rdfs.co/juso/FederatedState"/>
    <rdfs:comment xml:lang="en">
    These classes and properties are used to describe political and
    administrative divisions.
    </rdfs:comment>
    <rdfs:label xml:lang="en">Political Division Terms</rdfs:label>
  </rdf:Bag>
  <owl:Class rdf:about="http://rdfs.co/juso/PostalCode">
    <dcterms:issued rdf:datatype="http://www.w3.org/2001/XMLSchema#date">2015-10-02+09:00</dcterms:issued>
    <dcterms:modified rdf:datatype="http://www.w3.org/2001/XMLSchema#date">2015-10-02+09:00</dcterms:modified>
    <rdfs:isDefinedBy rdf:resource="http://rdfs.co/juso/"/>
    <rdfs:seeAlso rdf:resource="https://en.wikipedia.org/wiki/Postal_code"/>
    <status:term_status xml:lang="en">unstable</status:term_status>
    <skos:altLabel xml:lang="en">Eircode</skos:altLabel>
    <skos:altLabel xml:lang="en">PIN Code</skos:altLabel>
    <skos:altLabel xml:lang="en">Post Code</skos:altLabel>
    <skos:altLabel xml:lang="en">Postcode</skos:altLabel>
    <skos:altLabel xml:lang="en">ZIP Code</skos:altLabel>
    <skos:definition xml:lang="en">
    A postal code is a series of letters and/or digits, sometimes including
    spaces or punctuation, included in a postal address for the purpose of
    sorting mail.
    </skos:definition>
    <skos:prefLabel xml:lang="en">Postal Code</skos:prefLabel>
    <skos:prefLabel xml:lang="ko">우편번호</skos:prefLabel>
  </owl:Class>
  <owl:Class rdf:about="http://rdfs.co/juso/Province">
    <dcterms:issued rdf:datatype="http://www.w3.org/2001/XMLSchema#date">2015-10-02+09:00</dcterms:issued>
    <dcterms:modified rdf:datatype="http://www.w3.org/2001/XMLSchema#date">2015-10-02+09:00</dcterms:modified>
    <rdfs:isDefinedBy rdf:resource="http://rdfs.co/juso/"/>
    <rdfs:seeAlso rdf:resource="https://en.wikipedia.org/wiki/Province"/>
    <rdfs:subClassOf rdf:resource="http://rdfs.co/juso/AdministrativeDivision"/>
    <rdfs:subClassOf rdf:resource="http://schema.org/State"/>
    <owl:sameAs rdf:resource="http://dbpedia.org/ontology/Province"/>
    <status:term_status xml:lang="en">unstable</status:term_status>
    <skos:definition xml:lang="en">
    A province is almost always an administrative division, within a country or
    state.
    </skos:definition>
    <skos:prefLabel xml:lang="en">Province</skos:prefLabel>
    <skos:prefLabel xml:lang="ko">도</skos:prefLabel>
  </owl:Class>
  <owl:Class rdf:about="http://rdfs.co/juso/SecondLevelAdministrativeDivision">
    <dcterms:issued rdf:datatype="http://www.w3.org/2001/XMLSchema#date">2015-10-02+09:00</dcterms:issued>
    <dcterms:modified rdf:datatype="http://www.w3.org/2001/XMLSchema#date">2015-10-02+09:00</dcterms:modified>
    <rdfs:isDefinedBy rdf:resource="http://rdfs.co/juso/"/>
    <rdfs:seeAlso rdf:resource="http://www.geonames.org/ontology#A.ADM2"/>
    <rdfs:subClassOf rdf:resource="http://rdfs.co/juso/AdministrativeDivision"/>
    <status:term_status xml:lang="en">unstable</status:term_status>
    <skos:altLabel xml:lang="en">Second Administrative Level</skos:altLabel>
    <skos:altLabel xml:lang="en">Second-order Administrative Division</skos:altLabel>
    <skos:definition xml:lang="en">
    A subdivision of a first-level administrative division.
    </skos:definition>
    <skos:prefLabel xml:lang="en">Second-level Administrative Division</skos:prefLabel>
  </owl:Class>
  <owl:Class rdf:about="http://rdfs.co/juso/SpatialThing">
    <dcterms:issued rdf:datatype="http://www.w3.org/2001/XMLSchema#date">2015-10-02+09:00</dcterms:issued>
    <dcterms:modified rdf:datatype="http://www.w3.org/2001/XMLSchema#date">2015-10-02+09:00</dcterms:modified>
    <rdfs:isDefinedBy rdf:resource="http://rdfs.co/juso/"/>
    <owl:sameAs rdf:resource="http://www.opengis.net/ont/geosparql#SpatialObject"/>
    <owl:sameAs rdf:resource="http://www.w3.org/2003/01/geo/wgs84_pos#SpatialThing"/>
    <status:term_status xml:lang="en">testing</status:term_status>
    <skos:altLabel xml:lang="en">Spatial Object</skos:altLabel>
    <skos:definition xml:lang="en">
    Anything that has a spatial representation, i.e. size, shape, or position.
    e.g. people, places, objects, as well as abstract areas like cubes.
    </skos:definition>
    <skos:prefLabel xml:lang="en">Spatial Thing</skos:prefLabel>
  </owl:Class>
  <owl:Class rdf:about="http://rdfs.co/juso/Street">
    <dcterms:issued rdf:datatype="http://www.w3.org/2001/XMLSchema#date">2015-10-02+09:00</dcterms:issued>
    <dcterms:modified rdf:datatype="http://www.w3.org/2001/XMLSchema#date">2015-10-02+09:00</dcterms:modified>
    <rdfs:isDefinedBy rdf:resource="http://rdfs.co/juso/"/>
    <rdfs:seeAlso rdf:resource="http://www.geonames.org/ontology#R.ST"/>
    <rdfs:seeAlso rdf:resource="https://en.wikipedia.org/wiki/Street"/>
    <rdfs:subClassOf rdf:resource="http://rdfs.co/juso/Thoroughfare"/>
    <status:term_status xml:lang="en">unstable</status:term_status>
    <skos:definition xml:lang="en">
    A street is a public thoroughfare (usually paved) in a built environment.
    Practically all public streets in Western countries and the majority
    elsewhere (though not in Japan) are given a street or road name or at least
    a number to identify them and any addresses located along the streets.
    Alleys in some places do not have names.
    </skos:definition>
    <skos:prefLabel xml:lang="en">Street</skos:prefLabel>
  </owl:Class>
  <owl:Class rdf:about="http://rdfs.co/juso/ThirdLevelAdministrativeDivision">
    <dcterms:issued rdf:datatype="http://www.w3.org/2001/XMLSchema#date">2015-10-02+09:00</dcterms:issued>
    <dcterms:modified rdf:datatype="http://www.w3.org/2001/XMLSchema#date">2015-10-02+09:00</dcterms:modified>
    <rdfs:isDefinedBy rdf:resource="http://rdfs.co/juso/"/>
    <rdfs:seeAlso rdf:resource="http://www.geonames.org/ontology#A.ADM3"/>
    <rdfs:subClassOf rdf:resource="http://rdfs.co/juso/AdministrativeDivision"/>
    <status:term_status xml:lang="en">unstable</status:term_status>
    <skos:altLabel xml:lang="en">Third Administrative Level</skos:altLabel>
    <skos:altLabel xml:lang="en">Third-order Administrative Division</skos:altLabel>
    <skos:definition xml:lang="en">
    A subdivision of a second-level administrative division.
    </skos:definition>
    <skos:prefLabel xml:lang="en">Third-level Administrative Division</skos:prefLabel>
  </owl:Class>
  <owl:Class rdf:about="http://rdfs.co/juso/Thoroughfare">
    <dcterms:issued rdf:datatype="http://www.w3.org/2001/XMLSchema#date">2015-10-02+09:00</dcterms:issued>
    <dcterms:modified rdf:datatype="http://www.w3.org/2001/XMLSchema#date">2015-10-02+09:00</dcterms:modified>
    <rdfs:isDefinedBy rdf:resource="http://rdfs.co/juso/"/>
    <rdfs:seeAlso rdf:resource="https://en.wikipedia.org/wiki/Thoroughfare"/>
    <rdfs:subClassOf rdf:resource="http://rdfs.co/juso/Feature"/>
    <status:term_status xml:lang="en">unstable</status:term_status>
    <skos:definition xml:lang="en">
    A passage or way through from one location to another, which is usually
    used a component of an address. A thoroughfare is not necessarily a road,
    it might be a waterway or some other feature.
    </skos:definition>
    <skos:prefLabel xml:lang="en">Thoroughfare</skos:prefLabel>
  </owl:Class>
  <owl:Class rdf:about="http://rdfs.co/juso/Town">
    <dcterms:issued rdf:datatype="http://www.w3.org/2001/XMLSchema#date">2015-10-02+09:00</dcterms:issued>
    <dcterms:modified rdf:datatype="http://www.w3.org/2001/XMLSchema#date">2015-10-02+09:00</dcterms:modified>
    <rdfs:isDefinedBy rdf:resource="http://rdfs.co/juso/"/>
    <rdfs:seeAlso rdf:resource="https://en.wikipedia.org/wiki/Town"/>
    <rdfs:subClassOf rdf:resource="http://rdfs.co/juso/AdministrativeDivision"/>
    <owl:sameAs rdf:resource="http://dbpedia.org/ontology/Town"/>
    <owl:sameAs rdf:resource="http://linkedgeodata.org/ontology/Town"/>
    <status:term_status xml:lang="en">unstable</status:term_status>
    <skos:definition xml:lang="en">
    A town is a human settlement larger than a village but smaller than a city.
    The size definition for what constitutes a "town" varies considerably in
    different parts of the world.
    </skos:definition>
    <skos:prefLabel xml:lang="en">Town</skos:prefLabel>
    <skos:prefLabel xml:lang="ko">읍</skos:prefLabel>
  </owl:Class>
  <owl:Class rdf:about="http://rdfs.co/juso/Township">
    <dcterms:issued rdf:datatype="http://www.w3.org/2001/XMLSchema#date">2015-10-02+09:00</dcterms:issued>
    <dcterms:modified rdf:datatype="http://www.w3.org/2001/XMLSchema#date">2015-10-02+09:00</dcterms:modified>
    <rdfs:isDefinedBy rdf:resource="http://rdfs.co/juso/"/>
    <rdfs:seeAlso rdf:resource="https://en.wikipedia.org/wiki/Township"/>
    <rdfs:subClassOf rdf:resource="http://rdfs.co/juso/AdministrativeDivision"/>
    <status:term_status xml:lang="en">unstable</status:term_status>
    <skos:definition xml:lang="en">
    The word township is used to refer to different kinds of settlements in
    different countries.
    </skos:definition>
    <skos:prefLabel xml:lang="en">Township</skos:prefLabel>
    <skos:prefLabel xml:lang="ko">면</skos:prefLabel>
  </owl:Class>
  <owl:Class rdf:about="http://rdfs.co/juso/Village">
    <dcterms:issued rdf:datatype="http://www.w3.org/2001/XMLSchema#date">2015-10-02+09:00</dcterms:issued>
    <dcterms:modified rdf:datatype="http://www.w3.org/2001/XMLSchema#date">2015-10-02+09:00</dcterms:modified>
    <rdfs:isDefinedBy rdf:resource="http://rdfs.co/juso/"/>
    <rdfs:seeAlso rdf:resource="https://en.wikipedia.org/wiki/Village"/>
    <rdfs:subClassOf rdf:resource="http://rdfs.co/juso/AdministrativeDivision"/>
    <owl:sameAs rdf:resource="http://dbpedia.org/ontology/Village"/>
    <owl:sameAs rdf:resource="http://linkedgeodata.org/ontology/Village"/>
    <status:term_status xml:lang="en">unstable</status:term_status>
    <skos:definition xml:lang="en">
    A village is a clustered human settlement or community, larger than a
    hamlet but smaller than a town, with a population ranging from a few
    hundred to a few thousand.
    </skos:definition>
    <skos:prefLabel xml:lang="en">Village</skos:prefLabel>
    <skos:prefLabel xml:lang="ko">리</skos:prefLabel>
  </owl:Class>
  <owl:ObjectProperty rdf:about="http://rdfs.co/juso/address">
    <dcterms:issued rdf:datatype="http://www.w3.org/2001/XMLSchema#date">2015-10-02+09:00</dcterms:issued>
    <dcterms:modified rdf:datatype="http://www.w3.org/2001/XMLSchema#date">2015-10-02+09:00</dcterms:modified>
    <rdfs:domain rdf:resource="http://rdfs.co/juso/SpatialThing"/>
    <rdfs:isDefinedBy rdf:resource="http://rdfs.co/juso/"/>
    <rdfs:range rdf:resource="http://rdfs.co/juso/Address"/>
    <rdfs:subPropertyOf rdf:resource="http://ontology.eil.utoronto.ca/icontact.owl#address"/>
    <rdfs:subPropertyOf rdf:resource="http://www.w3.org/ns/locn#address"/>
    <status:term_status xml:lang="en">unstable</status:term_status>
    <skos:definition xml:lang="en">
    This property associates anything with its address.
    </skos:definition>
    <skos:prefLabel xml:lang="en">address</skos:prefLabel>
  </owl:ObjectProperty>
  <owl:DatatypeProperty rdf:about="http://rdfs.co/juso/alternate_name">
    <dcterms:issued rdf:datatype="http://www.w3.org/2001/XMLSchema#date">2015-12-30+09:00</dcterms:issued>
    <dcterms:modified rdf:datatype="http://www.w3.org/2001/XMLSchema#date">2015-12-30+09:00</dcterms:modified>
    <rdfs:domain rdf:resource="http://rdfs.co/juso/SpatialThing"/>
    <rdfs:isDefinedBy rdf:resource="http://rdfs.co/juso/"/>
    <rdfs:range rdf:resource="http://www.w3.org/2001/XMLSchema#string"/>
    <rdfs:seeAlso rdf:resource="http://www.geonames.org/ontology#alternateName"/>
    <rdfs:subPropertyOf rdf:resource="http://rdfs.co/juso/name"/>
    <owl:propertyDisjointWith rdf:resource="http://rdfs.co/juso/official_name"/>
    <status:term_status xml:lang="en">unstable</status:term_status>
    <skos:definition xml:lang="en">
    This property indicates the alternate name of the spatial thing.
    </skos:definition>
    <skos:prefLabel xml:lang="en">alternate name</skos:prefLabel>
    <skos:prefLabel xml:lang="ko">대체 이름</skos:prefLabel>
  </owl:DatatypeProperty>
  <owl:ObjectProperty rdf:about="http://rdfs.co/juso/country">
    <dcterms:issued rdf:datatype="http://www.w3.org/2001/XMLSchema#date">2015-10-02+09:00</dcterms:issued>
    <dcterms:modified rdf:datatype="http://www.w3.org/2001/XMLSchema#date">2015-10-02+09:00</dcterms:modified>
    <rdfs:domain rdf:resource="http://rdfs.co/juso/Address"/>
    <rdfs:isDefinedBy rdf:resource="http://rdfs.co/juso/"/>
    <rdfs:range rdf:resource="http://rdfs.co/juso/Country"/>
    <owl:sameAs rdf:resource="http://ontology.eil.utoronto.ca/icontact.owl#hasCountry"/>
    <status:term_status xml:lang="en">unstable</status:term_status>
    <skos:definition xml:lang="en">
    The uppermost politial division for the address, almost always a country.
    </skos:definition>
    <skos:prefLabel xml:lang="en">country</skos:prefLabel>
  </owl:ObjectProperty>
  <owl:DatatypeProperty rdf:about="http://rdfs.co/juso/endonym">
    <dcterms:issued rdf:datatype="http://www.w3.org/2001/XMLSchema#date">2015-10-02+09:00</dcterms:issued>
    <dcterms:modified rdf:datatype="http://www.w3.org/2001/XMLSchema#date">2015-10-02+09:00</dcterms:modified>
    <rdfs:domain rdf:resource="http://rdfs.co/juso/Feature"/>
    <rdfs:isDefinedBy rdf:resource="http://rdfs.co/juso/"/>
    <rdfs:range rdf:resource="http://www.w3.org/2001/XMLSchema#string"/>
    <rdfs:seeAlso rdf:resource="https://en.wikipedia.org/wiki/Exonym_and_endonym"/>
    <rdfs:subPropertyOf rdf:resource="http://rdfs.co/juso/name"/>
    <rdfs:subPropertyOf rdf:resource="http://www.geonames.org/ontology#officialName"/>
    <rdfs:subPropertyOf rdf:resource="http://www.w3.org/2004/02/skos/core#prefLabel"/>
    <status:term_status xml:lang="en">unstable</status:term_status>
    <skos:definition xml:lang="en">
    The endonym is a name given by members of a particular ethnolinguistic
    group to its homeland or a specific place within it.
    </skos:definition>
    <skos:prefLabel xml:lang="en">endonym</skos:prefLabel>
  </owl:DatatypeProperty>
  <owl:DatatypeProperty rdf:about="http://rdfs.co/juso/exonym">
    <dcterms:issued rdf:datatype="http://www.w3.org/2001/XMLSchema#date">2015-10-02+09:00</dcterms:issued>
    <dcterms:modified rdf:datatype="http://www.w3.org/2001/XMLSchema#date">2015-10-02+09:00</dcterms:modified>
    <rdfs:domain rdf:resource="http://rdfs.co/juso/Feature"/>
    <rdfs:isDefinedBy rdf:resource="http://rdfs.co/juso/"/>
    <rdfs:range rdf:resource="http://www.w3.org/2001/XMLSchema#string"/>
    <rdfs:seeAlso rdf:resource="https://en.wikipedia.org/wiki/Exonym_and_endonym"/>
    <rdfs:subPropertyOf rdf:resource="http://rdfs.co/juso/name"/>
    <rdfs:subPropertyOf rdf:resource="http://www.geonames.org/ontology#alternateName"/>
    <rdfs:subPropertyOf rdf:resource="http://www.w3.org/2004/02/skos/core#altLabel"/>
    <status:term_status xml:lang="en">unstable</status:term_status>
    <skos:definition xml:lang="en">
    The exonym is an external name for a geographical place: a common name used
    only outside the place in question, usually for historical reasons.
    </skos:definition>
    <skos:prefLabel xml:lang="en">exonym</skos:prefLabel>
  </owl:DatatypeProperty>
  <owl:ObjectProperty rdf:about="http://rdfs.co/juso/fifth_level_administrative_division">
    <dcterms:issued rdf:datatype="http://www.w3.org/2001/XMLSchema#date">2015-10-02+09:00</dcterms:issued>
    <dcterms:modified rdf:datatype="http://www.w3.org/2001/XMLSchema#date">2015-10-02+09:00</dcterms:modified>
    <rdfs:domain rdf:resource="http://rdfs.co/juso/Address"/>
    <rdfs:isDefinedBy rdf:resource="http://rdfs.co/juso/"/>
    <rdfs:range rdf:resource="http://rdfs.co/juso/FifthLevelAdministrativeDivision"/>
    <status:term_status xml:lang="en">unstable</status:term_status>
    <skos:definition xml:lang="en">
    The fifth-level administrative division of the address, if any.
    </skos:definition>
    <skos:prefLabel xml:lang="en">fifth-level administrative division</skos:prefLabel>
  </owl:ObjectProperty>
  <owl:ObjectProperty rdf:about="http://rdfs.co/juso/first_level_administrative_division">
    <dcterms:issued rdf:datatype="http://www.w3.org/2001/XMLSchema#date">2015-10-02+09:00</dcterms:issued>
    <dcterms:modified rdf:datatype="http://www.w3.org/2001/XMLSchema#date">2015-10-02+09:00</dcterms:modified>
    <rdfs:domain rdf:resource="http://rdfs.co/juso/Address"/>
    <rdfs:isDefinedBy rdf:resource="http://rdfs.co/juso/"/>
    <rdfs:range rdf:resource="http://rdfs.co/juso/FirstLevelAdministrativeDivision"/>
    <status:term_status xml:lang="en">unstable</status:term_status>
    <skos:definition xml:lang="en">
    The first-level administrative division (region) of the address, usually a
    county, state or other such area that typically encompasses several
    localities.
    </skos:definition>
    <skos:prefLabel xml:lang="en">first-level administrative division</skos:prefLabel>
  </owl:ObjectProperty>
  <owl:ObjectProperty rdf:about="http://rdfs.co/juso/fourth_level_administrative_division">
    <dcterms:issued rdf:datatype="http://www.w3.org/2001/XMLSchema#date">2015-10-02+09:00</dcterms:issued>
    <dcterms:modified rdf:datatype="http://www.w3.org/2001/XMLSchema#date">2015-10-02+09:00</dcterms:modified>
    <rdfs:domain rdf:resource="http://rdfs.co/juso/Address"/>
    <rdfs:isDefinedBy rdf:resource="http://rdfs.co/juso/"/>
    <rdfs:range rdf:resource="http://rdfs.co/juso/FourthLevelAdministrativeDivision"/>
    <status:term_status xml:lang="en">unstable</status:term_status>
    <skos:definition xml:lang="en">
    The fourth-level administrative division of the address, if any.
    </skos:definition>
    <skos:prefLabel xml:lang="en">fourth-level administrative division</skos:prefLabel>
  </owl:ObjectProperty>
  <owl:DatatypeProperty rdf:about="http://rdfs.co/juso/full_address">
    <dcterms:issued rdf:datatype="http://www.w3.org/2001/XMLSchema#date">2015-10-02+09:00</dcterms:issued>
    <dcterms:modified rdf:datatype="http://www.w3.org/2001/XMLSchema#date">2015-10-02+09:00</dcterms:modified>
    <rdfs:domain rdf:resource="http://rdfs.co/juso/Address"/>
    <rdfs:isDefinedBy rdf:resource="http://rdfs.co/juso/"/>
    <rdfs:range rdf:resource="http://www.w3.org/2001/XMLSchema#string"/>
    <owl:sameAs rdf:resource="http://www.w3.org/ns/locn#fullAddress"/>
    <status:term_status xml:lang="en">testing</status:term_status>
    <skos:definition xml:lang="en">
    The complete address written as a string, with or without formatting.
    </skos:definition>
    <skos:prefLabel xml:lang="en">full address</skos:prefLabel>
  </owl:DatatypeProperty>
  <owl:ObjectProperty rdf:about="http://rdfs.co/juso/geometry">
    <dcterms:issued rdf:datatype="http://www.w3.org/2001/XMLSchema#date">2015-10-02+09:00</dcterms:issued>
    <dcterms:modified rdf:datatype="http://www.w3.org/2001/XMLSchema#date">2015-10-02+09:00</dcterms:modified>
    <rdfs:domain rdf:resource="http://rdfs.co/juso/Feature"/>
    <rdfs:isDefinedBy rdf:resource="http://rdfs.co/juso/"/>
    <rdfs:range rdf:resource="http://rdfs.co/juso/Geometry"/>
    <rdfs:subPropertyOf rdf:resource="http://geovocab.org/geometry#geometry"/>
    <rdfs:subPropertyOf rdf:resource="http://www.w3.org/ns/locn#geometry"/>
    <status:term_status xml:lang="en">unstable</status:term_status>
    <skos:definition xml:lang="en">
    This property associates any feature with the corresponding geometry.
    </skos:definition>
    <skos:prefLabel xml:lang="en">geometry</skos:prefLabel>
  </owl:ObjectProperty>
  <owl:ObjectProperty rdf:about="http://rdfs.co/juso/historical_address">
    <dcterms:issued rdf:datatype="http://www.w3.org/2001/XMLSchema#date">2015-10-02+09:00</dcterms:issued>
    <dcterms:modified rdf:datatype="http://www.w3.org/2001/XMLSchema#date">2015-10-02+09:00</dcterms:modified>
    <rdfs:domain rdf:resource="http://rdfs.co/juso/SpatialThing"/>
    <rdfs:isDefinedBy rdf:resource="http://rdfs.co/juso/"/>
    <rdfs:range rdf:resource="http://rdfs.co/juso/Address"/>
    <status:term_status xml:lang="en">unstable</status:term_status>
    <skos:definition xml:lang="en">
    This property associates anything with one of its historical address.
    </skos:definition>
    <skos:prefLabel xml:lang="en">historical address</skos:prefLabel>
  </owl:ObjectProperty>
  <owl:DatatypeProperty rdf:about="http://rdfs.co/juso/itrf2000_lat">
    <dcterms:issued rdf:datatype="http://www.w3.org/2001/XMLSchema#date">2015-11-10+09:00</dcterms:issued>
    <dcterms:modified rdf:datatype="http://www.w3.org/2001/XMLSchema#date">2015-11-10+09:00</dcterms:modified>
    <rdfs:domain rdf:resource="http://rdfs.co/juso/Point"/>
    <rdfs:isDefinedBy rdf:resource="http://rdfs.co/juso/"/>
    <rdfs:range rdf:resource="http://www.w3.org/2001/XMLSchema#string"/>
    <status:term_status xml:lang="en">unstable</status:term_status>
    <skos:definition xml:lang="en">
    The ITRF2000 latitude of a point (decimal degrees).
    </skos:definition>
    <skos:prefLabel xml:lang="en">latitude (ITRF2000)</skos:prefLabel>
    <skos:prefLabel xml:lang="ko">위도(ITRF2000)</skos:prefLabel>
  </owl:DatatypeProperty>
  <owl:DatatypeProperty rdf:about="http://rdfs.co/juso/itrf2000_long">
    <dcterms:issued rdf:datatype="http://www.w3.org/2001/XMLSchema#date">2015-11-10+09:00</dcterms:issued>
    <dcterms:modified rdf:datatype="http://www.w3.org/2001/XMLSchema#date">2015-11-10+09:00</dcterms:modified>
    <rdfs:domain rdf:resource="http://rdfs.co/juso/Point"/>
    <rdfs:isDefinedBy rdf:resource="http://rdfs.co/juso/"/>
    <rdfs:range rdf:resource="http://www.w3.org/2001/XMLSchema#string"/>
    <status:term_status xml:lang="en">unstable</status:term_status>
    <skos:definition xml:lang="en">
    The ITRF2000 longitude of a point (decimal degrees).
    </skos:definition>
    <skos:prefLabel xml:lang="en">longitude (ITRF2000)</skos:prefLabel>
    <skos:prefLabel xml:lang="ko">경도(ITRF2000)</skos:prefLabel>
  </owl:DatatypeProperty>
  <owl:ObjectProperty rdf:about="http://rdfs.co/juso/locator">
    <dcterms:issued rdf:datatype="http://www.w3.org/2001/XMLSchema#date">2015-10-02+09:00</dcterms:issued>
    <dcterms:modified rdf:datatype="http://www.w3.org/2001/XMLSchema#date">2015-10-02+09:00</dcterms:modified>
    <rdfs:domain rdf:resource="http://rdfs.co/juso/Address"/>
    <rdfs:isDefinedBy rdf:resource="http://rdfs.co/juso/"/>
    <rdfs:range rdf:resource="http://rdfs.co/juso/Feature"/>
    <status:term_status xml:lang="en">unstable</status:term_status>
    <skos:definition xml:lang="en">
    The real world entity identified by the address. The locator could be the
    property or complex, of the building or part of the building, of it could
    be a room inside a building.
    </skos:definition>
    <skos:prefLabel xml:lang="en">locator</skos:prefLabel>
  </owl:ObjectProperty>
  <owl:DatatypeProperty rdf:about="http://rdfs.co/juso/locator_address">
    <dcterms:issued rdf:datatype="http://www.w3.org/2001/XMLSchema#date">2015-10-02+09:00</dcterms:issued>
    <dcterms:modified rdf:datatype="http://www.w3.org/2001/XMLSchema#date">2015-10-02+09:00</dcterms:modified>
    <rdfs:domain rdf:resource="http://rdfs.co/juso/Address"/>
    <rdfs:isDefinedBy rdf:resource="http://rdfs.co/juso/"/>
    <rdfs:range rdf:resource="http://www.w3.org/2001/XMLSchema#string"/>
    <status:term_status xml:lang="en">unstable</status:term_status>
    <skos:definition xml:lang="en">
    This property is used to describe a number or a sequence of characters that
    uniquely identifies the exact locator within the relevant scope(s), that is
    described by juso:locator.
    </skos:definition>
    <skos:prefLabel xml:lang="en">locator address</skos:prefLabel>
  </owl:DatatypeProperty>
  <owl:DatatypeProperty rdf:about="http://rdfs.co/juso/name">
    <dcterms:issued rdf:datatype="http://www.w3.org/2001/XMLSchema#date">2015-10-02+09:00</dcterms:issued>
    <dcterms:modified rdf:datatype="http://www.w3.org/2001/XMLSchema#date">2015-10-02+09:00</dcterms:modified>
    <rdfs:domain rdf:resource="http://rdfs.co/juso/SpatialThing"/>
    <rdfs:isDefinedBy rdf:resource="http://rdfs.co/juso/"/>
    <rdfs:range rdf:resource="http://www.w3.org/2001/XMLSchema#string"/>
    <rdfs:subPropertyOf rdf:resource="http://purl.org/dc/terms/title"/>
    <rdfs:subPropertyOf rdf:resource="http://schema.org/name"/>
    <status:term_status xml:lang="en">testing</status:term_status>
    <skos:definition xml:lang="en">
    This property indicates the name of the spatial thing.
    </skos:definition>
    <skos:prefLabel xml:lang="en">name</skos:prefLabel>
    <skos:prefLabel xml:lang="ko">이름</skos:prefLabel>
  </owl:DatatypeProperty>
  <owl:DatatypeProperty rdf:about="http://rdfs.co/juso/official_name">
    <dcterms:issued rdf:datatype="http://www.w3.org/2001/XMLSchema#date">2015-12-30+09:00</dcterms:issued>
    <dcterms:modified rdf:datatype="http://www.w3.org/2001/XMLSchema#date">2015-12-30+09:00</dcterms:modified>
    <rdfs:domain rdf:resource="http://rdfs.co/juso/SpatialThing"/>
    <rdfs:isDefinedBy rdf:resource="http://rdfs.co/juso/"/>
    <rdfs:range rdf:resource="http://www.w3.org/2001/XMLSchema#string"/>
    <rdfs:seeAlso rdf:resource="http://www.geonames.org/ontology#officialName"/>
    <rdfs:subPropertyOf rdf:resource="http://rdfs.co/juso/name"/>
    <status:term_status xml:lang="en">unstable</status:term_status>
    <skos:definition xml:lang="en">
    This property indicates the official name of the spatial thing.
    </skos:definition>
    <skos:prefLabel xml:lang="en">official name</skos:prefLabel>
    <skos:prefLabel xml:lang="ko">공식 이름</skos:prefLabel>
  </owl:DatatypeProperty>
  <owl:ObjectProperty rdf:about="http://rdfs.co/juso/parent">
    <dcterms:issued rdf:datatype="http://www.w3.org/2001/XMLSchema#date">2015-10-02+09:00</dcterms:issued>
    <dcterms:modified rdf:datatype="http://www.w3.org/2001/XMLSchema#date">2015-10-02+09:00</dcterms:modified>
    <rdfs:domain rdf:resource="http://rdfs.co/juso/Feature"/>
    <rdfs:isDefinedBy rdf:resource="http://rdfs.co/juso/"/>
    <rdfs:range rdf:resource="http://rdfs.co/juso/PoliticalDivision"/>
    <rdfs:subPropertyOf rdf:resource="http://rdfs.co/juso/political_division"/>
    <rdfs:subPropertyOf rdf:resource="http://www.geonames.org/ontology#parentFeature"/>
    <status:term_status xml:lang="en">unstable</status:term_status>
    <skos:definition xml:lang="en">
    A politial or administrative division that is a direct parent of the
    current feature.
    </skos:definition>
    <skos:prefLabel xml:lang="en">parent politial division</skos:prefLabel>
  </owl:ObjectProperty>
  <owl:TransitiveProperty rdf:about="http://rdfs.co/juso/political_division">
    <dcterms:issued rdf:datatype="http://www.w3.org/2001/XMLSchema#date">2015-10-02+09:00</dcterms:issued>
    <dcterms:modified rdf:datatype="http://www.w3.org/2001/XMLSchema#date">2015-10-02+09:00</dcterms:modified>
    <rdfs:domain rdf:resource="http://rdfs.co/juso/Feature"/>
    <rdfs:isDefinedBy rdf:resource="http://rdfs.co/juso/"/>
    <rdfs:range rdf:resource="http://rdfs.co/juso/PoliticalDivision"/>
    <status:term_status xml:lang="en">unstable</status:term_status>
    <skos:definition xml:lang="en">
    A politial or administrative division that contain the current feature.
    </skos:definition>
    <skos:prefLabel xml:lang="en">political division</skos:prefLabel>
  </owl:TransitiveProperty>
  <owl:DatatypeProperty rdf:about="http://rdfs.co/juso/post_office_box">
    <dcterms:issued rdf:datatype="http://www.w3.org/2001/XMLSchema#date">2015-10-02+09:00</dcterms:issued>
    <dcterms:modified rdf:datatype="http://www.w3.org/2001/XMLSchema#date">2015-10-02+09:00</dcterms:modified>
    <rdfs:domain rdf:resource="http://rdfs.co/juso/Address"/>
    <rdfs:isDefinedBy rdf:resource="http://rdfs.co/juso/"/>
    <rdfs:range rdf:resource="http://www.w3.org/2001/XMLSchema#string"/>
    <owl:sameAs rdf:resource="http://schema.org/postOfficeBoxNumber"/>
    <owl:sameAs rdf:resource="http://www.w3.org/ns/locn#poBox"/>
    <status:term_status xml:lang="en">unstable</status:term_status>
    <skos:definition xml:lang="en">
    This property describes the post office box number for PO box addresses.
    A post-office box or post office box (commonly referred to as a PO box or a
    postal box) is a uniquely addressable lockable box located on the premises
    of a post office station.
    </skos:definition>
    <skos:prefLabel xml:lang="en">post office box</skos:prefLabel>
  </owl:DatatypeProperty>
  <owl:DatatypeProperty rdf:about="http://rdfs.co/juso/postal_code">
    <dcterms:issued rdf:datatype="http://www.w3.org/2001/XMLSchema#date">2015-10-02+09:00</dcterms:issued>
    <dcterms:modified rdf:datatype="http://www.w3.org/2001/XMLSchema#date">2015-10-02+09:00</dcterms:modified>
    <rdfs:domain rdf:resource="http://rdfs.co/juso/Address"/>
    <rdfs:isDefinedBy rdf:resource="http://rdfs.co/juso/"/>
    <rdfs:range rdf:resource="http://rdfs.co/juso/PostalCode"/>
    <status:term_status xml:lang="en">unstable</status:term_status>
    <skos:definition xml:lang="en">
    This property associates any address with its postal code.
    </skos:definition>
    <skos:prefLabel xml:lang="en">postal code</skos:prefLabel>
  </owl:DatatypeProperty>
  <owl:ObjectProperty rdf:about="http://rdfs.co/juso/second_level_administrative_division">
    <dcterms:issued rdf:datatype="http://www.w3.org/2001/XMLSchema#date">2015-10-02+09:00</dcterms:issued>
    <dcterms:modified rdf:datatype="http://www.w3.org/2001/XMLSchema#date">2015-10-02+09:00</dcterms:modified>
    <rdfs:domain rdf:resource="http://rdfs.co/juso/Address"/>
    <rdfs:isDefinedBy rdf:resource="http://rdfs.co/juso/"/>
    <rdfs:range rdf:resource="http://rdfs.co/juso/SecondLevelAdministrativeDivision"/>
    <status:term_status xml:lang="en">unstable</status:term_status>
    <skos:definition xml:lang="en">
    The second-level administrative division (locality) of the address, usually
    a city.
    </skos:definition>
    <skos:prefLabel xml:lang="en">second-level administrative division</skos:prefLabel>
  </owl:ObjectProperty>
  <owl:DatatypeProperty rdf:about="http://rdfs.co/juso/short_name">
    <dcterms:issued rdf:datatype="http://www.w3.org/2001/XMLSchema#date">2015-12-30+09:00</dcterms:issued>
    <dcterms:modified rdf:datatype="http://www.w3.org/2001/XMLSchema#date">2015-12-30+09:00</dcterms:modified>
    <rdfs:domain rdf:resource="http://rdfs.co/juso/SpatialThing"/>
    <rdfs:isDefinedBy rdf:resource="http://rdfs.co/juso/"/>
    <rdfs:range rdf:resource="http://www.w3.org/2001/XMLSchema#string"/>
    <rdfs:seeAlso rdf:resource="http://www.geonames.org/ontology#shortName"/>
    <rdfs:subPropertyOf rdf:resource="http://rdfs.co/juso/alternate_name"/>
    <status:term_status xml:lang="en">unstable</status:term_status>
    <skos:definition xml:lang="en">
    This property indicates the relatively short name of the spatial thing.
    </skos:definition>
    <skos:prefLabel xml:lang="en">short name</skos:prefLabel>
    <skos:prefLabel xml:lang="ko">짧은 이름</skos:prefLabel>
  </owl:DatatypeProperty>
  <owl:ObjectProperty rdf:about="http://rdfs.co/juso/third_level_administrative_division">
    <dcterms:issued rdf:datatype="http://www.w3.org/2001/XMLSchema#date">2015-10-02+09:00</dcterms:issued>
    <dcterms:modified rdf:datatype="http://www.w3.org/2001/XMLSchema#date">2015-10-02+09:00</dcterms:modified>
    <rdfs:domain rdf:resource="http://rdfs.co/juso/Address"/>
    <rdfs:isDefinedBy rdf:resource="http://rdfs.co/juso/"/>
    <rdfs:range rdf:resource="http://rdfs.co/juso/ThirdLevelAdministrativeDivision"/>
    <status:term_status xml:lang="en">unstable</status:term_status>
    <skos:definition xml:lang="en">
    The third-level administrative division of the address, if any.
    </skos:definition>
    <skos:prefLabel xml:lang="en">third-level administrative division</skos:prefLabel>
  </owl:ObjectProperty>
  <owl:ObjectProperty rdf:about="http://rdfs.co/juso/thoroughfare">
    <dcterms:issued rdf:datatype="http://www.w3.org/2001/XMLSchema#date">2015-10-02+09:00</dcterms:issued>
    <dcterms:modified rdf:datatype="http://www.w3.org/2001/XMLSchema#date">2015-10-02+09:00</dcterms:modified>
    <rdfs:domain rdf:resource="http://rdfs.co/juso/Address"/>
    <rdfs:isDefinedBy rdf:resource="http://rdfs.co/juso/"/>
    <rdfs:range rdf:resource="http://rdfs.co/juso/Thoroughfare"/>
    <status:term_status xml:lang="en">unstable</status:term_status>
    <skos:definition xml:lang="en">
    An address component that represents the name of a passage or way through
    from one location to another. A thoroughfare is not necessarily a road, it
    might be a waterway or some other feature.
    </skos:definition>
    <skos:prefLabel xml:lang="en">thoroughfare</skos:prefLabel>
  </owl:ObjectProperty>
  <owl:DatatypeProperty rdf:about="http://rdfs.co/juso/thoroughfare_address">
    <dcterms:issued rdf:datatype="http://www.w3.org/2001/XMLSchema#date">2015-10-02+09:00</dcterms:issued>
    <dcterms:modified rdf:datatype="http://www.w3.org/2001/XMLSchema#date">2015-10-02+09:00</dcterms:modified>
    <rdfs:domain rdf:resource="http://rdfs.co/juso/Address"/>
    <rdfs:isDefinedBy rdf:resource="http://rdfs.co/juso/"/>
    <rdfs:range rdf:resource="http://www.w3.org/2001/XMLSchema#string"/>
    <rdfs:seeAlso rdf:resource="https://en.wikipedia.org/wiki/House_numbering"/>
    <status:term_status xml:lang="en">unstable</status:term_status>
    <skos:definition xml:lang="en">
    This property is used to describe a unique number given to each building
    (residential or not) or vacant lot with a mailbox in a street or other
    thoroughfares.
    </skos:definition>
    <skos:prefLabel xml:lang="en">thoroughfare address</skos:prefLabel>
  </owl:DatatypeProperty>
  <owl:DatatypeProperty rdf:about="http://rdfs.co/juso/wgs84_lat">
    <dcterms:issued rdf:datatype="http://www.w3.org/2001/XMLSchema#date">2015-11-10+09:00</dcterms:issued>
    <dcterms:modified rdf:datatype="http://www.w3.org/2001/XMLSchema#date">2015-11-10+09:00</dcterms:modified>
    <rdfs:domain rdf:resource="http://rdfs.co/juso/Point"/>
    <rdfs:isDefinedBy rdf:resource="http://rdfs.co/juso/"/>
    <rdfs:range rdf:resource="http://www.w3.org/2001/XMLSchema#string"/>
    <owl:sameAs rdf:resource="http://www.w3.org/2003/01/geo/wgs84_pos#lat"/>
    <status:term_status xml:lang="en">unstable</status:term_status>
    <skos:definition xml:lang="en">
    The WGS84 latitude of a point (decimal degrees).
    </skos:definition>
    <skos:prefLabel xml:lang="en">latitude (WGS84)</skos:prefLabel>
    <skos:prefLabel xml:lang="ko">위도(WGS84)</skos:prefLabel>
  </owl:DatatypeProperty>
  <owl:DatatypeProperty rdf:about="http://rdfs.co/juso/wgs84_long">
    <dcterms:issued rdf:datatype="http://www.w3.org/2001/XMLSchema#date">2015-11-10+09:00</dcterms:issued>
    <dcterms:modified rdf:datatype="http://www.w3.org/2001/XMLSchema#date">2015-11-10+09:00</dcterms:modified>
    <rdfs:domain rdf:resource="http://rdfs.co/juso/Point"/>
    <rdfs:isDefinedBy rdf:resource="http://rdfs.co/juso/"/>
    <rdfs:range rdf:resource="http://www.w3.org/2001/XMLSchema#string"/>
    <owl:sameAs rdf:resource="http://www.w3.org/2003/01/geo/wgs84_pos#long"/>
    <status:term_status xml:lang="en">unstable</status:term_status>
    <skos:definition xml:lang="en">
    The WGS84 longitude of a point (decimal degrees).
    </skos:definition>
    <skos:prefLabel xml:lang="en">longitude (WGS84)</skos:prefLabel>
    <skos:prefLabel xml:lang="ko">경도(WGS84)</skos:prefLabel>
  </owl:DatatypeProperty>
  <owl:TransitiveProperty rdf:about="http://rdfs.co/juso/within">
    <dcterms:issued rdf:datatype="http://www.w3.org/2001/XMLSchema#date">2015-10-02+09:00</dcterms:issued>
    <dcterms:modified rdf:datatype="http://www.w3.org/2001/XMLSchema#date">2015-10-02+09:00</dcterms:modified>
    <rdfs:domain rdf:resource="http://rdfs.co/juso/SpatialThing"/>
    <rdfs:isDefinedBy rdf:resource="http://rdfs.co/juso/"/>
    <rdfs:range rdf:resource="http://rdfs.co/juso/SpatialThing"/>
    <rdfs:subPropertyOf rdf:resource="http://www.w3.org/2003/01/geo/wgs84_pos#location"/>
    <rdfs:subPropertyOf rdf:resource="http://www.w3.org/ns/locn#location"/>
    <owl:inverseOf rdf:resource="http://geovocab.org/spatial#Pi"/>
    <owl:inverseOf rdf:resource="http://www.opengis.net/ont/geosparql#sfContains"/>
    <owl:sameAs rdf:resource="http://geovocab.org/spatial#P"/>
    <owl:sameAs rdf:resource="http://www.opengis.net/ont/geosparql#sfWithin"/>
    <status:term_status xml:lang="en">testing</status:term_status>
    <skos:definition xml:lang="en">
    A spatial thing that contains the current one within the borders of its own
    region.
    </skos:definition>
    <skos:prefLabel xml:lang="en">within</skos:prefLabel>
  </owl:TransitiveProperty>
  <rdf:Description rdf:about="http://schema.org/GeoCoordinates">
    <rdfs:subClassOf rdf:resource="http://rdfs.co/juso/Geometry"/>
  </rdf:Description>
  <rdf:Description rdf:about="http://schema.org/GeoShape">
    <rdfs:subClassOf rdf:resource="http://rdfs.co/juso/Geometry"/>
  </rdf:Description>
  <rdf:Description rdf:about="http://schema.org/Place">
    <rdfs:subClassOf rdf:resource="http://rdfs.co/juso/SpatialThing"/>
  </rdf:Description>
  <rdf:Description rdf:about="http://schema.org/PostalAddress">
    <rdfs:subClassOf rdf:resource="http://rdfs.co/juso/Address"/>
  </rdf:Description>
  <rdf:Description rdf:about="http://schema.org/address">
    <rdfs:subPropertyOf rdf:resource="http://rdfs.co/juso/address"/>
  </rdf:Description>
  <rdf:Description rdf:about="http://schema.org/containedIn">
    <rdfs:subPropertyOf rdf:resource="http://rdfs.co/juso/within"/>
  </rdf:Description>
  <rdf:Description rdf:about="http://schema.org/geo">
    <rdfs:subPropertyOf rdf:resource="http://rdfs.co/juso/geometry"/>
  </rdf:Description>
  <rdf:Description rdf:about="http://schema.org/postalCode">
    <owl:propertyChainAxiom>
      <rdf:Description>
        <rdf:first rdf:resource="http://rdfs.co/juso/postal_code"/>
        <rdf:rest>
          <rdf:Description>
            <rdf:first rdf:resource="http://www.w3.org/1999/02/22-rdf-syntax-ns#value"/>
            <rdf:rest rdf:resource="http://www.w3.org/1999/02/22-rdf-syntax-ns#nil"/>
          </rdf:Description>
        </rdf:rest>
      </rdf:Description>
    </owl:propertyChainAxiom>
  </rdf:Description>
  <rdf:Description rdf:about="http://www.geonames.org/ontology#alternateName">
    <rdfs:subPropertyOf rdf:resource="http://rdfs.co/juso/alternate_name"/>
  </rdf:Description>
  <rdf:Description rdf:about="http://www.geonames.org/ontology#name">
    <rdfs:subPropertyOf rdf:resource="http://rdfs.co/juso/name"/>
  </rdf:Description>
  <rdf:Description rdf:about="http://www.geonames.org/ontology#officialName">
    <rdfs:subPropertyOf rdf:resource="http://rdfs.co/juso/official_name"/>
  </rdf:Description>
  <rdf:Description rdf:about="http://www.geonames.org/ontology#shortName">
    <rdfs:subPropertyOf rdf:resource="http://rdfs.co/juso/short_name"/>
  </rdf:Description>
  <rdf:Description rdf:about="http://www.opengis.net/ont/geosparql#hasGeometry">
    <rdfs:subPropertyOf rdf:resource="http://rdfs.co/juso/geometry"/>
  </rdf:Description>
  <rdf:Description rdf:about="http://www.w3.org/2006/vcard/ns#Address">
    <rdfs:subClassOf rdf:resource="http://rdfs.co/juso/Address"/>
  </rdf:Description>
  <rdf:Description rdf:about="http://www.w3.org/2006/vcard/ns#postal-code">
    <owl:propertyChainAxiom>
      <rdf:Description>
        <rdf:first rdf:resource="http://rdfs.co/juso/postal_code"/>
        <rdf:rest>
          <rdf:Description>
            <rdf:first rdf:resource="http://www.w3.org/1999/02/22-rdf-syntax-ns#value"/>
            <rdf:rest rdf:resource="http://www.w3.org/1999/02/22-rdf-syntax-ns#nil"/>
          </rdf:Description>
        </rdf:rest>
      </rdf:Description>
    </owl:propertyChainAxiom>
  </rdf:Description>
  <rdf:Description rdf:about="http://www.w3.org/ns/locn#postCode">
    <owl:propertyChainAxiom>
      <rdf:Description>
        <rdf:first rdf:resource="http://rdfs.co/juso/postal_code"/>
        <rdf:rest>
          <rdf:Description>
            <rdf:first rdf:resource="http://www.w3.org/1999/02/22-rdf-syntax-ns#value"/>
            <rdf:rest rdf:resource="http://www.w3.org/1999/02/22-rdf-syntax-ns#nil"/>
          </rdf:Description>
        </rdf:rest>
      </rdf:Description>
    </owl:propertyChainAxiom>
  </rdf:Description>
</rdf:RDF>
