<?xml version="1.0" encoding="utf-8"?>
<rdf:RDF xmlns:adms="http://www.w3.org/ns/adms#"
   xmlns:cc="http://creativecommons.org/ns#"
   xmlns:dcam="http://purl.org/dc/dcam/"
   xmlns:dcterms="http://purl.org/dc/terms/"
   xmlns:foaf="http://xmlns.com/foaf/0.1/"
   xmlns:gn="http://www.geonames.org/ontology#"
   xmlns:juso.kr="http://rdfs.co/juso/kr/"
   xmlns:juso="http://rdfs.co/juso/"
   xmlns:org="http://www.w3.org/ns/org#"
   xmlns:owl="http://www.w3.org/2002/07/owl#"
   xmlns:rdf="http://www.w3.org/1999/02/22-rdf-syntax-ns#"
   xmlns:rdfs="http://www.w3.org/2000/01/rdf-schema#"
   xmlns:skos="http://www.w3.org/2004/02/skos/core#"
   xmlns:status="http://www.w3.org/2003/06/sw-vocab-status/ns#"
   xmlns:vann="http://purl.org/vocab/vann/"
   xmlns:voaf="http://purl.org/vocommons/voaf#"
   xmlns:xsd="http://www.w3.org/2001/XMLSchema#">
  <foaf:Person rdf:about="http://jayg.me/">
    <owl:sameAs rdf:resource="http://listinc.kr/id/member/jgkim"/>
    <org:memberOf rdf:resource="http://listinc.kr/id/listinc"/>
    <foaf:homepage rdf:resource="http://jayg.org/"/>
    <foaf:mbox_sha1sum>f03421e94730da58e8943d3a1d2c4c6b02898e14</foaf:mbox_sha1sum>
    <foaf:name xml:lang="en">James G. Kim</foaf:name>
    <foaf:name xml:lang="ko">김보람</foaf:name>
  </foaf:Person>
  <foaf:Organization rdf:about="http://listinc.kr/id/listinc">
    <rdf:type rdf:resource="http://www.w3.org/ns/org#Organization"/>
    <foaf:homepage rdf:resource="http://li-st.com/"/>
    <foaf:homepage rdf:resource="http://listinc.kr/"/>
    <foaf:mbox_sha1sum>de068365487dd2da1f2e88f1eaad0217bff79b40</foaf:mbox_sha1sum>
    <foaf:member rdf:resource="http://listinc.kr/id/member/jgkim"/>
    <foaf:name xml:lang="en">LiST Inc.</foaf:name>
    <foaf:name xml:lang="ko">주식회사 리스트</foaf:name>
  </foaf:Organization>
  <owl:Ontology rdf:about="http://rdfs.co/juso/kr/0.1.1">
    <cc:license rdf:resource="http://creativecommons.org/licenses/by/4.0/"/>
    <dcterms:creator rdf:resource="http://jayg.me/"/>
    <dcterms:description xml:lang="en">
    South Korea Extension to Juso Ontology is a Web vocabulary that extends
    &lt;a href="http://rdfs.co/juso/"&gt;Juso Ontology&lt;/a&gt; to descrbe geographical
    addresses and features in South Korea.
    </dcterms:description>
    <dcterms:hasFormat rdf:resource="http://rdfs.co/juso/kr/0.1.1/html"/>
    <dcterms:hasFormat rdf:resource="http://rdfs.co/juso/kr/0.1.1/rdf"/>
    <dcterms:hasFormat rdf:resource="http://rdfs.co/juso/kr/0.1.1/ttl"/>
    <dcterms:identifier>http://rdfs.co/juso/kr/0.1.1</dcterms:identifier>
    <dcterms:isVersionOf rdf:resource="http://rdfs.co/juso/kr/"/>
    <dcterms:issued rdf:datatype="http://www.w3.org/2001/XMLSchema#date">2015-10-02+09:00</dcterms:issued>
    <dcterms:modified rdf:datatype="http://www.w3.org/2001/XMLSchema#date">2015-11-10+09:00</dcterms:modified>
    <dcterms:publisher rdf:resource="http://listinc.kr/id/listinc"/>
    <dcterms:replaces rdf:resource="http://rdfs.co/juso/kr/0.1"/>
    <dcterms:rights>Copyright © 2015 LiST Inc. Some Rights Reserved.</dcterms:rights>
    <dcterms:title xml:lang="en">South Korea Extension to Juso Ontology</dcterms:title>
    <dcterms:title xml:lang="ko">대한민국 주소 온톨로지</dcterms:title>
    <dcterms:type rdf:resource="http://purl.org/adms/assettype/Ontology"/>
    <vann:example>
      <rdf:Description>
        <rdfs:comment rdf:datatype="http://www.w3.org/1999/02/22-rdf-syntax-ns#HTML">
    &lt;pre&gt;&lt;code&gt;_:YangyongBldg a juso.kr:Building ;
  juso:name "Yangyong Building"@en , "양용빌딩"@ko ;
  juso:geometry &amp;lt;http://geohash.org/wydjrzg6ece9&amp;gt; ;
  juso.kr:administrative_building_number "1156011700101210017028596" .

_:LiSTInc a juso:SpatialThing , foaf:Organization ;
  juso:name "LiST Inc."@en , "주식회사 리스트"@ko ;
  juso:within _:YangyongBldg ;
  juso:historical_address [
    a juso.kr:EastAsianAddress ;
    juso:full_address
      "대한민국 서울특별시 영등포구 당산동 121-17 양용빌딩 9층 150-040"@ko ,
      "9th Floor, Yangyong Building, 121-17, Dangsan-dong, Yeongdeungpo-gu, Seoul, 150-040, South Korea"@en ;
    juso:country &amp;lt;http://sws.geonames.org/1835841/&amp;gt; ;
    juso.kr:si_do &amp;lt;http://sws.geonames.org/1835847/&amp;gt; ;
    juso.kr:si_gun_gu &amp;lt;http://sws.geonames.org/1832536/&amp;gt; ;
    juso.kr:eup_myeon_dong &amp;lt;http://sws.geonames.org/8692617/&amp;gt; ;
    juso.kr:beonji "121" ;
    juso.kr:ho "17" ;
    juso:locator _:YangyongBldg ;
    juso:locator_address "9층"@ko , "9th Floor"@en ;
    juso:postal_code [
      a juso.kr:PostalCode1988 ;
      rdf:value "150-040"
    ]
  ] ;
  juso:address [
    a juso.kr:RoadNameAddress ;
    juso:full_address
      "대한민국 서울특별시 영등포구 버드나루로19길 3 (당산동) 양용빌딩 9층 07229"@ko ,
      "9th Floor, Yangyong Building, 3, Beodeunaru-ro 19-gil, Yeongdeungpo-gu, Seoul, 07229, South Korea"@en ;
    juso:country &amp;lt;http://sws.geonames.org/1835841/&amp;gt; ;
    juso.kr:si_do &amp;lt;http://sws.geonames.org/1835847/&amp;gt; ;
    juso.kr:si_gun_gu &amp;lt;http://sws.geonames.org/1832536/&amp;gt; ;
    juso.kr:eup_myeon_dong &amp;lt;http://sws.geonames.org/8692617/&amp;gt; ;
    juso:thoroughfare [
      a juso.kr:Road ;
      juso:name "Beodeunaru-ro 19-gil"@en , "버드나루로19길"@ko ;
      juso:parent &amp;lt;http://sws.geonames.org/8692617/&amp;gt;
      juso.kr:road_name_number "4154419" ;
      juso.kr:parent_road [
        a juso.kr:Street ;
        juso:name "Beodeunaru-ro"@en , "버드나루로"@ko ;
        juso:parent &amp;lt;http://sws.geonames.org/8692617/&amp;gt;
        juso.kr:road_name_number "3118010" ;
      ]
    ] ;
    juso.kr:building_number "3" ;
    juso:locator _:YangyongBldg ;
    juso:locator_address "9층"@ko , "9th Floor"@en ;
    juso:postal_code [
      a juso.kr:PostalCode2015 ;
      rdf:value "07229"
    ] ;
    juso.kr:landform &amp;lt;http://dbpedia.org/resource/Land_lot&amp;gt; ;
    juso.kr:floor &amp;lt;http://dbpedia.org/resource/Storey&amp;gt; ;
    juso.kr:eup_myeon_dong_serial_number "1"
  ] .

&amp;lt;http://sws.geonames.org/1832536/&amp;gt; a juso.kr:AutonomousDistrict ;
  juso.kr:si_gun_gu_code "11560" .

&amp;lt;http://sws.geonames.org/8692617/&amp;gt; a juso.kr:LegalStatusNeighborhood ;
  juso.kr:legal_status_neighborhood_code "1156011700" ;
  juso.kr:eup_myeon_dong_code "117" .&lt;/code&gt;&lt;/pre&gt;
    </rdfs:comment>
        <rdfs:label xml:lang="ko">LiST Inc.</rdfs:label>
      </rdf:Description>
    </vann:example>
    <vann:preferredNamespacePrefix>juso.kr</vann:preferredNamespacePrefix>
    <vann:preferredNamespaceUri>http://rdfs.co/juso/kr/</vann:preferredNamespaceUri>
    <vann:termGroup rdf:resource="http://rdfs.co/juso/kr/AddressGroup"/>
    <vann:termGroup rdf:resource="http://rdfs.co/juso/kr/AdministrativeDivisionGroup"/>
    <rdf:type rdf:resource="http://creativecommons.org/ns#Work"/>
    <rdf:type rdf:resource="http://purl.org/vocommons/voaf#Vocabulary"/>
    <rdf:type rdf:resource="http://www.w3.org/ns/adms#SemanticAsset"/>
    <rdfs:comment rdf:datatype="http://www.w3.org/1999/02/22-rdf-syntax-ns#HTML">
    &lt;div&gt;
      The master version of this vocabulary is maintained in &lt;a
      href="https://github.com/listinc/juso-ontology/tree/master/kr"&gt;the GitHub
      repository&lt;/a&gt; so others can contribute edits and improvements.
    &lt;/div&gt;
    </rdfs:comment>
    <rdfs:comment xml:lang="en">
    Most of the descriptions given here are from Wikipedia or from the related
    ontologies and vocabularies.
    </rdfs:comment>
    <rdfs:seeAlso rdf:resource="https://github.com/listinc/juso-ontology/tree/master/kr"/>
    <owl:versionInfo>0.1.1</owl:versionInfo>
    <skos:changeNote>
      <rdf:Description>
        <dcterms:creator rdf:resource="http://jayg.me/"/>
        <dcterms:date rdf:datatype="http://www.w3.org/2001/XMLSchema#date">2015-10-07+09:00</dcterms:date>
        <rdf:value xml:lang="en">
      Fixed the wrong use of rdf:XMLLiteral
      </rdf:value>
      </rdf:Description>
    </skos:changeNote>
    <skos:historyNote>
      <rdf:Description>
        <dcterms:creator rdf:resource="http://jayg.me/"/>
        <dcterms:date rdf:datatype="http://www.w3.org/2001/XMLSchema#date">2015-11-10+09:00</dcterms:date>
        <rdf:value xml:lang="en">
      Added juso:congnamul_x and juso:congnamul_y
      </rdf:value>
      </rdf:Description>
    </skos:historyNote>
    <adms:status rdf:resource="http://purl.org/adms/status/UnderDevelopment"/>
  </owl:Ontology>
  <rdf:Description rdf:about="http://rdfs.co/juso/kr/0.1.1/html">
    <dcterms:format>
      <dcterms:MediaType>
        <dcam:memberOf rdf:resource="http://purl.org/dc/terms/IMT"/>
        <rdf:value>text/html</rdf:value>
        <rdfs:label xml:lang="en">HTML</rdfs:label>
        <rdfs:seeAlso rdf:resource="http://www.iana.org/assignments/media-types/text/html"/>
        <owl:sameAs rdf:resource="https://w3id.org/spar/mediatype/text/html"/>
      </dcterms:MediaType>
    </dcterms:format>
  </rdf:Description>
  <rdf:Description rdf:about="http://rdfs.co/juso/kr/0.1.1/rdf">
    <dcterms:format>
      <dcterms:MediaType>
        <dcam:memberOf rdf:resource="http://purl.org/dc/terms/IMT"/>
        <rdf:value>application/rdf+xml</rdf:value>
        <rdfs:label xml:lang="en">RDF/XML</rdfs:label>
        <rdfs:seeAlso rdf:resource="http://www.iana.org/assignments/media-types/application/rdf+xml"/>
        <owl:sameAs rdf:resource="https://w3id.org/spar/mediatype/application/rdf%2Bxml"/>
      </dcterms:MediaType>
    </dcterms:format>
  </rdf:Description>
  <rdf:Description rdf:about="http://rdfs.co/juso/kr/0.1.1/ttl">
    <dcterms:format>
      <dcterms:MediaType>
        <dcam:memberOf rdf:resource="http://purl.org/dc/terms/IMT"/>
        <rdf:value>text/turtle</rdf:value>
        <rdfs:label xml:lang="en">Turtle</rdfs:label>
        <rdfs:seeAlso rdf:resource="http://www.iana.org/assignments/media-types/text/turtle"/>
        <owl:sameAs rdf:resource="https://w3id.org/spar/mediatype/text/turtle"/>
      </dcterms:MediaType>
    </dcterms:format>
  </rdf:Description>
  <rdf:Bag rdf:about="http://rdfs.co/juso/kr/AddressGroup">
    <rdf:_1 rdf:resource="http://rdfs.co/juso/kr/EastAsianAddress"/>
    <rdf:_10 rdf:resource="http://rdfs.co/juso/kr/Street"/>
    <rdf:_11 rdf:resource="http://rdfs.co/juso/kr/Road"/>
    <rdf:_12 rdf:resource="http://rdfs.co/juso/kr/road_name_number"/>
    <rdf:_13 rdf:resource="http://rdfs.co/juso/kr/parent_road"/>
    <rdf:_14 rdf:resource="http://rdfs.co/juso/kr/Building"/>
    <rdf:_15 rdf:resource="http://rdfs.co/juso/kr/administrative_building_number"/>
    <rdf:_16 rdf:resource="http://rdfs.co/juso/kr/MultiFamilyResidentialBuilding"/>
    <rdf:_17 rdf:resource="http://rdfs.co/juso/kr/PostalCode1970"/>
    <rdf:_18 rdf:resource="http://rdfs.co/juso/kr/PostalCode1988"/>
    <rdf:_19 rdf:resource="http://rdfs.co/juso/kr/PostalCode2015"/>
    <rdf:_2 rdf:resource="http://rdfs.co/juso/kr/RoadNameAddress"/>
    <rdf:_20 rdf:resource="http://rdfs.co/juso/kr/landform"/>
    <rdf:_21 rdf:resource="http://rdfs.co/juso/kr/floor"/>
    <rdf:_22 rdf:resource="http://rdfs.co/juso/kr/building_number"/>
    <rdf:_23 rdf:resource="http://rdfs.co/juso/kr/building_extra_number"/>
    <rdf:_24 rdf:resource="http://rdfs.co/juso/kr/eup_myeon_dong_serial_number"/>
    <rdf:_3 rdf:resource="http://rdfs.co/juso/kr/si_do"/>
    <rdf:_4 rdf:resource="http://rdfs.co/juso/kr/si_gun_gu"/>
    <rdf:_5 rdf:resource="http://rdfs.co/juso/kr/eup_myeon_dong"/>
    <rdf:_6 rdf:resource="http://rdfs.co/juso/kr/ri"/>
    <rdf:_7 rdf:resource="http://rdfs.co/juso/kr/beonji"/>
    <rdf:_8 rdf:resource="http://rdfs.co/juso/kr/ho"/>
    <rdf:_9 rdf:resource="http://rdfs.co/juso/kr/Boulevard"/>
    <rdfs:comment xml:lang="en">
     These classes and properties are used to describe addresses in South Korea.
     </rdfs:comment>
    <rdfs:label xml:lang="en">Address Terms</rdfs:label>
  </rdf:Bag>
  <owl:Class rdf:about="http://rdfs.co/juso/kr/AdministrativeCity">
    <dcterms:issued rdf:datatype="http://www.w3.org/2001/XMLSchema#date">2015-10-02+09:00</dcterms:issued>
    <dcterms:modified rdf:datatype="http://www.w3.org/2001/XMLSchema#date">2015-10-02+09:00</dcterms:modified>
    <rdfs:comment xml:lang="en">
    Since Jeju was given more autonomy, cities in Jeju could not be defined by
    the Local Autonomy Law so this new class of city was created for Jeju.
    </rdfs:comment>
    <rdfs:isDefinedBy rdf:resource="http://rdfs.co/juso/kr/"/>
    <rdfs:seeAlso rdf:resource="https://en.wikipedia.org/wiki/Cities_of_South_Korea"/>
    <rdfs:seeAlso rdf:resource="https://ko.wikipedia.org/wiki/행정시"/>
    <rdfs:subClassOf rdf:resource="http://rdfs.co/juso/City"/>
    <rdfs:subClassOf rdf:resource="http://rdfs.co/juso/SecondLevelAdministrativeDivision"/>
    <owl:disjointWith rdf:resource="http://rdfs.co/juso/kr/City"/>
    <status:term_status xml:lang="en">unstable</status:term_status>
    <skos:definition xml:lang="en">
    An Administrative city is a type of municipal city that are created in 1
    July 2006 after the 2005 referendum in Jeju and the province was given
    extensive administrative powers that had previously been reserved for the
    central government.
    </skos:definition>
    <skos:definition xml:lang="ko">
    행정시(行政市)는 대한민국의 행정 구역 중 하나로, 지방자치법 시행 이후 기초자치단체인 자치시로
    전환되면서 사실상 행정시의 기능은 완전히 사라졌다가 특별자치도 제도의 도입으로 제주특별자치도가
    2006년 7월 1일 출범하면서 행정시가 다시 나타났다.
    </skos:definition>
    <skos:prefLabel xml:lang="en">Administrative City</skos:prefLabel>
    <skos:prefLabel xml:lang="ko">행정시</skos:prefLabel>
  </owl:Class>
  <rdf:Bag rdf:about="http://rdfs.co/juso/kr/AdministrativeDivisionGroup">
    <rdf:_1 rdf:resource="http://rdfs.co/juso/kr/RegionalLocalGovernment"/>
    <rdf:_10 rdf:resource="http://rdfs.co/juso/kr/AdministrativeCity"/>
    <rdf:_11 rdf:resource="http://rdfs.co/juso/kr/County"/>
    <rdf:_12 rdf:resource="http://rdfs.co/juso/kr/AutonomousDistrict"/>
    <rdf:_13 rdf:resource="http://rdfs.co/juso/kr/NonAutonomousDistrict"/>
    <rdf:_14 rdf:resource="http://rdfs.co/juso/kr/si_gun_gu_code"/>
    <rdf:_15 rdf:resource="http://rdfs.co/juso/kr/Town"/>
    <rdf:_16 rdf:resource="http://rdfs.co/juso/kr/Township"/>
    <rdf:_17 rdf:resource="http://rdfs.co/juso/kr/LegalStatusNeighborhood"/>
    <rdf:_18 rdf:resource="http://rdfs.co/juso/kr/legal_status_neighborhood_code"/>
    <rdf:_19 rdf:resource="http://rdfs.co/juso/kr/AdministrativeNeighborhood"/>
    <rdf:_2 rdf:resource="http://rdfs.co/juso/kr/Province"/>
    <rdf:_20 rdf:resource="http://rdfs.co/juso/kr/administrative_neighborhood_code"/>
    <rdf:_21 rdf:resource="http://rdfs.co/juso/kr/eup_myeon_dong_code"/>
    <rdf:_22 rdf:resource="http://rdfs.co/juso/kr/LegalStatusVillage"/>
    <rdf:_23 rdf:resource="http://rdfs.co/juso/kr/AdministrativeVillage"/>
    <rdf:_3 rdf:resource="http://rdfs.co/juso/kr/SpecialAutonomousProvince"/>
    <rdf:_4 rdf:resource="http://rdfs.co/juso/kr/SpecialCity"/>
    <rdf:_5 rdf:resource="http://rdfs.co/juso/kr/MetropolitanCity"/>
    <rdf:_6 rdf:resource="http://rdfs.co/juso/kr/MetropolitanAutonomousCity"/>
    <rdf:_7 rdf:resource="http://rdfs.co/juso/kr/BasicLocalGovernment"/>
    <rdf:_8 rdf:resource="http://rdfs.co/juso/kr/City"/>
    <rdf:_9 rdf:resource="http://rdfs.co/juso/kr/SpecificCity"/>
    <rdfs:comment xml:lang="en">
    These classes and properties are used to describe administrative divisions
    in South Korea.
    </rdfs:comment>
    <rdfs:label xml:lang="en">Administrative Division Terms</rdfs:label>
    <rdfs:label xml:lang="ko">행정 구역 용어</rdfs:label>
  </rdf:Bag>
  <owl:Class rdf:about="http://rdfs.co/juso/kr/AdministrativeNeighborhood">
    <dcterms:issued rdf:datatype="http://www.w3.org/2001/XMLSchema#date">2015-10-02+09:00</dcterms:issued>
    <dcterms:modified rdf:datatype="http://www.w3.org/2001/XMLSchema#date">2015-10-02+09:00</dcterms:modified>
    <rdfs:comment xml:lang="en">
    In some cases, a single legal-status neighborhood is divided into several
    administrative neighborhoods. In such cases, each administrative dong has
    its own office and staff.
    </rdfs:comment>
    <rdfs:isDefinedBy rdf:resource="http://rdfs.co/juso/kr/"/>
    <rdfs:seeAlso rdf:resource="https://en.wikipedia.org/wiki/Dong_(administrative_division)"/>
    <rdfs:seeAlso rdf:resource="https://ko.wikipedia.org/wiki/동_(행정_구역)"/>
    <rdfs:subClassOf rdf:resource="http://rdfs.co/juso/Neighborhood"/>
    <rdfs:subClassOf rdf:resource="http://rdfs.co/juso/ThirdLevelAdministrativeDivision"/>
    <status:term_status xml:lang="en">unstable</status:term_status>
    <skos:definition xml:lang="en">
    An administrative neighborhood is the smallest level of urban government to
    have its own office and staff in South Korea.
    </skos:definition>
    <skos:definition xml:lang="ko">
    행정동(行政洞)은 대한민국의 행정 구역의 하나로 구 또는 시의 하부 행정 구역이다.
    </skos:definition>
    <skos:prefLabel xml:lang="en">Administrative Neighborhood</skos:prefLabel>
    <skos:prefLabel xml:lang="ko">행정동</skos:prefLabel>
  </owl:Class>
  <owl:Class rdf:about="http://rdfs.co/juso/kr/AdministrativeVillage">
    <dcterms:issued rdf:datatype="http://www.w3.org/2001/XMLSchema#date">2015-10-02+09:00</dcterms:issued>
    <dcterms:modified rdf:datatype="http://www.w3.org/2001/XMLSchema#date">2015-10-02+09:00</dcterms:modified>
    <rdfs:comment xml:lang="en">
    A legal-status village can be subdivided into one or more administrative
    villages.
    </rdfs:comment>
    <rdfs:isDefinedBy rdf:resource="http://rdfs.co/juso/kr/"/>
    <rdfs:seeAlso rdf:resource="https://en.wikipedia.org/wiki/Ri_(administrative_division)"/>
    <rdfs:seeAlso rdf:resource="https://ko.wikipedia.org/wiki/리_(행정_구역)"/>
    <rdfs:subClassOf rdf:resource="http://rdfs.co/juso/FourthLevelAdministrativeDivision"/>
    <rdfs:subClassOf rdf:resource="http://rdfs.co/juso/Village"/>
    <status:term_status xml:lang="en">unstable</status:term_status>
    <skos:definition xml:lang="en">
    A administrative village is an administrative unit in South Korea.
    </skos:definition>
    <skos:definition xml:lang="ko">
    대한민국의 리(里)는 읍(邑)·면(面)의 하부 행정 구역이며, 행정리(行政里)는 인구와 생활권을 고려하여
    법정리에 1개 또는 여러 개로 설치한 행정 구역이다.
    </skos:definition>
    <skos:prefLabel xml:lang="en">Administrative Village</skos:prefLabel>
    <skos:prefLabel xml:lang="ko">행정리</skos:prefLabel>
  </owl:Class>
  <owl:Class rdf:about="http://rdfs.co/juso/kr/AutonomousDistrict">
    <dcterms:issued rdf:datatype="http://www.w3.org/2001/XMLSchema#date">2015-10-02+09:00</dcterms:issued>
    <dcterms:modified rdf:datatype="http://www.w3.org/2001/XMLSchema#date">2015-10-02+09:00</dcterms:modified>
    <rdfs:isDefinedBy rdf:resource="http://rdfs.co/juso/kr/"/>
    <rdfs:seeAlso rdf:resource="https://en.wikipedia.org/wiki/Gu_(administrative_division)"/>
    <rdfs:seeAlso rdf:resource="https://ko.wikipedia.org/wiki/구_(행정_구역)"/>
    <rdfs:subClassOf rdf:resource="http://rdfs.co/juso/District"/>
    <rdfs:subClassOf rdf:resource="http://rdfs.co/juso/kr/BasicLocalGovernment"/>
    <owl:disjointWith rdf:resource="http://rdfs.co/juso/kr/NonAutonomousDistrict"/>
    <status:term_status xml:lang="en">unstable</status:term_status>
    <skos:definition xml:lang="en">
    An autonomous district of special and metropolitan cities is a municipal
    entity similar to a city with its own mayor along with its own
    legislative council.
    </skos:definition>
    <skos:definition xml:lang="ko">
    자치구(自治區)는 특별시, 광역시의 하위 행정 구역으로서 시, 군과 동급인 기초자치단체이다.
    </skos:definition>
    <skos:prefLabel xml:lang="en">Autonomous District</skos:prefLabel>
    <skos:prefLabel xml:lang="ko">자치구</skos:prefLabel>
  </owl:Class>
  <owl:Class rdf:about="http://rdfs.co/juso/kr/BasicLocalGovernment">
    <dcterms:issued rdf:datatype="http://www.w3.org/2001/XMLSchema#date">2015-10-02+09:00</dcterms:issued>
    <dcterms:modified rdf:datatype="http://www.w3.org/2001/XMLSchema#date">2015-10-02+09:00</dcterms:modified>
    <rdfs:comment xml:lang="en">
    Non-autonomous districts of municipal cities and administrative cities in
    Jeju are not basic local governments.
    </rdfs:comment>
    <rdfs:isDefinedBy rdf:resource="http://rdfs.co/juso/kr/"/>
    <rdfs:seeAlso rdf:resource="https://en.wikipedia.org/wiki/Administrative_divisions_of_South_Korea"/>
    <rdfs:seeAlso rdf:resource="https://ko.wikipedia.org/wiki/기초지방자치단체"/>
    <rdfs:subClassOf rdf:resource="http://rdfs.co/juso/SecondLevelAdministrativeDivision"/>
    <owl:disjointWith rdf:resource="http://rdfs.co/juso/kr/RegionalLocalGovernment"/>
    <status:term_status xml:lang="en">unstable</status:term_status>
    <skos:altLabel xml:lang="en">Lower-level Local Autonomy</skos:altLabel>
    <skos:altLabel xml:lang="en">Municipal Government</skos:altLabel>
    <skos:altLabel xml:lang="en">Municipality</skos:altLabel>
    <skos:definition xml:lang="en">
    Basic local governments are the municipal-level administrative division
    within South Korea.
    </skos:definition>
    <skos:definition xml:lang="ko">
    대한민국의 기초지방자치단체(基礎地方自治團體)는 지방자치단체에서 광역지방자치단체의 하부의
    조직으로서 광역지방자치단체보다 좁은 지역을 관할하는 지방 행정 조직이다.
    </skos:definition>
    <skos:prefLabel xml:lang="en">Basic Local Government</skos:prefLabel>
    <skos:prefLabel xml:lang="ko">기초지방자치단체</skos:prefLabel>
  </owl:Class>
  <owl:Class rdf:about="http://rdfs.co/juso/kr/Boulevard">
    <dcterms:issued rdf:datatype="http://www.w3.org/2001/XMLSchema#date">2015-10-02+09:00</dcterms:issued>
    <dcterms:modified rdf:datatype="http://www.w3.org/2001/XMLSchema#date">2015-10-02+09:00</dcterms:modified>
    <rdfs:isDefinedBy rdf:resource="http://rdfs.co/juso/kr/"/>
    <rdfs:seeAlso rdf:resource="https://ko.wikipedia.org/wiki/대한민국의_주소"/>
    <rdfs:subClassOf rdf:resource="http://rdfs.co/juso/Street"/>
    <status:term_status xml:lang="en">unstable</status:term_status>
    <skos:definition xml:lang="en">
    In the Road Name Address system, the word boulevard (daero) is used to
    describe two-way roads that have more than 40m width or 8 lanes.
    </skos:definition>
    <skos:definition xml:lang="ko">
    도로명주소에서 대로(大路)는 폭이 40m 이상이거나 왕복 8차선 이상의 도로를 의미한다.
    </skos:definition>
    <skos:prefLabel xml:lang="en">Boulevard</skos:prefLabel>
    <skos:prefLabel xml:lang="ko">대로</skos:prefLabel>
  </owl:Class>
  <owl:Class rdf:about="http://rdfs.co/juso/kr/Building">
    <dcterms:issued rdf:datatype="http://www.w3.org/2001/XMLSchema#date">2015-10-02+09:00</dcterms:issued>
    <dcterms:modified rdf:datatype="http://www.w3.org/2001/XMLSchema#date">2015-10-02+09:00</dcterms:modified>
    <rdfs:isDefinedBy rdf:resource="http://rdfs.co/juso/kr/"/>
    <rdfs:seeAlso rdf:resource="https://en.wikipedia.org/wiki/Building"/>
    <rdfs:seeAlso rdf:resource="https://ko.wikipedia.org/wiki/건축물"/>
    <rdfs:subClassOf rdf:resource="http://rdfs.co/juso/Feature"/>
    <status:term_status xml:lang="en">unstable</status:term_status>
    <skos:altLabel xml:lang="ko">건축물</skos:altLabel>
    <skos:altLabel xml:lang="ko">구축물</skos:altLabel>
    <skos:definition xml:lang="en">
    A building is a man-made structure with a roof and walls standing more or
    less permanently in one place, such as a house or factory.
    </skos:definition>
    <skos:definition xml:lang="ko">
    일반적으로 건물(建物)이란 일정 기간 동안 그 형상이 필요하기 때문에, 혹은 그것이 제공하는 공간이
    필요하기 때문에, 인간이 지은 지면에 고정되는 구조물을 뜻한다.
    </skos:definition>
    <skos:prefLabel xml:lang="en">Building</skos:prefLabel>
    <skos:prefLabel xml:lang="ko">건물</skos:prefLabel>
  </owl:Class>
  <owl:Class rdf:about="http://rdfs.co/juso/kr/City">
    <dcterms:issued rdf:datatype="http://www.w3.org/2001/XMLSchema#date">2015-10-02+09:00</dcterms:issued>
    <dcterms:modified rdf:datatype="http://www.w3.org/2001/XMLSchema#date">2015-10-02+09:00</dcterms:modified>
    <rdfs:comment xml:lang="en">
    Cities are ranked on the same level as county and autonomous district.
  </rdfs:comment>
    <rdfs:isDefinedBy rdf:resource="http://rdfs.co/juso/kr/"/>
    <rdfs:seeAlso rdf:resource="https://en.wikipedia.org/wiki/Cities_of_South_Korea"/>
    <rdfs:seeAlso rdf:resource="https://ko.wikipedia.org/wiki/시_(행정_구역)"/>
    <rdfs:subClassOf rdf:resource="http://rdfs.co/juso/City"/>
    <rdfs:subClassOf rdf:resource="http://rdfs.co/juso/kr/BasicLocalGovernment"/>
    <owl:disjointWith rdf:resource="http://rdfs.co/juso/kr/AdministrativeCity"/>
    <status:term_status xml:lang="en">unstable</status:term_status>
    <skos:definition xml:lang="en">
    A city is a municipal administrative unit in South Korea.
    </skos:definition>
    <skos:definition xml:lang="ko">
    시(市)는 대한민국 행정 구역의 하나로 행정시와 달리 기초지방자치단체에 해당한다.
    </skos:definition>
    <skos:prefLabel xml:lang="en">City</skos:prefLabel>
    <skos:prefLabel xml:lang="ko">시</skos:prefLabel>
  </owl:Class>
  <owl:Class rdf:about="http://rdfs.co/juso/kr/County">
    <dcterms:issued rdf:datatype="http://www.w3.org/2001/XMLSchema#date">2015-10-02+09:00</dcterms:issued>
    <dcterms:modified rdf:datatype="http://www.w3.org/2001/XMLSchema#date">2015-10-02+09:00</dcterms:modified>
    <rdfs:comment xml:lang="en">
    In South Korea, a county has a population of less than 150,000 (more than
    that would make it a city), is less densely populated than a district, and
    is more rural in character than either of the other 2 divisions.
    </rdfs:comment>
    <rdfs:isDefinedBy rdf:resource="http://rdfs.co/juso/kr/"/>
    <rdfs:seeAlso rdf:resource="https://en.wikipedia.org/wiki/Gun_(administrative_division)"/>
    <rdfs:seeAlso rdf:resource="https://ko.wikipedia.org/wiki/군_(행정_구역)"/>
    <rdfs:subClassOf rdf:resource="http://rdfs.co/juso/County"/>
    <rdfs:subClassOf rdf:resource="http://rdfs.co/juso/kr/BasicLocalGovernment"/>
    <status:term_status xml:lang="en">unstable</status:term_status>
    <skos:definition xml:lang="en">
    A county is an administrative unit in South Korea similar.
    </skos:definition>
    <skos:definition xml:lang="ko">
    군(郡)은 행정 구역의 하나로, 대한민국의 군은 도 및 광역시의 하부 행정 구역이자 기초지방자치단체이다.
    </skos:definition>
    <skos:prefLabel xml:lang="en">County</skos:prefLabel>
    <skos:prefLabel xml:lang="ko">군</skos:prefLabel>
  </owl:Class>
  <owl:Class rdf:about="http://rdfs.co/juso/kr/EastAsianAddress">
    <dcterms:issued rdf:datatype="http://www.w3.org/2001/XMLSchema#date">2015-10-02+09:00</dcterms:issued>
    <dcterms:modified rdf:datatype="http://www.w3.org/2001/XMLSchema#date">2015-10-02+09:00</dcterms:modified>
    <rdfs:isDefinedBy rdf:resource="http://rdfs.co/juso/kr/"/>
    <rdfs:seeAlso rdf:resource="https://en.wikipedia.org/wiki/Addresses_in_South_Korea"/>
    <rdfs:seeAlso rdf:resource="https://ko.wikipedia.org/wiki/대한민국의_주소"/>
    <rdfs:subClassOf rdf:resource="http://rdfs.co/juso/Address"/>
    <status:term_status xml:lang="en">testing</status:term_status>
    <skos:definition xml:lang="en">
    The previous addressing system used in South Korea was the the East Asian
    system, which is also used in Japan and North Korea (but not within the
      Chinese-speaking world), but although still commonly used, is no longer
    officially recognized since December 31, 2013.
    </skos:definition>
    <skos:definition xml:lang="ko">
    기존 대한민국에서 사용되던 지번 주소 체계는 토지 구획을 정리한 지번을 구분자로 이용하는 주소 체계로
    아직 널리 사용되고 있으나 2014년 1월 1일부터 도로명주소로 대체되어 공식적으로 폐지되었다.
    </skos:definition>
    <skos:prefLabel xml:lang="en">East Asian Address</skos:prefLabel>
    <skos:prefLabel xml:lang="ko">지번 주소</skos:prefLabel>
  </owl:Class>
  <owl:Class rdf:about="http://rdfs.co/juso/kr/LegalStatusNeighborhood">
    <dcterms:issued rdf:datatype="http://www.w3.org/2001/XMLSchema#date">2015-10-02+09:00</dcterms:issued>
    <dcterms:modified rdf:datatype="http://www.w3.org/2001/XMLSchema#date">2015-10-02+09:00</dcterms:modified>
    <rdfs:isDefinedBy rdf:resource="http://rdfs.co/juso/kr/"/>
    <rdfs:seeAlso rdf:resource="https://en.wikipedia.org/wiki/Dong_(administrative_division)"/>
    <rdfs:seeAlso rdf:resource="https://ko.wikipedia.org/wiki/법정동"/>
    <rdfs:subClassOf rdf:resource="http://rdfs.co/juso/Neighborhood"/>
    <rdfs:subClassOf rdf:resource="http://rdfs.co/juso/ThirdLevelAdministrativeDivision"/>
    <status:term_status xml:lang="en">unstable</status:term_status>
    <skos:definition xml:lang="en">
    A legal-status neighborhood is a submunicipal level administrative unit of
    a city and of those cities which are not divided into districts throughout
    Korea.
    </skos:definition>
    <skos:definition xml:lang="ko">
    법정동(法定洞)은 대한민국 법정 구역으로, 법률(관습법)로 지정된 일정한 명칭과 영역을 지닌
    구역이다.
    </skos:definition>
    <skos:prefLabel xml:lang="en">Legal-status Neighborhood</skos:prefLabel>
    <skos:prefLabel xml:lang="ko">법정동</skos:prefLabel>
  </owl:Class>
  <owl:Class rdf:about="http://rdfs.co/juso/kr/LegalStatusVillage">
    <dcterms:issued rdf:datatype="http://www.w3.org/2001/XMLSchema#date">2015-10-02+09:00</dcterms:issued>
    <dcterms:modified rdf:datatype="http://www.w3.org/2001/XMLSchema#date">2015-10-02+09:00</dcterms:modified>
    <rdfs:isDefinedBy rdf:resource="http://rdfs.co/juso/kr/"/>
    <rdfs:seeAlso rdf:resource="https://en.wikipedia.org/wiki/Ri_(administrative_division)"/>
    <rdfs:seeAlso rdf:resource="https://ko.wikipedia.org/wiki/리_(행정_구역)"/>
    <rdfs:subClassOf rdf:resource="http://rdfs.co/juso/FourthLevelAdministrativeDivision"/>
    <rdfs:subClassOf rdf:resource="http://rdfs.co/juso/Village"/>
    <status:term_status xml:lang="en">unstable</status:term_status>
    <skos:definition xml:lang="en">
    A legal-status village is an administrative unit in South Korea.
    </skos:definition>
    <skos:definition xml:lang="ko">
    대한민국의 리(里)는 읍(邑)·면(面)의 하부 행정 구역이며, 법정리(法定里)는 법령으로 정하여진 리로
    지번의 기준이 된다.
    </skos:definition>
    <skos:prefLabel xml:lang="en">Legal-status Village</skos:prefLabel>
    <skos:prefLabel xml:lang="ko">법정리</skos:prefLabel>
  </owl:Class>
  <owl:Class rdf:about="http://rdfs.co/juso/kr/MetropolitanAutonomousCity">
    <dcterms:issued rdf:datatype="http://www.w3.org/2001/XMLSchema#date">2015-10-02+09:00</dcterms:issued>
    <dcterms:modified rdf:datatype="http://www.w3.org/2001/XMLSchema#date">2015-10-02+09:00</dcterms:modified>
    <rdfs:comment xml:lang="en">
    The only metropolitan autonomous city in South Korea called Sejong opened 2
    July 2012.
    </rdfs:comment>
    <rdfs:isDefinedBy rdf:resource="http://rdfs.co/juso/kr/"/>
    <rdfs:seeAlso rdf:resource="https://en.wikipedia.org/wiki/Special_cities_of_South_Korea"/>
    <rdfs:seeAlso rdf:resource="https://ko.wikipedia.org/wiki/특별자치시"/>
    <rdfs:subClassOf rdf:resource="http://rdfs.co/juso/City"/>
    <rdfs:subClassOf rdf:resource="http://rdfs.co/juso/kr/RegionalLocalGovernment"/>
    <owl:disjointWith rdf:resource="http://rdfs.co/juso/kr/MetropolitanCity"/>
    <owl:disjointWith rdf:resource="http://rdfs.co/juso/kr/SpecialCity"/>
    <status:term_status xml:lang="en">unstable</status:term_status>
    <skos:definition xml:lang="en">
    In early 2007, the South Korean government created a special administrative
    district from parts of South Chungcheong and North Chungcheong provinces,
    near Daejeon, to relocate nine ministries and four national agencies from
    Seoul.
    </skos:definition>
    <skos:definition xml:lang="ko">
    특별자치시(特別自治市)는 대한민국의 행정 구역이다.
    </skos:definition>
    <skos:prefLabel xml:lang="en">Metropolitan Autonomous City</skos:prefLabel>
    <skos:prefLabel xml:lang="ko">특별자치시</skos:prefLabel>
  </owl:Class>
  <owl:Class rdf:about="http://rdfs.co/juso/kr/MetropolitanCity">
    <dcterms:issued rdf:datatype="http://www.w3.org/2001/XMLSchema#date">2015-10-02+09:00</dcterms:issued>
    <dcterms:modified rdf:datatype="http://www.w3.org/2001/XMLSchema#date">2015-10-02+09:00</dcterms:modified>
    <rdfs:comment xml:lang="en">
    They were called "directly-administered city" before 1995. These cities
    have equal status to the provinces.
    </rdfs:comment>
    <rdfs:isDefinedBy rdf:resource="http://rdfs.co/juso/kr/"/>
    <rdfs:seeAlso rdf:resource="https://en.wikipedia.org/wiki/Special_cities_of_South_Korea"/>
    <rdfs:seeAlso rdf:resource="https://ko.wikipedia.org/wiki/광역시"/>
    <rdfs:subClassOf rdf:resource="http://rdfs.co/juso/City"/>
    <rdfs:subClassOf rdf:resource="http://rdfs.co/juso/kr/RegionalLocalGovernment"/>
    <owl:disjointWith rdf:resource="http://rdfs.co/juso/kr/MetropolitanAutonomousCity"/>
    <owl:disjointWith rdf:resource="http://rdfs.co/juso/kr/SpecialCity"/>
    <status:term_status xml:lang="en">unstable</status:term_status>
    <skos:definition xml:lang="en">
    Metropolitan cities are the highest-ranked administrative divisions in
    South Korea.
    </skos:definition>
    <skos:definition xml:lang="ko">
    광역시(廣域市)는 대한민국의 행정 구역이다.
    </skos:definition>
    <skos:prefLabel xml:lang="en">Metropolitan City</skos:prefLabel>
    <skos:prefLabel xml:lang="ko">광역시</skos:prefLabel>
  </owl:Class>
  <owl:Class rdf:about="http://rdfs.co/juso/kr/MultiFamilyResidentialBuilding">
    <dcterms:issued rdf:datatype="http://www.w3.org/2001/XMLSchema#date">2015-10-02+09:00</dcterms:issued>
    <dcterms:modified rdf:datatype="http://www.w3.org/2001/XMLSchema#date">2015-10-02+09:00</dcterms:modified>
    <rdfs:isDefinedBy rdf:resource="http://rdfs.co/juso/kr/"/>
    <rdfs:seeAlso rdf:resource="https://en.wikipedia.org/wiki/Multi-family_residential"/>
    <rdfs:seeAlso rdf:resource="https://ko.wikipedia.org/wiki/공동_주택"/>
    <rdfs:subClassOf rdf:resource="http://rdfs.co/juso/kr/Building"/>
    <status:term_status xml:lang="en">unstable</status:term_status>
    <skos:altLabel xml:lang="en">MDU Building</skos:altLabel>
    <skos:altLabel xml:lang="en">Multi-dwelling Unit Building</skos:altLabel>
    <skos:definition xml:lang="en">
    A multifamily residential building is a building that contain multiple
    separate housing units for residential inhabitants.
    </skos:definition>
    <skos:definition xml:lang="ko">
    공동 주택(共同住宅)은 하나의 건물 내에 서로 독립적인 여러 세대가 공동으로 거주하는 주거의
    형태이다.
    </skos:definition>
    <skos:prefLabel xml:lang="en">Multi-family Residential Building</skos:prefLabel>
    <skos:prefLabel xml:lang="ko">공동 주택</skos:prefLabel>
  </owl:Class>
  <owl:Class rdf:about="http://rdfs.co/juso/kr/NonAutonomousDistrict">
    <dcterms:issued rdf:datatype="http://www.w3.org/2001/XMLSchema#date">2015-10-02+09:00</dcterms:issued>
    <dcterms:modified rdf:datatype="http://www.w3.org/2001/XMLSchema#date">2015-10-02+09:00</dcterms:modified>
    <rdfs:isDefinedBy rdf:resource="http://rdfs.co/juso/kr/"/>
    <rdfs:seeAlso rdf:resource="https://en.wikipedia.org/wiki/Gu_(administrative_division)"/>
    <rdfs:seeAlso rdf:resource="https://ko.wikipedia.org/wiki/구_(행정_구역)"/>
    <rdfs:subClassOf rdf:resource="http://rdfs.co/juso/District"/>
    <rdfs:subClassOf rdf:resource="http://rdfs.co/juso/SecondLevelAdministrativeDivision"/>
    <owl:disjointWith rdf:resource="http://rdfs.co/juso/kr/AutonomousDistrict"/>
    <status:term_status xml:lang="en">unstable</status:term_status>
    <skos:altLabel xml:lang="en">Administrative District</skos:altLabel>
    <skos:altLabel xml:lang="ko">행정구</skos:altLabel>
    <skos:definition xml:lang="en">
    Cities with over 500,000 people are allowed to have non-autonomous
    districts (notable exceptions to this rule are the cities of Gimhae,
    Hwaseong, and Namyangju).
    </skos:definition>
    <skos:definition xml:lang="ko">
    자치구가 아닌 일반구(一般區)는 인구 50만 명 이상인 시(기초자치단체)의 하위 행정 구역이다.
    </skos:definition>
    <skos:prefLabel xml:lang="en">Non-autonomous District</skos:prefLabel>
    <skos:prefLabel xml:lang="ko">일반구</skos:prefLabel>
  </owl:Class>
  <owl:Class rdf:about="http://rdfs.co/juso/kr/PostalCode1970">
    <dcterms:issued rdf:datatype="http://www.w3.org/2001/XMLSchema#date">2015-10-02+09:00</dcterms:issued>
    <dcterms:modified rdf:datatype="http://www.w3.org/2001/XMLSchema#date">2015-10-02+09:00</dcterms:modified>
    <rdfs:isDefinedBy rdf:resource="http://rdfs.co/juso/kr/"/>
    <rdfs:seeAlso rdf:resource="https://en.wikipedia.org/wiki/List_of_postal_codes"/>
    <rdfs:seeAlso rdf:resource="https://ko.wikipedia.org/wiki/대한민국의_우편번호"/>
    <rdfs:subClassOf rdf:resource="http://rdfs.co/juso/PostalCode"/>
    <status:term_status xml:lang="en">unstable</status:term_status>
    <skos:definition xml:lang="ko">
    1970년 7월 1일에 도입되어 1988년 1월 31일까지 사용된 대한민국 최초의 5자리 우편번호.
    </skos:definition>
    <skos:definition xml:lang="en">
    The first 5-digit postal code system in South Korea that was rolled out on
    July 1, 1970, and used until January 31, 1988.
    </skos:definition>
    <skos:prefLabel xml:lang="en">Postal Code (1970 - 1988)</skos:prefLabel>
    <skos:prefLabel xml:lang="ko">우편번호(1970 ~ 1988)</skos:prefLabel>
  </owl:Class>
  <owl:Class rdf:about="http://rdfs.co/juso/kr/PostalCode1988">
    <dcterms:issued rdf:datatype="http://www.w3.org/2001/XMLSchema#date">2015-10-02+09:00</dcterms:issued>
    <dcterms:modified rdf:datatype="http://www.w3.org/2001/XMLSchema#date">2015-10-02+09:00</dcterms:modified>
    <rdfs:isDefinedBy rdf:resource="http://rdfs.co/juso/kr/"/>
    <rdfs:seeAlso rdf:resource="https://en.wikipedia.org/wiki/List_of_postal_codes"/>
    <rdfs:seeAlso rdf:resource="https://ko.wikipedia.org/wiki/대한민국의_우편번호"/>
    <rdfs:subClassOf rdf:resource="http://rdfs.co/juso/PostalCode"/>
    <status:term_status xml:lang="en">unstable</status:term_status>
    <skos:definition xml:lang="ko">
    1988년 2월 1일에 도입되어 2015년 7월 31일까지 사용된 대한민국의 6자리 우편번호.
    </skos:definition>
    <skos:definition xml:lang="en">
    The 6-digit postal code system in South Korea that was rolled out on
    February 1, 1988, and used until July 31, 2015.
    </skos:definition>
    <skos:prefLabel xml:lang="en">Postal Code (1988 - 2015)</skos:prefLabel>
    <skos:prefLabel xml:lang="ko">우편번호(1988 ~ 2015)</skos:prefLabel>
  </owl:Class>
  <owl:Class rdf:about="http://rdfs.co/juso/kr/PostalCode2015">
    <dcterms:issued rdf:datatype="http://www.w3.org/2001/XMLSchema#date">2015-10-02+09:00</dcterms:issued>
    <dcterms:modified rdf:datatype="http://www.w3.org/2001/XMLSchema#date">2015-10-02+09:00</dcterms:modified>
    <rdfs:isDefinedBy rdf:resource="http://rdfs.co/juso/kr/"/>
    <rdfs:seeAlso rdf:resource="https://en.wikipedia.org/wiki/List_of_postal_codes_in_South_Korea"/>
    <rdfs:seeAlso rdf:resource="https://ko.wikipedia.org/wiki/대한민국의_우편번호"/>
    <rdfs:subClassOf rdf:resource="http://rdfs.co/juso/PostalCode"/>
    <status:term_status xml:lang="en">unstable</status:term_status>
    <skos:definition xml:lang="ko">
    2015년 8월 1일에 도입된 도로명주소 체계 기반 5자리 대한민국 우편번호.
    </skos:definition>
    <skos:definition xml:lang="en">
    The 5-digit postal code system based on the road name address system in
    South Korea, which has been rolled out on August 1, 2015.
    </skos:definition>
    <skos:prefLabel xml:lang="en">Postal Code (1988 - 2015)</skos:prefLabel>
    <skos:prefLabel xml:lang="ko">우편번호(1988 ~ 2015)</skos:prefLabel>
  </owl:Class>
  <owl:Class rdf:about="http://rdfs.co/juso/kr/Province">
    <dcterms:issued rdf:datatype="http://www.w3.org/2001/XMLSchema#date">2015-10-02+09:00</dcterms:issued>
    <dcterms:modified rdf:datatype="http://www.w3.org/2001/XMLSchema#date">2015-10-02+09:00</dcterms:modified>
    <rdfs:isDefinedBy rdf:resource="http://rdfs.co/juso/kr/"/>
    <rdfs:seeAlso rdf:resource="https://en.wikipedia.org/wiki/Provinces_of_South_Korea"/>
    <rdfs:seeAlso rdf:resource="https://ko.wikipedia.org/wiki/도_(행정_구역)"/>
    <rdfs:subClassOf rdf:resource="http://rdfs.co/juso/Province"/>
    <rdfs:subClassOf rdf:resource="http://rdfs.co/juso/kr/RegionalLocalGovernment"/>
    <owl:disjointWith rdf:resource="http://rdfs.co/juso/kr/SpecialAutonomousProvince"/>
    <status:term_status xml:lang="en">unstable</status:term_status>
    <skos:altLabel xml:lang="ko">일반도</skos:altLabel>
    <skos:definition xml:lang="en">
    A province are the highest-ranked administrative divisions in South Korea.
    </skos:definition>
    <skos:definition xml:lang="ko">
    도(道)는 대한민국의 행정 구역 이름으로 특별자치도와 구분된다.
    </skos:definition>
    <skos:prefLabel xml:lang="en">Province</skos:prefLabel>
    <skos:prefLabel xml:lang="ko">도</skos:prefLabel>
  </owl:Class>
  <owl:Class rdf:about="http://rdfs.co/juso/kr/RegionalLocalGovernment">
    <dcterms:issued rdf:datatype="http://www.w3.org/2001/XMLSchema#date">2015-10-02+09:00</dcterms:issued>
    <dcterms:modified rdf:datatype="http://www.w3.org/2001/XMLSchema#date">2015-10-02+09:00</dcterms:modified>
    <rdfs:isDefinedBy rdf:resource="http://rdfs.co/juso/kr/"/>
    <rdfs:seeAlso rdf:resource="https://en.wikipedia.org/wiki/Administrative_divisions_of_South_Korea"/>
    <rdfs:seeAlso rdf:resource="https://ko.wikipedia.org/wiki/광역자치단체"/>
    <rdfs:subClassOf rdf:resource="http://rdfs.co/juso/FirstLevelAdministrativeDivision"/>
    <owl:disjointWith rdf:resource="http://rdfs.co/juso/kr/BasicLocalGovernment"/>
    <status:term_status xml:lang="en">unstable</status:term_status>
    <skos:altLabel xml:lang="en">Metropolitan Government</skos:altLabel>
    <skos:altLabel xml:lang="en">Upper-level Local Autonomy</skos:altLabel>
    <skos:definition xml:lang="en">
    Regional local governments are the highest-ranked administrative division
    within South Korea.
    </skos:definition>
    <skos:definition xml:lang="ko">
    대한민국의 광역지방자치단체(廣域地方自治團體)는 지방자치단체 중 기초지방자치단체에 비해 넓은 구역과
    많은 주민을 관할하는 기초지방자치단체 상위의 행정 구역이다.
    </skos:definition>
    <skos:prefLabel xml:lang="en">Regional Local Government</skos:prefLabel>
    <skos:prefLabel xml:lang="ko">광역지방자치단체</skos:prefLabel>
  </owl:Class>
  <owl:Class rdf:about="http://rdfs.co/juso/kr/Road">
    <dcterms:issued rdf:datatype="http://www.w3.org/2001/XMLSchema#date">2015-10-02+09:00</dcterms:issued>
    <dcterms:modified rdf:datatype="http://www.w3.org/2001/XMLSchema#date">2015-10-02+09:00</dcterms:modified>
    <rdfs:isDefinedBy rdf:resource="http://rdfs.co/juso/kr/"/>
    <rdfs:seeAlso rdf:resource="https://ko.wikipedia.org/wiki/대한민국의_주소"/>
    <rdfs:subClassOf rdf:resource="http://rdfs.co/juso/Street"/>
    <status:term_status xml:lang="en">unstable</status:term_status>
    <skos:definition xml:lang="en">
    In the Road Name Address system, the word road (gil) is used to describe
    roads that have less than 12m width or 2 lanes.
    width or 2 lanes.
    </skos:definition>
    <skos:definition xml:lang="ko">
    도로명주소에서 길은 폭이 12m 미만이거나 2차로 미만인 도로를 의미한다.
    </skos:definition>
    <skos:prefLabel xml:lang="en">Road</skos:prefLabel>
    <skos:prefLabel xml:lang="ko">길</skos:prefLabel>
  </owl:Class>
  <owl:Class rdf:about="http://rdfs.co/juso/kr/RoadNameAddress">
    <dcterms:issued rdf:datatype="http://www.w3.org/2001/XMLSchema#date">2015-10-02+09:00</dcterms:issued>
    <dcterms:modified rdf:datatype="http://www.w3.org/2001/XMLSchema#date">2015-10-02+09:00</dcterms:modified>
    <rdfs:isDefinedBy rdf:resource="http://rdfs.co/juso/kr/"/>
    <rdfs:seeAlso rdf:resource="https://en.wikipedia.org/wiki/Addresses_in_South_Korea"/>
    <rdfs:seeAlso rdf:resource="https://ko.wikipedia.org/wiki/대한민국의_주소"/>
    <rdfs:subClassOf rdf:resource="http://rdfs.co/juso/Address"/>
    <status:term_status xml:lang="en">testing</status:term_status>
    <skos:definition xml:lang="en">
    The Road Name Address system, rolled out on January 1, 2014, uses street
    names and house numbers, and is similar to the systems used by the United
    States, Canada, and Europe.
    </skos:definition>
    <skos:definition xml:lang="ko">
    대한민국의 도로명주소란 부여된 도로명, 기초번호, 건물번호, 상세주소에 의하여 건물의 주소를 표기하는
    방식으로 2014년부터 사용되고 있다.
    </skos:definition>
    <skos:prefLabel xml:lang="en">Road Name Address</skos:prefLabel>
    <skos:prefLabel xml:lang="ko">도로명주소</skos:prefLabel>
  </owl:Class>
  <owl:Class rdf:about="http://rdfs.co/juso/kr/SpecialAutonomousProvince">
    <dcterms:issued rdf:datatype="http://www.w3.org/2001/XMLSchema#date">2015-10-02+09:00</dcterms:issued>
    <dcterms:modified rdf:datatype="http://www.w3.org/2001/XMLSchema#date">2015-10-02+09:00</dcterms:modified>
    <rdfs:comment xml:lang="en">
    Jeju is the only special autonomous province in South Korea.
    </rdfs:comment>
    <rdfs:isDefinedBy rdf:resource="http://rdfs.co/juso/kr/"/>
    <rdfs:seeAlso rdf:resource="https://en.wikipedia.org/wiki/Provinces_of_South_Korea"/>
    <rdfs:seeAlso rdf:resource="https://ko.wikipedia.org/wiki/특별자치도"/>
    <rdfs:subClassOf rdf:resource="http://rdfs.co/juso/Province"/>
    <rdfs:subClassOf rdf:resource="http://rdfs.co/juso/kr/RegionalLocalGovernment"/>
    <owl:disjointWith rdf:resource="http://rdfs.co/juso/kr/Province"/>
    <status:term_status xml:lang="en">unstable</status:term_status>
    <skos:altLabel xml:lang="en">Special Self-governing Province</skos:altLabel>
    <skos:definition xml:lang="en">
    A special autonomous province is a province with more autonomy over its
    economy and more powers are given to the provincial government.
    </skos:definition>
    <skos:definition xml:lang="ko">
    특별자치도(特別自治道)는 대한민국의 행정 구역으로, 일반 도(道)와 기능적으로 거의 동일하지만,
    관련 법률에 의거해 고도의 자치권이 보장된다.
    </skos:definition>
    <skos:prefLabel xml:lang="en">Special Autonomous Province</skos:prefLabel>
    <skos:prefLabel xml:lang="ko">특별자치도</skos:prefLabel>
  </owl:Class>
  <owl:Class rdf:about="http://rdfs.co/juso/kr/SpecialCity">
    <dcterms:issued rdf:datatype="http://www.w3.org/2001/XMLSchema#date">2015-10-02+09:00</dcterms:issued>
    <dcterms:modified rdf:datatype="http://www.w3.org/2001/XMLSchema#date">2015-10-02+09:00</dcterms:modified>
    <rdfs:isDefinedBy rdf:resource="http://rdfs.co/juso/kr/"/>
    <rdfs:seeAlso rdf:resource="https://en.wikipedia.org/wiki/Special_cities_of_South_Korea"/>
    <rdfs:seeAlso rdf:resource="https://ko.wikipedia.org/wiki/특별시"/>
    <rdfs:subClassOf rdf:resource="http://rdfs.co/juso/City"/>
    <rdfs:subClassOf rdf:resource="http://rdfs.co/juso/kr/RegionalLocalGovernment"/>
    <owl:disjointWith rdf:resource="http://rdfs.co/juso/kr/MetropolitanAutonomousCity"/>
    <owl:disjointWith rdf:resource="http://rdfs.co/juso/kr/MetropolitanCity"/>
    <status:term_status xml:lang="en">unstable</status:term_status>
    <skos:definition xml:lang="en">
    Seoul was designated a "special free city" separate from Gyeonggi Province
    on August 15, 1946; it became a "special city" on August 15, 1949.
    </skos:definition>
    <skos:definition xml:lang="ko">
    특별시(特別市)는 대한민국의 행정 구역으로 서울특별시가 유일하다.
    </skos:definition>
    <skos:prefLabel xml:lang="en">Special City</skos:prefLabel>
    <skos:prefLabel xml:lang="ko">특별시</skos:prefLabel>
  </owl:Class>
  <owl:Class rdf:about="http://rdfs.co/juso/kr/SpecificCity">
    <dcterms:issued rdf:datatype="http://www.w3.org/2001/XMLSchema#date">2015-10-02+09:00</dcterms:issued>
    <dcterms:modified rdf:datatype="http://www.w3.org/2001/XMLSchema#date">2015-10-02+09:00</dcterms:modified>
    <rdfs:comment xml:lang="en">
    Specific city are given powers to subdivide themselves into non-autonomous
    districts but, not all Specific city are subdivided into non-autonomous
    districts.
  </rdfs:comment>
    <rdfs:isDefinedBy rdf:resource="http://rdfs.co/juso/kr/"/>
    <rdfs:seeAlso rdf:resource="https://en.wikipedia.org/wiki/Cities_of_South_Korea"/>
    <rdfs:seeAlso rdf:resource="https://ko.wikipedia.org/wiki/특정시"/>
    <rdfs:subClassOf rdf:resource="http://rdfs.co/juso/kr/City"/>
    <status:term_status xml:lang="en">unstable</status:term_status>
    <skos:definition xml:lang="en">
    A Specific city is a municipal city that has a population greater than
    500,000 and has been designated as such by an order of the National
    Government under Article 175 of the Local Autonomy Law.
    </skos:definition>
    <skos:definition xml:lang="ko">
    특정시(特定市)는 대한민국의 광역자치단체인 도에 소속된 기초자치단체 중 지방자치법 제175조에 따라
    도지사의 권한 일부가 시장에게 위임된 시를 비공식적으로 일컫는 명칭으로 지방자치법에서는 이를 인구
    50만 이상 대도시라고 규정하고 있다.
    </skos:definition>
    <skos:prefLabel xml:lang="en">Specific City</skos:prefLabel>
    <skos:prefLabel xml:lang="ko">특정시</skos:prefLabel>
  </owl:Class>
  <owl:Class rdf:about="http://rdfs.co/juso/kr/Street">
    <dcterms:issued rdf:datatype="http://www.w3.org/2001/XMLSchema#date">2015-10-02+09:00</dcterms:issued>
    <dcterms:modified rdf:datatype="http://www.w3.org/2001/XMLSchema#date">2015-10-02+09:00</dcterms:modified>
    <rdfs:isDefinedBy rdf:resource="http://rdfs.co/juso/kr/"/>
    <rdfs:seeAlso rdf:resource="https://ko.wikipedia.org/wiki/대한민국의_주소"/>
    <rdfs:subClassOf rdf:resource="http://rdfs.co/juso/Street"/>
    <status:term_status xml:lang="en">unstable</status:term_status>
    <skos:definition xml:lang="en">
    In the Road Name Address system, the word street (ro) is used to
    describe two-way roads that are narrower than roads but have more than 12m
    width or 2 lanes.
    </skos:definition>
    <skos:definition xml:lang="ko">
    도로명주소에서 로(路)는 대로보다 작지만 폭이 12m 이상이거나 왕복 2차선 이상의 도로를
    의미한다.
    </skos:definition>
    <skos:prefLabel xml:lang="en">Street</skos:prefLabel>
    <skos:prefLabel xml:lang="ko">로</skos:prefLabel>
  </owl:Class>
  <owl:Class rdf:about="http://rdfs.co/juso/kr/Town">
    <dcterms:issued rdf:datatype="http://www.w3.org/2001/XMLSchema#date">2015-10-02+09:00</dcterms:issued>
    <dcterms:modified rdf:datatype="http://www.w3.org/2001/XMLSchema#date">2015-10-02+09:00</dcterms:modified>
    <rdfs:comment xml:lang="en">
    Along with "township", a town is one of the divisions of a county, and of
    some cities with a population of less than 500,000. Towns are subdivided
    into villages.
    </rdfs:comment>
    <rdfs:isDefinedBy rdf:resource="http://rdfs.co/juso/kr/"/>
    <rdfs:seeAlso rdf:resource="https://en.wikipedia.org/wiki/Eup_(administrative_division)"/>
    <rdfs:seeAlso rdf:resource="https://ko.wikipedia.org/wiki/읍"/>
    <rdfs:subClassOf rdf:resource="http://rdfs.co/juso/ThirdLevelAdministrativeDivision"/>
    <rdfs:subClassOf rdf:resource="http://rdfs.co/juso/Town"/>
    <status:term_status xml:lang="en">unstable</status:term_status>
    <skos:definition xml:lang="en">
    A town is an administrative unit in South Korea.
    </skos:definition>
    <skos:definition xml:lang="ko">
    대한민국의 읍(邑)은 시·군·구의 하부 행정 구역이다.
    </skos:definition>
    <skos:prefLabel xml:lang="en">Town</skos:prefLabel>
    <skos:prefLabel xml:lang="ko">읍</skos:prefLabel>
  </owl:Class>
  <owl:Class rdf:about="http://rdfs.co/juso/kr/Township">
    <dcterms:issued rdf:datatype="http://www.w3.org/2001/XMLSchema#date">2015-10-02+09:00</dcterms:issued>
    <dcterms:modified rdf:datatype="http://www.w3.org/2001/XMLSchema#date">2015-10-02+09:00</dcterms:modified>
    <rdfs:comment xml:lang="en">
    Along with town, township is of a county and some cities of fewer than
    500,000 population. Townships have smaller populations than towns and
    represent the rural areas of a county or city. Townships are subdivided
    into villages.
    </rdfs:comment>
    <rdfs:isDefinedBy rdf:resource="http://rdfs.co/juso/kr/"/>
    <rdfs:seeAlso rdf:resource="https://en.wikipedia.org/wiki/Myeon_(administrative_division)"/>
    <rdfs:seeAlso rdf:resource="https://ko.wikipedia.org/wiki/면_(행정_구역)"/>
    <rdfs:subClassOf rdf:resource="http://rdfs.co/juso/ThirdLevelAdministrativeDivision"/>
    <rdfs:subClassOf rdf:resource="http://rdfs.co/juso/Township"/>
    <status:term_status xml:lang="en">unstable</status:term_status>
    <skos:definition xml:lang="en">
    A township is an administrative unit in South Korea.
    </skos:definition>
    <skos:definition xml:lang="ko">
    면(面)은 대한민국의 자치시·군 또는 행정시의 하부 행정 구역 이름이다.
    </skos:definition>
    <skos:prefLabel xml:lang="en">Township</skos:prefLabel>
    <skos:prefLabel xml:lang="ko">면</skos:prefLabel>
  </owl:Class>
  <owl:DatatypeProperty rdf:about="http://rdfs.co/juso/kr/administrative_building_number">
    <dcterms:issued rdf:datatype="http://www.w3.org/2001/XMLSchema#date">2015-10-02+09:00</dcterms:issued>
    <dcterms:modified rdf:datatype="http://www.w3.org/2001/XMLSchema#date">2015-10-02+09:00</dcterms:modified>
    <rdfs:domain rdf:resource="http://rdfs.co/juso/kr/Building"/>
    <rdfs:isDefinedBy rdf:resource="http://rdfs.co/juso/kr/"/>
    <rdfs:range rdf:resource="http://www.w3.org/2001/XMLSchema#string"/>
    <status:term_status xml:lang="en">unstable</status:term_status>
    <skos:definition xml:lang="en">
    Each building is given a number for administration.
    </skos:definition>
    <skos:definition xml:lang="ko">
    건물은 관리 번호를 부여 받는다.
    </skos:definition>
    <skos:prefLabel xml:lang="en">administrative building number</skos:prefLabel>
    <skos:prefLabel xml:lang="ko">건물 관리 번호</skos:prefLabel>
  </owl:DatatypeProperty>
  <owl:DatatypeProperty rdf:about="http://rdfs.co/juso/kr/administrative_neighborhood_code">
    <dcterms:issued rdf:datatype="http://www.w3.org/2001/XMLSchema#date">2015-10-02+09:00</dcterms:issued>
    <dcterms:modified rdf:datatype="http://www.w3.org/2001/XMLSchema#date">2015-10-02+09:00</dcterms:modified>
    <rdfs:domain rdf:resource="http://rdfs.co/juso/kr/AdministrativeNeighborhood"/>
    <rdfs:isDefinedBy rdf:resource="http://rdfs.co/juso/kr/"/>
    <rdfs:range rdf:resource="http://www.w3.org/2001/XMLSchema#string"/>
    <status:term_status xml:lang="en">unstable</status:term_status>
    <skos:definition xml:lang="en">
    The unique administrative code for the administrative neighborhood.
    </skos:definition>
    <skos:definition xml:lang="ko">
    행정동에 부여된 행정 표준 코드.
    </skos:definition>
    <skos:prefLabel xml:lang="en">administrative neighborhood code</skos:prefLabel>
    <skos:prefLabel xml:lang="ko">행정동코드</skos:prefLabel>
  </owl:DatatypeProperty>
  <owl:DatatypeProperty rdf:about="http://rdfs.co/juso/kr/beonji">
    <dcterms:issued rdf:datatype="http://www.w3.org/2001/XMLSchema#date">2015-10-02+09:00</dcterms:issued>
    <dcterms:modified rdf:datatype="http://www.w3.org/2001/XMLSchema#date">2015-10-02+09:00</dcterms:modified>
    <rdfs:domain rdf:resource="http://rdfs.co/juso/kr/EastAsianAddress"/>
    <rdfs:isDefinedBy rdf:resource="http://rdfs.co/juso/kr/"/>
    <rdfs:range rdf:resource="http://www.w3.org/2001/XMLSchema#string"/>
    <rdfs:seeAlso rdf:resource="https://ko.wikipedia.org/wiki/지번_(토지)"/>
    <status:term_status xml:lang="en">unstable</status:term_status>
    <skos:definition xml:lang="en">
    Each neighborhood is divided into city blocks (beonji), which can range
    from several dozen to several thousand per neighborhood.
    </skos:definition>
    <skos:definition xml:lang="ko">
    번지(番地)는 토지를 구획할 때 어떤 특정한 토지에 붙이는 번호를 의미하는 지번이다.
    </skos:definition>
    <skos:prefLabel xml:lang="en">beonji</skos:prefLabel>
    <skos:prefLabel xml:lang="ko">번지</skos:prefLabel>
  </owl:DatatypeProperty>
  <owl:DatatypeProperty rdf:about="http://rdfs.co/juso/kr/building_extra_number">
    <dcterms:issued rdf:datatype="http://www.w3.org/2001/XMLSchema#date">2015-10-02+09:00</dcterms:issued>
    <dcterms:modified rdf:datatype="http://www.w3.org/2001/XMLSchema#date">2015-10-02+09:00</dcterms:modified>
    <rdfs:domain rdf:resource="http://rdfs.co/juso/kr/RoadNameAddress"/>
    <rdfs:isDefinedBy rdf:resource="http://rdfs.co/juso/kr/"/>
    <rdfs:range rdf:resource="http://www.w3.org/2001/XMLSchema#string"/>
    <rdfs:seeAlso rdf:resource="https://en.wikipedia.org/wiki/Addresses_in_South_Korea"/>
    <rdfs:seeAlso rdf:resource="https://ko.wikipedia.org/wiki/대한민국의_주소"/>
    <rdfs:subPropertyOf rdf:resource="http://rdfs.co/juso/thoroughfare_address"/>
    <status:term_status xml:lang="en">unstable</status:term_status>
    <skos:altLabel xml:lang="ko">건물 부 번</skos:altLabel>
    <skos:definition xml:lang="en">
    Buildings on a street or alley that is too small or too short to receive
    a name of its own share the same building number, followed by a hyphen,
    followed by a unique extra number afterwards.
    </skos:definition>
    <skos:definition xml:lang="ko">
    건물 번호는 본 번과 부 번으로 구성되는데, 한 건물이 두 개의 도로와 인접해 있을 경우, 보다 넓은
    도로로 건물 번호를 부여하고, 한 구간 내 여러 건물이 위치하고 있을 경우 -1, -2, -3처럼 부
    번을 부여하여 본 번을 부여받은 건물과 구별한다.
    </skos:definition>
    <skos:prefLabel xml:lang="en">building extra number</skos:prefLabel>
    <skos:prefLabel xml:lang="ko">건물 부 번호</skos:prefLabel>
  </owl:DatatypeProperty>
  <owl:DatatypeProperty rdf:about="http://rdfs.co/juso/kr/building_number">
    <dcterms:issued rdf:datatype="http://www.w3.org/2001/XMLSchema#date">2015-10-02+09:00</dcterms:issued>
    <dcterms:modified rdf:datatype="http://www.w3.org/2001/XMLSchema#date">2015-10-02+09:00</dcterms:modified>
    <rdfs:domain rdf:resource="http://rdfs.co/juso/kr/RoadNameAddress"/>
    <rdfs:isDefinedBy rdf:resource="http://rdfs.co/juso/kr/"/>
    <rdfs:range rdf:resource="http://www.w3.org/2001/XMLSchema#string"/>
    <rdfs:seeAlso rdf:resource="https://en.wikipedia.org/wiki/Addresses_in_South_Korea"/>
    <rdfs:seeAlso rdf:resource="https://ko.wikipedia.org/wiki/대한민국의_주소"/>
    <rdfs:subPropertyOf rdf:resource="http://rdfs.co/juso/thoroughfare_address"/>
    <status:term_status xml:lang="en">unstable</status:term_status>
    <skos:altLabel xml:lang="en">building main number</skos:altLabel>
    <skos:altLabel xml:lang="ko">건물 본 번</skos:altLabel>
    <skos:altLabel xml:lang="ko">건물 본 번호</skos:altLabel>
    <skos:definition xml:lang="en">
    Buildings are numbered along a street with even numbers on one side and odd
    numbers on the other, as in most European countries.
    </skos:definition>
    <skos:definition xml:lang="ko">
    건물 번호는 건물마다 부여된 번호로 건물번호 도로의 시작점으로부터 왼편에는 홀수를, 오른편에는 짝수를
    대로(Boulevard) 및 로(Street)의 경우 매20미터마다, 길(Road)의 경우 매10미터마다 2씩
    증가시키면서 부여한다.
    </skos:definition>
    <skos:prefLabel xml:lang="en">building number</skos:prefLabel>
    <skos:prefLabel xml:lang="ko">건물 번호</skos:prefLabel>
  </owl:DatatypeProperty>
  <owl:DatatypeProperty rdf:about="http://rdfs.co/juso/kr/congnamul_x">
    <dcterms:issued rdf:datatype="http://www.w3.org/2001/XMLSchema#date">2015-11-10+09:00</dcterms:issued>
    <dcterms:modified rdf:datatype="http://www.w3.org/2001/XMLSchema#date">2015-11-10+09:00</dcterms:modified>
    <rdfs:domain rdf:resource="http://rdfs.co/juso/Point"/>
    <rdfs:isDefinedBy rdf:resource="http://rdfs.co/juso/kr/"/>
    <rdfs:range rdf:resource="http://www.w3.org/2001/XMLSchema#string"/>
    <status:term_status xml:lang="en">unstable</status:term_status>
    <skos:definition xml:lang="en">
    The x coordinate of a point in the Congnamul coordination system.
    </skos:definition>
    <skos:definition xml:lang="ko">
    콩나물 지도와 다음 지도에서 사용하는 좌표계의 x 좌표.
    </skos:definition>
    <skos:prefLabel xml:lang="en">x coordinate (Congnamul)</skos:prefLabel>
    <skos:prefLabel xml:lang="ko">x 좌표(Congnamul)</skos:prefLabel>
  </owl:DatatypeProperty>
  <owl:DatatypeProperty rdf:about="http://rdfs.co/juso/kr/congnamul_y">
    <dcterms:issued rdf:datatype="http://www.w3.org/2001/XMLSchema#date">2015-11-10+09:00</dcterms:issued>
    <dcterms:modified rdf:datatype="http://www.w3.org/2001/XMLSchema#date">2015-11-10+09:00</dcterms:modified>
    <rdfs:domain rdf:resource="http://rdfs.co/juso/Point"/>
    <rdfs:isDefinedBy rdf:resource="http://rdfs.co/juso/kr/"/>
    <rdfs:range rdf:resource="http://www.w3.org/2001/XMLSchema#string"/>
    <status:term_status xml:lang="en">unstable</status:term_status>
    <skos:definition xml:lang="en">
    The y coordinate of a point in the Congnamul coordination system.
    </skos:definition>
    <skos:definition xml:lang="ko">
    콩나물 지도와 다음 지도에서 사용하는 좌표계의 y 좌표.
    </skos:definition>
    <skos:prefLabel xml:lang="en">y coordinate (Congnamul)</skos:prefLabel>
    <skos:prefLabel xml:lang="ko">y 좌표(Congnamul)</skos:prefLabel>
  </owl:DatatypeProperty>
  <owl:ObjectProperty rdf:about="http://rdfs.co/juso/kr/eup_myeon_dong">
    <dcterms:issued rdf:datatype="http://www.w3.org/2001/XMLSchema#date">2015-10-02+09:00</dcterms:issued>
    <dcterms:modified rdf:datatype="http://www.w3.org/2001/XMLSchema#date">2015-10-02+09:00</dcterms:modified>
    <rdfs:domain>
      <owl:Class>
        <owl:unionOf>
          <rdf:Description>
            <rdf:first rdf:resource="http://rdfs.co/juso/kr/EastAsianAddress"/>
            <rdf:rest>
              <rdf:Description>
                <rdf:first rdf:resource="http://rdfs.co/juso/kr/RoadNameAddress"/>
                <rdf:rest rdf:resource="http://www.w3.org/1999/02/22-rdf-syntax-ns#nil"/>
              </rdf:Description>
            </rdf:rest>
          </rdf:Description>
        </owl:unionOf>
      </owl:Class>
    </rdfs:domain>
    <rdfs:isDefinedBy rdf:resource="http://rdfs.co/juso/kr/"/>
    <rdfs:range>
      <owl:Class>
        <owl:unionOf>
          <rdf:Description>
            <rdf:first rdf:resource="http://rdfs.co/juso/kr/Town"/>
            <rdf:rest>
              <rdf:Description>
                <rdf:first rdf:resource="http://rdfs.co/juso/kr/Township"/>
                <rdf:rest>
                  <rdf:Description>
                    <rdf:first rdf:resource="http://rdfs.co/juso/kr/LegalStatusNeighborhood"/>
                    <rdf:rest>
                      <rdf:Description>
                        <rdf:first rdf:resource="http://rdfs.co/juso/kr/AdministrativeNeighborhood"/>
                        <rdf:rest rdf:resource="http://www.w3.org/1999/02/22-rdf-syntax-ns#nil"/>
                      </rdf:Description>
                    </rdf:rest>
                  </rdf:Description>
                </rdf:rest>
              </rdf:Description>
            </rdf:rest>
          </rdf:Description>
        </owl:unionOf>
      </owl:Class>
    </rdfs:range>
    <rdfs:subPropertyOf rdf:resource="http://rdfs.co/juso/third_level_administrative_division"/>
    <status:term_status xml:lang="en">unstable</status:term_status>
    <skos:definition xml:lang="en">
    The third-level administrative division of the address in South Korea,
    one of the four types of submunicipal-level divisions: towns (eup),
    townships (myeon), legal-status neighborhoods (beopjeongdong), and
    administrative neighborhoods (haengjeongdong).
    </skos:definition>
    <skos:definition xml:lang="ko">
    대한민국 주소의 읍면동급 행정 구역으로 읍, 면, 법정동, 행정동 중 하나에 해당한다.
    </skos:definition>
    <skos:prefLabel xml:lang="en">town, township, or neighborhood</skos:prefLabel>
    <skos:prefLabel xml:lang="ko">읍/면/동</skos:prefLabel>
  </owl:ObjectProperty>
  <owl:DatatypeProperty rdf:about="http://rdfs.co/juso/kr/eup_myeon_dong_code">
    <dcterms:issued rdf:datatype="http://www.w3.org/2001/XMLSchema#date">2015-10-02+09:00</dcterms:issued>
    <dcterms:modified rdf:datatype="http://www.w3.org/2001/XMLSchema#date">2015-10-02+09:00</dcterms:modified>
    <rdfs:domain>
      <owl:Class>
        <owl:unionOf>
          <rdf:Description>
            <rdf:first rdf:resource="http://rdfs.co/juso/kr/Town"/>
            <rdf:rest>
              <rdf:Description>
                <rdf:first rdf:resource="http://rdfs.co/juso/kr/Township"/>
                <rdf:rest>
                  <rdf:Description>
                    <rdf:first rdf:resource="http://rdfs.co/juso/kr/LegalStatusNeighborhood"/>
                    <rdf:rest>
                      <rdf:Description>
                        <rdf:first rdf:resource="http://rdfs.co/juso/kr/AdministrativeNeighborhood"/>
                        <rdf:rest rdf:resource="http://www.w3.org/1999/02/22-rdf-syntax-ns#nil"/>
                      </rdf:Description>
                    </rdf:rest>
                  </rdf:Description>
                </rdf:rest>
              </rdf:Description>
            </rdf:rest>
          </rdf:Description>
        </owl:unionOf>
      </owl:Class>
    </rdfs:domain>
    <rdfs:isDefinedBy rdf:resource="http://rdfs.co/juso/kr/"/>
    <rdfs:range rdf:resource="http://www.w3.org/2001/XMLSchema#string"/>
    <rdfs:seeAlso rdf:resource="https://ko.wikipedia.org/wiki/대한민국의_주소"/>
    <status:term_status xml:lang="en">unstable</status:term_status>
    <skos:definition xml:lang="en">
    Each of towns (eup), townships (myeon), or neighborhoods (dong) is given a
    3-number code.
    </skos:definition>
    <skos:definition xml:lang="ko">
    읍, 면, 동은 3자리 코드를 부여 받는다.
    </skos:definition>
    <skos:prefLabel xml:lang="en">code for town, township, neighborhood</skos:prefLabel>
    <skos:prefLabel xml:lang="ko">읍면동 코드</skos:prefLabel>
  </owl:DatatypeProperty>
  <owl:DatatypeProperty rdf:about="http://rdfs.co/juso/kr/eup_myeon_dong_serial_number">
    <dcterms:issued rdf:datatype="http://www.w3.org/2001/XMLSchema#date">2015-10-02+09:00</dcterms:issued>
    <dcterms:modified rdf:datatype="http://www.w3.org/2001/XMLSchema#date">2015-10-02+09:00</dcterms:modified>
    <rdfs:domain rdf:resource="http://rdfs.co/juso/kr/RoadNameAddress"/>
    <rdfs:isDefinedBy rdf:resource="http://rdfs.co/juso/kr/"/>
    <rdfs:range rdf:resource="http://www.w3.org/2001/XMLSchema#string"/>
    <status:term_status xml:lang="en">unstable</status:term_status>
    <skos:definition xml:lang="en">
    A serial number for town, township, or neighborhood to distinguish
    addresses that share the same code for city, county, or district, and
    the same road name number.
    </skos:definition>
    <skos:definition xml:lang="ko">
    시군구 코드와 도로명 번호가 중복되는 주소를 구분하기 위한 읍면동 일련 번호.
    </skos:definition>
    <skos:prefLabel xml:lang="en">serial number for town, township, or neighborhood</skos:prefLabel>
    <skos:prefLabel xml:lang="ko">읍면동 일련 번호</skos:prefLabel>
  </owl:DatatypeProperty>
  <owl:ObjectProperty rdf:about="http://rdfs.co/juso/kr/floor">
    <dcterms:issued rdf:datatype="http://www.w3.org/2001/XMLSchema#date">2015-10-02+09:00</dcterms:issued>
    <dcterms:modified rdf:datatype="http://www.w3.org/2001/XMLSchema#date">2015-10-02+09:00</dcterms:modified>
    <rdfs:domain rdf:resource="http://rdfs.co/juso/kr/RoadNameAddress"/>
    <rdfs:isDefinedBy rdf:resource="http://rdfs.co/juso/kr/"/>
    <rdfs:range>
      <owl:Class>
        <owl:oneOf>
          <rdf:Description>
            <rdf:first rdf:resource="http://dbpedia.org/resource/Storey"/>
            <rdf:rest>
              <rdf:Description>
                <rdf:first rdf:resource="http://dbpedia.org/resource/Basement"/>
                <rdf:rest>
                  <rdf:Description>
                    <rdf:first rdf:resource="http://dbpedia.org/resource/Sky"/>
                    <rdf:rest rdf:resource="http://www.w3.org/1999/02/22-rdf-syntax-ns#nil"/>
                  </rdf:Description>
                </rdf:rest>
              </rdf:Description>
            </rdf:rest>
          </rdf:Description>
        </owl:oneOf>
      </owl:Class>
    </rdfs:range>
    <status:term_status xml:lang="en">unstable</status:term_status>
    <skos:definition xml:lang="en">
    Whether the address locates a place on the ground, under the ground, or in
    the air.
    </skos:definition>
    <skos:definition xml:lang="ko">
    주소가 가리키는 곳이 지상인지, 지하인지, 공중인지 여부.
    </skos:definition>
    <skos:prefLabel xml:lang="en">floor</skos:prefLabel>
    <skos:prefLabel xml:lang="ko">층 구분</skos:prefLabel>
  </owl:ObjectProperty>
  <owl:DatatypeProperty rdf:about="http://rdfs.co/juso/kr/ho">
    <dcterms:issued rdf:datatype="http://www.w3.org/2001/XMLSchema#date">2015-10-02+09:00</dcterms:issued>
    <dcterms:modified rdf:datatype="http://www.w3.org/2001/XMLSchema#date">2015-10-02+09:00</dcterms:modified>
    <rdfs:comment xml:lang="en">
    Usually, the words "번지" and "호" are not included in the written address;
    instead, only their numbers, separated by a hyphen, are written.
    </rdfs:comment>
    <rdfs:domain rdf:resource="http://rdfs.co/juso/kr/EastAsianAddress"/>
    <rdfs:isDefinedBy rdf:resource="http://rdfs.co/juso/kr/"/>
    <rdfs:range rdf:resource="http://www.w3.org/2001/XMLSchema#string"/>
    <rdfs:seeAlso rdf:resource="https://en.wikipedia.org/wiki/House_numbering"/>
    <rdfs:seeAlso rdf:resource="https://ko.wikipedia.org/wiki/지번_(토지)"/>
    <status:term_status xml:lang="en">unstable</status:term_status>
    <skos:definition xml:lang="en">
    The building itself is given a house number (ho) within the city block.
    </skos:definition>
    <skos:definition xml:lang="ko">
    호(戶)는 건물에 부여된 각 번지 내 건물 번호이다.
    </skos:definition>
    <skos:prefLabel xml:lang="en">ho</skos:prefLabel>
    <skos:prefLabel xml:lang="ko">호</skos:prefLabel>
  </owl:DatatypeProperty>
  <owl:ObjectProperty rdf:about="http://rdfs.co/juso/kr/landform">
    <dcterms:issued rdf:datatype="http://www.w3.org/2001/XMLSchema#date">2015-10-02+09:00</dcterms:issued>
    <dcterms:modified rdf:datatype="http://www.w3.org/2001/XMLSchema#date">2015-10-02+09:00</dcterms:modified>
    <rdfs:domain rdf:resource="http://rdfs.co/juso/kr/RoadNameAddress"/>
    <rdfs:isDefinedBy rdf:resource="http://rdfs.co/juso/kr/"/>
    <rdfs:range>
      <owl:Class>
        <owl:oneOf>
          <rdf:Description>
            <rdf:first rdf:resource="http://dbpedia.org/resource/Land_lot"/>
            <rdf:rest>
              <rdf:Description>
                <rdf:first rdf:resource="http://dbpedia.org/resource/Mountain"/>
                <rdf:rest rdf:resource="http://www.w3.org/1999/02/22-rdf-syntax-ns#nil"/>
              </rdf:Description>
            </rdf:rest>
          </rdf:Description>
        </owl:oneOf>
      </owl:Class>
    </rdfs:range>
    <status:term_status xml:lang="en">unstable</status:term_status>
    <skos:definition xml:lang="en">
    Whether the address locates a land lot or a mountain.
    </skos:definition>
    <skos:definition xml:lang="ko">
    주소 필지의 산 여부.
    </skos:definition>
    <skos:prefLabel xml:lang="en">landform</skos:prefLabel>
    <skos:prefLabel xml:lang="ko">필지 구분</skos:prefLabel>
  </owl:ObjectProperty>
  <owl:DatatypeProperty rdf:about="http://rdfs.co/juso/kr/legal_status_neighborhood_code">
    <dcterms:issued rdf:datatype="http://www.w3.org/2001/XMLSchema#date">2015-10-02+09:00</dcterms:issued>
    <dcterms:modified rdf:datatype="http://www.w3.org/2001/XMLSchema#date">2015-10-02+09:00</dcterms:modified>
    <rdfs:domain rdf:resource="http://rdfs.co/juso/kr/LegalStatusNeighborhood"/>
    <rdfs:isDefinedBy rdf:resource="http://rdfs.co/juso/kr/"/>
    <rdfs:range rdf:resource="http://www.w3.org/2001/XMLSchema#string"/>
    <status:term_status xml:lang="en">unstable</status:term_status>
    <skos:definition xml:lang="en">
    The unique administrative code for the legal-status neighborhood.
    </skos:definition>
    <skos:definition xml:lang="ko">
    법정동에 부여된 행정 표준 코드.
    </skos:definition>
    <skos:prefLabel xml:lang="en">legal-status neighborhood code</skos:prefLabel>
    <skos:prefLabel xml:lang="ko">법정동코드</skos:prefLabel>
  </owl:DatatypeProperty>
  <owl:ObjectProperty rdf:about="http://rdfs.co/juso/kr/parent_road">
    <dcterms:issued rdf:datatype="http://www.w3.org/2001/XMLSchema#date">2015-10-02+09:00</dcterms:issued>
    <dcterms:modified rdf:datatype="http://www.w3.org/2001/XMLSchema#date">2015-10-02+09:00</dcterms:modified>
    <rdfs:domain>
      <owl:Class>
        <owl:unionOf>
          <rdf:Description>
            <rdf:first rdf:resource="http://rdfs.co/juso/kr/Boulevard"/>
            <rdf:rest>
              <rdf:Description>
                <rdf:first rdf:resource="http://rdfs.co/juso/kr/Street"/>
                <rdf:rest>
                  <rdf:Description>
                    <rdf:first rdf:resource="http://rdfs.co/juso/kr/Road"/>
                    <rdf:rest rdf:resource="http://www.w3.org/1999/02/22-rdf-syntax-ns#nil"/>
                  </rdf:Description>
                </rdf:rest>
              </rdf:Description>
            </rdf:rest>
          </rdf:Description>
        </owl:unionOf>
      </owl:Class>
    </rdfs:domain>
    <rdfs:isDefinedBy rdf:resource="http://rdfs.co/juso/kr/"/>
    <rdfs:range>
      <owl:Class>
        <owl:unionOf>
          <rdf:Description>
            <rdf:first rdf:resource="http://rdfs.co/juso/kr/Boulevard"/>
            <rdf:rest>
              <rdf:Description>
                <rdf:first rdf:resource="http://rdfs.co/juso/kr/Street"/>
                <rdf:rest>
                  <rdf:Description>
                    <rdf:first rdf:resource="http://rdfs.co/juso/kr/Road"/>
                    <rdf:rest rdf:resource="http://www.w3.org/1999/02/22-rdf-syntax-ns#nil"/>
                  </rdf:Description>
                </rdf:rest>
              </rdf:Description>
            </rdf:rest>
          </rdf:Description>
        </owl:unionOf>
      </owl:Class>
    </rdfs:range>
    <rdfs:subPropertyOf rdf:resource="http://www.geonames.org/ontology#parentFeature"/>
    <status:term_status xml:lang="en">unstable</status:term_status>
    <skos:definition xml:lang="en">
    A boulevard, street, or road that is a direct parent of the current one.
    </skos:definition>
    <skos:definition xml:lang="ko">
    이 도로의 상위에 있는 대로, 로, 길.
    </skos:definition>
    <skos:prefLabel xml:lang="en">parent boulevard, street, or road</skos:prefLabel>
    <skos:prefLabel xml:lang="ko">상위 도로</skos:prefLabel>
  </owl:ObjectProperty>
  <owl:ObjectProperty rdf:about="http://rdfs.co/juso/kr/ri">
    <dcterms:issued rdf:datatype="http://www.w3.org/2001/XMLSchema#date">2015-10-02+09:00</dcterms:issued>
    <dcterms:modified rdf:datatype="http://www.w3.org/2001/XMLSchema#date">2015-10-02+09:00</dcterms:modified>
    <rdfs:domain>
      <owl:Class>
        <owl:unionOf>
          <rdf:Description>
            <rdf:first rdf:resource="http://rdfs.co/juso/kr/EastAsianAddress"/>
            <rdf:rest>
              <rdf:Description>
                <rdf:first rdf:resource="http://rdfs.co/juso/kr/RoadNameAddress"/>
                <rdf:rest rdf:resource="http://www.w3.org/1999/02/22-rdf-syntax-ns#nil"/>
              </rdf:Description>
            </rdf:rest>
          </rdf:Description>
        </owl:unionOf>
      </owl:Class>
    </rdfs:domain>
    <rdfs:isDefinedBy rdf:resource="http://rdfs.co/juso/kr/"/>
    <rdfs:range>
      <owl:Class>
        <owl:unionOf>
          <rdf:Description>
            <rdf:first rdf:resource="http://rdfs.co/juso/kr/LegalStatusVillage"/>
            <rdf:rest>
              <rdf:Description>
                <rdf:first rdf:resource="http://rdfs.co/juso/kr/AdministrativeVillage"/>
                <rdf:rest rdf:resource="http://www.w3.org/1999/02/22-rdf-syntax-ns#nil"/>
              </rdf:Description>
            </rdf:rest>
          </rdf:Description>
        </owl:unionOf>
      </owl:Class>
    </rdfs:range>
    <rdfs:subPropertyOf rdf:resource="http://rdfs.co/juso/fourth_level_administrative_division"/>
    <status:term_status xml:lang="en">unstable</status:term_status>
    <skos:definition xml:lang="en">
    A legal-status village (beopjeongri) or administrative village
    (haengjeongri) for the fourth-level administrative division of the address
    in South Korea.
    </skos:definition>
    <skos:definition xml:lang="ko">
    대한민국 주소의 리통급 행정 구역 중 현재는 거의 사용되지 않는 통을 제외한 법정리 또는 행정리에
    해당한다.
    </skos:definition>
    <skos:prefLabel xml:lang="en">village</skos:prefLabel>
    <skos:prefLabel xml:lang="ko">리</skos:prefLabel>
  </owl:ObjectProperty>
  <owl:DatatypeProperty rdf:about="http://rdfs.co/juso/kr/road_name_number">
    <dcterms:issued rdf:datatype="http://www.w3.org/2001/XMLSchema#date">2015-10-02+09:00</dcterms:issued>
    <dcterms:modified rdf:datatype="http://www.w3.org/2001/XMLSchema#date">2015-10-02+09:00</dcterms:modified>
    <rdfs:domain>
      <owl:Class>
        <owl:unionOf>
          <rdf:Description>
            <rdf:first rdf:resource="http://rdfs.co/juso/kr/Boulevard"/>
            <rdf:rest>
              <rdf:Description>
                <rdf:first rdf:resource="http://rdfs.co/juso/kr/Street"/>
                <rdf:rest>
                  <rdf:Description>
                    <rdf:first rdf:resource="http://rdfs.co/juso/kr/Road"/>
                    <rdf:rest rdf:resource="http://www.w3.org/1999/02/22-rdf-syntax-ns#nil"/>
                  </rdf:Description>
                </rdf:rest>
              </rdf:Description>
            </rdf:rest>
          </rdf:Description>
        </owl:unionOf>
      </owl:Class>
    </rdfs:domain>
    <rdfs:isDefinedBy rdf:resource="http://rdfs.co/juso/kr/"/>
    <rdfs:range rdf:resource="http://www.w3.org/2001/XMLSchema#string"/>
    <rdfs:seeAlso rdf:resource="https://ko.wikipedia.org/wiki/대한민국의_주소"/>
    <status:term_status xml:lang="en">unstable</status:term_status>
    <skos:definition xml:lang="en">
    Each of boulevards, streets, or roads is given a 7-number code.
    </skos:definition>
    <skos:definition xml:lang="ko">
    대로, 로, 길은 7자리 코드를 부여 받는다.
    </skos:definition>
    <skos:prefLabel xml:lang="en">road name number</skos:prefLabel>
    <skos:prefLabel xml:lang="ko">도로명 번호</skos:prefLabel>
  </owl:DatatypeProperty>
  <owl:ObjectProperty rdf:about="http://rdfs.co/juso/kr/si_do">
    <dcterms:issued rdf:datatype="http://www.w3.org/2001/XMLSchema#date">2015-10-02+09:00</dcterms:issued>
    <dcterms:modified rdf:datatype="http://www.w3.org/2001/XMLSchema#date">2015-10-02+09:00</dcterms:modified>
    <rdfs:domain>
      <owl:Class>
        <owl:unionOf>
          <rdf:Description>
            <rdf:first rdf:resource="http://rdfs.co/juso/kr/EastAsianAddress"/>
            <rdf:rest>
              <rdf:Description>
                <rdf:first rdf:resource="http://rdfs.co/juso/kr/RoadNameAddress"/>
                <rdf:rest rdf:resource="http://www.w3.org/1999/02/22-rdf-syntax-ns#nil"/>
              </rdf:Description>
            </rdf:rest>
          </rdf:Description>
        </owl:unionOf>
      </owl:Class>
    </rdfs:domain>
    <rdfs:isDefinedBy rdf:resource="http://rdfs.co/juso/kr/"/>
    <rdfs:range rdf:resource="http://rdfs.co/juso/kr/RegionalLocalGovernment"/>
    <rdfs:subPropertyOf rdf:resource="http://rdfs.co/juso/first_level_administrative_division"/>
    <status:term_status xml:lang="en">unstable</status:term_status>
    <skos:definition xml:lang="en">
    The top tier of administrative division of the address in South Korea,
    one of the five types of provincial-level divisions: provinces (do),
    special autonomous provinces (teukbyeol-jachido), special cities
    (teukbyeolsi), metropolitan cities (gwangyeoksi) and metropolitan
    autonomous cities (teukbyeol-jachisi).
    </skos:definition>
    <skos:definition xml:lang="ko">
    대한민국 주소의 시도급 행정 구역으로 1개의 특별시, 6개의 광역시, 8개의 도, 1개의 특별자치시,
    1개의 특별자치도 중 하나에 해당한다.
    </skos:definition>
    <skos:prefLabel xml:lang="en">city or province</skos:prefLabel>
    <skos:prefLabel xml:lang="ko">시/도</skos:prefLabel>
  </owl:ObjectProperty>
  <owl:ObjectProperty rdf:about="http://rdfs.co/juso/kr/si_gun_gu">
    <dcterms:issued rdf:datatype="http://www.w3.org/2001/XMLSchema#date">2015-10-02+09:00</dcterms:issued>
    <dcterms:modified rdf:datatype="http://www.w3.org/2001/XMLSchema#date">2015-10-02+09:00</dcterms:modified>
    <rdfs:domain>
      <owl:Class>
        <owl:unionOf>
          <rdf:Description>
            <rdf:first rdf:resource="http://rdfs.co/juso/kr/EastAsianAddress"/>
            <rdf:rest>
              <rdf:Description>
                <rdf:first rdf:resource="http://rdfs.co/juso/kr/RoadNameAddress"/>
                <rdf:rest rdf:resource="http://www.w3.org/1999/02/22-rdf-syntax-ns#nil"/>
              </rdf:Description>
            </rdf:rest>
          </rdf:Description>
        </owl:unionOf>
      </owl:Class>
    </rdfs:domain>
    <rdfs:isDefinedBy rdf:resource="http://rdfs.co/juso/kr/"/>
    <rdfs:range>
      <owl:Class>
        <owl:unionOf>
          <rdf:Description>
            <rdf:first rdf:resource="http://rdfs.co/juso/kr/BasicLocalGovernment"/>
            <rdf:rest>
              <rdf:Description>
                <rdf:first rdf:resource="http://rdfs.co/juso/kr/NonAutonomousDistrict"/>
                <rdf:rest rdf:resource="http://www.w3.org/1999/02/22-rdf-syntax-ns#nil"/>
              </rdf:Description>
            </rdf:rest>
          </rdf:Description>
        </owl:unionOf>
      </owl:Class>
    </rdfs:range>
    <rdfs:subPropertyOf rdf:resource="http://rdfs.co/juso/second_level_administrative_division"/>
    <status:term_status xml:lang="en">unstable</status:term_status>
    <skos:definition xml:lang="en">
    The second-level administrative division of the address in South Korea,
    one of the six types of municipal-level divisions: cities (si), specific
    cities (teukjeongsi), administrative cities (haengjeongsi), county (gun),
    autonomous districts (jachigu), and non-autonomous districts (ilbangu).
    </skos:definition>
    <skos:definition xml:lang="ko">
    대한민국 주소의 시군구급 행정 구역으로 시, 특정시, 행정시, 군, 자치구, 일반구 중 하나에
    해당한다.
    </skos:definition>
    <skos:prefLabel xml:lang="en">city, county, or district</skos:prefLabel>
    <skos:prefLabel xml:lang="ko">시/군/구</skos:prefLabel>
  </owl:ObjectProperty>
  <owl:DatatypeProperty rdf:about="http://rdfs.co/juso/kr/si_gun_gu_code">
    <dcterms:issued rdf:datatype="http://www.w3.org/2001/XMLSchema#date">2015-10-02+09:00</dcterms:issued>
    <dcterms:modified rdf:datatype="http://www.w3.org/2001/XMLSchema#date">2015-10-02+09:00</dcterms:modified>
    <rdfs:domain>
      <owl:Class>
        <owl:unionOf>
          <rdf:Description>
            <rdf:first rdf:resource="http://rdfs.co/juso/kr/BasicLocalGovernment"/>
            <rdf:rest>
              <rdf:Description>
                <rdf:first rdf:resource="http://rdfs.co/juso/kr/NonAutonomousDistrict"/>
                <rdf:rest rdf:resource="http://www.w3.org/1999/02/22-rdf-syntax-ns#nil"/>
              </rdf:Description>
            </rdf:rest>
          </rdf:Description>
        </owl:unionOf>
      </owl:Class>
    </rdfs:domain>
    <rdfs:isDefinedBy rdf:resource="http://rdfs.co/juso/kr/"/>
    <rdfs:range rdf:resource="http://www.w3.org/2001/XMLSchema#string"/>
    <rdfs:seeAlso rdf:resource="https://ko.wikipedia.org/wiki/대한민국의_주소"/>
    <status:term_status xml:lang="en">unstable</status:term_status>
    <skos:definition xml:lang="en">
    Each of cities (si), counties (gun), or districts (gu) is given a 5-number
    code.
    </skos:definition>
    <skos:definition xml:lang="ko">
    시, 군, 구는 5자리 코드를 부여받는다.
    </skos:definition>
    <skos:prefLabel xml:lang="en">code for city, county, or district</skos:prefLabel>
    <skos:prefLabel xml:lang="ko">시군구 코드</skos:prefLabel>
  </owl:DatatypeProperty>
</rdf:RDF>
