<rdf:RDF
    xmlns:aat_term="http://vocab.getty.edu/aat/term/"
    xmlns:wgs="http://www.w3.org/2003/01/geo/wgs84_pos#"
    xmlns:bio="http://purl.org/vocab/bio/0.1/"
    xmlns:tgn_source="http://vocab.getty.edu/tgn/source/"
    xmlns:gvp="http://vocab.getty.edu/ontology#"
    xmlns:aat_source_rev="http://vocab.getty.edu/aat/source/rev/"
    xmlns:iso="http://purl.org/iso25964/skos-thes#"
    xmlns:tgn_scopeNote="http://vocab.getty.edu/tgn/scopeNote/"
    xmlns:ulan_rel="http://vocab.getty.edu/ulan/rel/"
    xmlns:vdpp="http://data.lirmm.fr/ontologies/vdpp#"
    xmlns:dct="http://purl.org/dc/terms/"
    xmlns:voag="http://voag.linkedmodel.org/voag#"
    xmlns:ulan_source="http://vocab.getty.edu/ulan/source/"
    xmlns:prov="http://www.w3.org/ns/prov#"
    xmlns:aat_source="http://vocab.getty.edu/aat/source/"
    xmlns:sd="http://www.w3.org/ns/sparql-service-description#"
    xmlns:vann="http://purl.org/vocab/vann/"
    xmlns:xsd="http://www.w3.org/2001/XMLSchema#"
    xmlns:aat="http://vocab.getty.edu/aat/"
    xmlns:ulan="http://vocab.getty.edu/ulan/"
    xmlns:wdrs="http://www.w3.org/2007/05/powder-s#"
    xmlns:tgn_rel="http://vocab.getty.edu/tgn/rel/"
    xmlns:rdfs="http://www.w3.org/2000/01/rdf-schema#"
    xmlns:aat_rev="http://vocab.getty.edu/aat/rev/"
    xmlns:rr="http://www.w3.org/ns/r2rml#"
    xmlns:fmt="http://www.w3.org/ns/formats/"
    xmlns:tgn="http://vocab.getty.edu/tgn/"
    xmlns:aat_scopeNote="http://vocab.getty.edu/aat/scopeNote/"
    xmlns:vaem="http://www.linkedmodel.org/schema/vaem#"
    xmlns:ulan_source_rev="http://vocab.getty.edu/ulan/source/rev/"
    xmlns:ulan_term="http://vocab.getty.edu/ulan/term/"
    xmlns:owl="http://www.w3.org/2002/07/owl#"
    xmlns:tgn_term="http://vocab.getty.edu/tgn/term/"
    xmlns:ulan_bio="http://vocab.getty.edu/ulan/bio/"
    xmlns:bibo="http://purl.org/ontology/bibo/"
    xmlns:gvp_lang="http://vocab.getty.edu/language/"
    xmlns:tgn_source_rev="http://vocab.getty.edu/tgn/source/rev/"
    xmlns:skosxl="http://www.w3.org/2008/05/skos-xl#"
    xmlns:rrx="http://purl.org/r2rml-ext/"
    xmlns:tgn_contrib="http://vocab.getty.edu/tgn/contrib/"
    xmlns:luc="http://www.ontotext.com/owlim/lucene#"
    xmlns:ulan_contrib="http://vocab.getty.edu/ulan/contrib/"
    xmlns:ptop="http://www.ontotext.com/proton/protontop#"
    xmlns:ontogeo="http://www.ontotext.com/owlim/geo#"
    xmlns:voaf="http://purl.org/vocommons/voaf#"
    xmlns:sesame="http://www.openrdf.org/schema/sesame#"
    xmlns:dc="http://purl.org/dc/elements/1.1/"
    xmlns:adms="http://www.w3.org/ns/adms#"
    xmlns:aat_contrib="http://vocab.getty.edu/aat/contrib/"
    xmlns:skos="http://www.w3.org/2004/02/skos/core#"
    xmlns:ulan_scopeNote="http://vocab.getty.edu/ulan/scopeNote/"
    xmlns:cc="http://creativecommons.org/ns#"
    xmlns:tgn_rev="http://vocab.getty.edu/tgn/rev/"
    xmlns:rdf="http://www.w3.org/1999/02/22-rdf-syntax-ns#"
    xmlns:schema="http://schema.org/"
    xmlns:void="http://rdfs.org/ns/void#"
    xmlns:aat_rel="http://vocab.getty.edu/aat/rel/"
    xmlns:ulan_event="http://vocab.getty.edu/ulan/event/"
    xmlns:dctype="http://purl.org/dc/dcmitype/"
    xmlns:vcard="http://www.w3.org/2006/vcard/ns#"
    xmlns:wv="http://vocab.org/waiver/terms/"
    xmlns:dcat="http://www.w3.org/ns/dcat#"
    xmlns:ulan_rev="http://vocab.getty.edu/ulan/rev/"
    xmlns:foaf="http://xmlns.com/foaf/0.1/">
  <owl:Ontology rdf:about="http://vocab.getty.edu/ontology">
    <rdfs:seeAlso rdf:resource="http://vocab.getty.edu/.well-known/void"/>
    <rdfs:comment>The GVP Ontology defines classes, properties and values (skos:Concepts) used in GVP LOD.
As of version 3.0, it is complete regarding AAT, TGN and ULAN, and will be extended in time with more elements needed for other GVP vocabularies (CONA).
It uses the SKOS, SKOS-XL, ISO 25964; DC, DCT, BIBO, FOAF, BIO, Schema, PROV, WGS84 ontologies, but we import only the first 3</rdfs:comment>
    <owl:imports rdf:resource="http://www.w3.org/2004/02/skos/core"/>
    <vann:preferredNamespacePrefix>gvp</vann:preferredNamespacePrefix>
    <rdfs:seeAlso rdf:resource="http://www.getty.edu/research/tools/vocabularies/lod/"/>
    <skos:changeNote>2.0 changes: replaced gvp:broaderTransitive with gvp:broaderExtended.
3.0 changes: replaced schema:startDate, endDate with gvp:estStart, estEnd; added ULAN). See details in referenced links.
3.1 &amp; 3.2: no changes.
3.3: added 6 associative relations: gvp:aat2886_used-function_as - gvp:aat2887_exemplified_by, gvp:tgn3103_located_on - gvp:tgn3104_is_location_of, and gvp:ulan2583_chairman_of - gvp:ulan2584_chaired_by</skos:changeNote>
    <dct:creator>
      <foaf:Organization rdf:about="http://www.ontotext.com">
        <rdfs:label>Ontotext Corp</rdfs:label>
        <foaf:name>Ontotext Corp</foaf:name>
      </foaf:Organization>
    </dct:creator>
    <owl:imports rdf:resource="http://purl.org/iso25964/skos-thes"/>
    <rdf:type rdf:resource="http://purl.org/vocommons/voaf#Vocabulary"/>
    <owl:versionInfo>3.3</owl:versionInfo>
    <vann:preferredNamespaceUri>http://vocab.getty.edu/ontology#</vann:preferredNamespaceUri>
    <skos:changeNote rdf:resource="http://vocab.getty.edu/doc#Version_2.0"/>
    <dct:modified rdf:datatype="http://www.w3.org/2001/XMLSchema#date"
    >2016-04-25</dct:modified>
    <dct:created rdf:datatype="http://www.w3.org/2001/XMLSchema#date"
    >2014-02-15</dct:created>
    <skos:changeNote rdf:resource="http://vocab.getty.edu/doc#Version_3.3"/>
    <rdfs:seeAlso rdf:resource="http://lov.okfn.org/dataset/lov/details/vocabulary_gvp.html"/>
    <skos:changeNote rdf:resource="http://vocab.getty.edu/doc#Version_3.0"/>
    <dc:format>meta/rdf-schema</dc:format>
    <rdfs:seeAlso rdf:resource="http://vocab.getty.edu/doc"/>
    <dct:issued rdf:datatype="http://www.w3.org/2001/XMLSchema#date"
    >2014-02-20</dct:issued>
    <rdfs:label>Getty Vocabulary Program ontology</rdfs:label>
    <owl:imports rdf:resource="http://www.w3.org/2008/05/skos-xl"/>
    <dct:creator>
      <foaf:Organization rdf:about="http://www.getty.edu/research/">
        <rdfs:label>Getty Research Institute</rdfs:label>
        <foaf:name>Getty Research Institute</foaf:name>
      </foaf:Organization>
    </dct:creator>
    <rdfs:seeAlso rdf:resource="http://vocab.getty.edu/doc/queries"/>
  </owl:Ontology>
  <owl:Class rdf:about="http://vocab.getty.edu/ontology#Biography">
    <rdfs:isDefinedBy rdf:resource="http://vocab.getty.edu/ontology"/>
    <rdfs:comment>Biography of a ULAN agent (schema:Person|Organization). Depending on the agent, has these fields:
- schema:description: one-line-biography
- gvp:estStart
- schema:birthPlace | foundationLocation, pointing to TGN
- gvp:estEnd
- schema:deathPlace | dissolutionLocation, pointing to TGN
- schema:gender, pointing to AAT (male, female, other)
- dct:contributor
The fields of the preferred biogrpahy are also available in the agent.</rdfs:comment>
  </owl:Class>
  <owl:Class rdf:about="http://vocab.getty.edu/ontology#Concept">
    <rdfs:isDefinedBy rdf:resource="http://vocab.getty.edu/ontology"/>
    <rdfs:subClassOf>
      <owl:Class rdf:about="http://vocab.getty.edu/ontology#Subject"/>
    </rdfs:subClassOf>
    <rdfs:subClassOf rdf:resource="http://www.w3.org/2004/02/skos/core#Concept"/>
    <rdfs:label>Concept</rdfs:label>
    <rdfs:comment>Proper concept. Used in AAT only; TGN &amp; ULAN have their own, e.g. gvp:PhysPlaceConcept &amp; gvp:PersonConcept. Used for indexing and cataloguing</rdfs:comment>
    <skos:example>rhyta (AAT)</skos:example>
    <dct:description>Proper concept. Used in AAT only; TGN &amp; ULAN have their own, e.g. gvp:PhysPlaceConcept &amp; gvp:PersonConcept. Used for indexing and cataloguing.
Example: rhyta (AAT)</dct:description>
  </owl:Class>
  <owl:Class rdf:about="http://vocab.getty.edu/ontology#Hierarchy">
    <rdfs:isDefinedBy rdf:resource="http://vocab.getty.edu/ontology"/>
    <rdfs:subClassOf>
      <owl:Class rdf:about="http://vocab.getty.edu/ontology#Subject"/>
    </rdfs:subClassOf>
    <rdfs:subClassOf rdf:resource="http://purl.org/iso25964/skos-thes#ThesaurusArray"/>
    <rdfs:label>Hierarchy</rdfs:label>
    <rdfs:comment>Top of a hierarchy. Used in AAT only. Not used for indexing or cataloguing</rdfs:comment>
    <skos:example>Containers (Hierarchy Name) (AAT)</skos:example>
    <dct:description>Top of a hierarchy. Used in AAT only. Not used for indexing or cataloguing.
Example: Containers (Hierarchy Name) (AAT)</dct:description>
  </owl:Class>
  <owl:Class rdf:about="http://vocab.getty.edu/ontology#AdminPlaceConcept">
    <rdfs:isDefinedBy rdf:resource="http://vocab.getty.edu/ontology"/>
    <rdfs:subClassOf>
      <owl:Class rdf:about="http://vocab.getty.edu/ontology#Subject"/>
    </rdfs:subClassOf>
    <rdfs:subClassOf rdf:resource="http://www.w3.org/2004/02/skos/core#Concept"/>
    <rdfs:label>AdminPlaceConcept</rdfs:label>
    <rdfs:comment>Place defined by administrative boundaries and conditions, including inhabited places, nations, and empires. Used in TGN only</rdfs:comment>
    <skos:example>Burgundy region in France (TGN)</skos:example>
    <dct:description>Place defined by administrative boundaries and conditions, including inhabited places, nations, and empires. Used in TGN only.
Example: Burgundy region in France (TGN)</dct:description>
  </owl:Class>
  <owl:Class rdf:about="http://vocab.getty.edu/ontology#UnknownPersonConcept">
    <rdfs:isDefinedBy rdf:resource="http://vocab.getty.edu/ontology"/>
    <rdfs:subClassOf>
      <owl:Class rdf:about="http://vocab.getty.edu/ontology#Subject"/>
    </rdfs:subClassOf>
    <rdfs:subClassOf rdf:resource="http://www.w3.org/2004/02/skos/core#Concept"/>
    <rdfs:label>UnknownPersonConcept</rdfs:label>
    <rdfs:comment>Unknown person representing a nationality/culture (the Unknown People by Culture facet)</rdfs:comment>
    <skos:example>500355202 Unknown Bulgarian (modern) (ULAN)</skos:example>
    <dct:description>Unknown person representing a nationality/culture (the Unknown People by Culture facet).
Example: 500355202 Unknown Bulgarian (modern) (ULAN)</dct:description>
  </owl:Class>
  <owl:Class rdf:about="http://vocab.getty.edu/ontology#ScopeNote">
    <rdfs:isDefinedBy rdf:resource="http://vocab.getty.edu/ontology"/>
    <rdfs:comment>Defines a GVP subject or provides usage information. Has fields:
- dc:identifier: numeric ID, also used in the URL.
- rdf:value: the note itself (as per SKOS Primer: 4.2 Advanced Documentation Features) with language tag
- dct:language: matches the language tag
- gvp:displayOrder, order of this note amongst others
- gvp:historicFlag, gvp:estStart, gvp:estEnd, rdfs:comment: Historic Information about applicability
- dct:source or subproperties thereof 
- dct:contributor or subproperties thereof</rdfs:comment>
    <dct:description>Defines a GVP subject or provides usage information. Has fields:
- dc:identifier: numeric ID, also used in the URL.
- rdf:value: the note itself (as per SKOS Primer: 4.2 Advanced Documentation Features) with language tag
- dct:language: matches the language tag
- gvp:displayOrder, order of this note amongst others
- gvp:historicFlag, vp:estStart, gvp:estEnd, rdfs:comment: Historic Information about applicability
- dct:source or subproperties thereof 
- dct:contributor or subproperties thereof</dct:description>
  </owl:Class>
  <owl:Class rdf:about="http://vocab.getty.edu/ontology#GuideTerm">
    <rdfs:isDefinedBy rdf:resource="http://vocab.getty.edu/ontology"/>
    <rdfs:subClassOf>
      <owl:Class rdf:about="http://vocab.getty.edu/ontology#Subject"/>
    </rdfs:subClassOf>
    <rdfs:subClassOf rdf:resource="http://purl.org/iso25964/skos-thes#ThesaurusArray"/>
    <rdfs:label>GuideTerm</rdfs:label>
    <rdfs:comment>Guide Term: place holder to create a level in the hierarchy. Used in AAT and ULAN. Not used for indexing or cataloguing.</rdfs:comment>
    <skos:example>&lt;vessels for serving and consuming food&gt; (AAT), ulan:500353455 &lt;named animals&gt; under facet Non-Artists (ULAN)</skos:example>
    <dct:description>Guide Term: place holder to create a level in the hierarchy. Used in AAT and ULAN. Not used for indexing or cataloguing..
Example: &lt;vessels for serving and consuming food&gt; (AAT), ulan:500353455 &lt;named animals&gt; under facet Non-Artists (ULAN)</dct:description>
  </owl:Class>
  <owl:Class rdf:about="http://vocab.getty.edu/ontology#Subject">
    <rdfs:isDefinedBy rdf:resource="http://vocab.getty.edu/ontology"/>
    <rdfs:label>Subject</rdfs:label>
    <rdfs:comment>Node in a GVP vocabulary hierarchy. 
May be Facet, GuideTerm, Hierarchy, Concept, AdminPlaceConcept, PhysPlaceConcept, PhysAdminPlaceConcept, or ObsoleteSubject.
Implemented as skos:Concept or iso:ThesaurusArray and skos:Collection</rdfs:comment>
    <dct:description>Node in a GVP vocabulary hierarchy. 
May be Facet, GuideTerm, Hierarchy, Concept, AdminPlaceConcept, PhysPlaceConcept, PhysAdminPlaceConcept, or ObsoleteSubject.
Implemented as skos:Concept or iso:ThesaurusArray and skos:Collection</dct:description>
  </owl:Class>
  <owl:Class rdf:about="http://vocab.getty.edu/ontology#GroupConcept">
    <rdfs:isDefinedBy rdf:resource="http://vocab.getty.edu/ontology"/>
    <rdfs:subClassOf rdf:resource="http://vocab.getty.edu/ontology#Subject"/>
    <rdfs:subClassOf rdf:resource="http://www.w3.org/2004/02/skos/core#Concept"/>
    <rdfs:label>GroupConcept</rdfs:label>
    <rdfs:comment>Two or more people who generally worked together to collectively create art. Not necessarily legally incorporated. A family of artists may be considered a "corporate body". Corresponds to crm:E74_Group, not its subclass crm:E40_Legal_Body</rdfs:comment>
    <skos:example>500356337 Albrecht Duerer Workshop (ULAN)</skos:example>
    <dct:description>Two or more people who generally worked together to collectively create art. Not necessarily legally incorporated. A family of artists may be considered a "corporate body". Corresponds to crm:E74_Group, not its subclass crm:E40_Legal_Body.
Example: 500356337 Albrecht Duerer Workshop (ULAN)</dct:description>
  </owl:Class>
  <owl:Class rdf:about="http://vocab.getty.edu/ontology#Facet">
    <rdfs:isDefinedBy rdf:resource="http://vocab.getty.edu/ontology"/>
    <rdfs:subClassOf rdf:resource="http://vocab.getty.edu/ontology#Subject"/>
    <rdfs:subClassOf rdf:resource="http://purl.org/iso25964/skos-thes#ThesaurusArray"/>
    <rdfs:label>Facet</rdfs:label>
    <rdfs:comment>One of the major divisions of a vocabulary</rdfs:comment>
    <skos:example>Objects Facet (AAT), World (TGN), Artists (ULAN)</skos:example>
    <dct:description>One of the major divisions of a vocabulary.
Example: Objects Facet (AAT), World (TGN), Artists (ULAN)</dct:description>
  </owl:Class>
  <owl:Class rdf:about="http://vocab.getty.edu/ontology#ObsoleteSubject">
    <rdfs:isDefinedBy rdf:resource="http://vocab.getty.edu/ontology"/>
    <rdfs:subClassOf rdf:resource="http://vocab.getty.edu/ontology#Subject"/>
    <rdfs:label>ObsoleteSubject</rdfs:label>
    <rdfs:comment>Obsolete subject: moved out of the publishable hierarchy, or merged to another (pointed by dct:isReplacedBy)</rdfs:comment>
    <skos:example>300375205 "shranks" (AAT) was merged to 300039264 "schranks" (AAT), so aat:300375205 dct:isReplacedBy aat:300039264</skos:example>
    <dct:description>Obsolete subject: moved out of the publishable hierarchy, or merged to another (pointed by dct:isReplacedBy).
Example: 300375205 "shranks" (AAT) was merged to 300039264 "schranks" (AAT), so aat:300375205 dct:isReplacedBy aat:300039264</dct:description>
  </owl:Class>
  <owl:Class rdf:about="http://vocab.getty.edu/ontology#PhysAdminPlaceConcept">
    <rdfs:isDefinedBy rdf:resource="http://vocab.getty.edu/ontology"/>
    <rdfs:subClassOf rdf:resource="http://vocab.getty.edu/ontology#Subject"/>
    <rdfs:subClassOf rdf:resource="http://www.w3.org/2004/02/skos/core#Concept"/>
    <rdfs:label>PhysAdminPlaceConcept</rdfs:label>
    <rdfs:comment>Place that is both administrative and physical. Rarely used. Used in TGN only</rdfs:comment>
    <skos:example>6003090 Kiik-Koba (TGN)</skos:example>
    <dct:description>Place that is both administrative and physical. Rarely used. Used in TGN only.
Example: 6003090 Kiik-Koba (TGN)</dct:description>
  </owl:Class>
  <owl:Class rdf:about="http://vocab.getty.edu/ontology#PersonConcept">
    <rdfs:isDefinedBy rdf:resource="http://vocab.getty.edu/ontology"/>
    <rdfs:subClassOf rdf:resource="http://vocab.getty.edu/ontology#Subject"/>
    <rdfs:subClassOf rdf:resource="http://www.w3.org/2004/02/skos/core#Concept"/>
    <rdfs:label>PersonConcept</rdfs:label>
    <rdfs:comment>A single individual. Usually people engaged in the design or creation of art or architecture ("Artists"); but may also include donors, patrons, rulers, sitters, art historians, etc ("Non-Artists")</rdfs:comment>
    <skos:example>500115493 Duerer, Albrecht (ULAN)</skos:example>
    <dct:description>A single individual. Usually people engaged in the design or creation of art or architecture ("Artists"); but may also include donors, patrons, rulers, sitters, art historians, etc ("Non-Artists").
Example: 500115493 Duerer, Albrecht (ULAN)</dct:description>
  </owl:Class>
  <owl:Class rdf:about="http://vocab.getty.edu/ontology#PhysPlaceConcept">
    <rdfs:isDefinedBy rdf:resource="http://vocab.getty.edu/ontology"/>
    <rdfs:subClassOf rdf:resource="http://vocab.getty.edu/ontology#Subject"/>
    <rdfs:subClassOf rdf:resource="http://www.w3.org/2004/02/skos/core#Concept"/>
    <rdfs:label>PhysPlaceConcept</rdfs:label>
    <rdfs:comment>Physical feature, defined by its physical characteristics on planet Earth, including mountains, rivers, and oceans. Used in TGN only</rdfs:comment>
    <skos:example>Amazon River (TGN)</skos:example>
    <dct:description>Physical feature, defined by its physical characteristics on planet Earth, including mountains, rivers, and oceans. Used in TGN only.
Example: Amazon River (TGN)</dct:description>
  </owl:Class>
  <owl:ObjectProperty rdf:about="http://vocab.getty.edu/ontology#ulan2697_leader_was">
    <dct:description>institution - leader was - person.&#xD;
Example: The leader of Samuel H. Kress Foundation was Rush Harrison Kress</dct:description>
    <dc:title>leader was - person</dc:title>
    <rdfs:isDefinedBy rdf:resource="http://vocab.getty.edu/ontology"/>
    <rdfs:range rdf:resource="http://www.w3.org/2004/02/skos/core#Concept"/>
    <dc:identifier>2697</dc:identifier>
    <rdfs:subPropertyOf rdf:resource="http://www.w3.org/2004/02/skos/core#related"/>
    <skos:example>The leader of Samuel H. Kress Foundation was Rush Harrison Kress</skos:example>
    <skos:prefLabel>ulan2697_leader_was</skos:prefLabel>
    <rdfs:isDefinedBy>
      <skos:ConceptScheme rdf:about="http://vocab.getty.edu/ulan/">
        <rdfs:seeAlso rdf:resource="http://www.getty.edu/research/tools/vocabularies/lod/"/>
        <vann:preferredNamespacePrefix>ulan</vann:preferredNamespacePrefix>
        <dct:created rdf:datatype="http://www.w3.org/2001/XMLSchema#date"
        >2015-03-25</dct:created>
        <dct:creator rdf:resource="http://www.getty.edu/research/"/>
        <rdfs:seeAlso rdf:resource="http://vocab.getty.edu/.well-known/void"/>
        <foaf:homepage rdf:resource="http://www.getty.edu/research/tools/vocabularies/ulan/"/>
        <rdfs:label>Union List of Artist Names</rdfs:label>
        <dct:creator rdf:resource="http://www.ontotext.com"/>
        <vann:preferredNamespaceUri>http://vocab.getty.edu/ulan/</vann:preferredNamespaceUri>
        <rdfs:seeAlso rdf:resource="http://vocab.getty.edu/"/>
        <rdfs:comment>The Union List of Artist Names concept scheme</rdfs:comment>
      </skos:ConceptScheme>
    </rdfs:isDefinedBy>
    <rdfs:domain rdf:resource="http://www.w3.org/2004/02/skos/core#Concept"/>
  </owl:ObjectProperty>
  <owl:ObjectProperty rdf:about="http://vocab.getty.edu/ontology#ulan2779_owned_by">
    <dct:description>person - owned by - firm.&#xD;
Example: Walter Scott Lenox was owned by Lenox China Co.</dct:description>
    <dc:identifier>2779</dc:identifier>
    <rdfs:isDefinedBy rdf:resource="http://vocab.getty.edu/ontology"/>
    <rdfs:range rdf:resource="http://www.w3.org/2004/02/skos/core#Concept"/>
    <rdfs:isDefinedBy rdf:resource="http://vocab.getty.edu/ulan/"/>
    <rdfs:domain rdf:resource="http://www.w3.org/2004/02/skos/core#Concept"/>
    <dc:title>owned by - firm</dc:title>
    <skos:prefLabel>ulan2779_owned_by</skos:prefLabel>
    <skos:example>Walter Scott Lenox was owned by Lenox China Co.</skos:example>
    <rdfs:subPropertyOf rdf:resource="http://www.w3.org/2004/02/skos/core#related"/>
  </owl:ObjectProperty>
  <owl:ObjectProperty rdf:about="http://vocab.getty.edu/ontology#aat2316_use">
    <skos:example>lapidaries use precious stone</skos:example>
    <rdfs:subPropertyOf rdf:resource="http://www.w3.org/2004/02/skos/core#related"/>
    <rdfs:isDefinedBy>
      <skos:ConceptScheme rdf:about="http://vocab.getty.edu/aat/">
        <dct:created rdf:datatype="http://www.w3.org/2001/XMLSchema#date"
        >2014-02-20</dct:created>
        <rdfs:label>Art and Architecture Thesaurus</rdfs:label>
        <rdfs:seeAlso rdf:resource="http://vocab.getty.edu/"/>
        <foaf:homepage rdf:resource="http://www.getty.edu/research/tools/vocabularies/aat/"/>
        <rdfs:seeAlso rdf:resource="http://www.getty.edu/research/tools/vocabularies/lod/"/>
        <vann:preferredNamespaceUri>http://vocab.getty.edu/aat/</vann:preferredNamespaceUri>
        <rdfs:comment>The Art and Architecture Thesaurus concept scheme</rdfs:comment>
        <vann:preferredNamespacePrefix>aat</vann:preferredNamespacePrefix>
        <dct:creator rdf:resource="http://www.ontotext.com"/>
        <rdfs:seeAlso rdf:resource="http://vocab.getty.edu/.well-known/void"/>
        <dct:creator rdf:resource="http://www.getty.edu/research/"/>
      </skos:ConceptScheme>
    </rdfs:isDefinedBy>
    <rdfs:domain rdf:resource="http://www.w3.org/2004/02/skos/core#Concept"/>
    <dc:title>use - material</dc:title>
    <dc:identifier>2316</dc:identifier>
    <rdfs:range rdf:resource="http://www.w3.org/2004/02/skos/core#Concept"/>
    <rdfs:isDefinedBy rdf:resource="http://vocab.getty.edu/ontology"/>
    <dct:description>[actors having] role - use - material.&#xD;
Example: lapidaries use precious stone; braziers (metalworkers) use brass (alloy)</dct:description>
    <skos:prefLabel>aat2316_use</skos:prefLabel>
    <skos:example>braziers (metalworkers) use brass (alloy)</skos:example>
  </owl:ObjectProperty>
  <owl:ObjectProperty rdf:about="http://vocab.getty.edu/ontology#ulan2840_performer_with">
    <dc:title>performer with - group</dc:title>
    <rdfs:domain rdf:resource="http://www.w3.org/2004/02/skos/core#Concept"/>
    <rdfs:range rdf:resource="http://www.w3.org/2004/02/skos/core#Concept"/>
    <rdfs:isDefinedBy rdf:resource="http://vocab.getty.edu/ulan/"/>
    <dc:identifier>2840</dc:identifier>
    <skos:prefLabel>ulan2840_performer_with</skos:prefLabel>
    <dct:description>person - performer with - group</dct:description>
    <rdfs:subPropertyOf rdf:resource="http://www.w3.org/2004/02/skos/core#related"/>
    <rdfs:isDefinedBy rdf:resource="http://vocab.getty.edu/ontology"/>
    <owl:inverseOf>
      <owl:ObjectProperty rdf:about="http://vocab.getty.edu/ontology#ulan2841_performer_was"/>
    </owl:inverseOf>
  </owl:ObjectProperty>
  <owl:ObjectProperty rdf:about="http://vocab.getty.edu/ontology#ulan2577_patron_was">
    <rdfs:range rdf:resource="http://www.w3.org/2004/02/skos/core#Concept"/>
    <dc:identifier>2577</dc:identifier>
    <rdfs:domain rdf:resource="http://www.w3.org/2004/02/skos/core#Concept"/>
    <rdfs:subPropertyOf rdf:resource="http://www.w3.org/2004/02/skos/core#related"/>
    <rdfs:isDefinedBy rdf:resource="http://vocab.getty.edu/ulan/"/>
    <dct:description>person - patron was - person.&#xD;
Example: James Caulfiel, Earl of Charlemont was the patron of William Chambers</dct:description>
    <skos:prefLabel>ulan2577_patron_was</skos:prefLabel>
    <skos:example>James Caulfiel, Earl of Charlemont was the patron of William Chambers</skos:example>
    <dc:title>patron was - person</dc:title>
    <rdfs:isDefinedBy rdf:resource="http://vocab.getty.edu/ontology"/>
  </owl:ObjectProperty>
  <owl:ObjectProperty rdf:about="http://vocab.getty.edu/ontology#ulan1553_child_by_marriage_of">
    <dc:identifier>1553</dc:identifier>
    <rdfs:domain rdf:resource="http://www.w3.org/2004/02/skos/core#Concept"/>
    <rdfs:isDefinedBy rdf:resource="http://vocab.getty.edu/ulan/"/>
    <dct:description>person - child by marriage (step child) - person.&#xD;
Example: Pieter Gerritsz van Roestraten is the child by marriage of Frans Hals</dct:description>
    <skos:example>Pieter Gerritsz van Roestraten is the child by marriage of Frans Hals</skos:example>
    <rdfs:isDefinedBy rdf:resource="http://vocab.getty.edu/ontology"/>
    <dc:title>child by marriage of - person</dc:title>
    <skos:prefLabel>ulan1553_child_by_marriage_of</skos:prefLabel>
    <rdfs:subPropertyOf rdf:resource="http://www.w3.org/2004/02/skos/core#related"/>
    <rdfs:range rdf:resource="http://www.w3.org/2004/02/skos/core#Concept"/>
  </owl:ObjectProperty>
  <owl:ObjectProperty rdf:about="http://vocab.getty.edu/ontology#aat2900_miscellaneous_relationship">
    <dc:identifier>2900</dc:identifier>
    <skos:prefLabel>aat2900_miscellaneous_relationship</skos:prefLabel>
    <rdfs:isDefinedBy rdf:resource="http://vocab.getty.edu/ontology"/>
    <rdfs:subPropertyOf rdf:resource="http://www.w3.org/2004/02/skos/core#related"/>
    <dct:description>any - [has] miscellaneous relationship [to] - any.&#xD;
Example: Conditions and Effects has miscellaneous relationship with Processes and Techniques</dct:description>
    <dc:title>miscellaneous relationship - any</dc:title>
    <rdfs:domain rdf:resource="http://www.w3.org/2004/02/skos/core#Concept"/>
    <rdf:type rdf:resource="http://www.w3.org/2002/07/owl#SymmetricProperty"/>
    <rdfs:range rdf:resource="http://www.w3.org/2004/02/skos/core#Concept"/>
    <skos:example>Conditions and Effects has miscellaneous relationship with Processes and Techniques</skos:example>
    <rdfs:isDefinedBy rdf:resource="http://vocab.getty.edu/aat/"/>
  </owl:ObjectProperty>
  <owl:ObjectProperty rdf:about="http://vocab.getty.edu/ontology#agentTypeNonPreferred">
    <rdfs:isDefinedBy rdf:resource="http://vocab.getty.edu/ontology"/>
    <rdfs:label>agentTypeNonPreferred</rdfs:label>
    <rdfs:domain rdf:resource="http://vocab.getty.edu/ontology#Subject"/>
    <rdfs:range rdf:resource="http://vocab.getty.edu/ontology#Subject"/>
    <rdfs:subPropertyOf>
      <owl:ObjectProperty rdf:about="http://vocab.getty.edu/ontology#agentType"/>
    </rdfs:subPropertyOf>
    <rdfs:comment>A secondary type of a ULAN Person or Corporate body. Domain is ULAN concept, range is AAT concept</rdfs:comment>
    <skos:example>Non-preferred types of "Albrecht Duerer Workshop" (ULAN) include "printmakers" and painters" (AAT)</skos:example>
    <dct:description>A secondary type of a ULAN Person or Corporate body. Domain is ULAN concept, range is AAT concept.
Example: Non-preferred types of "Albrecht Duerer Workshop" (ULAN) include "printmakers" and painters" (AAT)</dct:description>
  </owl:ObjectProperty>
  <owl:ObjectProperty rdf:about="http://vocab.getty.edu/ontology#tgn3005_possibly_identified_as">
    <dc:title>possibly identified as - place</dc:title>
    <rdfs:subPropertyOf rdf:resource="http://www.w3.org/2004/02/skos/core#related"/>
    <skos:example>The lost settlement of Sharuhen is possibly identified as Tel el-Far'ah (As Suwayda', Syria) (deserted settlement)</skos:example>
    <rdfs:range rdf:resource="http://www.w3.org/2004/02/skos/core#Concept"/>
    <rdfs:domain rdf:resource="http://www.w3.org/2004/02/skos/core#Concept"/>
    <rdfs:isDefinedBy>
      <skos:ConceptScheme rdf:about="http://vocab.getty.edu/tgn/">
        <vann:preferredNamespacePrefix>tgn</vann:preferredNamespacePrefix>
        <rdfs:seeAlso rdf:resource="http://vocab.getty.edu/.well-known/void"/>
        <dct:creator rdf:resource="http://www.ontotext.com"/>
        <rdfs:seeAlso rdf:resource="http://vocab.getty.edu/"/>
        <dct:created rdf:datatype="http://www.w3.org/2001/XMLSchema#date"
        >2014-06-15</dct:created>
        <dct:creator rdf:resource="http://www.getty.edu/research/"/>
        <rdfs:seeAlso rdf:resource="http://www.getty.edu/research/tools/vocabularies/lod/"/>
        <rdfs:comment>The Thesaurus of Geographic Names concept scheme</rdfs:comment>
        <rdfs:label>Thesaurus of Geographic Names</rdfs:label>
        <foaf:homepage rdf:resource="http://www.getty.edu/research/tools/vocabularies/tgn/"/>
        <vann:preferredNamespaceUri>http://vocab.getty.edu/tgn/</vann:preferredNamespaceUri>
      </skos:ConceptScheme>
    </rdfs:isDefinedBy>
    <dct:description>place - possibly identified as - place.&#xD;
Example: The lost settlement of Sharuhen is possibly identified as Tel el-Far'ah (As Suwayda', Syria) (deserted settlement)</dct:description>
    <skos:prefLabel>tgn3005_possibly_identified_as</skos:prefLabel>
    <dc:identifier>3005</dc:identifier>
    <rdf:type rdf:resource="http://www.w3.org/2002/07/owl#SymmetricProperty"/>
    <rdfs:isDefinedBy rdf:resource="http://vocab.getty.edu/ontology"/>
  </owl:ObjectProperty>
  <owl:ObjectProperty rdf:about="http://vocab.getty.edu/ontology#aat2332_affiliated_with">
    <dc:identifier>2332</dc:identifier>
    <dct:description>[actors having] role - [are] affiliated with - role [organization].&#xD;
Example: students are affiliated with schools (organizations); dukes are affiliated with duchies</dct:description>
    <rdfs:isDefinedBy rdf:resource="http://vocab.getty.edu/aat/"/>
    <skos:example>dukes are affiliated with duchies</skos:example>
    <rdfs:domain rdf:resource="http://www.w3.org/2004/02/skos/core#Concept"/>
    <rdfs:range rdf:resource="http://www.w3.org/2004/02/skos/core#Concept"/>
    <skos:example>students are affiliated with schools (organizations)</skos:example>
    <skos:prefLabel>aat2332_affiliated_with</skos:prefLabel>
    <rdfs:isDefinedBy rdf:resource="http://vocab.getty.edu/ontology"/>
    <dc:title>affiliated with - role</dc:title>
    <owl:inverseOf>
      <owl:ObjectProperty rdf:about="http://vocab.getty.edu/ontology#aat2333_have_affiliates"/>
    </owl:inverseOf>
    <rdfs:subPropertyOf rdf:resource="http://www.w3.org/2004/02/skos/core#related"/>
  </owl:ObjectProperty>
  <owl:ObjectProperty rdf:about="http://vocab.getty.edu/ontology#termFlag">
    <rdfs:isDefinedBy rdf:resource="http://vocab.getty.edu/ontology"/>
    <rdfs:label>termFlag</rdfs:label>
    <rdfs:domain rdf:resource="http://www.w3.org/2008/05/skos-xl#Label"/>
    <rdfs:range rdf:resource="http://www.w3.org/2004/02/skos/core#Concept"/>
    <dct:description>Term Flag</dct:description>
  </owl:ObjectProperty>
  <owl:ObjectProperty rdf:about="http://vocab.getty.edu/ontology#aat2321_used_by">
    <rdfs:subPropertyOf rdf:resource="http://www.w3.org/2004/02/skos/core#related"/>
    <skos:example>violoncellos are used by violoncellists</skos:example>
    <rdfs:domain rdf:resource="http://www.w3.org/2004/02/skos/core#Concept"/>
    <rdfs:range rdf:resource="http://www.w3.org/2004/02/skos/core#Concept"/>
    <skos:example>surveying instruments are used by surveyors</skos:example>
    <rdfs:isDefinedBy rdf:resource="http://vocab.getty.edu/ontology"/>
    <skos:prefLabel>aat2321_used_by</skos:prefLabel>
    <dc:title>used by - role</dc:title>
    <rdfs:isDefinedBy rdf:resource="http://vocab.getty.edu/aat/"/>
    <dc:identifier>2321</dc:identifier>
    <dct:description>things/equipment - [are] used by - [actors having] role.&#xD;
Example: violoncellos are used by violoncellists; surveying instruments are used by surveyors</dct:description>
    <owl:inverseOf>
      <owl:ObjectProperty rdf:about="http://vocab.getty.edu/ontology#aat2322_use"/>
    </owl:inverseOf>
  </owl:ObjectProperty>
  <owl:ObjectProperty rdf:about="http://vocab.getty.edu/ontology#ulan1571_guardian_of">
    <rdfs:isDefinedBy rdf:resource="http://vocab.getty.edu/ulan/"/>
    <dct:description>person - guardian of - person.&#xD;
Example: John Hoskins, the elder was the guardian of Samuel Cooper</dct:description>
    <dc:identifier>1571</dc:identifier>
    <rdfs:range rdf:resource="http://www.w3.org/2004/02/skos/core#Concept"/>
    <rdfs:domain rdf:resource="http://www.w3.org/2004/02/skos/core#Concept"/>
    <rdfs:isDefinedBy rdf:resource="http://vocab.getty.edu/ontology"/>
    <skos:prefLabel>ulan1571_guardian_of</skos:prefLabel>
    <skos:example>John Hoskins, the elder was the guardian of Samuel Cooper</skos:example>
    <dc:title>guardian of - person</dc:title>
    <rdfs:subPropertyOf rdf:resource="http://www.w3.org/2004/02/skos/core#related"/>
    <owl:inverseOf>
      <owl:ObjectProperty rdf:about="http://vocab.getty.edu/ontology#ulan1573_ward_of"/>
    </owl:inverseOf>
  </owl:ObjectProperty>
  <owl:ObjectProperty rdf:about="http://vocab.getty.edu/ontology#placeTypePreferred">
    <rdfs:isDefinedBy rdf:resource="http://vocab.getty.edu/ontology"/>
    <rdfs:label>placeTypePreferred</rdfs:label>
    <rdfs:domain rdf:resource="http://vocab.getty.edu/ontology#Subject"/>
    <rdfs:range rdf:resource="http://vocab.getty.edu/ontology#Subject"/>
    <rdfs:subPropertyOf>
      <owl:ObjectProperty rdf:about="http://vocab.getty.edu/ontology#placeType"/>
    </rdfs:subPropertyOf>
    <rdfs:comment>The primary type of a TGN Place. Domain is TGN concept, range is AAT concept</rdfs:comment>
    <skos:example>The preferred place type of Machupicchu, Peru is "deserted settlement" (current)</skos:example>
    <dct:description>The primary type of a TGN Place. Domain is TGN concept, range is AAT concept.
Example: The preferred place type of Machupicchu, Peru is "deserted settlement" (current)</dct:description>
  </owl:ObjectProperty>
  <owl:ObjectProperty rdf:about="http://vocab.getty.edu/ontology#aat2209_used-located_in">
    <rdfs:domain rdf:resource="http://www.w3.org/2004/02/skos/core#Concept"/>
    <rdfs:range rdf:resource="http://www.w3.org/2004/02/skos/core#Concept"/>
    <skos:example>cave paintings are located in caves</skos:example>
    <dct:description>things -used/located in -  locus/setting.&#xD;
Example: glassware is used/located in glassworks (buildings); cave paintings are located in caves</dct:description>
    <rdfs:subPropertyOf rdf:resource="http://www.w3.org/2004/02/skos/core#related"/>
    <rdfs:isDefinedBy rdf:resource="http://vocab.getty.edu/aat/"/>
    <dc:identifier>2209</dc:identifier>
    <skos:example>glassware is used/located in glassworks (buildings)</skos:example>
    <rdfs:isDefinedBy rdf:resource="http://vocab.getty.edu/ontology"/>
    <skos:prefLabel>aat2209_used-located_in</skos:prefLabel>
    <dc:title>used/located in - locus/setting</dc:title>
  </owl:ObjectProperty>
  <owl:ObjectProperty rdf:about="http://vocab.getty.edu/ontology#aat2818_source_for">
    <skos:example>timber (lumber) is the source for wood board</skos:example>
    <rdfs:isDefinedBy rdf:resource="http://vocab.getty.edu/aat/"/>
    <dc:identifier>2818</dc:identifier>
    <rdfs:isDefinedBy rdf:resource="http://vocab.getty.edu/ontology"/>
    <rdfs:domain rdf:resource="http://www.w3.org/2004/02/skos/core#Concept"/>
    <skos:prefLabel>aat2818_source_for</skos:prefLabel>
    <dct:description>material - [is] source for - material.&#xD;
Example: anhydrite is the source for gypsum; timber (lumber) is the source for wood board</dct:description>
    <rdfs:range rdf:resource="http://www.w3.org/2004/02/skos/core#Concept"/>
    <dc:title>source for - material</dc:title>
    <rdfs:subPropertyOf rdf:resource="http://www.w3.org/2004/02/skos/core#related"/>
    <skos:example>anhydrite is the source for gypsum</skos:example>
  </owl:ObjectProperty>
  <owl:ObjectProperty rdf:about="http://vocab.getty.edu/ontology#ulan1515_great-grandparent_of">
    <skos:prefLabel>ulan1515_great-grandparent_of</skos:prefLabel>
    <rdfs:subPropertyOf rdf:resource="http://www.w3.org/2004/02/skos/core#related"/>
    <rdfs:range rdf:resource="http://www.w3.org/2004/02/skos/core#Concept"/>
    <skos:example>Albrecht Adam is the great-grandparent of Richard Benno Adam</skos:example>
    <dc:title>great-grandparent of - person</dc:title>
    <owl:inverseOf>
      <owl:ObjectProperty rdf:about="http://vocab.getty.edu/ontology#ulan1516_great-grandchild_of"/>
    </owl:inverseOf>
    <rdfs:domain rdf:resource="http://www.w3.org/2004/02/skos/core#Concept"/>
    <dc:identifier>1515</dc:identifier>
    <rdfs:isDefinedBy rdf:resource="http://vocab.getty.edu/ulan/"/>
    <dct:description>person - great-grandparent of - person.&#xD;
Example: Albrecht Adam is the great-grandparent of Richard Benno Adam</dct:description>
    <rdfs:isDefinedBy rdf:resource="http://vocab.getty.edu/ontology"/>
  </owl:ObjectProperty>
  <owl:ObjectProperty rdf:about="http://vocab.getty.edu/ontology#aat2605_possess-exist_in">
    <dc:identifier>2605</dc:identifier>
    <skos:example>boudoir photographs possess/exist in boudoir (photograph size)</skos:example>
    <rdfs:isDefinedBy rdf:resource="http://vocab.getty.edu/aat/"/>
    <rdfs:domain rdf:resource="http://www.w3.org/2004/02/skos/core#Concept"/>
    <rdfs:subPropertyOf rdf:resource="http://www.w3.org/2004/02/skos/core#related"/>
    <skos:prefLabel>aat2605_possess-exist_in</skos:prefLabel>
    <rdfs:isDefinedBy rdf:resource="http://vocab.getty.edu/ontology"/>
    <skos:example>ruins possess/exist in ruined [contition]</skos:example>
    <dc:title>possess/exist in - attributes /associated concepts</dc:title>
    <rdfs:range rdf:resource="http://www.w3.org/2004/02/skos/core#Concept"/>
    <dct:description>things - possess/exist in - attributes /associated concepts.&#xD;
Example: boudoir photographs possess/exist in boudoir (photograph size); ruins possess/exist in ruined [contition]</dct:description>
  </owl:ObjectProperty>
  <owl:ObjectProperty rdf:about="http://vocab.getty.edu/ontology#aat2434_contextualized_in">
    <owl:inverseOf>
      <owl:ObjectProperty rdf:about="http://vocab.getty.edu/ontology#aat2435_context_for"/>
    </owl:inverseOf>
    <rdfs:range rdf:resource="http://www.w3.org/2004/02/skos/core#Concept"/>
    <dct:description>things - [are] context for - activity/event/process.&#xD;
Example: funeral books are contextualized in funerals; Christmas trees are contextualized in Christmas</dct:description>
    <dc:title>contextualized in - activity/event/process</dc:title>
    <rdfs:domain rdf:resource="http://www.w3.org/2004/02/skos/core#Concept"/>
    <skos:example>funeral books are contextualized in funerals</skos:example>
    <skos:example>Christmas trees are contextualized in Christmas</skos:example>
    <rdfs:isDefinedBy rdf:resource="http://vocab.getty.edu/aat/"/>
    <dc:identifier>2434</dc:identifier>
    <skos:prefLabel>aat2434_contextualized_in</skos:prefLabel>
    <rdfs:isDefinedBy rdf:resource="http://vocab.getty.edu/ontology"/>
    <rdfs:subPropertyOf rdf:resource="http://www.w3.org/2004/02/skos/core#related"/>
  </owl:ObjectProperty>
  <owl:ObjectProperty rdf:about="http://vocab.getty.edu/ontology#aat2409_takes_place_in">
    <rdfs:domain rdf:resource="http://www.w3.org/2004/02/skos/core#Concept"/>
    <dc:identifier>2409</dc:identifier>
    <rdfs:range rdf:resource="http://www.w3.org/2004/02/skos/core#Concept"/>
    <skos:example>medicine (discipline) takes place in hospitals (buildings)</skos:example>
    <rdfs:isDefinedBy rdf:resource="http://vocab.getty.edu/ontology"/>
    <dc:title>takes place in - locus/setting</dc:title>
    <dct:description>field of study/discipline - takes place in - locus/setting.&#xD;
Example: education takes place in schools (buildings); medicine (discipline) takes place in hospitals (buildings)</dct:description>
    <skos:prefLabel>aat2409_takes_place_in</skos:prefLabel>
    <rdfs:subPropertyOf rdf:resource="http://www.w3.org/2004/02/skos/core#related"/>
    <skos:example>education takes place in schools (buildings)</skos:example>
    <rdfs:isDefinedBy rdf:resource="http://vocab.getty.edu/aat/"/>
  </owl:ObjectProperty>
  <owl:ObjectProperty rdf:about="http://vocab.getty.edu/ontology#aat2894_exemplified_by">
    <dc:identifier>2894</dc:identifier>
    <rdfs:domain rdf:resource="http://www.w3.org/2004/02/skos/core#Concept"/>
    <owl:inverseOf>
      <owl:ObjectProperty rdf:about="http://vocab.getty.edu/ontology#aat2895_example_of"/>
    </owl:inverseOf>
    <dct:description>activity/event/[process/function] - [is] exemplified by - brand name.&#xD;
Example: deacidification [process/function] is exemplified by Papersave Process (TM)</dct:description>
    <skos:example>deacidification [process/function] is exemplified by Papersave Process (TM)</skos:example>
    <skos:prefLabel>aat2894_exemplified_by</skos:prefLabel>
    <rdfs:isDefinedBy rdf:resource="http://vocab.getty.edu/ontology"/>
    <dc:title>exemplified by - brand name</dc:title>
    <rdfs:subPropertyOf rdf:resource="http://www.w3.org/2004/02/skos/core#related"/>
    <rdfs:isDefinedBy rdf:resource="http://vocab.getty.edu/aat/"/>
    <rdfs:range rdf:resource="http://www.w3.org/2004/02/skos/core#Concept"/>
  </owl:ObjectProperty>
  <owl:ObjectProperty rdf:about="http://vocab.getty.edu/ontology#ulan1306_performs_with">
    <dct:description>person - performs with - person.&#xD;
Example: Harry Kipper performs with Harry Kipper (as part of 'The Kipper Kids')</dct:description>
    <rdfs:isDefinedBy rdf:resource="http://vocab.getty.edu/ulan/"/>
    <rdfs:domain rdf:resource="http://www.w3.org/2004/02/skos/core#Concept"/>
    <skos:example>Harry Kipper performs with Harry Kipper (as part of 'The Kipper Kids')</skos:example>
    <rdfs:isDefinedBy rdf:resource="http://vocab.getty.edu/ontology"/>
    <skos:prefLabel>ulan1306_performs_with</skos:prefLabel>
    <rdfs:subPropertyOf rdf:resource="http://www.w3.org/2004/02/skos/core#related"/>
    <rdf:type rdf:resource="http://www.w3.org/2002/07/owl#SymmetricProperty"/>
    <dc:identifier>1306</dc:identifier>
    <dc:title>performs with - person</dc:title>
    <rdfs:range rdf:resource="http://www.w3.org/2004/02/skos/core#Concept"/>
  </owl:ObjectProperty>
  <owl:ObjectProperty rdf:about="http://vocab.getty.edu/ontology#aat2412_involves">
    <skos:prefLabel>aat2412_involves</skos:prefLabel>
    <skos:example>horticulture involves gardening</skos:example>
    <rdfs:isDefinedBy rdf:resource="http://vocab.getty.edu/ontology"/>
    <dc:identifier>2412</dc:identifier>
    <rdfs:range rdf:resource="http://www.w3.org/2004/02/skos/core#Concept"/>
    <rdfs:isDefinedBy rdf:resource="http://vocab.getty.edu/aat/"/>
    <dc:title>involves - activity/event</dc:title>
    <rdfs:subPropertyOf rdf:resource="http://www.w3.org/2004/02/skos/core#related"/>
    <skos:example>photojournalism (discipline) involves journalistic photography</skos:example>
    <dct:description>field/discipline - involves - activity/event/[process/function].&#xD;
Example: photojournalism (discipline) involves journalistic photography; horticulture involves gardening</dct:description>
    <rdfs:domain rdf:resource="http://www.w3.org/2004/02/skos/core#Concept"/>
  </owl:ObjectProperty>
  <owl:ObjectProperty rdf:about="http://vocab.getty.edu/ontology#aat2834_decendant_of">
    <skos:example>Canis familiaris is the descendant of Canis lupus</skos:example>
    <skos:example>donkeys are the descendents of Equus asinus</skos:example>
    <rdfs:range rdf:resource="http://www.w3.org/2004/02/skos/core#Concept"/>
    <skos:prefLabel>aat2834_decendant_of</skos:prefLabel>
    <dc:title>decendant of - genus/species</dc:title>
    <dc:identifier>2834</dc:identifier>
    <rdfs:domain rdf:resource="http://www.w3.org/2004/02/skos/core#Concept"/>
    <rdfs:subPropertyOf rdf:resource="http://www.w3.org/2004/02/skos/core#related"/>
    <dct:description>genus/species - is decendant of -  genus/species.&#xD;
Example: Canis familiaris is the descendant of Canis lupus; donkeys are the descendents of Equus asinus</dct:description>
    <rdfs:isDefinedBy rdf:resource="http://vocab.getty.edu/ontology"/>
    <rdfs:isDefinedBy rdf:resource="http://vocab.getty.edu/aat/"/>
  </owl:ObjectProperty>
  <owl:ObjectProperty rdf:about="http://vocab.getty.edu/ontology#ulan1541_spouse_of">
    <rdfs:range rdf:resource="http://www.w3.org/2004/02/skos/core#Concept"/>
    <dct:description>person - spouse of - person.&#xD;
Example: Alfred Stieglitz and Georgia O'Keeffe were married to each other</dct:description>
    <rdfs:subPropertyOf rdf:resource="http://www.w3.org/2004/02/skos/core#related"/>
    <rdfs:domain rdf:resource="http://www.w3.org/2004/02/skos/core#Concept"/>
    <rdfs:isDefinedBy rdf:resource="http://vocab.getty.edu/ontology"/>
    <rdf:type rdf:resource="http://www.w3.org/2002/07/owl#SymmetricProperty"/>
    <dc:identifier>1541</dc:identifier>
    <skos:prefLabel>ulan1541_spouse_of</skos:prefLabel>
    <skos:example>Alfred Stieglitz and Georgia O'Keeffe were married to each other</skos:example>
    <dc:title>spouse of - person</dc:title>
    <rdfs:isDefinedBy rdf:resource="http://vocab.getty.edu/ulan/"/>
  </owl:ObjectProperty>
  <owl:ObjectProperty rdf:about="http://vocab.getty.edu/ontology#aat2821_based_on">
    <skos:example>pencils are based on plummets</skos:example>
    <skos:example>Neo-Gothic is based on Gothic (Medieval)</skos:example>
    <rdfs:isDefinedBy rdf:resource="http://vocab.getty.edu/aat/"/>
    <owl:inverseOf>
      <owl:ObjectProperty rdf:about="http://vocab.getty.edu/ontology#aat2822_basis_of"/>
    </owl:inverseOf>
    <rdfs:subPropertyOf rdf:resource="http://www.w3.org/2004/02/skos/core#related"/>
    <rdfs:isDefinedBy rdf:resource="http://vocab.getty.edu/ontology"/>
    <dc:identifier>2821</dc:identifier>
    <rdfs:domain rdf:resource="http://www.w3.org/2004/02/skos/core#Concept"/>
    <skos:prefLabel>aat2821_based_on</skos:prefLabel>
    <skos:example>curved [form attribute] is based on curves (geometric figures)</skos:example>
    <dc:title>based on - any</dc:title>
    <dct:description>any - [is] based on - any.&#xD;
Example: Neo-Gothic is based on Gothic (Medieval); curved [form attribute] is based on curves (geometric figures); pencils are based on plummets</dct:description>
    <rdfs:range rdf:resource="http://www.w3.org/2004/02/skos/core#Concept"/>
  </owl:ObjectProperty>
  <owl:ObjectProperty rdf:about="http://vocab.getty.edu/ontology#ulan1314_partner_was">
    <rdfs:isDefinedBy rdf:resource="http://vocab.getty.edu/ulan/"/>
    <rdfs:range rdf:resource="http://www.w3.org/2004/02/skos/core#Concept"/>
    <dc:identifier>1314</dc:identifier>
    <skos:prefLabel>ulan1314_partner_was</skos:prefLabel>
    <rdfs:subPropertyOf rdf:resource="http://www.w3.org/2004/02/skos/core#related"/>
    <rdfs:isDefinedBy rdf:resource="http://vocab.getty.edu/ontology"/>
    <dct:description>firm - partner was - person.&#xD;
Example: Louis H. Sullivan and Dankmar Adler were partners in Adler and Sullivan</dct:description>
    <skos:example>Louis H. Sullivan and Dankmar Adler were partners in Adler and Sullivan</skos:example>
    <dc:title>partner was - person</dc:title>
    <rdfs:domain rdf:resource="http://www.w3.org/2004/02/skos/core#Concept"/>
  </owl:ObjectProperty>
  <owl:ObjectProperty rdf:about="http://vocab.getty.edu/ontology#ulan1322_school_was">
    <dc:title>school was - person</dc:title>
    <rdfs:domain rdf:resource="http://www.w3.org/2004/02/skos/core#Concept"/>
    <rdfs:isDefinedBy rdf:resource="http://vocab.getty.edu/ontology"/>
    <rdfs:subPropertyOf rdf:resource="http://www.w3.org/2004/02/skos/core#related"/>
    <dc:identifier>1322</dc:identifier>
    <rdfs:range rdf:resource="http://www.w3.org/2004/02/skos/core#Concept"/>
    <skos:example>Pierre Saalburg attended Architectural Association. School of Architecture</skos:example>
    <dct:description>firm/group - school was - person.&#xD;
Example: Pierre Saalburg attended Architectural Association. School of Architecture</dct:description>
    <skos:prefLabel>ulan1322_school_was</skos:prefLabel>
    <rdfs:isDefinedBy rdf:resource="http://vocab.getty.edu/ulan/"/>
  </owl:ObjectProperty>
  <owl:ObjectProperty rdf:about="http://vocab.getty.edu/ontology#prefLabelGVP">
    <rdfs:isDefinedBy rdf:resource="http://vocab.getty.edu/ontology"/>
    <rdfs:label>prefLabelGVP</rdfs:label>
    <rdfs:domain rdf:resource="http://vocab.getty.edu/ontology#Subject"/>
    <rdfs:range rdf:resource="http://www.w3.org/2008/05/skos-xl#Label"/>
    <rdfs:comment>Term preferred by the Getty Vocabulary Program. The language is usually English. Applicable to AAT, ULAN, TGN. Used with skosxl:prefLabel</rdfs:comment>
    <dct:description>Term preferred by the Getty Vocabulary Program. The language is usually English. Applicable to AAT, ULAN, TGN. Used with skosxl:prefLabel</dct:description>
  </owl:ObjectProperty>
  <owl:ObjectProperty rdf:about="http://vocab.getty.edu/ontology#ulan1212_artist_was">
    <skos:prefLabel>ulan1212_artist_was</skos:prefLabel>
    <dct:description>person - artist was - person.&#xD;
Example: Charles-Pierre Coustou was artist to Louis XIV, King of France</dct:description>
    <rdfs:range rdf:resource="http://www.w3.org/2004/02/skos/core#Concept"/>
    <dc:title>artist was - person</dc:title>
    <rdfs:isDefinedBy rdf:resource="http://vocab.getty.edu/ulan/"/>
    <rdfs:isDefinedBy rdf:resource="http://vocab.getty.edu/ontology"/>
    <dc:identifier>1212</dc:identifier>
    <rdfs:subPropertyOf rdf:resource="http://www.w3.org/2004/02/skos/core#related"/>
    <skos:example>Charles-Pierre Coustou was artist to Louis XIV, King of France</skos:example>
    <rdfs:domain rdf:resource="http://www.w3.org/2004/02/skos/core#Concept"/>
  </owl:ObjectProperty>
  <owl:ObjectProperty rdf:about="http://vocab.getty.edu/ontology#broaderNonPreferred">
    <rdfs:isDefinedBy rdf:resource="http://vocab.getty.edu/ontology"/>
    <rdfs:label>broaderNonPreferred</rdfs:label>
    <rdfs:domain rdf:resource="http://vocab.getty.edu/ontology#Subject"/>
    <rdfs:range rdf:resource="http://vocab.getty.edu/ontology#Subject"/>
    <rdfs:subPropertyOf>
      <owl:ObjectProperty rdf:about="http://vocab.getty.edu/ontology#broader"/>
    </rdfs:subPropertyOf>
    <rdfs:comment>Auxiliary parents of a subject. Very often there are several non-preferred parents (poly-hierarchy). Can use to mark such parents with [N] in displays </rdfs:comment>
    <skos:example>Non-preferred: "baking dishes" BTG "dishes (vessels)" (AAT)</skos:example>
    <dct:description>Auxiliary parents of a subject. Very often there are several non-preferred parents (poly-hierarchy). Can use to mark such parents with [N] in displays .
Example: Non-preferred: "baking dishes" BTG "dishes (vessels)" (AAT)</dct:description>
  </owl:ObjectProperty>
  <owl:ObjectProperty rdf:about="http://vocab.getty.edu/ontology#placeType">
    <rdfs:isDefinedBy rdf:resource="http://vocab.getty.edu/ontology"/>
    <rdfs:label>placeType</rdfs:label>
    <rdfs:domain rdf:resource="http://vocab.getty.edu/ontology#Subject"/>
    <rdfs:range rdf:resource="http://vocab.getty.edu/ontology#Subject"/>
    <rdfs:comment>Type for a TGN place. Domain is TGN concept (AdminPlaceConcept or PhysPlaceConcept), range is AAT Concept</rdfs:comment>
    <skos:example>Machupicchu, Peru has preferred type "deserted settlement" (current) and non-preferred type "Inca center" (historic)</skos:example>
    <dct:description>Type for a TGN place. Domain is TGN concept (AdminPlaceConcept or PhysPlaceConcept), range is AAT Concept.
Example: Machupicchu, Peru has preferred type "deserted settlement" (current) and non-preferred type "Inca center" (historic)</dct:description>
  </owl:ObjectProperty>
  <owl:ObjectProperty rdf:about="http://vocab.getty.edu/ontology#ulan1573_ward_of">
    <rdfs:range rdf:resource="http://www.w3.org/2004/02/skos/core#Concept"/>
    <dc:identifier>1573</dc:identifier>
    <rdfs:subPropertyOf rdf:resource="http://www.w3.org/2004/02/skos/core#related"/>
    <rdfs:isDefinedBy rdf:resource="http://vocab.getty.edu/ontology"/>
    <rdfs:domain rdf:resource="http://www.w3.org/2004/02/skos/core#Concept"/>
    <skos:example>Samuel Cooper was a ward of John Hoskins, the elder</skos:example>
    <dc:title>ward of - person</dc:title>
    <skos:prefLabel>ulan1573_ward_of</skos:prefLabel>
    <dct:description>person - ward of - person.&#xD;
Example: Samuel Cooper was a ward of John Hoskins, the elder</dct:description>
    <rdfs:isDefinedBy rdf:resource="http://vocab.getty.edu/ulan/"/>
  </owl:ObjectProperty>
  <owl:ObjectProperty rdf:about="http://vocab.getty.edu/ontology#ulan1204_donor_was">
    <skos:example>Donor to the National Gallery of Art was Andrew W. Mellon</skos:example>
    <rdfs:subPropertyOf rdf:resource="http://www.w3.org/2004/02/skos/core#related"/>
    <rdfs:domain rdf:resource="http://www.w3.org/2004/02/skos/core#Concept"/>
    <skos:prefLabel>ulan1204_donor_was</skos:prefLabel>
    <rdfs:isDefinedBy rdf:resource="http://vocab.getty.edu/ulan/"/>
    <rdfs:isDefinedBy rdf:resource="http://vocab.getty.edu/ontology"/>
    <dc:title>donor was - person/firm/family</dc:title>
    <rdfs:range rdf:resource="http://www.w3.org/2004/02/skos/core#Concept"/>
    <dc:identifier>1204</dc:identifier>
    <dct:description>person/firm/family - donor was - person/firm/family.&#xD;
Example: Donor to the National Gallery of Art was Andrew W. Mellon</dct:description>
  </owl:ObjectProperty>
  <owl:ObjectProperty rdf:about="http://vocab.getty.edu/ontology#ulan1222_appointee_of">
    <rdfs:domain rdf:resource="http://www.w3.org/2004/02/skos/core#Concept"/>
    <rdfs:range rdf:resource="http://www.w3.org/2004/02/skos/core#Concept"/>
    <dc:title>appointee of - person</dc:title>
    <rdfs:isDefinedBy rdf:resource="http://vocab.getty.edu/ontology"/>
    <dc:identifier>1222</dc:identifier>
    <skos:example>Virginio Cesarini was appointee by Pope Urban VIII</skos:example>
    <rdfs:subPropertyOf rdf:resource="http://www.w3.org/2004/02/skos/core#related"/>
    <rdfs:isDefinedBy rdf:resource="http://vocab.getty.edu/ulan/"/>
    <skos:prefLabel>ulan1222_appointee_of</skos:prefLabel>
    <dct:description>person - appointee of - person.&#xD;
Example: Virginio Cesarini was appointee by Pope Urban VIII</dct:description>
  </owl:ObjectProperty>
  <owl:ObjectProperty rdf:about="http://vocab.getty.edu/ontology#aat2879_followed-developed_from">
    <rdfs:domain rdf:resource="http://www.w3.org/2004/02/skos/core#Concept"/>
    <skos:example>Greek (modern language) followed/developed from Ancient Greek (language)</skos:example>
    <dc:title>followed/developed from - language</dc:title>
    <skos:example>Egyptian, Coptic (language) followed/developed from Ancient Egyptian (language)</skos:example>
    <dc:identifier>2879</dc:identifier>
    <rdfs:isDefinedBy rdf:resource="http://vocab.getty.edu/aat/"/>
    <rdfs:range rdf:resource="http://www.w3.org/2004/02/skos/core#Concept"/>
    <dct:description>language - followed/developed from - language.&#xD;
Example: Greek (modern language) followed/developed from Ancient Greek (language); Egyptian, Coptic (language) followed/developed from Ancient Egyptian (language)</dct:description>
    <rdfs:subPropertyOf rdf:resource="http://www.w3.org/2004/02/skos/core#related"/>
    <rdfs:isDefinedBy rdf:resource="http://vocab.getty.edu/ontology"/>
    <skos:prefLabel>aat2879_followed-developed_from</skos:prefLabel>
  </owl:ObjectProperty>
  <owl:ObjectProperty rdf:about="http://vocab.getty.edu/ontology#aat2285_practiced-studied_by">
    <dc:title>practiced/studied by - role</dc:title>
    <skos:prefLabel>aat2285_practiced-studied_by</skos:prefLabel>
    <dc:identifier>2285</dc:identifier>
    <rdfs:isDefinedBy rdf:resource="http://vocab.getty.edu/ontology"/>
    <dct:description>field [of study, genre]/discipline - [is] practiced/studied by - a role.&#xD;
Example: Egyptology is practiced/studied by Egyptologists; architectural history is practiced/studied by architectural historians</dct:description>
    <skos:example>architectural history is practiced/studied by architectural historians</skos:example>
    <skos:example>Egyptology is practiced/studied by Egyptologists</skos:example>
    <owl:inverseOf>
      <owl:ObjectProperty rdf:about="http://vocab.getty.edu/ontology#aat2286_practice-study"/>
    </owl:inverseOf>
    <rdfs:isDefinedBy rdf:resource="http://vocab.getty.edu/aat/"/>
    <rdfs:range rdf:resource="http://www.w3.org/2004/02/skos/core#Concept"/>
    <rdfs:subPropertyOf rdf:resource="http://www.w3.org/2004/02/skos/core#related"/>
    <rdfs:domain rdf:resource="http://www.w3.org/2004/02/skos/core#Concept"/>
  </owl:ObjectProperty>
  <owl:ObjectProperty rdf:about="http://vocab.getty.edu/ontology#aat2801_conjuncted_with">
    <rdfs:isDefinedBy rdf:resource="http://vocab.getty.edu/aat/"/>
    <skos:example>dining tables are conjuncted with dining chairs</skos:example>
    <rdfs:isDefinedBy rdf:resource="http://vocab.getty.edu/ontology"/>
    <dct:description>things - [are] conjuncted with - things.&#xD;
Example: cups are conjuncted with saucers; dining tables are conjuncted with dining chairs</dct:description>
    <rdfs:domain rdf:resource="http://www.w3.org/2004/02/skos/core#Concept"/>
    <skos:prefLabel>aat2801_conjuncted_with</skos:prefLabel>
    <dc:title>conjuncted with - things</dc:title>
    <skos:example>cups are conjuncted with saucers</skos:example>
    <rdf:type rdf:resource="http://www.w3.org/2002/07/owl#SymmetricProperty"/>
    <dc:identifier>2801</dc:identifier>
    <rdfs:range rdf:resource="http://www.w3.org/2004/02/skos/core#Concept"/>
    <rdfs:subPropertyOf rdf:resource="http://www.w3.org/2004/02/skos/core#related"/>
  </owl:ObjectProperty>
  <owl:ObjectProperty rdf:about="http://vocab.getty.edu/ontology#biographyPreferred">
    <rdfs:isDefinedBy rdf:resource="http://vocab.getty.edu/ontology"/>
    <rdfs:label>biographyPreferred</rdfs:label>
    <rdfs:range rdf:resource="http://vocab.getty.edu/ontology#Biography"/>
    <rdfs:subPropertyOf>
      <owl:ObjectProperty rdf:about="http://vocab.getty.edu/ontology#biography"/>
    </rdfs:subPropertyOf>
    <rdfs:comment>Preferred biography of an ULAN agent. Domain is schema:Person/Organization, range is gvp:Biography. The biography fields are also directly available in the Person/Organization</rdfs:comment>
    <dct:description>Preferred biography of an ULAN agent. Domain is schema:Person/Organization, range is gvp:Biography. The biography fields are also directly available in the Person/Organization</dct:description>
  </owl:ObjectProperty>
  <owl:ObjectProperty rdf:about="http://vocab.getty.edu/ontology#ulan2781_dedicatee_of">
    <skos:example>Auguste Rodin is the dedicatee of The Rodin Museum in Philadelphia</skos:example>
    <rdfs:subPropertyOf rdf:resource="http://www.w3.org/2004/02/skos/core#related"/>
    <rdfs:domain rdf:resource="http://www.w3.org/2004/02/skos/core#Concept"/>
    <rdfs:isDefinedBy rdf:resource="http://vocab.getty.edu/ulan/"/>
    <skos:prefLabel>ulan2781_dedicatee_of</skos:prefLabel>
    <owl:inverseOf>
      <owl:ObjectProperty rdf:about="http://vocab.getty.edu/ontology#ulan2782_dedicated_to"/>
    </owl:inverseOf>
    <dc:title>dedicatee of - institution</dc:title>
    <rdfs:range rdf:resource="http://www.w3.org/2004/02/skos/core#Concept"/>
    <rdfs:isDefinedBy rdf:resource="http://vocab.getty.edu/ontology"/>
    <dct:description>person - dedicatee of - institution.&#xD;
Example: Auguste Rodin is the dedicatee of The Rodin Museum in Philadelphia</dct:description>
    <dc:identifier>2781</dc:identifier>
  </owl:ObjectProperty>
  <owl:ObjectProperty rdf:about="http://vocab.getty.edu/ontology#aat2336_has_associates">
    <rdfs:range rdf:resource="http://www.w3.org/2004/02/skos/core#Concept"/>
    <dct:description>style/period/culture/[relgion] - has associates - [actors having] role.&#xD;
Example: Abstract (fine arts style) has associates abstract artists; Roman Catholicism has associates popes</dct:description>
    <rdfs:domain rdf:resource="http://www.w3.org/2004/02/skos/core#Concept"/>
    <dc:title>has associates - role</dc:title>
    <rdfs:isDefinedBy rdf:resource="http://vocab.getty.edu/ontology"/>
    <skos:example>Abstract (fine arts style) has associates abstract artists</skos:example>
    <rdfs:isDefinedBy rdf:resource="http://vocab.getty.edu/aat/"/>
    <dc:identifier>2336</dc:identifier>
    <skos:example>Roman Catholicism has associates popes</skos:example>
    <rdfs:subPropertyOf rdf:resource="http://www.w3.org/2004/02/skos/core#related"/>
    <skos:prefLabel>aat2336_has_associates</skos:prefLabel>
  </owl:ObjectProperty>
  <owl:ObjectProperty rdf:about="http://vocab.getty.edu/ontology#aat2805_contextualized_in">
    <dc:title>contextualized in - things</dc:title>
    <skos:prefLabel>aat2805_contextualized_in</skos:prefLabel>
    <skos:example>predellas are contextualized in altarpieces</skos:example>
    <dct:description>[smaller] things - [are] contextualized in - [larger] things.&#xD;
Example: predellas are contextualized in altarpieces; chapters are contextualized in books</dct:description>
    <rdfs:isDefinedBy rdf:resource="http://vocab.getty.edu/aat/"/>
    <rdfs:subPropertyOf rdf:resource="http://www.w3.org/2004/02/skos/core#related"/>
    <owl:inverseOf>
      <owl:ObjectProperty rdf:about="http://vocab.getty.edu/ontology#aat2806_provide_context"/>
    </owl:inverseOf>
    <rdfs:range rdf:resource="http://www.w3.org/2004/02/skos/core#Concept"/>
    <skos:example>chapters are contextualized in books</skos:example>
    <dc:identifier>2805</dc:identifier>
    <rdfs:domain rdf:resource="http://www.w3.org/2004/02/skos/core#Concept"/>
    <rdfs:isDefinedBy rdf:resource="http://vocab.getty.edu/ontology"/>
  </owl:ObjectProperty>
  <owl:ObjectProperty rdf:about="http://vocab.getty.edu/ontology#ulan1106_apprentice_was">
    <dc:title>apprentice was - person</dc:title>
    <skos:example>Nicolas Hawksmoor was the apprentice of Christopher Wren</skos:example>
    <rdfs:range rdf:resource="http://www.w3.org/2004/02/skos/core#Concept"/>
    <rdfs:isDefinedBy rdf:resource="http://vocab.getty.edu/ontology"/>
    <dct:description>person - apprentice was - person.&#xD;
Example: Nicolas Hawksmoor was the apprentice of Christopher Wren</dct:description>
    <rdfs:domain rdf:resource="http://www.w3.org/2004/02/skos/core#Concept"/>
    <skos:prefLabel>ulan1106_apprentice_was</skos:prefLabel>
    <rdfs:subPropertyOf rdf:resource="http://www.w3.org/2004/02/skos/core#related"/>
    <rdfs:isDefinedBy rdf:resource="http://vocab.getty.edu/ulan/"/>
    <dc:identifier>1106</dc:identifier>
  </owl:ObjectProperty>
  <owl:ObjectProperty rdf:about="http://vocab.getty.edu/ontology#aat2881_reflected_in">
    <skos:prefLabel>aat2881_reflected_in</skos:prefLabel>
    <skos:example>Sanskrit is reflected in Vedas</skos:example>
    <dct:description>language - [is] reflected in - things.&#xD;
Example: Greek (language) is reflected in Greek alphabet; Sanskrit is reflected in Vedas</dct:description>
    <owl:inverseOf>
      <owl:ObjectProperty rdf:about="http://vocab.getty.edu/ontology#aat2882_reflect"/>
    </owl:inverseOf>
    <rdfs:subPropertyOf rdf:resource="http://www.w3.org/2004/02/skos/core#related"/>
    <rdfs:isDefinedBy rdf:resource="http://vocab.getty.edu/ontology"/>
    <rdfs:domain rdf:resource="http://www.w3.org/2004/02/skos/core#Concept"/>
    <rdfs:range rdf:resource="http://www.w3.org/2004/02/skos/core#Concept"/>
    <skos:example>Greek (language) is reflected in Greek alphabet</skos:example>
    <rdfs:isDefinedBy rdf:resource="http://vocab.getty.edu/aat/"/>
    <dc:identifier>2881</dc:identifier>
    <dc:title>reflected in - things</dc:title>
  </owl:ObjectProperty>
  <owl:ObjectProperty rdf:about="http://vocab.getty.edu/ontology#aat2333_have_affiliates">
    <rdfs:range rdf:resource="http://www.w3.org/2004/02/skos/core#Concept"/>
    <rdfs:domain rdf:resource="http://www.w3.org/2004/02/skos/core#Concept"/>
    <skos:prefLabel>aat2333_have_affiliates</skos:prefLabel>
    <rdfs:isDefinedBy rdf:resource="http://vocab.getty.edu/aat/"/>
    <dc:identifier>2333</dc:identifier>
    <rdfs:subPropertyOf rdf:resource="http://www.w3.org/2004/02/skos/core#related"/>
    <skos:example>schools (organizations) have as affiliates students</skos:example>
    <dc:title>have affiliates - role</dc:title>
    <rdfs:isDefinedBy rdf:resource="http://vocab.getty.edu/ontology"/>
    <dct:description>role [organizations] - have affiliates - [actors having] role.&#xD;
Example: schools (organizations) have as affiliates students; duchies have as affiliates dukes</dct:description>
    <skos:example>duchies have as affiliates dukes</skos:example>
  </owl:ObjectProperty>
  <owl:ObjectProperty rdf:about="http://vocab.getty.edu/ontology#broader">
    <rdfs:isDefinedBy rdf:resource="http://vocab.getty.edu/ontology"/>
    <rdfs:label>broader</rdfs:label>
    <rdfs:domain rdf:resource="http://vocab.getty.edu/ontology#Subject"/>
    <rdfs:range rdf:resource="http://vocab.getty.edu/ontology#Subject"/>
    <rdfs:comment>Parents of a subject. Each broader is also Preferred|NonPreferred and Partitive|Instantial|Generic</rdfs:comment>
    <dct:description>Parents of a subject. Each broader is also Preferred|NonPreferred and Partitive|Instantial|Generic</dct:description>
  </owl:ObjectProperty>
  <owl:ObjectProperty rdf:about="http://vocab.getty.edu/ontology#aat2504_used-located_in">
    <owl:inverseOf>
      <owl:ObjectProperty rdf:about="http://vocab.getty.edu/ontology#aat2505_locus-setting_for"/>
    </owl:inverseOf>
    <dct:description>material - [is] used/located in - locus/setting.&#xD;
Example: tephra is used/located in [at] volcanoes; brick (clay product) is used/located in brickworks (factories)</dct:description>
    <skos:example>brick (clay product) is used/located in brickworks (factories)</skos:example>
    <dc:title>used/located in - locus/setting</dc:title>
    <skos:prefLabel>aat2504_used-located_in</skos:prefLabel>
    <rdfs:isDefinedBy rdf:resource="http://vocab.getty.edu/aat/"/>
    <skos:example>tephra is used/located in [at] volcanoes</skos:example>
    <rdfs:range rdf:resource="http://www.w3.org/2004/02/skos/core#Concept"/>
    <rdfs:isDefinedBy rdf:resource="http://vocab.getty.edu/ontology"/>
    <rdfs:domain rdf:resource="http://www.w3.org/2004/02/skos/core#Concept"/>
    <rdfs:subPropertyOf rdf:resource="http://www.w3.org/2004/02/skos/core#related"/>
    <dc:identifier>2504</dc:identifier>
  </owl:ObjectProperty>
  <owl:ObjectProperty rdf:about="http://vocab.getty.edu/ontology#aat2415_required_for">
    <rdfs:isDefinedBy rdf:resource="http://vocab.getty.edu/aat/"/>
    <owl:inverseOf>
      <owl:ObjectProperty rdf:about="http://vocab.getty.edu/ontology#aat2416_requires"/>
    </owl:inverseOf>
    <dc:title>required for - activity/event</dc:title>
    <rdfs:subPropertyOf rdf:resource="http://www.w3.org/2004/02/skos/core#related"/>
    <skos:example>pewter is required for pewtersmithing</skos:example>
    <rdfs:domain rdf:resource="http://www.w3.org/2004/02/skos/core#Concept"/>
    <rdfs:isDefinedBy rdf:resource="http://vocab.getty.edu/ontology"/>
    <dc:identifier>2415</dc:identifier>
    <rdfs:range rdf:resource="http://www.w3.org/2004/02/skos/core#Concept"/>
    <dct:description>material - [is] required for - activity/event/[process/function].&#xD;
Example: dye is required for dying; pewter is required for pewtersmithing</dct:description>
    <skos:prefLabel>aat2415_required_for</skos:prefLabel>
    <skos:example>dye is required for dying</skos:example>
  </owl:ObjectProperty>
  <owl:ObjectProperty rdf:about="http://vocab.getty.edu/ontology#aat2312_perform">
    <rdfs:domain rdf:resource="http://www.w3.org/2004/02/skos/core#Concept"/>
    <skos:example>curators perform curating</skos:example>
    <skos:prefLabel>aat2312_perform</skos:prefLabel>
    <dc:identifier>2312</dc:identifier>
    <rdfs:subPropertyOf rdf:resource="http://www.w3.org/2004/02/skos/core#related"/>
    <rdfs:range rdf:resource="http://www.w3.org/2004/02/skos/core#Concept"/>
    <skos:example>clockmakers perform clockmaking</skos:example>
    <rdfs:isDefinedBy rdf:resource="http://vocab.getty.edu/ontology"/>
    <dct:description>[actors having] a role - perform - activity/event/process.&#xD;
Example: clockmakers perform clockmaking; curators perform curating</dct:description>
    <dc:title>perform - activity/event</dc:title>
    <rdfs:isDefinedBy rdf:resource="http://vocab.getty.edu/aat/"/>
  </owl:ObjectProperty>
  <owl:ObjectProperty rdf:about="http://vocab.getty.edu/ontology#aat2836_derived-made_from">
    <rdfs:range rdf:resource="http://www.w3.org/2004/02/skos/core#Concept"/>
    <dc:title>derived/made from - genus/species</dc:title>
    <rdfs:isDefinedBy rdf:resource="http://vocab.getty.edu/ontology"/>
    <owl:inverseOf>
      <owl:ObjectProperty rdf:about="http://vocab.getty.edu/ontology#aat2837_source_for"/>
    </owl:inverseOf>
    <dc:identifier>2836</dc:identifier>
    <skos:example>k?kaku are derived/made from Phormium tenax (species)</skos:example>
    <dct:description>things - [are] derived/made from - genus/species [or its parts].&#xD;
Example: k?kaku are derived/made from Phormium tenax (species); ostrich-egg cups are derived/made from Struthio camelus (species)</dct:description>
    <rdfs:subPropertyOf rdf:resource="http://www.w3.org/2004/02/skos/core#related"/>
    <skos:example>ostrich-egg cups are derived/made from Struthio camelus (species)</skos:example>
    <rdfs:domain rdf:resource="http://www.w3.org/2004/02/skos/core#Concept"/>
    <skos:prefLabel>aat2836_derived-made_from</skos:prefLabel>
    <rdfs:isDefinedBy rdf:resource="http://vocab.getty.edu/aat/"/>
  </owl:ObjectProperty>
  <owl:ObjectProperty rdf:about="http://vocab.getty.edu/ontology#tgn3612_administrative_entity_for">
    <rdfs:isDefinedBy rdf:resource="http://vocab.getty.edu/tgn/"/>
    <rdfs:range rdf:resource="http://www.w3.org/2004/02/skos/core#Concept"/>
    <rdfs:subPropertyOf rdf:resource="http://www.w3.org/2004/02/skos/core#related"/>
    <skos:example>Ortonovo (Massa-Carra province, Tuscany, Italy) is the administrative entity for Luni (La Spezia province, Liguria, Italy)</skos:example>
    <dc:title>administrative entity for - place</dc:title>
    <dct:description>place - administrative entity for - place.&#xD;
Example: Ortonovo (Massa-Carra province, Tuscany, Italy) is the administrative entity for Luni (La Spezia province, Liguria, Italy)</dct:description>
    <rdfs:isDefinedBy rdf:resource="http://vocab.getty.edu/ontology"/>
    <rdfs:domain rdf:resource="http://www.w3.org/2004/02/skos/core#Concept"/>
    <dc:identifier>3612</dc:identifier>
    <skos:prefLabel>tgn3612_administrative_entity_for</skos:prefLabel>
  </owl:ObjectProperty>
  <owl:ObjectProperty rdf:about="http://vocab.getty.edu/ontology#aat2110_meaning-usage_overlaps_with">
    <rdfs:subPropertyOf rdf:resource="http://www.w3.org/2004/02/skos/core#related"/>
    <rdfs:isDefinedBy rdf:resource="http://vocab.getty.edu/ontology"/>
    <skos:example>scribes has meaning/usage that overlaps with copyists</skos:example>
    <rdf:type rdf:resource="http://www.w3.org/2002/07/owl#SymmetricProperty"/>
    <dc:identifier>2110</dc:identifier>
    <skos:prefLabel>aat2110_meaning-usage_overlaps_with</skos:prefLabel>
    <dc:title>meaning/usage overlaps with - any</dc:title>
    <rdfs:range rdf:resource="http://www.w3.org/2004/02/skos/core#Concept"/>
    <rdfs:domain rdf:resource="http://www.w3.org/2004/02/skos/core#Concept"/>
    <rdfs:isDefinedBy rdf:resource="http://vocab.getty.edu/aat/"/>
    <skos:example>chimney hoods has meaning/usage that overlaps with chimney caps</skos:example>
    <dct:description>any - meaning/usage overlaps with - any.&#xD;
Example: chimney hoods has meaning/usage that overlaps with chimney caps; scribes has meaning/usage that overlaps with copyists</dct:description>
  </owl:ObjectProperty>
  <owl:ObjectProperty rdf:about="http://vocab.getty.edu/ontology#ulan1331_worked_with">
    <skos:example>Scarsellino and Domenichino worked with the Carracci family</skos:example>
    <rdfs:subPropertyOf rdf:resource="http://www.w3.org/2004/02/skos/core#related"/>
    <dc:title>worked with - person</dc:title>
    <dc:identifier>1331</dc:identifier>
    <owl:inverseOf>
      <owl:ObjectProperty rdf:about="http://vocab.getty.edu/ontology#ulan1332_worker_was"/>
    </owl:inverseOf>
    <skos:prefLabel>ulan1331_worked_with</skos:prefLabel>
    <rdfs:range rdf:resource="http://www.w3.org/2004/02/skos/core#Concept"/>
    <rdfs:isDefinedBy rdf:resource="http://vocab.getty.edu/ulan/"/>
    <rdfs:isDefinedBy rdf:resource="http://vocab.getty.edu/ontology"/>
    <dct:description>any - worked with - person.&#xD;
Example: Scarsellino and Domenichino worked with the Carracci family</dct:description>
    <rdfs:domain rdf:resource="http://www.w3.org/2004/02/skos/core#Concept"/>
  </owl:ObjectProperty>
  <owl:ObjectProperty rdf:about="http://vocab.getty.edu/ontology#broaderExtended">
    <rdfs:isDefinedBy rdf:resource="http://vocab.getty.edu/ontology"/>
    <rdfs:label>broaderExtended</rdfs:label>
    <rdfs:domain rdf:resource="http://vocab.getty.edu/ontology#Subject"/>
    <rdfs:range rdf:resource="http://vocab.getty.edu/ontology#Subject"/>
    <rdfs:comment>Appropriate ancestors. Meaningful closure of gvp:broader for query expansion. Use this, not skos:broaderTransitive</rdfs:comment>
    <skos:example>Mt Athos has ancestor places (BTPE) World, Europe, Greece, Macedonia, Pangaon ros regional division;
and place types (BTIE) inhabited place; and orthodox religious center, Christian religious center, religious center</skos:example>
    <dct:description>Appropriate ancestors. Meaningful closure of gvp:broader for query expansion. Use this, not skos:broaderTransitive.
Example: Mt Athos has ancestor places (BTPE) World, Europe, Greece, Macedonia, Pangaon ros regional division;
and place types (BTIE) inhabited place; and orthodox religious center, Christian religious center, religious center</dct:description>
  </owl:ObjectProperty>
  <owl:ObjectProperty rdf:about="http://vocab.getty.edu/ontology#aat2829_used-required_for">
    <rdfs:subPropertyOf rdf:resource="http://www.w3.org/2004/02/skos/core#related"/>
    <rdfs:isDefinedBy rdf:resource="http://vocab.getty.edu/ontology"/>
    <dc:title>used/required for - things</dc:title>
    <skos:prefLabel>aat2829_used-required_for</skos:prefLabel>
    <skos:example>varnish is used/required for oil paintings</skos:example>
    <rdfs:isDefinedBy rdf:resource="http://vocab.getty.edu/aat/"/>
    <rdfs:range rdf:resource="http://www.w3.org/2004/02/skos/core#Concept"/>
    <dc:identifier>2829</dc:identifier>
    <skos:example>wine is required/used for wine glasses</skos:example>
    <dct:description>material - [is] required/used for - things.&#xD;
Example: varnish is used/required for oil paintings; wine is required/used for wine glasses</dct:description>
    <rdfs:domain rdf:resource="http://www.w3.org/2004/02/skos/core#Concept"/>
  </owl:ObjectProperty>
  <owl:ObjectProperty rdf:about="http://vocab.getty.edu/ontology#aat2803_example_of">
    <rdfs:isDefinedBy rdf:resource="http://vocab.getty.edu/ontology"/>
    <rdfs:subPropertyOf rdf:resource="http://www.w3.org/2004/02/skos/core#related"/>
    <skos:prefLabel>aat2803_example_of</skos:prefLabel>
    <rdfs:domain rdf:resource="http://www.w3.org/2004/02/skos/core#Concept"/>
    <skos:example>Vaseline (TM) is an example of petrolium jelly</skos:example>
    <dc:title>example of - material</dc:title>
    <dct:description>brand name - [is] example of - material.&#xD;
Example: Vaseline (TM) is an example of petrolium jelly; Teflon (TM) is an example of polytetrafluoroethyelene</dct:description>
    <rdfs:range rdf:resource="http://www.w3.org/2004/02/skos/core#Concept"/>
    <skos:example>Teflon (TM) is an example of polytetrafluoroethyelene</skos:example>
    <dc:identifier>2803</dc:identifier>
    <rdfs:isDefinedBy rdf:resource="http://vocab.getty.edu/aat/"/>
  </owl:ObjectProperty>
  <owl:ObjectProperty rdf:about="http://vocab.getty.edu/ontology#prefLabelLoC">
    <rdfs:isDefinedBy rdf:resource="http://vocab.getty.edu/ontology"/>
    <rdfs:label>prefLabelLoC</rdfs:label>
    <rdfs:domain rdf:resource="http://vocab.getty.edu/ontology#Subject"/>
    <rdfs:range rdf:resource="http://www.w3.org/2008/05/skos-xl#Label"/>
    <rdfs:comment>Term preferred by Library of Congress, thus used for cataloging according to AACR2. Applicable to AAT and ULAN. Used with skosxl:prefLabel</rdfs:comment>
    <dct:description>Term preferred by Library of Congress, thus used for cataloging according to AACR2. Applicable to AAT and ULAN. Used with skosxl:prefLabel</dct:description>
  </owl:ObjectProperty>
  <owl:ObjectProperty rdf:about="http://vocab.getty.edu/ontology#contributorNonPreferred">
    <rdfs:isDefinedBy rdf:resource="http://vocab.getty.edu/ontology"/>
    <rdfs:label>contributorNonPreferred</rdfs:label>
    <rdfs:domain rdf:resource="http://www.w3.org/2008/05/skos-xl#Label"/>
    <rdfs:range rdf:resource="http://xmlns.com/foaf/0.1/Agent"/>
    <rdfs:subPropertyOf rdf:resource="http://purl.org/dc/terms/contributor"/>
    <rdfs:comment>Contributor for which the term is Non-preferred. Range is foaf:Agent</rdfs:comment>
    <skos:example>"Lycra" is non-preferred term for WHS</skos:example>
    <dct:description>Contributor for which the term is Non-preferred. Range is foaf:Agent.
Example: "Lycra" is non-preferred term for WHS</dct:description>
  </owl:ObjectProperty>
  <owl:ObjectProperty rdf:about="http://vocab.getty.edu/ontology#aat2427_produced_by">
    <rdfs:isDefinedBy rdf:resource="http://vocab.getty.edu/ontology"/>
    <skos:example>forgeries are produced by forging (copying)</skos:example>
    <rdfs:domain rdf:resource="http://www.w3.org/2004/02/skos/core#Concept"/>
    <dct:description>things - [are] produced by - activity/event/process.&#xD;
Example: vase paintings (visual works) are produced by vase painting (image making); forgeries are produced by forging (copying)</dct:description>
    <rdfs:subPropertyOf rdf:resource="http://www.w3.org/2004/02/skos/core#related"/>
    <skos:prefLabel>aat2427_produced_by</skos:prefLabel>
    <owl:inverseOf>
      <owl:ObjectProperty rdf:about="http://vocab.getty.edu/ontology#aat2428_produces"/>
    </owl:inverseOf>
    <rdfs:isDefinedBy rdf:resource="http://vocab.getty.edu/aat/"/>
    <skos:example>vase paintings (visual works) are produced by vase painting (image making)</skos:example>
    <dc:title>produced by - activity/event/process</dc:title>
    <rdfs:range rdf:resource="http://www.w3.org/2004/02/skos/core#Concept"/>
    <dc:identifier>2427</dc:identifier>
  </owl:ObjectProperty>
  <owl:ObjectProperty rdf:about="http://vocab.getty.edu/ontology#biographyNonPreferred">
    <rdfs:isDefinedBy rdf:resource="http://vocab.getty.edu/ontology"/>
    <rdfs:label>biographyNonPreferred</rdfs:label>
    <rdfs:range rdf:resource="http://vocab.getty.edu/ontology#Biography"/>
    <rdfs:subPropertyOf>
      <owl:ObjectProperty rdf:about="http://vocab.getty.edu/ontology#biography"/>
    </rdfs:subPropertyOf>
    <rdfs:comment>Non-preferred biography of an ULAN agent. Domain is schema:Person/Organization, range is gvp:Biography</rdfs:comment>
    <dct:description>Non-preferred biography of an ULAN agent. Domain is schema:Person/Organization, range is gvp:Biography</dct:description>
  </owl:ObjectProperty>
  <owl:ObjectProperty rdf:about="http://vocab.getty.edu/ontology#aat2602_possess-exist_in">
    <rdfs:subPropertyOf rdf:resource="http://www.w3.org/2004/02/skos/core#related"/>
    <skos:example>nomads possess/exist in [state of] nomadism</skos:example>
    <skos:example>adults possess/exist in adulthood</skos:example>
    <skos:prefLabel>aat2602_possess-exist_in</skos:prefLabel>
    <rdfs:domain rdf:resource="http://www.w3.org/2004/02/skos/core#Concept"/>
    <dc:identifier>2602</dc:identifier>
    <rdfs:isDefinedBy rdf:resource="http://vocab.getty.edu/ontology"/>
    <rdfs:range rdf:resource="http://www.w3.org/2004/02/skos/core#Concept"/>
    <dct:description>role [of actors] - possess/exist in - attributes /associated concepts.&#xD;
Example: adults possess/exist in adulthood; nomads possess/exist in [state of] nomadism</dct:description>
    <dc:title>possess/exist in - attributes /associated concepts</dc:title>
    <rdfs:isDefinedBy rdf:resource="http://vocab.getty.edu/aat/"/>
  </owl:ObjectProperty>
  <owl:ObjectProperty rdf:about="http://vocab.getty.edu/ontology#aat2849_involves">
    <rdfs:domain rdf:resource="http://www.w3.org/2004/02/skos/core#Concept"/>
    <skos:example>bullfighting involves bulls (animals)</skos:example>
    <dct:description>activity/event - involves - genus/species.&#xD;
Example: bullfighting involves bulls (animals); polo (field sport) involves Equus caballus (species)</dct:description>
    <skos:example>polo (field sport) involves Equus caballus (species)</skos:example>
    <dc:identifier>2849</dc:identifier>
    <skos:prefLabel>aat2849_involves</skos:prefLabel>
    <rdfs:range rdf:resource="http://www.w3.org/2004/02/skos/core#Concept"/>
    <rdfs:subPropertyOf rdf:resource="http://www.w3.org/2004/02/skos/core#related"/>
    <rdfs:isDefinedBy rdf:resource="http://vocab.getty.edu/ontology"/>
    <dc:title>involves - genus/species</dc:title>
    <rdfs:isDefinedBy rdf:resource="http://vocab.getty.edu/aat/"/>
  </owl:ObjectProperty>
  <owl:ObjectProperty rdf:about="http://vocab.getty.edu/ontology#ulan1552_parent_by_marriage_of">
    <dc:identifier>1552</dc:identifier>
    <owl:inverseOf rdf:resource="http://vocab.getty.edu/ontology#ulan1553_child_by_marriage_of"/>
    <rdfs:domain rdf:resource="http://www.w3.org/2004/02/skos/core#Concept"/>
    <rdfs:isDefinedBy rdf:resource="http://vocab.getty.edu/ulan/"/>
    <rdfs:isDefinedBy rdf:resource="http://vocab.getty.edu/ontology"/>
    <skos:example>Frans Hals is a parent by marriage of Pieter Gerritsz van Roestraten</skos:example>
    <rdfs:range rdf:resource="http://www.w3.org/2004/02/skos/core#Concept"/>
    <rdfs:subPropertyOf rdf:resource="http://www.w3.org/2004/02/skos/core#related"/>
    <dct:description>person - parent by marriage (step parent) - person.&#xD;
Example: Frans Hals is a parent by marriage of Pieter Gerritsz van Roestraten</dct:description>
    <dc:title>parent by marriage of - person</dc:title>
    <skos:prefLabel>ulan1552_parent_by_marriage_of</skos:prefLabel>
  </owl:ObjectProperty>
  <owl:ObjectProperty rdf:about="http://vocab.getty.edu/ontology#ulan1105_apprentice_of">
    <rdfs:isDefinedBy rdf:resource="http://vocab.getty.edu/ulan/"/>
    <rdfs:subPropertyOf rdf:resource="http://www.w3.org/2004/02/skos/core#related"/>
    <rdfs:isDefinedBy rdf:resource="http://vocab.getty.edu/ontology"/>
    <dc:identifier>1105</dc:identifier>
    <skos:example>Nicolas Hawksmoor was the apprentice of Christopher Wren</skos:example>
    <skos:prefLabel>ulan1105_apprentice_of</skos:prefLabel>
    <dct:description>person - apprentice of - person.&#xD;
Example: Nicolas Hawksmoor was the apprentice of Christopher Wren</dct:description>
    <rdfs:domain rdf:resource="http://www.w3.org/2004/02/skos/core#Concept"/>
    <owl:inverseOf rdf:resource="http://vocab.getty.edu/ontology#ulan1106_apprentice_was"/>
    <dc:title>apprentice of - person</dc:title>
    <rdfs:range rdf:resource="http://www.w3.org/2004/02/skos/core#Concept"/>
  </owl:ObjectProperty>
  <owl:ObjectProperty rdf:about="http://vocab.getty.edu/ontology#aat2551_reflect-produced_by">
    <rdfs:isDefinedBy rdf:resource="http://vocab.getty.edu/aat/"/>
    <skos:example>Judaica reflects/is produced by Judaism</skos:example>
    <dct:description>things - reflect/[are] produced by - style/period/culture/[religion/ideology].&#xD;
Example: Nasca lines reflect/are produced by Nasca [culture]; Judaica reflects/is produced by Judaism</dct:description>
    <rdfs:range rdf:resource="http://www.w3.org/2004/02/skos/core#Concept"/>
    <skos:prefLabel>aat2551_reflect-produced_by</skos:prefLabel>
    <dc:identifier>2551</dc:identifier>
    <rdfs:isDefinedBy rdf:resource="http://vocab.getty.edu/ontology"/>
    <dc:title>reflect/produced by - style/period/culture</dc:title>
    <owl:inverseOf>
      <owl:ObjectProperty rdf:about="http://vocab.getty.edu/ontology#aat2552_reflected_in-produces"/>
    </owl:inverseOf>
    <skos:example>Nasca lines reflect/are produced by Nasca [culture]</skos:example>
    <rdfs:domain rdf:resource="http://www.w3.org/2004/02/skos/core#Concept"/>
    <rdfs:subPropertyOf rdf:resource="http://www.w3.org/2004/02/skos/core#related"/>
  </owl:ObjectProperty>
  <owl:ObjectProperty rdf:about="http://vocab.getty.edu/ontology#aat2501_made_of-require">
    <dc:title>made of/require - material</dc:title>
    <dct:description>things - [are] made of/require - material.&#xD;
Example: obsidian mirrors are made of/require obsidian; ivories (sculptures) are made of/require ivory</dct:description>
    <rdfs:isDefinedBy rdf:resource="http://vocab.getty.edu/aat/"/>
    <rdfs:range rdf:resource="http://www.w3.org/2004/02/skos/core#Concept"/>
    <rdfs:subPropertyOf rdf:resource="http://www.w3.org/2004/02/skos/core#related"/>
    <rdfs:domain rdf:resource="http://www.w3.org/2004/02/skos/core#Concept"/>
    <owl:inverseOf>
      <owl:ObjectProperty rdf:about="http://vocab.getty.edu/ontology#aat2502_material_for"/>
    </owl:inverseOf>
    <skos:example>ivories (sculptures) are made of/require ivory</skos:example>
    <dc:identifier>2501</dc:identifier>
    <skos:prefLabel>aat2501_made_of-require</skos:prefLabel>
    <rdfs:isDefinedBy rdf:resource="http://vocab.getty.edu/ontology"/>
    <skos:example>obsidian mirrors are made of/require obsidian</skos:example>
  </owl:ObjectProperty>
  <owl:ObjectProperty rdf:about="http://vocab.getty.edu/ontology#aat2555_reflected_in">
    <dc:title>reflected in - activity/event</dc:title>
    <dct:description>style/period/culture /[religion/ideology] - [is] reflected in activity/event.&#xD;
Example: Dhokra (culture) is reflected in dhokra (casting technique); Red-figure [style] is reflected in red-figure vase painting</dct:description>
    <rdfs:isDefinedBy rdf:resource="http://vocab.getty.edu/ontology"/>
    <skos:prefLabel>aat2555_reflected_in</skos:prefLabel>
    <rdfs:isDefinedBy rdf:resource="http://vocab.getty.edu/aat/"/>
    <dc:identifier>2555</dc:identifier>
    <rdfs:range rdf:resource="http://www.w3.org/2004/02/skos/core#Concept"/>
    <skos:example>Dhokra (culture) is reflected in dhokra (casting technique)</skos:example>
    <skos:example>Red-figure [style] is reflected in red-figure vase painting</skos:example>
    <rdfs:domain rdf:resource="http://www.w3.org/2004/02/skos/core#Concept"/>
    <rdfs:subPropertyOf rdf:resource="http://www.w3.org/2004/02/skos/core#related"/>
  </owl:ObjectProperty>
  <owl:ObjectProperty rdf:about="http://vocab.getty.edu/ontology#tgn3103_located_on">
    <rdfs:domain rdf:resource="http://www.w3.org/2004/02/skos/core#Concept"/>
    <owl:inverseOf>
      <owl:ObjectProperty rdf:about="http://vocab.getty.edu/ontology#tgn3104_is_location_of"/>
    </owl:inverseOf>
    <rdfs:isDefinedBy rdf:resource="http://vocab.getty.edu/ontology"/>
    <rdfs:range rdf:resource="http://www.w3.org/2004/02/skos/core#Concept"/>
    <skos:example>tgn:7018835 Palmyra is located on tgn:7031416 Silk Road</skos:example>
    <dc:title>located on - place</dc:title>
    <rdfs:subPropertyOf rdf:resource="http://www.w3.org/2004/02/skos/core#related"/>
    <dct:description>place - located on - place.&#xD;
Example: tgn:7018835 Palmyra is located on tgn:7031416 Silk Road</dct:description>
    <rdfs:isDefinedBy rdf:resource="http://vocab.getty.edu/tgn/"/>
    <skos:prefLabel>tgn3103_located_on</skos:prefLabel>
    <dc:identifier>3103</dc:identifier>
  </owl:ObjectProperty>
  <owl:ObjectProperty rdf:about="http://vocab.getty.edu/ontology#aat2887_exemplified_by">
    <rdfs:range rdf:resource="http://www.w3.org/2004/02/skos/core#Concept"/>
    <skos:example>solvent - exemplified by - carbon disulfide</skos:example>
    <rdfs:isDefinedBy rdf:resource="http://vocab.getty.edu/aat/"/>
    <rdfs:domain rdf:resource="http://www.w3.org/2004/02/skos/core#Concept"/>
    <rdfs:subPropertyOf rdf:resource="http://www.w3.org/2004/02/skos/core#related"/>
    <dct:description>material - exemplified by - material.&#xD;
Example: solvent - exemplified by - carbon disulfide</dct:description>
    <rdfs:isDefinedBy rdf:resource="http://vocab.getty.edu/ontology"/>
    <dc:identifier>2887</dc:identifier>
    <skos:prefLabel>aat2887_exemplified_by</skos:prefLabel>
    <dc:title>exemplified by - material</dc:title>
  </owl:ObjectProperty>
  <owl:ObjectProperty rdf:about="http://vocab.getty.edu/ontology#ulan1315_principal_in">
    <rdfs:isDefinedBy rdf:resource="http://vocab.getty.edu/ulan/"/>
    <rdfs:range rdf:resource="http://www.w3.org/2004/02/skos/core#Concept"/>
    <dc:title>principal in - firm</dc:title>
    <rdfs:subPropertyOf rdf:resource="http://www.w3.org/2004/02/skos/core#related"/>
    <rdfs:isDefinedBy rdf:resource="http://vocab.getty.edu/ontology"/>
    <rdfs:domain rdf:resource="http://www.w3.org/2004/02/skos/core#Concept"/>
    <owl:inverseOf>
      <owl:ObjectProperty rdf:about="http://vocab.getty.edu/ontology#ulan1316_principal_was"/>
    </owl:inverseOf>
    <dct:description>person - principal in - firm.&#xD;
Example: Principal in Fontana Workshop was Orazio Fontana</dct:description>
    <skos:prefLabel>ulan1315_principal_in</skos:prefLabel>
    <skos:example>Principal in Fontana Workshop was Orazio Fontana</skos:example>
    <dc:identifier>1315</dc:identifier>
  </owl:ObjectProperty>
  <owl:ObjectProperty rdf:about="http://vocab.getty.edu/ontology#aat2822_basis_of">
    <rdfs:isDefinedBy rdf:resource="http://vocab.getty.edu/ontology"/>
    <rdfs:isDefinedBy rdf:resource="http://vocab.getty.edu/aat/"/>
    <rdfs:domain rdf:resource="http://www.w3.org/2004/02/skos/core#Concept"/>
    <skos:example>plummets are the basis of pencils</skos:example>
    <rdfs:subPropertyOf rdf:resource="http://www.w3.org/2004/02/skos/core#related"/>
    <rdfs:range rdf:resource="http://www.w3.org/2004/02/skos/core#Concept"/>
    <dct:description>any - [is] basis of - any.&#xD;
Example: Gothic (Medieval) is the basis of Neo-Gothic; curves (geometric figures) are the basis of curved [form attribute]; plummets are the basis of pencils</dct:description>
    <skos:prefLabel>aat2822_basis_of</skos:prefLabel>
    <skos:example>Gothic (Medieval) is the basis of Neo-Gothic</skos:example>
    <dc:title>basis of - any</dc:title>
    <skos:example>curves (geometric figures) are the basis of curved [form attribute]</skos:example>
    <dc:identifier>2822</dc:identifier>
  </owl:ObjectProperty>
  <owl:ObjectProperty rdf:about="http://vocab.getty.edu/ontology#ulan2576_patron_of">
    <dc:title>patron of - person</dc:title>
    <skos:prefLabel>ulan2576_patron_of</skos:prefLabel>
    <dct:description>person - patron of - person.&#xD;
Example: The patron of William Chambers was James Caulfiel, Earl of Charlemont</dct:description>
    <rdfs:isDefinedBy rdf:resource="http://vocab.getty.edu/ontology"/>
    <dc:identifier>2576</dc:identifier>
    <rdfs:subPropertyOf rdf:resource="http://www.w3.org/2004/02/skos/core#related"/>
    <rdfs:domain rdf:resource="http://www.w3.org/2004/02/skos/core#Concept"/>
    <owl:inverseOf rdf:resource="http://vocab.getty.edu/ontology#ulan2577_patron_was"/>
    <rdfs:range rdf:resource="http://www.w3.org/2004/02/skos/core#Concept"/>
    <skos:example>The patron of William Chambers was James Caulfiel, Earl of Charlemont</skos:example>
    <rdfs:isDefinedBy rdf:resource="http://vocab.getty.edu/ulan/"/>
  </owl:ObjectProperty>
  <owl:ObjectProperty rdf:about="http://vocab.getty.edu/ontology#tgn3202_capital_is">
    <rdfs:domain rdf:resource="http://www.w3.org/2004/02/skos/core#Concept"/>
    <rdfs:subPropertyOf rdf:resource="http://www.w3.org/2004/02/skos/core#related"/>
    <dc:title>capital is - city</dc:title>
    <dc:identifier>3202</dc:identifier>
    <rdfs:isDefinedBy rdf:resource="http://vocab.getty.edu/ontology"/>
    <dct:description>nation - capital is - city.&#xD;
Example: London was the capital of Maxima Caesariensis from 296 to 800 CE</dct:description>
    <skos:example>London was the capital of Maxima Caesariensis from 296 to 800 CE</skos:example>
    <rdfs:isDefinedBy rdf:resource="http://vocab.getty.edu/tgn/"/>
    <rdfs:range rdf:resource="http://www.w3.org/2004/02/skos/core#Concept"/>
    <skos:prefLabel>tgn3202_capital_is</skos:prefLabel>
  </owl:ObjectProperty>
  <owl:ObjectProperty rdf:about="http://vocab.getty.edu/ontology#aat2806_provide_context">
    <skos:example>altarpieces provide context for predellas</skos:example>
    <rdfs:isDefinedBy rdf:resource="http://vocab.getty.edu/aat/"/>
    <dct:description>[larger] things - provide context [for] - [smaller] things.&#xD;
Example: altarpieces provide context for predellas; books provide context for chapters</dct:description>
    <rdfs:domain rdf:resource="http://www.w3.org/2004/02/skos/core#Concept"/>
    <rdfs:isDefinedBy rdf:resource="http://vocab.getty.edu/ontology"/>
    <rdfs:range rdf:resource="http://www.w3.org/2004/02/skos/core#Concept"/>
    <skos:example>books provide context for chapters</skos:example>
    <dc:identifier>2806</dc:identifier>
    <skos:prefLabel>aat2806_provide_context</skos:prefLabel>
    <dc:title>provide context - things</dc:title>
    <rdfs:subPropertyOf rdf:resource="http://www.w3.org/2004/02/skos/core#related"/>
  </owl:ObjectProperty>
  <owl:ObjectProperty rdf:about="http://vocab.getty.edu/ontology#ulan1218_employee_was">
    <rdfs:subPropertyOf rdf:resource="http://www.w3.org/2004/02/skos/core#related"/>
    <rdfs:range rdf:resource="http://www.w3.org/2004/02/skos/core#Concept"/>
    <dc:identifier>1218</dc:identifier>
    <rdfs:isDefinedBy rdf:resource="http://vocab.getty.edu/ontology"/>
    <rdfs:domain rdf:resource="http://www.w3.org/2004/02/skos/core#Concept"/>
    <skos:prefLabel>ulan1218_employee_was</skos:prefLabel>
    <skos:example>Jean Tijou was an employee of Christopher Wren</skos:example>
    <dc:title>employee was - person/firm</dc:title>
    <dct:description>person - employee was - person/firm.&#xD;
Example: Jean Tijou was an employee of Christopher Wren</dct:description>
    <rdfs:isDefinedBy rdf:resource="http://vocab.getty.edu/ulan/"/>
  </owl:ObjectProperty>
  <owl:ObjectProperty rdf:about="http://vocab.getty.edu/ontology#ulan1554_adoptive_parent_of">
    <rdfs:domain rdf:resource="http://www.w3.org/2004/02/skos/core#Concept"/>
    <skos:example>Julius Caesar is the adoptive parent of Augustus, Emperor of Rome</skos:example>
    <skos:prefLabel>ulan1554_adoptive_parent_of</skos:prefLabel>
    <rdfs:subPropertyOf rdf:resource="http://www.w3.org/2004/02/skos/core#related"/>
    <dc:identifier>1554</dc:identifier>
    <dc:title>adoptive parent of - person</dc:title>
    <rdfs:isDefinedBy rdf:resource="http://vocab.getty.edu/ontology"/>
    <owl:inverseOf>
      <owl:ObjectProperty rdf:about="http://vocab.getty.edu/ontology#ulan1555_adopted_child_of"/>
    </owl:inverseOf>
    <rdfs:isDefinedBy rdf:resource="http://vocab.getty.edu/ulan/"/>
    <rdfs:range rdf:resource="http://www.w3.org/2004/02/skos/core#Concept"/>
    <dct:description>person - adoptive parent of - person.&#xD;
Example: Julius Caesar is the adoptive parent of Augustus, Emperor of Rome</dct:description>
  </owl:ObjectProperty>
  <owl:ObjectProperty rdf:about="http://vocab.getty.edu/ontology#aat2335_associated_with">
    <dc:identifier>2335</dc:identifier>
    <skos:example>popes are associated with Roman Catholicism</skos:example>
    <skos:example>abstract artists are associated with Abstract (fine arts style)</skos:example>
    <owl:inverseOf rdf:resource="http://vocab.getty.edu/ontology#aat2336_has_associates"/>
    <skos:prefLabel>aat2335_associated_with</skos:prefLabel>
    <rdfs:isDefinedBy rdf:resource="http://vocab.getty.edu/ontology"/>
    <rdfs:domain rdf:resource="http://www.w3.org/2004/02/skos/core#Concept"/>
    <rdfs:isDefinedBy rdf:resource="http://vocab.getty.edu/aat/"/>
    <rdfs:subPropertyOf rdf:resource="http://www.w3.org/2004/02/skos/core#related"/>
    <dc:title>associated with - style/period/culture</dc:title>
    <rdfs:range rdf:resource="http://www.w3.org/2004/02/skos/core#Concept"/>
    <dct:description>[actors having] role - [are] associated with - style/period/culture/[religion/ideology].&#xD;
Example: abstract artists are associated with Abstract (fine arts style); popes are associated with Roman Catholicism</dct:description>
  </owl:ObjectProperty>
  <owl:ObjectProperty rdf:about="http://vocab.getty.edu/ontology#ulan2795_representative_was">
    <dc:identifier>2795</dc:identifier>
    <rdfs:isDefinedBy rdf:resource="http://vocab.getty.edu/ontology"/>
    <rdfs:isDefinedBy rdf:resource="http://vocab.getty.edu/ulan/"/>
    <dc:title>representative was - person</dc:title>
    <rdfs:domain rdf:resource="http://www.w3.org/2004/02/skos/core#Concept"/>
    <skos:prefLabel>ulan2795_representative_was</skos:prefLabel>
    <rdfs:range rdf:resource="http://www.w3.org/2004/02/skos/core#Concept"/>
    <skos:example>The Noguch Museum - representative was Isamu Noguchi</skos:example>
    <rdfs:subPropertyOf rdf:resource="http://www.w3.org/2004/02/skos/core#related"/>
    <dct:description>institution - representative was - person.&#xD;
Example: The Noguch Museum - representative was Isamu Noguchi</dct:description>
  </owl:ObjectProperty>
  <owl:ObjectProperty rdf:about="http://vocab.getty.edu/ontology#biography">
    <rdfs:isDefinedBy rdf:resource="http://vocab.getty.edu/ontology"/>
    <rdfs:label>biography</rdfs:label>
    <rdfs:range rdf:resource="http://vocab.getty.edu/ontology#Biography"/>
    <rdfs:subPropertyOf rdf:resource="http://vocab.getty.edu/ontology#biography"/>
    <rdfs:comment>Biography of an ULAN agent. Domain is schema:Person/Organization, range is gvp:Biography. The preferred biography fields are also directly available in the Person/Organization</rdfs:comment>
    <dct:description>Biography of an ULAN agent. Domain is schema:Person/Organization, range is gvp:Biography. The preferred biography fields are also directly available in the Person/Organization</dct:description>
  </owl:ObjectProperty>
  <owl:ObjectProperty rdf:about="http://vocab.getty.edu/ontology#ulan1561_step-child_of">
    <rdfs:isDefinedBy rdf:resource="http://vocab.getty.edu/ulan/"/>
    <dc:identifier>1561</dc:identifier>
    <rdfs:isDefinedBy rdf:resource="http://vocab.getty.edu/ontology"/>
    <rdfs:subPropertyOf rdf:resource="http://www.w3.org/2004/02/skos/core#related"/>
    <rdfs:domain rdf:resource="http://www.w3.org/2004/02/skos/core#Concept"/>
    <dct:description>person - step-child of - person.&#xD;
Example: Hortense, Quene consort of Louis Bonaparte is the step-child of Napoleon I, Emperor of the French</dct:description>
    <rdfs:range rdf:resource="http://www.w3.org/2004/02/skos/core#Concept"/>
    <owl:inverseOf>
      <owl:ObjectProperty rdf:about="http://vocab.getty.edu/ontology#ulan1562_step-parent_of"/>
    </owl:inverseOf>
    <skos:prefLabel>ulan1561_step-child_of</skos:prefLabel>
    <skos:example>Hortense, Quene consort of Louis Bonaparte is the step-child of Napoleon I, Emperor of the French</skos:example>
    <dc:title>step-child of - person</dc:title>
  </owl:ObjectProperty>
  <owl:ObjectProperty rdf:about="http://vocab.getty.edu/ontology#ulan1514_gandparent_of">
    <dct:description>person - gandparent of - person.&#xD;
Example: Frank Lloyd Wright is the grandparent of Eric Lloyd Wright</dct:description>
    <skos:example>Frank Lloyd Wright is the grandparent of Eric Lloyd Wright</skos:example>
    <rdfs:range rdf:resource="http://www.w3.org/2004/02/skos/core#Concept"/>
    <skos:prefLabel>ulan1514_gandparent_of</skos:prefLabel>
    <rdfs:subPropertyOf rdf:resource="http://www.w3.org/2004/02/skos/core#related"/>
    <rdfs:isDefinedBy rdf:resource="http://vocab.getty.edu/ulan/"/>
    <rdfs:isDefinedBy rdf:resource="http://vocab.getty.edu/ontology"/>
    <dc:title>gandparent of - person</dc:title>
    <rdfs:domain rdf:resource="http://www.w3.org/2004/02/skos/core#Concept"/>
    <dc:identifier>1514</dc:identifier>
  </owl:ObjectProperty>
  <owl:ObjectProperty rdf:about="http://vocab.getty.edu/ontology#aat2418_uses">
    <skos:example>astronomy uses astronomical instruments</skos:example>
    <skos:example>divination [discipline] uses divination objects</skos:example>
    <dct:description>field [of study]/discipline - uses - things/[equipment].&#xD;
Example: astronomy uses astronomical instruments; divination [discipline] uses divination objects</dct:description>
    <skos:prefLabel>aat2418_uses</skos:prefLabel>
    <dc:title>uses - things</dc:title>
    <rdfs:domain rdf:resource="http://www.w3.org/2004/02/skos/core#Concept"/>
    <owl:inverseOf>
      <owl:ObjectProperty rdf:about="http://vocab.getty.edu/ontology#aat2419_used_for"/>
    </owl:inverseOf>
    <rdfs:subPropertyOf rdf:resource="http://www.w3.org/2004/02/skos/core#related"/>
    <rdfs:range rdf:resource="http://www.w3.org/2004/02/skos/core#Concept"/>
    <rdfs:isDefinedBy rdf:resource="http://vocab.getty.edu/aat/"/>
    <dc:identifier>2418</dc:identifier>
    <rdfs:isDefinedBy rdf:resource="http://vocab.getty.edu/ontology"/>
  </owl:ObjectProperty>
  <owl:ObjectProperty rdf:about="http://vocab.getty.edu/ontology#tgn3318_member_is">
    <rdfs:subPropertyOf rdf:resource="http://www.w3.org/2004/02/skos/core#related"/>
    <skos:prefLabel>tgn3318_member_is</skos:prefLabel>
    <skos:example>Austria is a member of the European Union since 1915</skos:example>
    <rdfs:domain rdf:resource="http://www.w3.org/2004/02/skos/core#Concept"/>
    <skos:example>Belgium is a member of the European Union since 1958</skos:example>
    <dc:title>member is - nation</dc:title>
    <rdfs:isDefinedBy rdf:resource="http://vocab.getty.edu/tgn/"/>
    <rdfs:range rdf:resource="http://www.w3.org/2004/02/skos/core#Concept"/>
    <rdfs:isDefinedBy rdf:resource="http://vocab.getty.edu/ontology"/>
    <dc:identifier>3318</dc:identifier>
    <dct:description>union - member is - nation.&#xD;
Example: Austria is a member of the European Union since 1915; Belgium is a member of the European Union since 1958</dct:description>
  </owl:ObjectProperty>
  <owl:ObjectProperty rdf:about="http://vocab.getty.edu/ontology#sourceNonPreferred">
    <rdfs:isDefinedBy rdf:resource="http://vocab.getty.edu/ontology"/>
    <rdfs:label>sourceNonPreferred</rdfs:label>
    <rdfs:domain rdf:resource="http://www.w3.org/2008/05/skos-xl#Label"/>
    <rdfs:range rdf:resource="http://purl.org/ontology/bibo/Document"/>
    <rdfs:subPropertyOf rdf:resource="http://purl.org/dc/terms/source"/>
    <rdfs:comment>Source for which the term is Non-preferred. Range is bibo:Document or bibo:DocumentPart</rdfs:comment>
    <skos:example>"Panderma" is non-preferred in Webster's New Geographical Dictionary (1988)</skos:example>
    <dct:description>Source for which the term is Non-preferred. Range is bibo:Document or bibo:DocumentPart.
Example: "Panderma" is non-preferred in Webster's New Geographical Dictionary (1988)</dct:description>
  </owl:ObjectProperty>
  <owl:ObjectProperty rdf:about="http://vocab.getty.edu/ontology#ulan1221_appointed_by">
    <skos:prefLabel>ulan1221_appointed_by</skos:prefLabel>
    <dc:title>appointed by - person</dc:title>
    <skos:example>Pope Urban VIII appointed Virginio Cesarini</skos:example>
    <dc:identifier>1221</dc:identifier>
    <rdfs:isDefinedBy rdf:resource="http://vocab.getty.edu/ulan/"/>
    <dct:description>person - appointed by - person.&#xD;
Example: Pope Urban VIII appointed Virginio Cesarini</dct:description>
    <rdfs:range rdf:resource="http://www.w3.org/2004/02/skos/core#Concept"/>
    <rdfs:isDefinedBy rdf:resource="http://vocab.getty.edu/ontology"/>
    <owl:inverseOf rdf:resource="http://vocab.getty.edu/ontology#ulan1222_appointee_of"/>
    <rdfs:domain rdf:resource="http://www.w3.org/2004/02/skos/core#Concept"/>
    <rdfs:subPropertyOf rdf:resource="http://www.w3.org/2004/02/skos/core#related"/>
  </owl:ObjectProperty>
  <owl:ObjectProperty rdf:about="http://vocab.getty.edu/ontology#ulan2582_administered_by">
    <rdfs:domain rdf:resource="http://www.w3.org/2004/02/skos/core#Concept"/>
    <skos:prefLabel>ulan2582_administered_by</skos:prefLabel>
    <rdfs:isDefinedBy rdf:resource="http://vocab.getty.edu/ulan/"/>
    <skos:example>Societe nationale des chemins de fer Francais. Agence des gares was administered by Georges Mathieu</skos:example>
    <dc:title>administered by - person</dc:title>
    <dc:identifier>2582</dc:identifier>
    <rdfs:range rdf:resource="http://www.w3.org/2004/02/skos/core#Concept"/>
    <rdfs:isDefinedBy rdf:resource="http://vocab.getty.edu/ontology"/>
    <dct:description>institution - administered by - person.&#xD;
Example: Societe nationale des chemins de fer Francais. Agence des gares was administered by Georges Mathieu</dct:description>
    <rdfs:subPropertyOf rdf:resource="http://www.w3.org/2004/02/skos/core#related"/>
  </owl:ObjectProperty>
  <owl:ObjectProperty rdf:about="http://vocab.getty.edu/ontology#tgn3412_predecessor_of">
    <rdfs:subPropertyOf rdf:resource="http://www.w3.org/2004/02/skos/core#related"/>
    <rdfs:isDefinedBy rdf:resource="http://vocab.getty.edu/tgn/"/>
    <dct:description>nation - predecessor of - nation.&#xD;
Example: Persia is the predecessor of Iran (nation)</dct:description>
    <skos:example>Persia is the predecessor of Iran (nation)</skos:example>
    <rdfs:domain rdf:resource="http://www.w3.org/2004/02/skos/core#Concept"/>
    <skos:prefLabel>tgn3412_predecessor_of</skos:prefLabel>
    <rdfs:isDefinedBy rdf:resource="http://vocab.getty.edu/ontology"/>
    <dc:title>predecessor of - nation</dc:title>
    <dc:identifier>3412</dc:identifier>
    <rdfs:range rdf:resource="http://www.w3.org/2004/02/skos/core#Concept"/>
  </owl:ObjectProperty>
  <owl:ObjectProperty rdf:about="http://vocab.getty.edu/ontology#ulan1313_partner_in">
    <rdfs:subPropertyOf rdf:resource="http://www.w3.org/2004/02/skos/core#related"/>
    <dc:title>partner in - firm</dc:title>
    <rdfs:range rdf:resource="http://www.w3.org/2004/02/skos/core#Concept"/>
    <skos:example>Parners of Adler and Sullivan included Louis H. Sullivan and Dankmar Adler</skos:example>
    <rdfs:isDefinedBy rdf:resource="http://vocab.getty.edu/ulan/"/>
    <skos:prefLabel>ulan1313_partner_in</skos:prefLabel>
    <dct:description>person - partner in - firm.&#xD;
Example: Parners of Adler and Sullivan included Louis H. Sullivan and Dankmar Adler</dct:description>
    <rdfs:isDefinedBy rdf:resource="http://vocab.getty.edu/ontology"/>
    <dc:identifier>1313</dc:identifier>
    <rdfs:domain rdf:resource="http://www.w3.org/2004/02/skos/core#Concept"/>
    <owl:inverseOf rdf:resource="http://vocab.getty.edu/ontology#ulan1314_partner_was"/>
  </owl:ObjectProperty>
  <owl:ObjectProperty rdf:about="http://vocab.getty.edu/ontology#ulan1211_artist_to">
    <rdfs:isDefinedBy rdf:resource="http://vocab.getty.edu/ontology"/>
    <rdfs:range rdf:resource="http://www.w3.org/2004/02/skos/core#Concept"/>
    <rdfs:subPropertyOf rdf:resource="http://www.w3.org/2004/02/skos/core#related"/>
    <dc:identifier>1211</dc:identifier>
    <dct:description>person - artist to - person.&#xD;
Example: Artist to Louis XIV, King of France was Charles-Pierre Coustou</dct:description>
    <skos:prefLabel>ulan1211_artist_to</skos:prefLabel>
    <skos:example>Artist to Louis XIV, King of France was Charles-Pierre Coustou</skos:example>
    <dc:title>artist to - person</dc:title>
    <rdfs:isDefinedBy rdf:resource="http://vocab.getty.edu/ulan/"/>
    <owl:inverseOf rdf:resource="http://vocab.getty.edu/ontology#ulan1212_artist_was"/>
    <rdfs:domain rdf:resource="http://www.w3.org/2004/02/skos/core#Concept"/>
  </owl:ObjectProperty>
  <owl:ObjectProperty rdf:about="http://vocab.getty.edu/ontology#broaderPartitiveExtended">
    <rdfs:label>broaderPartitiveExtended</rdfs:label>
    <rdfs:isDefinedBy rdf:resource="http://vocab.getty.edu/ontology"/>
    <rdfs:domain rdf:resource="http://vocab.getty.edu/ontology#Subject"/>
    <rdfs:comment>Ancestors (Partitive). Meaningful closure of gvp:broaderPartitive. Infers iso:broaderPartitive for pairs of directly related skos:Concepts</rdfs:comment>
    <owl:propertyChainAxiom rdf:parseType="Collection">
      <owl:ObjectProperty rdf:about="http://vocab.getty.edu/ontology#broaderPartitiveExtended"/>
      <owl:ObjectProperty rdf:about="http://vocab.getty.edu/ontology#broaderPartitive"/>
    </owl:propertyChainAxiom>
    <dct:description>Ancestors (Partitive). Meaningful closure of gvp:broaderPartitive. Infers iso:broaderPartitive for pairs of directly related skos:Concepts.
Example: anvil components BTP &lt;anvils and anvil accessories&gt; BTG &lt;forging and metal-shaping tools&gt;,
so anvil components BTPE &lt;forging and metal-shaping tools&gt;</dct:description>
    <skos:example>anvil components BTP &lt;anvils and anvil accessories&gt; BTG &lt;forging and metal-shaping tools&gt;,
so anvil components BTPE &lt;forging and metal-shaping tools&gt;</skos:example>
    <rdfs:range rdf:resource="http://vocab.getty.edu/ontology#Subject"/>
    <owl:propertyChainAxiom rdf:parseType="Collection">
      <owl:ObjectProperty rdf:about="http://vocab.getty.edu/ontology#broaderPartitiveExtended"/>
      <owl:ObjectProperty rdf:about="http://vocab.getty.edu/ontology#broaderGeneric"/>
    </owl:propertyChainAxiom>
    <rdfs:subPropertyOf rdf:resource="http://vocab.getty.edu/ontology#broaderExtended"/>
    <owl:propertyChainAxiom rdf:parseType="Collection">
      <owl:ObjectProperty rdf:about="http://vocab.getty.edu/ontology#broaderGeneric"/>
      <owl:ObjectProperty rdf:about="http://vocab.getty.edu/ontology#broaderPartitiveExtended"/>
    </owl:propertyChainAxiom>
  </owl:ObjectProperty>
  <owl:ObjectProperty rdf:about="http://vocab.getty.edu/ontology#aat2811_preceded">
    <skos:example>Acheulian preceded Micoquian</skos:example>
    <rdfs:subPropertyOf rdf:resource="http://www.w3.org/2004/02/skos/core#related"/>
    <rdfs:range rdf:resource="http://www.w3.org/2004/02/skos/core#Concept"/>
    <dc:identifier>2811</dc:identifier>
    <rdfs:isDefinedBy rdf:resource="http://vocab.getty.edu/aat/"/>
    <skos:example>Impressionist preceded Abstract Impressionist</skos:example>
    <rdfs:domain rdf:resource="http://www.w3.org/2004/02/skos/core#Concept"/>
    <rdfs:isDefinedBy rdf:resource="http://vocab.getty.edu/ontology"/>
    <dc:title>preceded - style/period/culture</dc:title>
    <owl:inverseOf>
      <owl:ObjectProperty rdf:about="http://vocab.getty.edu/ontology#aat2812_followed"/>
    </owl:inverseOf>
    <skos:prefLabel>aat2811_preceded</skos:prefLabel>
    <dct:description>style/period/culture/[religion/ideology] - preceded  - style/period/culture/[religion/ideology].&#xD;
Example: Impressionist preceded Abstract Impressionist; Acheulian preceded Micoquian</dct:description>
  </owl:ObjectProperty>
  <owl:ObjectProperty rdf:about="http://vocab.getty.edu/ontology#tgn3401_moved_from">
    <owl:inverseOf>
      <owl:ObjectProperty rdf:about="http://vocab.getty.edu/ontology#tgn3402_moved_to"/>
    </owl:inverseOf>
    <rdfs:range rdf:resource="http://www.w3.org/2004/02/skos/core#Concept"/>
    <dc:title>moved from - place</dc:title>
    <dct:description>place - moved from - place; Note: places that were physically moved from one location to another, often due to the threat or occurrence of natural disaster..&#xD;
Example: Troupville, Georgia, USA was moved to Valdosta (Lowndes county, Georgia, USA)</dct:description>
    <rdfs:isDefinedBy rdf:resource="http://vocab.getty.edu/tgn/"/>
    <dc:identifier>3401</dc:identifier>
    <skos:prefLabel>tgn3401_moved_from</skos:prefLabel>
    <rdfs:domain rdf:resource="http://www.w3.org/2004/02/skos/core#Concept"/>
    <skos:example>Troupville, Georgia, USA was moved to Valdosta (Lowndes county, Georgia, USA)</skos:example>
    <rdfs:subPropertyOf rdf:resource="http://www.w3.org/2004/02/skos/core#related"/>
    <skos:scopeNote>Note: places that were physically moved from one location to another, often due to the threat or occurrence of natural disaster.</skos:scopeNote>
    <rdfs:isDefinedBy rdf:resource="http://vocab.getty.edu/ontology"/>
  </owl:ObjectProperty>
  <owl:ObjectProperty rdf:about="http://vocab.getty.edu/ontology#ulan1214_court_artist_was">
    <rdfs:subPropertyOf rdf:resource="http://www.w3.org/2004/02/skos/core#related"/>
    <rdfs:isDefinedBy rdf:resource="http://vocab.getty.edu/ulan/"/>
    <rdfs:isDefinedBy rdf:resource="http://vocab.getty.edu/ontology"/>
    <dct:description>person - court artist was - person.&#xD;
Example: Peter Paul Rubens was court artist to Gonzaga Vincenzo I, Duke of Mantua; Francisco de Goya was court artist to Charles IV, King of Spain</dct:description>
    <rdfs:range rdf:resource="http://www.w3.org/2004/02/skos/core#Concept"/>
    <skos:prefLabel>ulan1214_court_artist_was</skos:prefLabel>
    <skos:example>Francisco de Goya was court artist to Charles IV, King of Spain</skos:example>
    <dc:identifier>1214</dc:identifier>
    <rdfs:domain rdf:resource="http://www.w3.org/2004/02/skos/core#Concept"/>
    <dc:title>court artist was - person</dc:title>
    <skos:example>Peter Paul Rubens was court artist to Gonzaga Vincenzo I, Duke of Mantua</skos:example>
  </owl:ObjectProperty>
  <owl:ObjectProperty rdf:about="http://vocab.getty.edu/ontology#tgn3402_moved_to">
    <rdfs:range rdf:resource="http://www.w3.org/2004/02/skos/core#Concept"/>
    <rdfs:domain rdf:resource="http://www.w3.org/2004/02/skos/core#Concept"/>
    <dct:description>place - moved to - place.&#xD;
Example: Valdosta (Lowndes county, Georgia, USA) moved from Troupville (Georgia, USA)</dct:description>
    <rdfs:subPropertyOf rdf:resource="http://www.w3.org/2004/02/skos/core#related"/>
    <skos:example>Valdosta (Lowndes county, Georgia, USA) moved from Troupville (Georgia, USA)</skos:example>
    <rdfs:isDefinedBy rdf:resource="http://vocab.getty.edu/ontology"/>
    <dc:title>moved to - place</dc:title>
    <rdfs:isDefinedBy rdf:resource="http://vocab.getty.edu/tgn/"/>
    <dc:identifier>3402</dc:identifier>
    <skos:prefLabel>tgn3402_moved_to</skos:prefLabel>
  </owl:ObjectProperty>
  <owl:ObjectProperty rdf:about="http://vocab.getty.edu/ontology#aat2216_require">
    <rdfs:isDefinedBy rdf:resource="http://vocab.getty.edu/aat/"/>
    <dc:title>require - things</dc:title>
    <skos:example>compact disc players require compact discs</skos:example>
    <skos:example>broderie anglaise requires eyelets</skos:example>
    <rdfs:subPropertyOf rdf:resource="http://www.w3.org/2004/02/skos/core#related"/>
    <rdfs:isDefinedBy rdf:resource="http://vocab.getty.edu/ontology"/>
    <rdfs:domain rdf:resource="http://www.w3.org/2004/02/skos/core#Concept"/>
    <skos:prefLabel>aat2216_require</skos:prefLabel>
    <dc:identifier>2216</dc:identifier>
    <rdfs:range rdf:resource="http://www.w3.org/2004/02/skos/core#Concept"/>
    <dct:description>things - require - things [in order to exist or work].&#xD;
Example: broderie anglaise requires eyelets; compact disc players require compact discs</dct:description>
  </owl:ObjectProperty>
  <owl:ObjectProperty rdf:about="http://vocab.getty.edu/ontology#ulan1422_founded">
    <rdfs:subPropertyOf rdf:resource="http://www.w3.org/2004/02/skos/core#related"/>
    <rdfs:isDefinedBy rdf:resource="http://vocab.getty.edu/ontology"/>
    <dc:title>founded - firm/group</dc:title>
    <rdfs:domain rdf:resource="http://www.w3.org/2004/02/skos/core#Concept"/>
    <skos:example>The United States Congress founded the National Gallery of Art</skos:example>
    <skos:prefLabel>ulan1422_founded</skos:prefLabel>
    <dct:description>firm/group - founded - firm/group.&#xD;
Example: The United States Congress founded the National Gallery of Art</dct:description>
    <rdfs:range rdf:resource="http://www.w3.org/2004/02/skos/core#Concept"/>
    <rdfs:isDefinedBy rdf:resource="http://vocab.getty.edu/ulan/"/>
    <dc:identifier>1422</dc:identifier>
  </owl:ObjectProperty>
  <owl:ObjectProperty rdf:about="http://vocab.getty.edu/ontology#broaderNonConcept">
    <rdfs:isDefinedBy rdf:resource="http://vocab.getty.edu/ontology"/>
    <rdfs:label>broaderNonConcept</rdfs:label>
    <rdfs:domain rdf:resource="http://www.w3.org/2004/02/skos/core#Concept"/>
    <rdfs:range rdf:resource="http://vocab.getty.edu/ontology#GuideTerm"/>
    <rdfs:comment>Chain of gvp:broader from Concept to GuideTerms, without intervening Concept</rdfs:comment>
    <dct:description>Chain of gvp:broader from Concept to GuideTerms, without intervening Concept</dct:description>
  </owl:ObjectProperty>
  <owl:ObjectProperty rdf:about="http://vocab.getty.edu/ontology#ulan1551_sibling_by_marriage_of">
    <rdfs:domain rdf:resource="http://www.w3.org/2004/02/skos/core#Concept"/>
    <dc:title>sibling by marriage of - person</dc:title>
    <skos:example>Peter Paul Rubens and Susanne Fourment are siblings by marriage</skos:example>
    <rdfs:subPropertyOf rdf:resource="http://www.w3.org/2004/02/skos/core#related"/>
    <rdfs:range rdf:resource="http://www.w3.org/2004/02/skos/core#Concept"/>
    <dc:identifier>1551</dc:identifier>
    <dct:description>person - sibling by marriage (step sibling) - person.&#xD;
Example: Peter Paul Rubens and Susanne Fourment are siblings by marriage</dct:description>
    <rdf:type rdf:resource="http://www.w3.org/2002/07/owl#SymmetricProperty"/>
    <rdfs:isDefinedBy rdf:resource="http://vocab.getty.edu/ulan/"/>
    <skos:prefLabel>ulan1551_sibling_by_marriage_of</skos:prefLabel>
    <rdfs:isDefinedBy rdf:resource="http://vocab.getty.edu/ontology"/>
  </owl:ObjectProperty>
  <owl:ObjectProperty rdf:about="http://vocab.getty.edu/ontology#aat2563_located_in">
    <rdfs:range rdf:resource="http://www.w3.org/2004/02/skos/core#Concept"/>
    <rdfs:subPropertyOf rdf:resource="http://www.w3.org/2004/02/skos/core#related"/>
    <skos:example>First Nations (culture) is located/reflected in First Nations reserves</skos:example>
    <dct:description>style/period/culture/[religion/ideology] - is located/[reflected] in - locus/setting.&#xD;
Example: First Nations (culture) is located/reflected in First Nations reserves; Brahmanism is located/reflected in agraharas</dct:description>
    <skos:prefLabel>aat2563_located_in</skos:prefLabel>
    <rdfs:isDefinedBy rdf:resource="http://vocab.getty.edu/aat/"/>
    <rdfs:isDefinedBy rdf:resource="http://vocab.getty.edu/ontology"/>
    <rdfs:domain rdf:resource="http://www.w3.org/2004/02/skos/core#Concept"/>
    <dc:identifier>2563</dc:identifier>
    <dc:title>located in - locus/setting</dc:title>
    <skos:example>Brahmanism is located/reflected in agraharas</skos:example>
  </owl:ObjectProperty>
  <owl:ObjectProperty rdf:about="http://vocab.getty.edu/ontology#aat2411_involved_in">
    <rdfs:range rdf:resource="http://www.w3.org/2004/02/skos/core#Concept"/>
    <rdfs:subPropertyOf rdf:resource="http://www.w3.org/2004/02/skos/core#related"/>
    <skos:example>gardening is involved in horticulture</skos:example>
    <skos:prefLabel>aat2411_involved_in</skos:prefLabel>
    <dct:description>activity/event/[process/function] - [is] involved in - field/discipline.&#xD;
Example: journalistic photography is involved in photojournalism (discipline); gardening is involved in horticulture</dct:description>
    <rdfs:domain rdf:resource="http://www.w3.org/2004/02/skos/core#Concept"/>
    <rdfs:isDefinedBy rdf:resource="http://vocab.getty.edu/aat/"/>
    <rdfs:isDefinedBy rdf:resource="http://vocab.getty.edu/ontology"/>
    <dc:identifier>2411</dc:identifier>
    <skos:example>journalistic photography is involved in photojournalism (discipline)</skos:example>
    <dc:title>involved in - field/discipline</dc:title>
    <owl:inverseOf rdf:resource="http://vocab.getty.edu/ontology#aat2412_involves"/>
  </owl:ObjectProperty>
  <owl:ObjectProperty rdf:about="http://vocab.getty.edu/ontology#aat2408_locus-setting_for">
    <rdfs:domain rdf:resource="http://www.w3.org/2004/02/skos/core#Concept"/>
    <dc:identifier>2408</dc:identifier>
    <rdfs:subPropertyOf rdf:resource="http://www.w3.org/2004/02/skos/core#related"/>
    <skos:example>hospitals (buildings) are the locus/setting for medicine (discipline)</skos:example>
    <rdfs:isDefinedBy rdf:resource="http://vocab.getty.edu/aat/"/>
    <rdfs:range rdf:resource="http://www.w3.org/2004/02/skos/core#Concept"/>
    <rdfs:isDefinedBy rdf:resource="http://vocab.getty.edu/ontology"/>
    <dc:title>locus/setting for - field/discipline</dc:title>
    <skos:prefLabel>aat2408_locus-setting_for</skos:prefLabel>
    <dct:description>locus/setting - [is] locus/setting for - field of study/discipline.&#xD;
Example: schools (buildings) are the locus/setting for education; hospitals (buildings) are the locus/setting for medicine (discipline)</dct:description>
    <skos:example>schools (buildings) are the locus/setting for education</skos:example>
    <owl:inverseOf rdf:resource="http://vocab.getty.edu/ontology#aat2409_takes_place_in"/>
  </owl:ObjectProperty>
  <owl:ObjectProperty rdf:about="http://vocab.getty.edu/ontology#tgn3317_member_of">
    <dc:identifier>3317</dc:identifier>
    <dct:description>nation - member of - union.&#xD;
Example: Austria is a member of the European Union since 1915; Belgium is a member of the European Union since 1958</dct:description>
    <dc:title>member of - union</dc:title>
    <skos:example>Belgium is a member of the European Union since 1958</skos:example>
    <skos:example>Austria is a member of the European Union since 1915</skos:example>
    <skos:prefLabel>tgn3317_member_of</skos:prefLabel>
    <rdfs:domain rdf:resource="http://www.w3.org/2004/02/skos/core#Concept"/>
    <rdfs:isDefinedBy rdf:resource="http://vocab.getty.edu/ontology"/>
    <owl:inverseOf rdf:resource="http://vocab.getty.edu/ontology#tgn3318_member_is"/>
    <rdfs:subPropertyOf rdf:resource="http://www.w3.org/2004/02/skos/core#related"/>
    <rdfs:isDefinedBy rdf:resource="http://vocab.getty.edu/tgn/"/>
    <rdfs:range rdf:resource="http://www.w3.org/2004/02/skos/core#Concept"/>
  </owl:ObjectProperty>
  <owl:ObjectProperty rdf:about="http://vocab.getty.edu/ontology#aat2845_used-located_in">
    <skos:prefLabel>aat2845_used-located_in</skos:prefLabel>
    <dc:identifier>2845</dc:identifier>
    <owl:inverseOf>
      <owl:ObjectProperty rdf:about="http://vocab.getty.edu/ontology#aat2846_locus-setting_for"/>
    </owl:inverseOf>
    <rdfs:range rdf:resource="http://www.w3.org/2004/02/skos/core#Concept"/>
    <rdfs:isDefinedBy rdf:resource="http://vocab.getty.edu/aat/"/>
    <dct:description>genus/species - [is] used/located in -  locus/setting.&#xD;
Example: Elephantidae(family) are used/located in elephant houses; Vitaceae (family) is used/located in vineyards</dct:description>
    <skos:example>Elephantidae(family) are used/located in elephant houses</skos:example>
    <rdfs:domain rdf:resource="http://www.w3.org/2004/02/skos/core#Concept"/>
    <dc:title>used/located in - locus/setting</dc:title>
    <rdfs:subPropertyOf rdf:resource="http://www.w3.org/2004/02/skos/core#related"/>
    <skos:example>Vitaceae (family) is used/located in vineyards</skos:example>
    <rdfs:isDefinedBy rdf:resource="http://vocab.getty.edu/ontology"/>
  </owl:ObjectProperty>
  <owl:ObjectProperty rdf:about="http://vocab.getty.edu/ontology#tgn3201_capital_of">
    <rdfs:subPropertyOf rdf:resource="http://www.w3.org/2004/02/skos/core#related"/>
    <rdfs:isDefinedBy rdf:resource="http://vocab.getty.edu/ontology"/>
    <skos:example>Thecapital of Maxima Caesariensis from 296 to 800 CE was London</skos:example>
    <rdfs:isDefinedBy rdf:resource="http://vocab.getty.edu/tgn/"/>
    <dc:title>capital of - nation</dc:title>
    <owl:inverseOf rdf:resource="http://vocab.getty.edu/ontology#tgn3202_capital_is"/>
    <skos:prefLabel>tgn3201_capital_of</skos:prefLabel>
    <dct:description>city - capital of - nation.&#xD;
Example: Thecapital of Maxima Caesariensis from 296 to 800 CE was London</dct:description>
    <rdfs:range rdf:resource="http://www.w3.org/2004/02/skos/core#Concept"/>
    <dc:identifier>3201</dc:identifier>
    <rdfs:domain rdf:resource="http://www.w3.org/2004/02/skos/core#Concept"/>
  </owl:ObjectProperty>
  <owl:ObjectProperty rdf:about="http://vocab.getty.edu/ontology#aat2601_possessed_by-existing_in">
    <owl:inverseOf rdf:resource="http://vocab.getty.edu/ontology#aat2602_possess-exist_in"/>
    <rdfs:subPropertyOf rdf:resource="http://www.w3.org/2004/02/skos/core#related"/>
    <skos:example>adulthood is possessed by/existing in adults</skos:example>
    <dc:identifier>2601</dc:identifier>
    <rdfs:isDefinedBy rdf:resource="http://vocab.getty.edu/ontology"/>
    <skos:example>nomadism is possessed by/existing in nomads</skos:example>
    <rdfs:isDefinedBy rdf:resource="http://vocab.getty.edu/aat/"/>
    <dct:description>attributes /associated concepts - [is] possessed by/existing in - role [of actors].&#xD;
Example: adulthood is possessed by/existing in adults; nomadism is possessed by/existing in nomads</dct:description>
    <dc:title>possessed by/existing in - role</dc:title>
    <skos:prefLabel>aat2601_possessed_by-existing_in</skos:prefLabel>
    <rdfs:range rdf:resource="http://www.w3.org/2004/02/skos/core#Concept"/>
    <rdfs:domain rdf:resource="http://www.w3.org/2004/02/skos/core#Concept"/>
  </owl:ObjectProperty>
  <owl:ObjectProperty rdf:about="http://vocab.getty.edu/ontology#broaderPreferred">
    <rdfs:isDefinedBy rdf:resource="http://vocab.getty.edu/ontology"/>
    <rdfs:comment>Main parent of a subject. Needed to display the hierarchy</rdfs:comment>
    <rdfs:subPropertyOf>
      <owl:ObjectProperty rdf:about="http://vocab.getty.edu/ontology#broaderPreferredExtended"/>
    </rdfs:subPropertyOf>
    <skos:example>Preferred: "baking dishes" (AAT) BTG "bakeware" (AAT); Sofia (TGN) BTP Bulgaria (TGN)</skos:example>
    <rdfs:domain rdf:resource="http://vocab.getty.edu/ontology#Subject"/>
    <rdfs:range rdf:resource="http://vocab.getty.edu/ontology#Subject"/>
    <rdfs:label>broaderPreferred</rdfs:label>
    <dct:description>Main parent of a subject. Needed to display the hierarchy.
Example: Preferred: "baking dishes" (AAT) BTG "bakeware" (AAT); Sofia (TGN) BTP Bulgaria (TGN)</dct:description>
    <rdfs:subPropertyOf rdf:resource="http://vocab.getty.edu/ontology#broader"/>
  </owl:ObjectProperty>
  <owl:ObjectProperty rdf:about="http://vocab.getty.edu/ontology#aat2852_involved_with">
    <dc:title>involved with - things</dc:title>
    <rdfs:isDefinedBy rdf:resource="http://vocab.getty.edu/ontology"/>
    <skos:prefLabel>aat2852_involved_with</skos:prefLabel>
    <dc:identifier>2852</dc:identifier>
    <owl:inverseOf>
      <owl:ObjectProperty rdf:about="http://vocab.getty.edu/ontology#aat2853_involve"/>
    </owl:inverseOf>
    <skos:example>Rosa (genus) is involved with rose bowls</skos:example>
    <skos:example>Camelus (genus) is involved with camel saddles</skos:example>
    <rdfs:isDefinedBy rdf:resource="http://vocab.getty.edu/aat/"/>
    <dct:description>genus/species - [is] involved with - things/[equipment].&#xD;
Example: Rosa (genus) is involved with rose bowls; Camelus (genus) is involved with camel saddles</dct:description>
    <rdfs:subPropertyOf rdf:resource="http://www.w3.org/2004/02/skos/core#related"/>
    <rdfs:domain rdf:resource="http://www.w3.org/2004/02/skos/core#Concept"/>
    <rdfs:range rdf:resource="http://www.w3.org/2004/02/skos/core#Concept"/>
  </owl:ObjectProperty>
  <owl:ObjectProperty rdf:about="http://vocab.getty.edu/ontology#ulan2581_administrator_of">
    <rdfs:domain rdf:resource="http://www.w3.org/2004/02/skos/core#Concept"/>
    <rdfs:isDefinedBy rdf:resource="http://vocab.getty.edu/ontology"/>
    <rdfs:subPropertyOf rdf:resource="http://www.w3.org/2004/02/skos/core#related"/>
    <rdfs:range rdf:resource="http://www.w3.org/2004/02/skos/core#Concept"/>
    <skos:example>Georges Mathieu was the administrator of Societe nationale des chemins de fer Francais. Agence des gares</skos:example>
    <skos:prefLabel>ulan2581_administrator_of</skos:prefLabel>
    <dct:description>person - administrator of - institution.&#xD;
Example: Georges Mathieu was the administrator of Societe nationale des chemins de fer Francais. Agence des gares</dct:description>
    <dc:identifier>2581</dc:identifier>
    <rdfs:isDefinedBy rdf:resource="http://vocab.getty.edu/ulan/"/>
    <dc:title>administrator of - institution</dc:title>
    <owl:inverseOf rdf:resource="http://vocab.getty.edu/ontology#ulan2582_administered_by"/>
  </owl:ObjectProperty>
  <owl:ObjectProperty rdf:about="http://vocab.getty.edu/ontology#aat2322_use">
    <skos:prefLabel>aat2322_use</skos:prefLabel>
    <rdfs:range rdf:resource="http://www.w3.org/2004/02/skos/core#Concept"/>
    <rdfs:isDefinedBy rdf:resource="http://vocab.getty.edu/aat/"/>
    <dc:identifier>2322</dc:identifier>
    <rdfs:domain rdf:resource="http://www.w3.org/2004/02/skos/core#Concept"/>
    <dc:title>use - things</dc:title>
    <rdfs:subPropertyOf rdf:resource="http://www.w3.org/2004/02/skos/core#related"/>
    <dct:description>[actors having] role - use - things/equipment.&#xD;
Example: violoncellists use violoncellos; surveyors use surveying instruments</dct:description>
    <skos:example>violoncellists use violoncellos</skos:example>
    <rdfs:isDefinedBy rdf:resource="http://vocab.getty.edu/ontology"/>
    <skos:example>surveyors use surveying instruments</skos:example>
  </owl:ObjectProperty>
  <owl:ObjectProperty rdf:about="http://vocab.getty.edu/ontology#broaderInstantial">
    <skos:example>Rembrandt van Rijn BTI Persons/Artists (ULAN)</skos:example>
    <dct:description>BTI (Kind/Instance, "example of") relation. We also infer iso-thes:broaderInstantial, which goes only between Concepts.
Example: Rembrandt van Rijn BTI Persons/Artists (ULAN)</dct:description>
    <rdfs:range rdf:resource="http://vocab.getty.edu/ontology#Subject"/>
    <rdfs:isDefinedBy rdf:resource="http://vocab.getty.edu/ontology"/>
    <rdfs:comment>BTI (Kind/Instance, "example of") relation. We also infer iso-thes:broaderInstantial, which goes only between Concepts</rdfs:comment>
    <rdfs:subPropertyOf>
      <owl:ObjectProperty rdf:about="http://vocab.getty.edu/ontology#broaderInstantialExtended"/>
    </rdfs:subPropertyOf>
    <rdfs:subPropertyOf rdf:resource="http://vocab.getty.edu/ontology#broader"/>
    <rdfs:label>broaderInstantial</rdfs:label>
    <rdfs:domain rdf:resource="http://vocab.getty.edu/ontology#Subject"/>
  </owl:ObjectProperty>
  <owl:ObjectProperty rdf:about="http://vocab.getty.edu/ontology#ulan2572_founder_of">
    <dc:title>founder of - institution</dc:title>
    <rdfs:subPropertyOf rdf:resource="http://www.w3.org/2004/02/skos/core#related"/>
    <rdfs:domain rdf:resource="http://www.w3.org/2004/02/skos/core#Concept"/>
    <dct:description>person - founder of - institution.&#xD;
Example: Louis Comfort Tiffany was the founder of Tiffany Glass &amp; Decorating Company</dct:description>
    <rdfs:isDefinedBy rdf:resource="http://vocab.getty.edu/ulan/"/>
    <owl:inverseOf>
      <owl:ObjectProperty rdf:about="http://vocab.getty.edu/ontology#ulan2573_founded_by"/>
    </owl:inverseOf>
    <rdfs:isDefinedBy rdf:resource="http://vocab.getty.edu/ontology"/>
    <skos:example>Louis Comfort Tiffany was the founder of Tiffany Glass &amp; Decorating Company</skos:example>
    <rdfs:range rdf:resource="http://www.w3.org/2004/02/skos/core#Concept"/>
    <dc:identifier>2572</dc:identifier>
    <skos:prefLabel>ulan2572_founder_of</skos:prefLabel>
  </owl:ObjectProperty>
  <owl:ObjectProperty rdf:about="http://vocab.getty.edu/ontology#ulan1412_predecessor_of">
    <skos:prefLabel>ulan1412_predecessor_of</skos:prefLabel>
    <rdfs:isDefinedBy rdf:resource="http://vocab.getty.edu/ulan/"/>
    <dc:title>predecessor of - firm/group</dc:title>
    <rdfs:isDefinedBy rdf:resource="http://vocab.getty.edu/ontology"/>
    <rdfs:range rdf:resource="http://www.w3.org/2004/02/skos/core#Concept"/>
    <dct:description>firm/group - predecessor of - firm/group.&#xD;
Example: Richard Meier &amp; Associates is the predecessor of Richard Meier &amp; Partners Architects LLP</dct:description>
    <rdfs:subPropertyOf rdf:resource="http://www.w3.org/2004/02/skos/core#related"/>
    <skos:example>Richard Meier &amp; Associates is the predecessor of Richard Meier &amp; Partners Architects LLP</skos:example>
    <rdfs:domain rdf:resource="http://www.w3.org/2004/02/skos/core#Concept"/>
    <dc:identifier>1412</dc:identifier>
  </owl:ObjectProperty>
  <owl:ObjectProperty rdf:about="http://vocab.getty.edu/ontology#ulan1511_child_of">
    <rdfs:isDefinedBy rdf:resource="http://vocab.getty.edu/ulan/"/>
    <dc:title>child of - person</dc:title>
    <rdfs:isDefinedBy rdf:resource="http://vocab.getty.edu/ontology"/>
    <dct:description>person - child of - person.&#xD;
Example: Rembrandt van Rijn is the child of Neeltgen Willemsdr van Zuydtbroeck</dct:description>
    <rdfs:subPropertyOf rdf:resource="http://www.w3.org/2004/02/skos/core#related"/>
    <skos:example>Rembrandt van Rijn is the child of Neeltgen Willemsdr van Zuydtbroeck</skos:example>
    <dc:identifier>1511</dc:identifier>
    <skos:prefLabel>ulan1511_child_of</skos:prefLabel>
    <rdfs:domain rdf:resource="http://www.w3.org/2004/02/skos/core#Concept"/>
    <owl:inverseOf>
      <owl:ObjectProperty rdf:about="http://vocab.getty.edu/ontology#ulan1512_parent_of"/>
    </owl:inverseOf>
    <rdfs:range rdf:resource="http://www.w3.org/2004/02/skos/core#Concept"/>
  </owl:ObjectProperty>
  <owl:ObjectProperty rdf:about="http://vocab.getty.edu/ontology#contributorPreferred">
    <rdfs:isDefinedBy rdf:resource="http://vocab.getty.edu/ontology"/>
    <rdfs:label>contributorPreferred</rdfs:label>
    <rdfs:domain rdf:resource="http://www.w3.org/2008/05/skos-xl#Label"/>
    <rdfs:range rdf:resource="http://xmlns.com/foaf/0.1/Agent"/>
    <rdfs:subPropertyOf rdf:resource="http://purl.org/dc/terms/contributor"/>
    <rdfs:comment>Contributor for which the term is Preferred. Range is foaf:Agent</rdfs:comment>
    <skos:example>"organza" is preferred term for WHS</skos:example>
    <dct:description>Contributor for which the term is Preferred. Range is foaf:Agent.
Example: "organza" is preferred term for WHS</dct:description>
  </owl:ObjectProperty>
  <owl:ObjectProperty rdf:about="http://vocab.getty.edu/ontology#sourceAlternatePreferred">
    <rdfs:isDefinedBy rdf:resource="http://vocab.getty.edu/ontology"/>
    <rdfs:label>sourceAlternatePreferred</rdfs:label>
    <rdfs:domain rdf:resource="http://www.w3.org/2008/05/skos-xl#Label"/>
    <rdfs:range rdf:resource="http://purl.org/ontology/bibo/Document"/>
    <rdfs:subPropertyOf rdf:resource="http://purl.org/dc/terms/source"/>
    <rdfs:comment>Source for which the term is Alternate Preferred. Range is bibo:Document or bibo:DocumentPart</rdfs:comment>
    <skos:example>"Kayseri" is alternate preferred in Webster's New Geographical Dictionary (1988)</skos:example>
    <dct:description>Source for which the term is Alternate Preferred. Range is bibo:Document or bibo:DocumentPart.
Example: "Kayseri" is alternate preferred in Webster's New Geographical Dictionary (1988)</dct:description>
  </owl:ObjectProperty>
  <owl:ObjectProperty rdf:about="http://vocab.getty.edu/ontology#ulan1532_uncle-aunt_of">
    <rdfs:subPropertyOf rdf:resource="http://www.w3.org/2004/02/skos/core#related"/>
    <rdfs:domain rdf:resource="http://www.w3.org/2004/02/skos/core#Concept"/>
    <rdfs:isDefinedBy rdf:resource="http://vocab.getty.edu/ulan/"/>
    <dc:identifier>1532</dc:identifier>
    <rdfs:range rdf:resource="http://www.w3.org/2004/02/skos/core#Concept"/>
    <dc:title>uncle/aunt of - person</dc:title>
    <skos:example>Edouard Manet is the uncle/aunt of Julie Manet</skos:example>
    <dct:description>person - uncle/aunt of - person.&#xD;
Example: Edouard Manet is the uncle/aunt of Julie Manet</dct:description>
    <skos:prefLabel>ulan1532_uncle-aunt_of</skos:prefLabel>
    <rdfs:isDefinedBy rdf:resource="http://vocab.getty.edu/ontology"/>
  </owl:ObjectProperty>
  <owl:ObjectProperty rdf:about="http://vocab.getty.edu/ontology#aat2221_act_upon">
    <owl:inverseOf>
      <owl:ObjectProperty rdf:about="http://vocab.getty.edu/ontology#aat2222_are_acted_upon"/>
    </owl:inverseOf>
    <skos:prefLabel>aat2221_act_upon</skos:prefLabel>
    <rdfs:domain rdf:resource="http://www.w3.org/2004/02/skos/core#Concept"/>
    <dct:description>[actors having] role - act upon - genus/species.&#xD;
Example: jockeys act upon Equus caballus(species); tappers act upon Acer saccharum(species)</dct:description>
    <dc:title>act upon - genus/species</dc:title>
    <skos:example>tappers act upon Acer saccharum(species)</skos:example>
    <dc:identifier>2221</dc:identifier>
    <skos:example>jockeys act upon Equus caballus(species)</skos:example>
    <rdfs:subPropertyOf rdf:resource="http://www.w3.org/2004/02/skos/core#related"/>
    <rdfs:isDefinedBy rdf:resource="http://vocab.getty.edu/aat/"/>
    <rdfs:range rdf:resource="http://www.w3.org/2004/02/skos/core#Concept"/>
    <rdfs:isDefinedBy rdf:resource="http://vocab.getty.edu/ontology"/>
  </owl:ObjectProperty>
  <owl:ObjectProperty rdf:about="http://vocab.getty.edu/ontology#aat2326_create">
    <skos:example>draftsmen create drawings</skos:example>
    <dc:title>create - things</dc:title>
    <rdfs:range rdf:resource="http://www.w3.org/2004/02/skos/core#Concept"/>
    <dc:identifier>2326</dc:identifier>
    <rdfs:isDefinedBy rdf:resource="http://vocab.getty.edu/ontology"/>
    <rdfs:isDefinedBy rdf:resource="http://vocab.getty.edu/aat/"/>
    <rdfs:domain rdf:resource="http://www.w3.org/2004/02/skos/core#Concept"/>
    <rdfs:subPropertyOf rdf:resource="http://www.w3.org/2004/02/skos/core#related"/>
    <dct:description>[actors having] role - create - things.&#xD;
Example: draftsmen create drawings; poets create poems</dct:description>
    <skos:prefLabel>aat2326_create</skos:prefLabel>
    <skos:example>poets create poems</skos:example>
  </owl:ObjectProperty>
  <owl:ObjectProperty rdf:about="http://vocab.getty.edu/ontology#aat2397_focus_of">
    <rdfs:subPropertyOf rdf:resource="http://www.w3.org/2004/02/skos/core#related"/>
    <dc:title>focus of - field/discipline</dc:title>
    <rdfs:isDefinedBy rdf:resource="http://vocab.getty.edu/ontology"/>
    <skos:example>manuscripts are the focus of codicology</skos:example>
    <skos:example>Plantae (kingdom) is the focus of botany</skos:example>
    <rdfs:range rdf:resource="http://www.w3.org/2004/02/skos/core#Concept"/>
    <skos:example>music is the focus of musicology</skos:example>
    <owl:inverseOf>
      <owl:ObjectProperty rdf:about="http://vocab.getty.edu/ontology#aat2398_focuses_on"/>
    </owl:inverseOf>
    <dct:description>any - [is] focus of - field [of study]/discipline.&#xD;
Example: manuscripts are the focus of codicology; music is the focus of musicology; Plantae (kingdom) is the focus of botany</dct:description>
    <dc:identifier>2397</dc:identifier>
    <rdfs:isDefinedBy rdf:resource="http://vocab.getty.edu/aat/"/>
    <rdfs:domain rdf:resource="http://www.w3.org/2004/02/skos/core#Concept"/>
    <skos:prefLabel>aat2397_focus_of</skos:prefLabel>
  </owl:ObjectProperty>
  <owl:ObjectProperty rdf:about="http://vocab.getty.edu/ontology#aat2554_reflects">
    <skos:example>dhokra (casting technique) reflects Dhokra (culture)</skos:example>
    <rdfs:range rdf:resource="http://www.w3.org/2004/02/skos/core#Concept"/>
    <rdfs:isDefinedBy rdf:resource="http://vocab.getty.edu/ontology"/>
    <rdfs:domain rdf:resource="http://www.w3.org/2004/02/skos/core#Concept"/>
    <dct:description>activity/event - reflects - style/period/culture /[religion/ideology].&#xD;
Example: dhokra (casting technique) reflects Dhokra (culture); red-figure vase painting reflects Red-figure [style]</dct:description>
    <owl:inverseOf rdf:resource="http://vocab.getty.edu/ontology#aat2555_reflected_in"/>
    <dc:identifier>2554</dc:identifier>
    <skos:prefLabel>aat2554_reflects</skos:prefLabel>
    <dc:title>reflects - style/period/culture</dc:title>
    <skos:example>red-figure vase painting reflects Red-figure [style]</skos:example>
    <rdfs:subPropertyOf rdf:resource="http://www.w3.org/2004/02/skos/core#related"/>
    <rdfs:isDefinedBy rdf:resource="http://vocab.getty.edu/aat/"/>
  </owl:ObjectProperty>
  <owl:ObjectProperty rdf:about="http://vocab.getty.edu/ontology#aat2809_coexisted_with">
    <rdfs:subPropertyOf rdf:resource="http://www.w3.org/2004/02/skos/core#related"/>
    <skos:example>Early Minoan coexisted with Prepalatial</skos:example>
    <dct:description>style/period/culture/[religion/ideology] - coexisted with -  style/period/culture/[religion/ideology].&#xD;
Example: Sangoan coexisted with Fauresmith; Early Minoan coexisted with Prepalatial</dct:description>
    <dc:title>coexisted with - style/period/culture</dc:title>
    <rdfs:isDefinedBy rdf:resource="http://vocab.getty.edu/aat/"/>
    <skos:prefLabel>aat2809_coexisted_with</skos:prefLabel>
    <rdfs:isDefinedBy rdf:resource="http://vocab.getty.edu/ontology"/>
    <dc:identifier>2809</dc:identifier>
    <rdf:type rdf:resource="http://www.w3.org/2002/07/owl#SymmetricProperty"/>
    <rdfs:domain rdf:resource="http://www.w3.org/2004/02/skos/core#Concept"/>
    <rdfs:range rdf:resource="http://www.w3.org/2004/02/skos/core#Concept"/>
    <skos:example>Sangoan coexisted with Fauresmith</skos:example>
  </owl:ObjectProperty>
  <owl:ObjectProperty rdf:about="http://vocab.getty.edu/ontology#ulan2575_directed_by">
    <rdfs:isDefinedBy rdf:resource="http://vocab.getty.edu/ulan/"/>
    <dc:identifier>2575</dc:identifier>
    <dc:title>directed by - person</dc:title>
    <skos:example>Gobelins Tapestry Manufactory was directed by Jean Jans I</skos:example>
    <rdfs:range rdf:resource="http://www.w3.org/2004/02/skos/core#Concept"/>
    <skos:prefLabel>ulan2575_directed_by</skos:prefLabel>
    <dct:description>institution - directed by - person.&#xD;
Example: Gobelins Tapestry Manufactory was directed by Jean Jans I</dct:description>
    <rdfs:isDefinedBy rdf:resource="http://vocab.getty.edu/ontology"/>
    <rdfs:subPropertyOf rdf:resource="http://www.w3.org/2004/02/skos/core#related"/>
    <rdfs:domain rdf:resource="http://www.w3.org/2004/02/skos/core#Concept"/>
  </owl:ObjectProperty>
  <owl:ObjectProperty rdf:about="http://vocab.getty.edu/ontology#ulan1309_advisor_of">
    <rdfs:range rdf:resource="http://www.w3.org/2004/02/skos/core#Concept"/>
    <skos:example>Thomas Cromwell, Earl of Essex was the advisor of Henry VIII, King of England</skos:example>
    <rdfs:isDefinedBy rdf:resource="http://vocab.getty.edu/ontology"/>
    <dct:description>person - advisor of - person.&#xD;
Example: Thomas Cromwell, Earl of Essex was the advisor of Henry VIII, King of England</dct:description>
    <rdfs:domain rdf:resource="http://www.w3.org/2004/02/skos/core#Concept"/>
    <dc:title>advisor of - person</dc:title>
    <rdfs:subPropertyOf rdf:resource="http://www.w3.org/2004/02/skos/core#related"/>
    <rdfs:isDefinedBy rdf:resource="http://vocab.getty.edu/ulan/"/>
    <skos:prefLabel>ulan1309_advisor_of</skos:prefLabel>
    <dc:identifier>1309</dc:identifier>
    <owl:inverseOf>
      <owl:ObjectProperty rdf:about="http://vocab.getty.edu/ontology#ulan1310_advised_by"/>
    </owl:inverseOf>
  </owl:ObjectProperty>
  <owl:ObjectProperty rdf:about="http://vocab.getty.edu/ontology#aat2558_reflected_in">
    <rdfs:isDefinedBy rdf:resource="http://vocab.getty.edu/aat/"/>
    <skos:example>Ancient Greek [culture] is reflected in classics (discipline)</skos:example>
    <rdfs:subPropertyOf rdf:resource="http://www.w3.org/2004/02/skos/core#related"/>
    <dc:identifier>2558</dc:identifier>
    <skos:prefLabel>aat2558_reflected_in</skos:prefLabel>
    <skos:example>Buddhism is reflected in bugatu [dance discipline]</skos:example>
    <dc:title>reflected in - field/discipline</dc:title>
    <rdfs:domain rdf:resource="http://www.w3.org/2004/02/skos/core#Concept"/>
    <rdfs:range rdf:resource="http://www.w3.org/2004/02/skos/core#Concept"/>
    <rdfs:isDefinedBy rdf:resource="http://vocab.getty.edu/ontology"/>
    <dct:description>style/period/culture /[religion/ideology] - [is] reflected in field/discipline.&#xD;
Example: Buddhism is reflected in bugatu [dance discipline]; Christianity is reflected in church history; Ancient Greek [culture] is reflected in classics (discipline)</dct:description>
    <skos:example>Christianity is reflected in church history</skos:example>
  </owl:ObjectProperty>
  <owl:ObjectProperty rdf:about="http://vocab.getty.edu/ontology#aat2431_required_for">
    <dc:title>required for - activity/event/process</dc:title>
    <skos:example>dowels are required for doweling</skos:example>
    <rdfs:range rdf:resource="http://www.w3.org/2004/02/skos/core#Concept"/>
    <rdfs:isDefinedBy rdf:resource="http://vocab.getty.edu/aat/"/>
    <owl:inverseOf>
      <owl:ObjectProperty rdf:about="http://vocab.getty.edu/ontology#aat2432_requires"/>
    </owl:inverseOf>
    <dct:description>things/equipment - [are] required for - activity/event/process.&#xD;
Example: painting equipment is required for painting (image making); dowels are required for doweling</dct:description>
    <rdfs:isDefinedBy rdf:resource="http://vocab.getty.edu/ontology"/>
    <rdfs:subPropertyOf rdf:resource="http://www.w3.org/2004/02/skos/core#related"/>
    <skos:example>painting equipment is required for painting (image making)</skos:example>
    <skos:prefLabel>aat2431_required_for</skos:prefLabel>
    <dc:identifier>2431</dc:identifier>
    <rdfs:domain rdf:resource="http://www.w3.org/2004/02/skos/core#Concept"/>
  </owl:ObjectProperty>
  <owl:ObjectProperty rdf:about="http://vocab.getty.edu/ontology#aat2837_source_for">
    <rdfs:range rdf:resource="http://www.w3.org/2004/02/skos/core#Concept"/>
    <dc:identifier>2837</dc:identifier>
    <dc:title>source for - things</dc:title>
    <skos:example>Struthio camelus(species) is the source for ostrich-egg cups</skos:example>
    <rdfs:domain rdf:resource="http://www.w3.org/2004/02/skos/core#Concept"/>
    <rdfs:subPropertyOf rdf:resource="http://www.w3.org/2004/02/skos/core#related"/>
    <skos:prefLabel>aat2837_source_for</skos:prefLabel>
    <dct:description>genus/species [or its parts] - [is] source for - things.&#xD;
Example: Phormium tenax (species) is the source for k?kaku; Struthio camelus(species) is the source for ostrich-egg cups</dct:description>
    <rdfs:isDefinedBy rdf:resource="http://vocab.getty.edu/ontology"/>
    <rdfs:isDefinedBy rdf:resource="http://vocab.getty.edu/aat/"/>
    <skos:example>Phormium tenax (species) is the source for k?kaku</skos:example>
  </owl:ObjectProperty>
  <owl:ObjectProperty rdf:about="http://vocab.getty.edu/ontology#aat2853_involve">
    <rdfs:isDefinedBy rdf:resource="http://vocab.getty.edu/ontology"/>
    <skos:example>camel saddles involve Camelus (genus)</skos:example>
    <dct:description>things/[equipment] - involve - genus/species.&#xD;
Example: rose bowls involve Rosa (genus); camel saddles involve Camelus (genus)</dct:description>
    <rdfs:domain rdf:resource="http://www.w3.org/2004/02/skos/core#Concept"/>
    <dc:identifier>2853</dc:identifier>
    <dc:title>involve - genus/species</dc:title>
    <rdfs:subPropertyOf rdf:resource="http://www.w3.org/2004/02/skos/core#related"/>
    <rdfs:isDefinedBy rdf:resource="http://vocab.getty.edu/aat/"/>
    <skos:example>rose bowls involve Rosa (genus)</skos:example>
    <rdfs:range rdf:resource="http://www.w3.org/2004/02/skos/core#Concept"/>
    <skos:prefLabel>aat2853_involve</skos:prefLabel>
  </owl:ObjectProperty>
  <owl:ObjectProperty rdf:about="http://vocab.getty.edu/ontology#aat2416_requires">
    <skos:prefLabel>aat2416_requires</skos:prefLabel>
    <dct:description>activity/event/[process/function] - requires - material.&#xD;
Example: dying requires dye; pewtersmithing requires pewter</dct:description>
    <rdfs:range rdf:resource="http://www.w3.org/2004/02/skos/core#Concept"/>
    <rdfs:isDefinedBy rdf:resource="http://vocab.getty.edu/ontology"/>
    <dc:title>requires - material</dc:title>
    <rdfs:domain rdf:resource="http://www.w3.org/2004/02/skos/core#Concept"/>
    <skos:example>dying requires dye</skos:example>
    <rdfs:isDefinedBy rdf:resource="http://vocab.getty.edu/aat/"/>
    <skos:example>pewtersmithing requires pewter</skos:example>
    <dc:identifier>2416</dc:identifier>
    <rdfs:subPropertyOf rdf:resource="http://www.w3.org/2004/02/skos/core#related"/>
  </owl:ObjectProperty>
  <owl:ObjectProperty rdf:about="http://vocab.getty.edu/ontology#broaderInstantialExtended">
    <rdfs:isDefinedBy rdf:resource="http://vocab.getty.edu/ontology"/>
    <rdfs:label>broaderInstantialExtended</rdfs:label>
    <rdfs:domain rdf:resource="http://vocab.getty.edu/ontology#Subject"/>
    <rdfs:range rdf:resource="http://vocab.getty.edu/ontology#Subject"/>
    <skos:example>Mt Athos (TGN) BTI orthodox religious center (AAT) BTG Christian religious center (AAT),
so Mt Athos (TGN) BTIE Christian religious center (AAT)</skos:example>
    <dct:description>Ancestors (Instantial). Meaningful closure of gvp:broaderInstantial. Infers iso:broaderInstantial for pairs of directly related skos:Concepts.</dct:description>
    <owl:propertyChainAxiom rdf:parseType="Collection">
      <owl:ObjectProperty rdf:about="http://vocab.getty.edu/ontology#broaderInstantialExtended"/>
      <owl:ObjectProperty rdf:about="http://vocab.getty.edu/ontology#broaderGeneric"/>
    </owl:propertyChainAxiom>
    <rdfs:subPropertyOf rdf:resource="http://vocab.getty.edu/ontology#broaderExtended"/>
  </owl:ObjectProperty>
  <owl:ObjectProperty rdf:about="http://vocab.getty.edu/ontology#aat2208_locus-setting_for">
    <dct:description>locus/setting - [is] locus/setting for - things.&#xD;
Example: glassworks (buildings) are the locus/setting for glassware; caves are the locus/setting for cave paintings</dct:description>
    <rdfs:isDefinedBy rdf:resource="http://vocab.getty.edu/ontology"/>
    <rdfs:subPropertyOf rdf:resource="http://www.w3.org/2004/02/skos/core#related"/>
    <dc:identifier>2208</dc:identifier>
    <skos:prefLabel>aat2208_locus-setting_for</skos:prefLabel>
    <rdfs:domain rdf:resource="http://www.w3.org/2004/02/skos/core#Concept"/>
    <owl:inverseOf rdf:resource="http://vocab.getty.edu/ontology#aat2209_used-located_in"/>
    <dc:title>locus/setting for - things</dc:title>
    <skos:example>caves are the locus/setting for cave paintings</skos:example>
    <rdfs:range rdf:resource="http://www.w3.org/2004/02/skos/core#Concept"/>
    <rdfs:isDefinedBy rdf:resource="http://vocab.getty.edu/aat/"/>
    <skos:example>glassworks (buildings) are the locus/setting for glassware</skos:example>
  </owl:ObjectProperty>
  <owl:ObjectProperty rdf:about="http://vocab.getty.edu/ontology#aat2878_preceded-source_for">
    <rdfs:isDefinedBy rdf:resource="http://vocab.getty.edu/ontology"/>
    <rdfs:subPropertyOf rdf:resource="http://www.w3.org/2004/02/skos/core#related"/>
    <rdfs:domain rdf:resource="http://www.w3.org/2004/02/skos/core#Concept"/>
    <rdfs:range rdf:resource="http://www.w3.org/2004/02/skos/core#Concept"/>
    <skos:example>Ancient Egyptian (language) preceded/is source for Egyptian, Coptic (language)</skos:example>
    <dc:identifier>2878</dc:identifier>
    <owl:inverseOf rdf:resource="http://vocab.getty.edu/ontology#aat2879_followed-developed_from"/>
    <rdfs:isDefinedBy rdf:resource="http://vocab.getty.edu/aat/"/>
    <dc:title>preceded/source for - language</dc:title>
    <skos:prefLabel>aat2878_preceded-source_for</skos:prefLabel>
    <dct:description>language - preceded/[is] source for - language.&#xD;
Example: Ancient Greek (language) preceded/is source for Greek (modern language); Ancient Egyptian (language) preceded/is source for Egyptian, Coptic (language)</dct:description>
    <skos:example>Ancient Greek (language) preceded/is source for Greek (modern language)</skos:example>
  </owl:ObjectProperty>
  <owl:ObjectProperty rdf:about="http://vocab.getty.edu/ontology#aat2295_located_in">
    <skos:example>mountains are located in mountain ranges</skos:example>
    <dc:title>located in - locus/setting</dc:title>
    <rdfs:isDefinedBy rdf:resource="http://vocab.getty.edu/ontology"/>
    <skos:prefLabel>aat2295_located_in</skos:prefLabel>
    <dct:description>locus/setting - [is] located in - locus/setting.&#xD;
Example: national capitals are located in nations; mountains are located in mountain ranges</dct:description>
    <skos:example>national capitals are located in nations</skos:example>
    <rdfs:isDefinedBy rdf:resource="http://vocab.getty.edu/aat/"/>
    <dc:identifier>2295</dc:identifier>
    <rdfs:subPropertyOf rdf:resource="http://www.w3.org/2004/02/skos/core#related"/>
    <rdfs:domain rdf:resource="http://www.w3.org/2004/02/skos/core#Concept"/>
    <rdfs:range rdf:resource="http://www.w3.org/2004/02/skos/core#Concept"/>
  </owl:ObjectProperty>
  <owl:ObjectProperty rdf:about="http://vocab.getty.edu/ontology#aat2502_material_for">
    <rdfs:subPropertyOf rdf:resource="http://www.w3.org/2004/02/skos/core#related"/>
    <skos:prefLabel>aat2502_material_for</skos:prefLabel>
    <rdfs:isDefinedBy rdf:resource="http://vocab.getty.edu/ontology"/>
    <rdfs:range rdf:resource="http://www.w3.org/2004/02/skos/core#Concept"/>
    <skos:example>ivory is material for ivories (sculptures)</skos:example>
    <skos:example>obsidian is material for obsidian mirrors</skos:example>
    <rdfs:domain rdf:resource="http://www.w3.org/2004/02/skos/core#Concept"/>
    <rdfs:isDefinedBy rdf:resource="http://vocab.getty.edu/aat/"/>
    <dc:title>material for - things</dc:title>
    <dc:identifier>2502</dc:identifier>
    <dct:description>material - [is] material for - things.&#xD;
Example: obsidian is material for obsidian mirrors; ivory is material for ivories (sculptures)</dct:description>
  </owl:ObjectProperty>
  <owl:ObjectProperty rdf:about="http://vocab.getty.edu/ontology#termKind">
    <rdfs:isDefinedBy rdf:resource="http://vocab.getty.edu/ontology"/>
    <rdfs:label>termKind</rdfs:label>
    <rdfs:domain rdf:resource="http://www.w3.org/2008/05/skos-xl#Label"/>
    <rdfs:range rdf:resource="http://www.w3.org/2004/02/skos/core#Concept"/>
    <dct:description>Term Kind</dct:description>
  </owl:ObjectProperty>
  <owl:ObjectProperty rdf:about="http://vocab.getty.edu/ontology#aat2552_reflected_in-produces">
    <rdfs:isDefinedBy rdf:resource="http://vocab.getty.edu/aat/"/>
    <skos:prefLabel>aat2552_reflected_in-produces</skos:prefLabel>
    <rdfs:subPropertyOf rdf:resource="http://www.w3.org/2004/02/skos/core#related"/>
    <rdfs:range rdf:resource="http://www.w3.org/2004/02/skos/core#Concept"/>
    <dct:description>style/period/culture/[religion/ideology] - [is] reflected in/produces - things.&#xD;
Example: Nasca [culture] produces/is reflected in Nasca lines; Judaism produces/is reflected in Judaica</dct:description>
    <rdfs:isDefinedBy rdf:resource="http://vocab.getty.edu/ontology"/>
    <dc:identifier>2552</dc:identifier>
    <skos:example>Nasca [culture] produces/is reflected in Nasca lines</skos:example>
    <rdfs:domain rdf:resource="http://www.w3.org/2004/02/skos/core#Concept"/>
    <dc:title>reflected in/produces - things</dc:title>
    <skos:example>Judaism produces/is reflected in Judaica</skos:example>
  </owl:ObjectProperty>
  <owl:ObjectProperty rdf:about="http://vocab.getty.edu/ontology#aat2215_required_for">
    <skos:prefLabel>aat2215_required_for</skos:prefLabel>
    <dc:identifier>2215</dc:identifier>
    <owl:inverseOf rdf:resource="http://vocab.getty.edu/ontology#aat2216_require"/>
    <rdfs:range rdf:resource="http://www.w3.org/2004/02/skos/core#Concept"/>
    <skos:example>compact discs are required for compact disc players</skos:example>
    <dc:title>required for - things</dc:title>
    <skos:example>eyelets are required for broderie anglaise</skos:example>
    <dct:description>things - [are] required for -  things.&#xD;
Example: eyelets are required for broderie anglaise; compact discs are required for compact disc players</dct:description>
    <rdfs:isDefinedBy rdf:resource="http://vocab.getty.edu/ontology"/>
    <rdfs:subPropertyOf rdf:resource="http://www.w3.org/2004/02/skos/core#related"/>
    <rdfs:isDefinedBy rdf:resource="http://vocab.getty.edu/aat/"/>
    <rdfs:domain rdf:resource="http://www.w3.org/2004/02/skos/core#Concept"/>
  </owl:ObjectProperty>
  <owl:ObjectProperty rdf:about="http://vocab.getty.edu/ontology#aat2281_have_counterpart">
    <rdfs:isDefinedBy rdf:resource="http://vocab.getty.edu/aat/"/>
    <dc:title>have counterpart - role</dc:title>
    <skos:example>duchesses have counterpart dukes</skos:example>
    <skos:example>godesses have counterpart gods</skos:example>
    <rdfs:domain rdf:resource="http://www.w3.org/2004/02/skos/core#Concept"/>
    <rdfs:isDefinedBy rdf:resource="http://vocab.getty.edu/ontology"/>
    <rdfs:range rdf:resource="http://www.w3.org/2004/02/skos/core#Concept"/>
    <skos:prefLabel>aat2281_have_counterpart</skos:prefLabel>
    <rdf:type rdf:resource="http://www.w3.org/2002/07/owl#SymmetricProperty"/>
    <dc:identifier>2281</dc:identifier>
    <rdfs:subPropertyOf rdf:resource="http://www.w3.org/2004/02/skos/core#related"/>
    <dct:description>role -[is] counterpart to - role.&#xD;
Example: duchesses have counterpart dukes; godesses have counterpart gods</dct:description>
  </owl:ObjectProperty>
  <owl:ObjectProperty rdf:about="http://vocab.getty.edu/ontology#ulan1317_member_of">
    <skos:example>A member of the Foundation of Documents of Architecture is the National Gallery of Art</skos:example>
    <rdfs:isDefinedBy rdf:resource="http://vocab.getty.edu/ontology"/>
    <rdfs:range rdf:resource="http://www.w3.org/2004/02/skos/core#Concept"/>
    <skos:prefLabel>ulan1317_member_of</skos:prefLabel>
    <owl:inverseOf>
      <owl:ObjectProperty rdf:about="http://vocab.getty.edu/ontology#ulan1318_member_was"/>
    </owl:inverseOf>
    <dct:description>firm/group - member of - person/firm/group.&#xD;
Example: A member of the Foundation of Documents of Architecture is the National Gallery of Art</dct:description>
    <dc:identifier>1317</dc:identifier>
    <rdfs:isDefinedBy rdf:resource="http://vocab.getty.edu/ulan/"/>
    <rdfs:domain rdf:resource="http://www.w3.org/2004/02/skos/core#Concept"/>
    <rdfs:subPropertyOf rdf:resource="http://www.w3.org/2004/02/skos/core#related"/>
    <dc:title>member of - person/firm/group</dc:title>
  </owl:ObjectProperty>
  <owl:ObjectProperty rdf:about="http://vocab.getty.edu/ontology#aat2212_produced_by">
    <skos:example>stereoscopic photographs are produced by stereoscopic cameras</skos:example>
    <dct:description>things - [are] produced by - things/[equipment].&#xD;
Example: stereoscopic photographs are produced by stereoscopic cameras; punchwork is produced by punches (marking tools)</dct:description>
    <rdfs:range rdf:resource="http://www.w3.org/2004/02/skos/core#Concept"/>
    <rdfs:isDefinedBy rdf:resource="http://vocab.getty.edu/ontology"/>
    <skos:example>punchwork is produced by punches (marking tools)</skos:example>
    <dc:identifier>2212</dc:identifier>
    <rdfs:isDefinedBy rdf:resource="http://vocab.getty.edu/aat/"/>
    <skos:prefLabel>aat2212_produced_by</skos:prefLabel>
    <dc:title>produced by - things</dc:title>
    <rdfs:subPropertyOf rdf:resource="http://www.w3.org/2004/02/skos/core#related"/>
    <rdfs:domain rdf:resource="http://www.w3.org/2004/02/skos/core#Concept"/>
  </owl:ObjectProperty>
  <owl:ObjectProperty rdf:about="http://vocab.getty.edu/ontology#termPOS">
    <rdfs:isDefinedBy rdf:resource="http://vocab.getty.edu/ontology"/>
    <rdfs:label>termPOS</rdfs:label>
    <rdfs:domain rdf:resource="http://www.w3.org/2008/05/skos-xl#Label"/>
    <rdfs:range rdf:resource="http://www.w3.org/2004/02/skos/core#Concept"/>
    <dct:description>Part of Speech</dct:description>
  </owl:ObjectProperty>
  <owl:ObjectProperty rdf:about="http://vocab.getty.edu/ontology#aat2398_focuses_on">
    <rdfs:isDefinedBy rdf:resource="http://vocab.getty.edu/ontology"/>
    <dct:description>field [of study]/discipline - focuses on - any.&#xD;
Example: codicology focuses on manuscripts; musicology focuses on music; bontany focuses on Plantae (kingdom)</dct:description>
    <dc:identifier>2398</dc:identifier>
    <dc:title>focuses on - any</dc:title>
    <skos:prefLabel>aat2398_focuses_on</skos:prefLabel>
    <rdfs:range rdf:resource="http://www.w3.org/2004/02/skos/core#Concept"/>
    <skos:example>codicology focuses on manuscripts</skos:example>
    <skos:example>musicology focuses on music</skos:example>
    <rdfs:isDefinedBy rdf:resource="http://vocab.getty.edu/aat/"/>
    <rdfs:domain rdf:resource="http://www.w3.org/2004/02/skos/core#Concept"/>
    <rdfs:subPropertyOf rdf:resource="http://www.w3.org/2004/02/skos/core#related"/>
    <skos:example>bontany focuses on Plantae (kingdom)</skos:example>
  </owl:ObjectProperty>
  <owl:ObjectProperty rdf:about="http://vocab.getty.edu/ontology#aat2892_example_of">
    <skos:prefLabel>aat2892_example_of</skos:prefLabel>
    <rdfs:isDefinedBy rdf:resource="http://vocab.getty.edu/aat/"/>
    <rdfs:range rdf:resource="http://www.w3.org/2004/02/skos/core#Concept"/>
    <dc:identifier>2892</dc:identifier>
    <skos:example>Pictrography (TM) prints are examples of photothermographic transfer prints</skos:example>
    <rdfs:isDefinedBy rdf:resource="http://vocab.getty.edu/ontology"/>
    <rdfs:subPropertyOf rdf:resource="http://www.w3.org/2004/02/skos/core#related"/>
    <rdfs:domain rdf:resource="http://www.w3.org/2004/02/skos/core#Concept"/>
    <dc:title>example of - things</dc:title>
    <dct:description>brand name - [is] example of - things.&#xD;
Example: Pictrography (TM) prints are examples of photothermographic transfer prints</dct:description>
  </owl:ObjectProperty>
  <owl:ObjectProperty rdf:about="http://vocab.getty.edu/ontology#aat2876_characterized_by">
    <skos:example>Celtic (culture) is characterized by Celtic (language)</skos:example>
    <dct:description>style/period/culture - [is] characterized by - language.&#xD;
Example: Afar (culture) is characterized by Afar (language); Celtic (culture) is characterized by Celtic (language)</dct:description>
    <skos:example>Afar (culture) is characterized by Afar (language)</skos:example>
    <dc:title>characterized by - language</dc:title>
    <rdfs:subPropertyOf rdf:resource="http://www.w3.org/2004/02/skos/core#related"/>
    <rdfs:domain rdf:resource="http://www.w3.org/2004/02/skos/core#Concept"/>
    <rdfs:isDefinedBy rdf:resource="http://vocab.getty.edu/ontology"/>
    <rdfs:isDefinedBy rdf:resource="http://vocab.getty.edu/aat/"/>
    <dc:identifier>2876</dc:identifier>
    <rdfs:range rdf:resource="http://www.w3.org/2004/02/skos/core#Concept"/>
    <skos:prefLabel>aat2876_characterized_by</skos:prefLabel>
  </owl:ObjectProperty>
  <owl:ObjectProperty rdf:about="http://vocab.getty.edu/ontology#aat2612_possessed_by-existing_in">
    <rdfs:domain rdf:resource="http://www.w3.org/2004/02/skos/core#Concept"/>
    <skos:example>dry rot is possessed by/existing in wood(plant material)</skos:example>
    <rdfs:isDefinedBy rdf:resource="http://vocab.getty.edu/ontology"/>
    <skos:prefLabel>aat2612_possessed_by-existing_in</skos:prefLabel>
    <rdfs:range rdf:resource="http://www.w3.org/2004/02/skos/core#Concept"/>
    <dc:identifier>2612</dc:identifier>
    <dct:description>attributes /associated concepts - is possessed by/existing in - material.&#xD;
Example: dry rot is possessed by/existing in wood(plant material); dielectric properties are possessed by/existing in dielectric (material)</dct:description>
    <skos:example>dielectric properties are possessed by/existing in dielectric (material)</skos:example>
    <dc:title>possessed by/existing in - material</dc:title>
    <rdfs:isDefinedBy rdf:resource="http://vocab.getty.edu/aat/"/>
    <rdfs:subPropertyOf rdf:resource="http://www.w3.org/2004/02/skos/core#related"/>
    <owl:inverseOf>
      <owl:ObjectProperty rdf:about="http://vocab.getty.edu/ontology#aat2613_possess-exist_in"/>
    </owl:inverseOf>
  </owl:ObjectProperty>
  <owl:ObjectProperty rdf:about="http://vocab.getty.edu/ontology#aat2425_produces">
    <skos:prefLabel>aat2425_produces</skos:prefLabel>
    <dct:description>activity/event/process - produces - material.&#xD;
Example: wiredrawing produces wire; papermaking produces paper</dct:description>
    <rdfs:domain rdf:resource="http://www.w3.org/2004/02/skos/core#Concept"/>
    <rdfs:isDefinedBy rdf:resource="http://vocab.getty.edu/aat/"/>
    <skos:example>wiredrawing produces wire</skos:example>
    <rdfs:subPropertyOf rdf:resource="http://www.w3.org/2004/02/skos/core#related"/>
    <rdfs:range rdf:resource="http://www.w3.org/2004/02/skos/core#Concept"/>
    <dc:title>produces - material</dc:title>
    <skos:example>papermaking produces paper</skos:example>
    <dc:identifier>2425</dc:identifier>
    <rdfs:isDefinedBy rdf:resource="http://vocab.getty.edu/ontology"/>
  </owl:ObjectProperty>
  <owl:ObjectProperty rdf:about="http://vocab.getty.edu/ontology#aat2292_work-live_in">
    <rdfs:range rdf:resource="http://www.w3.org/2004/02/skos/core#Concept"/>
    <rdfs:isDefinedBy rdf:resource="http://vocab.getty.edu/ontology"/>
    <skos:example>nuns live/work in convents (nunneries)</skos:example>
    <rdfs:subPropertyOf rdf:resource="http://www.w3.org/2004/02/skos/core#related"/>
    <dc:title>work/live in - locus/setting</dc:title>
    <dc:identifier>2292</dc:identifier>
    <dct:description>[actor or institution having] role - work/live/[exist] in - locus/setting.&#xD;
Example: rope-makers live/work in roperies; nuns live/work in convents (nunneries); libraries (institutions) live/work in libraries (buildings)</dct:description>
    <rdfs:isDefinedBy rdf:resource="http://vocab.getty.edu/aat/"/>
    <rdfs:domain rdf:resource="http://www.w3.org/2004/02/skos/core#Concept"/>
    <skos:prefLabel>aat2292_work-live_in</skos:prefLabel>
    <skos:example>libraries (institutions) live/work in libraries (buildings)</skos:example>
    <skos:example>rope-makers live/work in roperies</skos:example>
  </owl:ObjectProperty>
  <owl:ObjectProperty rdf:about="http://vocab.getty.edu/ontology#tgn3104_is_location_of">
    <skos:example>tgn:7031416 Silk Road is location of tgn:7018835 Palmyra</skos:example>
    <dct:description>place - is location of - place.&#xD;
Example: tgn:7031416 Silk Road is location of tgn:7018835 Palmyra</dct:description>
    <rdfs:subPropertyOf rdf:resource="http://www.w3.org/2004/02/skos/core#related"/>
    <rdfs:range rdf:resource="http://www.w3.org/2004/02/skos/core#Concept"/>
    <dc:title>is location of - place</dc:title>
    <rdfs:domain rdf:resource="http://www.w3.org/2004/02/skos/core#Concept"/>
    <dc:identifier>3104</dc:identifier>
    <rdfs:isDefinedBy rdf:resource="http://vocab.getty.edu/ontology"/>
    <rdfs:isDefinedBy rdf:resource="http://vocab.getty.edu/tgn/"/>
    <skos:prefLabel>tgn3104_is_location_of</skos:prefLabel>
  </owl:ObjectProperty>
  <owl:ObjectProperty rdf:about="http://vocab.getty.edu/ontology#aat2424_produced_by">
    <dct:description>material - [is] produced by - activity/event/process.&#xD;
Example: wire is produced by wiredrawing; paper is produced by papermaking</dct:description>
    <rdfs:domain rdf:resource="http://www.w3.org/2004/02/skos/core#Concept"/>
    <skos:example>paper is produced by papermaking</skos:example>
    <dc:title>produced by - activity/event/process</dc:title>
    <skos:example>wire is produced by wiredrawing</skos:example>
    <rdfs:subPropertyOf rdf:resource="http://www.w3.org/2004/02/skos/core#related"/>
    <rdfs:isDefinedBy rdf:resource="http://vocab.getty.edu/aat/"/>
    <skos:prefLabel>aat2424_produced_by</skos:prefLabel>
    <dc:identifier>2424</dc:identifier>
    <owl:inverseOf rdf:resource="http://vocab.getty.edu/ontology#aat2425_produces"/>
    <rdfs:range rdf:resource="http://www.w3.org/2004/02/skos/core#Concept"/>
    <rdfs:isDefinedBy rdf:resource="http://vocab.getty.edu/ontology"/>
  </owl:ObjectProperty>
  <owl:ObjectProperty rdf:about="http://vocab.getty.edu/ontology#ulan2574_director_of">
    <owl:inverseOf rdf:resource="http://vocab.getty.edu/ontology#ulan2575_directed_by"/>
    <skos:prefLabel>ulan2574_director_of</skos:prefLabel>
    <rdfs:isDefinedBy rdf:resource="http://vocab.getty.edu/ontology"/>
    <dc:identifier>2574</dc:identifier>
    <skos:example>Jean Jans I directed Gobelins Tapestry Manufactory</skos:example>
    <dct:description>person - director of - institution.&#xD;
Example: Jean Jans I directed Gobelins Tapestry Manufactory</dct:description>
    <rdfs:isDefinedBy rdf:resource="http://vocab.getty.edu/ulan/"/>
    <rdfs:domain rdf:resource="http://www.w3.org/2004/02/skos/core#Concept"/>
    <dc:title>director of - institution</dc:title>
    <rdfs:subPropertyOf rdf:resource="http://www.w3.org/2004/02/skos/core#related"/>
    <rdfs:range rdf:resource="http://www.w3.org/2004/02/skos/core#Concept"/>
  </owl:ObjectProperty>
  <owl:ObjectProperty rdf:about="http://vocab.getty.edu/ontology#aat2604_possessed_by-existing_in">
    <rdfs:range rdf:resource="http://www.w3.org/2004/02/skos/core#Concept"/>
    <rdfs:subPropertyOf rdf:resource="http://www.w3.org/2004/02/skos/core#related"/>
    <rdfs:domain rdf:resource="http://www.w3.org/2004/02/skos/core#Concept"/>
    <dct:description>attributes /associated concepts - [is] possessed by/existing in - things.&#xD;
Example: boudoir (photograph size) is possessed by/existing in boudoir photographs; ruined [condition] is possessed by/existing in ruins</dct:description>
    <skos:example>ruined [condition] is possessed by/existing in ruins</skos:example>
    <rdfs:isDefinedBy rdf:resource="http://vocab.getty.edu/aat/"/>
    <skos:prefLabel>aat2604_possessed_by-existing_in</skos:prefLabel>
    <dc:title>possessed by/existing in - things</dc:title>
    <rdfs:isDefinedBy rdf:resource="http://vocab.getty.edu/ontology"/>
    <skos:example>boudoir (photograph size) is possessed by/existing in boudoir photographs</skos:example>
    <dc:identifier>2604</dc:identifier>
    <owl:inverseOf rdf:resource="http://vocab.getty.edu/ontology#aat2605_possess-exist_in"/>
  </owl:ObjectProperty>
  <owl:ObjectProperty rdf:about="http://vocab.getty.edu/ontology#aat2562_locus-setting_for">
    <owl:inverseOf rdf:resource="http://vocab.getty.edu/ontology#aat2563_located_in"/>
    <rdfs:domain rdf:resource="http://www.w3.org/2004/02/skos/core#Concept"/>
    <dc:title>locus/setting for - style/period/culture</dc:title>
    <skos:prefLabel>aat2562_locus-setting_for</skos:prefLabel>
    <rdfs:isDefinedBy rdf:resource="http://vocab.getty.edu/aat/"/>
    <dc:identifier>2562</dc:identifier>
    <skos:example>agraharas are the locus/setting for Brahmanism</skos:example>
    <rdfs:range rdf:resource="http://www.w3.org/2004/02/skos/core#Concept"/>
    <skos:example>First Nations reserves are the locus/setting for First Nations (culture)</skos:example>
    <rdfs:isDefinedBy rdf:resource="http://vocab.getty.edu/ontology"/>
    <dct:description>locus/setting - [is] locus/setting for - style/period/culture/[religion/ideology].&#xD;
Example: First Nations reserves are the locus/setting for First Nations (culture); agraharas are the locus/setting for Brahmanism</dct:description>
    <rdfs:subPropertyOf rdf:resource="http://www.w3.org/2004/02/skos/core#related"/>
  </owl:ObjectProperty>
  <owl:ObjectProperty rdf:about="http://vocab.getty.edu/ontology#ulan1224_crowned">
    <rdfs:isDefinedBy rdf:resource="http://vocab.getty.edu/ontology"/>
    <rdfs:domain rdf:resource="http://www.w3.org/2004/02/skos/core#Concept"/>
    <skos:prefLabel>ulan1224_crowned</skos:prefLabel>
    <rdfs:range rdf:resource="http://www.w3.org/2004/02/skos/core#Concept"/>
    <dct:description>person - crowned - person.&#xD;
Example: Emperor Charlemagne was crowned by Pope Leo III</dct:description>
    <dc:identifier>1224</dc:identifier>
    <rdfs:isDefinedBy rdf:resource="http://vocab.getty.edu/ulan/"/>
    <dc:title>crowned - person</dc:title>
    <rdfs:subPropertyOf rdf:resource="http://www.w3.org/2004/02/skos/core#related"/>
    <skos:example>Emperor Charlemagne was crowned by Pope Leo III</skos:example>
  </owl:ObjectProperty>
  <owl:ObjectProperty rdf:about="http://vocab.getty.edu/ontology#eventNonPreferred">
    <rdfs:isDefinedBy rdf:resource="http://vocab.getty.edu/ontology"/>
    <rdfs:label>eventNonPreferred</rdfs:label>
    <rdfs:range rdf:resource="http://purl.org/vocab/bio/0.1/Event"/>
    <rdfs:subPropertyOf rdf:resource="http://purl.org/vocab/bio/0.1/event"/>
    <rdfs:comment>Non-preferred life event of an ULAN agent. Domain is schema:Person/Organization, range is bio:Event</rdfs:comment>
    <dct:description>Non-preferred life event of an ULAN agent. Domain is schema:Person/Organization, range is bio:Event</dct:description>
  </owl:ObjectProperty>
  <owl:ObjectProperty rdf:about="http://vocab.getty.edu/ontology#tgn3611_administrative_dependent_of">
    <rdfs:subPropertyOf rdf:resource="http://www.w3.org/2004/02/skos/core#related"/>
    <owl:inverseOf rdf:resource="http://vocab.getty.edu/ontology#tgn3612_administrative_entity_for"/>
    <skos:example>Luni (La Spezia province, Liguria, Italy) is the admisistrative dependent of Ortonovo (Massa-Carrara province, Tuscany, Italy)</skos:example>
    <rdfs:range rdf:resource="http://www.w3.org/2004/02/skos/core#Concept"/>
    <skos:prefLabel>tgn3611_administrative_dependent_of</skos:prefLabel>
    <dct:description>place - administrative dependent of - place; New.&#xD;
Example: Luni (La Spezia province, Liguria, Italy) is the admisistrative dependent of Ortonovo (Massa-Carrara province, Tuscany, Italy)</dct:description>
    <rdfs:domain rdf:resource="http://www.w3.org/2004/02/skos/core#Concept"/>
    <dc:identifier>3611</dc:identifier>
    <rdfs:isDefinedBy rdf:resource="http://vocab.getty.edu/tgn/"/>
    <skos:scopeNote>New</skos:scopeNote>
    <dc:title>administrative dependent of - place</dc:title>
    <rdfs:isDefinedBy rdf:resource="http://vocab.getty.edu/ontology"/>
  </owl:ObjectProperty>
  <owl:ObjectProperty rdf:about="http://vocab.getty.edu/ontology#ulan1575_godchild_of">
    <rdfs:domain rdf:resource="http://www.w3.org/2004/02/skos/core#Concept"/>
    <rdfs:isDefinedBy rdf:resource="http://vocab.getty.edu/ontology"/>
    <dct:description>person - godchild of - person.&#xD;
Example: Jean I Nocret is the godchild of Jean-Baptiste Goy</dct:description>
    <dc:identifier>1575</dc:identifier>
    <rdfs:subPropertyOf rdf:resource="http://www.w3.org/2004/02/skos/core#related"/>
    <skos:example>Jean I Nocret is the godchild of Jean-Baptiste Goy</skos:example>
    <skos:prefLabel>ulan1575_godchild_of</skos:prefLabel>
    <rdfs:isDefinedBy rdf:resource="http://vocab.getty.edu/ulan/"/>
    <rdfs:range rdf:resource="http://www.w3.org/2004/02/skos/core#Concept"/>
    <dc:title>godchild of - person</dc:title>
  </owl:ObjectProperty>
  <owl:ObjectProperty rdf:about="http://vocab.getty.edu/ontology#broaderPartitive">
    <dct:description>BTP (Part/Whole, "part of") relation. We also infer iso-thes:broaderPartitive, which goes only between Concepts.
Example: Tuscany (TGN) BTP Italy (TGN)</dct:description>
    <rdfs:subPropertyOf rdf:resource="http://vocab.getty.edu/ontology#broaderPartitiveExtended"/>
    <skos:example>Tuscany (TGN) BTP Italy (TGN)</skos:example>
    <rdfs:comment>BTP (Part/Whole, "part of") relation. We also infer iso-thes:broaderPartitive, which goes only between Concepts</rdfs:comment>
    <rdfs:subPropertyOf rdf:resource="http://vocab.getty.edu/ontology#broader"/>
    <rdfs:range rdf:resource="http://vocab.getty.edu/ontology#Subject"/>
    <rdfs:domain rdf:resource="http://vocab.getty.edu/ontology#Subject"/>
    <rdfs:label>broaderPartitive</rdfs:label>
    <rdfs:isDefinedBy rdf:resource="http://vocab.getty.edu/ontology"/>
  </owl:ObjectProperty>
  <owl:ObjectProperty rdf:about="http://vocab.getty.edu/ontology#aat2831_associated_with">
    <rdf:type rdf:resource="http://www.w3.org/2002/07/owl#SymmetricProperty"/>
    <rdfs:isDefinedBy rdf:resource="http://vocab.getty.edu/ontology"/>
    <rdfs:subPropertyOf rdf:resource="http://www.w3.org/2004/02/skos/core#related"/>
    <skos:example>Anthonomus grandis (species) [boll weevil] is associated with Gossypium (genus) [cotton]</skos:example>
    <dct:description>genus/species/[other living organism term] - [is] associated with - genus/species.&#xD;
Example: Anthonomus grandis (species) [boll weevil] is associated with Gossypium (genus) [cotton]; Amphiprioninae (subfamily) [clown fish] is associated with Actiniaria (order) [sea anemone]</dct:description>
    <skos:example>Amphiprioninae (subfamily) [clown fish] is associated with Actiniaria (order) [sea anemone]</skos:example>
    <dc:title>associated with - genus/species</dc:title>
    <dc:identifier>2831</dc:identifier>
    <rdfs:domain rdf:resource="http://www.w3.org/2004/02/skos/core#Concept"/>
    <skos:prefLabel>aat2831_associated_with</skos:prefLabel>
    <rdfs:range rdf:resource="http://www.w3.org/2004/02/skos/core#Concept"/>
    <rdfs:isDefinedBy rdf:resource="http://vocab.getty.edu/aat/"/>
  </owl:ObjectProperty>
  <owl:ObjectProperty rdf:about="http://vocab.getty.edu/ontology#ulan2794_representative_of">
    <owl:inverseOf rdf:resource="http://vocab.getty.edu/ontology#ulan2795_representative_was"/>
    <dc:title>representative of - institution</dc:title>
    <rdfs:subPropertyOf rdf:resource="http://www.w3.org/2004/02/skos/core#related"/>
    <rdfs:isDefinedBy rdf:resource="http://vocab.getty.edu/ulan/"/>
    <rdfs:isDefinedBy rdf:resource="http://vocab.getty.edu/ontology"/>
    <rdfs:domain rdf:resource="http://www.w3.org/2004/02/skos/core#Concept"/>
    <dct:description>person - representative of - institution.&#xD;
Example: The Noguch Museum - representative was Isamu Noguchi</dct:description>
    <skos:prefLabel>ulan2794_representative_of</skos:prefLabel>
    <skos:example>The Noguch Museum - representative was Isamu Noguchi</skos:example>
    <dc:identifier>2794</dc:identifier>
    <rdfs:range rdf:resource="http://www.w3.org/2004/02/skos/core#Concept"/>
  </owl:ObjectProperty>
  <owl:ObjectProperty rdf:about="http://vocab.getty.edu/ontology#historicFlag">
    <rdfs:isDefinedBy rdf:resource="http://vocab.getty.edu/ontology"/>
    <rdfs:label>historicFlag</rdfs:label>
    <rdfs:range rdf:resource="http://www.w3.org/2004/02/skos/core#Concept"/>
    <dct:description>Historic Flag</dct:description>
  </owl:ObjectProperty>
  <owl:ObjectProperty rdf:about="http://schema.org/dissolutionLocation">
    <rdfs:isDefinedBy rdf:resource="http://vocab.getty.edu/ontology"/>
    <rdfs:label>dissolutionLocation</rdfs:label>
    <rdfs:domain rdf:resource="http://schema.org/Organization"/>
    <rdfs:range rdf:resource="http://schema.org/Place"/>
    <rdfs:comment>The place where the Organization was dissolved</rdfs:comment>
    <dct:description>The place where the Organization was dissolved.
Schema has properties foundationLocation and dissolutionDate but no dissolutionLocation. 
In contrast, for a person all 4 properties are present: birth/death place/date.
We posted issue https://github.com/schemaorg/schemaorg/issues/302, which looks like it will have a positive outcome in the far future.
And we define the property here</dct:description>
    <rdfs:seeAlso rdf:resource="https://github.com/schemaorg/schemaorg/issues/302"/>
  </owl:ObjectProperty>
  <owl:ObjectProperty rdf:about="http://vocab.getty.edu/ontology#aat2222_are_acted_upon">
    <rdfs:domain rdf:resource="http://www.w3.org/2004/02/skos/core#Concept"/>
    <dct:description>genus/species - is acted upon [by] - [actors having] role.&#xD;
Example: Equus caballus(species) is acted upon by jockeys; Acer saccharum(species) is acted upon by tappers</dct:description>
    <rdfs:isDefinedBy rdf:resource="http://vocab.getty.edu/aat/"/>
    <skos:example>Acer saccharum(species) is acted upon by tappers</skos:example>
    <dc:title>are acted upon - role</dc:title>
    <skos:example>Equus caballus(species) is acted upon by jockeys</skos:example>
    <dc:identifier>2222</dc:identifier>
    <rdfs:isDefinedBy rdf:resource="http://vocab.getty.edu/ontology"/>
    <rdfs:range rdf:resource="http://www.w3.org/2004/02/skos/core#Concept"/>
    <rdfs:subPropertyOf rdf:resource="http://www.w3.org/2004/02/skos/core#related"/>
    <skos:prefLabel>aat2222_are_acted_upon</skos:prefLabel>
  </owl:ObjectProperty>
  <owl:ObjectProperty rdf:about="http://vocab.getty.edu/ontology#sourcePreferred">
    <rdfs:isDefinedBy rdf:resource="http://vocab.getty.edu/ontology"/>
    <rdfs:label>sourcePreferred</rdfs:label>
    <rdfs:domain rdf:resource="http://www.w3.org/2008/05/skos-xl#Label"/>
    <rdfs:range rdf:resource="http://purl.org/ontology/bibo/Document"/>
    <rdfs:subPropertyOf rdf:resource="http://purl.org/dc/terms/source"/>
    <rdfs:comment>Source for which the term is Preferred. Range is bibo:Document or bibo:DocumentPart</rdfs:comment>
    <skos:example>"Isfahan" is preferred in Webster's New Geographical Dictionary (1988)</skos:example>
    <dct:description>Source for which the term is Preferred. Range is bibo:Document or bibo:DocumentPart.
Example: "Isfahan" is preferred in Webster's New Geographical Dictionary (1988)</dct:description>
  </owl:ObjectProperty>
  <owl:ObjectProperty rdf:about="http://vocab.getty.edu/ontology#aat2435_context_for">
    <rdfs:subPropertyOf rdf:resource="http://www.w3.org/2004/02/skos/core#related"/>
    <rdfs:domain rdf:resource="http://www.w3.org/2004/02/skos/core#Concept"/>
    <rdfs:isDefinedBy rdf:resource="http://vocab.getty.edu/aat/"/>
    <dc:identifier>2435</dc:identifier>
    <rdfs:isDefinedBy rdf:resource="http://vocab.getty.edu/ontology"/>
    <skos:example>funerals are the context for funeral books</skos:example>
    <skos:prefLabel>aat2435_context_for</skos:prefLabel>
    <skos:example>Christmas is the context for Christmas trees</skos:example>
    <dct:description>activity/event/process - [is] contextualized in - thing.&#xD;
Example: funerals are the context for funeral books; Christmas is the context for Christmas trees</dct:description>
    <dc:title>context for - things</dc:title>
    <rdfs:range rdf:resource="http://www.w3.org/2004/02/skos/core#Concept"/>
  </owl:ObjectProperty>
  <owl:ObjectProperty rdf:about="http://vocab.getty.edu/ontology#aat2218_used-function_as">
    <rdfs:isDefinedBy rdf:resource="http://vocab.getty.edu/aat/"/>
    <dct:description>things - [are] used/function as - things.&#xD;
Example: arc lamps are used/function as lighthouse lamps;  toile peinte is used/function as cartoons (working drawings)</dct:description>
    <owl:inverseOf>
      <owl:ObjectProperty rdf:about="http://vocab.getty.edu/ontology#aat2219_have_form"/>
    </owl:inverseOf>
    <rdfs:isDefinedBy rdf:resource="http://vocab.getty.edu/ontology"/>
    <skos:example>arc lamps are used/function as lighthouse lamps</skos:example>
    <skos:prefLabel>aat2218_used-function_as</skos:prefLabel>
    <dc:title>used/function as - things</dc:title>
    <skos:example>toile peinte is used/function as cartoons (working drawings)</skos:example>
    <dc:identifier>2218</dc:identifier>
    <rdfs:subPropertyOf rdf:resource="http://www.w3.org/2004/02/skos/core#related"/>
    <rdfs:domain rdf:resource="http://www.w3.org/2004/02/skos/core#Concept"/>
    <rdfs:range rdf:resource="http://www.w3.org/2004/02/skos/core#Concept"/>
  </owl:ObjectProperty>
  <owl:ObjectProperty rdf:about="http://vocab.getty.edu/ontology#ulan1102_student_of">
    <dct:description>person - student of - person.&#xD;
Example: Pierre Subleyras was the student of Rivalz, Antoine</dct:description>
    <rdfs:domain rdf:resource="http://www.w3.org/2004/02/skos/core#Concept"/>
    <dc:title>student of - person</dc:title>
    <skos:prefLabel>ulan1102_student_of</skos:prefLabel>
    <rdfs:subPropertyOf rdf:resource="http://www.w3.org/2004/02/skos/core#related"/>
    <rdfs:range rdf:resource="http://www.w3.org/2004/02/skos/core#Concept"/>
    <skos:example>Pierre Subleyras was the student of Rivalz, Antoine</skos:example>
    <dc:identifier>1102</dc:identifier>
    <rdfs:isDefinedBy rdf:resource="http://vocab.getty.edu/ulan/"/>
    <rdfs:isDefinedBy rdf:resource="http://vocab.getty.edu/ontology"/>
  </owl:ObjectProperty>
  <owl:ObjectProperty rdf:about="http://vocab.getty.edu/ontology#aat2885_involves">
    <skos:example>Celtic culture involves Celtic crosses (design motif)</skos:example>
    <dc:identifier>2885</dc:identifier>
    <rdfs:range rdf:resource="http://www.w3.org/2004/02/skos/core#Concept"/>
    <rdfs:subPropertyOf rdf:resource="http://www.w3.org/2004/02/skos/core#related"/>
    <skos:prefLabel>aat2885_involves</skos:prefLabel>
    <dct:description>any - involves - attributes /associated concepts.&#xD;
Example: climate change involves climate;  infestation involves insect damage; Celtic culture involves Celtic crosses (design motif)</dct:description>
    <skos:example>climate change involves climate</skos:example>
    <rdfs:isDefinedBy rdf:resource="http://vocab.getty.edu/ontology"/>
    <rdfs:isDefinedBy rdf:resource="http://vocab.getty.edu/aat/"/>
    <rdfs:domain rdf:resource="http://www.w3.org/2004/02/skos/core#Concept"/>
    <skos:example>infestation involves insect damage</skos:example>
    <dc:title>involves - attributes /associated concepts</dc:title>
  </owl:ObjectProperty>
  <owl:ObjectProperty rdf:about="http://vocab.getty.edu/ontology#aat2319_involves">
    <rdfs:isDefinedBy rdf:resource="http://vocab.getty.edu/ontology"/>
    <dct:description>activity/event - involves - [actors having] role.&#xD;
Example: weddings involve bridegrooms; martyrdoms involve martyrs</dct:description>
    <rdfs:domain rdf:resource="http://www.w3.org/2004/02/skos/core#Concept"/>
    <rdfs:range rdf:resource="http://www.w3.org/2004/02/skos/core#Concept"/>
    <rdfs:isDefinedBy rdf:resource="http://vocab.getty.edu/aat/"/>
    <skos:prefLabel>aat2319_involves</skos:prefLabel>
    <rdfs:subPropertyOf rdf:resource="http://www.w3.org/2004/02/skos/core#related"/>
    <skos:example>weddings involve bridegrooms</skos:example>
    <skos:example>martyrdoms involve martyrs</skos:example>
    <dc:title>involves - role</dc:title>
    <dc:identifier>2319</dc:identifier>
  </owl:ObjectProperty>
  <owl:ObjectProperty rdf:about="http://vocab.getty.edu/ontology#aat2311_performed_by">
    <skos:example>clockmaking is performed by clockmakers</skos:example>
    <rdfs:range rdf:resource="http://www.w3.org/2004/02/skos/core#Concept"/>
    <dc:identifier>2311</dc:identifier>
    <rdfs:domain rdf:resource="http://www.w3.org/2004/02/skos/core#Concept"/>
    <skos:example>curating is performed by curators</skos:example>
    <rdfs:isDefinedBy rdf:resource="http://vocab.getty.edu/ontology"/>
    <dc:title>performed by - role</dc:title>
    <skos:prefLabel>aat2311_performed_by</skos:prefLabel>
    <dct:description>activity/event/[process/function] - [is] performed by - [actors having] a role.&#xD;
Example: clockmaking is performed by clockmakers; curating is performed by curators</dct:description>
    <rdfs:isDefinedBy rdf:resource="http://vocab.getty.edu/aat/"/>
    <owl:inverseOf rdf:resource="http://vocab.getty.edu/ontology#aat2312_perform"/>
    <rdfs:subPropertyOf rdf:resource="http://www.w3.org/2004/02/skos/core#related"/>
  </owl:ObjectProperty>
  <owl:ObjectProperty rdf:about="http://vocab.getty.edu/ontology#aat2848_involved_in">
    <rdfs:subPropertyOf rdf:resource="http://www.w3.org/2004/02/skos/core#related"/>
    <skos:prefLabel>aat2848_involved_in</skos:prefLabel>
    <rdfs:domain rdf:resource="http://www.w3.org/2004/02/skos/core#Concept"/>
    <rdfs:isDefinedBy rdf:resource="http://vocab.getty.edu/aat/"/>
    <dc:title>involved in - activity/event</dc:title>
    <rdfs:range rdf:resource="http://www.w3.org/2004/02/skos/core#Concept"/>
    <dct:description>genus/species - is involved in - activity/event.&#xD;
Example: bulls (animals) are involved in bullfighting; Equus caballus (species) is involved in polo(field sport)</dct:description>
    <skos:example>Equus caballus (species) is involved in polo(field sport)</skos:example>
    <dc:identifier>2848</dc:identifier>
    <skos:example>bulls (animals) are involved in bullfighting</skos:example>
    <owl:inverseOf rdf:resource="http://vocab.getty.edu/ontology#aat2849_involves"/>
    <rdfs:isDefinedBy rdf:resource="http://vocab.getty.edu/ontology"/>
  </owl:ObjectProperty>
  <owl:ObjectProperty rdf:about="http://vocab.getty.edu/ontology#ulan1308_assisted_by">
    <dc:identifier>1308</dc:identifier>
    <dc:title>assisted by - person</dc:title>
    <rdfs:subPropertyOf rdf:resource="http://www.w3.org/2004/02/skos/core#related"/>
    <dct:description>person - assisted by - person.&#xD;
Example: Pablo Picasso was assisted by Bernard Castelli</dct:description>
    <rdfs:domain rdf:resource="http://www.w3.org/2004/02/skos/core#Concept"/>
    <rdfs:isDefinedBy rdf:resource="http://vocab.getty.edu/ontology"/>
    <skos:example>Pablo Picasso was assisted by Bernard Castelli</skos:example>
    <rdfs:isDefinedBy rdf:resource="http://vocab.getty.edu/ulan/"/>
    <rdfs:range rdf:resource="http://www.w3.org/2004/02/skos/core#Concept"/>
    <skos:prefLabel>ulan1308_assisted_by</skos:prefLabel>
  </owl:ObjectProperty>
  <owl:ObjectProperty rdf:about="http://vocab.getty.edu/ontology#tgn3102_coextensive_with">
    <skos:prefLabel>tgn3102_coextensive_with</skos:prefLabel>
    <rdfs:isDefinedBy rdf:resource="http://vocab.getty.edu/ontology"/>
    <dc:title>coextensive with - place</dc:title>
    <rdfs:subPropertyOf rdf:resource="http://www.w3.org/2004/02/skos/core#related"/>
    <rdfs:isDefinedBy rdf:resource="http://vocab.getty.edu/tgn/"/>
    <rdf:type rdf:resource="http://www.w3.org/2002/07/owl#SymmetricProperty"/>
    <dct:description>place - coextensive with - place.&#xD;
Example: Kings county (New York, USA) is coextensive with Brooklyn (New York, USA)</dct:description>
    <dc:identifier>3102</dc:identifier>
    <rdfs:domain rdf:resource="http://www.w3.org/2004/02/skos/core#Concept"/>
    <skos:example>Kings county (New York, USA) is coextensive with Brooklyn (New York, USA)</skos:example>
    <rdfs:range rdf:resource="http://www.w3.org/2004/02/skos/core#Concept"/>
  </owl:ObjectProperty>
  <owl:ObjectProperty rdf:about="http://vocab.getty.edu/ontology#aat2608_causes-required_for">
    <skos:prefLabel>aat2608_causes-required_for</skos:prefLabel>
    <skos:example>creasing (process) causes/is required for creases (condition)</skos:example>
    <rdfs:isDefinedBy rdf:resource="http://vocab.getty.edu/aat/"/>
    <dc:identifier>2608</dc:identifier>
    <rdfs:isDefinedBy rdf:resource="http://vocab.getty.edu/ontology"/>
    <rdfs:range rdf:resource="http://www.w3.org/2004/02/skos/core#Concept"/>
    <dct:description>activity/event/[process/function] - causes/[is] required for - [a] state/condition/attributes.&#xD;
Example: waterproofing causes/is required for watertighness; creasing (process) causes/is required for creases (condition)</dct:description>
    <rdfs:subPropertyOf rdf:resource="http://www.w3.org/2004/02/skos/core#related"/>
    <rdfs:domain rdf:resource="http://www.w3.org/2004/02/skos/core#Concept"/>
    <dc:title>causes/required for - attributes /associated concepts</dc:title>
    <skos:example>waterproofing causes/is required for watertighness</skos:example>
  </owl:ObjectProperty>
  <owl:ObjectProperty rdf:about="http://vocab.getty.edu/ontology#aat2508_produced-processed_by">
    <dc:title>produced/processed by - things</dc:title>
    <rdfs:isDefinedBy rdf:resource="http://vocab.getty.edu/ontology"/>
    <dct:description>material - [is] produced/processed by - things/[equipment].&#xD;
Example: cotton gins produce/process cotton (fiber); waterwells produce/process groundwater</dct:description>
    <rdfs:isDefinedBy rdf:resource="http://vocab.getty.edu/aat/"/>
    <rdfs:domain rdf:resource="http://www.w3.org/2004/02/skos/core#Concept"/>
    <skos:prefLabel>aat2508_produced-processed_by</skos:prefLabel>
    <rdfs:subPropertyOf rdf:resource="http://www.w3.org/2004/02/skos/core#related"/>
    <skos:example>cotton gins produce/process cotton (fiber)</skos:example>
    <rdfs:range rdf:resource="http://www.w3.org/2004/02/skos/core#Concept"/>
    <dc:identifier>2508</dc:identifier>
    <skos:example>waterwells produce/process groundwater</skos:example>
  </owl:ObjectProperty>
  <owl:ObjectProperty rdf:about="http://vocab.getty.edu/ontology#ulan1318_member_was">
    <rdfs:subPropertyOf rdf:resource="http://www.w3.org/2004/02/skos/core#related"/>
    <rdfs:domain rdf:resource="http://www.w3.org/2004/02/skos/core#Concept"/>
    <rdfs:isDefinedBy rdf:resource="http://vocab.getty.edu/ontology"/>
    <skos:example>The National Gallery of Art was/is a member of the Foundation of Documentation of Architecture</skos:example>
    <dc:title>member was - firm/group</dc:title>
    <rdfs:range rdf:resource="http://www.w3.org/2004/02/skos/core#Concept"/>
    <dc:identifier>1318</dc:identifier>
    <rdfs:isDefinedBy rdf:resource="http://vocab.getty.edu/ulan/"/>
    <skos:prefLabel>ulan1318_member_was</skos:prefLabel>
    <dct:description>person/firm/group - member was - firm/group.&#xD;
Example: The National Gallery of Art was/is a member of the Foundation of Documentation of Architecture</dct:description>
  </owl:ObjectProperty>
  <owl:ObjectProperty rdf:about="http://vocab.getty.edu/ontology#ulan2778_owner_of">
    <rdfs:subPropertyOf rdf:resource="http://www.w3.org/2004/02/skos/core#related"/>
    <dc:title>owner of - person</dc:title>
    <dct:description>firm - owner of - person.&#xD;
Example: Walter Scott Lenox was the owner of Lenox China Co.</dct:description>
    <owl:inverseOf rdf:resource="http://vocab.getty.edu/ontology#ulan2779_owned_by"/>
    <rdfs:domain rdf:resource="http://www.w3.org/2004/02/skos/core#Concept"/>
    <rdfs:range rdf:resource="http://www.w3.org/2004/02/skos/core#Concept"/>
    <skos:prefLabel>ulan2778_owner_of</skos:prefLabel>
    <rdfs:isDefinedBy rdf:resource="http://vocab.getty.edu/ontology"/>
    <dc:identifier>2778</dc:identifier>
    <skos:example>Walter Scott Lenox was the owner of Lenox China Co.</skos:example>
    <rdfs:isDefinedBy rdf:resource="http://vocab.getty.edu/ulan/"/>
  </owl:ObjectProperty>
  <owl:ObjectProperty rdf:about="http://vocab.getty.edu/ontology#aat2815_composed_of">
    <dct:description>material - [is] composed of - material.&#xD;
Example: composite white is composed of titanium white; desert varnish is composed of iron oxide</dct:description>
    <rdfs:subPropertyOf rdf:resource="http://www.w3.org/2004/02/skos/core#related"/>
    <skos:example>composite white is composed of titanium white</skos:example>
    <rdfs:domain rdf:resource="http://www.w3.org/2004/02/skos/core#Concept"/>
    <skos:prefLabel>aat2815_composed_of</skos:prefLabel>
    <rdfs:isDefinedBy rdf:resource="http://vocab.getty.edu/ontology"/>
    <dc:title>composed of - material</dc:title>
    <dc:identifier>2815</dc:identifier>
    <rdfs:isDefinedBy rdf:resource="http://vocab.getty.edu/aat/"/>
    <rdfs:range rdf:resource="http://www.w3.org/2004/02/skos/core#Concept"/>
    <skos:example>desert varnish is composed of iron oxide</skos:example>
  </owl:ObjectProperty>
  <owl:ObjectProperty rdf:about="http://vocab.getty.edu/ontology#aat2846_locus-setting_for">
    <skos:prefLabel>aat2846_locus-setting_for</skos:prefLabel>
    <rdfs:isDefinedBy rdf:resource="http://vocab.getty.edu/aat/"/>
    <rdfs:subPropertyOf rdf:resource="http://www.w3.org/2004/02/skos/core#related"/>
    <dc:identifier>2846</dc:identifier>
    <rdfs:range rdf:resource="http://www.w3.org/2004/02/skos/core#Concept"/>
    <skos:example>vineyards are the locus/setting of Vitaceae (family)</skos:example>
    <dc:title>locus/setting for - genus/species</dc:title>
    <skos:example>elephant houses are the locus/setting for Elephantidae(family)</skos:example>
    <rdfs:domain rdf:resource="http://www.w3.org/2004/02/skos/core#Concept"/>
    <rdfs:isDefinedBy rdf:resource="http://vocab.getty.edu/ontology"/>
    <dct:description>locus/setting - [is] locus/setting for - genus/species.&#xD;
Example: elephant houses are the locus/setting for Elephantidae(family); vineyards are the locus/setting of Vitaceae (family)</dct:description>
  </owl:ObjectProperty>
  <owl:ObjectProperty rdf:about="http://vocab.getty.edu/ontology#aat2219_have_form">
    <dc:title>have form - things</dc:title>
    <skos:prefLabel>aat2219_have_form</skos:prefLabel>
    <rdfs:domain rdf:resource="http://www.w3.org/2004/02/skos/core#Concept"/>
    <rdfs:range rdf:resource="http://www.w3.org/2004/02/skos/core#Concept"/>
    <skos:example>cartoons (working drawings) have the form of toile peinte</skos:example>
    <rdfs:subPropertyOf rdf:resource="http://www.w3.org/2004/02/skos/core#related"/>
    <rdfs:isDefinedBy rdf:resource="http://vocab.getty.edu/aat/"/>
    <dc:identifier>2219</dc:identifier>
    <rdfs:isDefinedBy rdf:resource="http://vocab.getty.edu/ontology"/>
    <dct:description>things - have form [of] - things.&#xD;
Example: lighthouse lamps have the form of arc lamps; cartoons (working drawings) have the form of toile peinte</dct:description>
    <skos:example>lighthouse lamps have the form of arc lamps</skos:example>
  </owl:ObjectProperty>
  <owl:ObjectProperty rdf:about="http://vocab.getty.edu/ontology#ulan1531_nephew-niece_of">
    <rdfs:range rdf:resource="http://www.w3.org/2004/02/skos/core#Concept"/>
    <skos:prefLabel>ulan1531_nephew-niece_of</skos:prefLabel>
    <owl:inverseOf rdf:resource="http://vocab.getty.edu/ontology#ulan1532_uncle-aunt_of"/>
    <dc:title>nephew/niece of - person</dc:title>
    <rdfs:domain rdf:resource="http://www.w3.org/2004/02/skos/core#Concept"/>
    <rdfs:isDefinedBy rdf:resource="http://vocab.getty.edu/ontology"/>
    <dc:identifier>1531</dc:identifier>
    <rdfs:isDefinedBy rdf:resource="http://vocab.getty.edu/ulan/"/>
    <rdfs:subPropertyOf rdf:resource="http://www.w3.org/2004/02/skos/core#related"/>
    <skos:example>Jan Brueghel, the elder is the nephew/neice of  Pieter Coecke van Aeist, the younger</skos:example>
    <dct:description>person - nephew/niece of - person.&#xD;
Example: Jan Brueghel, the elder is the nephew/neice of  Pieter Coecke van Aeist, the younger</dct:description>
  </owl:ObjectProperty>
  <owl:ObjectProperty rdf:about="http://vocab.getty.edu/ontology#ulan1205_client_of">
    <owl:inverseOf>
      <owl:ObjectProperty rdf:about="http://vocab.getty.edu/ontology#ulan1206_client_was"/>
    </owl:inverseOf>
    <dc:identifier>1205</dc:identifier>
    <rdfs:isDefinedBy rdf:resource="http://vocab.getty.edu/ulan/"/>
    <dct:description>person/firm/family - client of - person/firm/family.&#xD;
Example: The Chicago Herald was the client of Burnham and Root</dct:description>
    <rdfs:subPropertyOf rdf:resource="http://www.w3.org/2004/02/skos/core#related"/>
    <dc:title>client of - person/firm/family</dc:title>
    <skos:prefLabel>ulan1205_client_of</skos:prefLabel>
    <rdfs:isDefinedBy rdf:resource="http://vocab.getty.edu/ontology"/>
    <rdfs:domain rdf:resource="http://www.w3.org/2004/02/skos/core#Concept"/>
    <rdfs:range rdf:resource="http://www.w3.org/2004/02/skos/core#Concept"/>
    <skos:example>The Chicago Herald was the client of Burnham and Root</skos:example>
  </owl:ObjectProperty>
  <owl:ObjectProperty rdf:about="http://vocab.getty.edu/ontology#ulan1513_grandchild_of">
    <dct:description>person - grandchild of - person.&#xD;
Example: Eric Lloyd Wright is the grandchild of Frank Lloyd Wright</dct:description>
    <rdfs:isDefinedBy rdf:resource="http://vocab.getty.edu/ulan/"/>
    <skos:example>Eric Lloyd Wright is the grandchild of Frank Lloyd Wright</skos:example>
    <owl:inverseOf rdf:resource="http://vocab.getty.edu/ontology#ulan1514_gandparent_of"/>
    <dc:identifier>1513</dc:identifier>
    <rdfs:isDefinedBy rdf:resource="http://vocab.getty.edu/ontology"/>
    <skos:prefLabel>ulan1513_grandchild_of</skos:prefLabel>
    <dc:title>grandchild of - person</dc:title>
    <rdfs:range rdf:resource="http://www.w3.org/2004/02/skos/core#Concept"/>
    <rdfs:subPropertyOf rdf:resource="http://www.w3.org/2004/02/skos/core#related"/>
    <rdfs:domain rdf:resource="http://www.w3.org/2004/02/skos/core#Concept"/>
  </owl:ObjectProperty>
  <owl:ObjectProperty rdf:about="http://vocab.getty.edu/ontology#ulan1555_adopted_child_of">
    <rdfs:domain rdf:resource="http://www.w3.org/2004/02/skos/core#Concept"/>
    <rdfs:isDefinedBy rdf:resource="http://vocab.getty.edu/ontology"/>
    <rdfs:range rdf:resource="http://www.w3.org/2004/02/skos/core#Concept"/>
    <dc:title>adopted child of - person</dc:title>
    <dc:identifier>1555</dc:identifier>
    <skos:example>Augusts, Emperor of Rome is the adopted child of Julius Caesar</skos:example>
    <rdfs:subPropertyOf rdf:resource="http://www.w3.org/2004/02/skos/core#related"/>
    <dct:description>person - adopted child of - person.&#xD;
Example: Augusts, Emperor of Rome is the adopted child of Julius Caesar</dct:description>
    <rdfs:isDefinedBy rdf:resource="http://vocab.getty.edu/ulan/"/>
    <skos:prefLabel>ulan1555_adopted_child_of</skos:prefLabel>
  </owl:ObjectProperty>
  <owl:ObjectProperty rdf:about="http://vocab.getty.edu/ontology#aat2205_causes-is_required">
    <skos:example>on-demand printing causes/is required for on-demand publishing</skos:example>
    <rdfs:range rdf:resource="http://www.w3.org/2004/02/skos/core#Concept"/>
    <skos:prefLabel>aat2205_causes-is_required</skos:prefLabel>
    <rdfs:domain rdf:resource="http://www.w3.org/2004/02/skos/core#Concept"/>
    <dc:identifier>2205</dc:identifier>
    <rdfs:isDefinedBy rdf:resource="http://vocab.getty.edu/ontology"/>
    <dc:title>causes/is required - activity/event</dc:title>
    <dct:description>activity/event/[process/function] - causes/is required for - activity/event/[process/function].&#xD;
Example: on-demand printing causes/is required for on-demand publishing;  preserving causes/is required for preservation</dct:description>
    <rdfs:isDefinedBy rdf:resource="http://vocab.getty.edu/aat/"/>
    <rdfs:subPropertyOf rdf:resource="http://www.w3.org/2004/02/skos/core#related"/>
    <skos:example>preserving causes/is required for preservation</skos:example>
    <owl:inverseOf>
      <owl:ObjectProperty rdf:about="http://vocab.getty.edu/ontology#aat2206_caused_by-requires"/>
    </owl:inverseOf>
  </owl:ObjectProperty>
  <owl:ObjectProperty rdf:about="http://vocab.getty.edu/ontology#tgn3411_successor_of">
    <skos:example>Iran (nation) is the successor of Persia</skos:example>
    <dct:description>nation - successor of - nation.&#xD;
Example: Iran (nation) is the successor of Persia</dct:description>
    <skos:prefLabel>tgn3411_successor_of</skos:prefLabel>
    <rdfs:range rdf:resource="http://www.w3.org/2004/02/skos/core#Concept"/>
    <rdfs:isDefinedBy rdf:resource="http://vocab.getty.edu/tgn/"/>
    <rdfs:subPropertyOf rdf:resource="http://www.w3.org/2004/02/skos/core#related"/>
    <rdfs:domain rdf:resource="http://www.w3.org/2004/02/skos/core#Concept"/>
    <dc:identifier>3411</dc:identifier>
    <owl:inverseOf rdf:resource="http://vocab.getty.edu/ontology#tgn3412_predecessor_of"/>
    <rdfs:isDefinedBy rdf:resource="http://vocab.getty.edu/ontology"/>
    <dc:title>successor of - nation</dc:title>
  </owl:ObjectProperty>
  <owl:ObjectProperty rdf:about="http://vocab.getty.edu/ontology#aat2419_used_for">
    <rdfs:isDefinedBy rdf:resource="http://vocab.getty.edu/ontology"/>
    <skos:example>astronomical instruments are used for astronomy</skos:example>
    <dc:title>used for - field/discipline</dc:title>
    <rdfs:range rdf:resource="http://www.w3.org/2004/02/skos/core#Concept"/>
    <skos:example>divination objects are used for divination [discipline]</skos:example>
    <dct:description>things/[equipment] - [are] used for - field [of study]/discipline.&#xD;
Example: astronomical instruments are used for astronomy; divination objects are used for divination [discipline]</dct:description>
    <rdfs:subPropertyOf rdf:resource="http://www.w3.org/2004/02/skos/core#related"/>
    <rdfs:isDefinedBy rdf:resource="http://vocab.getty.edu/aat/"/>
    <skos:prefLabel>aat2419_used_for</skos:prefLabel>
    <rdfs:domain rdf:resource="http://www.w3.org/2004/02/skos/core#Concept"/>
    <dc:identifier>2419</dc:identifier>
  </owl:ObjectProperty>
  <owl:ObjectProperty rdf:about="http://vocab.getty.edu/ontology#ulan1581_descendant_of">
    <dc:identifier>1581</dc:identifier>
    <owl:inverseOf>
      <owl:ObjectProperty rdf:about="http://vocab.getty.edu/ontology#ulan1582_ancestor_of"/>
    </owl:inverseOf>
    <skos:prefLabel>ulan1581_descendant_of</skos:prefLabel>
    <rdfs:isDefinedBy rdf:resource="http://vocab.getty.edu/ulan/"/>
    <dc:title>descendant of - person</dc:title>
    <rdfs:isDefinedBy rdf:resource="http://vocab.getty.edu/ontology"/>
    <dct:description>person - descendant of - person.&#xD;
Example: Paolo Caliari is the descendant of Paolo Veronese</dct:description>
    <rdfs:range rdf:resource="http://www.w3.org/2004/02/skos/core#Concept"/>
    <rdfs:domain rdf:resource="http://www.w3.org/2004/02/skos/core#Concept"/>
    <skos:example>Paolo Caliari is the descendant of Paolo Veronese</skos:example>
    <rdfs:subPropertyOf rdf:resource="http://www.w3.org/2004/02/skos/core#related"/>
  </owl:ObjectProperty>
  <owl:ObjectProperty rdf:about="http://vocab.getty.edu/ontology#placeTypeNonPreferred">
    <rdfs:isDefinedBy rdf:resource="http://vocab.getty.edu/ontology"/>
    <rdfs:label>placeTypeNonPreferred</rdfs:label>
    <rdfs:domain rdf:resource="http://vocab.getty.edu/ontology#Subject"/>
    <rdfs:range rdf:resource="http://vocab.getty.edu/ontology#Subject"/>
    <rdfs:subPropertyOf rdf:resource="http://vocab.getty.edu/ontology#placeType"/>
    <rdfs:comment>A secondary type for a TGN Place. Domain is TGN concept, range is AAT concept</rdfs:comment>
    <skos:example>A non-preferred type of Machupicchu, Peru is "Inca center" (historical)</skos:example>
    <dct:description>A secondary type for a TGN Place. Domain is TGN concept, range is AAT concept.
Example: A non-preferred type of Machupicchu, Peru is "Inca center" (historical)</dct:description>
  </owl:ObjectProperty>
  <owl:ObjectProperty rdf:about="http://vocab.getty.edu/ontology#aat2325_created_by">
    <rdfs:subPropertyOf rdf:resource="http://www.w3.org/2004/02/skos/core#related"/>
    <dc:title>created by - role</dc:title>
    <skos:prefLabel>aat2325_created_by</skos:prefLabel>
    <dc:identifier>2325</dc:identifier>
    <rdfs:domain rdf:resource="http://www.w3.org/2004/02/skos/core#Concept"/>
    <owl:inverseOf rdf:resource="http://vocab.getty.edu/ontology#aat2326_create"/>
    <skos:example>poems are created by poets</skos:example>
    <dct:description>things - [are] created by - [actors having] role.&#xD;
Example: drawings are created by draftsmen; poems are created by poets</dct:description>
    <rdfs:isDefinedBy rdf:resource="http://vocab.getty.edu/aat/"/>
    <rdfs:range rdf:resource="http://www.w3.org/2004/02/skos/core#Concept"/>
    <rdfs:isDefinedBy rdf:resource="http://vocab.getty.edu/ontology"/>
    <skos:example>drawings are created by draftsmen</skos:example>
  </owl:ObjectProperty>
  <owl:ObjectProperty rdf:about="http://vocab.getty.edu/ontology#ulan1562_step-parent_of">
    <rdfs:range rdf:resource="http://www.w3.org/2004/02/skos/core#Concept"/>
    <skos:example>Napoleon I, Emperor of the French is the step-parent of Hortense, Quene consort of Louis Bonaparte</skos:example>
    <rdfs:subPropertyOf rdf:resource="http://www.w3.org/2004/02/skos/core#related"/>
    <dc:identifier>1562</dc:identifier>
    <rdfs:isDefinedBy rdf:resource="http://vocab.getty.edu/ontology"/>
    <dc:title>step-parent of - person</dc:title>
    <rdfs:domain rdf:resource="http://www.w3.org/2004/02/skos/core#Concept"/>
    <dct:description>person - step-parent of - person.&#xD;
Example: Napoleon I, Emperor of the French is the step-parent of Hortense, Quene consort of Louis Bonaparte</dct:description>
    <rdfs:isDefinedBy rdf:resource="http://vocab.getty.edu/ulan/"/>
    <skos:prefLabel>ulan1562_step-parent_of</skos:prefLabel>
  </owl:ObjectProperty>
  <owl:ObjectProperty rdf:about="http://vocab.getty.edu/ontology#termType">
    <rdfs:isDefinedBy rdf:resource="http://vocab.getty.edu/ontology"/>
    <rdfs:label>termType</rdfs:label>
    <rdfs:domain rdf:resource="http://www.w3.org/2008/05/skos-xl#Label"/>
    <rdfs:range rdf:resource="http://www.w3.org/2004/02/skos/core#Concept"/>
    <dct:description>Term Type</dct:description>
  </owl:ObjectProperty>
  <owl:ObjectProperty rdf:about="http://vocab.getty.edu/ontology#aat2421_locus-setting_for">
    <rdfs:range rdf:resource="http://www.w3.org/2004/02/skos/core#Concept"/>
    <dct:description>locus/setting - [is] locus/setting for - activity/event/[process/function].&#xD;
Example: smelters (metalworking plants) are the locus/setting for smelting; pilgrimage centers are the locus/setting for pilgrimages</dct:description>
    <skos:prefLabel>aat2421_locus-setting_for</skos:prefLabel>
    <skos:example>smelters (metalworking plants) are the locus/setting for smelting</skos:example>
    <rdfs:subPropertyOf rdf:resource="http://www.w3.org/2004/02/skos/core#related"/>
    <dc:title>locus/setting for - activity/event</dc:title>
    <rdfs:isDefinedBy rdf:resource="http://vocab.getty.edu/ontology"/>
    <rdfs:domain rdf:resource="http://www.w3.org/2004/02/skos/core#Concept"/>
    <owl:inverseOf>
      <owl:ObjectProperty rdf:about="http://vocab.getty.edu/ontology#aat2422_takes_place_in"/>
    </owl:inverseOf>
    <dc:identifier>2421</dc:identifier>
    <rdfs:isDefinedBy rdf:resource="http://vocab.getty.edu/aat/"/>
    <skos:example>pilgrimage centers are the locus/setting for pilgrimages</skos:example>
  </owl:ObjectProperty>
  <owl:ObjectProperty rdf:about="http://vocab.getty.edu/ontology#ulan1203_donor_of">
    <rdfs:range rdf:resource="http://www.w3.org/2004/02/skos/core#Concept"/>
    <rdfs:isDefinedBy rdf:resource="http://vocab.getty.edu/ulan/"/>
    <rdfs:subPropertyOf rdf:resource="http://www.w3.org/2004/02/skos/core#related"/>
    <owl:inverseOf rdf:resource="http://vocab.getty.edu/ontology#ulan1204_donor_was"/>
    <rdfs:isDefinedBy rdf:resource="http://vocab.getty.edu/ontology"/>
    <rdfs:domain rdf:resource="http://www.w3.org/2004/02/skos/core#Concept"/>
    <dc:identifier>1203</dc:identifier>
    <skos:example>Andrew W. Mellon was a donor of National Gallery of Art</skos:example>
    <skos:prefLabel>ulan1203_donor_of</skos:prefLabel>
    <dct:description>person/firm/family - donor of - person/firm/family.&#xD;
Example: Andrew W. Mellon was a donor of National Gallery of Art</dct:description>
    <dc:title>donor of - person/firm/family</dc:title>
  </owl:ObjectProperty>
  <owl:ObjectProperty rdf:about="http://vocab.getty.edu/ontology#ulan1101_teacher_of">
    <rdfs:isDefinedBy rdf:resource="http://vocab.getty.edu/ontology"/>
    <rdfs:range rdf:resource="http://www.w3.org/2004/02/skos/core#Concept"/>
    <dct:description>person - teacher of - person.&#xD;
Example: Rivalz, Antoine was the teacher of Pierre Subleyras</dct:description>
    <skos:prefLabel>ulan1101_teacher_of</skos:prefLabel>
    <rdfs:subPropertyOf rdf:resource="http://www.w3.org/2004/02/skos/core#related"/>
    <dc:identifier>1101</dc:identifier>
    <skos:example>Rivalz, Antoine was the teacher of Pierre Subleyras</skos:example>
    <rdfs:domain rdf:resource="http://www.w3.org/2004/02/skos/core#Concept"/>
    <dc:title>teacher of - person</dc:title>
    <rdfs:isDefinedBy rdf:resource="http://vocab.getty.edu/ulan/"/>
    <owl:inverseOf rdf:resource="http://vocab.getty.edu/ontology#ulan1102_student_of"/>
  </owl:ObjectProperty>
  <owl:ObjectProperty rdf:about="http://vocab.getty.edu/ontology#aat2802_exemplified_by">
    <owl:inverseOf rdf:resource="http://vocab.getty.edu/ontology#aat2803_example_of"/>
    <dct:description>material - [is] exemplified by - brand name.&#xD;
Example: petrolium jelly is exemplified by Vaseline (TM); polytetrafluoroethyelene is exemplified by Teflon (TM)</dct:description>
    <skos:example>polytetrafluoroethyelene is exemplified by Teflon (TM)</skos:example>
    <rdfs:domain rdf:resource="http://www.w3.org/2004/02/skos/core#Concept"/>
    <dc:title>exemplified by - brand name</dc:title>
    <skos:example>petrolium jelly is exemplified by Vaseline (TM)</skos:example>
    <rdfs:isDefinedBy rdf:resource="http://vocab.getty.edu/aat/"/>
    <rdfs:isDefinedBy rdf:resource="http://vocab.getty.edu/ontology"/>
    <skos:prefLabel>aat2802_exemplified_by</skos:prefLabel>
    <rdfs:subPropertyOf rdf:resource="http://www.w3.org/2004/02/skos/core#related"/>
    <dc:identifier>2802</dc:identifier>
    <rdfs:range rdf:resource="http://www.w3.org/2004/02/skos/core#Concept"/>
  </owl:ObjectProperty>
  <owl:ObjectProperty rdf:about="http://vocab.getty.edu/ontology#ulan1107_influenced">
    <dct:description>person - influenced - person.&#xD;
Example: Rembrandt van Rijn influenced Salomon Koninck</dct:description>
    <rdfs:isDefinedBy rdf:resource="http://vocab.getty.edu/ontology"/>
    <rdfs:isDefinedBy rdf:resource="http://vocab.getty.edu/ulan/"/>
    <skos:example>Rembrandt van Rijn influenced Salomon Koninck</skos:example>
    <rdfs:range rdf:resource="http://www.w3.org/2004/02/skos/core#Concept"/>
    <rdfs:domain rdf:resource="http://www.w3.org/2004/02/skos/core#Concept"/>
    <owl:inverseOf>
      <owl:ObjectProperty rdf:about="http://vocab.getty.edu/ontology#ulan1108_influenced_by"/>
    </owl:inverseOf>
    <rdfs:subPropertyOf rdf:resource="http://www.w3.org/2004/02/skos/core#related"/>
    <skos:prefLabel>ulan1107_influenced</skos:prefLabel>
    <dc:title>influenced - person</dc:title>
    <dc:identifier>1107</dc:identifier>
  </owl:ObjectProperty>
  <owl:ObjectProperty rdf:about="http://vocab.getty.edu/ontology#ulan2675_professor_was">
    <rdfs:subPropertyOf rdf:resource="http://www.w3.org/2004/02/skos/core#related"/>
    <rdfs:domain rdf:resource="http://www.w3.org/2004/02/skos/core#Concept"/>
    <skos:example>A professor at Bauhaus was Paul Klee</skos:example>
    <dc:title>professor was - person</dc:title>
    <skos:prefLabel>ulan2675_professor_was</skos:prefLabel>
    <rdfs:isDefinedBy rdf:resource="http://vocab.getty.edu/ontology"/>
    <dct:description>institution - professor was - person.&#xD;
Example: A professor at Bauhaus was Paul Klee</dct:description>
    <rdfs:isDefinedBy rdf:resource="http://vocab.getty.edu/ulan/"/>
    <rdfs:range rdf:resource="http://www.w3.org/2004/02/skos/core#Concept"/>
    <dc:identifier>2675</dc:identifier>
  </owl:ObjectProperty>
  <owl:ObjectProperty rdf:about="http://vocab.getty.edu/ontology#aat2884_involved_with">
    <dc:identifier>2884</dc:identifier>
    <rdfs:range rdf:resource="http://www.w3.org/2004/02/skos/core#Concept"/>
    <rdfs:isDefinedBy rdf:resource="http://vocab.getty.edu/aat/"/>
    <rdfs:subPropertyOf rdf:resource="http://www.w3.org/2004/02/skos/core#related"/>
    <skos:example>insect damage is involved with infestation</skos:example>
    <skos:example>climate is involved with climate change</skos:example>
    <rdfs:domain rdf:resource="http://www.w3.org/2004/02/skos/core#Concept"/>
    <dc:title>involved with - any</dc:title>
    <rdfs:isDefinedBy rdf:resource="http://vocab.getty.edu/ontology"/>
    <owl:inverseOf rdf:resource="http://vocab.getty.edu/ontology#aat2885_involves"/>
    <skos:example>Celtic crosses (design motif) are involved with Celtic culture</skos:example>
    <skos:prefLabel>aat2884_involved_with</skos:prefLabel>
    <dct:description>attributes /associated concepts - [are] involved with - any.&#xD;
Example: climate is involved with climate change; insect damage is involved with infestation; Celtic crosses (design motif) are involved with Celtic culture</dct:description>
  </owl:ObjectProperty>
  <owl:ObjectProperty rdf:about="http://vocab.getty.edu/ontology#aat2432_requires">
    <skos:example>doweling requires dowels</skos:example>
    <dct:description>activity/event/process - requires - things/equipment.&#xD;
Example: painting (image making) requires painting equipment; doweling requires dowels</dct:description>
    <skos:example>painting (image making) requires painting equipment</skos:example>
    <dc:title>requires - things</dc:title>
    <rdfs:range rdf:resource="http://www.w3.org/2004/02/skos/core#Concept"/>
    <rdfs:isDefinedBy rdf:resource="http://vocab.getty.edu/aat/"/>
    <skos:prefLabel>aat2432_requires</skos:prefLabel>
    <dc:identifier>2432</dc:identifier>
    <rdfs:subPropertyOf rdf:resource="http://www.w3.org/2004/02/skos/core#related"/>
    <rdfs:isDefinedBy rdf:resource="http://vocab.getty.edu/ontology"/>
    <rdfs:domain rdf:resource="http://www.w3.org/2004/02/skos/core#Concept"/>
  </owl:ObjectProperty>
  <owl:ObjectProperty rdf:about="http://vocab.getty.edu/ontology#ulan1421_founded_by">
    <skos:example>National Gallery of Art was founded by United States Congress</skos:example>
    <dct:description>firm/group - founded by - firm/group.&#xD;
Example: National Gallery of Art was founded by United States Congress</dct:description>
    <dc:title>founded by - firm/group</dc:title>
    <rdfs:isDefinedBy rdf:resource="http://vocab.getty.edu/ulan/"/>
    <rdfs:domain rdf:resource="http://www.w3.org/2004/02/skos/core#Concept"/>
    <rdfs:range rdf:resource="http://www.w3.org/2004/02/skos/core#Concept"/>
    <skos:prefLabel>ulan1421_founded_by</skos:prefLabel>
    <rdfs:subPropertyOf rdf:resource="http://www.w3.org/2004/02/skos/core#related"/>
    <dc:identifier>1421</dc:identifier>
    <owl:inverseOf rdf:resource="http://vocab.getty.edu/ontology#ulan1422_founded"/>
    <rdfs:isDefinedBy rdf:resource="http://vocab.getty.edu/ontology"/>
  </owl:ObjectProperty>
  <owl:ObjectProperty rdf:about="http://vocab.getty.edu/ontology#ulan1112_master_was">
    <skos:prefLabel>ulan1112_master_was</skos:prefLabel>
    <dc:title>master was - person</dc:title>
    <rdfs:subPropertyOf rdf:resource="http://www.w3.org/2004/02/skos/core#related"/>
    <rdfs:domain rdf:resource="http://www.w3.org/2004/02/skos/core#Concept"/>
    <dc:identifier>1112</dc:identifier>
    <rdfs:range rdf:resource="http://www.w3.org/2004/02/skos/core#Concept"/>
    <skos:example>Peter Paul Rubens - master of Jan Thomas</skos:example>
    <rdfs:isDefinedBy rdf:resource="http://vocab.getty.edu/ontology"/>
    <rdfs:isDefinedBy rdf:resource="http://vocab.getty.edu/ulan/"/>
    <dct:description>person - master was - person.&#xD;
Example: Peter Paul Rubens - master of Jan Thomas</dct:description>
  </owl:ObjectProperty>
  <owl:ObjectProperty rdf:about="http://vocab.getty.edu/ontology#aat2828_use-require">
    <rdfs:domain rdf:resource="http://www.w3.org/2004/02/skos/core#Concept"/>
    <rdfs:isDefinedBy rdf:resource="http://vocab.getty.edu/ontology"/>
    <skos:example>wine glasses use/require wine</skos:example>
    <owl:inverseOf rdf:resource="http://vocab.getty.edu/ontology#aat2829_used-required_for"/>
    <rdfs:range rdf:resource="http://www.w3.org/2004/02/skos/core#Concept"/>
    <dct:description>things - use/require - material.&#xD;
Example: oil paintings use/require varnish; wine glasses use/require wine</dct:description>
    <rdfs:subPropertyOf rdf:resource="http://www.w3.org/2004/02/skos/core#related"/>
    <dc:title>use/require - material</dc:title>
    <rdfs:isDefinedBy rdf:resource="http://vocab.getty.edu/aat/"/>
    <skos:prefLabel>aat2828_use-require</skos:prefLabel>
    <skos:example>oil paintings use/require varnish</skos:example>
    <dc:identifier>2828</dc:identifier>
  </owl:ObjectProperty>
  <owl:ObjectProperty rdf:about="http://vocab.getty.edu/ontology#ulan1582_ancestor_of">
    <dct:description>person - ancestor of - person.&#xD;
Example: Paolo Veronese is the ancestor of Paolo Caliari</dct:description>
    <dc:title>ancestor of - person</dc:title>
    <skos:prefLabel>ulan1582_ancestor_of</skos:prefLabel>
    <rdfs:subPropertyOf rdf:resource="http://www.w3.org/2004/02/skos/core#related"/>
    <dc:identifier>1582</dc:identifier>
    <rdfs:domain rdf:resource="http://www.w3.org/2004/02/skos/core#Concept"/>
    <rdfs:isDefinedBy rdf:resource="http://vocab.getty.edu/ulan/"/>
    <rdfs:range rdf:resource="http://www.w3.org/2004/02/skos/core#Concept"/>
    <rdfs:isDefinedBy rdf:resource="http://vocab.getty.edu/ontology"/>
    <skos:example>Paolo Veronese is the ancestor of Paolo Caliari</skos:example>
  </owl:ObjectProperty>
  <owl:ObjectProperty rdf:about="http://vocab.getty.edu/ontology#ulan2693_president_was">
    <skos:example>A president of National Gallery of Art was David K. E. Bruce</skos:example>
    <rdfs:range rdf:resource="http://www.w3.org/2004/02/skos/core#Concept"/>
    <rdfs:isDefinedBy rdf:resource="http://vocab.getty.edu/ontology"/>
    <rdfs:domain rdf:resource="http://www.w3.org/2004/02/skos/core#Concept"/>
    <dct:description>institution - president was - person.&#xD;
Example: A president of National Gallery of Art was David K. E. Bruce</dct:description>
    <rdfs:isDefinedBy rdf:resource="http://vocab.getty.edu/ulan/"/>
    <dc:title>president was - person</dc:title>
    <rdfs:subPropertyOf rdf:resource="http://www.w3.org/2004/02/skos/core#related"/>
    <dc:identifier>2693</dc:identifier>
    <skos:prefLabel>ulan2693_president_was</skos:prefLabel>
  </owl:ObjectProperty>
  <owl:ObjectProperty rdf:about="http://vocab.getty.edu/ontology#ulan2573_founded_by">
    <rdfs:isDefinedBy rdf:resource="http://vocab.getty.edu/ulan/"/>
    <skos:example>Tiffany Glass &amp; Decorating Company was founded by Louis Comfort Tiffany</skos:example>
    <skos:prefLabel>ulan2573_founded_by</skos:prefLabel>
    <rdfs:subPropertyOf rdf:resource="http://www.w3.org/2004/02/skos/core#related"/>
    <rdfs:range rdf:resource="http://www.w3.org/2004/02/skos/core#Concept"/>
    <dc:title>founded by - person</dc:title>
    <rdfs:domain rdf:resource="http://www.w3.org/2004/02/skos/core#Concept"/>
    <rdfs:isDefinedBy rdf:resource="http://vocab.getty.edu/ontology"/>
    <dct:description>institution - founded by - person.&#xD;
Example: Tiffany Glass &amp; Decorating Company was founded by Louis Comfort Tiffany</dct:description>
    <dc:identifier>2573</dc:identifier>
  </owl:ObjectProperty>
  <owl:ObjectProperty rdf:about="http://vocab.getty.edu/ontology#ulan2583_chairman_of">
    <dct:description>person - chairman of - institution</dct:description>
    <rdfs:isDefinedBy rdf:resource="http://vocab.getty.edu/ontology"/>
    <dc:identifier>2583</dc:identifier>
    <dc:title>chairman of - institution</dc:title>
    <rdfs:subPropertyOf rdf:resource="http://www.w3.org/2004/02/skos/core#related"/>
    <rdfs:isDefinedBy rdf:resource="http://vocab.getty.edu/ulan/"/>
    <rdfs:domain rdf:resource="http://www.w3.org/2004/02/skos/core#Concept"/>
    <skos:prefLabel>ulan2583_chairman_of</skos:prefLabel>
    <rdfs:range rdf:resource="http://www.w3.org/2004/02/skos/core#Concept"/>
    <owl:inverseOf>
      <owl:ObjectProperty rdf:about="http://vocab.getty.edu/ontology#ulan2584_chaired_by"/>
    </owl:inverseOf>
  </owl:ObjectProperty>
  <owl:ObjectProperty rdf:about="http://vocab.getty.edu/ontology#ulan1316_principal_was">
    <dc:title>principal was - person</dc:title>
    <skos:example>Orazio Fontana was principal in Fontana Workshop</skos:example>
    <rdfs:isDefinedBy rdf:resource="http://vocab.getty.edu/ulan/"/>
    <dc:identifier>1316</dc:identifier>
    <dct:description>firm - principal was - person.&#xD;
Example: Orazio Fontana was principal in Fontana Workshop</dct:description>
    <rdfs:domain rdf:resource="http://www.w3.org/2004/02/skos/core#Concept"/>
    <rdfs:isDefinedBy rdf:resource="http://vocab.getty.edu/ontology"/>
    <skos:prefLabel>ulan1316_principal_was</skos:prefLabel>
    <rdfs:range rdf:resource="http://www.w3.org/2004/02/skos/core#Concept"/>
    <rdfs:subPropertyOf rdf:resource="http://www.w3.org/2004/02/skos/core#related"/>
  </owl:ObjectProperty>
  <owl:ObjectProperty rdf:about="http://vocab.getty.edu/ontology#aat2812_followed">
    <skos:example>Micoquian followed Acheulian</skos:example>
    <rdfs:isDefinedBy rdf:resource="http://vocab.getty.edu/aat/"/>
    <rdfs:isDefinedBy rdf:resource="http://vocab.getty.edu/ontology"/>
    <dc:identifier>2812</dc:identifier>
    <dc:title>followed - style/period/culture</dc:title>
    <skos:prefLabel>aat2812_followed</skos:prefLabel>
    <rdfs:range rdf:resource="http://www.w3.org/2004/02/skos/core#Concept"/>
    <skos:example>Abstract Impressionism followed Impressionist</skos:example>
    <rdfs:domain rdf:resource="http://www.w3.org/2004/02/skos/core#Concept"/>
    <dct:description>style/period/culture/[religion/ideology] - followed  - style/period/culture/[religion/ideology].&#xD;
Example: Abstract Impressionism followed Impressionist; Micoquian followed Acheulian</dct:description>
    <rdfs:subPropertyOf rdf:resource="http://www.w3.org/2004/02/skos/core#related"/>
  </owl:ObjectProperty>
  <owl:ObjectProperty rdf:about="http://vocab.getty.edu/ontology#ulan2696_leader_of">
    <rdfs:range rdf:resource="http://www.w3.org/2004/02/skos/core#Concept"/>
    <rdfs:isDefinedBy rdf:resource="http://vocab.getty.edu/ulan/"/>
    <dc:title>leader of - institution</dc:title>
    <rdfs:subPropertyOf rdf:resource="http://www.w3.org/2004/02/skos/core#related"/>
    <dct:description>person - leader of - institution.&#xD;
Example: Rush Harrison Kress was the leader of Samuel H. Kress Foundation</dct:description>
    <skos:prefLabel>ulan2696_leader_of</skos:prefLabel>
    <owl:inverseOf rdf:resource="http://vocab.getty.edu/ontology#ulan2697_leader_was"/>
    <rdfs:isDefinedBy rdf:resource="http://vocab.getty.edu/ontology"/>
    <rdfs:domain rdf:resource="http://www.w3.org/2004/02/skos/core#Concept"/>
    <skos:example>Rush Harrison Kress was the leader of Samuel H. Kress Foundation</skos:example>
    <dc:identifier>2696</dc:identifier>
  </owl:ObjectProperty>
  <owl:ObjectProperty rdf:about="http://vocab.getty.edu/ontology#ulan1108_influenced_by">
    <rdfs:range rdf:resource="http://www.w3.org/2004/02/skos/core#Concept"/>
    <dc:identifier>1108</dc:identifier>
    <dct:description>person - influenced by - person.&#xD;
Example: Salomon Koninck was influenced by Rembrandt van Rijn</dct:description>
    <rdfs:domain rdf:resource="http://www.w3.org/2004/02/skos/core#Concept"/>
    <rdfs:isDefinedBy rdf:resource="http://vocab.getty.edu/ulan/"/>
    <rdfs:subPropertyOf rdf:resource="http://www.w3.org/2004/02/skos/core#related"/>
    <skos:example>Salomon Koninck was influenced by Rembrandt van Rijn</skos:example>
    <rdfs:isDefinedBy rdf:resource="http://vocab.getty.edu/ontology"/>
    <skos:prefLabel>ulan1108_influenced_by</skos:prefLabel>
    <dc:title>influenced by - person</dc:title>
  </owl:ObjectProperty>
  <owl:ObjectProperty rdf:about="http://vocab.getty.edu/ontology#ulan1201_patron_of">
    <rdfs:domain rdf:resource="http://www.w3.org/2004/02/skos/core#Concept"/>
    <skos:prefLabel>ulan1201_patron_of</skos:prefLabel>
    <rdfs:isDefinedBy rdf:resource="http://vocab.getty.edu/ulan/"/>
    <dc:identifier>1201</dc:identifier>
    <rdfs:subPropertyOf rdf:resource="http://www.w3.org/2004/02/skos/core#related"/>
    <dc:title>patron of - person/firm/family</dc:title>
    <rdfs:isDefinedBy rdf:resource="http://vocab.getty.edu/ontology"/>
    <skos:example>Cosimo I, Grand-Duke of Tuscany was the patron of Donatello</skos:example>
    <owl:inverseOf>
      <owl:ObjectProperty rdf:about="http://vocab.getty.edu/ontology#ulan1202_patron_was"/>
    </owl:inverseOf>
    <rdfs:range rdf:resource="http://www.w3.org/2004/02/skos/core#Concept"/>
    <dct:description>person - patron of - person/firm/family.&#xD;
Example: Cosimo I, Grand-Duke of Tuscany was the patron of Donatello</dct:description>
  </owl:ObjectProperty>
  <owl:ObjectProperty rdf:about="http://vocab.getty.edu/ontology#aat2842_source_for">
    <dc:identifier>2842</dc:identifier>
    <rdfs:domain rdf:resource="http://www.w3.org/2004/02/skos/core#Concept"/>
    <rdfs:range rdf:resource="http://www.w3.org/2004/02/skos/core#Concept"/>
    <skos:prefLabel>aat2842_source_for</skos:prefLabel>
    <rdfs:isDefinedBy rdf:resource="http://vocab.getty.edu/ontology"/>
    <skos:example>Acer (genus) is the source for maple (wood)</skos:example>
    <dct:description>genus/species - [is] source for - material.&#xD;
Example: Vicugna pacos (species) is the source for alpaca (wool); Acer (genus) is the source for maple (wood)</dct:description>
    <rdfs:isDefinedBy rdf:resource="http://vocab.getty.edu/aat/"/>
    <skos:example>Vicugna pacos (species) is the source for alpaca (wool)</skos:example>
    <dc:title>source for - material</dc:title>
    <rdfs:subPropertyOf rdf:resource="http://www.w3.org/2004/02/skos/core#related"/>
  </owl:ObjectProperty>
  <owl:ObjectProperty rdf:about="http://vocab.getty.edu/ontology#ulan2677_teacher_was">
    <dc:title>teacher was - person</dc:title>
    <rdfs:isDefinedBy rdf:resource="http://vocab.getty.edu/ulan/"/>
    <skos:prefLabel>ulan2677_teacher_was</skos:prefLabel>
    <rdfs:range rdf:resource="http://www.w3.org/2004/02/skos/core#Concept"/>
    <rdfs:isDefinedBy rdf:resource="http://vocab.getty.edu/ontology"/>
    <dct:description>institution - teacher was - person.&#xD;
Example: A teacher at Black Mountain College was Willem De Kooning</dct:description>
    <rdfs:domain rdf:resource="http://www.w3.org/2004/02/skos/core#Concept"/>
    <skos:example>A teacher at Black Mountain College was Willem De Kooning</skos:example>
    <rdfs:subPropertyOf rdf:resource="http://www.w3.org/2004/02/skos/core#related"/>
    <dc:identifier>2677</dc:identifier>
  </owl:ObjectProperty>
  <owl:ObjectProperty rdf:about="http://vocab.getty.edu/ontology#aat2841_derived-made_from">
    <skos:example>maple (wood) is derived from Acer (genus)</skos:example>
    <rdfs:domain rdf:resource="http://www.w3.org/2004/02/skos/core#Concept"/>
    <skos:prefLabel>aat2841_derived-made_from</skos:prefLabel>
    <dc:identifier>2841</dc:identifier>
    <dc:title>derived/made from - genus/species</dc:title>
    <dct:description>material - [is] derived/made from - genus/species.&#xD;
Example: alpaca (wool) is derived from Vicugna pacos (species); maple (wood) is derived from Acer (genus)</dct:description>
    <rdfs:subPropertyOf rdf:resource="http://www.w3.org/2004/02/skos/core#related"/>
    <rdfs:range rdf:resource="http://www.w3.org/2004/02/skos/core#Concept"/>
    <owl:inverseOf rdf:resource="http://vocab.getty.edu/ontology#aat2842_source_for"/>
    <rdfs:isDefinedBy rdf:resource="http://vocab.getty.edu/ontology"/>
    <skos:example>alpaca (wool) is derived from Vicugna pacos (species)</skos:example>
    <rdfs:isDefinedBy rdf:resource="http://vocab.getty.edu/aat/"/>
  </owl:ObjectProperty>
  <owl:ObjectProperty rdf:about="http://vocab.getty.edu/ontology#aat2294_locus-setting_for">
    <rdfs:range rdf:resource="http://www.w3.org/2004/02/skos/core#Concept"/>
    <owl:inverseOf rdf:resource="http://vocab.getty.edu/ontology#aat2295_located_in"/>
    <rdfs:isDefinedBy rdf:resource="http://vocab.getty.edu/ontology"/>
    <rdfs:subPropertyOf rdf:resource="http://www.w3.org/2004/02/skos/core#related"/>
    <dc:title>locus/setting for - locus/setting</dc:title>
    <dct:description>locus/setting - [is] locus setting for - locus/setting.&#xD;
Example: nations are the locus/setting for national capitals; mountain ranges are the locus/setting for mountains</dct:description>
    <dc:identifier>2294</dc:identifier>
    <rdfs:isDefinedBy rdf:resource="http://vocab.getty.edu/aat/"/>
    <skos:prefLabel>aat2294_locus-setting_for</skos:prefLabel>
    <rdfs:domain rdf:resource="http://www.w3.org/2004/02/skos/core#Concept"/>
    <skos:example>mountain ranges are the locus/setting for mountains</skos:example>
    <skos:example>nations are the locus/setting for national capitals</skos:example>
  </owl:ObjectProperty>
  <owl:ObjectProperty rdf:about="http://vocab.getty.edu/ontology#agentTypePreferred">
    <rdfs:isDefinedBy rdf:resource="http://vocab.getty.edu/ontology"/>
    <rdfs:label>agentTypePreferred</rdfs:label>
    <rdfs:domain rdf:resource="http://vocab.getty.edu/ontology#Subject"/>
    <rdfs:range rdf:resource="http://vocab.getty.edu/ontology#Subject"/>
    <rdfs:subPropertyOf>
      <owl:ObjectProperty rdf:about="http://vocab.getty.edu/ontology#agentType"/>
    </rdfs:subPropertyOf>
    <rdfs:comment>The primary type of a ULAN Person or Corporate body. Domain is ULAN concept, range is AAT concept</rdfs:comment>
    <skos:example>The preferred type of "Albrecht Duerer Workshop" (ULAN) is "workshop" (AAT)</skos:example>
    <dct:description>The primary type of a ULAN Person or Corporate body. Domain is ULAN concept, range is AAT concept.
Example: The preferred type of "Albrecht Duerer Workshop" (ULAN) is "workshop" (AAT)</dct:description>
  </owl:ObjectProperty>
  <owl:ObjectProperty rdf:about="http://vocab.getty.edu/ontology#aat2505_locus-setting_for">
    <rdfs:subPropertyOf rdf:resource="http://www.w3.org/2004/02/skos/core#related"/>
    <rdfs:isDefinedBy rdf:resource="http://vocab.getty.edu/aat/"/>
    <rdfs:domain rdf:resource="http://www.w3.org/2004/02/skos/core#Concept"/>
    <skos:example>volcanoes are locus/setting for  tephra</skos:example>
    <skos:example>brickworks (factories) are locus/setting for brick (clay product)</skos:example>
    <rdfs:range rdf:resource="http://www.w3.org/2004/02/skos/core#Concept"/>
    <dct:description>locus/setting - [is] locus/setting for - material.&#xD;
Example: volcanoes are locus/setting for  tephra; brickworks (factories) are locus/setting for brick (clay product)</dct:description>
    <dc:identifier>2505</dc:identifier>
    <rdfs:isDefinedBy rdf:resource="http://vocab.getty.edu/ontology"/>
    <dc:title>locus/setting for - material</dc:title>
    <skos:prefLabel>aat2505_locus-setting_for</skos:prefLabel>
  </owl:ObjectProperty>
  <owl:ObjectProperty rdf:about="http://vocab.getty.edu/ontology#eventPreferred">
    <rdfs:isDefinedBy rdf:resource="http://vocab.getty.edu/ontology"/>
    <rdfs:label>eventPreferred</rdfs:label>
    <rdfs:range rdf:resource="http://purl.org/vocab/bio/0.1/Event"/>
    <rdfs:subPropertyOf rdf:resource="http://purl.org/vocab/bio/0.1/event"/>
    <rdfs:comment>Preferred life event of an ULAN agent. Domain is schema:Person/Organization, range is bio:Event</rdfs:comment>
    <dct:description>Preferred life event of an ULAN agent. Domain is schema:Person/Organization, range is bio:Event</dct:description>
  </owl:ObjectProperty>
  <owl:ObjectProperty rdf:about="http://vocab.getty.edu/ontology#aat2315_used_by">
    <rdfs:range rdf:resource="http://www.w3.org/2004/02/skos/core#Concept"/>
    <skos:example>precious stone is used by lapidiaries</skos:example>
    <dct:description>material - [is] used by - [actor having] role.&#xD;
Example: precious stone is used by lapidiaries; brass (alloy) is used by braziers (metalworkers)</dct:description>
    <rdfs:subPropertyOf rdf:resource="http://www.w3.org/2004/02/skos/core#related"/>
    <owl:inverseOf rdf:resource="http://vocab.getty.edu/ontology#aat2316_use"/>
    <skos:example>brass (alloy) is used by braziers (metalworkers)</skos:example>
    <dc:identifier>2315</dc:identifier>
    <rdfs:isDefinedBy rdf:resource="http://vocab.getty.edu/ontology"/>
    <rdfs:isDefinedBy rdf:resource="http://vocab.getty.edu/aat/"/>
    <dc:title>used by - role</dc:title>
    <rdfs:domain rdf:resource="http://www.w3.org/2004/02/skos/core#Concept"/>
    <skos:prefLabel>aat2315_used_by</skos:prefLabel>
  </owl:ObjectProperty>
  <owl:ObjectProperty rdf:about="http://vocab.getty.edu/ontology#ulan1411_successor_of">
    <skos:example>Richard Meier &amp; Partners Architects LLP is the successor of Richard Meier &amp; Associates</skos:example>
    <rdfs:isDefinedBy rdf:resource="http://vocab.getty.edu/ontology"/>
    <rdfs:domain rdf:resource="http://www.w3.org/2004/02/skos/core#Concept"/>
    <owl:inverseOf rdf:resource="http://vocab.getty.edu/ontology#ulan1412_predecessor_of"/>
    <dc:title>successor of - firm/group</dc:title>
    <skos:prefLabel>ulan1411_successor_of</skos:prefLabel>
    <rdfs:range rdf:resource="http://www.w3.org/2004/02/skos/core#Concept"/>
    <rdfs:isDefinedBy rdf:resource="http://vocab.getty.edu/ulan/"/>
    <dct:description>firm/group - successor of - firm/group.&#xD;
Example: Richard Meier &amp; Partners Architects LLP is the successor of Richard Meier &amp; Associates</dct:description>
    <dc:identifier>1411</dc:identifier>
    <rdfs:subPropertyOf rdf:resource="http://www.w3.org/2004/02/skos/core#related"/>
  </owl:ObjectProperty>
  <owl:ObjectProperty rdf:about="http://vocab.getty.edu/ontology#ulan1310_advised_by">
    <rdfs:subPropertyOf rdf:resource="http://www.w3.org/2004/02/skos/core#related"/>
    <skos:example>Henry VIII, King of England was advised by Thomas Cromwell, Earl of Essex</skos:example>
    <dc:title>advised by - person</dc:title>
    <skos:prefLabel>ulan1310_advised_by</skos:prefLabel>
    <rdfs:isDefinedBy rdf:resource="http://vocab.getty.edu/ontology"/>
    <rdfs:range rdf:resource="http://www.w3.org/2004/02/skos/core#Concept"/>
    <dc:identifier>1310</dc:identifier>
    <rdfs:domain rdf:resource="http://www.w3.org/2004/02/skos/core#Concept"/>
    <dct:description>person - advised by - person.&#xD;
Example: Henry VIII, King of England was advised by Thomas Cromwell, Earl of Essex</dct:description>
    <rdfs:isDefinedBy rdf:resource="http://vocab.getty.edu/ulan/"/>
  </owl:ObjectProperty>
  <owl:ObjectProperty rdf:about="http://vocab.getty.edu/ontology#aat2206_caused_by-requires">
    <skos:example>on-demand publishing is caused by/requires on-demand printing</skos:example>
    <skos:prefLabel>aat2206_caused_by-requires</skos:prefLabel>
    <skos:example>preservation is caused by/requires preserving</skos:example>
    <dc:title>caused by/requires - activity/event</dc:title>
    <rdfs:range rdf:resource="http://www.w3.org/2004/02/skos/core#Concept"/>
    <dct:description>activity/event/[process/function] - [is] caused by/dependent upon - activity/event/[process/function].&#xD;
Example: on-demand publishing is caused by/requires on-demand printing; preservation is caused by/requires preserving</dct:description>
    <rdfs:isDefinedBy rdf:resource="http://vocab.getty.edu/aat/"/>
    <rdfs:domain rdf:resource="http://www.w3.org/2004/02/skos/core#Concept"/>
    <dc:identifier>2206</dc:identifier>
    <rdfs:isDefinedBy rdf:resource="http://vocab.getty.edu/ontology"/>
    <rdfs:subPropertyOf rdf:resource="http://www.w3.org/2004/02/skos/core#related"/>
  </owl:ObjectProperty>
  <owl:ObjectProperty rdf:about="http://vocab.getty.edu/ontology#ulan2579_trustee_was">
    <skos:example>National Galleries of Scotland trustee was George Douglas Haig</skos:example>
    <rdfs:subPropertyOf rdf:resource="http://www.w3.org/2004/02/skos/core#related"/>
    <rdfs:isDefinedBy rdf:resource="http://vocab.getty.edu/ulan/"/>
    <dc:identifier>2579</dc:identifier>
    <dct:description>institution - trustee was - person.&#xD;
Example: National Galleries of Scotland trustee was George Douglas Haig</dct:description>
    <rdfs:isDefinedBy rdf:resource="http://vocab.getty.edu/ontology"/>
    <rdfs:domain rdf:resource="http://www.w3.org/2004/02/skos/core#Concept"/>
    <dc:title>trustee was - person</dc:title>
    <skos:prefLabel>ulan2579_trustee_was</skos:prefLabel>
    <rdfs:range rdf:resource="http://www.w3.org/2004/02/skos/core#Concept"/>
  </owl:ObjectProperty>
  <owl:ObjectProperty rdf:about="http://vocab.getty.edu/ontology#aat2833_ancestor_of">
    <dc:identifier>2833</dc:identifier>
    <skos:example>Equus asinus is the ancestor of donkeys</skos:example>
    <dct:description>genus/species - is ancestor of -  another genus/species.&#xD;
Example: Canis lupus is the ancestor of Canis familiaris; Equus asinus is the ancestor of donkeys</dct:description>
    <skos:prefLabel>aat2833_ancestor_of</skos:prefLabel>
    <skos:example>Canis lupus is the ancestor of Canis familiaris</skos:example>
    <owl:inverseOf rdf:resource="http://vocab.getty.edu/ontology#aat2834_decendant_of"/>
    <dc:title>ancestor of - genus/species</dc:title>
    <rdfs:range rdf:resource="http://www.w3.org/2004/02/skos/core#Concept"/>
    <rdfs:subPropertyOf rdf:resource="http://www.w3.org/2004/02/skos/core#related"/>
    <rdfs:isDefinedBy rdf:resource="http://vocab.getty.edu/ontology"/>
    <rdfs:domain rdf:resource="http://www.w3.org/2004/02/skos/core#Concept"/>
    <rdfs:isDefinedBy rdf:resource="http://vocab.getty.edu/aat/"/>
  </owl:ObjectProperty>
  <owl:ObjectProperty rdf:about="http://vocab.getty.edu/ontology#aat2329_involves">
    <rdfs:domain rdf:resource="http://www.w3.org/2004/02/skos/core#Concept"/>
    <rdfs:range rdf:resource="http://www.w3.org/2004/02/skos/core#Concept"/>
    <dc:title>involves - role</dc:title>
    <rdfs:isDefinedBy rdf:resource="http://vocab.getty.edu/ontology"/>
    <skos:example>portraits involve sitters</skos:example>
    <rdfs:subPropertyOf rdf:resource="http://www.w3.org/2004/02/skos/core#related"/>
    <dc:identifier>2329</dc:identifier>
    <rdfs:isDefinedBy rdf:resource="http://vocab.getty.edu/aat/"/>
    <skos:prefLabel>aat2329_involves</skos:prefLabel>
    <dct:description>things - involve - [actors having] role.&#xD;
Example: portraits involve sitters; motion pictures (visual works) involve actors (performing artists)</dct:description>
    <skos:example>motion pictures (visual works) involve actors (performing artists)</skos:example>
  </owl:ObjectProperty>
  <owl:ObjectProperty rdf:about="http://vocab.getty.edu/ontology#ulan1008_meaning_-usage_overlaps_with">
    <dct:description>any - meaning /usage overlaps with - any.&#xD;
Example: The meaning or usage of unknown Zimbabwean overlaps with unknown Rodesian</dct:description>
    <dc:title>meaning /usage overlaps with - any</dc:title>
    <rdf:type rdf:resource="http://www.w3.org/2002/07/owl#SymmetricProperty"/>
    <rdfs:subPropertyOf rdf:resource="http://www.w3.org/2004/02/skos/core#related"/>
    <skos:prefLabel>ulan1008_meaning_-usage_overlaps_with</skos:prefLabel>
    <rdfs:isDefinedBy rdf:resource="http://vocab.getty.edu/ulan/"/>
    <rdfs:domain rdf:resource="http://www.w3.org/2004/02/skos/core#Concept"/>
    <dc:identifier>1008</dc:identifier>
    <skos:example>The meaning or usage of unknown Zimbabwean overlaps with unknown Rodesian</skos:example>
    <rdfs:isDefinedBy rdf:resource="http://vocab.getty.edu/ontology"/>
    <rdfs:range rdf:resource="http://www.w3.org/2004/02/skos/core#Concept"/>
  </owl:ObjectProperty>
  <owl:ObjectProperty rdf:about="http://vocab.getty.edu/ontology#broaderPreferredExtended">
    <rdfs:isDefinedBy rdf:resource="http://vocab.getty.edu/ontology"/>
    <rdfs:label>broaderPreferredExtended</rdfs:label>
    <rdfs:domain rdf:resource="http://vocab.getty.edu/ontology#Subject"/>
    <rdfs:range rdf:resource="http://vocab.getty.edu/ontology#Subject"/>
    <rdfs:comment>Preferred Ancestors. Meaningful closure of gvp:broaderPreferred. Needed to display the hierarchy</rdfs:comment>
    <skos:example>Mt Athos has preferred ancestor places (BTPE) World, Europe, Greece, Macedonia, Pangaon ros regional division;
and prefererd place type (BTIE) inhabited place</skos:example>
    <dct:description>Preferred Ancestors. Meaningful closure of gvp:broaderPreferred. Needed to display the hierarchy.
Example: Mt Athos has preferred ancestor places (BTPE) World, Europe, Greece, Macedonia, Pangaon ros regional division;
and prefererd place type (BTIE) inhabited place</dct:description>
  </owl:ObjectProperty>
  <owl:ObjectProperty rdf:about="http://vocab.getty.edu/ontology#ulan2692_president_of">
    <dct:description>person - president of - institution.&#xD;
Example: David K. E. Bruce was president of National Gallery of Art</dct:description>
    <rdfs:domain rdf:resource="http://www.w3.org/2004/02/skos/core#Concept"/>
    <rdfs:isDefinedBy rdf:resource="http://vocab.getty.edu/ontology"/>
    <rdfs:range rdf:resource="http://www.w3.org/2004/02/skos/core#Concept"/>
    <skos:example>David K. E. Bruce was president of National Gallery of Art</skos:example>
    <dc:title>president of - institution</dc:title>
    <rdfs:subPropertyOf rdf:resource="http://www.w3.org/2004/02/skos/core#related"/>
    <owl:inverseOf rdf:resource="http://vocab.getty.edu/ontology#ulan2693_president_was"/>
    <dc:identifier>2692</dc:identifier>
    <rdfs:isDefinedBy rdf:resource="http://vocab.getty.edu/ulan/"/>
    <skos:prefLabel>ulan2692_president_of</skos:prefLabel>
  </owl:ObjectProperty>
  <owl:ObjectProperty rdf:about="http://vocab.getty.edu/ontology#ulan1111_master_of">
    <rdfs:range rdf:resource="http://www.w3.org/2004/02/skos/core#Concept"/>
    <dc:identifier>1111</dc:identifier>
    <rdfs:isDefinedBy rdf:resource="http://vocab.getty.edu/ontology"/>
    <rdfs:subPropertyOf rdf:resource="http://www.w3.org/2004/02/skos/core#related"/>
    <dc:title>master of - person</dc:title>
    <rdfs:isDefinedBy rdf:resource="http://vocab.getty.edu/ulan/"/>
    <owl:inverseOf rdf:resource="http://vocab.getty.edu/ontology#ulan1112_master_was"/>
    <rdfs:domain rdf:resource="http://www.w3.org/2004/02/skos/core#Concept"/>
    <skos:prefLabel>ulan1111_master_of</skos:prefLabel>
    <skos:example>Peter Paul Rubens - master of Jan Thomas</skos:example>
    <dct:description>person - master of - person.&#xD;
Example: Peter Paul Rubens - master of Jan Thomas</dct:description>
  </owl:ObjectProperty>
  <owl:ObjectProperty rdf:about="http://vocab.getty.edu/ontology#agentType">
    <rdfs:isDefinedBy rdf:resource="http://vocab.getty.edu/ontology"/>
    <rdfs:label>agentType</rdfs:label>
    <rdfs:domain rdf:resource="http://vocab.getty.edu/ontology#Subject"/>
    <rdfs:range rdf:resource="http://vocab.getty.edu/ontology#Subject"/>
    <rdfs:comment>Type of a ULAN PersonConcept or GroupConcept. Domain is ULAN concept, range is AAT concept</rdfs:comment>
    <dct:description>Type of a ULAN PersonConcept or GroupConcept. Domain is ULAN concept, range is AAT concept</dct:description>
  </owl:ObjectProperty>
  <owl:ObjectProperty rdf:about="http://vocab.getty.edu/ontology#ulan2674_professor_at">
    <owl:inverseOf rdf:resource="http://vocab.getty.edu/ontology#ulan2675_professor_was"/>
    <rdfs:isDefinedBy rdf:resource="http://vocab.getty.edu/ontology"/>
    <dc:title>professor at - institution</dc:title>
    <rdfs:range rdf:resource="http://www.w3.org/2004/02/skos/core#Concept"/>
    <skos:example>Paul Klee was a professor at Bauhaus</skos:example>
    <rdfs:domain rdf:resource="http://www.w3.org/2004/02/skos/core#Concept"/>
    <skos:prefLabel>ulan2674_professor_at</skos:prefLabel>
    <rdfs:subPropertyOf rdf:resource="http://www.w3.org/2004/02/skos/core#related"/>
    <dct:description>person - professor at - institution.&#xD;
Example: Paul Klee was a professor at Bauhaus</dct:description>
    <dc:identifier>2674</dc:identifier>
    <rdfs:isDefinedBy rdf:resource="http://vocab.getty.edu/ulan/"/>
  </owl:ObjectProperty>
  <owl:ObjectProperty rdf:about="http://vocab.getty.edu/ontology#ulan1321_school_of">
    <rdfs:subPropertyOf rdf:resource="http://www.w3.org/2004/02/skos/core#related"/>
    <rdfs:isDefinedBy rdf:resource="http://vocab.getty.edu/ontology"/>
    <rdfs:domain rdf:resource="http://www.w3.org/2004/02/skos/core#Concept"/>
    <skos:example>The school of Pierre Saalburg was the Architectural Association. School of Architecture</skos:example>
    <skos:prefLabel>ulan1321_school_of</skos:prefLabel>
    <dct:description>person - school of - firm/group.&#xD;
Example: The school of Pierre Saalburg was the Architectural Association. School of Architecture</dct:description>
    <dc:identifier>1321</dc:identifier>
    <owl:inverseOf rdf:resource="http://vocab.getty.edu/ontology#ulan1322_school_was"/>
    <rdfs:isDefinedBy rdf:resource="http://vocab.getty.edu/ulan/"/>
    <rdfs:range rdf:resource="http://www.w3.org/2004/02/skos/core#Concept"/>
    <dc:title>school of - firm/group</dc:title>
  </owl:ObjectProperty>
  <owl:ObjectProperty rdf:about="http://vocab.getty.edu/ontology#ulan1516_great-grandchild_of">
    <rdfs:subPropertyOf rdf:resource="http://www.w3.org/2004/02/skos/core#related"/>
    <rdfs:isDefinedBy rdf:resource="http://vocab.getty.edu/ulan/"/>
    <rdfs:domain rdf:resource="http://www.w3.org/2004/02/skos/core#Concept"/>
    <skos:example>Richard Benno Adam is the great-grandchild of Albrecht Adam</skos:example>
    <dc:title>great-grandchild of - person</dc:title>
    <rdfs:range rdf:resource="http://www.w3.org/2004/02/skos/core#Concept"/>
    <rdfs:isDefinedBy rdf:resource="http://vocab.getty.edu/ontology"/>
    <dc:identifier>1516</dc:identifier>
    <skos:prefLabel>ulan1516_great-grandchild_of</skos:prefLabel>
    <dct:description>person - great-grandchild of - person.&#xD;
Example: Richard Benno Adam is the great-grandchild of Albrecht Adam</dct:description>
  </owl:ObjectProperty>
  <owl:ObjectProperty rdf:about="http://vocab.getty.edu/ontology#nationalityPreferred">
    <rdfs:isDefinedBy rdf:resource="http://vocab.getty.edu/ontology"/>
    <rdfs:label>nationalityPreferred</rdfs:label>
    <rdfs:range rdf:resource="http://vocab.getty.edu/ontology#Subject"/>
    <rdfs:subPropertyOf rdf:resource="http://schema.org/nationality"/>
    <rdfs:comment>Preferred nationality/culture/race/ethnicity/religion/sexual orientation of an ULAN agent. Domain is schema:Person/Organization, range is AAT concept</rdfs:comment>
    <dct:description>Preferred nationality/culture/race/ethnicity/religion/sexual orientation of an ULAN agent. Domain is schema:Person/Organization, range is AAT concept</dct:description>
  </owl:ObjectProperty>
  <owl:ObjectProperty rdf:about="http://vocab.getty.edu/ontology#ulan2829_student_was">
    <rdfs:range rdf:resource="http://www.w3.org/2004/02/skos/core#Concept"/>
    <rdfs:subPropertyOf rdf:resource="http://www.w3.org/2004/02/skos/core#related"/>
    <dc:title>student was - person</dc:title>
    <rdfs:domain rdf:resource="http://www.w3.org/2004/02/skos/core#Concept"/>
    <dct:description>institution - student was - person.&#xD;
Example: Bauhaus student was Zdanek Rossman</dct:description>
    <rdfs:isDefinedBy rdf:resource="http://vocab.getty.edu/ontology"/>
    <rdfs:isDefinedBy rdf:resource="http://vocab.getty.edu/ulan/"/>
    <skos:prefLabel>ulan2829_student_was</skos:prefLabel>
    <dc:identifier>2829</dc:identifier>
    <skos:example>Bauhaus student was Zdanek Rossman</skos:example>
  </owl:ObjectProperty>
  <owl:ObjectProperty rdf:about="http://vocab.getty.edu/ontology#ulan2651_publisher_of">
    <rdfs:domain rdf:resource="http://www.w3.org/2004/02/skos/core#Concept"/>
    <dc:identifier>2651</dc:identifier>
    <dc:title>publisher of - person</dc:title>
    <rdfs:isDefinedBy rdf:resource="http://vocab.getty.edu/ontology"/>
    <dct:description>firm - publisher of - person.&#xD;
Example: Negretti and Zambra was the publisher of Pierre Joseph Rossier</dct:description>
    <rdfs:isDefinedBy rdf:resource="http://vocab.getty.edu/ulan/"/>
    <rdfs:subPropertyOf rdf:resource="http://www.w3.org/2004/02/skos/core#related"/>
    <skos:example>Negretti and Zambra was the publisher of Pierre Joseph Rossier</skos:example>
    <rdfs:range rdf:resource="http://www.w3.org/2004/02/skos/core#Concept"/>
    <skos:prefLabel>ulan2651_publisher_of</skos:prefLabel>
  </owl:ObjectProperty>
  <owl:ObjectProperty rdf:about="http://vocab.getty.edu/ontology#tgn3510_historical_connection">
    <dc:title>historical connection - any</dc:title>
    <dct:description>any - historical connection - any.&#xD;
Example: Guyenne, France (historical region) has a historical connection to Gascogne (France) (historical region)</dct:description>
    <rdfs:domain rdf:resource="http://www.w3.org/2004/02/skos/core#Concept"/>
    <rdfs:range rdf:resource="http://www.w3.org/2004/02/skos/core#Concept"/>
    <rdfs:subPropertyOf rdf:resource="http://www.w3.org/2004/02/skos/core#related"/>
    <rdfs:isDefinedBy rdf:resource="http://vocab.getty.edu/ontology"/>
    <rdfs:isDefinedBy rdf:resource="http://vocab.getty.edu/tgn/"/>
    <rdf:type rdf:resource="http://www.w3.org/2002/07/owl#SymmetricProperty"/>
    <dc:identifier>3510</dc:identifier>
    <skos:prefLabel>tgn3510_historical_connection</skos:prefLabel>
    <skos:example>Guyenne, France (historical region) has a historical connection to Gascogne (France) (historical region)</skos:example>
  </owl:ObjectProperty>
  <owl:ObjectProperty rdf:about="http://vocab.getty.edu/ontology#ulan1217_employee_of">
    <dct:description>person/firm - employee of - person.&#xD;
Example: Employee of Christopher Wren was Jean Tijou</dct:description>
    <rdfs:range rdf:resource="http://www.w3.org/2004/02/skos/core#Concept"/>
    <rdfs:isDefinedBy rdf:resource="http://vocab.getty.edu/ontology"/>
    <skos:example>Employee of Christopher Wren was Jean Tijou</skos:example>
    <dc:identifier>1217</dc:identifier>
    <skos:prefLabel>ulan1217_employee_of</skos:prefLabel>
    <dc:title>employee of - person</dc:title>
    <rdfs:subPropertyOf rdf:resource="http://www.w3.org/2004/02/skos/core#related"/>
    <rdfs:domain rdf:resource="http://www.w3.org/2004/02/skos/core#Concept"/>
    <rdfs:isDefinedBy rdf:resource="http://vocab.getty.edu/ulan/"/>
    <owl:inverseOf rdf:resource="http://vocab.getty.edu/ontology#ulan1218_employee_was"/>
  </owl:ObjectProperty>
  <owl:ObjectProperty rdf:about="http://vocab.getty.edu/ontology#aat2211_produce">
    <dct:description>things/[equipment] - produce - things.&#xD;
Example: stereoscopic cameras produce stereoscopic photographs; punches (marking tools) produce punchwork</dct:description>
    <rdfs:isDefinedBy rdf:resource="http://vocab.getty.edu/ontology"/>
    <dc:identifier>2211</dc:identifier>
    <owl:inverseOf rdf:resource="http://vocab.getty.edu/ontology#aat2212_produced_by"/>
    <skos:prefLabel>aat2211_produce</skos:prefLabel>
    <rdfs:range rdf:resource="http://www.w3.org/2004/02/skos/core#Concept"/>
    <rdfs:subPropertyOf rdf:resource="http://www.w3.org/2004/02/skos/core#related"/>
    <skos:example>punches (marking tools) produce punchwork</skos:example>
    <rdfs:isDefinedBy rdf:resource="http://vocab.getty.edu/aat/"/>
    <rdfs:domain rdf:resource="http://www.w3.org/2004/02/skos/core#Concept"/>
    <dc:title>produce - things</dc:title>
    <skos:example>stereoscopic cameras produce stereoscopic photographs</skos:example>
  </owl:ObjectProperty>
  <owl:ObjectProperty rdf:about="http://vocab.getty.edu/ontology#ulan1213_court_artist_to">
    <skos:prefLabel>ulan1213_court_artist_to</skos:prefLabel>
    <owl:inverseOf rdf:resource="http://vocab.getty.edu/ontology#ulan1214_court_artist_was"/>
    <dc:title>court artist to - person</dc:title>
    <dc:identifier>1213</dc:identifier>
    <rdfs:subPropertyOf rdf:resource="http://www.w3.org/2004/02/skos/core#related"/>
    <rdfs:range rdf:resource="http://www.w3.org/2004/02/skos/core#Concept"/>
    <rdfs:domain rdf:resource="http://www.w3.org/2004/02/skos/core#Concept"/>
    <skos:example>Court artist to Gonzaga Vincenzo I, Duke of Mantua was Peter Paul Rubens</skos:example>
    <rdfs:isDefinedBy rdf:resource="http://vocab.getty.edu/ulan/"/>
    <dct:description>person - court artist to - person.&#xD;
Example: Court artist to Gonzaga Vincenzo I, Duke of Mantua was Peter Paul Rubens; court artist to Charles IV, King of Spain was Francisco de Goya</dct:description>
    <rdfs:isDefinedBy rdf:resource="http://vocab.getty.edu/ontology"/>
    <skos:example>court artist to Charles IV, King of Spain was Francisco de Goya</skos:example>
  </owl:ObjectProperty>
  <owl:ObjectProperty rdf:about="http://vocab.getty.edu/ontology#aat2318_involved_in">
    <dc:identifier>2318</dc:identifier>
    <skos:example>martyrs are involved in martyrdoms</skos:example>
    <owl:inverseOf rdf:resource="http://vocab.getty.edu/ontology#aat2319_involves"/>
    <rdfs:subPropertyOf rdf:resource="http://www.w3.org/2004/02/skos/core#related"/>
    <rdfs:domain rdf:resource="http://www.w3.org/2004/02/skos/core#Concept"/>
    <rdfs:range rdf:resource="http://www.w3.org/2004/02/skos/core#Concept"/>
    <rdfs:isDefinedBy rdf:resource="http://vocab.getty.edu/aat/"/>
    <dc:title>involved in - activity/event</dc:title>
    <skos:prefLabel>aat2318_involved_in</skos:prefLabel>
    <rdfs:isDefinedBy rdf:resource="http://vocab.getty.edu/ontology"/>
    <dct:description>[actors having] role -[are] involved - activity/event.&#xD;
Example: bridegrooms are involved in weddings; martyrs are involved in martyrdoms</dct:description>
    <skos:example>bridegrooms are involved in weddings</skos:example>
  </owl:ObjectProperty>
  <owl:ObjectProperty rdf:about="http://vocab.getty.edu/ontology#ulan1574_godparent_of">
    <dc:identifier>1574</dc:identifier>
    <rdfs:isDefinedBy rdf:resource="http://vocab.getty.edu/ontology"/>
    <rdfs:range rdf:resource="http://www.w3.org/2004/02/skos/core#Concept"/>
    <skos:example>Jean-Baptiste Goy is godparent of Jean I Nocret</skos:example>
    <owl:inverseOf rdf:resource="http://vocab.getty.edu/ontology#ulan1575_godchild_of"/>
    <dct:description>person - godparent of - person.&#xD;
Example: Jean-Baptiste Goy is godparent of Jean I Nocret</dct:description>
    <rdfs:isDefinedBy rdf:resource="http://vocab.getty.edu/ulan/"/>
    <rdfs:domain rdf:resource="http://www.w3.org/2004/02/skos/core#Concept"/>
    <skos:prefLabel>ulan1574_godparent_of</skos:prefLabel>
    <dc:title>godparent of - person</dc:title>
    <rdfs:subPropertyOf rdf:resource="http://www.w3.org/2004/02/skos/core#related"/>
  </owl:ObjectProperty>
  <owl:ObjectProperty rdf:about="http://vocab.getty.edu/ontology#broaderGenericExtended">
    <rdfs:label>broaderGenericExtended</rdfs:label>
    <rdfs:comment>Ancestors (Generic). Meaningful closure of gvp:broaderGeneric. Infers iso:broaderGeneric for pairs of directly related skos:Concepts</rdfs:comment>
    <rdfs:domain rdf:resource="http://vocab.getty.edu/ontology#Subject"/>
    <dct:description>Ancestors (Generic). Meaningful closure of gvp:broaderGeneric. Infers iso:broaderGeneric for pairs of directly related skos:Concepts.
Example: &lt;anvils and anvil accessories&gt; BTG &lt;forging and metal-shaping tools&gt; BTG &lt;forging and metal-shaping equipment&gt;,
so &lt;anvils and anvil accessories&gt; BTGE &lt;forging and metal-shaping equipment&gt;</dct:description>
    <rdfs:subPropertyOf rdf:resource="http://vocab.getty.edu/ontology#broaderExtended"/>
    <rdfs:isDefinedBy rdf:resource="http://vocab.getty.edu/ontology"/>
    <skos:example>&lt;anvils and anvil accessories&gt; BTG &lt;forging and metal-shaping tools&gt; BTG &lt;forging and metal-shaping equipment&gt;,
so &lt;anvils and anvil accessories&gt; BTGE &lt;forging and metal-shaping equipment&gt;</skos:example>
    <rdfs:range rdf:resource="http://vocab.getty.edu/ontology#Subject"/>
    <owl:propertyChainAxiom rdf:parseType="Collection">
      <owl:ObjectProperty rdf:about="http://vocab.getty.edu/ontology#broaderGenericExtended"/>
      <owl:ObjectProperty rdf:about="http://vocab.getty.edu/ontology#broaderGeneric"/>
    </owl:propertyChainAxiom>
  </owl:ObjectProperty>
  <owl:ObjectProperty rdf:about="http://vocab.getty.edu/ontology#termDisplay">
    <rdfs:isDefinedBy rdf:resource="http://vocab.getty.edu/ontology"/>
    <rdfs:label>termDisplay</rdfs:label>
    <rdfs:domain rdf:resource="http://www.w3.org/2008/05/skos-xl#Label"/>
    <rdfs:range rdf:resource="http://www.w3.org/2004/02/skos/core#Concept"/>
    <dct:description>Term Display</dct:description>
  </owl:ObjectProperty>
  <owl:ObjectProperty rdf:about="http://vocab.getty.edu/ontology#broaderGeneric">
    <rdfs:subPropertyOf rdf:resource="http://vocab.getty.edu/ontology#broader"/>
    <dct:description>BTG (Genus/Species, "is a") relation. We also infer iso-thes:broaderGeneric, which goes only between Concepts.
Example: calcite (AAT) BTG mineral (AAT)</dct:description>
    <rdfs:subPropertyOf rdf:resource="http://vocab.getty.edu/ontology#broaderGenericExtended"/>
    <rdfs:range rdf:resource="http://vocab.getty.edu/ontology#Subject"/>
    <rdfs:comment>BTG (Genus/Species, "is a") relation. We also infer iso-thes:broaderGeneric, which goes only between Concepts</rdfs:comment>
    <skos:example>calcite (AAT) BTG mineral (AAT)</skos:example>
    <rdfs:isDefinedBy rdf:resource="http://vocab.getty.edu/ontology"/>
    <rdfs:label>broaderGeneric</rdfs:label>
    <rdfs:domain rdf:resource="http://vocab.getty.edu/ontology#Subject"/>
  </owl:ObjectProperty>
  <owl:ObjectProperty rdf:about="http://vocab.getty.edu/ontology#ulan1206_client_was">
    <rdfs:domain rdf:resource="http://www.w3.org/2004/02/skos/core#Concept"/>
    <rdfs:range rdf:resource="http://www.w3.org/2004/02/skos/core#Concept"/>
    <skos:prefLabel>ulan1206_client_was</skos:prefLabel>
    <rdfs:isDefinedBy rdf:resource="http://vocab.getty.edu/ulan/"/>
    <dc:title>client was - person/firm/family</dc:title>
    <dc:identifier>1206</dc:identifier>
    <rdfs:isDefinedBy rdf:resource="http://vocab.getty.edu/ontology"/>
    <dct:description>person/firm/family - client was - person/firm/family.&#xD;
Example: Burnham and Root's client was the Chicago Herald</dct:description>
    <skos:example>Burnham and Root's client was the Chicago Herald</skos:example>
    <rdfs:subPropertyOf rdf:resource="http://www.w3.org/2004/02/skos/core#related"/>
  </owl:ObjectProperty>
  <owl:ObjectProperty rdf:about="http://vocab.getty.edu/ontology#aat2328_involved_with">
    <dc:identifier>2328</dc:identifier>
    <skos:example>actors (performing artists) are involved with motion pictures (visual works)</skos:example>
    <owl:inverseOf rdf:resource="http://vocab.getty.edu/ontology#aat2329_involves"/>
    <skos:prefLabel>aat2328_involved_with</skos:prefLabel>
    <rdfs:isDefinedBy rdf:resource="http://vocab.getty.edu/ontology"/>
    <skos:example>sitters are involved with portraits</skos:example>
    <dct:description>[actors having] role - [are] involved in- things.&#xD;
Example: sitters are involved with portraits; actors (performing artists) are involved with motion pictures (visual works)</dct:description>
    <rdfs:range rdf:resource="http://www.w3.org/2004/02/skos/core#Concept"/>
    <dc:title>involved with - things</dc:title>
    <rdfs:domain rdf:resource="http://www.w3.org/2004/02/skos/core#Concept"/>
    <rdfs:subPropertyOf rdf:resource="http://www.w3.org/2004/02/skos/core#related"/>
    <rdfs:isDefinedBy rdf:resource="http://vocab.getty.edu/aat/"/>
  </owl:ObjectProperty>
  <owl:ObjectProperty rdf:about="http://vocab.getty.edu/ontology#ulan1202_patron_was">
    <skos:prefLabel>ulan1202_patron_was</skos:prefLabel>
    <rdfs:isDefinedBy rdf:resource="http://vocab.getty.edu/ontology"/>
    <rdfs:isDefinedBy rdf:resource="http://vocab.getty.edu/ulan/"/>
    <dct:description>person/firm/family - patron was - person.&#xD;
Example: The patron of Donatello was Cosimo I, Grand-Duke of Tuscany</dct:description>
    <dc:title>patron was - person</dc:title>
    <skos:example>The patron of Donatello was Cosimo I, Grand-Duke of Tuscany</skos:example>
    <dc:identifier>1202</dc:identifier>
    <rdfs:domain rdf:resource="http://www.w3.org/2004/02/skos/core#Concept"/>
    <rdfs:range rdf:resource="http://www.w3.org/2004/02/skos/core#Concept"/>
    <rdfs:subPropertyOf rdf:resource="http://www.w3.org/2004/02/skos/core#related"/>
  </owl:ObjectProperty>
  <owl:ObjectProperty rdf:about="http://vocab.getty.edu/ontology#ulan2650_publisher_was">
    <rdfs:range rdf:resource="http://www.w3.org/2004/02/skos/core#Concept"/>
    <dc:identifier>2650</dc:identifier>
    <rdfs:isDefinedBy rdf:resource="http://vocab.getty.edu/ontology"/>
    <skos:example>The publisher for Pierre Joseph Rossier was Negretti and Zambra</skos:example>
    <rdfs:isDefinedBy rdf:resource="http://vocab.getty.edu/ulan/"/>
    <dct:description>person - publisher was - firm.&#xD;
Example: The publisher for Pierre Joseph Rossier was Negretti and Zambra</dct:description>
    <rdfs:subPropertyOf rdf:resource="http://www.w3.org/2004/02/skos/core#related"/>
    <skos:prefLabel>ulan2650_publisher_was</skos:prefLabel>
    <dc:title>publisher was - firm</dc:title>
    <owl:inverseOf rdf:resource="http://vocab.getty.edu/ontology#ulan2651_publisher_of"/>
    <rdfs:domain rdf:resource="http://www.w3.org/2004/02/skos/core#Concept"/>
  </owl:ObjectProperty>
  <owl:ObjectProperty rdf:about="http://vocab.getty.edu/ontology#aat2507_produce-process">
    <skos:prefLabel>aat2507_produce-process</skos:prefLabel>
    <rdfs:domain rdf:resource="http://www.w3.org/2004/02/skos/core#Concept"/>
    <rdfs:range rdf:resource="http://www.w3.org/2004/02/skos/core#Concept"/>
    <owl:inverseOf rdf:resource="http://vocab.getty.edu/ontology#aat2508_produced-processed_by"/>
    <rdfs:isDefinedBy rdf:resource="http://vocab.getty.edu/aat/"/>
    <dct:description>things/[equipment] - produce/process - material.&#xD;
Example: cotton (fiber) is produced/processed by cotton gins; groundwater is produced/processed by water wells</dct:description>
    <rdfs:subPropertyOf rdf:resource="http://www.w3.org/2004/02/skos/core#related"/>
    <skos:example>cotton (fiber) is produced/processed by cotton gins</skos:example>
    <skos:example>groundwater is produced/processed by water wells</skos:example>
    <dc:title>produce/process - material</dc:title>
    <dc:identifier>2507</dc:identifier>
    <rdfs:isDefinedBy rdf:resource="http://vocab.getty.edu/ontology"/>
  </owl:ObjectProperty>
  <owl:ObjectProperty rdf:about="http://vocab.getty.edu/ontology#aat2428_produces">
    <rdfs:range rdf:resource="http://www.w3.org/2004/02/skos/core#Concept"/>
    <dc:title>produces - things</dc:title>
    <rdfs:isDefinedBy rdf:resource="http://vocab.getty.edu/ontology"/>
    <rdfs:domain rdf:resource="http://www.w3.org/2004/02/skos/core#Concept"/>
    <dc:identifier>2428</dc:identifier>
    <skos:example>forging (copying) produces forgeries</skos:example>
    <dct:description>activity/event/process - produces - things.&#xD;
Example: vase painting (image making) produces vase paintings (visual works); forging (copying) produces forgeries</dct:description>
    <rdfs:subPropertyOf rdf:resource="http://www.w3.org/2004/02/skos/core#related"/>
    <rdfs:isDefinedBy rdf:resource="http://vocab.getty.edu/aat/"/>
    <skos:example>vase painting (image making) produces vase paintings (visual works)</skos:example>
    <skos:prefLabel>aat2428_produces</skos:prefLabel>
  </owl:ObjectProperty>
  <owl:ObjectProperty rdf:about="http://vocab.getty.edu/ontology#ulan1302_associate_of">
    <skos:prefLabel>ulan1302_associate_of</skos:prefLabel>
    <dc:title>associate of - person</dc:title>
    <rdfs:isDefinedBy rdf:resource="http://vocab.getty.edu/ulan/"/>
    <rdfs:subPropertyOf rdf:resource="http://www.w3.org/2004/02/skos/core#related"/>
    <dct:description>person - associate of - person.&#xD;
Example: Frank Lloyd Wright was an associate of Giannini and Hilgart</dct:description>
    <dc:identifier>1302</dc:identifier>
    <rdfs:range rdf:resource="http://www.w3.org/2004/02/skos/core#Concept"/>
    <skos:example>Frank Lloyd Wright was an associate of Giannini and Hilgart</skos:example>
    <rdfs:isDefinedBy rdf:resource="http://vocab.getty.edu/ontology"/>
    <rdf:type rdf:resource="http://www.w3.org/2002/07/owl#SymmetricProperty"/>
    <rdfs:domain rdf:resource="http://www.w3.org/2004/02/skos/core#Concept"/>
  </owl:ObjectProperty>
  <owl:ObjectProperty rdf:about="http://vocab.getty.edu/ontology#ulan1223_crowned_by">
    <rdfs:isDefinedBy rdf:resource="http://vocab.getty.edu/ontology"/>
    <dc:title>crowned by - person</dc:title>
    <skos:example>Pope Leo III crowned Emperor Charlemagne</skos:example>
    <rdfs:domain rdf:resource="http://www.w3.org/2004/02/skos/core#Concept"/>
    <skos:prefLabel>ulan1223_crowned_by</skos:prefLabel>
    <dct:description>person - crowned by - person.&#xD;
Example: Pope Leo III crowned Emperor Charlemagne</dct:description>
    <owl:inverseOf rdf:resource="http://vocab.getty.edu/ontology#ulan1224_crowned"/>
    <dc:identifier>1223</dc:identifier>
    <rdfs:range rdf:resource="http://www.w3.org/2004/02/skos/core#Concept"/>
    <rdfs:isDefinedBy rdf:resource="http://vocab.getty.edu/ulan/"/>
    <rdfs:subPropertyOf rdf:resource="http://www.w3.org/2004/02/skos/core#related"/>
  </owl:ObjectProperty>
  <owl:ObjectProperty rdf:about="http://vocab.getty.edu/ontology#nationalityNonPreferred">
    <rdfs:isDefinedBy rdf:resource="http://vocab.getty.edu/ontology"/>
    <rdfs:label>nationalityNonPreferred</rdfs:label>
    <rdfs:range rdf:resource="http://vocab.getty.edu/ontology#Subject"/>
    <rdfs:subPropertyOf rdf:resource="http://schema.org/nationality"/>
    <rdfs:comment>Non-preferred nationality/culture/race/ethnicity/religion/sexual orientation of an ULAN agent. Domain is schema:Person/Organization, range is AAT concept</rdfs:comment>
    <dct:description>Non-preferred nationality/culture/race/ethnicity/religion/sexual orientation of an ULAN agent. Domain is schema:Person/Organization, range is AAT concept</dct:description>
  </owl:ObjectProperty>
  <owl:ObjectProperty rdf:about="http://vocab.getty.edu/ontology#ulan1542_consort_of">
    <skos:prefLabel>ulan1542_consort_of</skos:prefLabel>
    <rdfs:range rdf:resource="http://www.w3.org/2004/02/skos/core#Concept"/>
    <rdfs:subPropertyOf rdf:resource="http://www.w3.org/2004/02/skos/core#related"/>
    <dc:identifier>1542</dc:identifier>
    <dct:description>person - consort of - person.&#xD;
Example: Empress Livia was the consort of Augustus, Emperor of Rome</dct:description>
    <rdfs:isDefinedBy rdf:resource="http://vocab.getty.edu/ontology"/>
    <rdfs:isDefinedBy rdf:resource="http://vocab.getty.edu/ulan/"/>
    <rdfs:domain rdf:resource="http://www.w3.org/2004/02/skos/core#Concept"/>
    <owl:inverseOf>
      <owl:ObjectProperty rdf:about="http://vocab.getty.edu/ontology#ulan1543_consort_was"/>
    </owl:inverseOf>
    <dc:title>consort of - person</dc:title>
    <skos:example>Empress Livia was the consort of Augustus, Emperor of Rome</skos:example>
  </owl:ObjectProperty>
  <owl:ObjectProperty rdf:about="http://vocab.getty.edu/ontology#aat2891_exemplified_by">
    <rdfs:range rdf:resource="http://www.w3.org/2004/02/skos/core#Concept"/>
    <dc:identifier>2891</dc:identifier>
    <rdfs:isDefinedBy rdf:resource="http://vocab.getty.edu/ontology"/>
    <skos:prefLabel>aat2891_exemplified_by</skos:prefLabel>
    <rdfs:domain rdf:resource="http://www.w3.org/2004/02/skos/core#Concept"/>
    <rdfs:subPropertyOf rdf:resource="http://www.w3.org/2004/02/skos/core#related"/>
    <dc:title>exemplified by - brand name</dc:title>
    <skos:example>photothermographic transfer prints are exemplified by Pictrography (TM) prints</skos:example>
    <owl:inverseOf rdf:resource="http://vocab.getty.edu/ontology#aat2892_example_of"/>
    <rdfs:isDefinedBy rdf:resource="http://vocab.getty.edu/aat/"/>
    <dct:description>things - [are] exemplied by - brand name.&#xD;
Example: photothermographic transfer prints are exemplified by Pictrography (TM) prints</dct:description>
  </owl:ObjectProperty>
  <owl:ObjectProperty rdf:about="http://vocab.getty.edu/ontology#ulan1543_consort_was">
    <skos:example>Augustus, Emperor of Rome's consort was Empress Livia</skos:example>
    <dc:title>consort was - person</dc:title>
    <skos:prefLabel>ulan1543_consort_was</skos:prefLabel>
    <dc:identifier>1543</dc:identifier>
    <rdfs:range rdf:resource="http://www.w3.org/2004/02/skos/core#Concept"/>
    <rdfs:subPropertyOf rdf:resource="http://www.w3.org/2004/02/skos/core#related"/>
    <rdfs:isDefinedBy rdf:resource="http://vocab.getty.edu/ontology"/>
    <dct:description>person - consort was - person.&#xD;
Example: Augustus, Emperor of Rome's consort was Empress Livia</dct:description>
    <rdfs:domain rdf:resource="http://www.w3.org/2004/02/skos/core#Concept"/>
    <rdfs:isDefinedBy rdf:resource="http://vocab.getty.edu/ulan/"/>
  </owl:ObjectProperty>
  <owl:ObjectProperty rdf:about="http://vocab.getty.edu/ontology#tgn3301_ally_of">
    <rdfs:isDefinedBy rdf:resource="http://vocab.getty.edu/ontology"/>
    <rdfs:isDefinedBy rdf:resource="http://vocab.getty.edu/tgn/"/>
    <skos:example>Siena, Arezzo, Pisa, and Pistoia were Ghibeline allies during the 13th and 14th centuries.</skos:example>
    <rdfs:domain rdf:resource="http://www.w3.org/2004/02/skos/core#Concept"/>
    <dct:description>nation - ally of - nation.&#xD;
Example: Siena, Arezzo, Pisa, and Pistoia were Ghibeline allies during the 13th and 14th centuries.</dct:description>
    <rdfs:range rdf:resource="http://www.w3.org/2004/02/skos/core#Concept"/>
    <rdfs:subPropertyOf rdf:resource="http://www.w3.org/2004/02/skos/core#related"/>
    <dc:identifier>3301</dc:identifier>
    <rdf:type rdf:resource="http://www.w3.org/2002/07/owl#SymmetricProperty"/>
    <skos:prefLabel>tgn3301_ally_of</skos:prefLabel>
    <dc:title>ally of - nation</dc:title>
  </owl:ObjectProperty>
  <owl:ObjectProperty rdf:about="http://vocab.getty.edu/ontology#aat2886_used-function_as">
    <skos:prefLabel>aat2886_used-function_as</skos:prefLabel>
    <dct:description>material - used/function as - material.&#xD;
Example: carbon disulfide - is used/functions as - solvent</dct:description>
    <skos:example>carbon disulfide - is used/functions as - solvent</skos:example>
    <rdfs:isDefinedBy rdf:resource="http://vocab.getty.edu/ontology"/>
    <dc:identifier>2886</dc:identifier>
    <rdfs:domain rdf:resource="http://www.w3.org/2004/02/skos/core#Concept"/>
    <rdfs:subPropertyOf rdf:resource="http://www.w3.org/2004/02/skos/core#related"/>
    <owl:inverseOf rdf:resource="http://vocab.getty.edu/ontology#aat2887_exemplified_by"/>
    <dc:title>used/function as - material</dc:title>
    <rdfs:range rdf:resource="http://www.w3.org/2004/02/skos/core#Concept"/>
    <rdfs:isDefinedBy rdf:resource="http://vocab.getty.edu/aat/"/>
  </owl:ObjectProperty>
  <owl:ObjectProperty rdf:about="http://vocab.getty.edu/ontology#ulan1332_worker_was">
    <skos:prefLabel>ulan1332_worker_was</skos:prefLabel>
    <dc:title>worker was - any</dc:title>
    <rdfs:isDefinedBy rdf:resource="http://vocab.getty.edu/ontology"/>
    <rdfs:subPropertyOf rdf:resource="http://www.w3.org/2004/02/skos/core#related"/>
    <dc:identifier>1332</dc:identifier>
    <rdfs:domain rdf:resource="http://www.w3.org/2004/02/skos/core#Concept"/>
    <rdfs:range rdf:resource="http://www.w3.org/2004/02/skos/core#Concept"/>
    <skos:example>Workers for the Carracci family included Scarsellino and Domenichino</skos:example>
    <dct:description>person - worker was - any.&#xD;
Example: Workers for the Carracci family included Scarsellino and Domenichino</dct:description>
    <rdfs:isDefinedBy rdf:resource="http://vocab.getty.edu/ulan/"/>
  </owl:ObjectProperty>
  <owl:ObjectProperty rdf:about="http://vocab.getty.edu/ontology#aat2817_derived-made_from">
    <rdfs:isDefinedBy rdf:resource="http://vocab.getty.edu/aat/"/>
    <rdfs:subPropertyOf rdf:resource="http://www.w3.org/2004/02/skos/core#related"/>
    <rdfs:range rdf:resource="http://www.w3.org/2004/02/skos/core#Concept"/>
    <dc:identifier>2817</dc:identifier>
    <rdfs:domain rdf:resource="http://www.w3.org/2004/02/skos/core#Concept"/>
    <owl:inverseOf rdf:resource="http://vocab.getty.edu/ontology#aat2818_source_for"/>
    <dc:title>derived/made from - material</dc:title>
    <skos:example>gypsum is derived/made from from anhydrite</skos:example>
    <skos:prefLabel>aat2817_derived-made_from</skos:prefLabel>
    <rdfs:isDefinedBy rdf:resource="http://vocab.getty.edu/ontology"/>
    <skos:example>wood board is derived/made from timber (lumber)</skos:example>
    <dct:description>material - [is] derived/made from - material.&#xD;
Example: gypsum is derived/made from from anhydrite; wood board is derived/made from timber (lumber)</dct:description>
  </owl:ObjectProperty>
  <owl:ObjectProperty rdf:about="http://vocab.getty.edu/ontology#aat2291_locus-setting_for">
    <dct:description>locus/setting - [is] locus setting for - [actor or institution having] role.&#xD;
Example: roperies are the locus/setting of rope-makers; convents (built complexes) are the locus/setting of nuns; libraries (buildings) are the locus/setting of libraries (institutions)</dct:description>
    <rdfs:isDefinedBy rdf:resource="http://vocab.getty.edu/aat/"/>
    <skos:example>roperies are the locus/setting of rope-makers</skos:example>
    <rdfs:subPropertyOf rdf:resource="http://www.w3.org/2004/02/skos/core#related"/>
    <skos:example>convents (built complexes) are the locus/setting of nuns</skos:example>
    <skos:prefLabel>aat2291_locus-setting_for</skos:prefLabel>
    <rdfs:range rdf:resource="http://www.w3.org/2004/02/skos/core#Concept"/>
    <dc:title>locus/setting for - role</dc:title>
    <rdfs:isDefinedBy rdf:resource="http://vocab.getty.edu/ontology"/>
    <skos:example>libraries (buildings) are the locus/setting of libraries (institutions)</skos:example>
    <dc:identifier>2291</dc:identifier>
    <rdfs:domain rdf:resource="http://www.w3.org/2004/02/skos/core#Concept"/>
    <owl:inverseOf rdf:resource="http://vocab.getty.edu/ontology#aat2292_work-live_in"/>
  </owl:ObjectProperty>
  <owl:ObjectProperty rdf:about="http://vocab.getty.edu/ontology#contributorAlternatePreferred">
    <rdfs:isDefinedBy rdf:resource="http://vocab.getty.edu/ontology"/>
    <rdfs:label>contributorAlternatePreferred</rdfs:label>
    <rdfs:domain rdf:resource="http://www.w3.org/2008/05/skos-xl#Label"/>
    <rdfs:range rdf:resource="http://xmlns.com/foaf/0.1/Agent"/>
    <rdfs:subPropertyOf rdf:resource="http://purl.org/dc/terms/contributor"/>
    <rdfs:comment>Contributor for which the term is Alternate Preferred. Range is foaf:Agent</rdfs:comment>
    <dct:description>Contributor for which the term is Alternate Preferred. Range is foaf:Agent</dct:description>
  </owl:ObjectProperty>
  <owl:ObjectProperty rdf:about="http://vocab.getty.edu/ontology#aat2557_reflects">
    <skos:example>classics (discipline) reflects Ancient Greek [culture]</skos:example>
    <skos:example>church history reflects Christianity</skos:example>
    <dc:title>reflects - style/period/culture</dc:title>
    <rdfs:isDefinedBy rdf:resource="http://vocab.getty.edu/aat/"/>
    <skos:example>bugatu [dance discipline] reflects Buddhism</skos:example>
    <rdfs:domain rdf:resource="http://www.w3.org/2004/02/skos/core#Concept"/>
    <rdfs:subPropertyOf rdf:resource="http://www.w3.org/2004/02/skos/core#related"/>
    <skos:prefLabel>aat2557_reflects</skos:prefLabel>
    <rdfs:range rdf:resource="http://www.w3.org/2004/02/skos/core#Concept"/>
    <dct:description>field/discipline - reflects - style/period/culture /[religion/ideology].&#xD;
Example: bugatu [dance discipline] reflects Buddhism; church history reflects Christianity; classics (discipline) reflects Ancient Greek [culture]</dct:description>
    <rdfs:isDefinedBy rdf:resource="http://vocab.getty.edu/ontology"/>
    <dc:identifier>2557</dc:identifier>
    <owl:inverseOf rdf:resource="http://vocab.getty.edu/ontology#aat2558_reflected_in"/>
  </owl:ObjectProperty>
  <owl:ObjectProperty rdf:about="http://vocab.getty.edu/ontology#ulan2584_chaired_by">
    <dc:title>chaired by - person</dc:title>
    <rdfs:range rdf:resource="http://www.w3.org/2004/02/skos/core#Concept"/>
    <rdfs:isDefinedBy rdf:resource="http://vocab.getty.edu/ulan/"/>
    <dct:description>institution - chaired by - person</dct:description>
    <dc:identifier>2584</dc:identifier>
    <rdfs:isDefinedBy rdf:resource="http://vocab.getty.edu/ontology"/>
    <skos:prefLabel>ulan2584_chaired_by</skos:prefLabel>
    <rdfs:subPropertyOf rdf:resource="http://www.w3.org/2004/02/skos/core#related"/>
    <rdfs:domain rdf:resource="http://www.w3.org/2004/02/skos/core#Concept"/>
  </owl:ObjectProperty>
  <owl:ObjectProperty rdf:about="http://vocab.getty.edu/ontology#aat2422_takes_place_in">
    <skos:example>pilgrimages take place in pilgrimage centers</skos:example>
    <rdfs:domain rdf:resource="http://www.w3.org/2004/02/skos/core#Concept"/>
    <dct:description>activity/event/[process/function] - takes place in - locus/setting.&#xD;
Example: smelting takes place in smelters (metalworking plants); pilgrimages take place in pilgrimage centers</dct:description>
    <rdfs:range rdf:resource="http://www.w3.org/2004/02/skos/core#Concept"/>
    <skos:example>smelting takes place in smelters (metalworking plants)</skos:example>
    <rdfs:subPropertyOf rdf:resource="http://www.w3.org/2004/02/skos/core#related"/>
    <rdfs:isDefinedBy rdf:resource="http://vocab.getty.edu/aat/"/>
    <rdfs:isDefinedBy rdf:resource="http://vocab.getty.edu/ontology"/>
    <dc:identifier>2422</dc:identifier>
    <dc:title>takes place in - locus/setting</dc:title>
    <skos:prefLabel>aat2422_takes_place_in</skos:prefLabel>
  </owl:ObjectProperty>
  <owl:ObjectProperty rdf:about="http://vocab.getty.edu/ontology#ulan2782_dedicated_to">
    <rdfs:isDefinedBy rdf:resource="http://vocab.getty.edu/ulan/"/>
    <rdfs:subPropertyOf rdf:resource="http://www.w3.org/2004/02/skos/core#related"/>
    <dc:title>dedicated to - person</dc:title>
    <rdfs:isDefinedBy rdf:resource="http://vocab.getty.edu/ontology"/>
    <rdfs:domain rdf:resource="http://www.w3.org/2004/02/skos/core#Concept"/>
    <dc:identifier>2782</dc:identifier>
    <dct:description>institution - dedicated to - person.&#xD;
Example: The Rodin Museum in Philadelphia is didicated to Auguste Rodin</dct:description>
    <rdfs:range rdf:resource="http://www.w3.org/2004/02/skos/core#Concept"/>
    <skos:prefLabel>ulan2782_dedicated_to</skos:prefLabel>
    <skos:example>The Rodin Museum in Philadelphia is didicated to Auguste Rodin</skos:example>
  </owl:ObjectProperty>
  <owl:ObjectProperty rdf:about="http://vocab.getty.edu/ontology#ulan2676_teacher_at">
    <owl:inverseOf rdf:resource="http://vocab.getty.edu/ontology#ulan2677_teacher_was"/>
    <rdfs:domain rdf:resource="http://www.w3.org/2004/02/skos/core#Concept"/>
    <dc:identifier>2676</dc:identifier>
    <rdfs:range rdf:resource="http://www.w3.org/2004/02/skos/core#Concept"/>
    <rdfs:subPropertyOf rdf:resource="http://www.w3.org/2004/02/skos/core#related"/>
    <dc:title>teacher at - institution</dc:title>
    <rdfs:isDefinedBy rdf:resource="http://vocab.getty.edu/ontology"/>
    <skos:example>Willem De Kooning was a teacher at Black Mountain College</skos:example>
    <skos:prefLabel>ulan2676_teacher_at</skos:prefLabel>
    <rdfs:isDefinedBy rdf:resource="http://vocab.getty.edu/ulan/"/>
    <dct:description>person - teacher at - institution.&#xD;
Example: Willem De Kooning was a teacher at Black Mountain College</dct:description>
  </owl:ObjectProperty>
  <owl:ObjectProperty rdf:about="http://vocab.getty.edu/ontology#ulan1512_parent_of">
    <rdfs:subPropertyOf rdf:resource="http://www.w3.org/2004/02/skos/core#related"/>
    <skos:example>Rembrandt van Rijn is the parent of Rumbertus van Rijn</skos:example>
    <skos:prefLabel>ulan1512_parent_of</skos:prefLabel>
    <rdfs:domain rdf:resource="http://www.w3.org/2004/02/skos/core#Concept"/>
    <rdfs:isDefinedBy rdf:resource="http://vocab.getty.edu/ulan/"/>
    <dc:identifier>1512</dc:identifier>
    <dct:description>person - parent of - person.&#xD;
Example: Rembrandt van Rijn is the parent of Rumbertus van Rijn</dct:description>
    <rdfs:isDefinedBy rdf:resource="http://vocab.getty.edu/ontology"/>
    <dc:title>parent of - person</dc:title>
    <rdfs:range rdf:resource="http://www.w3.org/2004/02/skos/core#Concept"/>
  </owl:ObjectProperty>
  <owl:ObjectProperty rdf:about="http://vocab.getty.edu/ontology#ulan1590_possibly_related_to">
    <dct:description>person - possibly related to (familial relationship) - person.&#xD;
Example: A familial relationship between Ramon Destorrents, the younger and Ramon Destorrents, the elder is possible</dct:description>
    <rdfs:range rdf:resource="http://www.w3.org/2004/02/skos/core#Concept"/>
    <dc:title>possibly related to - person</dc:title>
    <dc:identifier>1590</dc:identifier>
    <skos:prefLabel>ulan1590_possibly_related_to</skos:prefLabel>
    <rdfs:domain rdf:resource="http://www.w3.org/2004/02/skos/core#Concept"/>
    <rdfs:isDefinedBy rdf:resource="http://vocab.getty.edu/ulan/"/>
    <rdfs:subPropertyOf rdf:resource="http://www.w3.org/2004/02/skos/core#related"/>
    <rdfs:isDefinedBy rdf:resource="http://vocab.getty.edu/ontology"/>
    <rdf:type rdf:resource="http://www.w3.org/2002/07/owl#SymmetricProperty"/>
    <skos:example>A familial relationship between Ramon Destorrents, the younger and Ramon Destorrents, the elder is possible</skos:example>
  </owl:ObjectProperty>
  <owl:ObjectProperty rdf:about="http://vocab.getty.edu/ontology#aat2895_example_of">
    <skos:example>Papersave Process (TM) is example of deacidification [process/function]</skos:example>
    <dc:title>example of - activity/event</dc:title>
    <rdfs:domain rdf:resource="http://www.w3.org/2004/02/skos/core#Concept"/>
    <rdfs:isDefinedBy rdf:resource="http://vocab.getty.edu/ontology"/>
    <skos:prefLabel>aat2895_example_of</skos:prefLabel>
    <dc:identifier>2895</dc:identifier>
    <dct:description>brand name - [is] example of - activity/event/[process/function].&#xD;
Example: Papersave Process (TM) is example of deacidification [process/function]</dct:description>
    <rdfs:subPropertyOf rdf:resource="http://www.w3.org/2004/02/skos/core#related"/>
    <rdfs:isDefinedBy rdf:resource="http://vocab.getty.edu/aat/"/>
    <rdfs:range rdf:resource="http://www.w3.org/2004/02/skos/core#Concept"/>
  </owl:ObjectProperty>
  <owl:ObjectProperty rdf:about="http://vocab.getty.edu/ontology#ulan2578_trustee_of">
    <skos:example>George Douglas Haig was a trustee of the National Galleries of Scotland</skos:example>
    <skos:prefLabel>ulan2578_trustee_of</skos:prefLabel>
    <owl:inverseOf rdf:resource="http://vocab.getty.edu/ontology#ulan2579_trustee_was"/>
    <rdfs:subPropertyOf rdf:resource="http://www.w3.org/2004/02/skos/core#related"/>
    <rdfs:isDefinedBy rdf:resource="http://vocab.getty.edu/ontology"/>
    <dc:title>trustee of - institution</dc:title>
    <dc:identifier>2578</dc:identifier>
    <rdfs:isDefinedBy rdf:resource="http://vocab.getty.edu/ulan/"/>
    <rdfs:domain rdf:resource="http://www.w3.org/2004/02/skos/core#Concept"/>
    <rdfs:range rdf:resource="http://www.w3.org/2004/02/skos/core#Concept"/>
    <dct:description>person - trustee of - institution.&#xD;
Example: George Douglas Haig was a trustee of the National Galleries of Scotland</dct:description>
  </owl:ObjectProperty>
  <owl:ObjectProperty rdf:about="http://vocab.getty.edu/ontology#aat2286_practice-study">
    <skos:example>Egyptologists practice/study Egyptology</skos:example>
    <dc:identifier>2286</dc:identifier>
    <dct:description>[actor having] role - practice/study - field [of study, genre]/discipline.&#xD;
Example: Egyptologists practice/study Egyptology; architectural historians practice/study architectural history</dct:description>
    <rdfs:subPropertyOf rdf:resource="http://www.w3.org/2004/02/skos/core#related"/>
    <rdfs:isDefinedBy rdf:resource="http://vocab.getty.edu/ontology"/>
    <skos:prefLabel>aat2286_practice-study</skos:prefLabel>
    <skos:example>architectural historians practice/study architectural history</skos:example>
    <rdfs:domain rdf:resource="http://www.w3.org/2004/02/skos/core#Concept"/>
    <rdfs:range rdf:resource="http://www.w3.org/2004/02/skos/core#Concept"/>
    <rdfs:isDefinedBy rdf:resource="http://vocab.getty.edu/aat/"/>
    <dc:title>practice/study - field/discipline</dc:title>
  </owl:ObjectProperty>
  <owl:ObjectProperty rdf:about="http://vocab.getty.edu/ontology#ulan1307_assistant_of">
    <rdfs:isDefinedBy rdf:resource="http://vocab.getty.edu/ontology"/>
    <rdfs:range rdf:resource="http://www.w3.org/2004/02/skos/core#Concept"/>
    <owl:inverseOf rdf:resource="http://vocab.getty.edu/ontology#ulan1308_assisted_by"/>
    <rdfs:isDefinedBy rdf:resource="http://vocab.getty.edu/ulan/"/>
    <rdfs:subPropertyOf rdf:resource="http://www.w3.org/2004/02/skos/core#related"/>
    <skos:example>Bernard Castelli was assistant of Pablo Picasso</skos:example>
    <skos:prefLabel>ulan1307_assistant_of</skos:prefLabel>
    <rdfs:domain rdf:resource="http://www.w3.org/2004/02/skos/core#Concept"/>
    <dc:title>assistant of - person</dc:title>
    <dc:identifier>1307</dc:identifier>
    <dct:description>person - assistant of - person.&#xD;
Example: Bernard Castelli was assistant of Pablo Picasso</dct:description>
  </owl:ObjectProperty>
  <owl:ObjectProperty rdf:about="http://vocab.getty.edu/ontology#ulan2828_student_at">
    <skos:example>Zdanek Rossman was a student at Bauhaus</skos:example>
    <dc:title>student at - institution</dc:title>
    <dct:description>person - student at - institution.&#xD;
Example: Zdanek Rossman was a student at Bauhaus</dct:description>
    <owl:inverseOf rdf:resource="http://vocab.getty.edu/ontology#ulan2829_student_was"/>
    <rdfs:domain rdf:resource="http://www.w3.org/2004/02/skos/core#Concept"/>
    <rdfs:isDefinedBy rdf:resource="http://vocab.getty.edu/ulan/"/>
    <dc:identifier>2828</dc:identifier>
    <rdfs:isDefinedBy rdf:resource="http://vocab.getty.edu/ontology"/>
    <rdfs:subPropertyOf rdf:resource="http://www.w3.org/2004/02/skos/core#related"/>
    <rdfs:range rdf:resource="http://www.w3.org/2004/02/skos/core#Concept"/>
    <skos:prefLabel>ulan2828_student_at</skos:prefLabel>
  </owl:ObjectProperty>
  <owl:ObjectProperty rdf:about="http://vocab.getty.edu/ontology#ulan2841_performer_was">
    <rdfs:domain rdf:resource="http://www.w3.org/2004/02/skos/core#Concept"/>
    <dct:description>group - performer was - person</dct:description>
    <rdfs:range rdf:resource="http://www.w3.org/2004/02/skos/core#Concept"/>
    <rdfs:subPropertyOf rdf:resource="http://www.w3.org/2004/02/skos/core#related"/>
    <rdfs:isDefinedBy rdf:resource="http://vocab.getty.edu/ontology"/>
    <rdfs:isDefinedBy rdf:resource="http://vocab.getty.edu/ulan/"/>
    <dc:title>performer was - person</dc:title>
    <dc:identifier>2841</dc:identifier>
    <skos:prefLabel>ulan2841_performer_was</skos:prefLabel>
  </owl:ObjectProperty>
  <owl:ObjectProperty rdf:about="http://vocab.getty.edu/ontology#aat2875_characteristic_of">
    <dct:description>language - [is] characteristic of - style/period/culture.&#xD;
Example: Afar (language) is characteristic of Afar (culture); Celtic (language) was characteristic of Celtic (culture)</dct:description>
    <dc:title>characteristic of - style/period/culture</dc:title>
    <skos:prefLabel>aat2875_characteristic_of</skos:prefLabel>
    <rdfs:domain rdf:resource="http://www.w3.org/2004/02/skos/core#Concept"/>
    <rdfs:range rdf:resource="http://www.w3.org/2004/02/skos/core#Concept"/>
    <owl:inverseOf rdf:resource="http://vocab.getty.edu/ontology#aat2876_characterized_by"/>
    <rdfs:isDefinedBy rdf:resource="http://vocab.getty.edu/aat/"/>
    <skos:example>Celtic (language) was characteristic of Celtic (culture)</skos:example>
    <rdfs:isDefinedBy rdf:resource="http://vocab.getty.edu/ontology"/>
    <skos:example>Afar (language) is characteristic of Afar (culture)</skos:example>
    <rdfs:subPropertyOf rdf:resource="http://www.w3.org/2004/02/skos/core#related"/>
    <dc:identifier>2875</dc:identifier>
  </owl:ObjectProperty>
  <owl:ObjectProperty rdf:about="http://vocab.getty.edu/ontology#aat2814_constituent_of">
    <rdfs:isDefinedBy rdf:resource="http://vocab.getty.edu/ontology"/>
    <rdfs:subPropertyOf rdf:resource="http://www.w3.org/2004/02/skos/core#related"/>
    <rdfs:isDefinedBy rdf:resource="http://vocab.getty.edu/aat/"/>
    <dc:identifier>2814</dc:identifier>
    <rdfs:domain rdf:resource="http://www.w3.org/2004/02/skos/core#Concept"/>
    <skos:example>iron oxide is a constituent of desert varnish</skos:example>
    <owl:inverseOf rdf:resource="http://vocab.getty.edu/ontology#aat2815_composed_of"/>
    <dct:description>material - [is] constituent of - material.&#xD;
Example: titanium white is a constituent of composite white; iron oxide is a constituent of desert varnish</dct:description>
    <dc:title>constituent of - material</dc:title>
    <skos:prefLabel>aat2814_constituent_of</skos:prefLabel>
    <skos:example>titanium white is a constituent of composite white</skos:example>
    <rdfs:range rdf:resource="http://www.w3.org/2004/02/skos/core#Concept"/>
  </owl:ObjectProperty>
  <owl:ObjectProperty rdf:about="http://vocab.getty.edu/ontology#aat2607_caused_by-requires">
    <skos:prefLabel>aat2607_caused_by-requires</skos:prefLabel>
    <rdfs:range rdf:resource="http://www.w3.org/2004/02/skos/core#Concept"/>
    <dc:identifier>2607</dc:identifier>
    <dct:description>attributes /associated concepts - [is] caused by/requires - an activity/event/[process/function].&#xD;
Example: watertightness is caused by/requires waterproofing; creases (condition) is caused by/requires creasing (process)</dct:description>
    <skos:example>creases (condition) is caused by/requires creasing (process)</skos:example>
    <skos:example>watertightness is caused by/requires waterproofing</skos:example>
    <rdfs:isDefinedBy rdf:resource="http://vocab.getty.edu/aat/"/>
    <rdfs:subPropertyOf rdf:resource="http://www.w3.org/2004/02/skos/core#related"/>
    <rdfs:isDefinedBy rdf:resource="http://vocab.getty.edu/ontology"/>
    <rdfs:domain rdf:resource="http://www.w3.org/2004/02/skos/core#Concept"/>
    <owl:inverseOf rdf:resource="http://vocab.getty.edu/ontology#aat2608_causes-required_for"/>
    <dc:title>caused by/requires - activity/event</dc:title>
  </owl:ObjectProperty>
  <owl:ObjectProperty rdf:about="http://vocab.getty.edu/ontology#aat2613_possess-exist_in">
    <dct:description>material - possesses/exists in - condition/state/[property].&#xD;
Example: wood(plant material) possesses/exists in [condition of] dry rot; dielectric (material) possesses/exists in dielectric properties</dct:description>
    <rdfs:subPropertyOf rdf:resource="http://www.w3.org/2004/02/skos/core#related"/>
    <dc:identifier>2613</dc:identifier>
    <dc:title>possess/exist in - attributes /associated concepts</dc:title>
    <rdfs:range rdf:resource="http://www.w3.org/2004/02/skos/core#Concept"/>
    <skos:example>wood(plant material) possesses/exists in [condition of] dry rot</skos:example>
    <skos:example>dielectric (material) possesses/exists in dielectric properties</skos:example>
    <rdfs:domain rdf:resource="http://www.w3.org/2004/02/skos/core#Concept"/>
    <rdfs:isDefinedBy rdf:resource="http://vocab.getty.edu/aat/"/>
    <rdfs:isDefinedBy rdf:resource="http://vocab.getty.edu/ontology"/>
    <skos:prefLabel>aat2613_possess-exist_in</skos:prefLabel>
  </owl:ObjectProperty>
  <owl:ObjectProperty rdf:about="http://vocab.getty.edu/ontology#aat2882_reflect">
    <skos:prefLabel>aat2882_reflect</skos:prefLabel>
    <dc:identifier>2882</dc:identifier>
    <dct:description>things - reflect - language.&#xD;
Example: Greek alphabet reflects Greek (language); Vedas reflect Sanskrit</dct:description>
    <rdfs:domain rdf:resource="http://www.w3.org/2004/02/skos/core#Concept"/>
    <dc:title>reflect - language</dc:title>
    <rdfs:isDefinedBy rdf:resource="http://vocab.getty.edu/ontology"/>
    <rdfs:subPropertyOf rdf:resource="http://www.w3.org/2004/02/skos/core#related"/>
    <skos:example>Vedas reflect Sanskrit</skos:example>
    <rdfs:isDefinedBy rdf:resource="http://vocab.getty.edu/aat/"/>
    <rdfs:range rdf:resource="http://www.w3.org/2004/02/skos/core#Concept"/>
    <skos:example>Greek alphabet reflects Greek (language)</skos:example>
  </owl:ObjectProperty>
  <owl:DatatypeProperty rdf:about="http://vocab.getty.edu/ontology#qualifier">
    <rdfs:isDefinedBy rdf:resource="http://vocab.getty.edu/ontology"/>
    <rdfs:domain rdf:resource="http://www.w3.org/2008/05/skos-xl#Label"/>
    <rdfs:range rdf:resource="http://www.w3.org/1999/02/22-rdf-syntax-ns#Literal"/>
    <rdfs:label>qualifier</rdfs:label>
    <rdfs:comment>Clarifies and disambiguates terms with the same spelling but different meaning.
Appended in parentheses to gvp:term, forming skosxsl:literalForm.
Every qualifier is in the same language as the term</rdfs:comment>
    <skos:example>Rhea (vessels)=rhyta (a kind of drinking vessel) vs rhea (species)=Boehmeria nivea (Chinese grass)</skos:example>
    <dct:description>Clarifies and disambiguates terms with the same spelling but different meaning.
Appended in parentheses to gvp:term, forming skosxsl:literalForm.
Every qualifier is in the same language as the term.
Example: "Rhea (vessels)"=rhyta (a kind of drinking vessel) vs "Rhea (species)"=Boehmeria nivea (Chinese grass)</dct:description>
  </owl:DatatypeProperty>
  <owl:DatatypeProperty rdf:about="http://vocab.getty.edu/ontology#term">
    <rdfs:isDefinedBy rdf:resource="http://vocab.getty.edu/ontology"/>
    <rdfs:domain rdf:resource="http://www.w3.org/2008/05/skos-xl#Label"/>
    <rdfs:range rdf:resource="http://www.w3.org/1999/02/22-rdf-syntax-ns#Literal"/>
    <rdfs:label>term</rdfs:label>
    <rdfs:comment>Term (label), used as the basic (prefix) part of skosxsl:literalForm</rdfs:comment>
    <dct:description>Term (label), used as the basic (prefix) part of skosxsl:literalForm</dct:description>
  </owl:DatatypeProperty>
  <owl:DatatypeProperty rdf:about="http://vocab.getty.edu/ontology#estStart">
    <rdfs:isDefinedBy rdf:resource="http://vocab.getty.edu/ontology"/>
    <rdfs:label>estStart</rdfs:label>
    <rdfs:comment>Estimated start date of term, relation, type assignment, event, biography</rdfs:comment>
    <dct:description>Estimated start date of term, relation, type assignment, event, biography</dct:description>
  </owl:DatatypeProperty>
  <owl:DatatypeProperty rdf:about="http://vocab.getty.edu/ontology#estEnd">
    <rdfs:isDefinedBy rdf:resource="http://vocab.getty.edu/ontology"/>
    <rdfs:label>estEnd</rdfs:label>
    <rdfs:comment>Estimated end date of term, relation, type assignment, event, biography</rdfs:comment>
    <dct:description>Estimated end date of term, relation, type assignment, event, biography</dct:description>
  </owl:DatatypeProperty>
  <owl:DatatypeProperty rdf:about="http://vocab.getty.edu/ontology#parentString">
    <rdfs:isDefinedBy rdf:resource="http://vocab.getty.edu/ontology"/>
    <rdfs:label>parentString</rdfs:label>
    <rdfs:domain rdf:resource="http://vocab.getty.edu/ontology#Subject"/>
    <rdfs:range rdf:resource="http://www.w3.org/1999/02/22-rdf-syntax-ns#Literal"/>
    <rdfs:comment>Preferred labels of *all* of the subject's preferred ancestors, listed bottom up. Useful to show the subject's full context</rdfs:comment>
    <skos:note>Display version of gvp:broaderPreferredExtended</skos:note>
    <skos:example>For aat:300226882 baking dishes: bakeware, &lt;vessels for cooking food&gt;, &lt;containers for cooking food&gt;, &lt;culinary containers&gt;, &lt;containers by function or context&gt;, containers (receptacles), Containers (Hierarchy Name), Furnishings and Equipment (Hierarchy Name), Objects Facet</skos:example>
    <dct:description>Preferred labels of *all* of the subject's preferred ancestors, listed bottom up. Useful to show the subject's full context.
Display version of gvp:broaderPreferredExtended.
For aat:300226882 baking dishes: bakeware, &lt;vessels for cooking food&gt;, &lt;containers for cooking food&gt;, &lt;culinary containers&gt;, &lt;containers by function or context&gt;, containers (receptacles), Containers (Hierarchy Name), Furnishings and Equipment (Hierarchy Name), Objects Facet</dct:description>
  </owl:DatatypeProperty>
  <owl:DatatypeProperty rdf:about="http://vocab.getty.edu/ontology#parentStringAbbrev">
    <rdfs:isDefinedBy rdf:resource="http://vocab.getty.edu/ontology"/>
    <rdfs:label>parentStringAbbrev</rdfs:label>
    <rdfs:domain rdf:resource="http://vocab.getty.edu/ontology#Subject"/>
    <rdfs:range rdf:resource="http://www.w3.org/1999/02/22-rdf-syntax-ns#Literal"/>
    <rdfs:comment>Preferred labels of *some* of the subject's preferred ancestors, listed bottom up. Useful to show the subject's context</rdfs:comment>
    <skos:note>Shortened display version of gvp:broaderPreferredExtended</skos:note>
    <skos:example>For aat:300226882 baking dishes: bakeware, &lt;vessels for cooking food&gt;, ... Furnishings and Equipment (Hierarchy Name)</skos:example>
    <dct:description>Preferred labels of *some* of the subject's preferred ancestors, listed bottom up. Useful to show the subject's context.
Shortened display version of gvp:broaderPreferredExtended.
Example for aat:300226882 baking dishes: bakeware, &lt;vessels for cooking food&gt;, ... Furnishings and Equipment (Hierarchy Name)</dct:description>
  </owl:DatatypeProperty>
  <owl:DatatypeProperty rdf:about="http://vocab.getty.edu/ontology#isNoted">
    <rdfs:isDefinedBy rdf:resource="http://vocab.getty.edu/ontology"/>
    <rdfs:label>isNoted</rdfs:label>
    <rdfs:domain rdf:resource="http://vocab.getty.edu/ontology#Subject"/>
    <rdfs:range rdf:resource="http://www.w3.org/2001/XMLSchema#boolean"/>
    <rdfs:comment>One amongst several homographic concepts may be especially noted so it's easier to find</rdfs:comment>
    <skos:example>tgn:7008038 Paris, France is noted but tgn:2106600 Paris, Texas is not (except if you're Fassbinder)</skos:example>
    <dct:description>One amongst several homographic concepts may be especially noted so it's easier to find.
Example: tgn:7008038 Paris, France is noted but tgn:2106600 Paris, Texas is not (except if you're Fassbinder)</dct:description>
  </owl:DatatypeProperty>
  <owl:DatatypeProperty rdf:about="http://vocab.getty.edu/ontology#displayOrder">
    <rdfs:isDefinedBy rdf:resource="http://vocab.getty.edu/ontology"/>
    <rdfs:label>displayOrder</rdfs:label>
    <rdfs:range rdf:resource="http://www.w3.org/2001/XMLSchema#positiveInteger"/>
    <rdfs:comment>Display order of subject or term amongst its siblings.
If all are 1 then use alphabetical. Domain is gvp:Subject or skosxl:Label</rdfs:comment>
    <dct:description>Display order of subject or term amongst its siblings.
If all are 1 then use alphabetical. Domain is gvp:Subject or skosxl:Label</dct:description>
  </owl:DatatypeProperty>
  <owl:SymmetricProperty rdf:about="http://vocab.getty.edu/ontology#tgn3110_meaning-usage_overlaps_with">
    <dc:identifier>3110</dc:identifier>
    <skos:example>Judaea (Israel) (historical region) meaning/usage overlaps with Holy Land (Asia) (historical region)</skos:example>
    <dc:title>meaning/usage overlaps with - any</dc:title>
    <rdfs:domain rdf:resource="http://www.w3.org/2004/02/skos/core#Concept"/>
    <rdfs:isDefinedBy rdf:resource="http://vocab.getty.edu/tgn/"/>
    <rdfs:range rdf:resource="http://www.w3.org/2004/02/skos/core#Concept"/>
    <rdfs:subPropertyOf rdf:resource="http://www.w3.org/2004/02/skos/core#related"/>
    <rdfs:isDefinedBy rdf:resource="http://vocab.getty.edu/ontology"/>
    <dct:description>any - meaning/usage overlaps with - any.&#xD;
Example: Judaea (Israel) (historical region) meaning/usage overlaps with Holy Land (Asia) (historical region)</dct:description>
    <skos:prefLabel>tgn3110_meaning-usage_overlaps_with</skos:prefLabel>
    <rdf:type rdf:resource="http://www.w3.org/2002/07/owl#ObjectProperty"/>
  </owl:SymmetricProperty>
  <owl:SymmetricProperty rdf:about="http://vocab.getty.edu/ontology#aat2807_derived_from_common_source">
    <skos:example>mustard(material) is derived from common source with mustard oil</skos:example>
    <dct:description>material - [is] derived from common source [as] - material.&#xD;
Example: malachite (mineral) is derived from common source with azurite (mineral); mustard(material) is derived from common source with mustard oil</dct:description>
    <skos:example>malachite (mineral) is derived from common source with azurite (mineral)</skos:example>
    <rdfs:isDefinedBy rdf:resource="http://vocab.getty.edu/ontology"/>
    <rdf:type rdf:resource="http://www.w3.org/2002/07/owl#ObjectProperty"/>
    <dc:title>derived from common source - material</dc:title>
    <rdfs:domain rdf:resource="http://www.w3.org/2004/02/skos/core#Concept"/>
    <rdfs:isDefinedBy rdf:resource="http://vocab.getty.edu/aat/"/>
    <skos:prefLabel>aat2807_derived_from_common_source</skos:prefLabel>
    <dc:identifier>2807</dc:identifier>
    <rdfs:range rdf:resource="http://www.w3.org/2004/02/skos/core#Concept"/>
    <rdfs:subPropertyOf rdf:resource="http://www.w3.org/2004/02/skos/core#related"/>
  </owl:SymmetricProperty>
  <owl:SymmetricProperty rdf:about="http://vocab.getty.edu/ontology#ulan1548_domestic_partner_of">
    <rdfs:isDefinedBy rdf:resource="http://vocab.getty.edu/ulan/"/>
    <rdfs:subPropertyOf rdf:resource="http://www.w3.org/2004/02/skos/core#related"/>
    <rdfs:range rdf:resource="http://www.w3.org/2004/02/skos/core#Concept"/>
    <dc:identifier>1548</dc:identifier>
    <rdfs:domain rdf:resource="http://www.w3.org/2004/02/skos/core#Concept"/>
    <dct:description>person - domestic partner of - person</dct:description>
    <rdfs:isDefinedBy rdf:resource="http://vocab.getty.edu/ontology"/>
    <skos:prefLabel>ulan1548_domestic_partner_of</skos:prefLabel>
    <dc:title>domestic partner of - person</dc:title>
    <rdf:type rdf:resource="http://www.w3.org/2002/07/owl#ObjectProperty"/>
  </owl:SymmetricProperty>
  <owl:SymmetricProperty rdf:about="http://vocab.getty.edu/ontology#aat2100_distinguished_from">
    <rdfs:isDefinedBy rdf:resource="http://vocab.getty.edu/aat/"/>
    <skos:example>historic farms are distinguished from abandoned farms</skos:example>
    <dc:identifier>2100</dc:identifier>
    <rdfs:subPropertyOf rdf:resource="http://www.w3.org/2004/02/skos/core#related"/>
    <rdfs:domain rdf:resource="http://www.w3.org/2004/02/skos/core#Concept"/>
    <dct:description>any - distinguished from - any.&#xD;
Example: historic farms are distinguished from abandoned farms; naive art is distinguished from outsider art</dct:description>
    <rdf:type rdf:resource="http://www.w3.org/2002/07/owl#ObjectProperty"/>
    <rdfs:isDefinedBy rdf:resource="http://vocab.getty.edu/ontology"/>
    <dc:title>distinguished from - any</dc:title>
    <skos:example>naive art is distinguished from outsider art</skos:example>
    <skos:prefLabel>aat2100_distinguished_from</skos:prefLabel>
    <rdfs:range rdf:resource="http://www.w3.org/2004/02/skos/core#Concept"/>
  </owl:SymmetricProperty>
  <owl:SymmetricProperty rdf:about="http://vocab.getty.edu/ontology#ulan1500_related_to">
    <skos:example>Titian and Tizianello have a familial relationship with each other</skos:example>
    <dct:description>person - related to (familial relationship) - person.&#xD;
Example: Titian and Tizianello have a familial relationship with each other</dct:description>
    <dc:title>related to - person</dc:title>
    <rdfs:isDefinedBy rdf:resource="http://vocab.getty.edu/ontology"/>
    <skos:prefLabel>ulan1500_related_to</skos:prefLabel>
    <rdfs:isDefinedBy rdf:resource="http://vocab.getty.edu/ulan/"/>
    <rdfs:subPropertyOf rdf:resource="http://www.w3.org/2004/02/skos/core#related"/>
    <rdfs:range rdf:resource="http://www.w3.org/2004/02/skos/core#Concept"/>
    <dc:identifier>1500</dc:identifier>
    <rdf:type rdf:resource="http://www.w3.org/2002/07/owl#ObjectProperty"/>
    <rdfs:domain rdf:resource="http://www.w3.org/2004/02/skos/core#Concept"/>
  </owl:SymmetricProperty>
  <owl:SymmetricProperty rdf:about="http://vocab.getty.edu/ontology#tgn3006_formerly_identified_as">
    <rdfs:isDefinedBy rdf:resource="http://vocab.getty.edu/tgn/"/>
    <dct:description>place - formerly identified as - place; New.&#xD;
Example: The deserted settlement of Machupicchu was formerly identified as Tampu Tocco</dct:description>
    <skos:example>The deserted settlement of Machupicchu was formerly identified as Tampu Tocco</skos:example>
    <rdfs:domain rdf:resource="http://www.w3.org/2004/02/skos/core#Concept"/>
    <rdf:type rdf:resource="http://www.w3.org/2002/07/owl#ObjectProperty"/>
    <rdfs:isDefinedBy rdf:resource="http://vocab.getty.edu/ontology"/>
    <skos:scopeNote>New</skos:scopeNote>
    <dc:identifier>3006</dc:identifier>
    <skos:prefLabel>tgn3006_formerly_identified_as</skos:prefLabel>
    <rdfs:range rdf:resource="http://www.w3.org/2004/02/skos/core#Concept"/>
    <rdfs:subPropertyOf rdf:resource="http://www.w3.org/2004/02/skos/core#related"/>
    <dc:title>formerly identified as - place</dc:title>
  </owl:SymmetricProperty>
  <owl:SymmetricProperty rdf:about="http://vocab.getty.edu/ontology#ulan1000_related_to">
    <skos:example>Herman Miller, Inc. is related to Irving Harper</skos:example>
    <rdfs:isDefinedBy rdf:resource="http://vocab.getty.edu/ontology"/>
    <rdfs:isDefinedBy rdf:resource="http://vocab.getty.edu/ulan/"/>
    <skos:example>Frank Lloyd Wright is related to Francis Conroy Sullivan</skos:example>
    <skos:prefLabel>ulan1000_related_to</skos:prefLabel>
    <rdfs:subPropertyOf rdf:resource="http://www.w3.org/2004/02/skos/core#related"/>
    <dc:identifier>1000</dc:identifier>
    <skos:example>National Endowment for the Humanities is related to Connecticut Humanities Council</skos:example>
    <rdfs:range rdf:resource="http://www.w3.org/2004/02/skos/core#Concept"/>
    <dct:description>any - related to - any.&#xD;
Example: Frank Lloyd Wright is related to Francis Conroy Sullivan; Herman Miller, Inc. is related to Irving Harper; National Endowment for the Humanities is related to Connecticut Humanities Council</dct:description>
    <dc:title>related to - any</dc:title>
    <rdf:type rdf:resource="http://www.w3.org/2002/07/owl#ObjectProperty"/>
    <rdfs:domain rdf:resource="http://www.w3.org/2004/02/skos/core#Concept"/>
  </owl:SymmetricProperty>
  <owl:SymmetricProperty rdf:about="http://vocab.getty.edu/ontology#ulan2550_friend_of">
    <dc:title>friend of - person</dc:title>
    <rdf:type rdf:resource="http://www.w3.org/2002/07/owl#ObjectProperty"/>
    <rdfs:isDefinedBy rdf:resource="http://vocab.getty.edu/ontology"/>
    <rdfs:range rdf:resource="http://www.w3.org/2004/02/skos/core#Concept"/>
    <rdfs:isDefinedBy rdf:resource="http://vocab.getty.edu/ulan/"/>
    <rdfs:domain rdf:resource="http://www.w3.org/2004/02/skos/core#Concept"/>
    <dc:identifier>2550</dc:identifier>
    <rdfs:subPropertyOf rdf:resource="http://www.w3.org/2004/02/skos/core#related"/>
    <dct:description>person - friend of (personal relationship) - person.&#xD;
Example: Alfred Stieglitz and Frank Simon Herrmann were friends</dct:description>
    <skos:example>Alfred Stieglitz and Frank Simon Herrmann were friends</skos:example>
    <skos:prefLabel>ulan2550_friend_of</skos:prefLabel>
  </owl:SymmetricProperty>
  <owl:SymmetricProperty rdf:about="http://vocab.getty.edu/ontology#ulan1414_joint_venture_with">
    <rdfs:domain rdf:resource="http://www.w3.org/2004/02/skos/core#Concept"/>
    <skos:prefLabel>ulan1414_joint_venture_with</skos:prefLabel>
    <rdfs:range rdf:resource="http://www.w3.org/2004/02/skos/core#Concept"/>
    <dc:identifier>1414</dc:identifier>
    <skos:example>Schwetye Luchini Architects is in a joint venture with ACME Architects</skos:example>
    <rdf:type rdf:resource="http://www.w3.org/2002/07/owl#ObjectProperty"/>
    <rdfs:subPropertyOf rdf:resource="http://www.w3.org/2004/02/skos/core#related"/>
    <rdfs:isDefinedBy rdf:resource="http://vocab.getty.edu/ontology"/>
    <rdfs:isDefinedBy rdf:resource="http://vocab.getty.edu/ulan/"/>
    <dc:title>joint venture with - firm/group</dc:title>
    <dct:description>firm/group - joint venture with - firm/group.&#xD;
Example: Schwetye Luchini Architects is in a joint venture with ACME Architects</dct:description>
  </owl:SymmetricProperty>
  <owl:SymmetricProperty rdf:about="http://vocab.getty.edu/ontology#aat2000_related_to">
    <skos:prefLabel>aat2000_related_to</skos:prefLabel>
    <rdfs:isDefinedBy rdf:resource="http://vocab.getty.edu/aat/"/>
    <dct:description>any - related to - any; generic relationship, not explained.&#xD;
Example: gulf red is related to light red (pigment)</dct:description>
    <rdfs:range rdf:resource="http://www.w3.org/2004/02/skos/core#Concept"/>
    <skos:scopeNote>generic relationship, not explained</skos:scopeNote>
    <dc:identifier>2000</dc:identifier>
    <rdf:type rdf:resource="http://www.w3.org/2002/07/owl#ObjectProperty"/>
    <rdfs:isDefinedBy rdf:resource="http://vocab.getty.edu/ontology"/>
    <rdfs:domain rdf:resource="http://www.w3.org/2004/02/skos/core#Concept"/>
    <skos:example>gulf red is related to light red (pigment)</skos:example>
    <rdfs:subPropertyOf rdf:resource="http://www.w3.org/2004/02/skos/core#related"/>
    <dc:title>related to - any</dc:title>
  </owl:SymmetricProperty>
  <owl:SymmetricProperty rdf:about="http://vocab.getty.edu/ontology#ulan1113_fellow_student_of">
    <rdfs:domain rdf:resource="http://www.w3.org/2004/02/skos/core#Concept"/>
    <rdfs:subPropertyOf rdf:resource="http://www.w3.org/2004/02/skos/core#related"/>
    <skos:example>John Sloan was a fellow student of Thomas Hart Benton</skos:example>
    <skos:prefLabel>ulan1113_fellow_student_of</skos:prefLabel>
    <rdfs:isDefinedBy rdf:resource="http://vocab.getty.edu/ulan/"/>
    <rdf:type rdf:resource="http://www.w3.org/2002/07/owl#ObjectProperty"/>
    <dct:description>person - fellow student of - person.&#xD;
Example: Alexander Calder was a fellow student of John Sloan; John Sloan was a fellow student of Thomas Hart Benton</dct:description>
    <dc:identifier>1113</dc:identifier>
    <rdfs:isDefinedBy rdf:resource="http://vocab.getty.edu/ontology"/>
    <rdfs:range rdf:resource="http://www.w3.org/2004/02/skos/core#Concept"/>
    <dc:title>fellow student of - person</dc:title>
    <skos:example>Alexander Calder was a fellow student of John Sloan</skos:example>
  </owl:SymmetricProperty>
  <owl:SymmetricProperty rdf:about="http://vocab.getty.edu/ontology#ulan1311_partner_of">
    <dct:description>person - partner of - person.&#xD;
Example: Frank Gehry and James Glymph are partners</dct:description>
    <rdfs:subPropertyOf rdf:resource="http://www.w3.org/2004/02/skos/core#related"/>
    <rdfs:domain rdf:resource="http://www.w3.org/2004/02/skos/core#Concept"/>
    <skos:prefLabel>ulan1311_partner_of</skos:prefLabel>
    <rdfs:range rdf:resource="http://www.w3.org/2004/02/skos/core#Concept"/>
    <rdfs:isDefinedBy rdf:resource="http://vocab.getty.edu/ontology"/>
    <rdfs:isDefinedBy rdf:resource="http://vocab.getty.edu/ulan/"/>
    <dc:title>partner of - person</dc:title>
    <skos:example>Frank Gehry and James Glymph are partners</skos:example>
    <rdf:type rdf:resource="http://www.w3.org/2002/07/owl#ObjectProperty"/>
    <dc:identifier>1311</dc:identifier>
  </owl:SymmetricProperty>
  <owl:SymmetricProperty rdf:about="http://vocab.getty.edu/ontology#ulan1521_cousin_of">
    <skos:prefLabel>ulan1521_cousin_of</skos:prefLabel>
    <rdfs:subPropertyOf rdf:resource="http://www.w3.org/2004/02/skos/core#related"/>
    <dc:identifier>1521</dc:identifier>
    <rdfs:isDefinedBy rdf:resource="http://vocab.getty.edu/ontology"/>
    <rdfs:range rdf:resource="http://www.w3.org/2004/02/skos/core#Concept"/>
    <dct:description>person - cousin of - person.&#xD;
Example: Richard Meier and Frank Gehry are cousins</dct:description>
    <rdf:type rdf:resource="http://www.w3.org/2002/07/owl#ObjectProperty"/>
    <rdfs:domain rdf:resource="http://www.w3.org/2004/02/skos/core#Concept"/>
    <rdfs:isDefinedBy rdf:resource="http://vocab.getty.edu/ulan/"/>
    <skos:example>Richard Meier and Frank Gehry are cousins</skos:example>
    <dc:title>cousin of - person</dc:title>
  </owl:SymmetricProperty>
  <owl:SymmetricProperty rdf:about="http://vocab.getty.edu/ontology#aat2824_has_parallels_with">
    <skos:example>Gnathian (pottery style) has parallels with West Slope (pottery style)</skos:example>
    <rdfs:subPropertyOf rdf:resource="http://www.w3.org/2004/02/skos/core#related"/>
    <rdfs:isDefinedBy rdf:resource="http://vocab.getty.edu/aat/"/>
    <dct:description>style/period/culture/[religion/ideology] - has parallels with - style/period/culture/[religion/ideology].&#xD;
Example: Lagozza [culture] has parallels with Chasseen [culture];  Gnathian (pottery style) has parallels with West Slope (pottery style)</dct:description>
    <rdfs:range rdf:resource="http://www.w3.org/2004/02/skos/core#Concept"/>
    <rdfs:isDefinedBy rdf:resource="http://vocab.getty.edu/ontology"/>
    <rdf:type rdf:resource="http://www.w3.org/2002/07/owl#ObjectProperty"/>
    <dc:title>has parallels with - style/period/culture</dc:title>
    <skos:example>Lagozza [culture] has parallels with Chasseen [culture]</skos:example>
    <rdfs:domain rdf:resource="http://www.w3.org/2004/02/skos/core#Concept"/>
    <dc:identifier>2824</dc:identifier>
    <skos:prefLabel>aat2824_has_parallels_with</skos:prefLabel>
  </owl:SymmetricProperty>
  <owl:SymmetricProperty rdf:about="http://vocab.getty.edu/ontology#ulan1547_romantic_partner_of">
    <dc:title>romantic partner of - person</dc:title>
    <rdfs:isDefinedBy rdf:resource="http://vocab.getty.edu/ulan/"/>
    <skos:prefLabel>ulan1547_romantic_partner_of</skos:prefLabel>
    <skos:example>Pablo Picasso and Gaby Lespinasse were romantic partners</skos:example>
    <rdfs:domain rdf:resource="http://www.w3.org/2004/02/skos/core#Concept"/>
    <dc:identifier>1547</dc:identifier>
    <rdfs:range rdf:resource="http://www.w3.org/2004/02/skos/core#Concept"/>
    <rdfs:subPropertyOf rdf:resource="http://www.w3.org/2004/02/skos/core#related"/>
    <dct:description>person - romantic partner of - person.&#xD;
Example: Pablo Picasso and Gaby Lespinasse were romantic partners; Vincent van Gogh and Clasina Hoornik were romantic partners</dct:description>
    <rdf:type rdf:resource="http://www.w3.org/2002/07/owl#ObjectProperty"/>
    <rdfs:isDefinedBy rdf:resource="http://vocab.getty.edu/ontology"/>
    <skos:example>Vincent van Gogh and Clasina Hoornik were romantic partners</skos:example>
  </owl:SymmetricProperty>
  <owl:SymmetricProperty rdf:about="http://vocab.getty.edu/ontology#ulan1556_half-sibling_of">
    <dct:description>person - half-sibling of - person.&#xD;
Example: Juan Bautista Monegro and Luis de Carbajal are half siblings</dct:description>
    <dc:title>half-sibling of - person</dc:title>
    <rdf:type rdf:resource="http://www.w3.org/2002/07/owl#ObjectProperty"/>
    <rdfs:isDefinedBy rdf:resource="http://vocab.getty.edu/ontology"/>
    <rdfs:isDefinedBy rdf:resource="http://vocab.getty.edu/ulan/"/>
    <rdfs:range rdf:resource="http://www.w3.org/2004/02/skos/core#Concept"/>
    <dc:identifier>1556</dc:identifier>
    <rdfs:domain rdf:resource="http://www.w3.org/2004/02/skos/core#Concept"/>
    <skos:example>Juan Bautista Monegro and Luis de Carbajal are half siblings</skos:example>
    <rdfs:subPropertyOf rdf:resource="http://www.w3.org/2004/02/skos/core#related"/>
    <skos:prefLabel>ulan1556_half-sibling_of</skos:prefLabel>
  </owl:SymmetricProperty>
  <owl:SymmetricProperty rdf:about="http://vocab.getty.edu/ontology#ulan1413_administration_overlaps_with">
    <rdfs:isDefinedBy rdf:resource="http://vocab.getty.edu/ontology"/>
    <skos:prefLabel>ulan1413_administration_overlaps_with</skos:prefLabel>
    <rdfs:isDefinedBy rdf:resource="http://vocab.getty.edu/ulan/"/>
    <dct:description>firm/group - administration overlaps with - firm/group.&#xD;
Example: The administration of the Numismatic Collection overlaps with Bode Museum</dct:description>
    <skos:example>The administration of the Numismatic Collection overlaps with Bode Museum</skos:example>
    <rdfs:domain rdf:resource="http://www.w3.org/2004/02/skos/core#Concept"/>
    <rdfs:subPropertyOf rdf:resource="http://www.w3.org/2004/02/skos/core#related"/>
    <dc:title>administration overlaps with - firm/group</dc:title>
    <rdf:type rdf:resource="http://www.w3.org/2002/07/owl#ObjectProperty"/>
    <dc:identifier>1413</dc:identifier>
    <rdfs:range rdf:resource="http://www.w3.org/2004/02/skos/core#Concept"/>
  </owl:SymmetricProperty>
  <owl:SymmetricProperty rdf:about="http://vocab.getty.edu/ontology#aat2826_used_with">
    <dc:identifier>2826</dc:identifier>
    <rdfs:range rdf:resource="http://www.w3.org/2004/02/skos/core#Concept"/>
    <skos:prefLabel>aat2826_used_with</skos:prefLabel>
    <rdf:type rdf:resource="http://www.w3.org/2002/07/owl#ObjectProperty"/>
    <dct:description>material - [is] used with - material.&#xD;
Example: watercolor paper is used with watercolor (paint); arriccio is used with intonaco</dct:description>
    <rdfs:domain rdf:resource="http://www.w3.org/2004/02/skos/core#Concept"/>
    <skos:example>arriccio is used with intonaco</skos:example>
    <rdfs:isDefinedBy rdf:resource="http://vocab.getty.edu/ontology"/>
    <rdfs:subPropertyOf rdf:resource="http://www.w3.org/2004/02/skos/core#related"/>
    <dc:title>used with - material</dc:title>
    <skos:example>watercolor paper is used with watercolor (paint)</skos:example>
    <rdfs:isDefinedBy rdf:resource="http://vocab.getty.edu/aat/"/>
  </owl:SymmetricProperty>
  <owl:SymmetricProperty rdf:about="http://vocab.getty.edu/ontology#ulan1544_significant_other_of">
    <rdfs:isDefinedBy rdf:resource="http://vocab.getty.edu/ulan/"/>
    <dct:description>person - significant other of - person.&#xD;
Example: Jeanne Hebuterne was the significant other of Amedeo Modigliani</dct:description>
    <rdfs:subPropertyOf rdf:resource="http://www.w3.org/2004/02/skos/core#related"/>
    <rdf:type rdf:resource="http://www.w3.org/2002/07/owl#ObjectProperty"/>
    <rdfs:range rdf:resource="http://www.w3.org/2004/02/skos/core#Concept"/>
    <skos:prefLabel>ulan1544_significant_other_of</skos:prefLabel>
    <rdfs:domain rdf:resource="http://www.w3.org/2004/02/skos/core#Concept"/>
    <skos:example>Jeanne Hebuterne was the significant other of Amedeo Modigliani</skos:example>
    <dc:title>significant other of - person</dc:title>
    <dc:identifier>1544</dc:identifier>
    <rdfs:isDefinedBy rdf:resource="http://vocab.getty.edu/ontology"/>
  </owl:SymmetricProperty>
  <owl:SymmetricProperty rdf:about="http://vocab.getty.edu/ontology#ulan1303_collaborated_with">
    <dc:title>collaborated with - person</dc:title>
    <rdfs:domain rdf:resource="http://www.w3.org/2004/02/skos/core#Concept"/>
    <rdf:type rdf:resource="http://www.w3.org/2002/07/owl#ObjectProperty"/>
    <dct:description>person - collaborated with - person.&#xD;
Example: Pablo Picasso collaborated with Georges Braque</dct:description>
    <skos:prefLabel>ulan1303_collaborated_with</skos:prefLabel>
    <rdfs:subPropertyOf rdf:resource="http://www.w3.org/2004/02/skos/core#related"/>
    <rdfs:isDefinedBy rdf:resource="http://vocab.getty.edu/ulan/"/>
    <skos:example>Pablo Picasso collaborated with Georges Braque</skos:example>
    <dc:identifier>1303</dc:identifier>
    <rdfs:range rdf:resource="http://www.w3.org/2004/02/skos/core#Concept"/>
    <rdfs:isDefinedBy rdf:resource="http://vocab.getty.edu/ontology"/>
  </owl:SymmetricProperty>
  <owl:SymmetricProperty rdf:about="http://vocab.getty.edu/ontology#ulan1550_relative_by_marriage">
    <dc:title>relative by marriage - person</dc:title>
    <dct:description>person - relative by marriage (in-law) - person.&#xD;
Example: Juana Galarza d Goicoechea and Francisco de Goya are related by marriage</dct:description>
    <dc:identifier>1550</dc:identifier>
    <rdfs:subPropertyOf rdf:resource="http://www.w3.org/2004/02/skos/core#related"/>
    <rdfs:domain rdf:resource="http://www.w3.org/2004/02/skos/core#Concept"/>
    <rdfs:isDefinedBy rdf:resource="http://vocab.getty.edu/ontology"/>
    <skos:prefLabel>ulan1550_relative_by_marriage</skos:prefLabel>
    <rdfs:isDefinedBy rdf:resource="http://vocab.getty.edu/ulan/"/>
    <skos:example>Juana Galarza d Goicoechea and Francisco de Goya are related by marriage</skos:example>
    <rdf:type rdf:resource="http://www.w3.org/2002/07/owl#ObjectProperty"/>
    <rdfs:range rdf:resource="http://www.w3.org/2004/02/skos/core#Concept"/>
  </owl:SymmetricProperty>
  <owl:SymmetricProperty rdf:about="http://vocab.getty.edu/ontology#ulan1557_step-sibling_of">
    <rdfs:domain rdf:resource="http://www.w3.org/2004/02/skos/core#Concept"/>
    <dc:identifier>1557</dc:identifier>
    <skos:prefLabel>ulan1557_step-sibling_of</skos:prefLabel>
    <dc:title>step-sibling of - person</dc:title>
    <rdf:type rdf:resource="http://www.w3.org/2002/07/owl#ObjectProperty"/>
    <rdfs:isDefinedBy rdf:resource="http://vocab.getty.edu/ulan/"/>
    <dct:description>person - step-sibling of - person.&#xD;
Example: W. L. Wyllie and Lionel Percy Smythe are step-siblings</dct:description>
    <rdfs:subPropertyOf rdf:resource="http://www.w3.org/2004/02/skos/core#related"/>
    <rdfs:range rdf:resource="http://www.w3.org/2004/02/skos/core#Concept"/>
    <skos:example>W. L. Wyllie and Lionel Percy Smythe are step-siblings</skos:example>
    <rdfs:isDefinedBy rdf:resource="http://vocab.getty.edu/ontology"/>
  </owl:SymmetricProperty>
  <owl:SymmetricProperty rdf:about="http://vocab.getty.edu/ontology#tgn3000_related_to">
    <rdfs:isDefinedBy rdf:resource="http://vocab.getty.edu/tgn/"/>
    <dc:identifier>3000</dc:identifier>
    <rdf:type rdf:resource="http://www.w3.org/2002/07/owl#ObjectProperty"/>
    <rdfs:subPropertyOf rdf:resource="http://www.w3.org/2004/02/skos/core#related"/>
    <rdfs:range rdf:resource="http://www.w3.org/2004/02/skos/core#Concept"/>
    <skos:prefLabel>tgn3000_related_to</skos:prefLabel>
    <dc:title>related to - any</dc:title>
    <rdfs:domain rdf:resource="http://www.w3.org/2004/02/skos/core#Concept"/>
    <skos:example>Fountains Abbey is related to Studley Royal</skos:example>
    <dct:description>any - related to - any.&#xD;
Example: Fountains Abbey is related to Studley Royal; Austria-Hungary is related to Magyarorszag</dct:description>
    <rdfs:isDefinedBy rdf:resource="http://vocab.getty.edu/ontology"/>
    <skos:example>Austria-Hungary is related to Magyarorszag</skos:example>
  </owl:SymmetricProperty>
  <owl:SymmetricProperty rdf:about="http://vocab.getty.edu/ontology#aat2001_formerly_referred_to">
    <rdfs:domain rdf:resource="http://www.w3.org/2004/02/skos/core#Concept"/>
    <dct:description>any - formerly referred - any.&#xD;
Example: gigues formerly referred to fiddles</dct:description>
    <dc:title>formerly referred to - any</dc:title>
    <skos:example>gigues formerly referred to fiddles</skos:example>
    <dc:identifier>2001</dc:identifier>
    <rdfs:subPropertyOf rdf:resource="http://www.w3.org/2004/02/skos/core#related"/>
    <rdfs:isDefinedBy rdf:resource="http://vocab.getty.edu/ontology"/>
    <rdfs:range rdf:resource="http://www.w3.org/2004/02/skos/core#Concept"/>
    <rdfs:isDefinedBy rdf:resource="http://vocab.getty.edu/aat/"/>
    <rdf:type rdf:resource="http://www.w3.org/2002/07/owl#ObjectProperty"/>
    <skos:prefLabel>aat2001_formerly_referred_to</skos:prefLabel>
  </owl:SymmetricProperty>
  <owl:SymmetricProperty rdf:about="http://vocab.getty.edu/ontology#aat2203_associated_with">
    <dc:identifier>2203</dc:identifier>
    <rdf:type rdf:resource="http://www.w3.org/2002/07/owl#ObjectProperty"/>
    <skos:example>Easter is associated with Lent</skos:example>
    <rdfs:range rdf:resource="http://www.w3.org/2004/02/skos/core#Concept"/>
    <dct:description>activity/event/[process/function] - [is] associated with - activity/event/[process/function].&#xD;
Example: Easter is associated with Lent; cavalry exercises are associated with dressage</dct:description>
    <rdfs:subPropertyOf rdf:resource="http://www.w3.org/2004/02/skos/core#related"/>
    <skos:prefLabel>aat2203_associated_with</skos:prefLabel>
    <rdfs:domain rdf:resource="http://www.w3.org/2004/02/skos/core#Concept"/>
    <rdfs:isDefinedBy rdf:resource="http://vocab.getty.edu/aat/"/>
    <skos:example>cavalry exercises are associated with dressage</skos:example>
    <rdfs:isDefinedBy rdf:resource="http://vocab.getty.edu/ontology"/>
    <dc:title>associated with - activity/event</dc:title>
  </owl:SymmetricProperty>
  <owl:SymmetricProperty rdf:about="http://vocab.getty.edu/ontology#tgn3101_near-adjacent_to">
    <dc:identifier>3101</dc:identifier>
    <rdfs:domain rdf:resource="http://www.w3.org/2004/02/skos/core#Concept"/>
    <rdfs:range rdf:resource="http://www.w3.org/2004/02/skos/core#Concept"/>
    <rdf:type rdf:resource="http://www.w3.org/2002/07/owl#ObjectProperty"/>
    <rdfs:isDefinedBy rdf:resource="http://vocab.getty.edu/ontology"/>
    <dct:description>any - near/adjacent to - any.&#xD;
Example: Saint Paul (Minnesota, USA), is linked to its 'Twin City' Minneapolis (Hennepin county, Minnesota, USA)</dct:description>
    <skos:prefLabel>tgn3101_near-adjacent_to</skos:prefLabel>
    <dc:title>near/adjacent to - any</dc:title>
    <rdfs:isDefinedBy rdf:resource="http://vocab.getty.edu/tgn/"/>
    <skos:example>Saint Paul (Minnesota, USA), is linked to its 'Twin City' Minneapolis (Hennepin county, Minnesota, USA)</skos:example>
    <rdfs:subPropertyOf rdf:resource="http://www.w3.org/2004/02/skos/core#related"/>
  </owl:SymmetricProperty>
  <owl:SymmetricProperty rdf:about="http://vocab.getty.edu/ontology#ulan1501_sibling_of">
    <rdfs:domain rdf:resource="http://www.w3.org/2004/02/skos/core#Concept"/>
    <skos:example>Philippe Rubens is the sibling of Peter Paul Rubens</skos:example>
    <dc:title>sibling of - person</dc:title>
    <rdfs:isDefinedBy rdf:resource="http://vocab.getty.edu/ulan/"/>
    <rdfs:range rdf:resource="http://www.w3.org/2004/02/skos/core#Concept"/>
    <dc:identifier>1501</dc:identifier>
    <rdf:type rdf:resource="http://www.w3.org/2002/07/owl#ObjectProperty"/>
    <rdfs:subPropertyOf rdf:resource="http://www.w3.org/2004/02/skos/core#related"/>
    <skos:prefLabel>ulan1501_sibling_of</skos:prefLabel>
    <dct:description>person - sibling of - person.&#xD;
Example: Philippe Rubens is the sibling of Peter Paul Rubens</dct:description>
    <rdfs:isDefinedBy rdf:resource="http://vocab.getty.edu/ontology"/>
  </owl:SymmetricProperty>
  <owl:SymmetricProperty rdf:about="http://vocab.getty.edu/ontology#ulan1003_associated_with">
    <rdfs:range rdf:resource="http://www.w3.org/2004/02/skos/core#Concept"/>
    <skos:example>United Nations is associated with World Bank</skos:example>
    <rdfs:subPropertyOf rdf:resource="http://www.w3.org/2004/02/skos/core#related"/>
    <dc:title>associated with - any</dc:title>
    <rdfs:isDefinedBy rdf:resource="http://vocab.getty.edu/ulan/"/>
    <dc:identifier>1003</dc:identifier>
    <rdfs:domain rdf:resource="http://www.w3.org/2004/02/skos/core#Concept"/>
    <rdf:type rdf:resource="http://www.w3.org/2002/07/owl#ObjectProperty"/>
    <dct:description>any - associated with - any.&#xD;
Example: Richard Meier is associated with Renny B.Saltzman; United Nations is associated with World Bank</dct:description>
    <rdfs:isDefinedBy rdf:resource="http://vocab.getty.edu/ontology"/>
    <skos:prefLabel>ulan1003_associated_with</skos:prefLabel>
    <skos:example>Richard Meier is associated with Renny B.Saltzman</skos:example>
  </owl:SymmetricProperty>
  <owl:SymmetricProperty rdf:about="http://vocab.getty.edu/ontology#ulan1005_possibly_identified_with">
    <dct:description>any - possibly identified with - any.&#xD;
Example: Master of the Saint John Altarpiece is possibly identified with Hughe Jacobsz; Bauart is possibly identified with Gruppe BAUart</dct:description>
    <dc:identifier>1005</dc:identifier>
    <rdfs:domain rdf:resource="http://www.w3.org/2004/02/skos/core#Concept"/>
    <skos:example>Bauart is possibly identified with Gruppe BAUart</skos:example>
    <dc:title>possibly identified with - any</dc:title>
    <rdfs:isDefinedBy rdf:resource="http://vocab.getty.edu/ontology"/>
    <skos:example>Master of the Saint John Altarpiece is possibly identified with Hughe Jacobsz</skos:example>
    <rdfs:range rdf:resource="http://www.w3.org/2004/02/skos/core#Concept"/>
    <skos:prefLabel>ulan1005_possibly_identified_with</skos:prefLabel>
    <rdf:type rdf:resource="http://www.w3.org/2002/07/owl#ObjectProperty"/>
    <rdfs:isDefinedBy rdf:resource="http://vocab.getty.edu/ulan/"/>
    <rdfs:subPropertyOf rdf:resource="http://www.w3.org/2004/02/skos/core#related"/>
  </owl:SymmetricProperty>
  <owl:SymmetricProperty rdf:about="http://vocab.getty.edu/ontology#ulan1006_formerly_identified_with">
    <dc:identifier>1006</dc:identifier>
    <rdfs:isDefinedBy rdf:resource="http://vocab.getty.edu/ontology"/>
    <dct:description>any - formerly identified with - any.&#xD;
Example: Tommaso is formerly identified with Tommaso di Stefano Lunetti; GreenWorks is formerly identified with Mike Faha &amp; Associates</dct:description>
    <dc:title>formerly identified with - any</dc:title>
    <rdfs:subPropertyOf rdf:resource="http://www.w3.org/2004/02/skos/core#related"/>
    <rdfs:isDefinedBy rdf:resource="http://vocab.getty.edu/ulan/"/>
    <rdfs:domain rdf:resource="http://www.w3.org/2004/02/skos/core#Concept"/>
    <rdf:type rdf:resource="http://www.w3.org/2002/07/owl#ObjectProperty"/>
    <skos:example>Tommaso is formerly identified with Tommaso di Stefano Lunetti</skos:example>
    <rdfs:range rdf:resource="http://www.w3.org/2004/02/skos/core#Concept"/>
    <skos:example>GreenWorks is formerly identified with Mike Faha &amp; Associates</skos:example>
    <skos:prefLabel>ulan1006_formerly_identified_with</skos:prefLabel>
  </owl:SymmetricProperty>
  <owl:SymmetricProperty rdf:about="http://vocab.getty.edu/ontology#ulan1305_worked_with">
    <dc:identifier>1305</dc:identifier>
    <skos:prefLabel>ulan1305_worked_with</skos:prefLabel>
    <dct:description>person - worked with - person.&#xD;
Example: William Cleare worked with Christopher Wren; Frank Lloyd Wright work with Aaron G. Green</dct:description>
    <skos:example>Frank Lloyd Wright work with Aaron G. Green</skos:example>
    <dc:title>worked with - person</dc:title>
    <rdfs:isDefinedBy rdf:resource="http://vocab.getty.edu/ulan/"/>
    <rdfs:isDefinedBy rdf:resource="http://vocab.getty.edu/ontology"/>
    <rdf:type rdf:resource="http://www.w3.org/2002/07/owl#ObjectProperty"/>
    <rdfs:range rdf:resource="http://www.w3.org/2004/02/skos/core#Concept"/>
    <rdfs:subPropertyOf rdf:resource="http://www.w3.org/2004/02/skos/core#related"/>
    <rdfs:domain rdf:resource="http://www.w3.org/2004/02/skos/core#Concept"/>
    <skos:example>William Cleare worked with Christopher Wren</skos:example>
  </owl:SymmetricProperty>
  <owl:SymmetricProperty rdf:about="http://vocab.getty.edu/ontology#ulan1301_colleague_of">
    <skos:example>Titian was a colleague of Maria Giovanni Verdizotti</skos:example>
    <rdfs:isDefinedBy rdf:resource="http://vocab.getty.edu/ulan/"/>
    <skos:prefLabel>ulan1301_colleague_of</skos:prefLabel>
    <rdfs:isDefinedBy rdf:resource="http://vocab.getty.edu/ontology"/>
    <rdf:type rdf:resource="http://www.w3.org/2002/07/owl#ObjectProperty"/>
    <rdfs:subPropertyOf rdf:resource="http://www.w3.org/2004/02/skos/core#related"/>
    <dct:description>person - colleague of - person.&#xD;
Example: Titian was a colleague of Maria Giovanni Verdizotti</dct:description>
    <rdfs:domain rdf:resource="http://www.w3.org/2004/02/skos/core#Concept"/>
    <dc:title>colleague of - person</dc:title>
    <dc:identifier>1301</dc:identifier>
    <rdfs:range rdf:resource="http://www.w3.org/2004/02/skos/core#Concept"/>
  </owl:SymmetricProperty>
  <owl:SymmetricProperty rdf:about="http://vocab.getty.edu/ontology#ulan1007_distinguished_from">
    <dc:identifier>1007</dc:identifier>
    <rdfs:isDefinedBy rdf:resource="http://vocab.getty.edu/ulan/"/>
    <dc:title>distinguished from - any</dc:title>
    <rdfs:subPropertyOf rdf:resource="http://www.w3.org/2004/02/skos/core#related"/>
    <skos:prefLabel>ulan1007_distinguished_from</skos:prefLabel>
    <skos:example>The Noguchi Museum is distinguished form Isamu Noguchi Garden Museum Japan</skos:example>
    <dct:description>any - distinguished from - any.&#xD;
Example: Laura Theresa Alma-Tadema is distinguished from Lawrence Alma-Tadema; The Noguchi Museum is distinguished form Isamu Noguchi Garden Museum Japan</dct:description>
    <rdfs:isDefinedBy rdf:resource="http://vocab.getty.edu/ontology"/>
    <rdf:type rdf:resource="http://www.w3.org/2002/07/owl#ObjectProperty"/>
    <rdfs:range rdf:resource="http://www.w3.org/2004/02/skos/core#Concept"/>
    <skos:example>Laura Theresa Alma-Tadema is distinguished from Lawrence Alma-Tadema</skos:example>
    <rdfs:domain rdf:resource="http://www.w3.org/2004/02/skos/core#Concept"/>
  </owl:SymmetricProperty>
  <owl:SymmetricProperty rdf:about="http://vocab.getty.edu/ontology#tgn3001_distinguished_from">
    <skos:prefLabel>tgn3001_distinguished_from</skos:prefLabel>
    <rdfs:isDefinedBy rdf:resource="http://vocab.getty.edu/tgn/"/>
    <rdfs:domain rdf:resource="http://www.w3.org/2004/02/skos/core#Concept"/>
    <rdfs:range rdf:resource="http://www.w3.org/2004/02/skos/core#Concept"/>
    <dct:description>any - distinguished from - any.&#xD;
Example: The Ancient Mesopotamian Kingdom 'Assyria' is distinguished from the Roman Province of the same name</dct:description>
    <dc:title>distinguished from - any</dc:title>
    <skos:example>The Ancient Mesopotamian Kingdom 'Assyria' is distinguished from the Roman Province of the same name</skos:example>
    <rdfs:isDefinedBy rdf:resource="http://vocab.getty.edu/ontology"/>
    <dc:identifier>3001</dc:identifier>
    <rdf:type rdf:resource="http://www.w3.org/2002/07/owl#ObjectProperty"/>
    <rdfs:subPropertyOf rdf:resource="http://www.w3.org/2004/02/skos/core#related"/>
  </owl:SymmetricProperty>
  <skos:Concept rdf:about="http://vocab.getty.edu/term/display/Indexing">
    <skos:inScheme>
      <skos:ConceptScheme rdf:about="http://vocab.getty.edu/term/display/">
        <rdfs:isDefinedBy rdf:resource="http://vocab.getty.edu/ontology"/>
        <rdfs:label>Term Display concept scheme</rdfs:label>
        <dct:description>Term Display concept scheme</dct:description>
      </skos:ConceptScheme>
    </skos:inScheme>
    <skos:notation>I</skos:notation>
    <skos:prefLabel>Use in Indexes/lists</skos:prefLabel>
    <skos:scopeNote>Use in indexes or permuted lists where inverted order is appropriate</skos:scopeNote>
    <dct:description>Use in indexes or permuted lists where inverted order is appropriate</dct:description>
  </skos:Concept>
  <skos:Concept rdf:about="http://vocab.getty.edu/term/POS/Adjectival">
    <skos:inScheme>
      <skos:ConceptScheme rdf:about="http://vocab.getty.edu/term/POS/">
        <rdfs:isDefinedBy rdf:resource="http://vocab.getty.edu/ontology"/>
        <rdfs:label>Part of Speech concept scheme</rdfs:label>
        <dct:description>Part of Speech concept scheme</dct:description>
      </skos:ConceptScheme>
    </skos:inScheme>
    <skos:notation>A</skos:notation>
    <skos:prefLabel>Adjectival</skos:prefLabel>
    <skos:scopeNote>This term may be combined with others in post-coordinated compound terms</skos:scopeNote>
    <skos:example>"Renaissance" (as in "Renaissance cathedral"), "painter's" (as in "painter's smock")</skos:example>
    <dct:description>This term may be combined with others in post-coordinated compound terms.
Example: "Renaissance" (as in "Renaissance cathedral"), "painter's" (as in "painter's smock")</dct:description>
  </skos:Concept>
  <skos:Concept rdf:about="http://vocab.getty.edu/term/kind/Abbreviation">
    <skos:inScheme>
      <skos:ConceptScheme rdf:about="http://vocab.getty.edu/term/kind/">
        <rdfs:isDefinedBy rdf:resource="http://vocab.getty.edu/ontology"/>
        <rdfs:label>Term Kind concept scheme</rdfs:label>
        <dct:description>Term Kind concept scheme</dct:description>
      </skos:ConceptScheme>
    </skos:inScheme>
    <skos:notation>A</skos:notation>
    <skos:prefLabel>Abbreviation</skos:prefLabel>
    <skos:scopeNote>Term is an abbreviation, initialism, or acronym</skos:scopeNote>
    <skos:example>"FLIM" is abbrevaition for "fluorescence lifetime imaging microscopy"</skos:example>
    <dct:description>Term is an abbreviation, initialism, or acronym.
Example: "FLIM" is abbrevaition for "fluorescence lifetime imaging microscopy"</dct:description>
  </skos:Concept>
  <skos:Concept rdf:about="http://vocab.getty.edu/term/kind/CommonTerm">
    <skos:inScheme rdf:resource="http://vocab.getty.edu/term/kind/"/>
    <skos:notation>C</skos:notation>
    <skos:prefLabel>Common term</skos:prefLabel>
    <skos:scopeNote>Preferred common language term. Used for subjects that also include a Scientific term. Used in AAT only</skos:scopeNote>
    <skos:example>"frankincense" (species) is common term for "Boswellia sacra" (species)</skos:example>
    <dct:description>Preferred common language term. Used for subjects that also include a Scientific term. Used in AAT only.
Example: "frankincense" (species) is common term for "Boswellia sacra" (species)</dct:description>
  </skos:Concept>
  <skos:Concept rdf:about="http://vocab.getty.edu/term/kind/ISOnumeric3">
    <skos:inScheme rdf:resource="http://vocab.getty.edu/term/kind/"/>
    <skos:notation>ISO3N</skos:notation>
    <skos:prefLabel>ISO numeric-3 code</skos:prefLabel>
    <skos:scopeNote>ISO 3166-1 numeric country code as "ISOnnn" (though ISO specifies only "nnn"). Used in TGN only</skos:scopeNote>
    <skos:example>"ISO414" for Kuwait</skos:example>
    <dct:description>ISO 3166-1 numeric country code as "ISOnnn" (though ISO specifies only "nnn"). Used in TGN only.
Example: "ISO414" for Kuwait</dct:description>
  </skos:Concept>
  <skos:Concept rdf:about="http://vocab.getty.edu/term/kind/Neologism">
    <skos:inScheme rdf:resource="http://vocab.getty.edu/term/kind/"/>
    <skos:notation>N</skos:notation>
    <skos:prefLabel>Neologism</skos:prefLabel>
    <skos:scopeNote>Term that is new to the language, generally having been coined due to new technology. Used in AAT only.</skos:scopeNote>
    <skos:example>"folksonomy", "podcasting"</skos:example>
    <dct:description>Term that is new to the language, generally having been coined due to new technology. Used in AAT only..
Example: "folksonomy", "podcasting"</dct:description>
  </skos:Concept>
  <skos:Concept rdf:about="http://vocab.getty.edu/term/kind/ISOnumeric2">
    <skos:inScheme rdf:resource="http://vocab.getty.edu/term/kind/"/>
    <skos:notation>ISO2N</skos:notation>
    <skos:prefLabel>ISO numeric-2 code</skos:prefLabel>
    <skos:scopeNote>May be used in TGN, but no code of this kind is present</skos:scopeNote>
    <dct:description>May be used in TGN, but no code of this kind is present</dct:description>
  </skos:Concept>
  <ptop:TypeRestr rdf:about="http://vocab.getty.edu/ontology#Infer_broaderNonConcept_TypeRestr">
    <ptop:premise rdf:resource="http://vocab.getty.edu/ontology#broader"/>
    <ptop:type1 rdf:resource="http://www.w3.org/2004/02/skos/core#Concept"/>
    <ptop:type2 rdf:resource="http://vocab.getty.edu/ontology#GuideTerm"/>
    <ptop:conclusion rdf:resource="http://vocab.getty.edu/ontology#broaderNonConcept"/>
  </ptop:TypeRestr>
  <skos:Concept rdf:about="http://vocab.getty.edu/term/kind/ISOalpha2">
    <skos:inScheme rdf:resource="http://vocab.getty.edu/term/kind/"/>
    <skos:notation>ISO2L</skos:notation>
    <skos:prefLabel>ISO alpha-2 code</skos:prefLabel>
    <skos:scopeNote>ISO 3166-1 alpha-2 country code. Used in TGN</skos:scopeNote>
    <skos:example>"AQ" for Antarctica</skos:example>
    <dct:description>ISO 3166-1 alpha-2 country code. Used in TGN.
Example: "AQ" for Antarctica</dct:description>
  </skos:Concept>
  <rdf:Description rdf:about="http://www.w3.org/2004/02/skos/core#hiddenLabel">
    <owl:propertyChainAxiom rdf:parseType="Collection">
      <rdf:Description rdf:about="http://www.w3.org/2008/05/skos-xl#hiddenLabel"/>
      <rdf:Description rdf:about="http://www.w3.org/2008/05/skos-xl#literalForm"/>
    </owl:propertyChainAxiom>
  </rdf:Description>
  <skos:Concept rdf:about="http://vocab.getty.edu/term/kind/ISOalpha3">
    <skos:inScheme rdf:resource="http://vocab.getty.edu/term/kind/"/>
    <skos:notation>ISO3L</skos:notation>
    <skos:prefLabel>ISO alpha-3 code</skos:prefLabel>
    <skos:scopeNote>ISO 3166-1 alpha-3 country code. Used in TGN</skos:scopeNote>
    <skos:example>"ATA" for Antarctica</skos:example>
    <dct:description>ISO 3166-1 alpha-3 country code. Used in TGN.
Example: "ATA" for Antarctica</dct:description>
  </skos:Concept>
  <skos:Concept rdf:about="http://vocab.getty.edu/term/kind/FIPSCode">
    <skos:inScheme rdf:resource="http://vocab.getty.edu/term/kind/"/>
    <skos:notation>FIPS</skos:notation>
    <skos:prefLabel>FIPS Code</skos:prefLabel>
    <skos:scopeNote>FIPS region code. Used in TGN</skos:scopeNote>
    <skos:example>"MX21" for Puebla, Mexico</skos:example>
    <dct:description>FIPS region code. Used in TGN.
Example: "MX21" for Puebla, Mexico</dct:description>
  </skos:Concept>
  <skos:Concept rdf:about="http://vocab.getty.edu/term/kind/USPSCode">
    <skos:inScheme rdf:resource="http://vocab.getty.edu/term/kind/"/>
    <skos:notation>USPS</skos:notation>
    <skos:prefLabel>US Postal Service Code</skos:prefLabel>
    <skos:scopeNote>Used in TGN only</skos:scopeNote>
    <skos:example>"CA" for California</skos:example>
    <dct:description>Used in TGN only.
Example: "CA" for California</dct:description>
  </skos:Concept>
  <skos:Concept rdf:about="http://vocab.getty.edu/term/kind/FullTerm">
    <skos:inScheme rdf:resource="http://vocab.getty.edu/term/kind/"/>
    <skos:notation>F</skos:notation>
    <skos:prefLabel>Full term</skos:prefLabel>
    <skos:scopeNote>Full-form term. Used when the descriptor is a shorter form, or the subject also includes an Abbreviation. Used in AAT only</skos:scopeNote>
    <skos:example>"Extensible Markup Language" is the full term for "XML" (which is preferred)</skos:example>
    <dct:description>Full-form term. Used when the descriptor is a shorter form, or the subject also includes an Abbreviation. Used in AAT only.
Example: "Extensible Markup Language" is the full term for "XML" (which is preferred)</dct:description>
  </skos:Concept>
  <skos:Concept rdf:about="http://vocab.getty.edu/term/kind/OfficialName">
    <skos:inScheme rdf:resource="http://vocab.getty.edu/term/kind/"/>
    <skos:notation>O</skos:notation>
    <skos:prefLabel>Official Name</skos:prefLabel>
    <skos:scopeNote>Used in TGN and ULAN</skos:scopeNote>
    <skos:example>"Noyen-sur-Seine" is official name of 7030197 "Noyen" (TGN)</skos:example>
    <dct:description>Used in TGN and ULAN.
Example: "Noyen-sur-Seine" is official name of 7030197 "Noyen" (TGN)</dct:description>
  </skos:Concept>
  <skos:Concept rdf:about="http://vocab.getty.edu/term/kind/SiteName">
    <skos:inScheme rdf:resource="http://vocab.getty.edu/term/kind/"/>
    <skos:notation>S</skos:notation>
    <skos:prefLabel>Site Name</skos:prefLabel>
    <skos:scopeNote>Used in TGN only</skos:scopeNote>
    <skos:example>"Flavia Solva", a deserted settlement and archaeological site (TGN)</skos:example>
    <dct:description>Used in TGN only.
Example: "Flavia Solva", a deserted settlement and archaeological site (TGN)</dct:description>
  </skos:Concept>
  <skos:Concept rdf:about="http://vocab.getty.edu/term/kind/ScientificOrTechnical">
    <skos:inScheme rdf:resource="http://vocab.getty.edu/term/kind/"/>
    <skos:notation>S</skos:notation>
    <skos:prefLabel>Scientific or Technical term</skos:prefLabel>
    <skos:scopeNote>Scientific taxon name (genus, species, etc). Used in AAT only. All such are emitted marked with English language, and most have the same string marked with Latin</skos:scopeNote>
    <skos:example>"Boswellia sacra"@la, also emitted as "Boswellia sacra"@en, is scientific name of "frankincense"</skos:example>
    <dct:description>Scientific taxon name (genus, species, etc). Used in AAT only. All such are emitted marked with English language, and most have the same string marked with Latin.
Example: "Boswellia sacra"@la, also emitted as "Boswellia sacra"@en, is scientific name of "frankincense"</dct:description>
  </skos:Concept>
  <skos:Concept rdf:about="http://vocab.getty.edu/historic/currentAndHistoric">
    <skos:inScheme>
      <skos:ConceptScheme rdf:about="http://vocab.getty.edu/historic/">
        <rdfs:isDefinedBy rdf:resource="http://vocab.getty.edu/ontology"/>
        <rdfs:label>Historic Flag concept scheme</rdfs:label>
        <dct:description>Historic Flag concept scheme</dct:description>
      </skos:ConceptScheme>
    </skos:inScheme>
    <skos:notation>B</skos:notation>
    <skos:prefLabel>Both Current and Historic</skos:prefLabel>
    <skos:scopeNote>Valid/used both in the past and currently</skos:scopeNote>
    <skos:example>Saint Petersburg (TGN)</skos:example>
    <dct:description>Valid/used both in the past and currently.
Example: Saint Petersburg (TGN)</dct:description>
  </skos:Concept>
  <rdf:Description rdf:about="http://www.w3.org/2004/02/skos/core#prefLabel">
    <owl:propertyChainAxiom rdf:parseType="Collection">
      <rdf:Description rdf:about="http://www.w3.org/2008/05/skos-xl#prefLabel"/>
      <rdf:Description rdf:about="http://www.w3.org/2008/05/skos-xl#literalForm"/>
    </owl:propertyChainAxiom>
  </rdf:Description>
  <ptop:PropChainType2 rdf:about="http://vocab.getty.edu/ontology#Infer_skosBroader_PropChainType2">
    <ptop:premise1 rdf:resource="http://vocab.getty.edu/ontology#broaderNonConcept"/>
    <ptop:premise2 rdf:resource="http://vocab.getty.edu/ontology#broader"/>
    <ptop:type2 rdf:resource="http://www.w3.org/2004/02/skos/core#Concept"/>
    <ptop:conclusion rdf:resource="http://www.w3.org/2004/02/skos/core#broader"/>
  </ptop:PropChainType2>
  <ptop:PropRestr rdf:about="http://vocab.getty.edu/ontology#Infer_isoBroaderPartitive">
    <ptop:premise rdf:resource="http://vocab.getty.edu/ontology#broaderPartitiveExtended"/>
    <ptop:restriction rdf:resource="http://www.w3.org/2004/02/skos/core#broader"/>
    <ptop:conclusion rdf:resource="http://purl.org/iso25964/skos-thes#broaderPartitive"/>
  </ptop:PropRestr>
  <skos:Concept rdf:about="http://vocab.getty.edu/term/POS/Noun">
    <skos:inScheme rdf:resource="http://vocab.getty.edu/term/POS/"/>
    <skos:notation>N</skos:notation>
    <skos:prefLabel>Noun</skos:prefLabel>
    <skos:scopeNote>Term is a noun but we are uncertain if it is plural or singular</skos:scopeNote>
    <skos:example>Panthera leo</skos:example>
    <dct:description>Term is a noun but we are uncertain if it is plural or singular.
Example: Panthera leo</dct:description>
  </skos:Concept>
  <ptop:PropChainRestr rdf:about="http://vocab.getty.edu/ontology#Infer_broaderPreferredExtended">
    <ptop:premise1 rdf:resource="http://vocab.getty.edu/ontology#broaderPreferredExtended"/>
    <ptop:premise2 rdf:resource="http://vocab.getty.edu/ontology#broaderPreferred"/>
    <ptop:restriction rdf:resource="http://vocab.getty.edu/ontology#broaderExtended"/>
    <ptop:conclusion rdf:resource="http://vocab.getty.edu/ontology#broaderPreferredExtended"/>
  </ptop:PropChainRestr>
  <ptop:PropRestr rdf:about="http://vocab.getty.edu/ontology#Infer_isoBroaderGeneric">
    <ptop:premise rdf:resource="http://vocab.getty.edu/ontology#broaderGenericExtended"/>
    <ptop:restriction rdf:resource="http://www.w3.org/2004/02/skos/core#broader"/>
    <ptop:conclusion rdf:resource="http://purl.org/iso25964/skos-thes#broaderGeneric"/>
  </ptop:PropRestr>
  <rdf:Description rdf:about="http://purl.org/dc/terms/isReplacedBy">
    <owl:inverseOf rdf:resource="http://purl.org/dc/terms/replaces"/>
  </rdf:Description>
  <skos:Concept rdf:about="http://vocab.getty.edu/term/kind/Pseudonym">
    <skos:inScheme rdf:resource="http://vocab.getty.edu/term/kind/"/>
    <skos:notation>P</skos:notation>
    <skos:prefLabel>Pseudonym</skos:prefLabel>
    <skos:scopeNote>Used in TGN and ULAN</skos:scopeNote>
    <skos:example>"Frisco" is nickname for San Francisco (TGN)</skos:example>
    <dct:description>Used in TGN and ULAN.
Example: "Frisco" is nickname for San Francisco (TGN)</dct:description>
  </skos:Concept>
  <skos:Concept rdf:about="http://vocab.getty.edu/term/POS/VerbalNounGerund">
    <skos:inScheme rdf:resource="http://vocab.getty.edu/term/POS/"/>
    <skos:notation>VN</skos:notation>
    <skos:prefLabel>Verbal Noun/Gerund</skos:prefLabel>
    <skos:scopeNote>Term is a verbal noun or gerund</skos:scopeNote>
    <skos:example>polishing</skos:example>
    <dct:description>Term is a verbal noun or gerund.
Example: polishing</dct:description>
  </skos:Concept>
  <ptop:TypeRestr rdf:about="http://vocab.getty.edu/ontology#Infer_skosBroader_TypeRestr">
    <ptop:premise rdf:resource="http://vocab.getty.edu/ontology#broader"/>
    <ptop:type1 rdf:resource="http://www.w3.org/2004/02/skos/core#Concept"/>
    <ptop:type2 rdf:resource="http://www.w3.org/2004/02/skos/core#Concept"/>
    <ptop:conclusion rdf:resource="http://www.w3.org/2004/02/skos/core#broader"/>
  </ptop:TypeRestr>
  <skos:Concept rdf:about="http://vocab.getty.edu/historic/current">
    <skos:inScheme rdf:resource="http://vocab.getty.edu/historic/"/>
    <skos:notation>C</skos:notation>
    <skos:prefLabel>Current</skos:prefLabel>
    <skos:scopeNote>Valid/used currently</skos:scopeNote>
    <dct:description>Valid/used currently</dct:description>
  </skos:Concept>
  <skos:Concept rdf:about="http://vocab.getty.edu/term/type/UsedForTerm">
    <skos:inScheme>
      <skos:ConceptScheme rdf:about="http://vocab.getty.edu/term/type/">
        <rdfs:isDefinedBy rdf:resource="http://vocab.getty.edu/ontology"/>
        <rdfs:label>Term Type concept scheme</rdfs:label>
        <dct:description>Term Type concept scheme</dct:description>
      </skos:ConceptScheme>
    </skos:inScheme>
    <skos:notation>UF</skos:notation>
    <skos:prefLabel>Used for Term</skos:prefLabel>
    <skos:scopeNote>A synonym</skos:scopeNote>
    <skos:example>"handschriften" (Dutch) instead of "manuscripten"</skos:example>
    <dct:description>A synonym.
Example: "handschriften" (Dutch) instead of "manuscripten"</dct:description>
  </skos:Concept>
  <rdf:Description rdf:about="http://vocab.getty.edu/aat/300189559">
    <skos:exactMatch rdf:resource="http://www.wikidata.org/entity/Q6581097"/>
    <skos:exactMatch rdf:resource="http://rdaregistry.info/termList/gender/1002"/>
  </rdf:Description>
  <skos:Concept rdf:about="http://vocab.getty.edu/term/display/Display">
    <skos:inScheme rdf:resource="http://vocab.getty.edu/term/display/"/>
    <skos:notation>D</skos:notation>
    <skos:prefLabel>Use for Display</skos:prefLabel>
    <skos:scopeNote>Use in displays where natural order is appropriate</skos:scopeNote>
    <dct:description>Use in displays where natural order is appropriate</dct:description>
    <skos:notation>Y</skos:notation>
  </skos:Concept>
  <skos:Concept rdf:about="http://vocab.getty.edu/term/kind/BirthName">
    <skos:inScheme rdf:resource="http://vocab.getty.edu/term/kind/"/>
    <skos:notation>BN</skos:notation>
    <skos:prefLabel>Birth Name</skos:prefLabel>
    <skos:scopeNote>Birth Name of an ULAN agent</skos:scopeNote>
    <skos:example>TODO</skos:example>
    <dct:description>Birth Name of an ULAN agent.
Example: TODO</dct:description>
  </skos:Concept>
  <skos:Concept rdf:about="http://vocab.getty.edu/term/POS/SingularNoun">
    <skos:inScheme rdf:resource="http://vocab.getty.edu/term/POS/"/>
    <skos:notation>SN</skos:notation>
    <skos:prefLabel>Singular Noun</skos:prefLabel>
    <skos:scopeNote>A term that is singular (the same word may be plural in another language)</skos:scopeNote>
    <skos:example>"filigrane" is the French singular for "watermark"</skos:example>
    <dct:description>A term that is singular (the same word may be plural in another language).
Example: "filigrane" is the French singular for "watermark"</dct:description>
  </skos:Concept>
  <rdf:Description rdf:about="http://vocab.getty.edu/aat/300189557">
    <skos:exactMatch rdf:resource="http://www.wikidata.org/entity/Q6581072"/>
    <skos:exactMatch rdf:resource="http://rdaregistry.info/termList/gender/1001"/>
  </rdf:Description>
  <ptop:PropChainType2 rdf:about="http://vocab.getty.edu/ontology#Infer_broaderNonConcept_PropChainType2">
    <ptop:premise1 rdf:resource="http://vocab.getty.edu/ontology#broaderNonConcept"/>
    <ptop:premise2 rdf:resource="http://vocab.getty.edu/ontology#broader"/>
    <ptop:type2 rdf:resource="http://vocab.getty.edu/ontology#GuideTerm"/>
    <ptop:conclusion rdf:resource="http://vocab.getty.edu/ontology#broaderNonConcept"/>
  </ptop:PropChainType2>
  <skos:Concept rdf:about="http://vocab.getty.edu/term/kind/ChemicalName">
    <skos:inScheme rdf:resource="http://vocab.getty.edu/term/kind/"/>
    <skos:notation>CN</skos:notation>
    <skos:prefLabel>Chemical Name</skos:prefLabel>
    <skos:scopeNote>Term is the chemical name for the descriptor. Used in AAT only</skos:scopeNote>
    <skos:example>"sodium tetraborate decahydrate" is chemical name for "borax"</skos:example>
    <dct:description>Term is the chemical name for the descriptor. Used in AAT only.
Example: "sodium tetraborate decahydrate" is chemical name for "borax"</dct:description>
  </skos:Concept>
  <skos:Concept rdf:about="http://vocab.getty.edu/term/type/AlternateDescriptor">
    <skos:inScheme rdf:resource="http://vocab.getty.edu/term/type/"/>
    <skos:notation>AD</skos:notation>
    <skos:prefLabel>Alternate Descriptor</skos:prefLabel>
    <skos:scopeNote>A lexical variant, eg singular</skos:scopeNote>
    <skos:example>"manuscript" (English) instead of "manuscripts"</skos:example>
    <dct:description>A lexical variant, eg singular.
Example: "manuscript" (English) instead of "manuscripts"</dct:description>
  </skos:Concept>
  <skos:Concept rdf:about="http://vocab.getty.edu/historic/historic">
    <skos:inScheme rdf:resource="http://vocab.getty.edu/historic/"/>
    <skos:notation>H</skos:notation>
    <skos:prefLabel>Historic</skos:prefLabel>
    <skos:scopeNote>Valid/used in the past but not currently</skos:scopeNote>
    <skos:example>"Lutetia" is a historic name for "Paris" (TGN). "weyneschot" is a 16th-century spelling for "wainscoting" (AAT)</skos:example>
    <dct:description>Valid/used in the past but not currently.
Example: "Lutetia" is a historic name for "Paris" (TGN). "weyneschot" is a 16th-century spelling for "wainscoting" (AAT)</dct:description>
  </skos:Concept>
  <skos:Concept rdf:about="http://vocab.getty.edu/term/kind/ProvisionalName">
    <skos:inScheme rdf:resource="http://vocab.getty.edu/term/kind/"/>
    <skos:notation>PN</skos:notation>
    <skos:prefLabel>Provisional Name</skos:prefLabel>
    <skos:scopeNote>Used in TGN only</skos:scopeNote>
    <skos:example>"Rockton" was provisional name considered before adoption of "Kent" (Ohio)</skos:example>
    <dct:description>Used in TGN only.
Example: "Rockton" was provisional name considered before adoption of "Kent" (Ohio)</dct:description>
  </skos:Concept>
  <skos:Concept rdf:about="http://vocab.getty.edu/term/kind/Code">
    <skos:inScheme rdf:resource="http://vocab.getty.edu/term/kind/"/>
    <skos:notation>79000</skos:notation>
    <skos:prefLabel>Code</skos:prefLabel>
    <skos:scopeNote>Code, similar to Abbreviation</skos:scopeNote>
    <skos:example>"sq yds", "m2"</skos:example>
    <dct:description>Code, similar to Abbreviation.
Example: "sq yds", "m2"</dct:description>
  </skos:Concept>
  <skos:Concept rdf:about="http://vocab.getty.edu/term/flag/Vernacular">
    <skos:inScheme>
      <skos:ConceptScheme rdf:about="http://vocab.getty.edu/term/flag/">
        <rdfs:isDefinedBy rdf:resource="http://vocab.getty.edu/ontology"/>
        <rdfs:label>Term Flag concept scheme</rdfs:label>
        <dct:description>Term Flag concept scheme</dct:description>
      </skos:ConceptScheme>
    </skos:inScheme>
    <skos:notation>V</skos:notation>
    <skos:prefLabel>Vernacular</skos:prefLabel>
    <skos:scopeNote>Term is the vernacular for a certain place</skos:scopeNote>
    <skos:example>"kachoga" is the Vernacular for 300266169 "bird-and-flower paintings" (AAT). "Firenze" is the vernacular in Italian (TGN)</skos:example>
    <dct:description>Term is the vernacular for a certain place.
Example: "kachoga" is the Vernacular for 300266169 "bird-and-flower paintings" (AAT). "Firenze" is the vernacular in Italian (TGN)</dct:description>
  </skos:Concept>
  <skos:Concept rdf:about="http://vocab.getty.edu/term/POS/BothSingularAndPlural">
    <skos:inScheme rdf:resource="http://vocab.getty.edu/term/POS/"/>
    <skos:notation>B</skos:notation>
    <skos:prefLabel>Both Singular and Plural</skos:prefLabel>
    <skos:scopeNote>A term that is used for both the singular and plural in the same language</skos:scopeNote>
    <skos:example>"chassis" is both singular and plural in French</skos:example>
    <dct:description>A term that is used for both the singular and plural in the same language.
Example: "chassis" is both singular and plural in French</dct:description>
  </skos:Concept>
  <skos:Concept rdf:about="http://vocab.getty.edu/term/kind/FullName">
    <skos:inScheme rdf:resource="http://vocab.getty.edu/term/kind/"/>
    <skos:notation>FN</skos:notation>
    <skos:prefLabel>Full Name</skos:prefLabel>
    <skos:scopeNote>Full Name of an ULAN agent</skos:scopeNote>
    <skos:example>TODO</skos:example>
    <dct:description>Full Name of an ULAN agent.
Example: TODO</dct:description>
  </skos:Concept>
  <skos:Concept rdf:about="http://vocab.getty.edu/term/POS/PluralNoun">
    <skos:inScheme rdf:resource="http://vocab.getty.edu/term/POS/"/>
    <skos:notation>PN</skos:notation>
    <skos:prefLabel>Plural Noun</skos:prefLabel>
    <skos:scopeNote>A term that is plural (the same word may be singular in another language)</skos:scopeNote>
    <skos:example>"filigrane" is the Italian plural for "watermarks"</skos:example>
    <dct:description>A term that is plural (the same word may be singular in another language).
Example: "filigrane" is the Italian plural for "watermarks"</dct:description>
  </skos:Concept>
  <ptop:PropRestr rdf:about="http://vocab.getty.edu/ontology#Infer_isoBroaderInstantial">
    <ptop:premise rdf:resource="http://vocab.getty.edu/ontology#broaderInstantialExtended"/>
    <ptop:restriction rdf:resource="http://www.w3.org/2004/02/skos/core#broader"/>
    <ptop:conclusion rdf:resource="http://purl.org/iso25964/skos-thes#broaderInstantial"/>
  </ptop:PropRestr>
  <rdf:Description rdf:about="http://www.w3.org/2004/02/skos/core#altLabel">
    <owl:propertyChainAxiom rdf:parseType="Collection">
      <rdf:Description rdf:about="http://www.w3.org/2008/05/skos-xl#altLabel"/>
      <rdf:Description rdf:about="http://www.w3.org/2008/05/skos-xl#literalForm"/>
    </owl:propertyChainAxiom>
  </rdf:Description>
  <skos:Concept rdf:about="http://vocab.getty.edu/term/flag/LiteralTranslation">
    <skos:inScheme rdf:resource="http://vocab.getty.edu/term/flag/"/>
    <skos:notation>T</skos:notation>
    <skos:prefLabel>Literal Translation</skos:prefLabel>
    <skos:scopeNote>Literal translation of a name.  Defined for ULAN, but currently there are no examples of this</skos:scopeNote>
    <dct:description>Literal translation of a name.  Defined for ULAN, but currently there are no examples of this</dct:description>
  </skos:Concept>
  <skos:Concept rdf:about="http://vocab.getty.edu/historic/localUse">
    <skos:inScheme rdf:resource="http://vocab.getty.edu/historic/"/>
    <skos:notation>LU</skos:notation>
    <skos:prefLabel>Local Use</skos:prefLabel>
    <skos:scopeNote>Used locally for Unidentified Named People mentioned in some document (ULAN only)</skos:scopeNote>
    <skos:example>500051176 Abinetti (ULAN) is an unknown artist mentioned in documentation of lot 209 of an auction held 29 Jan 1824 in London</skos:example>
    <dct:description>Used locally for Unidentified Named People mentioned in some document (ULAN only).
Example: 500051176 Abinetti (ULAN) is an unknown artist mentioned in documentation of lot 209 of an auction held 29 Jan 1824 in London</dct:description>
  </skos:Concept>
  <skos:Concept rdf:about="http://vocab.getty.edu/term/kind/CommonName">
    <skos:inScheme rdf:resource="http://vocab.getty.edu/term/kind/"/>
    <skos:notation>CN</skos:notation>
    <skos:prefLabel>Common Name</skos:prefLabel>
    <skos:scopeNote>Common Name of an ULAN agent</skos:scopeNote>
    <skos:example>TODO</skos:example>
    <dct:description>Common Name of an ULAN agent.
Example: TODO</dct:description>
  </skos:Concept>
  <skos:Concept rdf:about="http://vocab.getty.edu/term/flag/LoanTerm">
    <skos:inScheme rdf:resource="http://vocab.getty.edu/term/flag/"/>
    <skos:notation>L</skos:notation>
    <skos:prefLabel>Loan Term</skos:prefLabel>
    <skos:scopeNote>Term borrowed from another language that has become naturalized in American English</skos:scopeNote>
    <skos:example>papier mache</skos:example>
    <dct:description>Term borrowed from another language that has become naturalized in American English.
Example: papier mache</dct:description>
  </skos:Concept>
  <skos:Concept rdf:about="http://vocab.getty.edu/term/kind/JargonOrSlang">
    <skos:inScheme rdf:resource="http://vocab.getty.edu/term/kind/"/>
    <skos:notation>J</skos:notation>
    <skos:prefLabel>Jargon or Slang</skos:prefLabel>
    <skos:scopeNote>Slang or jargon term. Used in AAT only</skos:scopeNote>
    <skos:example>"fool's gold" is slang for "pyrite"</skos:example>
    <dct:description>Slang or jargon term. Used in AAT only.
Example: "fool's gold" is slang for "pyrite"</dct:description>
  </skos:Concept>
  <skos:Concept rdf:about="http://vocab.getty.edu/term/type/Descriptor">
    <skos:inScheme rdf:resource="http://vocab.getty.edu/term/type/"/>
    <skos:notation>D</skos:notation>
    <skos:prefLabel>Descriptor</skos:prefLabel>
    <skos:scopeNote>Main term. Getty usually uses the plural</skos:scopeNote>
    <skos:example>"manuscripts" (English)</skos:example>
    <dct:description>Main term. Getty usually uses the plural.
Example: "manuscripts" (English)</dct:description>
  </skos:Concept>
  <skos:Concept rdf:about="http://vocab.getty.edu/term/POS/PastParticiple">
    <skos:inScheme rdf:resource="http://vocab.getty.edu/term/POS/"/>
    <skos:notation>PP</skos:notation>
    <skos:prefLabel>Past Participle</skos:prefLabel>
    <skos:scopeNote>Rarely used but if at all, is most likely to apply in Attributes and Properties</skos:scopeNote>
    <skos:example>hand-painted</skos:example>
    <dct:description>Rarely used but if at all, is most likely to apply in Attributes and Properties.
Example: hand-painted</dct:description>
  </skos:Concept>
</rdf:RDF>
