<?xml version="1.0"?>
<rdf:RDF xmlns:pns="http://data.press.net/ontology/stuff/" xmlns:geo="http://www.w3.org/2003/01/geo/wgs84_pos#" xmlns:dcterms="http://purl.org/dc/terms/" xmlns:foaf="http://xmlns.com/foaf/0.1/" xmlns:vs="http://www.w3.org/2003/06/sw-vocab-status/ns#" xmlns:owl="http://www.w3.org/2002/07/owl#" xmlns:xsd="http://www.w3.org/2001/XMLSchema#" xmlns:time="http://www.w3.org/2006/time#" xmlns:pni="http://data.press.net/ontology/identifier/" xmlns:rdfs="http://www.w3.org/2000/01/rdf-schema#" xmlns:pnt="http://data.press.net/ontology/tag/" xmlns:rdf="http://www.w3.org/1999/02/22-rdf-syntax-ns#" xmlns:pna="http://data.press.net/ontology/asset/">
    <owl:Ontology rdf:about="http://data.press.net/ontology/stuff/">
        <dcterms:title xml:lang="en">SNaP Stuff Ontology</dcterms:title>
        <dcterms:created rdf:datatype="http://www.w3.org/2001/XMLSchema#date">2011-07-28</dcterms:created>
        <dcterms:modified rdf:datatype="http://www.w3.org/2001/XMLSchema#date">2012-06-18</dcterms:modified>
        <dcterms:license rdf:resource="http://creativecommons.org/licenses/by-nd/3.0/" />
        <rdfs:comment xml:lang="en">The Stuff Ontology models real world entities. There are two kinds of stuff: tangibles and intangibles. Tangible stuff includes persons, locations and organizations. Intangibles are abstract concepts such as smoking, feminism or love.</rdfs:comment>
        <foaf:maker>
            <foaf:Person rdf:about="http://uk.linkedin.com/in/paulwilton">
                <foaf:name>Paul Wilton</foaf:name>
            </foaf:Person>
        </foaf:maker>
        <foaf:maker>
            <foaf:Person rdf:about="http://uk.linkedin.com/in/pauliharman">
                <foaf:name>Paul Harman</foaf:name>
            </foaf:Person>
        </foaf:maker>
        <foaf:maker>
            <foaf:Person rdf:about="http://uk.linkedin.com/in/jarredmcginnis">
                <foaf:name>Jarred McGinnis</foaf:name>
            </foaf:Person>
        </foaf:maker>
        <owl:versionInfo rdf:datatype="http://www.w3.org/2001/XMLSchema#string">0.4.1</owl:versionInfo>
    </owl:Ontology>
    <owl:Class rdf:about="http://data.press.net/ontology/stuff/Stuff">
        <rdfs:label xml:lang="en">Generic Stuff Class</rdfs:label>
        <rdfs:comment xml:lang="en">Generic Stuff Class  - a base class for all domain stuff</rdfs:comment>
        <rdfs:subClassOf rdf:resource="http://data.press.net/ontology/tag/Tag" />
        <rdfs:subClassOf rdf:resource="http://data.press.net/ontology/identifier/Identifiable" />
        <rdfs:isDefinedBy rdf:resource="http://data.press.net/ontology/stuff/" />
        <vs:term_status>testing</vs:term_status>
    </owl:Class>
    <owl:Class rdf:about="http://data.press.net/ontology/stuff/Tangible">
        <rdfs:subClassOf rdf:resource="http://data.press.net/ontology/stuff/Stuff" />
        <rdfs:label xml:lang="en">A base Class for Tangible Stuff</rdfs:label>
        <rdfs:comment xml:lang="en">A base class for all tangible stuff (eg people, places, physical things)</rdfs:comment>
        <rdfs:isDefinedBy rdf:resource="http://data.press.net/ontology/stuff/" />
        <vs:term_status>testing</vs:term_status>
    </owl:Class>
    <owl:Class rdf:about="http://data.press.net/ontology/stuff/Intangible">
        <rdfs:subClassOf rdf:resource="http://data.press.net/ontology/stuff/Stuff" />
        <rdfs:label xml:lang="en">A base class for Intangible Stuff</rdfs:label>
        <rdfs:comment xml:lang="en">A base class for all intangible stuff (eg love, conservatism, fashion)</rdfs:comment>
        <rdfs:isDefinedBy rdf:resource="http://data.press.net/ontology/stuff/" />
        <vs:term_status>testing</vs:term_status>
    </owl:Class>
    <owl:Class rdf:about="http://data.press.net/ontology/stuff/Person">
        <rdfs:subClassOf rdf:resource="http://data.press.net/ontology/stuff/Tangible" />
        <rdfs:subClassOf rdf:resource="http://xmlns.com/foaf/0.1/Person" />
        <rdfs:label xml:lang="en">A Person - a base class for people instances.</rdfs:label>
        <rdfs:comment xml:lang="en">A Person - a base class for people instances. Also a subclass of foaf:Person</rdfs:comment>
        <rdfs:isDefinedBy rdf:resource="http://data.press.net/ontology/stuff/" />
        <vs:term_status>testing</vs:term_status>
    </owl:Class>
    <owl:Class rdf:about="http://data.press.net/ontology/stuff/Organization">
        <rdfs:subClassOf rdf:resource="http://data.press.net/ontology/stuff/Tangible" />
        <rdfs:subClassOf rdf:resource="http://xmlns.com/foaf/0.1/Organization" />
        <rdfs:label xml:lang="en">An Organization - a base class for instances of organizations</rdfs:label>
        <rdfs:comment xml:lang="en">An Organization - a base class for instances of organizations. Also a subclass of foaf:Organization</rdfs:comment>
        <rdfs:isDefinedBy rdf:resource="http://data.press.net/ontology/stuff/" />
        <vs:term_status>testing</vs:term_status>
    </owl:Class>
    <owl:Class rdf:about="http://data.press.net/ontology/stuff/Location">
        <rdfs:subClassOf rdf:resource="http://data.press.net/ontology/stuff/Tangible" />
        <rdfs:subClassOf rdf:resource="http://www.w3.org/2003/01/geo/wgs84_pos#SpatialThing" />
        <rdfs:label xml:lang="en">A Location - a base class for Locations</rdfs:label>
        <rdfs:comment xml:lang="en">A Location - a base class for Locations. Also a subclass of geo:SpatialThing</rdfs:comment>
        <rdfs:isDefinedBy rdf:resource="http://data.press.net/ontology/stuff/" />
        <vs:term_status>testing</vs:term_status>
    </owl:Class>
    <owl:DatatypeProperty rdf:about="http://data.press.net/ontology/stuff/label">
        <rdfs:subPropertyOf rdf:resource="http://www.w3.org/2000/01/rdf-schema#label" />
        <rdfs:domain rdf:resource="http://data.press.net/ontology/stuff/Stuff" />
        <rdfs:range rdf:resource="http://www.w3.org/2001/XMLSchema#string" />
        <rdfs:label xml:lang="en">The definitive label of a Stuff instance</rdfs:label>
        <rdfs:comment xml:lang="en">String property that indicates the definitive label of a Stuff instance. This might be the full name of a Person, Organization or something Intangible</rdfs:comment>
        <rdfs:isDefinedBy rdf:resource="http://data.press.net/ontology/stuff/" />
        <vs:term_status>testing</vs:term_status>
    </owl:DatatypeProperty>
    <owl:DatatypeProperty rdf:about="http://data.press.net/ontology/stuff/alias">
        <rdfs:subPropertyOf rdf:resource="http://www.w3.org/2000/01/rdf-schema#label" />
        <rdfs:domain rdf:resource="http://data.press.net/ontology/stuff/Stuff" />
        <rdfs:range rdf:resource="http://www.w3.org/2001/XMLSchema#string" />
        <rdfs:label xml:lang="en">An alias label of a Stuff instance</rdfs:label>
        <rdfs:comment xml:lang="en">String property that indicates an alias of a Stuff instance. For example 'Television' might have an alias of 'TV'.</rdfs:comment>
        <rdfs:isDefinedBy rdf:resource="http://data.press.net/ontology/stuff/" />
        <vs:term_status>testing</vs:term_status>
    </owl:DatatypeProperty>
    <owl:DatatypeProperty rdf:about="http://data.press.net/ontology/stuff/comment">
        <rdfs:subPropertyOf rdf:resource="http://www.w3.org/2000/01/rdf-schema#comment" />
        <rdfs:domain rdf:resource="http://data.press.net/ontology/stuff/Stuff" />
        <rdfs:range rdf:resource="http://www.w3.org/2001/XMLSchema#string" />
        <rdfs:label xml:lang="en">The definitive description of a Stuff instance</rdfs:label>
        <rdfs:comment xml:lang="en">String property that indicates the definitive description of a Stuff instance.</rdfs:comment>
        <rdfs:isDefinedBy rdf:resource="http://data.press.net/ontology/stuff/" />
        <vs:term_status>testing</vs:term_status>
    </owl:DatatypeProperty>
    <owl:DatatypeProperty rdf:about="http://data.press.net/ontology/stuff/name">
        <rdfs:subPropertyOf rdf:resource="http://data.press.net/ontology/stuff/label" />
        <rdfs:subPropertyOf rdf:resource="http://xmlns.com/foaf/0.1/name" />
        <rdfs:domain rdf:resource="http://xmlns.com/foaf/0.1/Agent" />
        <rdfs:range rdf:resource="http://www.w3.org/2001/XMLSchema#string" />
        <rdfs:label xml:lang="en">The definitive name of a Person or Organization</rdfs:label>
        <rdfs:comment xml:lang="en">String property that indicates the definitive full name of a Person or Organization via foaf:Agent. Also infers Stuff label via pns:label</rdfs:comment>
        <rdfs:isDefinedBy rdf:resource="http://data.press.net/ontology/stuff/" />
        <vs:term_status>testing</vs:term_status>
    </owl:DatatypeProperty>
    <owl:DatatypeProperty rdf:about="http://data.press.net/ontology/stuff/shortName">
        <rdfs:subPropertyOf rdf:resource="http://data.press.net/ontology/stuff/label" />
        <rdfs:domain rdf:resource="http://xmlns.com/foaf/0.1/Agent" />
        <rdfs:range rdf:resource="http://www.w3.org/2001/XMLSchema#string" />
        <rdfs:label xml:lang="en">A short name of a Person or Organization</rdfs:label>
        <rdfs:comment xml:lang="en">String property that indicates the short name of a Person or Organization via foaf:Agent. Also infers Stuff label via pns:label. For example 'Man Utd'</rdfs:comment>
        <rdfs:isDefinedBy rdf:resource="http://data.press.net/ontology/stuff/" />
        <vs:term_status>testing</vs:term_status>
    </owl:DatatypeProperty>
    <owl:DatatypeProperty rdf:about="http://data.press.net/ontology/stuff/longName">
        <rdfs:subPropertyOf rdf:resource="http://data.press.net/ontology/stuff/label" />
        <rdfs:domain rdf:resource="http://xmlns.com/foaf/0.1/Agent" />
        <rdfs:range rdf:resource="http://www.w3.org/2001/XMLSchema#string" />
        <rdfs:label xml:lang="en">A long name of a Person or Organization</rdfs:label>
        <rdfs:comment xml:lang="en">String property that indicates the long name of a Person or Organization via foaf:Agent. Also infers Stuff label via pns:label. For example 'Manchester United F.C.'</rdfs:comment>
        <rdfs:isDefinedBy rdf:resource="http://data.press.net/ontology/stuff/" />
        <vs:term_status>testing</vs:term_status>
    </owl:DatatypeProperty>
    <owl:ObjectProperty rdf:about="http://data.press.net/ontology/stuff/hasImage">
        <rdfs:subPropertyOf>
            <owl:ObjectProperty rdf:about="http://data.press.net/ontology/stuff/hasAsset">
                <rdfs:domain rdf:resource="http://data.press.net/ontology/stuff/Stuff" />
                <rdfs:range rdf:resource="http://data.press.net/ontology/asset/Asset" />
                <rdfs:label xml:lang="en">Property that associates assets directly with domain entities.</rdfs:label>
                <rdfs:comment xml:lang="en">Property that associates assets directly with domain entities, e.g. official biography, corporate logo</rdfs:comment>
                <rdfs:isDefinedBy rdf:resource="http://data.press.net/ontology/stuff/" />
                <vs:term_status>testing</vs:term_status>
            </owl:ObjectProperty>
        </rdfs:subPropertyOf>
        <rdfs:domain rdf:resource="http://data.press.net/ontology/stuff/Stuff" />
        <rdfs:range rdf:resource="http://data.press.net/ontology/asset/Image" />
        <rdfs:label xml:lang="en">Property that associates images with domain entities.</rdfs:label>
        <rdfs:comment xml:lang="en">Property that associates images with domain entities, e.g. official photograph, corporate logo</rdfs:comment>
        <rdfs:isDefinedBy rdf:resource="http://data.press.net/ontology/stuff/" />
        <vs:term_status>testing</vs:term_status>
    </owl:ObjectProperty>
    <owl:ObjectProperty rdf:about="http://data.press.net/ontology/stuff/placeOfBirth">
        <rdfs:subPropertyOf>
            <owl:ObjectProperty rdf:about="http://data.press.net/ontology/stuff/notablyAssociatedWith">
                <rdfs:domain rdf:resource="http://data.press.net/ontology/stuff/Stuff" />
                <rdfs:range rdf:resource="http://data.press.net/ontology/stuff/Stuff" />
                <rdfs:comment xml:lang="en">Property that notably associates stuff together, for example Karl Lagerfeld is notably associated with Fashion</rdfs:comment>
                <rdfs:label xml:lang="en">Property that notably associates stuff together</rdfs:label>
                <rdfs:isDefinedBy rdf:resource="http://data.press.net/ontology/stuff/" />
                <vs:term_status>testing</vs:term_status>
            </owl:ObjectProperty>
        </rdfs:subPropertyOf>
        <rdfs:domain rdf:resource="http://data.press.net/ontology/stuff/Person" />
        <rdfs:range rdf:resource="http://data.press.net/ontology/stuff/Location" />
        <rdfs:comment xml:lang="en">Property of a Person. A person's place of birth</rdfs:comment>
        <rdfs:label xml:lang="en">A person's place of birth</rdfs:label>
        <rdfs:isDefinedBy rdf:resource="http://data.press.net/ontology/stuff/" />
        <vs:term_status>testing</vs:term_status>
    </owl:ObjectProperty>
    <owl:ObjectProperty rdf:about="http://data.press.net/ontology/stuff/dateOfBirth">
        <rdfs:domain rdf:resource="http://data.press.net/ontology/stuff/Person" />
        <rdfs:range rdf:resource="http://www.w3.org/2006/time#Instant" />
        <rdfs:comment xml:lang="en">Property of a Person. A person's date of birth</rdfs:comment>
        <rdfs:label xml:lang="en">A person's date of birth</rdfs:label>
        <rdfs:isDefinedBy rdf:resource="http://data.press.net/ontology/stuff/" />
        <vs:term_status>testing</vs:term_status>
    </owl:ObjectProperty>
    <owl:ObjectProperty rdf:about="http://data.press.net/ontology/stuff/dateOfDeath">
        <rdfs:domain rdf:resource="http://data.press.net/ontology/stuff/Person" />
        <rdfs:range rdf:resource="http://www.w3.org/2006/time#Instant" />
        <rdfs:comment xml:lang="en">Property of a Person. A person's date of death</rdfs:comment>
        <rdfs:label xml:lang="en">A person's date of death</rdfs:label>
        <rdfs:isDefinedBy rdf:resource="http://data.press.net/ontology/stuff/" />
        <vs:term_status>testing</vs:term_status>
    </owl:ObjectProperty>
    <owl:TransitiveProperty rdf:about="http://data.press.net/ontology/stuff/parentLocation">
        <rdfs:domain rdf:resource="http://data.press.net/ontology/stuff/Location" />
        <rdfs:range rdf:resource="http://data.press.net/ontology/stuff/Location" />
        <rdfs:comment xml:lang="en">Property of a Location. References the parent location of this location</rdfs:comment>
        <rdfs:label xml:lang="en">A parent location</rdfs:label>
        <rdfs:isDefinedBy rdf:resource="http://data.press.net/ontology/stuff/" />
        <vs:term_status>testing</vs:term_status>
    </owl:TransitiveProperty>
</rdf:RDF>