<?xml version="1.0" encoding="utf-8"?>
<!DOCTYPE rdf:RDF [
  <!ENTITY xsd     "http://www.w3.org/2001/XMLSchema#">
  <!ENTITY rdf     "http://www.w3.org/1999/02/22-rdf-syntax-ns#">
  <!ENTITY rdfs    "http://www.w3.org/2000/01/rdf-schema#">
  <!ENTITY owl     "http://www.w3.org/2002/07/owl#">
  <!ENTITY dcterms "http://purl.org/dc/terms/">
  <!ENTITY dcDoc   "dublincore.org/documents/dcmi-terms/">
  <!ENTITY foaf    "http://xmlns.com/foaf/0.1/">
  <!ENTITY sioc    "http://rdfs.org/sioc/ns#">
  <!ENTITY schema  "http://schema.org/">
  <!ENTITY cc      "http://creativecommons.org/ns#">
  <!ENTITY skos    "http://www.w3.org/2004/02/skos/core#">
  <!ENTITY skosDoc "http://www.w3.org/TR/skos-primer/">
  <!ENTITY dcat    "http://www.w3.org/ns/dcat#">
  <!ENTITY xhv     "http://www.w3.org/1999/xhtml/vocab#">
  <!ENTITY wdrs    "http://www.w3.org/2007/05/powder-s#">
  <!ENTITY vann    "http://purl.org/vocab/vann/">
  <!ENTITY rad    "http://www.w3.org/ns/radion#">
  <!ENTITY documentation "https://joinup.ec.europa.eu/asset/radion/description">
  <!ENTITY documentationTitle "RADion RDF Schema">
  <!ENTITY methodology "https://joinup.ec.europa.eu/elibrary/document/isa-deliverable-process-and-methodology-developing-core-vocabularies">
  <!ENTITY methodologyTitle "Process and Methodology for Developing Core Vocabularies">
  <!ENTITY forum "http://joinup.ec.europa.eu/asset/radion/forum/all">
  <!ENTITY forumTitle "Public comments on RADion">
]>

<rdf:RDF xmlns:xsd     = "&xsd;"
         xmlns:rdf     = "&rdf;"
         xmlns:rdfs    = "&rdfs;"
         xmlns:owl     = "&owl;"
         xmlns:dcterms = "&dcterms;"
         xmlns:foaf    = "&foaf;"
         xmlns:sioc    = "&sioc;"
         xmlns:schema  = "&schema;"
         xmlns:cc      = "&cc;"
         xmlns:skos    = "&skos;"
         xmlns:dcat    = "&dcat;"
         xmlns:xhv     = "&xhv;"
         xmlns:wdrs    = "&wdrs;"
         xmlns:vann    = "&vann;"
         xmlns         = "&rad;"
         xml:base      = "&rad;"
         xml:lang = "en">

<!-- Document metadata -->

  <owl:Ontology rdf:about="&rad;">
    <rdfs:label xml:lang="en">Repository Asset Distribution (RADion)</rdfs:label>
    <rdfs:comment xml:lang="en">This file specifies the set of RDF classes and properties used in RADion</rdfs:comment>
    <owl:versionInfo xml:lang="en">Version 1.2 11 October 2012</owl:versionInfo>
    <dcterms:modified rdf:datatype="&xsd;date">2012-10-11</dcterms:modified>
    <xhv:last rdf:resource="&rad;"/>
<!--    
    <xhv:prev rdf:resource=""/>
    <xhv:next rdf:resource=""/>
-->    
    <vann:preferredNamespaceUri>&rad;</vann:preferredNamespaceUri>
    <vann:preferredNamespacePrefix>radion</vann:preferredNamespacePrefix>
    <dcterms:creator rdf:parseType="Resource">
      <rdfs:seeAlso rdf:resource="http://makxdekkers.com/makxdekkers.rdf#me"/>
      <foaf:name>Makx Dekkers</foaf:name>
      <foaf:homepage rdf:resource="http://makxdekkers.com/"/>
    </dcterms:creator>
    <dcterms:creator rdf:parseType="Resource">
      <rdfs:seeAlso rdf:resource="http://andrea-perego.name/foaf/#me"/>
      <foaf:name>Andrea Perego</foaf:name>
      <foaf:homepage rdf:resource="http://andrea-perego.name/"/>
      <schema:affiliation rdf:parseType="Resource">
        <foaf:name>European Commission, JRC-IES</foaf:name>
      </schema:affiliation>
    </dcterms:creator>
    <dcterms:creator rdf:parseType="Resource">
      <rdfs:seeAlso rdf:resource="http://philarcher.org/foaf.rdf#me"/>
      <foaf:name>Phil Archer</foaf:name>
      <foaf:homepage rdf:resource="http://philarcher.org/"/>
      <schema:affiliation rdf:parseType="Resource">
        <foaf:name>W3C/ERCIM</foaf:name>
      </schema:affiliation>
    </dcterms:creator>
    <foaf:maker rdf:parseType="Resource">
      <foaf:name>ADMS Working Group</foaf:name>
      <foaf:page rdf:resource="http://joinup.ec.europa.eu/asset/adms/home"/>
    </foaf:maker>
    <dcterms:description rdf:parseType="Literal"><p>The Repository Asset Distribution (RADion) was developed under the European 
          Commission's <a href="http://ec.europa.eu/isa/">ISA Programme</a>. More information is available from the European Commission's
          <a href="http://joinup.ec.europa.eu/asset/radion/description">Joinup portal</a>. This includes background information,
          use cases, the conceptual model and full definitions for all terms used.</p> 
    </dcterms:description>
    <dcterms:abstract>RADion, and the higher level vocabularies that build upon it, are 
    intended as a model that facilitates federation 
    and co-operation. It is not the primary intention that repository owners 
    redesign or convert their current systems and data to conform to RADion, but 
    rather that it acts as a common layer among repositories that want to 
    exchange data.
    </dcterms:abstract>
    <wdrs:describedby>
      <rdf:Description rdf:about="&documentation;">
        <dcterms:title>&documentationTitle;</dcterms:title>
      </rdf:Description>
    </wdrs:describedby>
    <dcterms:conformsTo>
      <rdf:Description rdf:about="&methodology;">
        <dcterms:title>&methodologyTitle;</dcterms:title>
      </rdf:Description>
    </dcterms:conformsTo>
    <dcterms:relation>
      <sioc:Forum rdf:about="&forum;">
        <dcterms:title>&forumTitle;</dcterms:title>
      </sioc:Forum>
    </dcterms:relation>
    <dcterms:rights>Copyright &#169; 2012 European Commission.</dcterms:rights>
    <dcterms:license>
      <rdf:Description rdf:about="https://joinup.ec.europa.eu/category/licence/isa-open-metadata-licence-v11">
        <dcterms:title>ISA Open Metadata Licence v1.1</dcterms:title>
        <cc:attributionName>European Commission</cc:attributionName>
        <cc:attributionURL rdf:resource="http://ec.europa.eu/"/>
      </rdf:Description>
    </dcterms:license>
    <cc:attributionName>European Commission</cc:attributionName>
    <cc:attributionURL rdf:resource="http://ec.europa.eu/"/>
  </owl:Ontology>  

<!-- The three primary classes -->

  <rdfs:Class rdf:about="&rad;Repository">
    <rdfs:label xml:lang="en">Repository</rdfs:label>
    <rdfs:comment xml:lang="en">A Repository is a system or service that provides facilities for storage and 
    maintenance of descriptions of Assets and Distributions. A Repository will typically contain descriptions 
    of several Assets and functionality that allows users to search and access these descriptions. The 
    Distributions - the actual files themselves - will typically be available from the Repository or 
    elsewhere on the World Wide Web.</rdfs:comment>
    <rdfs:isDefinedBy rdf:resource="&documentation;" />
    <dcterms:identifier>rad:Repository</dcterms:identifier>
  </rdfs:Class>
 
  <rdf:Description rdf:about="&rad;Asset">
    <rdfs:label xml:lang="en">Asset</rdfs:label>
    <rdfs:comment xml:lang="en">An Asset represents the conceptual content of a resource. A particular 
    Asset may have zero or more Distributions in different formats.</rdfs:comment>
    <rdfs:isDefinedBy rdf:resource="&documentation;" />
    <dcterms:identifier>rad:Asset</dcterms:identifier>
  </rdf:Description>

  <rdfs:Class rdf:about="&rad;Distribution">
    <rdfs:label xml:lang="en">Distribution</rdfs:label>
    <rdfs:comment xml:lang="en">A Distribution is a particular representation or concretisation of an 
    Asset in the form of a downloadable computer file that implements the intellectual content of an 
    Asset. A particular Distribution is typically associated with one Asset.</rdfs:comment>
    <rdfs:isDefinedBy rdf:resource="&documentation;" />
    <dcterms:identifier>rad:Distribution</dcterms:identifier>
  </rdfs:Class>

<!-- Secondary classes -->

  <rdf:Description rdf:about="&dcterms;Agent">
    <rdfs:label xml:lang="en">Agent</rdfs:label>
    <rdfs:comment xml:lang="en">A resource that acts or has the power to act.</rdfs:comment>
    <vann:usageNote xml:lang="en">The dcterms:Agent class (or a sub class of it) is used in RADion to represent the publisher of a Repository or its components.</vann:usageNote>
    <rdfs:isDefinedBy rdf:resource="&dcterms;" />
    <dcterms:identifier>dcterms:Agent</dcterms:identifier>
  </rdf:Description>

  <rdf:Description rdf:about="&dcterms;Location">
    <rdfs:label xml:lang="en">Location</rdfs:label>
    <rdfs:comment xml:lang="en">The dcterms:Location class fully represents the RADion class of Geographic Coverage.</rdfs:comment>
    <vann:usageNote xml:lang="en" rdf:parseType="Literal">The <a href="https://joinup.ec.europa.eu/asset/core_location/description">Location Core Vocabulary</a> also uses dcterms:Location.</vann:usageNote>
    <rdfs:isDefinedBy rdf:resource="&dcDoc;" />
    <dcterms:identifier>dcterms:Location</dcterms:identifier>
  </rdf:Description>

  <rdf:Description rdf:about="&dcterms;LinguisticSystem">
    <rdfs:label xml:lang="en">Language</rdfs:label>
    <rdfs:comment xml:lang="en">The dcterms:LinguisticSystem class fully represents the RADion concept of Language.</rdfs:comment>
    <vann:usageNote xml:lang="en">Used in RADion to provide the language of textual information within an Asset, e.g. the language of the terms in a controlled vocabulary (ideally the set of tags defined by RFC 3066 ) or the language that a specification is written in.</vann:usageNote>
    <rdfs:isDefinedBy rdf:resource="&dcterms;" />
    <dcterms:identifier>dcterms:LinguisticSystem</dcterms:identifier>
  </rdf:Description>

  <rdf:Description rdf:about="&dcterms;FileFormat">
    <rdfs:label xml:lang="en">File Format</rdfs:label>
    <rdfs:comment xml:lang="en">The dcterms:FileFormat class fully represents the RADion concept of a file format.</rdfs:comment>
    <vann:usageNote xml:lang="en">Used in RADion to provide the technical format that a Distribution is available in, e.g. PDF for a document, XML for a schema.</vann:usageNote>
    <rdfs:isDefinedBy rdf:resource="&dcterms;" />
    <dcterms:identifier>dcterms:FileFormat</dcterms:identifier>
  </rdf:Description>

  <rdf:Description rdf:about="&dcterms;LicenseDocument">
    <rdfs:label xml:lang="en">License</rdfs:label>
    <rdfs:comment xml:lang="en">The dcterms:LicenseDocument class fully represents the RADion concept of a Licence</rdfs:comment>
    <vann:usageNote xml:lang="en">Used in RADion to provide the conditions or restrictions that apply to the use of a Distribution, e.g. whether it is in the public domain, or that some restrictions apply like in cases attribution is required, or the Asset can only be used for non-commercial purposes etc.</vann:usageNote>
    <rdfs:isDefinedBy rdf:resource="&dcterms;" />
    <dcterms:identifier>dcterms:LicenseDocument</dcterms:identifier>
  </rdf:Description>

<!-- "Data types" -->

  <rdf:Description rdf:about="&rdfs;Literal">
    <rdfs:label xml:lang="en">string, URI, dateTime, text</rdfs:label>
    <rdfs:comment xml:lang="en">At the conceptual level, the rdfs:Literal datatype fully represents the RADion datatypes of 
    a string (an untyped literal) and text (string plus language tag). The RADion datatype of 
    dateTime is also served since that requires a string conformant with ISO 8601:2004 which is 
    true of all relevant xsd datatypes. Likewise a Literal datatyped as xsd:anyURI will fulfil 
    the needs of RADion's URI data type.</rdfs:comment>
    <rdfs:isDefinedBy rdf:resource="&rdfs;" />
    <dcterms:identifier>rdfs:Literal</dcterms:identifier>
  </rdf:Description>

  <rdf:Description rdf:about="&skos;Concept"> 
    <rdfs:label xml:lang="en">Code</rdfs:label>
    <rdfs:comment rdf:parseType="Literal"><p>The Conceptual Model includes a 'Code' datatype that 
      is used by several classes. This is expressed using the <a href="&skosDoc;">SKOS vocabulary</a> with
      a particular 'code' usually being a skos:Concept that is part of a scheme. 
      The intention is that the skos:Concept class be used as follows;</p><ul>
      <li>for the content property, use skos:notation</li>
      <li>the 'list' property will be taken care of by means of the skos:inScheme property;</li>
      <li>the list agency property is likely to be applied to the scheme as a whole for which dcterms:creator is appropriate;</li>
      <li>the list version property can be fulfilled using schema:version (see <a href="http://schema.org/CreativeWork">http://schema.org/CreativeWork</a>)</li></ul>
    </rdfs:comment>
    <rdfs:isDefinedBy rdf:resource="&skosDoc;" />
    <dcterms:identifier>skos:Concept</dcterms:identifier>
  </rdf:Description>

<!-- Properties (alphabetical) -->

  <rdf:Description rdf:about="&dcterms;alternative">
    <rdfs:label xml:lang="en">alternative name</rdfs:label>
    <rdfs:comment xml:lang="en">The dcterms:alternative property fully represents the RADion property of Alternative Name.</rdfs:comment>
    <vann:usageNote xml:lang="en">Used in RADion to provide an alternative name for the Asset: this information may be used to provide additional access points, e.g. allowing indexing of any acronyms, nicknames, shorthand notations or other identifying information that a user might expect to find the Asset under.  The range of dcterms:alternative is rdfs:Literal</vann:usageNote>
    <rdfs:isDefinedBy rdf:resource="&dcterms;" />
    <dcterms:identifier>dcterms:alternative</dcterms:identifier>
  </rdf:Description>

  <rdf:Description rdf:about="&xhv;last">
    <rdfs:label xml:lang="en">current version</rdfs:label>
    <rdfs:comment xml:lang="en">The xhv:last property fully represents the RADion relationship of Current version</rdfs:comment>
    <rdfs:isDefinedBy rdf:resource="&xhv;" />
    <vann:usageNote xml:lang="en">RADion uses the XHTML 'last' property to link an Asset to the most recent (i.e. current) version.</vann:usageNote>
    <dcterms:identifier>xhv:last</dcterms:identifier>
  </rdf:Description>

  <rdf:Description rdf:about="&dcterms;created">
    <rdfs:label xml:lang="en">date created</rdfs:label>
    <rdfs:comment xml:lang="en">The dcterms:created property fully represents the RADion property of Date of Creation.</rdfs:comment>
    <vann:usageNote xml:lang="en">RADion uses this to provide the creation date of this version of the Repository, Asset or Distribution. RADion expects a datatyped value and for it to be conformant with ISO 8601, preferably using an xsd data type.</vann:usageNote>
    <rdfs:isDefinedBy rdf:resource="&dcterms;" />
    <dcterms:identifier>dcterms:created</dcterms:identifier>
  </rdf:Description>

  <rdf:Description rdf:about="&dcterms;modified">
    <rdfs:label xml:lang="en">date modified</rdfs:label>
    <rdfs:comment xml:lang="en">The dcterms:modified property fully represents the RADion property Date of Last Modification.</rdfs:comment>
    <vann:usageNote xml:lang="en">RADion uses this to provide the date of latest update of the Repository, Asset or Distribution. RADion expects a datatyped value and for it to be conformant with ISO 8601, preferably using an xsd data type.</vann:usageNote>
    <rdfs:isDefinedBy rdf:resource="&dcterms;" />
    <dcterms:identifier>dcterms:modified</dcterms:identifier>
  </rdf:Description>

  <rdf:Description rdf:about="&dcterms;description">
    <rdfs:label xml:lang="en">description</rdfs:label>
    <rdfs:comment xml:lang="en">The dcterms:description property fully covers the RADion property of the same name.</rdfs:comment>
    <vann:usageNote xml:lang="en">Used in RADion to provide descriptive text for the Repository, Asset or Distribution.</vann:usageNote>
    <rdfs:isDefinedBy rdf:resource="&dcterms;" />
    <dcterms:identifier>dcterms:description</dcterms:identifier>
  </rdf:Description>

  <rdf:Property rdf:about="&rad;distribution">
    <rdfs:label xml:lang="en">distribution</rdfs:label>
    <rdfs:comment xml:lang="en">The distribution relationship associates an Asset (its domain) with a Distribution (its range). It is the inverse of distributionOf</rdfs:comment>
    <rdfs:isDefinedBy rdf:resource="&documentation;" />
    <rdfs:domain rdf:resource="#Asset" />
    <rdfs:range rdf:resource="#Distribution" />
    <dcterms:identifier>rad:distribution</dcterms:identifier>
  </rdf:Property>

  <rdf:Property rdf:about="&rad;distributionOf">
    <rdfs:label xml:lang="en">distributionOf</rdfs:label>
    <rdfs:comment xml:lang="en">The distributionOf relationship associates a Distribution (its domain) with the Asset (its range) of which it is a Distribution. It is the inverse of distribution</rdfs:comment>
    <rdfs:isDefinedBy rdf:resource="&documentation;" />
    <rdfs:domain rdf:resource="#Distribution" />
    <rdfs:range rdf:resource="#Asset" />
    <dcterms:identifier>rad:distributionOf</dcterms:identifier>
  </rdf:Property>

  <rdf:Description rdf:about="&dcterms;format">
    <rdfs:label xml:lang="en">format</rdfs:label>
    <rdfs:comment xml:lang="en">The dcterms:format property fully represents the RADion relationship of the same name</rdfs:comment>
    <vann:usageNote xml:lang="en">Used in RADion to link to the format that the Distribution is available in (e.g. PDF, XML, RDF/XML, HTML) which is provided as a property of dcterms:FileFormat</vann:usageNote>
    <rdfs:isDefinedBy rdf:resource="&dcterms;" />
    <dcterms:identifier>dcterms:format</dcterms:identifier>
  </rdf:Description>

  <rdf:Description rdf:about="&dcterms;hasPart">
    <rdfs:label xml:lang="en">includes</rdfs:label>
    <rdfs:comment xml:lang="en">The dcterms:hasPart property fully represents the RADion relationship of includes.</rdfs:comment>
    <vann:usageNote xml:lang="en">RADion uses dcterms:hasPart to link a Repository to an Asset.</vann:usageNote>
    <rdfs:isDefinedBy rdf:resource="&dcterms;" />
    <dcterms:identifier>dcterms:hasPart</dcterms:identifier>
  </rdf:Description>

  <rdf:Property rdf:about="&rad;keyword">
    <rdfs:label xml:lang="en">keyword</rdfs:label>
    <rdfs:comment xml:lang="en">A word or phrase used to succinctly descibe the Asset</rdfs:comment>
    <rdfs:isDefinedBy rdf:resource="&documentation;" />
    <rdfs:range rdf:resource="&rdfs;Literal" />
    <dcterms:identifier>rad:keyword</dcterms:identifier>
  </rdf:Property>

  <rdf:Description rdf:about="&rdfs;label">
    <rdfs:label xml:lang="en">label or name</rdfs:label>
    <rdfs:comment xml:lang="en">The rdfs:label property fully represents the RADion properties of name and label.</rdfs:comment>
    <vann:usageNote xml:lang="en">RADion uses this to provide the name or label of any class.</vann:usageNote>
    <rdfs:isDefinedBy rdf:resource="&rdfs;" />
    <dcterms:identifier>rdfs:label</dcterms:identifier>
  </rdf:Description>

  <rdf:Description rdf:about="&dcterms;language">
    <rdfs:label xml:lang="en">language</rdfs:label>
    <rdfs:comment xml:lang="en">The dcterms:language property fully represents the RADion property of the same name.</rdfs:comment>
    <vann:usageNote xml:lang="en">RADion uses this to provide the language of the Asset. </vann:usageNote>
    <rdfs:isDefinedBy rdf:resource="&dcterms;" />
    <dcterms:identifier>dcterms:language</dcterms:identifier>
  </rdf:Description>

  <rdf:Description rdf:about="&dcterms;license">
    <rdfs:label xml:lang="en">license</rdfs:label>
    <rdfs:comment xml:lang="en">The dcterms:license property fully represents the RADion relationship of the same name.</rdfs:comment>
    <vann:usageNote xml:lang="en">Used in RADion to link to the conditions or restrictions for (re-use) of the Distribution. Note that the range is dcterms:LicenseDocument</vann:usageNote>
    <rdfs:isDefinedBy rdf:resource="&dcterms;" />
    <dcterms:identifier>dcterms:license</dcterms:identifier>
  </rdf:Description>

  <rdf:Description rdf:about="&xhv;next">
    <rdfs:label xml:lang="en">next version</rdfs:label>
    <rdfs:comment xml:lang="en">The xhv:next property fully represents the RADion relationship of Next version</rdfs:comment>
    <rdfs:isDefinedBy rdf:resource="&xhv;" />
    <vann:usageNote xml:lang="en">RADion uses the XHTML 'next' property to link an Asset to the next most recent version.</vann:usageNote>
    <dcterms:identifier>xhv:next</dcterms:identifier>
  </rdf:Description>

  <rdf:Description rdf:about="&xhv;prev">
    <rdfs:label xml:lang="en">previous version</rdfs:label>
    <rdfs:comment xml:lang="en">The xhv:prev property fully represents the RADion relationship of Previous version</rdfs:comment>
    <rdfs:isDefinedBy rdf:resource="&xhv;" />
    <vann:usageNote xml:lang="en">RADion uses the XHTML 'previous' property to link an Asset to the previous version.</vann:usageNote>
    <dcterms:identifier>xhv:prev</dcterms:identifier>
  </rdf:Description>

  <rdf:Description rdf:about="&dcterms;publisher">
    <rdfs:label xml:lang="en">publisher</rdfs:label>
    <rdfs:comment xml:lang="en">The dcterms:publisher property fully represents the RADion relationship of the same name</rdfs:comment>
    <vann:usageNote xml:lang="en">Used in RADion to link to the organisation responsible for the publication of the Asset, Repository or Distribution. Note that the range is dcterms:Agent.</vann:usageNote>
    <rdfs:isDefinedBy rdf:resource="&dcterms;" />
    <dcterms:identifier>dcterms:publisher</dcterms:identifier>
  </rdf:Description>

  <rdf:Description rdf:about="&dcterms;relation">
    <rdfs:label xml:lang="en">relation</rdfs:label>
    <rdfs:comment xml:lang="en">The dcterms:relation property fully represents the RADion related asset property.</rdfs:comment>
    <vann:usageNote xml:lang="en">Used in RADion to link any Asset to any other related Asset. RADion expects the object to be of type rad:Asset.</vann:usageNote>
    <rdfs:isDefinedBy rdf:resource="&dcterms;" />
    <dcterms:identifier>dcterms:relation</dcterms:identifier>
  </rdf:Description>

  <rdf:Description rdf:about="&dcterms;isPartOf">
    <rdfs:label xml:lang="en">repository origin</rdfs:label>
    <rdfs:comment xml:lang="en">The dcterms:isPartOf property fully represents the RADion relationship of repository origin..</rdfs:comment>
    <vann:usageNote xml:lang="en">RADion uses dcterms:isPartOf to link an Asset to a Repository.</vann:usageNote>
    <rdfs:isDefinedBy rdf:resource="&dcterms;" />
    <dcterms:identifier>dcterms:isPartOf</dcterms:identifier>
  </rdf:Description>

  <rdf:Description rdf:about="&dcterms;spatial">
    <rdfs:label xml:lang="en">spatial coverage</rdfs:label>
    <rdfs:comment xml:lang="en">The dcterms:spatial property fully represents the RADion relationship of spatial coverage.</rdfs:comment>
    <vann:usageNote xml:lang="en">RADion uses this to link to the geographic region or jurisdiction that the Asset or Repository applies to. Note that the range is dcterms:Location.</vann:usageNote>
    <rdfs:isDefinedBy rdf:resource="&dcDoc;" />
    <dcterms:identifier>dcterms:spatial</dcterms:identifier>
  </rdf:Description>

  <rdf:Description rdf:about="&dcterms;subject">
    <rdfs:label xml:lang="en">theme, theme taxonomy</rdfs:label>
    <rdfs:comment xml:lang="en">The dcterms:subject property fully represents the RADion properties of theme and theme taxonomy.</rdfs:comment>
    <vann:usageNote xml:lang="en">The theme relationship associates an Asset with a specific Theme and theme taxonomy 
    does the same job for the repository as a whole. Themes are typically, but not necessarily,
    encoded as a skos:Concept, arranged in a skos:ConceptScheme.</vann:usageNote>
    <rdfs:isDefinedBy rdf:resource="&dcDoc;" />
    <dcterms:identifier>dcterms:subject</dcterms:identifier>
  </rdf:Description>

  <rdf:Description rdf:about="&dcterms;type">
    <rdfs:label xml:lang="en">type</rdfs:label>
    <rdfs:comment xml:lang="en">The dcterms:type property fully represents the RADion property of type.</rdfs:comment>
    <vann:usageNote xml:lang="en">Used in RADion to link a Licence or Publisher to its type.</vann:usageNote>
    <rdfs:isDefinedBy rdf:resource="&documentation;" />
    <dcterms:identifier>dcterms:type</dcterms:identifier>
  </rdf:Description>

  <rdf:Property rdf:about="&rad;version">
    <rdfs:label xml:lang="en">version</rdfs:label>
    <rdfs:comment xml:lang="en">The version number or other designation of the Asset; the value should be a free text string</rdfs:comment>
    <rdfs:isDefinedBy rdf:resource="&documentation;" />
    <rdfs:range rdf:resource="&rdfs;Literal" />
    <dcterms:identifier>rad:version</dcterms:identifier>
  </rdf:Property>

  <rdf:Property rdf:about="&rad;versionNotes">
    <rdfs:label xml:lang="en">version notes</rdfs:label>
    <rdfs:comment xml:lang="en">Notes on the particular version of the Asset.</rdfs:comment>
    <rdfs:isDefinedBy rdf:resource="&documentation;" />
    <rdfs:range rdf:resource="&rdfs;Literal" />
    <dcterms:identifier>rad:versionNotes</dcterms:identifier>
  </rdf:Property>

</rdf:RDF>