<?xml version="1.0"?>


<!DOCTYPE rdf:RDF [
    <!ENTITY terms "http://purl.org/dc/terms/" >
    <!ENTITY vann "http://purl.org/vocab/vann/" >
    <!ENTITY cc "http://creativecommons.org/ns#" >
    <!ENTITY owl "http://www.w3.org/2002/07/owl#" >
    <!ENTITY dc "http://purl.org/dc/elements/1.1/" >
    <!ENTITY xsd "http://www.w3.org/2001/XMLSchema#" >
    <!ENTITY skos "http://www.w3.org/2004/02/skos/core#" >
    <!ENTITY rdfs "http://www.w3.org/2000/01/rdf-schema#" >
    <!ENTITY rdf "http://www.w3.org/1999/02/22-rdf-syntax-ns#" >
    <!ENTITY demlab "http://www.demcare.eu/ontologies/demlab.owl#" >
]>


<rdf:RDF xmlns="http://www.demcare.eu/ontologies/demlab.owl#"
     xml:base="http://www.demcare.eu/ontologies/demlab.owl"
     xmlns:dc="http://purl.org/dc/elements/1.1/"
     xmlns:rdfs="http://www.w3.org/2000/01/rdf-schema#"
     xmlns:terms="http://purl.org/dc/terms/"
     xmlns:owl="http://www.w3.org/2002/07/owl#"
     xmlns:xsd="http://www.w3.org/2001/XMLSchema#"
     xmlns:rdf="http://www.w3.org/1999/02/22-rdf-syntax-ns#"
     xmlns:vann="http://purl.org/vocab/vann/"
     xmlns:skos="http://www.w3.org/2004/02/skos/core#"
     xmlns:cc="http://creativecommons.org/ns#"
	 xmlns:foaf="http://xmlns.com/foaf/0.1/"
     xmlns:demlab="http://www.demcare.eu/ontologies/demlab.owl#">
    <owl:Ontology rdf:about="http://www.demcare.eu/ontologies/demlab.owl">
        <owl:versionInfo rdf:datatype="&xsd;decimal">1.0</owl:versionInfo>
        <rdfs:seeAlso>http://www.demcare.eu/</rdfs:seeAlso>
        <terms:date>2014-09-02</terms:date>
        <terms:title xml:lang="en">Dem@Care Lab Ontology for Dementia Assessment</terms:title>
		<dc:creator>
			<foaf:Person rdf:about="http://www.iti.gr/iti/people/Georgios_Meditskos.html#gmeditsk">
				<foaf:name>Georgios Meditskos</foaf:name>
				<foaf:homepage rdf:resource="http://www.iti.gr/iti/people/Georgios_Meditskos.html" />
			</foaf:Person>
		</dc:creator>
		<dc:creator>
			<foaf:Person rdf:about="http://www.iti.gr/iti/people/Ioannis_Kompatsiaris.html#ikom">
				<foaf:name>Ioannis Kompatsiaris</foaf:name>
				<foaf:homepage rdf:resource="http://www.iti.gr/iti/people/Ioannis_Kompatsiaris.html" />
			</foaf:Person>
		</dc:creator>		
        <dc:description xml:lang="en">The ontology has been developed in the framework of the Dem@Care project for representing the experimentation protocol towards diagnostic support and assessment of Dementia in a controlled environment. The aim of the protocol is to provide a brief overview of their health status of the participants during consultation (cognition, behaviours and function), and to correlate the system (sensor) data with the data collected using typical dementia care assessment tools.

The ontology describes the basic Steps of the experimentation protocol (Directed Activities, Semi-directed Activities and Free Discussion with the Clinician), the Tasks that are involved, as well as the measurement types relevant to each Task. The defined protocol can be reused and further extended, adding new steps, tasks and measured data.

Documentation regarding the ontology vocabulary can be found at http://www.demcare.eu/ontologies/demlab.html</dc:description>
        <vann:preferredNamespacePrefix>demlab</vann:preferredNamespacePrefix>
        <rdfs:seeAlso>http://www.demcare.eu/downloads/D8.1ExperimentationProtocols.pdf</rdfs:seeAlso>
        <terms:rights xml:lang="en">This ontology is licensed under Creative Commons CC BY 3.0 It is developed in the framework of the Dem@Care project (http://www.demcare.eu/) and supported by the Information Technologies Institute (http://www.iti.gr) of the Centre for Research and Technology Hellas.</terms:rights>
        <cc:license rdf:resource="http://creativecommons.org/licenses/by/3.0/"/>
        <owl:versionIRI rdf:resource="http://www.demcare.eu/ontologies/demlab.owl/1.0"/>
        <owl:imports rdf:resource="http://www.w3.org/2006/time"/>
        <owl:imports rdf:resource="http://xmlns.com/foaf/0.1/"/>
    </owl:Ontology>
    


    <!-- 
    ///////////////////////////////////////////////////////////////////////////////////////
    //
    // Annotation properties
    //
    ///////////////////////////////////////////////////////////////////////////////////////
     -->

    


    <!-- http://purl.org/dc/elements/1.1/contributor -->

    <owl:AnnotationProperty rdf:about="&dc;contributor"/>
    


    <!-- http://purl.org/dc/elements/1.1/coverage -->

    <owl:AnnotationProperty rdf:about="&dc;coverage"/>
    


    <!-- http://purl.org/dc/elements/1.1/creator -->

    <owl:AnnotationProperty rdf:about="&dc;creator"/>
    


    <!-- http://purl.org/dc/elements/1.1/format -->

    <owl:AnnotationProperty rdf:about="&dc;format"/>
    


    <!-- http://purl.org/dc/elements/1.1/identifier -->

    <owl:AnnotationProperty rdf:about="&dc;identifier"/>
    


    <!-- http://purl.org/dc/elements/1.1/language -->

    <owl:AnnotationProperty rdf:about="&dc;language"/>
    


    <!-- http://purl.org/dc/elements/1.1/publisher -->

    <owl:AnnotationProperty rdf:about="&dc;publisher"/>
    


    <!-- http://purl.org/dc/elements/1.1/relation -->

    <owl:AnnotationProperty rdf:about="&dc;relation"/>
    


    <!-- http://purl.org/dc/elements/1.1/rights -->

    <owl:AnnotationProperty rdf:about="&dc;rights"/>
    


    <!-- http://purl.org/dc/elements/1.1/source -->

    <owl:AnnotationProperty rdf:about="&dc;source"/>
    


    <!-- http://purl.org/dc/elements/1.1/subject -->

    <owl:AnnotationProperty rdf:about="&dc;subject"/>
    


    <!-- http://purl.org/dc/elements/1.1/type -->

    <owl:AnnotationProperty rdf:about="&dc;type"/>
    


    <!-- http://purl.org/dc/terms/abstract -->

    <owl:AnnotationProperty rdf:about="&terms;abstract">
        <rdfs:label xml:lang="en">Abstract</rdfs:label>
        <terms:issued rdf:datatype="&xsd;date">2000-07-11</terms:issued>
        <terms:modified rdf:datatype="&xsd;date">2008-01-14</terms:modified>
        <rdfs:comment xml:lang="en">A summary of the resource.</rdfs:comment>
        <terms:hasVersion rdf:resource="http://dublincore.org/usage/terms/history/#abstract-003"/>
        <rdfs:subPropertyOf rdf:resource="&dc;description"/>
        <rdfs:isDefinedBy rdf:resource="http://purl.org/dc/terms/"/>
        <rdfs:subPropertyOf rdf:resource="&terms;description"/>
    </owl:AnnotationProperty>
    


    <!-- http://purl.org/dc/terms/accessRights -->

    <owl:AnnotationProperty rdf:about="&terms;accessRights">
        <rdfs:label xml:lang="en">Access Rights</rdfs:label>
        <terms:issued rdf:datatype="&xsd;date">2003-02-15</terms:issued>
        <terms:modified rdf:datatype="&xsd;date">2008-01-14</terms:modified>
        <terms:description xml:lang="en">Access Rights may include information regarding access or restrictions based on privacy, security, or other policies.</terms:description>
        <rdfs:comment xml:lang="en">Information about who can access the resource or an indication of its security status.</rdfs:comment>
        <terms:hasVersion rdf:resource="http://dublincore.org/usage/terms/history/#accessRights-002"/>
        <rdfs:subPropertyOf rdf:resource="&dc;rights"/>
        <rdfs:isDefinedBy rdf:resource="http://purl.org/dc/terms/"/>
    </owl:AnnotationProperty>
    


    <!-- http://purl.org/dc/terms/accrualMethod -->

    <owl:AnnotationProperty rdf:about="&terms;accrualMethod">
        <rdfs:label xml:lang="en">Accrual Method</rdfs:label>
        <terms:issued rdf:datatype="&xsd;date">2005-06-13</terms:issued>
        <terms:modified rdf:datatype="&xsd;date">2010-10-11</terms:modified>
        <rdfs:comment xml:lang="en">The method by which items are added to a collection.</rdfs:comment>
        <terms:hasVersion rdf:resource="http://dublincore.org/usage/terms/history/#accrualMethod-003"/>
        <rdfs:domain rdf:resource="http://purl.org/dc/dcmitype/Collection"/>
        <rdfs:isDefinedBy rdf:resource="http://purl.org/dc/terms/"/>
    </owl:AnnotationProperty>
    


    <!-- http://purl.org/dc/terms/accrualPeriodicity -->

    <owl:AnnotationProperty rdf:about="&terms;accrualPeriodicity">
        <rdfs:label xml:lang="en">Accrual Periodicity</rdfs:label>
        <terms:issued rdf:datatype="&xsd;date">2005-06-13</terms:issued>
        <terms:modified rdf:datatype="&xsd;date">2010-10-11</terms:modified>
        <rdfs:comment xml:lang="en">The frequency with which items are added to a collection.</rdfs:comment>
        <terms:hasVersion rdf:resource="http://dublincore.org/usage/terms/history/#accrualPeriodicity-003"/>
        <rdfs:domain rdf:resource="http://purl.org/dc/dcmitype/Collection"/>
        <rdfs:isDefinedBy rdf:resource="http://purl.org/dc/terms/"/>
    </owl:AnnotationProperty>
    


    <!-- http://purl.org/dc/terms/accrualPolicy -->

    <owl:AnnotationProperty rdf:about="&terms;accrualPolicy">
        <rdfs:label xml:lang="en">Accrual Policy</rdfs:label>
        <terms:issued rdf:datatype="&xsd;date">2005-06-13</terms:issued>
        <terms:modified rdf:datatype="&xsd;date">2010-10-11</terms:modified>
        <rdfs:comment xml:lang="en">The policy governing the addition of items to a collection.</rdfs:comment>
        <terms:hasVersion rdf:resource="http://dublincore.org/usage/terms/history/#accrualPolicy-003"/>
        <rdfs:domain rdf:resource="http://purl.org/dc/dcmitype/Collection"/>
        <rdfs:isDefinedBy rdf:resource="http://purl.org/dc/terms/"/>
    </owl:AnnotationProperty>
    


    <!-- http://purl.org/dc/terms/alternative -->

    <owl:AnnotationProperty rdf:about="&terms;alternative">
        <rdfs:label xml:lang="en">Alternative Title</rdfs:label>
        <terms:issued rdf:datatype="&xsd;date">2000-07-11</terms:issued>
        <terms:modified rdf:datatype="&xsd;date">2010-10-11</terms:modified>
        <rdfs:comment xml:lang="en">An alternative name for the resource.</rdfs:comment>
        <terms:description xml:lang="en">The distinction between titles and alternative titles is application-specific.</terms:description>
        <terms:hasVersion rdf:resource="http://dublincore.org/usage/terms/history/#alternative-003"/>
        <rdfs:subPropertyOf rdf:resource="&dc;title"/>
        <rdfs:isDefinedBy rdf:resource="http://purl.org/dc/terms/"/>
    </owl:AnnotationProperty>
    


    <!-- http://purl.org/dc/terms/available -->

    <owl:AnnotationProperty rdf:about="&terms;available">
        <rdfs:label xml:lang="en">Date Available</rdfs:label>
        <terms:issued rdf:datatype="&xsd;date">2000-07-11</terms:issued>
        <terms:modified rdf:datatype="&xsd;date">2008-01-14</terms:modified>
        <rdfs:comment xml:lang="en">Date (often a range) that the resource became or will become available.</rdfs:comment>
        <terms:hasVersion rdf:resource="http://dublincore.org/usage/terms/history/#available-003"/>
        <rdfs:subPropertyOf rdf:resource="&dc;date"/>
        <rdfs:isDefinedBy rdf:resource="http://purl.org/dc/terms/"/>
    </owl:AnnotationProperty>
    


    <!-- http://purl.org/dc/terms/bibliographicCitation -->

    <owl:AnnotationProperty rdf:about="&terms;bibliographicCitation">
        <rdfs:label xml:lang="en">Bibliographic Citation</rdfs:label>
        <terms:issued rdf:datatype="&xsd;date">2003-02-15</terms:issued>
        <terms:modified rdf:datatype="&xsd;date">2008-01-14</terms:modified>
        <rdfs:comment xml:lang="en">A bibliographic reference for the resource.</rdfs:comment>
        <terms:description xml:lang="en">Recommended practice is to include sufficient bibliographic detail to identify the resource as unambiguously as possible.</terms:description>
        <terms:hasVersion rdf:resource="http://dublincore.org/usage/terms/history/#bibliographicCitation-002"/>
        <rdfs:subPropertyOf rdf:resource="&dc;identifier"/>
        <rdfs:isDefinedBy rdf:resource="http://purl.org/dc/terms/"/>
        <rdfs:domain rdf:resource="&terms;BibliographicResource"/>
    </owl:AnnotationProperty>
    


    <!-- http://purl.org/dc/terms/conformsTo -->

    <owl:AnnotationProperty rdf:about="&terms;conformsTo">
        <rdfs:label xml:lang="en">Conforms To</rdfs:label>
        <terms:issued rdf:datatype="&xsd;date">2001-05-21</terms:issued>
        <terms:modified rdf:datatype="&xsd;date">2008-01-14</terms:modified>
        <rdfs:comment xml:lang="en">An established standard to which the described resource conforms.</rdfs:comment>
        <terms:hasVersion rdf:resource="http://dublincore.org/usage/terms/history/#conformsTo-003"/>
        <rdfs:subPropertyOf rdf:resource="&dc;relation"/>
        <rdfs:isDefinedBy rdf:resource="http://purl.org/dc/terms/"/>
        <rdfs:subPropertyOf rdf:resource="&terms;relation"/>
    </owl:AnnotationProperty>
    


    <!-- http://purl.org/dc/terms/contributor -->

    <owl:AnnotationProperty rdf:about="&terms;contributor">
        <rdfs:label xml:lang="en">Contributor</rdfs:label>
        <terms:issued rdf:datatype="&xsd;date">2008-01-14</terms:issued>
        <terms:modified rdf:datatype="&xsd;date">2010-10-11</terms:modified>
        <rdfs:comment xml:lang="en">An entity responsible for making contributions to the resource.</rdfs:comment>
        <terms:description xml:lang="en">Examples of a Contributor include a person, an organization, or a service.</terms:description>
        <terms:hasVersion rdf:resource="http://dublincore.org/usage/terms/history/#contributorT-001"/>
        <rdfs:subPropertyOf rdf:resource="&dc;contributor"/>
        <rdfs:isDefinedBy rdf:resource="http://purl.org/dc/terms/"/>
    </owl:AnnotationProperty>
    


    <!-- http://purl.org/dc/terms/coverage -->

    <owl:AnnotationProperty rdf:about="&terms;coverage">
        <rdfs:label xml:lang="en">Coverage</rdfs:label>
        <terms:issued rdf:datatype="&xsd;date">2008-01-14</terms:issued>
        <terms:modified rdf:datatype="&xsd;date">2008-01-14</terms:modified>
        <terms:description xml:lang="en">Spatial topic and spatial applicability may be a named place or a location specified by its geographic coordinates. Temporal topic may be a named period, date, or date range. A jurisdiction may be a named administrative entity or a geographic place to which the resource applies. Recommended best practice is to use a controlled vocabulary such as the Thesaurus of Geographic Names [TGN]. Where appropriate, named places or time periods can be used in preference to numeric identifiers such as sets of coordinates or date ranges.</terms:description>
        <rdfs:comment xml:lang="en">The spatial or temporal topic of the resource, the spatial applicability of the resource, or the jurisdiction under which the resource is relevant.</rdfs:comment>
        <terms:hasVersion rdf:resource="http://dublincore.org/usage/terms/history/#coverageT-001"/>
        <rdfs:subPropertyOf rdf:resource="&dc;coverage"/>
        <rdfs:isDefinedBy rdf:resource="http://purl.org/dc/terms/"/>
    </owl:AnnotationProperty>
    


    <!-- http://purl.org/dc/terms/created -->

    <owl:AnnotationProperty rdf:about="&terms;created">
        <rdfs:label xml:lang="en">Date Created</rdfs:label>
        <terms:issued rdf:datatype="&xsd;date">2000-07-11</terms:issued>
        <terms:modified rdf:datatype="&xsd;date">2008-01-14</terms:modified>
        <rdfs:comment xml:lang="en">Date of creation of the resource.</rdfs:comment>
        <terms:hasVersion rdf:resource="http://dublincore.org/usage/terms/history/#created-003"/>
        <rdfs:subPropertyOf rdf:resource="&dc;date"/>
        <rdfs:isDefinedBy rdf:resource="http://purl.org/dc/terms/"/>
    </owl:AnnotationProperty>
    


    <!-- http://purl.org/dc/terms/creator -->

    <owl:AnnotationProperty rdf:about="&terms;creator">
        <rdfs:label xml:lang="en">Creator</rdfs:label>
        <terms:issued rdf:datatype="&xsd;date">2008-01-14</terms:issued>
        <terms:modified rdf:datatype="&xsd;date">2010-10-11</terms:modified>
        <rdfs:comment xml:lang="en">An entity primarily responsible for making the resource.</rdfs:comment>
        <terms:description xml:lang="en">Examples of a Creator include a person, an organization, or a service.</terms:description>
        <terms:hasVersion rdf:resource="http://dublincore.org/usage/terms/history/#creatorT-002"/>
        <rdfs:subPropertyOf rdf:resource="&dc;creator"/>
        <rdfs:isDefinedBy rdf:resource="http://purl.org/dc/terms/"/>
    </owl:AnnotationProperty>
    


    <!-- http://purl.org/dc/terms/date -->

    <owl:AnnotationProperty rdf:about="&terms;date">
        <rdfs:label xml:lang="en">Date</rdfs:label>
        <terms:issued rdf:datatype="&xsd;date">2008-01-14</terms:issued>
        <terms:modified rdf:datatype="&xsd;date">2008-01-14</terms:modified>
        <rdfs:comment xml:lang="en">A point or period of time associated with an event in the lifecycle of the resource.</rdfs:comment>
        <terms:description xml:lang="en">Date may be used to express temporal information at any level of granularity.  Recommended best practice is to use an encoding scheme, such as the W3CDTF profile of ISO 8601 [W3CDTF].</terms:description>
        <terms:hasVersion rdf:resource="http://dublincore.org/usage/terms/history/#dateT-001"/>
        <rdfs:subPropertyOf rdf:resource="&dc;date"/>
        <rdfs:isDefinedBy rdf:resource="http://purl.org/dc/terms/"/>
    </owl:AnnotationProperty>
    


    <!-- http://purl.org/dc/terms/dateAccepted -->

    <owl:AnnotationProperty rdf:about="&terms;dateAccepted">
        <rdfs:label xml:lang="en">Date Accepted</rdfs:label>
        <terms:issued rdf:datatype="&xsd;date">2002-07-13</terms:issued>
        <terms:modified rdf:datatype="&xsd;date">2008-01-14</terms:modified>
        <rdfs:comment xml:lang="en">Date of acceptance of the resource.</rdfs:comment>
        <terms:description xml:lang="en">Examples of resources to which a Date Accepted may be relevant are a thesis (accepted by a university department) or an article (accepted by a journal).</terms:description>
        <terms:hasVersion rdf:resource="http://dublincore.org/usage/terms/history/#dateAccepted-002"/>
        <rdfs:subPropertyOf rdf:resource="&dc;date"/>
        <rdfs:isDefinedBy rdf:resource="http://purl.org/dc/terms/"/>
    </owl:AnnotationProperty>
    


    <!-- http://purl.org/dc/terms/dateCopyrighted -->

    <owl:AnnotationProperty rdf:about="&terms;dateCopyrighted">
        <rdfs:label xml:lang="en">Date Copyrighted</rdfs:label>
        <terms:issued rdf:datatype="&xsd;date">2002-07-13</terms:issued>
        <terms:modified rdf:datatype="&xsd;date">2008-01-14</terms:modified>
        <rdfs:comment xml:lang="en">Date of copyright.</rdfs:comment>
        <terms:hasVersion rdf:resource="http://dublincore.org/usage/terms/history/#dateCopyrighted-002"/>
        <rdfs:subPropertyOf rdf:resource="&dc;date"/>
        <rdfs:isDefinedBy rdf:resource="http://purl.org/dc/terms/"/>
    </owl:AnnotationProperty>
    


    <!-- http://purl.org/dc/terms/dateSubmitted -->

    <owl:AnnotationProperty rdf:about="&terms;dateSubmitted">
        <rdfs:label xml:lang="en">Date Submitted</rdfs:label>
        <terms:issued rdf:datatype="&xsd;date">2002-07-13</terms:issued>
        <terms:modified rdf:datatype="&xsd;date">2008-01-14</terms:modified>
        <rdfs:comment xml:lang="en">Date of submission of the resource.</rdfs:comment>
        <terms:description xml:lang="en">Examples of resources to which a Date Submitted may be relevant are a thesis (submitted to a university department) or an article (submitted to a journal).</terms:description>
        <terms:hasVersion rdf:resource="http://dublincore.org/usage/terms/history/#dateSubmitted-002"/>
        <rdfs:subPropertyOf rdf:resource="&dc;date"/>
        <rdfs:isDefinedBy rdf:resource="http://purl.org/dc/terms/"/>
    </owl:AnnotationProperty>
    


    <!-- http://purl.org/dc/terms/description -->

    <owl:AnnotationProperty rdf:about="&terms;description">
        <rdfs:label xml:lang="en">Description</rdfs:label>
        <terms:issued rdf:datatype="&xsd;date">2008-01-14</terms:issued>
        <terms:modified rdf:datatype="&xsd;date">2008-01-14</terms:modified>
        <rdfs:comment xml:lang="en">An account of the resource.</rdfs:comment>
        <terms:description xml:lang="en">Description may include but is not limited to: an abstract, a table of contents, a graphical representation, or a free-text account of the resource.</terms:description>
        <terms:hasVersion rdf:resource="http://dublincore.org/usage/terms/history/#descriptionT-001"/>
        <rdfs:subPropertyOf rdf:resource="&dc;description"/>
        <rdfs:isDefinedBy rdf:resource="http://purl.org/dc/terms/"/>
    </owl:AnnotationProperty>
    


    <!-- http://purl.org/dc/terms/educationLevel -->

    <owl:AnnotationProperty rdf:about="&terms;educationLevel">
        <rdfs:label xml:lang="en">Audience Education Level</rdfs:label>
        <terms:issued rdf:datatype="&xsd;date">2002-07-13</terms:issued>
        <terms:modified rdf:datatype="&xsd;date">2008-01-14</terms:modified>
        <rdfs:comment xml:lang="en">A class of entity, defined in terms of progression through an educational or training context, for which the described resource is intended.</rdfs:comment>
        <terms:hasVersion rdf:resource="http://dublincore.org/usage/terms/history/#educationLevel-002"/>
        <rdfs:isDefinedBy rdf:resource="http://purl.org/dc/terms/"/>
    </owl:AnnotationProperty>
    


    <!-- http://purl.org/dc/terms/extent -->

    <owl:AnnotationProperty rdf:about="&terms;extent">
        <rdfs:label xml:lang="en">Extent</rdfs:label>
        <terms:issued rdf:datatype="&xsd;date">2000-07-11</terms:issued>
        <terms:modified rdf:datatype="&xsd;date">2008-01-14</terms:modified>
        <rdfs:comment xml:lang="en">The size or duration of the resource.</rdfs:comment>
        <terms:hasVersion rdf:resource="http://dublincore.org/usage/terms/history/#extent-003"/>
        <rdfs:subPropertyOf rdf:resource="&dc;format"/>
        <rdfs:isDefinedBy rdf:resource="http://purl.org/dc/terms/"/>
    </owl:AnnotationProperty>
    


    <!-- http://purl.org/dc/terms/format -->

    <owl:AnnotationProperty rdf:about="&terms;format">
        <rdfs:label xml:lang="en">Format</rdfs:label>
        <terms:issued rdf:datatype="&xsd;date">2008-01-14</terms:issued>
        <terms:modified rdf:datatype="&xsd;date">2008-01-14</terms:modified>
        <terms:description xml:lang="en">Examples of dimensions include size and duration. Recommended best practice is to use a controlled vocabulary such as the list of Internet Media Types [MIME].</terms:description>
        <rdfs:comment xml:lang="en">The file format, physical medium, or dimensions of the resource.</rdfs:comment>
        <terms:hasVersion rdf:resource="http://dublincore.org/usage/terms/history/#formatT-001"/>
        <rdfs:subPropertyOf rdf:resource="&dc;format"/>
        <rdfs:isDefinedBy rdf:resource="http://purl.org/dc/terms/"/>
    </owl:AnnotationProperty>
    


    <!-- http://purl.org/dc/terms/hasFormat -->

    <owl:AnnotationProperty rdf:about="&terms;hasFormat">
        <rdfs:label xml:lang="en">Has Format</rdfs:label>
        <terms:issued rdf:datatype="&xsd;date">2000-07-11</terms:issued>
        <terms:modified rdf:datatype="&xsd;date">2008-01-14</terms:modified>
        <rdfs:comment xml:lang="en">A related resource that is substantially the same as the pre-existing described resource, but in another format.</rdfs:comment>
        <skos:note xml:lang="en">This term is intended to be used with non-literal values as defined in the DCMI Abstract Model (http://dublincore.org/documents/abstract-model/).  As of December 2007, the DCMI Usage Board is seeking a way to express this intention with a formal range declaration.</skos:note>
        <terms:hasVersion rdf:resource="http://dublincore.org/usage/terms/history/#hasFormat-003"/>
        <rdfs:subPropertyOf rdf:resource="&dc;relation"/>
        <rdfs:isDefinedBy rdf:resource="http://purl.org/dc/terms/"/>
        <rdfs:subPropertyOf rdf:resource="&terms;relation"/>
    </owl:AnnotationProperty>
    


    <!-- http://purl.org/dc/terms/hasPart -->

    <owl:AnnotationProperty rdf:about="&terms;hasPart">
        <rdfs:label xml:lang="en">Has Part</rdfs:label>
        <terms:issued rdf:datatype="&xsd;date">2000-07-11</terms:issued>
        <terms:modified rdf:datatype="&xsd;date">2008-01-14</terms:modified>
        <rdfs:comment xml:lang="en">A related resource that is included either physically or logically in the described resource.</rdfs:comment>
        <skos:note xml:lang="en">This term is intended to be used with non-literal values as defined in the DCMI Abstract Model (http://dublincore.org/documents/abstract-model/).  As of December 2007, the DCMI Usage Board is seeking a way to express this intention with a formal range declaration.</skos:note>
        <terms:hasVersion rdf:resource="http://dublincore.org/usage/terms/history/#hasPart-003"/>
        <rdfs:subPropertyOf rdf:resource="&dc;relation"/>
        <rdfs:isDefinedBy rdf:resource="http://purl.org/dc/terms/"/>
        <rdfs:subPropertyOf rdf:resource="&terms;relation"/>
    </owl:AnnotationProperty>
    


    <!-- http://purl.org/dc/terms/hasVersion -->

    <owl:AnnotationProperty rdf:about="&terms;hasVersion">
        <rdfs:label xml:lang="en">Has Version</rdfs:label>
        <terms:issued rdf:datatype="&xsd;date">2000-07-11</terms:issued>
        <terms:modified rdf:datatype="&xsd;date">2008-01-14</terms:modified>
        <rdfs:comment xml:lang="en">A related resource that is a version, edition, or adaptation of the described resource.</rdfs:comment>
        <skos:note xml:lang="en">This term is intended to be used with non-literal values as defined in the DCMI Abstract Model (http://dublincore.org/documents/abstract-model/).  As of December 2007, the DCMI Usage Board is seeking a way to express this intention with a formal range declaration.</skos:note>
        <terms:hasVersion rdf:resource="http://dublincore.org/usage/terms/history/#hasVersion-003"/>
        <rdfs:subPropertyOf rdf:resource="&dc;relation"/>
        <rdfs:isDefinedBy rdf:resource="http://purl.org/dc/terms/"/>
        <rdfs:subPropertyOf rdf:resource="&terms;relation"/>
    </owl:AnnotationProperty>
    


    <!-- http://purl.org/dc/terms/identifier -->

    <owl:AnnotationProperty rdf:about="&terms;identifier">
        <rdfs:label xml:lang="en">Identifier</rdfs:label>
        <terms:issued rdf:datatype="&xsd;date">2008-01-14</terms:issued>
        <terms:modified rdf:datatype="&xsd;date">2008-01-14</terms:modified>
        <rdfs:comment xml:lang="en">An unambiguous reference to the resource within a given context.</rdfs:comment>
        <terms:description xml:lang="en">Recommended best practice is to identify the resource by means of a string conforming to a formal identification system. </terms:description>
        <terms:hasVersion rdf:resource="http://dublincore.org/usage/terms/history/#identifierT-001"/>
        <rdfs:subPropertyOf rdf:resource="&dc;identifier"/>
        <rdfs:isDefinedBy rdf:resource="http://purl.org/dc/terms/"/>
    </owl:AnnotationProperty>
    


    <!-- http://purl.org/dc/terms/isFormatOf -->

    <owl:AnnotationProperty rdf:about="&terms;isFormatOf">
        <rdfs:label xml:lang="en">Is Format Of</rdfs:label>
        <terms:issued rdf:datatype="&xsd;date">2000-07-11</terms:issued>
        <terms:modified rdf:datatype="&xsd;date">2008-01-14</terms:modified>
        <rdfs:comment xml:lang="en">A related resource that is substantially the same as the described resource, but in another format.</rdfs:comment>
        <skos:note xml:lang="en">This term is intended to be used with non-literal values as defined in the DCMI Abstract Model (http://dublincore.org/documents/abstract-model/).  As of December 2007, the DCMI Usage Board is seeking a way to express this intention with a formal range declaration.</skos:note>
        <terms:hasVersion rdf:resource="http://dublincore.org/usage/terms/history/#isFormatOf-003"/>
        <rdfs:subPropertyOf rdf:resource="&dc;relation"/>
        <rdfs:isDefinedBy rdf:resource="http://purl.org/dc/terms/"/>
        <rdfs:subPropertyOf rdf:resource="&terms;relation"/>
    </owl:AnnotationProperty>
    


    <!-- http://purl.org/dc/terms/isPartOf -->

    <owl:AnnotationProperty rdf:about="&terms;isPartOf">
        <rdfs:label xml:lang="en">Is Part Of</rdfs:label>
        <terms:issued rdf:datatype="&xsd;date">2000-07-11</terms:issued>
        <terms:modified rdf:datatype="&xsd;date">2008-01-14</terms:modified>
        <rdfs:comment xml:lang="en">A related resource in which the described resource is physically or logically included.</rdfs:comment>
        <skos:note xml:lang="en">This term is intended to be used with non-literal values as defined in the DCMI Abstract Model (http://dublincore.org/documents/abstract-model/).  As of December 2007, the DCMI Usage Board is seeking a way to express this intention with a formal range declaration.</skos:note>
        <terms:hasVersion rdf:resource="http://dublincore.org/usage/terms/history/#isPartOf-003"/>
        <rdfs:subPropertyOf rdf:resource="&dc;relation"/>
        <rdfs:isDefinedBy rdf:resource="http://purl.org/dc/terms/"/>
        <rdfs:subPropertyOf rdf:resource="&terms;relation"/>
    </owl:AnnotationProperty>
    


    <!-- http://purl.org/dc/terms/isReferencedBy -->

    <owl:AnnotationProperty rdf:about="&terms;isReferencedBy">
        <rdfs:label xml:lang="en">Is Referenced By</rdfs:label>
        <terms:issued rdf:datatype="&xsd;date">2000-07-11</terms:issued>
        <terms:modified rdf:datatype="&xsd;date">2008-01-14</terms:modified>
        <rdfs:comment xml:lang="en">A related resource that references, cites, or otherwise points to the described resource.</rdfs:comment>
        <skos:note xml:lang="en">This term is intended to be used with non-literal values as defined in the DCMI Abstract Model (http://dublincore.org/documents/abstract-model/).  As of December 2007, the DCMI Usage Board is seeking a way to express this intention with a formal range declaration.</skos:note>
        <terms:hasVersion rdf:resource="http://dublincore.org/usage/terms/history/#isReferencedBy-003"/>
        <rdfs:subPropertyOf rdf:resource="&dc;relation"/>
        <rdfs:isDefinedBy rdf:resource="http://purl.org/dc/terms/"/>
        <rdfs:subPropertyOf rdf:resource="&terms;relation"/>
    </owl:AnnotationProperty>
    


    <!-- http://purl.org/dc/terms/isReplacedBy -->

    <owl:AnnotationProperty rdf:about="&terms;isReplacedBy">
        <rdfs:label xml:lang="en">Is Replaced By</rdfs:label>
        <terms:issued rdf:datatype="&xsd;date">2000-07-11</terms:issued>
        <terms:modified rdf:datatype="&xsd;date">2008-01-14</terms:modified>
        <rdfs:comment xml:lang="en">A related resource that supplants, displaces, or supersedes the described resource.</rdfs:comment>
        <skos:note xml:lang="en">This term is intended to be used with non-literal values as defined in the DCMI Abstract Model (http://dublincore.org/documents/abstract-model/).  As of December 2007, the DCMI Usage Board is seeking a way to express this intention with a formal range declaration.</skos:note>
        <terms:hasVersion rdf:resource="http://dublincore.org/usage/terms/history/#isReplacedBy-003"/>
        <rdfs:subPropertyOf rdf:resource="&dc;relation"/>
        <rdfs:isDefinedBy rdf:resource="http://purl.org/dc/terms/"/>
        <rdfs:subPropertyOf rdf:resource="&terms;relation"/>
    </owl:AnnotationProperty>
    


    <!-- http://purl.org/dc/terms/isRequiredBy -->

    <owl:AnnotationProperty rdf:about="&terms;isRequiredBy">
        <rdfs:label xml:lang="en">Is Required By</rdfs:label>
        <terms:issued rdf:datatype="&xsd;date">2000-07-11</terms:issued>
        <terms:modified rdf:datatype="&xsd;date">2008-01-14</terms:modified>
        <rdfs:comment xml:lang="en">A related resource that requires the described resource to support its function, delivery, or coherence.</rdfs:comment>
        <skos:note xml:lang="en">This term is intended to be used with non-literal values as defined in the DCMI Abstract Model (http://dublincore.org/documents/abstract-model/).  As of December 2007, the DCMI Usage Board is seeking a way to express this intention with a formal range declaration.</skos:note>
        <terms:hasVersion rdf:resource="http://dublincore.org/usage/terms/history/#isRequiredBy-003"/>
        <rdfs:subPropertyOf rdf:resource="&dc;relation"/>
        <rdfs:isDefinedBy rdf:resource="http://purl.org/dc/terms/"/>
        <rdfs:subPropertyOf rdf:resource="&terms;relation"/>
    </owl:AnnotationProperty>
    


    <!-- http://purl.org/dc/terms/isVersionOf -->

    <owl:AnnotationProperty rdf:about="&terms;isVersionOf">
        <rdfs:label xml:lang="en">Is Version Of</rdfs:label>
        <terms:issued rdf:datatype="&xsd;date">2000-07-11</terms:issued>
        <terms:modified rdf:datatype="&xsd;date">2008-01-14</terms:modified>
        <rdfs:comment xml:lang="en">A related resource of which the described resource is a version, edition, or adaptation.</rdfs:comment>
        <terms:description xml:lang="en">Changes in version imply substantive changes in content rather than differences in format.</terms:description>
        <skos:note xml:lang="en">This term is intended to be used with non-literal values as defined in the DCMI Abstract Model (http://dublincore.org/documents/abstract-model/).  As of December 2007, the DCMI Usage Board is seeking a way to express this intention with a formal range declaration.</skos:note>
        <terms:hasVersion rdf:resource="http://dublincore.org/usage/terms/history/#isVersionOf-003"/>
        <rdfs:subPropertyOf rdf:resource="&dc;relation"/>
        <rdfs:isDefinedBy rdf:resource="http://purl.org/dc/terms/"/>
        <rdfs:subPropertyOf rdf:resource="&terms;relation"/>
    </owl:AnnotationProperty>
    


    <!-- http://purl.org/dc/terms/issued -->

    <owl:AnnotationProperty rdf:about="&terms;issued">
        <rdfs:label xml:lang="en">Date Issued</rdfs:label>
        <terms:issued rdf:datatype="&xsd;date">2000-07-11</terms:issued>
        <terms:modified rdf:datatype="&xsd;date">2008-01-14</terms:modified>
        <rdfs:comment xml:lang="en">Date of formal issuance (e.g., publication) of the resource.</rdfs:comment>
        <terms:hasVersion rdf:resource="http://dublincore.org/usage/terms/history/#issued-003"/>
        <rdfs:subPropertyOf rdf:resource="&dc;date"/>
        <rdfs:isDefinedBy rdf:resource="http://purl.org/dc/terms/"/>
    </owl:AnnotationProperty>
    


    <!-- http://purl.org/dc/terms/language -->

    <owl:AnnotationProperty rdf:about="&terms;language">
        <rdfs:label xml:lang="en">Language</rdfs:label>
        <terms:modified rdf:datatype="&xsd;date">2008-01-14</terms:modified>
        <terms:issued rdf:datatype="&xsd;date">2008-01-14</terms:issued>
        <rdfs:comment xml:lang="en">A language of the resource.</rdfs:comment>
        <terms:description xml:lang="en">Recommended best practice is to use a controlled vocabulary such as RFC 4646 [RFC4646].</terms:description>
        <terms:hasVersion rdf:resource="http://dublincore.org/usage/terms/history/#languageT-001"/>
        <rdfs:subPropertyOf rdf:resource="&dc;language"/>
        <rdfs:isDefinedBy rdf:resource="http://purl.org/dc/terms/"/>
    </owl:AnnotationProperty>
    


    <!-- http://purl.org/dc/terms/license -->

    <owl:AnnotationProperty rdf:about="&terms;license">
        <rdfs:label xml:lang="en">License</rdfs:label>
        <terms:issued rdf:datatype="&xsd;date">2004-06-14</terms:issued>
        <terms:modified rdf:datatype="&xsd;date">2008-01-14</terms:modified>
        <rdfs:comment xml:lang="en">A legal document giving official permission to do something with the resource.</rdfs:comment>
        <terms:hasVersion rdf:resource="http://dublincore.org/usage/terms/history/#license-002"/>
        <rdfs:subPropertyOf rdf:resource="&dc;rights"/>
        <rdfs:isDefinedBy rdf:resource="http://purl.org/dc/terms/"/>
    </owl:AnnotationProperty>
    


    <!-- http://purl.org/dc/terms/mediator -->

    <owl:AnnotationProperty rdf:about="&terms;mediator">
        <rdfs:label xml:lang="en">Mediator</rdfs:label>
        <terms:issued rdf:datatype="&xsd;date">2001-05-21</terms:issued>
        <terms:modified rdf:datatype="&xsd;date">2008-01-14</terms:modified>
        <rdfs:comment xml:lang="en">An entity that mediates access to the resource and for whom the resource is intended or useful.</rdfs:comment>
        <terms:description xml:lang="en">In an educational context, a mediator might be a parent, teacher, teaching assistant, or care-giver.</terms:description>
        <terms:hasVersion rdf:resource="http://dublincore.org/usage/terms/history/#mediator-003"/>
        <rdfs:isDefinedBy rdf:resource="http://purl.org/dc/terms/"/>
    </owl:AnnotationProperty>
    


    <!-- http://purl.org/dc/terms/medium -->

    <owl:AnnotationProperty rdf:about="&terms;medium">
        <rdfs:label xml:lang="en">Medium</rdfs:label>
        <terms:issued rdf:datatype="&xsd;date">2000-07-11</terms:issued>
        <terms:modified rdf:datatype="&xsd;date">2008-01-14</terms:modified>
        <rdfs:comment xml:lang="en">The material or physical carrier of the resource.</rdfs:comment>
        <terms:hasVersion rdf:resource="http://dublincore.org/usage/terms/history/#medium-003"/>
        <rdfs:subPropertyOf rdf:resource="&dc;format"/>
        <rdfs:isDefinedBy rdf:resource="http://purl.org/dc/terms/"/>
    </owl:AnnotationProperty>
    


    <!-- http://purl.org/dc/terms/modified -->

    <owl:AnnotationProperty rdf:about="&terms;modified">
        <rdfs:label xml:lang="en">Date Modified</rdfs:label>
        <terms:issued rdf:datatype="&xsd;date">2000-07-11</terms:issued>
        <terms:modified rdf:datatype="&xsd;date">2008-01-14</terms:modified>
        <rdfs:comment xml:lang="en">Date on which the resource was changed.</rdfs:comment>
        <terms:hasVersion rdf:resource="http://dublincore.org/usage/terms/history/#modified-003"/>
        <rdfs:subPropertyOf rdf:resource="&dc;date"/>
        <rdfs:isDefinedBy rdf:resource="http://purl.org/dc/terms/"/>
    </owl:AnnotationProperty>
    


    <!-- http://purl.org/dc/terms/publisher -->

    <owl:AnnotationProperty rdf:about="&terms;publisher">
        <rdfs:label xml:lang="en">Publisher</rdfs:label>
        <terms:issued rdf:datatype="&xsd;date">2008-01-14</terms:issued>
        <terms:modified rdf:datatype="&xsd;date">2010-10-11</terms:modified>
        <rdfs:comment xml:lang="en">An entity responsible for making the resource available.</rdfs:comment>
        <terms:description xml:lang="en">Examples of a Publisher include a person, an organization, or a service.</terms:description>
        <terms:hasVersion rdf:resource="http://dublincore.org/usage/terms/history/#publisherT-001"/>
        <rdfs:subPropertyOf rdf:resource="&dc;publisher"/>
        <rdfs:isDefinedBy rdf:resource="http://purl.org/dc/terms/"/>
    </owl:AnnotationProperty>
    


    <!-- http://purl.org/dc/terms/references -->

    <owl:AnnotationProperty rdf:about="&terms;references">
        <rdfs:label xml:lang="en">References</rdfs:label>
        <terms:issued rdf:datatype="&xsd;date">2000-07-11</terms:issued>
        <terms:modified rdf:datatype="&xsd;date">2008-01-14</terms:modified>
        <rdfs:comment xml:lang="en">A related resource that is referenced, cited, or otherwise pointed to by the described resource.</rdfs:comment>
        <skos:note xml:lang="en">This term is intended to be used with non-literal values as defined in the DCMI Abstract Model (http://dublincore.org/documents/abstract-model/).  As of December 2007, the DCMI Usage Board is seeking a way to express this intention with a formal range declaration.</skos:note>
        <terms:hasVersion rdf:resource="http://dublincore.org/usage/terms/history/#references-003"/>
        <rdfs:subPropertyOf rdf:resource="&dc;relation"/>
        <rdfs:isDefinedBy rdf:resource="http://purl.org/dc/terms/"/>
        <rdfs:subPropertyOf rdf:resource="&terms;relation"/>
    </owl:AnnotationProperty>
    


    <!-- http://purl.org/dc/terms/relation -->

    <owl:AnnotationProperty rdf:about="&terms;relation">
        <rdfs:label xml:lang="en">Relation</rdfs:label>
        <terms:modified rdf:datatype="&xsd;date">2008-01-14</terms:modified>
        <terms:issued rdf:datatype="&xsd;date">2008-01-14</terms:issued>
        <rdfs:comment xml:lang="en">A related resource.</rdfs:comment>
        <terms:description xml:lang="en">Recommended best practice is to identify the related resource by means of a string conforming to a formal identification system. </terms:description>
        <skos:note xml:lang="en">This term is intended to be used with non-literal values as defined in the DCMI Abstract Model (http://dublincore.org/documents/abstract-model/).  As of December 2007, the DCMI Usage Board is seeking a way to express this intention with a formal range declaration.</skos:note>
        <terms:hasVersion rdf:resource="http://dublincore.org/usage/terms/history/#relationT-001"/>
        <rdfs:subPropertyOf rdf:resource="&dc;relation"/>
        <rdfs:isDefinedBy rdf:resource="http://purl.org/dc/terms/"/>
    </owl:AnnotationProperty>
    


    <!-- http://purl.org/dc/terms/replaces -->

    <owl:AnnotationProperty rdf:about="&terms;replaces">
        <rdfs:label xml:lang="en">Replaces</rdfs:label>
        <terms:issued rdf:datatype="&xsd;date">2000-07-11</terms:issued>
        <terms:modified rdf:datatype="&xsd;date">2008-01-14</terms:modified>
        <rdfs:comment xml:lang="en">A related resource that is supplanted, displaced, or superseded by the described resource.</rdfs:comment>
        <skos:note xml:lang="en">This term is intended to be used with non-literal values as defined in the DCMI Abstract Model (http://dublincore.org/documents/abstract-model/).  As of December 2007, the DCMI Usage Board is seeking a way to express this intention with a formal range declaration.</skos:note>
        <terms:hasVersion rdf:resource="http://dublincore.org/usage/terms/history/#replaces-003"/>
        <rdfs:subPropertyOf rdf:resource="&dc;relation"/>
        <rdfs:isDefinedBy rdf:resource="http://purl.org/dc/terms/"/>
        <rdfs:subPropertyOf rdf:resource="&terms;relation"/>
    </owl:AnnotationProperty>
    


    <!-- http://purl.org/dc/terms/requires -->

    <owl:AnnotationProperty rdf:about="&terms;requires">
        <rdfs:label xml:lang="en">Requires</rdfs:label>
        <terms:issued rdf:datatype="&xsd;date">2000-07-11</terms:issued>
        <terms:modified rdf:datatype="&xsd;date">2008-01-14</terms:modified>
        <rdfs:comment xml:lang="en">A related resource that is required by the described resource to support its function, delivery, or coherence.</rdfs:comment>
        <skos:note xml:lang="en">This term is intended to be used with non-literal values as defined in the DCMI Abstract Model (http://dublincore.org/documents/abstract-model/).  As of December 2007, the DCMI Usage Board is seeking a way to express this intention with a formal range declaration.</skos:note>
        <terms:hasVersion rdf:resource="http://dublincore.org/usage/terms/history/#requires-003"/>
        <rdfs:subPropertyOf rdf:resource="&dc;relation"/>
        <rdfs:isDefinedBy rdf:resource="http://purl.org/dc/terms/"/>
        <rdfs:subPropertyOf rdf:resource="&terms;relation"/>
    </owl:AnnotationProperty>
    


    <!-- http://purl.org/dc/terms/rights -->

    <owl:AnnotationProperty rdf:about="&terms;rights">
        <rdfs:label xml:lang="en">Rights</rdfs:label>
        <terms:issued rdf:datatype="&xsd;date">2008-01-14</terms:issued>
        <terms:modified rdf:datatype="&xsd;date">2008-01-14</terms:modified>
        <rdfs:comment xml:lang="en">Information about rights held in and over the resource.</rdfs:comment>
        <terms:description xml:lang="en">Typically, rights information includes a statement about various property rights associated with the resource, including intellectual property rights.</terms:description>
        <terms:hasVersion rdf:resource="http://dublincore.org/usage/terms/history/#rightsT-001"/>
        <rdfs:subPropertyOf rdf:resource="&dc;rights"/>
        <rdfs:isDefinedBy rdf:resource="http://purl.org/dc/terms/"/>
    </owl:AnnotationProperty>
    


    <!-- http://purl.org/dc/terms/source -->

    <owl:AnnotationProperty rdf:about="&terms;source">
        <rdfs:label xml:lang="en">Source</rdfs:label>
        <terms:issued rdf:datatype="&xsd;date">2008-01-14</terms:issued>
        <terms:modified rdf:datatype="&xsd;date">2008-01-14</terms:modified>
        <rdfs:comment xml:lang="en">A related resource from which the described resource is derived.</rdfs:comment>
        <terms:description xml:lang="en">The described resource may be derived from the related resource in whole or in part. Recommended best practice is to identify the related resource by means of a string conforming to a formal identification system.</terms:description>
        <skos:note xml:lang="en">This term is intended to be used with non-literal values as defined in the DCMI Abstract Model (http://dublincore.org/documents/abstract-model/).  As of December 2007, the DCMI Usage Board is seeking a way to express this intention with a formal range declaration.</skos:note>
        <terms:hasVersion rdf:resource="http://dublincore.org/usage/terms/history/#sourceT-001"/>
        <rdfs:subPropertyOf rdf:resource="&dc;source"/>
        <rdfs:isDefinedBy rdf:resource="http://purl.org/dc/terms/"/>
        <rdfs:subPropertyOf rdf:resource="&terms;relation"/>
    </owl:AnnotationProperty>
    


    <!-- http://purl.org/dc/terms/spatial -->

    <owl:AnnotationProperty rdf:about="&terms;spatial">
        <rdfs:label xml:lang="en">Spatial Coverage</rdfs:label>
        <terms:issued rdf:datatype="&xsd;date">2000-07-11</terms:issued>
        <terms:modified rdf:datatype="&xsd;date">2008-01-14</terms:modified>
        <rdfs:comment xml:lang="en">Spatial characteristics of the resource.</rdfs:comment>
        <terms:hasVersion rdf:resource="http://dublincore.org/usage/terms/history/#spatial-003"/>
        <rdfs:subPropertyOf rdf:resource="&dc;coverage"/>
        <rdfs:isDefinedBy rdf:resource="http://purl.org/dc/terms/"/>
    </owl:AnnotationProperty>
    


    <!-- http://purl.org/dc/terms/subject -->

    <owl:AnnotationProperty rdf:about="&terms;subject">
        <rdfs:label xml:lang="en">Subject</rdfs:label>
        <terms:issued rdf:datatype="&xsd;date">2008-01-14</terms:issued>
        <terms:modified rdf:datatype="&xsd;date">2012-06-14</terms:modified>
        <rdfs:comment xml:lang="en">The topic of the resource.</rdfs:comment>
        <skos:note xml:lang="en">This term is intended to be used with non-literal values as defined in the DCMI Abstract Model (http://dublincore.org/documents/abstract-model/).  As of December 2007, the DCMI Usage Board is seeking a way to express this intention with a formal range declaration.</skos:note>
        <terms:description xml:lang="en">Typically, the subject will be represented using keywords, key phrases, or classification codes. Recommended best practice is to use a controlled vocabulary.</terms:description>
        <terms:hasVersion rdf:resource="http://dublincore.org/usage/terms/history/#subjectT-002"/>
        <rdfs:subPropertyOf rdf:resource="&dc;subject"/>
        <rdfs:isDefinedBy rdf:resource="http://purl.org/dc/terms/"/>
    </owl:AnnotationProperty>
    


    <!-- http://purl.org/dc/terms/tableOfContents -->

    <owl:AnnotationProperty rdf:about="&terms;tableOfContents">
        <rdfs:label xml:lang="en">Table Of Contents</rdfs:label>
        <terms:issued rdf:datatype="&xsd;date">2000-07-11</terms:issued>
        <terms:modified rdf:datatype="&xsd;date">2008-01-14</terms:modified>
        <rdfs:comment xml:lang="en">A list of subunits of the resource.</rdfs:comment>
        <terms:hasVersion rdf:resource="http://dublincore.org/usage/terms/history/#tableOfContents-003"/>
        <rdfs:subPropertyOf rdf:resource="&dc;description"/>
        <rdfs:isDefinedBy rdf:resource="http://purl.org/dc/terms/"/>
        <rdfs:subPropertyOf rdf:resource="&terms;description"/>
    </owl:AnnotationProperty>
    


    <!-- http://purl.org/dc/terms/temporal -->

    <owl:AnnotationProperty rdf:about="&terms;temporal">
        <rdfs:label xml:lang="en">Temporal Coverage</rdfs:label>
        <terms:issued rdf:datatype="&xsd;date">2000-07-11</terms:issued>
        <terms:modified rdf:datatype="&xsd;date">2008-01-14</terms:modified>
        <rdfs:comment xml:lang="en">Temporal characteristics of the resource.</rdfs:comment>
        <terms:hasVersion rdf:resource="http://dublincore.org/usage/terms/history/#temporal-003"/>
        <rdfs:subPropertyOf rdf:resource="&dc;coverage"/>
        <rdfs:isDefinedBy rdf:resource="http://purl.org/dc/terms/"/>
    </owl:AnnotationProperty>
    


    <!-- http://purl.org/dc/terms/title -->

    <owl:AnnotationProperty rdf:about="&terms;title">
        <rdfs:label xml:lang="en">Title</rdfs:label>
        <terms:issued rdf:datatype="&xsd;date">2008-01-14</terms:issued>
        <terms:modified rdf:datatype="&xsd;date">2010-10-11</terms:modified>
        <rdfs:comment xml:lang="en">A name given to the resource.</rdfs:comment>
        <terms:hasVersion rdf:resource="http://dublincore.org/usage/terms/history/#titleT-002"/>
        <rdfs:subPropertyOf rdf:resource="&dc;title"/>
        <rdfs:isDefinedBy rdf:resource="http://purl.org/dc/terms/"/>
    </owl:AnnotationProperty>
    


    <!-- http://purl.org/dc/terms/type -->

    <owl:AnnotationProperty rdf:about="&terms;type">
        <rdfs:label xml:lang="en">Type</rdfs:label>
        <terms:modified rdf:datatype="&xsd;date">2008-01-14</terms:modified>
        <terms:issued rdf:datatype="&xsd;date">2008-01-14</terms:issued>
        <terms:description xml:lang="en">Recommended best practice is to use a controlled vocabulary such as the DCMI Type Vocabulary [DCMITYPE]. To describe the file format, physical medium, or dimensions of the resource, use the Format element.</terms:description>
        <rdfs:comment xml:lang="en">The nature or genre of the resource.</rdfs:comment>
        <terms:hasVersion rdf:resource="http://dublincore.org/usage/terms/history/#typeT-001"/>
        <rdfs:subPropertyOf rdf:resource="&dc;type"/>
        <rdfs:isDefinedBy rdf:resource="http://purl.org/dc/terms/"/>
    </owl:AnnotationProperty>
    


    <!-- http://purl.org/dc/terms/valid -->

    <owl:AnnotationProperty rdf:about="&terms;valid">
        <rdfs:label xml:lang="en">Date Valid</rdfs:label>
        <terms:issued rdf:datatype="&xsd;date">2000-07-11</terms:issued>
        <terms:modified rdf:datatype="&xsd;date">2008-01-14</terms:modified>
        <rdfs:comment xml:lang="en">Date (often a range) of validity of a resource.</rdfs:comment>
        <terms:hasVersion rdf:resource="http://dublincore.org/usage/terms/history/#valid-003"/>
        <rdfs:subPropertyOf rdf:resource="&dc;date"/>
        <rdfs:isDefinedBy rdf:resource="http://purl.org/dc/terms/"/>
    </owl:AnnotationProperty>
    


    <!-- http://purl.org/vocab/vann/preferredNamespacePrefix -->

    <owl:AnnotationProperty rdf:about="&vann;preferredNamespacePrefix"/>
    


    <!-- http://www.w3.org/2004/02/skos/core#note -->

    <owl:AnnotationProperty rdf:about="&skos;note"/>
    


    <!-- 
    ///////////////////////////////////////////////////////////////////////////////////////
    //
    // Datatypes
    //
    ///////////////////////////////////////////////////////////////////////////////////////
     -->

    


    <!-- http://purl.org/dc/terms/Box -->

    <rdfs:Datatype rdf:about="&terms;Box">
        <rdfs:label xml:lang="en">DCMI Box</rdfs:label>
        <terms:issued rdf:datatype="&xsd;date">2000-07-11</terms:issued>
        <terms:modified rdf:datatype="&xsd;date">2008-01-14</terms:modified>
        <rdfs:comment xml:lang="en">The set of regions in space defined by their geographic coordinates according to the DCMI Box Encoding Scheme.</rdfs:comment>
        <rdfs:seeAlso rdf:resource="http://dublincore.org/documents/dcmi-box/"/>
        <terms:hasVersion rdf:resource="http://dublincore.org/usage/terms/history/#Box-003"/>
        <rdfs:isDefinedBy rdf:resource="http://purl.org/dc/terms/"/>
    </rdfs:Datatype>
    


    <!-- http://purl.org/dc/terms/ISO3166 -->

    <rdfs:Datatype rdf:about="&terms;ISO3166">
        <rdfs:label xml:lang="en">ISO 3166</rdfs:label>
        <terms:issued rdf:datatype="&xsd;date">2000-07-11</terms:issued>
        <terms:modified rdf:datatype="&xsd;date">2008-01-14</terms:modified>
        <rdfs:comment xml:lang="en">The set of codes listed in ISO 3166-1 for the representation of names of countries.</rdfs:comment>
        <terms:hasVersion rdf:resource="http://dublincore.org/usage/terms/history/#ISO3166-004"/>
        <rdfs:isDefinedBy rdf:resource="http://purl.org/dc/terms/"/>
        <rdfs:seeAlso rdf:resource="http://www.iso.org/iso/en/prods-services/iso3166ma/02iso-3166-code-lists/list-en1.html"/>
    </rdfs:Datatype>
    


    <!-- http://purl.org/dc/terms/ISO639-2 -->

    <rdfs:Datatype rdf:about="&terms;ISO639-2">
        <rdfs:label xml:lang="en">ISO 639-2</rdfs:label>
        <terms:issued rdf:datatype="&xsd;date">2000-07-11</terms:issued>
        <terms:modified rdf:datatype="&xsd;date">2008-01-14</terms:modified>
        <rdfs:comment xml:lang="en">The three-letter alphabetic codes listed in ISO639-2 for the representation of names of languages.</rdfs:comment>
        <terms:hasVersion rdf:resource="http://dublincore.org/usage/terms/history/#ISO639-2-003"/>
        <rdfs:seeAlso rdf:resource="http://lcweb.loc.gov/standards/iso639-2/langhome.html"/>
        <rdfs:isDefinedBy rdf:resource="http://purl.org/dc/terms/"/>
    </rdfs:Datatype>
    


    <!-- http://purl.org/dc/terms/ISO639-3 -->

    <rdfs:Datatype rdf:about="&terms;ISO639-3">
        <rdfs:label xml:lang="en">ISO 639-3</rdfs:label>
        <terms:issued rdf:datatype="&xsd;date">2008-01-14</terms:issued>
        <rdfs:comment xml:lang="en">The set of three-letter codes listed in ISO 639-3 for the representation of names of languages.</rdfs:comment>
        <terms:hasVersion rdf:resource="http://dublincore.org/usage/terms/history/#ISO639-3-001"/>
        <rdfs:isDefinedBy rdf:resource="http://purl.org/dc/terms/"/>
        <rdfs:seeAlso rdf:resource="http://www.sil.org/iso639-3/"/>
    </rdfs:Datatype>
    


    <!-- http://purl.org/dc/terms/Period -->

    <rdfs:Datatype rdf:about="&terms;Period">
        <rdfs:label xml:lang="en">DCMI Period</rdfs:label>
        <terms:issued rdf:datatype="&xsd;date">2000-07-11</terms:issued>
        <terms:modified rdf:datatype="&xsd;date">2008-01-14</terms:modified>
        <rdfs:comment xml:lang="en">The set of time intervals defined by their limits according to the DCMI Period Encoding Scheme.</rdfs:comment>
        <rdfs:seeAlso rdf:resource="http://dublincore.org/documents/dcmi-period/"/>
        <terms:hasVersion rdf:resource="http://dublincore.org/usage/terms/history/#Period-003"/>
        <rdfs:isDefinedBy rdf:resource="http://purl.org/dc/terms/"/>
    </rdfs:Datatype>
    


    <!-- http://purl.org/dc/terms/Point -->

    <rdfs:Datatype rdf:about="&terms;Point">
        <rdfs:label xml:lang="en">DCMI Point</rdfs:label>
        <terms:issued rdf:datatype="&xsd;date">2000-07-11</terms:issued>
        <terms:modified rdf:datatype="&xsd;date">2008-01-14</terms:modified>
        <rdfs:comment xml:lang="en">The set of points in space defined by their geographic coordinates according to the DCMI Point Encoding Scheme.</rdfs:comment>
        <rdfs:seeAlso rdf:resource="http://dublincore.org/documents/dcmi-point/"/>
        <terms:hasVersion rdf:resource="http://dublincore.org/usage/terms/history/#Point-003"/>
        <rdfs:isDefinedBy rdf:resource="http://purl.org/dc/terms/"/>
    </rdfs:Datatype>
    


    <!-- http://purl.org/dc/terms/RFC1766 -->

    <rdfs:Datatype rdf:about="&terms;RFC1766">
        <rdfs:label xml:lang="en">RFC 1766</rdfs:label>
        <terms:issued rdf:datatype="&xsd;date">2000-07-11</terms:issued>
        <terms:modified rdf:datatype="&xsd;date">2008-01-14</terms:modified>
        <rdfs:comment xml:lang="en">The set of tags, constructed according to RFC 1766, for the identification of languages.</rdfs:comment>
        <terms:hasVersion rdf:resource="http://dublincore.org/usage/terms/history/#RFC1766-003"/>
        <rdfs:isDefinedBy rdf:resource="http://purl.org/dc/terms/"/>
        <rdfs:seeAlso rdf:resource="http://www.ietf.org/rfc/rfc1766.txt"/>
    </rdfs:Datatype>
    


    <!-- http://purl.org/dc/terms/RFC3066 -->

    <rdfs:Datatype rdf:about="&terms;RFC3066">
        <rdfs:label xml:lang="en">RFC 3066</rdfs:label>
        <terms:issued rdf:datatype="&xsd;date">2002-07-13</terms:issued>
        <terms:modified rdf:datatype="&xsd;date">2008-01-14</terms:modified>
        <terms:description xml:lang="en">RFC 3066 has been obsoleted by RFC 4646.</terms:description>
        <rdfs:comment xml:lang="en">The set of tags constructed according to RFC 3066 for the identification of languages.</rdfs:comment>
        <terms:hasVersion rdf:resource="http://dublincore.org/usage/terms/history/#RFC3066-002"/>
        <rdfs:isDefinedBy rdf:resource="http://purl.org/dc/terms/"/>
        <rdfs:seeAlso rdf:resource="http://www.ietf.org/rfc/rfc3066.txt"/>
    </rdfs:Datatype>
    


    <!-- http://purl.org/dc/terms/RFC4646 -->

    <rdfs:Datatype rdf:about="&terms;RFC4646">
        <rdfs:label xml:lang="en">RFC 4646</rdfs:label>
        <terms:issued rdf:datatype="&xsd;date">2008-01-14</terms:issued>
        <terms:description xml:lang="en">RFC 4646 obsoletes RFC 3066.</terms:description>
        <rdfs:comment xml:lang="en">The set of tags constructed according to RFC 4646 for the identification of languages.</rdfs:comment>
        <terms:hasVersion rdf:resource="http://dublincore.org/usage/terms/history/#RFC4646-001"/>
        <rdfs:isDefinedBy rdf:resource="http://purl.org/dc/terms/"/>
        <rdfs:seeAlso rdf:resource="http://www.ietf.org/rfc/rfc4646.txt"/>
    </rdfs:Datatype>
    


    <!-- http://purl.org/dc/terms/RFC5646 -->

    <rdfs:Datatype rdf:about="&terms;RFC5646">
        <rdfs:label xml:lang="en">RFC 5646</rdfs:label>
        <terms:issued rdf:datatype="&xsd;date">2010-10-11</terms:issued>
        <terms:description xml:lang="en">RFC 5646 obsoletes RFC 4646.</terms:description>
        <rdfs:comment xml:lang="en">The set of tags constructed according to RFC 5646 for the identification of languages.</rdfs:comment>
        <terms:hasVersion rdf:resource="http://dublincore.org/usage/terms/history/#RFC5646-001"/>
        <rdfs:isDefinedBy rdf:resource="http://purl.org/dc/terms/"/>
        <rdfs:seeAlso rdf:resource="http://www.ietf.org/rfc/rfc5646.txt"/>
    </rdfs:Datatype>
    


    <!-- http://purl.org/dc/terms/URI -->

    <rdfs:Datatype rdf:about="&terms;URI">
        <rdfs:label xml:lang="en">URI</rdfs:label>
        <terms:issued rdf:datatype="&xsd;date">2000-07-11</terms:issued>
        <terms:modified rdf:datatype="&xsd;date">2008-01-14</terms:modified>
        <rdfs:comment xml:lang="en">The set of identifiers constructed according to the generic syntax for Uniform Resource Identifiers as specified by the Internet Engineering Task Force.</rdfs:comment>
        <terms:hasVersion rdf:resource="http://dublincore.org/usage/terms/history/#URI-003"/>
        <rdfs:isDefinedBy rdf:resource="http://purl.org/dc/terms/"/>
        <rdfs:seeAlso rdf:resource="http://www.ietf.org/rfc/rfc3986.txt"/>
    </rdfs:Datatype>
    


    <!-- http://purl.org/dc/terms/W3CDTF -->

    <rdfs:Datatype rdf:about="&terms;W3CDTF">
        <rdfs:label xml:lang="en">W3C-DTF</rdfs:label>
        <terms:issued rdf:datatype="&xsd;date">2000-07-11</terms:issued>
        <terms:modified rdf:datatype="&xsd;date">2008-01-14</terms:modified>
        <rdfs:comment xml:lang="en">The set of dates and times constructed according to the W3C Date and Time Formats Specification.</rdfs:comment>
        <terms:hasVersion rdf:resource="http://dublincore.org/usage/terms/history/#W3CDTF-003"/>
        <rdfs:isDefinedBy rdf:resource="http://purl.org/dc/terms/"/>
        <rdfs:seeAlso rdf:resource="http://www.w3.org/TR/NOTE-datetime"/>
    </rdfs:Datatype>
    


    <!-- http://www.w3.org/2001/XMLSchema#date -->

    <rdfs:Datatype rdf:about="&xsd;date"/>
    


    <!-- 
    ///////////////////////////////////////////////////////////////////////////////////////
    //
    // Object Properties
    //
    ///////////////////////////////////////////////////////////////////////////////////////
     -->

    


    <!-- http://purl.org/dc/terms/accessRights -->

    <owl:ObjectProperty rdf:about="&terms;accessRights">
        <rdfs:label xml:lang="en">Access Rights</rdfs:label>
        <terms:issued rdf:datatype="&xsd;date">2003-02-15</terms:issued>
        <terms:modified rdf:datatype="&xsd;date">2008-01-14</terms:modified>
        <terms:description xml:lang="en">Access Rights may include information regarding access or restrictions based on privacy, security, or other policies.</terms:description>
        <rdfs:comment xml:lang="en">Information about who can access the resource or an indication of its security status.</rdfs:comment>
        <terms:hasVersion rdf:resource="http://dublincore.org/usage/terms/history/#accessRights-002"/>
        <rdfs:isDefinedBy rdf:resource="http://purl.org/dc/terms/"/>
        <rdfs:range rdf:resource="&terms;RightsStatement"/>
        <rdfs:subPropertyOf rdf:resource="&terms;rights"/>
    </owl:ObjectProperty>
    


    <!-- http://purl.org/dc/terms/accrualMethod -->

    <owl:ObjectProperty rdf:about="&terms;accrualMethod">
        <rdfs:label xml:lang="en">Accrual Method</rdfs:label>
        <terms:issued rdf:datatype="&xsd;date">2005-06-13</terms:issued>
        <terms:modified rdf:datatype="&xsd;date">2010-10-11</terms:modified>
        <rdfs:comment xml:lang="en">The method by which items are added to a collection.</rdfs:comment>
        <terms:hasVersion rdf:resource="http://dublincore.org/usage/terms/history/#accrualMethod-003"/>
        <rdfs:isDefinedBy rdf:resource="http://purl.org/dc/terms/"/>
        <rdfs:range rdf:resource="&terms;MethodOfAccrual"/>
    </owl:ObjectProperty>
    


    <!-- http://purl.org/dc/terms/accrualPeriodicity -->

    <owl:ObjectProperty rdf:about="&terms;accrualPeriodicity">
        <rdfs:label xml:lang="en">Accrual Periodicity</rdfs:label>
        <terms:issued rdf:datatype="&xsd;date">2005-06-13</terms:issued>
        <terms:modified rdf:datatype="&xsd;date">2010-10-11</terms:modified>
        <rdfs:comment xml:lang="en">The frequency with which items are added to a collection.</rdfs:comment>
        <terms:hasVersion rdf:resource="http://dublincore.org/usage/terms/history/#accrualPeriodicity-003"/>
        <rdfs:isDefinedBy rdf:resource="http://purl.org/dc/terms/"/>
        <rdfs:range rdf:resource="&terms;Frequency"/>
    </owl:ObjectProperty>
    


    <!-- http://purl.org/dc/terms/accrualPolicy -->

    <owl:ObjectProperty rdf:about="&terms;accrualPolicy">
        <rdfs:label xml:lang="en">Accrual Policy</rdfs:label>
        <terms:issued rdf:datatype="&xsd;date">2005-06-13</terms:issued>
        <terms:modified rdf:datatype="&xsd;date">2010-10-11</terms:modified>
        <rdfs:comment xml:lang="en">The policy governing the addition of items to a collection.</rdfs:comment>
        <terms:hasVersion rdf:resource="http://dublincore.org/usage/terms/history/#accrualPolicy-003"/>
        <rdfs:isDefinedBy rdf:resource="http://purl.org/dc/terms/"/>
        <rdfs:range rdf:resource="&terms;Policy"/>
    </owl:ObjectProperty>
    


    <!-- http://purl.org/dc/terms/audience -->

    <owl:ObjectProperty rdf:about="&terms;audience">
        <rdfs:label xml:lang="en">Audience</rdfs:label>
        <terms:issued rdf:datatype="&xsd;date">2001-05-21</terms:issued>
        <terms:modified rdf:datatype="&xsd;date">2008-01-14</terms:modified>
        <rdfs:comment xml:lang="en">A class of entity for whom the resource is intended or useful.</rdfs:comment>
        <terms:hasVersion rdf:resource="http://dublincore.org/usage/terms/history/#audience-003"/>
        <rdfs:isDefinedBy rdf:resource="http://purl.org/dc/terms/"/>
        <rdfs:range rdf:resource="&terms;AgentClass"/>
    </owl:ObjectProperty>
    


    <!-- http://purl.org/dc/terms/conformsTo -->

    <owl:ObjectProperty rdf:about="&terms;conformsTo">
        <rdfs:label xml:lang="en">Conforms To</rdfs:label>
        <terms:issued rdf:datatype="&xsd;date">2001-05-21</terms:issued>
        <terms:modified rdf:datatype="&xsd;date">2008-01-14</terms:modified>
        <rdfs:comment xml:lang="en">An established standard to which the described resource conforms.</rdfs:comment>
        <terms:hasVersion rdf:resource="http://dublincore.org/usage/terms/history/#conformsTo-003"/>
        <rdfs:isDefinedBy rdf:resource="http://purl.org/dc/terms/"/>
        <rdfs:range rdf:resource="&terms;Standard"/>
    </owl:ObjectProperty>
    


    <!-- http://purl.org/dc/terms/contributor -->

    <owl:ObjectProperty rdf:about="&terms;contributor">
        <rdfs:label xml:lang="en">Contributor</rdfs:label>
        <terms:issued rdf:datatype="&xsd;date">2008-01-14</terms:issued>
        <terms:modified rdf:datatype="&xsd;date">2010-10-11</terms:modified>
        <rdfs:comment xml:lang="en">An entity responsible for making contributions to the resource.</rdfs:comment>
        <terms:description xml:lang="en">Examples of a Contributor include a person, an organization, or a service.</terms:description>
        <terms:hasVersion rdf:resource="http://dublincore.org/usage/terms/history/#contributorT-001"/>
        <rdfs:isDefinedBy rdf:resource="http://purl.org/dc/terms/"/>
        <rdfs:range rdf:resource="&terms;Agent"/>
    </owl:ObjectProperty>
    


    <!-- http://purl.org/dc/terms/coverage -->

    <owl:ObjectProperty rdf:about="&terms;coverage">
        <rdfs:label xml:lang="en">Coverage</rdfs:label>
        <terms:issued rdf:datatype="&xsd;date">2008-01-14</terms:issued>
        <terms:modified rdf:datatype="&xsd;date">2008-01-14</terms:modified>
        <terms:description xml:lang="en">Spatial topic and spatial applicability may be a named place or a location specified by its geographic coordinates. Temporal topic may be a named period, date, or date range. A jurisdiction may be a named administrative entity or a geographic place to which the resource applies. Recommended best practice is to use a controlled vocabulary such as the Thesaurus of Geographic Names [TGN]. Where appropriate, named places or time periods can be used in preference to numeric identifiers such as sets of coordinates or date ranges.</terms:description>
        <rdfs:comment xml:lang="en">The spatial or temporal topic of the resource, the spatial applicability of the resource, or the jurisdiction under which the resource is relevant.</rdfs:comment>
        <terms:hasVersion rdf:resource="http://dublincore.org/usage/terms/history/#coverageT-001"/>
        <rdfs:isDefinedBy rdf:resource="http://purl.org/dc/terms/"/>
        <rdfs:range rdf:resource="&terms;LocationPeriodOrJurisdiction"/>
    </owl:ObjectProperty>
    


    <!-- http://purl.org/dc/terms/creator -->

    <owl:ObjectProperty rdf:about="&terms;creator">
        <rdfs:label xml:lang="en">Creator</rdfs:label>
        <terms:issued rdf:datatype="&xsd;date">2008-01-14</terms:issued>
        <terms:modified rdf:datatype="&xsd;date">2010-10-11</terms:modified>
        <rdfs:comment xml:lang="en">An entity primarily responsible for making the resource.</rdfs:comment>
        <terms:description xml:lang="en">Examples of a Creator include a person, an organization, or a service.</terms:description>
        <terms:hasVersion rdf:resource="http://dublincore.org/usage/terms/history/#creatorT-002"/>
        <rdfs:isDefinedBy rdf:resource="http://purl.org/dc/terms/"/>
        <rdfs:range rdf:resource="&terms;Agent"/>
        <rdfs:subPropertyOf rdf:resource="&terms;contributor"/>
    </owl:ObjectProperty>
    


    <!-- http://purl.org/dc/terms/educationLevel -->

    <owl:ObjectProperty rdf:about="&terms;educationLevel">
        <rdfs:label xml:lang="en">Audience Education Level</rdfs:label>
        <terms:issued rdf:datatype="&xsd;date">2002-07-13</terms:issued>
        <terms:modified rdf:datatype="&xsd;date">2008-01-14</terms:modified>
        <rdfs:comment xml:lang="en">A class of entity, defined in terms of progression through an educational or training context, for which the described resource is intended.</rdfs:comment>
        <terms:hasVersion rdf:resource="http://dublincore.org/usage/terms/history/#educationLevel-002"/>
        <rdfs:isDefinedBy rdf:resource="http://purl.org/dc/terms/"/>
        <rdfs:range rdf:resource="&terms;AgentClass"/>
        <rdfs:subPropertyOf rdf:resource="&terms;audience"/>
    </owl:ObjectProperty>
    


    <!-- http://purl.org/dc/terms/extent -->

    <owl:ObjectProperty rdf:about="&terms;extent">
        <rdfs:label xml:lang="en">Extent</rdfs:label>
        <terms:issued rdf:datatype="&xsd;date">2000-07-11</terms:issued>
        <terms:modified rdf:datatype="&xsd;date">2008-01-14</terms:modified>
        <rdfs:comment xml:lang="en">The size or duration of the resource.</rdfs:comment>
        <terms:hasVersion rdf:resource="http://dublincore.org/usage/terms/history/#extent-003"/>
        <rdfs:isDefinedBy rdf:resource="http://purl.org/dc/terms/"/>
        <rdfs:range rdf:resource="&terms;SizeOrDuration"/>
        <rdfs:subPropertyOf rdf:resource="&terms;format"/>
    </owl:ObjectProperty>
    


    <!-- http://purl.org/dc/terms/format -->

    <owl:ObjectProperty rdf:about="&terms;format">
        <rdfs:label xml:lang="en">Format</rdfs:label>
        <terms:issued rdf:datatype="&xsd;date">2008-01-14</terms:issued>
        <terms:modified rdf:datatype="&xsd;date">2008-01-14</terms:modified>
        <terms:description xml:lang="en">Examples of dimensions include size and duration. Recommended best practice is to use a controlled vocabulary such as the list of Internet Media Types [MIME].</terms:description>
        <rdfs:comment xml:lang="en">The file format, physical medium, or dimensions of the resource.</rdfs:comment>
        <terms:hasVersion rdf:resource="http://dublincore.org/usage/terms/history/#formatT-001"/>
        <rdfs:isDefinedBy rdf:resource="http://purl.org/dc/terms/"/>
        <rdfs:range rdf:resource="&terms;MediaTypeOrExtent"/>
    </owl:ObjectProperty>
    


    <!-- http://purl.org/dc/terms/instructionalMethod -->

    <owl:ObjectProperty rdf:about="&terms;instructionalMethod">
        <rdfs:label xml:lang="en">Instructional Method</rdfs:label>
        <terms:issued rdf:datatype="&xsd;date">2005-06-13</terms:issued>
        <terms:modified rdf:datatype="&xsd;date">2008-01-14</terms:modified>
        <rdfs:comment xml:lang="en">A process, used to engender knowledge, attitudes and skills, that the described resource is designed to support.</rdfs:comment>
        <terms:description xml:lang="en">Instructional Method will typically include ways of presenting instructional materials or conducting instructional activities, patterns of learner-to-learner and learner-to-instructor interactions, and mechanisms by which group and individual levels of learning are measured.  Instructional methods include all aspects of the instruction and learning processes from planning and implementation through evaluation and feedback.</terms:description>
        <terms:hasVersion rdf:resource="http://dublincore.org/usage/terms/history/#instructionalMethod-002"/>
        <rdfs:isDefinedBy rdf:resource="http://purl.org/dc/terms/"/>
        <rdfs:range rdf:resource="&terms;MethodOfInstruction"/>
    </owl:ObjectProperty>
    


    <!-- http://purl.org/dc/terms/language -->

    <owl:ObjectProperty rdf:about="&terms;language">
        <rdfs:label xml:lang="en">Language</rdfs:label>
        <terms:modified rdf:datatype="&xsd;date">2008-01-14</terms:modified>
        <terms:issued rdf:datatype="&xsd;date">2008-01-14</terms:issued>
        <rdfs:comment xml:lang="en">A language of the resource.</rdfs:comment>
        <terms:description xml:lang="en">Recommended best practice is to use a controlled vocabulary such as RFC 4646 [RFC4646].</terms:description>
        <terms:hasVersion rdf:resource="http://dublincore.org/usage/terms/history/#languageT-001"/>
        <rdfs:isDefinedBy rdf:resource="http://purl.org/dc/terms/"/>
        <rdfs:range rdf:resource="&terms;LinguisticSystem"/>
    </owl:ObjectProperty>
    


    <!-- http://purl.org/dc/terms/license -->

    <owl:ObjectProperty rdf:about="&terms;license">
        <rdfs:label xml:lang="en">License</rdfs:label>
        <terms:issued rdf:datatype="&xsd;date">2004-06-14</terms:issued>
        <terms:modified rdf:datatype="&xsd;date">2008-01-14</terms:modified>
        <rdfs:comment xml:lang="en">A legal document giving official permission to do something with the resource.</rdfs:comment>
        <terms:hasVersion rdf:resource="http://dublincore.org/usage/terms/history/#license-002"/>
        <rdfs:isDefinedBy rdf:resource="http://purl.org/dc/terms/"/>
        <rdfs:range rdf:resource="&terms;LicenseDocument"/>
        <rdfs:subPropertyOf rdf:resource="&terms;rights"/>
    </owl:ObjectProperty>
    


    <!-- http://purl.org/dc/terms/mediator -->

    <owl:ObjectProperty rdf:about="&terms;mediator">
        <rdfs:label xml:lang="en">Mediator</rdfs:label>
        <terms:issued rdf:datatype="&xsd;date">2001-05-21</terms:issued>
        <terms:modified rdf:datatype="&xsd;date">2008-01-14</terms:modified>
        <rdfs:comment xml:lang="en">An entity that mediates access to the resource and for whom the resource is intended or useful.</rdfs:comment>
        <terms:description xml:lang="en">In an educational context, a mediator might be a parent, teacher, teaching assistant, or care-giver.</terms:description>
        <terms:hasVersion rdf:resource="http://dublincore.org/usage/terms/history/#mediator-003"/>
        <rdfs:isDefinedBy rdf:resource="http://purl.org/dc/terms/"/>
        <rdfs:range rdf:resource="&terms;AgentClass"/>
        <rdfs:subPropertyOf rdf:resource="&terms;audience"/>
    </owl:ObjectProperty>
    


    <!-- http://purl.org/dc/terms/medium -->

    <owl:ObjectProperty rdf:about="&terms;medium">
        <rdfs:label xml:lang="en">Medium</rdfs:label>
        <terms:issued rdf:datatype="&xsd;date">2000-07-11</terms:issued>
        <terms:modified rdf:datatype="&xsd;date">2008-01-14</terms:modified>
        <rdfs:comment xml:lang="en">The material or physical carrier of the resource.</rdfs:comment>
        <terms:hasVersion rdf:resource="http://dublincore.org/usage/terms/history/#medium-003"/>
        <rdfs:isDefinedBy rdf:resource="http://purl.org/dc/terms/"/>
        <rdfs:range rdf:resource="&terms;PhysicalMedium"/>
        <rdfs:domain rdf:resource="&terms;PhysicalResource"/>
        <rdfs:subPropertyOf rdf:resource="&terms;format"/>
    </owl:ObjectProperty>
    


    <!-- http://purl.org/dc/terms/provenance -->

    <owl:ObjectProperty rdf:about="&terms;provenance">
        <rdfs:label xml:lang="en">Provenance</rdfs:label>
        <terms:issued rdf:datatype="&xsd;date">2004-09-20</terms:issued>
        <terms:modified rdf:datatype="&xsd;date">2008-01-14</terms:modified>
        <rdfs:comment xml:lang="en">A statement of any changes in ownership and custody of the resource since its creation that are significant for its authenticity, integrity, and interpretation.</rdfs:comment>
        <terms:description xml:lang="en">The statement may include a description of any changes successive custodians made to the resource.</terms:description>
        <terms:hasVersion rdf:resource="http://dublincore.org/usage/terms/history/#provenance-002"/>
        <rdfs:isDefinedBy rdf:resource="http://purl.org/dc/terms/"/>
        <rdfs:range rdf:resource="&terms;ProvenanceStatement"/>
    </owl:ObjectProperty>
    


    <!-- http://purl.org/dc/terms/publisher -->

    <owl:ObjectProperty rdf:about="&terms;publisher">
        <rdfs:label xml:lang="en">Publisher</rdfs:label>
        <terms:issued rdf:datatype="&xsd;date">2008-01-14</terms:issued>
        <terms:modified rdf:datatype="&xsd;date">2010-10-11</terms:modified>
        <rdfs:comment xml:lang="en">An entity responsible for making the resource available.</rdfs:comment>
        <terms:description xml:lang="en">Examples of a Publisher include a person, an organization, or a service.</terms:description>
        <terms:hasVersion rdf:resource="http://dublincore.org/usage/terms/history/#publisherT-001"/>
        <rdfs:isDefinedBy rdf:resource="http://purl.org/dc/terms/"/>
        <rdfs:range rdf:resource="&terms;Agent"/>
    </owl:ObjectProperty>
    


    <!-- http://purl.org/dc/terms/rights -->

    <owl:ObjectProperty rdf:about="&terms;rights">
        <rdfs:label xml:lang="en">Rights</rdfs:label>
        <terms:issued rdf:datatype="&xsd;date">2008-01-14</terms:issued>
        <terms:modified rdf:datatype="&xsd;date">2008-01-14</terms:modified>
        <rdfs:comment xml:lang="en">Information about rights held in and over the resource.</rdfs:comment>
        <terms:description xml:lang="en">Typically, rights information includes a statement about various property rights associated with the resource, including intellectual property rights.</terms:description>
        <terms:hasVersion rdf:resource="http://dublincore.org/usage/terms/history/#rightsT-001"/>
        <rdfs:isDefinedBy rdf:resource="http://purl.org/dc/terms/"/>
        <rdfs:range rdf:resource="&terms;RightsStatement"/>
    </owl:ObjectProperty>
    


    <!-- http://purl.org/dc/terms/rightsHolder -->

    <owl:ObjectProperty rdf:about="&terms;rightsHolder">
        <rdfs:label xml:lang="en">Rights Holder</rdfs:label>
        <terms:issued rdf:datatype="&xsd;date">2004-06-14</terms:issued>
        <terms:modified rdf:datatype="&xsd;date">2008-01-14</terms:modified>
        <rdfs:comment xml:lang="en">A person or organization owning or managing rights over the resource.</rdfs:comment>
        <terms:hasVersion rdf:resource="http://dublincore.org/usage/terms/history/#rightsHolder-002"/>
        <rdfs:isDefinedBy rdf:resource="http://purl.org/dc/terms/"/>
        <rdfs:range rdf:resource="&terms;Agent"/>
    </owl:ObjectProperty>
    


    <!-- http://purl.org/dc/terms/spatial -->

    <owl:ObjectProperty rdf:about="&terms;spatial">
        <rdfs:label xml:lang="en">Spatial Coverage</rdfs:label>
        <terms:issued rdf:datatype="&xsd;date">2000-07-11</terms:issued>
        <terms:modified rdf:datatype="&xsd;date">2008-01-14</terms:modified>
        <rdfs:comment xml:lang="en">Spatial characteristics of the resource.</rdfs:comment>
        <terms:hasVersion rdf:resource="http://dublincore.org/usage/terms/history/#spatial-003"/>
        <rdfs:isDefinedBy rdf:resource="http://purl.org/dc/terms/"/>
        <rdfs:range rdf:resource="&terms;Location"/>
        <rdfs:subPropertyOf rdf:resource="&terms;coverage"/>
    </owl:ObjectProperty>
    


    <!-- http://purl.org/dc/terms/temporal -->

    <owl:ObjectProperty rdf:about="&terms;temporal">
        <rdfs:label xml:lang="en">Temporal Coverage</rdfs:label>
        <terms:issued rdf:datatype="&xsd;date">2000-07-11</terms:issued>
        <terms:modified rdf:datatype="&xsd;date">2008-01-14</terms:modified>
        <rdfs:comment xml:lang="en">Temporal characteristics of the resource.</rdfs:comment>
        <terms:hasVersion rdf:resource="http://dublincore.org/usage/terms/history/#temporal-003"/>
        <rdfs:isDefinedBy rdf:resource="http://purl.org/dc/terms/"/>
        <rdfs:range rdf:resource="&terms;PeriodOfTime"/>
        <rdfs:subPropertyOf rdf:resource="&terms;coverage"/>
    </owl:ObjectProperty>
    


    <!-- http://purl.org/dc/terms/type -->

    <owl:ObjectProperty rdf:about="&terms;type">
        <rdfs:label xml:lang="en">Type</rdfs:label>
        <terms:modified rdf:datatype="&xsd;date">2008-01-14</terms:modified>
        <terms:issued rdf:datatype="&xsd;date">2008-01-14</terms:issued>
        <terms:description xml:lang="en">Recommended best practice is to use a controlled vocabulary such as the DCMI Type Vocabulary [DCMITYPE]. To describe the file format, physical medium, or dimensions of the resource, use the Format element.</terms:description>
        <rdfs:comment xml:lang="en">The nature or genre of the resource.</rdfs:comment>
        <terms:hasVersion rdf:resource="http://dublincore.org/usage/terms/history/#typeT-001"/>
        <rdfs:isDefinedBy rdf:resource="http://purl.org/dc/terms/"/>
        <rdfs:range rdf:resource="&rdfs;Class"/>
    </owl:ObjectProperty>
    


    <!-- http://www.demcare.eu/ontologies/demlab.owl#activityStatus -->

    <owl:ObjectProperty rdf:about="&demlab;activityStatus">
        <rdfs:comment>The status of a semi-directed activity</rdfs:comment>
        <rdfs:seeAlso rdf:resource="&demlab;ActivityStatusType"/>
        <rdfs:range rdf:resource="&demlab;ActivityStatusType"/>
        <rdfs:seeAlso rdf:resource="&demlab;CognitiveAbilitiesData"/>
        <rdfs:domain rdf:resource="&demlab;CognitiveAbilitiesData"/>
    </owl:ObjectProperty>
    


    <!-- http://www.demcare.eu/ontologies/demlab.owl#areasOfInterestExplored -->

    <owl:ObjectProperty rdf:about="&demlab;areasOfInterestExplored">
        <rdfs:comment xml:lang="en">Zones of no interest</rdfs:comment>
        <rdfs:domain rdf:resource="&demlab;OrganisationEfficiencyData"/>
        <rdfs:seeAlso rdf:resource="&demlab;OrganisationEfficiencyData"/>
        <rdfs:range rdf:resource="&demlab;Zone"/>
    </owl:ObjectProperty>
    


    <!-- http://www.demcare.eu/ontologies/demlab.owl#areasOfNoInterestExplored -->

    <owl:ObjectProperty rdf:about="&demlab;areasOfNoInterestExplored">
        <rdfs:comment xml:lang="en">Zones of interest</rdfs:comment>
        <rdfs:domain rdf:resource="&demlab;OrganisationEfficiencyData"/>
        <rdfs:seeAlso rdf:resource="&demlab;OrganisationEfficiencyData"/>
        <rdfs:range rdf:resource="&demlab;Zone"/>
    </owl:ObjectProperty>
    


    <!-- http://www.demcare.eu/ontologies/demlab.owl#containsAssessment -->

    <owl:ObjectProperty rdf:about="&demlab;containsAssessment">
        <rdfs:comment>A ClinicalRecord contains a ClinicalAssessment</rdfs:comment>
        <rdfs:range rdf:resource="&demlab;ClinicalAssessment"/>
        <rdfs:seeAlso rdf:resource="&demlab;ClinicalAssessment"/>
        <rdfs:domain rdf:resource="&demlab;ClinicalRecord"/>
        <rdfs:seeAlso rdf:resource="&demlab;ClinicalRecord"/>
    </owl:ObjectProperty>
    


    <!-- http://www.demcare.eu/ontologies/demlab.owl#handTrajectory -->

    <owl:ObjectProperty rdf:about="&demlab;handTrajectory">
        <rdfs:comment xml:lang="en">Associates an instance of FunctionalAbilitiesData with a hand trajectory type</rdfs:comment>
        <rdfs:domain rdf:resource="&demlab;FunctionalAbilitiesData"/>
        <rdfs:seeAlso rdf:resource="&demlab;FunctionalAbilitiesData"/>
        <rdfs:range rdf:resource="&demlab;HandTrajectoryType"/>
        <rdfs:seeAlso rdf:resource="&demlab;HandTrajectoryType"/>
    </owl:ObjectProperty>
    


    <!-- http://www.demcare.eu/ontologies/demlab.owl#hasClinicalDiagnosis -->

    <owl:ObjectProperty rdf:about="&demlab;hasClinicalDiagnosis">
        <rdfs:comment xml:lang="en">The value of the DiagnosisAssessment</rdfs:comment>
        <rdfs:domain rdf:resource="&demlab;DiagnosisAssessment"/>
        <rdfs:seeAlso rdf:resource="&demlab;DiagnosisAssessment"/>
        <rdfs:range rdf:resource="&demlab;DiagnosisType"/>
        <rdfs:seeAlso rdf:resource="&demlab;DiagnosisType"/>
        <rdfs:subPropertyOf rdf:resource="&owl;topObjectProperty"/>
    </owl:ObjectProperty>
    


    <!-- http://www.demcare.eu/ontologies/demlab.owl#hasClinicalRecord -->

    <owl:ObjectProperty rdf:about="&demlab;hasClinicalRecord">
        <rdfs:comment xml:lang="en">Each participant is associated with a clinical record</rdfs:comment>
        <rdfs:seeAlso rdf:resource="&demlab;ClinicalRecord"/>
        <rdfs:range rdf:resource="&demlab;ClinicalRecord"/>
        <rdfs:domain rdf:resource="&demlab;Participant"/>
    </owl:ObjectProperty>
    


    <!-- http://www.demcare.eu/ontologies/demlab.owl#hasParticipant -->

    <owl:ObjectProperty rdf:about="&demlab;hasParticipant">
        <rdfs:comment xml:lang="en">The participant of the protocol</rdfs:comment>
        <rdfs:range rdf:resource="&demlab;Participant"/>
        <rdfs:seeAlso rdf:resource="&demlab;Person"/>
        <rdfs:domain rdf:resource="&demlab;Protocol"/>
        <rdfs:seeAlso rdf:resource="&demlab;Protocol"/>
    </owl:ObjectProperty>
    


    <!-- http://www.demcare.eu/ontologies/demlab.owl#hasProtocolStep -->

    <owl:ObjectProperty rdf:about="&demlab;hasProtocolStep">
        <rdfs:comment xml:lang="en">Each Protocol consists of one or more ProtocolSteps</rdfs:comment>
        <rdfs:domain rdf:resource="&demlab;Protocol"/>
        <rdfs:seeAlso rdf:resource="&demlab;Protocol"/>
        <rdfs:seeAlso rdf:resource="&demlab;ProtocolStep"/>
        <rdfs:range rdf:resource="&demlab;ProtocolStep"/>
    </owl:ObjectProperty>
    


    <!-- http://www.demcare.eu/ontologies/demlab.owl#involvesTask -->

    <owl:ObjectProperty rdf:about="&demlab;involvesTask">
        <rdfs:comment xml:lang="en">Each ProtocolStep involves one or more Tasks</rdfs:comment>
        <rdfs:seeAlso rdf:resource="&demlab;ProtocolStep"/>
        <rdfs:domain rdf:resource="&demlab;ProtocolStep"/>
        <rdfs:seeAlso rdf:resource="&demlab;Task"/>
        <rdfs:range rdf:resource="&demlab;Task"/>
    </owl:ObjectProperty>
    


    <!-- http://www.demcare.eu/ontologies/demlab.owl#isClinicalRecordOf -->

    <owl:ObjectProperty rdf:about="&demlab;isClinicalRecordOf">
        <owl:inverseOf rdf:resource="&demlab;hasClinicalRecord"/>
    </owl:ObjectProperty>
    


    <!-- http://www.demcare.eu/ontologies/demlab.owl#measuredData -->

    <owl:ObjectProperty rdf:about="&demlab;measuredData">
        <rdfs:seeAlso xml:lang="en">Associates a Task with a MeasuredData instance</rdfs:seeAlso>
        <rdfs:range rdf:resource="&demlab;MeasuredData"/>
        <rdfs:seeAlso rdf:resource="&demlab;MeasuredData"/>
        <rdfs:domain rdf:resource="&demlab;Task"/>
        <rdfs:seeAlso rdf:resource="&demlab;Task"/>
    </owl:ObjectProperty>
    


    <!-- http://www.demcare.eu/ontologies/demlab.owl#participates -->

    <owl:ObjectProperty rdf:about="&demlab;participates">
        <rdfs:seeAlso rdf:resource="&demlab;hasParticipant"/>
        <owl:inverseOf rdf:resource="&demlab;hasParticipant"/>
    </owl:ObjectProperty>
    


    <!-- 
    ///////////////////////////////////////////////////////////////////////////////////////
    //
    // Data properties
    //
    ///////////////////////////////////////////////////////////////////////////////////////
     -->

    


    <!-- http://purl.org/dc/terms/alternative -->

    <owl:DatatypeProperty rdf:about="&terms;alternative">
        <rdfs:label xml:lang="en">Alternative Title</rdfs:label>
        <terms:issued rdf:datatype="&xsd;date">2000-07-11</terms:issued>
        <terms:modified rdf:datatype="&xsd;date">2010-10-11</terms:modified>
        <rdfs:comment xml:lang="en">An alternative name for the resource.</rdfs:comment>
        <terms:description xml:lang="en">The distinction between titles and alternative titles is application-specific.</terms:description>
        <terms:hasVersion rdf:resource="http://dublincore.org/usage/terms/history/#alternative-003"/>
        <rdfs:isDefinedBy rdf:resource="http://purl.org/dc/terms/"/>
        <rdfs:subPropertyOf rdf:resource="&terms;title"/>
        <rdfs:range rdf:resource="&rdfs;Literal"/>
    </owl:DatatypeProperty>
    


    <!-- http://purl.org/dc/terms/available -->

    <owl:DatatypeProperty rdf:about="&terms;available">
        <rdfs:label xml:lang="en">Date Available</rdfs:label>
        <terms:issued rdf:datatype="&xsd;date">2000-07-11</terms:issued>
        <terms:modified rdf:datatype="&xsd;date">2008-01-14</terms:modified>
        <rdfs:comment xml:lang="en">Date (often a range) that the resource became or will become available.</rdfs:comment>
        <terms:hasVersion rdf:resource="http://dublincore.org/usage/terms/history/#available-003"/>
        <rdfs:isDefinedBy rdf:resource="http://purl.org/dc/terms/"/>
        <rdfs:subPropertyOf rdf:resource="&terms;date"/>
        <rdfs:range rdf:resource="&rdfs;Literal"/>
    </owl:DatatypeProperty>
    


    <!-- http://purl.org/dc/terms/bibliographicCitation -->

    <owl:DatatypeProperty rdf:about="&terms;bibliographicCitation">
        <rdfs:label xml:lang="en">Bibliographic Citation</rdfs:label>
        <terms:issued rdf:datatype="&xsd;date">2003-02-15</terms:issued>
        <terms:modified rdf:datatype="&xsd;date">2008-01-14</terms:modified>
        <rdfs:comment xml:lang="en">A bibliographic reference for the resource.</rdfs:comment>
        <terms:description xml:lang="en">Recommended practice is to include sufficient bibliographic detail to identify the resource as unambiguously as possible.</terms:description>
        <terms:hasVersion rdf:resource="http://dublincore.org/usage/terms/history/#bibliographicCitation-002"/>
        <rdfs:isDefinedBy rdf:resource="http://purl.org/dc/terms/"/>
        <rdfs:subPropertyOf rdf:resource="&terms;identifier"/>
        <rdfs:range rdf:resource="&rdfs;Literal"/>
    </owl:DatatypeProperty>
    


    <!-- http://purl.org/dc/terms/created -->

    <owl:DatatypeProperty rdf:about="&terms;created">
        <rdfs:label xml:lang="en">Date Created</rdfs:label>
        <terms:issued rdf:datatype="&xsd;date">2000-07-11</terms:issued>
        <terms:modified rdf:datatype="&xsd;date">2008-01-14</terms:modified>
        <rdfs:comment xml:lang="en">Date of creation of the resource.</rdfs:comment>
        <terms:hasVersion rdf:resource="http://dublincore.org/usage/terms/history/#created-003"/>
        <rdfs:isDefinedBy rdf:resource="http://purl.org/dc/terms/"/>
        <rdfs:subPropertyOf rdf:resource="&terms;date"/>
        <rdfs:range rdf:resource="&rdfs;Literal"/>
    </owl:DatatypeProperty>
    


    <!-- http://purl.org/dc/terms/date -->

    <owl:DatatypeProperty rdf:about="&terms;date">
        <rdfs:label xml:lang="en">Date</rdfs:label>
        <terms:issued rdf:datatype="&xsd;date">2008-01-14</terms:issued>
        <terms:modified rdf:datatype="&xsd;date">2008-01-14</terms:modified>
        <rdfs:comment xml:lang="en">A point or period of time associated with an event in the lifecycle of the resource.</rdfs:comment>
        <terms:description xml:lang="en">Date may be used to express temporal information at any level of granularity.  Recommended best practice is to use an encoding scheme, such as the W3CDTF profile of ISO 8601 [W3CDTF].</terms:description>
        <terms:hasVersion rdf:resource="http://dublincore.org/usage/terms/history/#dateT-001"/>
        <rdfs:isDefinedBy rdf:resource="http://purl.org/dc/terms/"/>
        <rdfs:range rdf:resource="&rdfs;Literal"/>
    </owl:DatatypeProperty>
    


    <!-- http://purl.org/dc/terms/dateAccepted -->

    <owl:DatatypeProperty rdf:about="&terms;dateAccepted">
        <rdfs:label xml:lang="en">Date Accepted</rdfs:label>
        <terms:issued rdf:datatype="&xsd;date">2002-07-13</terms:issued>
        <terms:modified rdf:datatype="&xsd;date">2008-01-14</terms:modified>
        <rdfs:comment xml:lang="en">Date of acceptance of the resource.</rdfs:comment>
        <terms:description xml:lang="en">Examples of resources to which a Date Accepted may be relevant are a thesis (accepted by a university department) or an article (accepted by a journal).</terms:description>
        <terms:hasVersion rdf:resource="http://dublincore.org/usage/terms/history/#dateAccepted-002"/>
        <rdfs:isDefinedBy rdf:resource="http://purl.org/dc/terms/"/>
        <rdfs:subPropertyOf rdf:resource="&terms;date"/>
        <rdfs:range rdf:resource="&rdfs;Literal"/>
    </owl:DatatypeProperty>
    


    <!-- http://purl.org/dc/terms/dateCopyrighted -->

    <owl:DatatypeProperty rdf:about="&terms;dateCopyrighted">
        <rdfs:label xml:lang="en">Date Copyrighted</rdfs:label>
        <terms:issued rdf:datatype="&xsd;date">2002-07-13</terms:issued>
        <terms:modified rdf:datatype="&xsd;date">2008-01-14</terms:modified>
        <rdfs:comment xml:lang="en">Date of copyright.</rdfs:comment>
        <terms:hasVersion rdf:resource="http://dublincore.org/usage/terms/history/#dateCopyrighted-002"/>
        <rdfs:isDefinedBy rdf:resource="http://purl.org/dc/terms/"/>
        <rdfs:subPropertyOf rdf:resource="&terms;date"/>
        <rdfs:range rdf:resource="&rdfs;Literal"/>
    </owl:DatatypeProperty>
    


    <!-- http://purl.org/dc/terms/dateSubmitted -->

    <owl:DatatypeProperty rdf:about="&terms;dateSubmitted">
        <rdfs:label xml:lang="en">Date Submitted</rdfs:label>
        <terms:issued rdf:datatype="&xsd;date">2002-07-13</terms:issued>
        <terms:modified rdf:datatype="&xsd;date">2008-01-14</terms:modified>
        <rdfs:comment xml:lang="en">Date of submission of the resource.</rdfs:comment>
        <terms:description xml:lang="en">Examples of resources to which a Date Submitted may be relevant are a thesis (submitted to a university department) or an article (submitted to a journal).</terms:description>
        <terms:hasVersion rdf:resource="http://dublincore.org/usage/terms/history/#dateSubmitted-002"/>
        <rdfs:isDefinedBy rdf:resource="http://purl.org/dc/terms/"/>
        <rdfs:subPropertyOf rdf:resource="&terms;date"/>
        <rdfs:range rdf:resource="&rdfs;Literal"/>
    </owl:DatatypeProperty>
    


    <!-- http://purl.org/dc/terms/identifier -->

    <owl:DatatypeProperty rdf:about="&terms;identifier">
        <rdfs:label xml:lang="en">Identifier</rdfs:label>
        <terms:issued rdf:datatype="&xsd;date">2008-01-14</terms:issued>
        <terms:modified rdf:datatype="&xsd;date">2008-01-14</terms:modified>
        <rdfs:comment xml:lang="en">An unambiguous reference to the resource within a given context.</rdfs:comment>
        <terms:description xml:lang="en">Recommended best practice is to identify the resource by means of a string conforming to a formal identification system. </terms:description>
        <terms:hasVersion rdf:resource="http://dublincore.org/usage/terms/history/#identifierT-001"/>
        <rdfs:isDefinedBy rdf:resource="http://purl.org/dc/terms/"/>
        <rdfs:range rdf:resource="&rdfs;Literal"/>
    </owl:DatatypeProperty>
    


    <!-- http://purl.org/dc/terms/issued -->

    <owl:DatatypeProperty rdf:about="&terms;issued">
        <rdfs:label xml:lang="en">Date Issued</rdfs:label>
        <terms:issued rdf:datatype="&xsd;date">2000-07-11</terms:issued>
        <terms:modified rdf:datatype="&xsd;date">2008-01-14</terms:modified>
        <rdfs:comment xml:lang="en">Date of formal issuance (e.g., publication) of the resource.</rdfs:comment>
        <terms:hasVersion rdf:resource="http://dublincore.org/usage/terms/history/#issued-003"/>
        <rdfs:isDefinedBy rdf:resource="http://purl.org/dc/terms/"/>
        <rdfs:subPropertyOf rdf:resource="&terms;date"/>
        <rdfs:range rdf:resource="&rdfs;Literal"/>
    </owl:DatatypeProperty>
    


    <!-- http://purl.org/dc/terms/modified -->

    <owl:DatatypeProperty rdf:about="&terms;modified">
        <rdfs:label xml:lang="en">Date Modified</rdfs:label>
        <terms:issued rdf:datatype="&xsd;date">2000-07-11</terms:issued>
        <terms:modified rdf:datatype="&xsd;date">2008-01-14</terms:modified>
        <rdfs:comment xml:lang="en">Date on which the resource was changed.</rdfs:comment>
        <terms:hasVersion rdf:resource="http://dublincore.org/usage/terms/history/#modified-003"/>
        <rdfs:isDefinedBy rdf:resource="http://purl.org/dc/terms/"/>
        <rdfs:subPropertyOf rdf:resource="&terms;date"/>
        <rdfs:range rdf:resource="&rdfs;Literal"/>
    </owl:DatatypeProperty>
    


    <!-- http://purl.org/dc/terms/title -->

    <owl:DatatypeProperty rdf:about="&terms;title">
        <rdfs:label xml:lang="en">Title</rdfs:label>
        <terms:issued rdf:datatype="&xsd;date">2008-01-14</terms:issued>
        <terms:modified rdf:datatype="&xsd;date">2010-10-11</terms:modified>
        <rdfs:comment xml:lang="en">A name given to the resource.</rdfs:comment>
        <terms:hasVersion rdf:resource="http://dublincore.org/usage/terms/history/#titleT-002"/>
        <rdfs:isDefinedBy rdf:resource="http://purl.org/dc/terms/"/>
        <rdfs:range rdf:resource="&rdfs;Literal"/>
    </owl:DatatypeProperty>
    


    <!-- http://purl.org/dc/terms/valid -->

    <owl:DatatypeProperty rdf:about="&terms;valid">
        <rdfs:label xml:lang="en">Date Valid</rdfs:label>
        <terms:issued rdf:datatype="&xsd;date">2000-07-11</terms:issued>
        <terms:modified rdf:datatype="&xsd;date">2008-01-14</terms:modified>
        <rdfs:comment xml:lang="en">Date (often a range) of validity of a resource.</rdfs:comment>
        <terms:hasVersion rdf:resource="http://dublincore.org/usage/terms/history/#valid-003"/>
        <rdfs:isDefinedBy rdf:resource="http://purl.org/dc/terms/"/>
        <rdfs:subPropertyOf rdf:resource="&terms;date"/>
        <rdfs:range rdf:resource="&rdfs;Literal"/>
    </owl:DatatypeProperty>
    


    <!-- http://www.demcare.eu/ontologies/demlab.owl#apathyInventory -->

    <owl:DatatypeProperty rdf:about="&demlab;apathyInventory">
        <rdfs:comment xml:lang="en">Apathy Inventory (AI) and diagnostic criteria for apathy</rdfs:comment>
        <rdfs:domain rdf:resource="&demlab;NeuropsychiatricAndMoodAssessment"/>
        <rdfs:seeAlso rdf:resource="&demlab;NeuropsychiatricAndMoodAssessment"/>
    </owl:DatatypeProperty>
    


    <!-- http://www.demcare.eu/ontologies/demlab.owl#articulation -->

    <owl:DatatypeProperty rdf:about="&demlab;articulation">
        <rdfs:comment xml:lang="en">Measures the articulation control of the participant</rdfs:comment>
        <rdfs:domain rdf:resource="&demlab;VoiceData"/>
    </owl:DatatypeProperty>
    


    <!-- http://www.demcare.eu/ontologies/demlab.owl#compliantInstructionsOrder -->

    <owl:DatatypeProperty rdf:about="&demlab;compliantInstructionsOrder">
        <rdfs:comment xml:lang="en">Whether the participant followed the activity order suggested by the instructions sheet</rdfs:comment>
        <rdfs:seeAlso rdf:resource="&demlab;CognitiveAbilitiesData"/>
        <rdfs:domain rdf:resource="&demlab;CognitiveAbilitiesData"/>
    </owl:DatatypeProperty>
    


    <!-- http://www.demcare.eu/ontologies/demlab.owl#distanceWalked -->

    <owl:DatatypeProperty rdf:about="&demlab;distanceWalked">
        <rdfs:comment xml:lang="en">Total distance walked</rdfs:comment>
        <rdfs:domain rdf:resource="&demlab;OrganisationEfficiencyData"/>
        <rdfs:seeAlso rdf:resource="&demlab;OrganisationEfficiencyData"/>
    </owl:DatatypeProperty>
    


    <!-- http://www.demcare.eu/ontologies/demlab.owl#dsm_ivDepressionCriteria -->

    <owl:DatatypeProperty rdf:about="&demlab;dsm_ivDepressionCriteria">
        <rdfs:comment xml:lang="en">DSM-IV Criteria for depression</rdfs:comment>
        <rdfs:seeAlso xml:lang="en">http://en.wikipedia.org/wiki/Diagnostic_and_Statistical_Manual_of_Mental_Disorders</rdfs:seeAlso>
        <rdfs:domain rdf:resource="&demlab;NeuropsychiatricAndMoodAssessment"/>
    </owl:DatatypeProperty>
    


    <!-- http://www.demcare.eu/ontologies/demlab.owl#dynamicBalance -->

    <owl:DatatypeProperty rdf:about="&demlab;dynamicBalance">
        <rdfs:comment xml:lang="en">Dynamical balance during the walking (e.g., people trajectory study)</rdfs:comment>
        <rdfs:domain rdf:resource="&demlab;GaitData"/>
        <rdfs:seeAlso rdf:resource="&demlab;GaitData"/>
    </owl:DatatypeProperty>
    


    <!-- http://www.demcare.eu/ontologies/demlab.owl#fabScore -->

    <owl:DatatypeProperty rdf:about="&demlab;fabScore">
        <rdfs:comment xml:lang="en">Frontal Assessment Battery score</rdfs:comment>
        <rdfs:domain rdf:resource="&demlab;CognitiveAbilitiesAssessment"/>
        <rdfs:seeAlso rdf:resource="&demlab;CognitiveAbilitiesAssessment"/>
    </owl:DatatypeProperty>
    


    <!-- http://www.demcare.eu/ontologies/demlab.owl#freeAndCuedRemindingAssessment -->

    <owl:DatatypeProperty rdf:about="&demlab;freeAndCuedRemindingAssessment">
        <rdfs:comment xml:lang="en">The Free and Cued Selective Reminding Test</rdfs:comment>
        <rdfs:domain rdf:resource="&demlab;CognitiveAbilitiesAssessment"/>
        <rdfs:seeAlso rdf:resource="&demlab;CognitiveAbilitiesAssessment"/>
    </owl:DatatypeProperty>
    


    <!-- http://www.demcare.eu/ontologies/demlab.owl#hasMMSEScore -->

    <owl:DatatypeProperty rdf:about="&demlab;hasMMSEScore">
        <rdfs:comment xml:lang="en">Mini-Mental State Exam score</rdfs:comment>
        <rdfs:domain rdf:resource="&demlab;CognitiveAbilitiesAssessment"/>
        <rdfs:seeAlso rdf:resource="&demlab;CognitiveAbilitiesAssessment"/>
    </owl:DatatypeProperty>
    


    <!-- http://www.demcare.eu/ontologies/demlab.owl#hasUPDRSScore -->

    <owl:DatatypeProperty rdf:about="&demlab;hasUPDRSScore">
        <rdfs:comment xml:lang="en">Part III of the Unified Parkinson’s Disease Rating Scale</rdfs:comment>
        <rdfs:seeAlso rdf:resource="&demlab;MotricityAbilitiesAssessment"/>
        <rdfs:domain rdf:resource="&demlab;MotricityAbilitiesAssessment"/>
    </owl:DatatypeProperty>
    


    <!-- http://www.demcare.eu/ontologies/demlab.owl#iadl_e -->

    <owl:DatatypeProperty rdf:about="&demlab;iadl_e">
        <rdfs:comment xml:lang="en">Allows the quantification of autonomy</rdfs:comment>
        <rdfs:seeAlso rdf:resource="&demlab;AutonomyAssessment"/>
        <rdfs:domain rdf:resource="&demlab;AutonomyAssessment"/>
    </owl:DatatypeProperty>
    


    <!-- http://www.demcare.eu/ontologies/demlab.owl#latency -->

    <owl:DatatypeProperty rdf:about="&demlab;latency">
        <rdfs:comment xml:lang="en">Time of latency between the end of instructions (stimulation) and the beginning of the task</rdfs:comment>
        <rdfs:seeAlso rdf:resource="&demlab;LatencyData"/>
        <rdfs:domain rdf:resource="&demlab;LatencyData"/>
    </owl:DatatypeProperty>
    


    <!-- http://www.demcare.eu/ontologies/demlab.owl#npi -->

    <owl:DatatypeProperty rdf:about="&demlab;npi">
        <rdfs:comment xml:lang="en">Neuropsychiatric Inventory</rdfs:comment>
        <rdfs:seeAlso rdf:resource="&demlab;NeuropsychiatricAndMoodAssessment"/>
        <rdfs:domain rdf:resource="&demlab;NeuropsychiatricAndMoodAssessment"/>
    </owl:DatatypeProperty>
    


    <!-- http://www.demcare.eu/ontologies/demlab.owl#pauseRate -->

    <owl:DatatypeProperty rdf:about="&demlab;pauseRate">
        <rdfs:comment xml:lang="en">Pause rate during sentence repetition and mono/dual tasks</rdfs:comment>
        <rdfs:seeAlso rdf:resource="&demlab;ArticulationControlTask"/>
        <rdfs:seeAlso rdf:resource="&demlab;CountingBackwardsTask"/>
        <rdfs:seeAlso rdf:resource="&demlab;SentenceRepeatingTask"/>
        <rdfs:seeAlso rdf:resource="&demlab;VoiceData"/>
        <rdfs:domain rdf:resource="&demlab;VoiceData"/>
        <rdfs:seeAlso rdf:resource="&demlab;WalkingCountingBackwardsTask"/>
    </owl:DatatypeProperty>
    


    <!-- http://www.demcare.eu/ontologies/demlab.owl#repetitions -->

    <owl:DatatypeProperty rdf:about="&demlab;repetitions">
        <rdfs:comment xml:lang="en">Number of repetitions during semi-directed activities</rdfs:comment>
        <rdfs:domain rdf:resource="&demlab;CognitiveAbilitiesData"/>
        <rdfs:seeAlso rdf:resource="&demlab;SemiDirectedTask"/>
    </owl:DatatypeProperty>
    


    <!-- http://www.demcare.eu/ontologies/demlab.owl#shortCognitiveBatteryAssessment -->

    <owl:DatatypeProperty rdf:about="&demlab;shortCognitiveBatteryAssessment">
        <rdfs:comment xml:lang="en">Short Cognitive Battery</rdfs:comment>
        <rdfs:seeAlso rdf:resource="&demlab;CognitiveAbilitiesAssessment"/>
        <rdfs:domain rdf:resource="&demlab;CognitiveAbilitiesAssessment"/>
    </owl:DatatypeProperty>
    


    <!-- http://www.demcare.eu/ontologies/demlab.owl#speechFluency -->

    <owl:DatatypeProperty rdf:about="&demlab;speechFluency">
        <rdfs:comment xml:lang="en">Speech fluency during sentence repetition and picture description tasks</rdfs:comment>
        <rdfs:seeAlso rdf:resource="&demlab;VoiceData"/>
        <rdfs:domain rdf:resource="&demlab;VoiceData"/>
    </owl:DatatypeProperty>
    


    <!-- http://www.demcare.eu/ontologies/demlab.owl#speechRate -->

    <owl:DatatypeProperty rdf:about="&demlab;speechRate">
        <rdfs:comment xml:lang="en">Speech fluency during sentence repetition and picture description tasks</rdfs:comment>
        <rdfs:domain rdf:resource="&demlab;VoiceData"/>
        <rdfs:seeAlso rdf:resource="&demlab;VoiceData"/>
    </owl:DatatypeProperty>
    


    <!-- http://www.demcare.eu/ontologies/demlab.owl#stepLength -->

    <owl:DatatypeProperty rdf:about="&demlab;stepLength">
        <rdfs:comment xml:lang="en">Step length</rdfs:comment>
        <rdfs:seeAlso rdf:resource="&demlab;GaitData"/>
        <rdfs:domain rdf:resource="&demlab;GaitData"/>
    </owl:DatatypeProperty>
    


    <!-- http://www.demcare.eu/ontologies/demlab.owl#stoppingDisplacement -->

    <owl:DatatypeProperty rdf:about="&demlab;stoppingDisplacement">
        <rdfs:comment xml:lang="en">Stopping displacement during walking</rdfs:comment>
        <rdfs:seeAlso rdf:resource="&demlab;GaitData"/>
        <rdfs:domain rdf:resource="&demlab;GaitData"/>
    </owl:DatatypeProperty>
    


    <!-- http://www.demcare.eu/ontologies/demlab.owl#stressLevel -->

    <owl:DatatypeProperty rdf:about="&demlab;stressLevel">
        <rdfs:seeAlso xml:lang="en">Stress level</rdfs:seeAlso>
        <rdfs:seeAlso rdf:resource="&demlab;StressData"/>
        <rdfs:domain rdf:resource="&demlab;StressData"/>
    </owl:DatatypeProperty>
    


    <!-- http://www.demcare.eu/ontologies/demlab.owl#trailMakingTest -->

    <owl:DatatypeProperty rdf:about="&demlab;trailMakingTest">
        <rdfs:comment xml:lang="en">Trail making test A and B</rdfs:comment>
        <rdfs:domain rdf:resource="&demlab;CognitiveAbilitiesAssessment"/>
        <rdfs:seeAlso rdf:resource="&demlab;CognitiveAbilitiesAssessment"/>
    </owl:DatatypeProperty>
    


    <!-- http://www.demcare.eu/ontologies/demlab.owl#verbalReactionSpontaneity -->

    <owl:DatatypeProperty rdf:about="&demlab;verbalReactionSpontaneity">
        <rdfs:comment xml:lang="en">Time between the end of assessor’s speech and the beginning of participant’s speech (Discussion Task)</rdfs:comment>
        <rdfs:seeAlso rdf:resource="&demlab;DiscussionInvolvementData"/>
        <rdfs:domain rdf:resource="&demlab;DiscussionInvolvementData"/>
    </owl:DatatypeProperty>
    


    <!-- http://www.demcare.eu/ontologies/demlab.owl#verbalReactionTime -->

    <owl:DatatypeProperty rdf:about="&demlab;verbalReactionTime">
        <rdfs:comment xml:lang="en">Time interval between the end of assessor’s speech and the beginning of participant’s speech (Sentence Repetition Task)</rdfs:comment>
        <rdfs:domain rdf:resource="&demlab;VoiceData"/>
        <rdfs:seeAlso rdf:resource="&demlab;VoiceData"/>
    </owl:DatatypeProperty>
    


    <!-- http://www.demcare.eu/ontologies/demlab.owl#vowelDuration -->

    <owl:DatatypeProperty rdf:about="&demlab;vowelDuration">
        <rdfs:seeAlso xml:lang="en">Vowel duration</rdfs:seeAlso>
        <rdfs:comment rdf:resource="&demlab;VoiceData"/>
        <rdfs:domain rdf:resource="&demlab;VoiceData"/>
        <rdfs:subPropertyOf rdf:resource="&owl;topDataProperty"/>
    </owl:DatatypeProperty>
    


    <!-- http://www.demcare.eu/ontologies/demlab.owl#walkingSpeed -->

    <owl:DatatypeProperty rdf:about="&demlab;walkingSpeed">
        <rdfs:comment xml:lang="en">Walking speed</rdfs:comment>
        <rdfs:seeAlso rdf:resource="&demlab;GaitData"/>
        <rdfs:domain rdf:resource="&demlab;GaitData"/>
    </owl:DatatypeProperty>
    


    <!-- http://www.demcare.eu/ontologies/demlab.owl#walkingSpeedInstantaneous -->

    <owl:DatatypeProperty rdf:about="&demlab;walkingSpeedInstantaneous">
        <rdfs:comment xml:lang="en">Walking speed instantaneous (mono task walking activity/dual task)</rdfs:comment>
        <rdfs:seeAlso rdf:resource="&demlab;GaitData"/>
        <rdfs:domain rdf:resource="&demlab;GaitData"/>
    </owl:DatatypeProperty>
    


    <!-- 
    ///////////////////////////////////////////////////////////////////////////////////////
    //
    // Classes
    //
    ///////////////////////////////////////////////////////////////////////////////////////
     -->

    


    <!-- http://purl.org/dc/dcam/VocabularyEncodingScheme -->

    <owl:Class rdf:about="http://purl.org/dc/dcam/VocabularyEncodingScheme"/>
    


    <!-- http://purl.org/dc/terms/Agent -->

    <owl:Class rdf:about="&terms;Agent">
        <rdfs:label xml:lang="en">Agent</rdfs:label>
        <terms:issued rdf:datatype="&xsd;date">2008-01-14</terms:issued>
        <rdfs:comment xml:lang="en">A resource that acts or has the power to act.</rdfs:comment>
        <terms:description xml:lang="en">Examples of Agent include person, organization, and software agent.</terms:description>
        <terms:hasVersion rdf:resource="http://dublincore.org/usage/terms/history/#Agent-001"/>
        <rdfs:isDefinedBy rdf:resource="http://purl.org/dc/terms/"/>
    </owl:Class>
    


    <!-- http://purl.org/dc/terms/AgentClass -->

    <owl:Class rdf:about="&terms;AgentClass">
        <rdfs:label xml:lang="en">Agent Class</rdfs:label>
        <rdfs:subClassOf rdf:resource="&rdfs;Class"/>
        <terms:issued rdf:datatype="&xsd;date">2008-01-14</terms:issued>
        <terms:modified rdf:datatype="&xsd;date">2012-06-14</terms:modified>
        <rdfs:comment xml:lang="en">A group of agents.</rdfs:comment>
        <terms:description xml:lang="en">Examples of Agent Class include groups seen as classes, such as students, women, charities, lecturers.</terms:description>
        <terms:hasVersion rdf:resource="http://dublincore.org/usage/terms/history/#AgentClass-003"/>
        <rdfs:isDefinedBy rdf:resource="http://purl.org/dc/terms/"/>
    </owl:Class>
    


    <!-- http://purl.org/dc/terms/BibliographicResource -->

    <owl:Class rdf:about="&terms;BibliographicResource">
        <rdfs:label xml:lang="en">Bibliographic Resource</rdfs:label>
        <terms:issued rdf:datatype="&xsd;date">2008-01-14</terms:issued>
        <rdfs:comment xml:lang="en">A book, article, or other documentary resource.</rdfs:comment>
        <terms:hasVersion rdf:resource="http://dublincore.org/usage/terms/history/#BibliographicResource-001"/>
        <rdfs:isDefinedBy rdf:resource="http://purl.org/dc/terms/"/>
    </owl:Class>
    


    <!-- http://purl.org/dc/terms/FileFormat -->

    <owl:Class rdf:about="&terms;FileFormat">
        <rdfs:label xml:lang="en">File Format</rdfs:label>
        <rdfs:subClassOf rdf:resource="&terms;MediaType"/>
        <terms:issued rdf:datatype="&xsd;date">2008-01-14</terms:issued>
        <rdfs:comment xml:lang="en">A digital resource format.</rdfs:comment>
        <terms:description xml:lang="en">Examples include the formats defined by the list of Internet Media Types.</terms:description>
        <terms:hasVersion rdf:resource="http://dublincore.org/usage/terms/history/#FileFormat-001"/>
        <rdfs:isDefinedBy rdf:resource="http://purl.org/dc/terms/"/>
    </owl:Class>
    


    <!-- http://purl.org/dc/terms/Frequency -->

    <owl:Class rdf:about="&terms;Frequency">
        <rdfs:label xml:lang="en">Frequency</rdfs:label>
        <terms:issued rdf:datatype="&xsd;date">2008-01-14</terms:issued>
        <rdfs:comment xml:lang="en">A rate at which something recurs.</rdfs:comment>
        <terms:hasVersion rdf:resource="http://dublincore.org/usage/terms/history/#Frequency-001"/>
        <rdfs:isDefinedBy rdf:resource="http://purl.org/dc/terms/"/>
    </owl:Class>
    


    <!-- http://purl.org/dc/terms/Jurisdiction -->

    <owl:Class rdf:about="&terms;Jurisdiction">
        <rdfs:label xml:lang="en">Jurisdiction</rdfs:label>
        <rdfs:subClassOf rdf:resource="&terms;LocationPeriodOrJurisdiction"/>
        <terms:issued rdf:datatype="&xsd;date">2008-01-14</terms:issued>
        <rdfs:comment xml:lang="en">The extent or range of judicial, law enforcement, or other authority.</rdfs:comment>
        <terms:hasVersion rdf:resource="http://dublincore.org/usage/terms/history/#Jurisdiction-001"/>
        <rdfs:isDefinedBy rdf:resource="http://purl.org/dc/terms/"/>
    </owl:Class>
    


    <!-- http://purl.org/dc/terms/LicenseDocument -->

    <owl:Class rdf:about="&terms;LicenseDocument">
        <rdfs:label xml:lang="en">License Document</rdfs:label>
        <rdfs:subClassOf rdf:resource="&terms;RightsStatement"/>
        <terms:issued rdf:datatype="&xsd;date">2008-01-14</terms:issued>
        <rdfs:comment xml:lang="en">A legal document giving official permission to do something with a Resource.</rdfs:comment>
        <terms:hasVersion rdf:resource="http://dublincore.org/usage/terms/history/#LicenseDocument-001"/>
        <rdfs:isDefinedBy rdf:resource="http://purl.org/dc/terms/"/>
    </owl:Class>
    


    <!-- http://purl.org/dc/terms/LinguisticSystem -->

    <owl:Class rdf:about="&terms;LinguisticSystem">
        <rdfs:label xml:lang="en">Linguistic System</rdfs:label>
        <terms:issued rdf:datatype="&xsd;date">2008-01-14</terms:issued>
        <rdfs:comment xml:lang="en">A system of signs, symbols, sounds, gestures, or rules used in communication.</rdfs:comment>
        <terms:description xml:lang="en">Examples include written, spoken, sign, and computer languages.</terms:description>
        <terms:hasVersion rdf:resource="http://dublincore.org/usage/terms/history/#LinguisticSystem-001"/>
        <rdfs:isDefinedBy rdf:resource="http://purl.org/dc/terms/"/>
    </owl:Class>
    


    <!-- http://purl.org/dc/terms/Location -->

    <owl:Class rdf:about="&terms;Location">
        <rdfs:label xml:lang="en">Location</rdfs:label>
        <rdfs:subClassOf rdf:resource="&terms;LocationPeriodOrJurisdiction"/>
        <terms:issued rdf:datatype="&xsd;date">2008-01-14</terms:issued>
        <rdfs:comment xml:lang="en">A spatial region or named place.</rdfs:comment>
        <terms:hasVersion rdf:resource="http://dublincore.org/usage/terms/history/#Location-001"/>
        <rdfs:isDefinedBy rdf:resource="http://purl.org/dc/terms/"/>
    </owl:Class>
    


    <!-- http://purl.org/dc/terms/LocationPeriodOrJurisdiction -->

    <owl:Class rdf:about="&terms;LocationPeriodOrJurisdiction">
        <rdfs:label xml:lang="en">Location, Period, or Jurisdiction</rdfs:label>
        <terms:issued rdf:datatype="&xsd;date">2008-01-14</terms:issued>
        <rdfs:comment xml:lang="en">A location, period of time, or jurisdiction.</rdfs:comment>
        <terms:hasVersion rdf:resource="http://dublincore.org/usage/terms/history/#LocationPeriodOrJurisdiction-001"/>
        <rdfs:isDefinedBy rdf:resource="http://purl.org/dc/terms/"/>
    </owl:Class>
    


    <!-- http://purl.org/dc/terms/MediaType -->

    <owl:Class rdf:about="&terms;MediaType">
        <rdfs:label xml:lang="en">Media Type</rdfs:label>
        <rdfs:subClassOf rdf:resource="&terms;MediaTypeOrExtent"/>
        <terms:issued rdf:datatype="&xsd;date">2008-01-14</terms:issued>
        <rdfs:comment xml:lang="en">A file format or physical medium.</rdfs:comment>
        <terms:hasVersion rdf:resource="http://dublincore.org/usage/terms/history/#MediaType-001"/>
        <rdfs:isDefinedBy rdf:resource="http://purl.org/dc/terms/"/>
    </owl:Class>
    


    <!-- http://purl.org/dc/terms/MediaTypeOrExtent -->

    <owl:Class rdf:about="&terms;MediaTypeOrExtent">
        <rdfs:label xml:lang="en">Media Type or Extent</rdfs:label>
        <terms:issued rdf:datatype="&xsd;date">2008-01-14</terms:issued>
        <rdfs:comment xml:lang="en">A media type or extent.</rdfs:comment>
        <terms:hasVersion rdf:resource="http://dublincore.org/usage/terms/history/#MediaTypeOrExtent-001"/>
        <rdfs:isDefinedBy rdf:resource="http://purl.org/dc/terms/"/>
    </owl:Class>
    


    <!-- http://purl.org/dc/terms/MethodOfAccrual -->

    <owl:Class rdf:about="&terms;MethodOfAccrual">
        <rdfs:label xml:lang="en">Method of Accrual</rdfs:label>
        <terms:issued rdf:datatype="&xsd;date">2008-01-14</terms:issued>
        <rdfs:comment xml:lang="en">A method by which resources are added to a collection.</rdfs:comment>
        <terms:hasVersion rdf:resource="http://dublincore.org/usage/terms/history/#MethodOfAccrual-001"/>
        <rdfs:isDefinedBy rdf:resource="http://purl.org/dc/terms/"/>
    </owl:Class>
    


    <!-- http://purl.org/dc/terms/MethodOfInstruction -->

    <owl:Class rdf:about="&terms;MethodOfInstruction">
        <rdfs:label xml:lang="en">Method of Instruction</rdfs:label>
        <terms:issued rdf:datatype="&xsd;date">2008-01-14</terms:issued>
        <rdfs:comment xml:lang="en">A process that is used to engender knowledge, attitudes, and skills.</rdfs:comment>
        <terms:hasVersion rdf:resource="http://dublincore.org/usage/terms/history/#MethodOfInstruction-001"/>
        <rdfs:isDefinedBy rdf:resource="http://purl.org/dc/terms/"/>
    </owl:Class>
    


    <!-- http://purl.org/dc/terms/PeriodOfTime -->

    <owl:Class rdf:about="&terms;PeriodOfTime">
        <rdfs:label xml:lang="en">Period of Time</rdfs:label>
        <rdfs:subClassOf rdf:resource="&terms;LocationPeriodOrJurisdiction"/>
        <terms:issued rdf:datatype="&xsd;date">2008-01-14</terms:issued>
        <rdfs:comment xml:lang="en">An interval of time that is named or defined by its start and end dates.</rdfs:comment>
        <terms:hasVersion rdf:resource="http://dublincore.org/usage/terms/history/#PeriodOfTime-001"/>
        <rdfs:isDefinedBy rdf:resource="http://purl.org/dc/terms/"/>
    </owl:Class>
    


    <!-- http://purl.org/dc/terms/PhysicalMedium -->

    <owl:Class rdf:about="&terms;PhysicalMedium">
        <rdfs:label xml:lang="en">Physical Medium</rdfs:label>
        <rdfs:subClassOf rdf:resource="&terms;MediaType"/>
        <terms:issued rdf:datatype="&xsd;date">2008-01-14</terms:issued>
        <rdfs:comment xml:lang="en">A physical material or carrier.</rdfs:comment>
        <terms:description xml:lang="en">Examples include paper, canvas, or DVD.</terms:description>
        <terms:hasVersion rdf:resource="http://dublincore.org/usage/terms/history/#PhysicalMedium-001"/>
        <rdfs:isDefinedBy rdf:resource="http://purl.org/dc/terms/"/>
    </owl:Class>
    


    <!-- http://purl.org/dc/terms/PhysicalResource -->

    <owl:Class rdf:about="&terms;PhysicalResource">
        <rdfs:label xml:lang="en">Physical Resource</rdfs:label>
        <terms:issued rdf:datatype="&xsd;date">2008-01-14</terms:issued>
        <rdfs:comment xml:lang="en">A material thing.</rdfs:comment>
        <terms:hasVersion rdf:resource="http://dublincore.org/usage/terms/history/#PhysicalResource-001"/>
        <rdfs:isDefinedBy rdf:resource="http://purl.org/dc/terms/"/>
    </owl:Class>
    


    <!-- http://purl.org/dc/terms/Policy -->

    <owl:Class rdf:about="&terms;Policy">
        <rdfs:label xml:lang="en">Policy</rdfs:label>
        <terms:issued rdf:datatype="&xsd;date">2008-01-14</terms:issued>
        <rdfs:comment xml:lang="en">A plan or course of action by an authority, intended to influence and determine decisions, actions, and other matters.</rdfs:comment>
        <terms:hasVersion rdf:resource="http://dublincore.org/usage/terms/history/#Policy-001"/>
        <rdfs:isDefinedBy rdf:resource="http://purl.org/dc/terms/"/>
    </owl:Class>
    


    <!-- http://purl.org/dc/terms/ProvenanceStatement -->

    <owl:Class rdf:about="&terms;ProvenanceStatement">
        <rdfs:label xml:lang="en">Provenance Statement</rdfs:label>
        <terms:issued rdf:datatype="&xsd;date">2008-01-14</terms:issued>
        <rdfs:comment xml:lang="en">A statement of any changes in ownership and custody of a resource since its creation that are significant for its authenticity, integrity, and interpretation.</rdfs:comment>
        <terms:hasVersion rdf:resource="http://dublincore.org/usage/terms/history/#ProvenanceStatement-001"/>
        <rdfs:isDefinedBy rdf:resource="http://purl.org/dc/terms/"/>
    </owl:Class>
    


    <!-- http://purl.org/dc/terms/RightsStatement -->

    <owl:Class rdf:about="&terms;RightsStatement">
        <rdfs:label xml:lang="en">Rights Statement</rdfs:label>
        <terms:issued rdf:datatype="&xsd;date">2008-01-14</terms:issued>
        <rdfs:comment xml:lang="en">A statement about the intellectual property rights (IPR) held in or over a Resource, a legal document giving official permission to do something with a resource, or a statement about access rights.</rdfs:comment>
        <terms:hasVersion rdf:resource="http://dublincore.org/usage/terms/history/#RightsStatement-001"/>
        <rdfs:isDefinedBy rdf:resource="http://purl.org/dc/terms/"/>
    </owl:Class>
    


    <!-- http://purl.org/dc/terms/SizeOrDuration -->

    <owl:Class rdf:about="&terms;SizeOrDuration">
        <rdfs:label xml:lang="en">Size or Duration</rdfs:label>
        <rdfs:subClassOf rdf:resource="&terms;MediaTypeOrExtent"/>
        <terms:issued rdf:datatype="&xsd;date">2008-01-14</terms:issued>
        <rdfs:comment xml:lang="en">A dimension or extent, or a time taken to play or execute.</rdfs:comment>
        <terms:description xml:lang="en">Examples include a number of pages, a specification of length, width, and breadth, or a period in hours, minutes, and seconds.</terms:description>
        <terms:hasVersion rdf:resource="http://dublincore.org/usage/terms/history/#SizeOrDuration-001"/>
        <rdfs:isDefinedBy rdf:resource="http://purl.org/dc/terms/"/>
    </owl:Class>
    


    <!-- http://purl.org/dc/terms/Standard -->

    <owl:Class rdf:about="&terms;Standard">
        <rdfs:label xml:lang="en">Standard</rdfs:label>
        <terms:issued rdf:datatype="&xsd;date">2008-01-14</terms:issued>
        <rdfs:comment xml:lang="en">A basis for comparison; a reference point against which other things can be evaluated.</rdfs:comment>
        <terms:hasVersion rdf:resource="http://dublincore.org/usage/terms/history/#Standard-001"/>
        <rdfs:isDefinedBy rdf:resource="http://purl.org/dc/terms/"/>
    </owl:Class>
    


    <!-- http://www.demcare.eu/ontologies/demlab.owl#ActivityStatusType -->

    <owl:Class rdf:about="&demlab;ActivityStatusType">
        <owl:equivalentClass>
            <owl:Class>
                <owl:oneOf rdf:parseType="Collection">
                    <rdf:Description rdf:about="&demlab;completed"/>
                    <rdf:Description rdf:about="&demlab;incomplete"/>
                    <rdf:Description rdf:about="&demlab;omitted"/>
                </owl:oneOf>
            </owl:Class>
        </owl:equivalentClass>
    </owl:Class>
    


    <!-- http://www.demcare.eu/ontologies/demlab.owl#AnswerPhoneTask -->

    <owl:Class rdf:about="&demlab;AnswerPhoneTask">
        <rdfs:subClassOf rdf:resource="&demlab;SemiDirectedTask"/>
        <rdfs:comment xml:lang="en">- The phone is scheduled to ring 10 minutes after the entering of the participant inside the room. 
- During this task, the clinician explains that there is a mistake on the phone bill: the amount was wrong. Consequently, it is expected that the participant corrects his/her phone check and corrects the account balance (tasks normally established before the phone call according to the constraint).</rdfs:comment>
    </owl:Class>
    


    <!-- http://www.demcare.eu/ontologies/demlab.owl#ArticulationControlTask -->

    <owl:Class rdf:about="&demlab;ArticulationControlTask">
        <rdfs:subClassOf rdf:resource="&demlab;DirectedTask"/>
        <rdfs:subClassOf>
            <owl:Restriction>
                <owl:onProperty rdf:resource="&demlab;measuredData"/>
                <owl:allValuesFrom>
                    <owl:Class>
                        <owl:unionOf rdf:parseType="Collection">
                            <rdf:Description rdf:about="&demlab;LatencyData"/>
                            <rdf:Description rdf:about="&demlab;StressData"/>
                            <rdf:Description rdf:about="&demlab;VoiceData"/>
                        </owl:unionOf>
                    </owl:Class>
                </owl:allValuesFrom>
            </owl:Restriction>
        </rdfs:subClassOf>
        <rdfs:comment xml:lang="en">The participant is asked to pronounce repeatedly a predefined diadochokinetic “Pataka” token as rapid as possible stopping this action upon a sign by the clinician. The clinician will stop the action in 10 sec.

This task is used for assessing:
- Latency: time of latency between the end of instructions (stimulation) and the beginning of the task
- Stress level
- Voice: e.g. speech rate, pause rate etc.</rdfs:comment>
    </owl:Class>
    


    <!-- http://www.demcare.eu/ontologies/demlab.owl#AutonomyAssessment -->

    <owl:Class rdf:about="&demlab;AutonomyAssessment">
        <rdfs:subClassOf rdf:resource="&demlab;ClinicalAssessment"/>
        <rdfs:subClassOf>
            <owl:Restriction>
                <owl:onProperty rdf:resource="&demlab;iadl_e"/>
                <owl:cardinality rdf:datatype="&xsd;nonNegativeInteger">1</owl:cardinality>
            </owl:Restriction>
        </rdfs:subClassOf>
        <rdfs:comment xml:lang="en">Autonomy is assessed based on the performance of the participant during the SemiDirectedActivitiesStep. The property iadl_e (Instrumental Activities of Daily Living for Elderly) can be used to quantify autonomy</rdfs:comment>
        <rdfs:seeAlso rdf:resource="&demlab;SemiDirectedActivitiesStep"/>
        <rdfs:seeAlso rdf:resource="&demlab;iadl_e"/>
    </owl:Class>
    


    <!-- http://www.demcare.eu/ontologies/demlab.owl#CallPsychologistTask -->

    <owl:Class rdf:about="&demlab;CallPsychologistTask">
        <rdfs:subClassOf rdf:resource="&demlab;SemiDirectedTask"/>
        <rdfs:comment xml:lang="en">- The participant has to call the psychologist. Two phone numbers are proposed to the participant (1 visit card of the hair dressing,+ 1 visit card of the CHUN with phone number of a psychologist). 
- According the constraint, the participant has to call the psychologist within the 5 first minutes.</rdfs:comment>
    </owl:Class>
    


    <!-- http://www.demcare.eu/ontologies/demlab.owl#ClinicalAssessment -->

    <owl:Class rdf:about="&demlab;ClinicalAssessment">
        <rdfs:comment xml:lang="en">Root concept for the five types of clinical assessment</rdfs:comment>
        <rdfs:seeAlso rdf:resource="&demlab;AutonomyAssessment"/>
        <rdfs:seeAlso rdf:resource="&demlab;CognitiveAbilitiesAssessment"/>
        <rdfs:seeAlso rdf:resource="&demlab;DiagnosisAssessment"/>
        <rdfs:seeAlso rdf:resource="&demlab;MotricityAbilitiesAssessment"/>
        <rdfs:seeAlso rdf:resource="&demlab;NeuropsychiatricAndMoodAssessment"/>
    </owl:Class>
    


    <!-- http://www.demcare.eu/ontologies/demlab.owl#ClinicalRecord -->

    <owl:Class rdf:about="&demlab;ClinicalRecord">
        <rdfs:subClassOf>
            <owl:Restriction>
                <owl:onProperty rdf:resource="&demlab;containsAssessment"/>
                <owl:allValuesFrom>
                    <owl:Class>
                        <owl:unionOf rdf:parseType="Collection">
                            <rdf:Description rdf:about="&demlab;AutonomyAssessment"/>
                            <rdf:Description rdf:about="&demlab;CognitiveAbilitiesAssessment"/>
                            <rdf:Description rdf:about="&demlab;DiagnosisAssessment"/>
                            <rdf:Description rdf:about="&demlab;MotricityAbilitiesAssessment"/>
                            <rdf:Description rdf:about="&demlab;NeuropsychiatricAndMoodAssessment"/>
                        </owl:unionOf>
                    </owl:Class>
                </owl:allValuesFrom>
            </owl:Restriction>
        </rdfs:subClassOf>
        <rdfs:subClassOf>
            <owl:Restriction>
                <owl:onProperty rdf:resource="&demlab;isClinicalRecordOf"/>
                <owl:onClass rdf:resource="&demlab;Participant"/>
                <owl:qualifiedCardinality rdf:datatype="&xsd;nonNegativeInteger">1</owl:qualifiedCardinality>
            </owl:Restriction>
        </rdfs:subClassOf>
        <rdfs:comment xml:lang="en">A ClinicalRecord contains information about the five types of clinical assessment</rdfs:comment>
        <rdfs:seeAlso rdf:resource="&demlab;ClinicalAssessment"/>
        <rdfs:seeAlso rdf:resource="&demlab;containsAssessment"/>
    </owl:Class>
    


    <!-- http://www.demcare.eu/ontologies/demlab.owl#CognitiveAbilitiesAssessment -->

    <owl:Class rdf:about="&demlab;CognitiveAbilitiesAssessment">
        <rdfs:subClassOf rdf:resource="&demlab;ClinicalAssessment"/>
        <rdfs:subClassOf>
            <owl:Restriction>
                <owl:onProperty rdf:resource="&demlab;shortCognitiveBatteryAssessment"/>
                <owl:cardinality rdf:datatype="&xsd;nonNegativeInteger">1</owl:cardinality>
            </owl:Restriction>
        </rdfs:subClassOf>
        <rdfs:subClassOf>
            <owl:Restriction>
                <owl:onProperty rdf:resource="&demlab;fabScore"/>
                <owl:cardinality rdf:datatype="&xsd;nonNegativeInteger">1</owl:cardinality>
            </owl:Restriction>
        </rdfs:subClassOf>
        <rdfs:subClassOf>
            <owl:Restriction>
                <owl:onProperty rdf:resource="&demlab;hasMMSEScore"/>
                <owl:cardinality rdf:datatype="&xsd;nonNegativeInteger">1</owl:cardinality>
            </owl:Restriction>
        </rdfs:subClassOf>
        <rdfs:subClassOf>
            <owl:Restriction>
                <owl:onProperty rdf:resource="&demlab;freeAndCuedRemindingAssessment"/>
                <owl:cardinality rdf:datatype="&xsd;nonNegativeInteger">1</owl:cardinality>
            </owl:Restriction>
        </rdfs:subClassOf>
        <rdfs:subClassOf>
            <owl:Restriction>
                <owl:onProperty rdf:resource="&demlab;trailMakingTest"/>
                <owl:cardinality rdf:datatype="&xsd;nonNegativeInteger">1</owl:cardinality>
            </owl:Restriction>
        </rdfs:subClassOf>
        <rdfs:comment xml:lang="en">The Cognitive abilities assessment is performed in terms of five scores:
- Mini-Mental State Exam (MMSE). 
- Frontal Assessment Battery (FAB). 
- Trail making test A and B. 
- Short Cognitive Battery. 
- The Free and Cued Selective Reminding Test</rdfs:comment>
        <rdfs:seeAlso rdf:resource="&demlab;fabScore"/>
        <rdfs:seeAlso rdf:resource="&demlab;freeAndCuedRemindingAssessment"/>
        <rdfs:seeAlso rdf:resource="&demlab;hasMMSEScore"/>
        <rdfs:seeAlso rdf:resource="&demlab;shortCognitiveBatteryAssessment"/>
        <rdfs:seeAlso rdf:resource="&demlab;trailMakingTest"/>
    </owl:Class>
    


    <!-- http://www.demcare.eu/ontologies/demlab.owl#CognitiveAbilitiesData -->

    <owl:Class rdf:about="&demlab;CognitiveAbilitiesData">
        <rdfs:subClassOf rdf:resource="&demlab;MeasuredData"/>
        <rdfs:subClassOf>
            <owl:Restriction>
                <owl:onProperty rdf:resource="&demlab;compliantInstructionsOrder"/>
                <owl:qualifiedCardinality rdf:datatype="&xsd;nonNegativeInteger">1</owl:qualifiedCardinality>
                <owl:onDataRange rdf:resource="&xsd;boolean"/>
            </owl:Restriction>
        </rdfs:subClassOf>
        <rdfs:subClassOf>
            <owl:Restriction>
                <owl:onProperty rdf:resource="&demlab;repetitions"/>
                <owl:cardinality rdf:datatype="&xsd;nonNegativeInteger">1</owl:cardinality>
            </owl:Restriction>
        </rdfs:subClassOf>
        <rdfs:subClassOf>
            <owl:Restriction>
                <owl:onProperty rdf:resource="&demlab;activityStatus"/>
                <owl:onClass rdf:resource="&demlab;ActivityStatusType"/>
                <owl:qualifiedCardinality rdf:datatype="&xsd;nonNegativeInteger">1</owl:qualifiedCardinality>
            </owl:Restriction>
        </rdfs:subClassOf>
        <rdfs:comment xml:lang="en">Explore functional abilities for the completion of specific activities</rdfs:comment>
    </owl:Class>
    


    <!-- http://www.demcare.eu/ontologies/demlab.owl#CountingBackwardsTask -->

    <owl:Class rdf:about="&demlab;CountingBackwardsTask">
        <rdfs:subClassOf rdf:resource="&demlab;DirectedTask"/>
        <rdfs:subClassOf>
            <owl:Restriction>
                <owl:onProperty rdf:resource="&demlab;measuredData"/>
                <owl:allValuesFrom>
                    <owl:Class>
                        <owl:unionOf rdf:parseType="Collection">
                            <rdf:Description rdf:about="&demlab;LatencyData"/>
                            <rdf:Description rdf:about="&demlab;StressData"/>
                            <rdf:Description rdf:about="&demlab;VoiceData"/>
                        </owl:unionOf>
                    </owl:Class>
                </owl:allValuesFrom>
            </owl:Restriction>
        </rdfs:subClassOf>
        <rdfs:comment xml:lang="en">(MonoTask) The participant is standing and the clinician asks him/her to count aloud backwards: 
- From 305 to 285 (to change tens and hundreds) one by one; or 
- From 20 to 0 if they make counting mistakes after 2 attempts of the previous backwards counting

This task is used for assessing:
- Latency: time of latency between the end of instructions (stimulation) and the beginning of the task
- Stress level
- Voice: e.g. speech fluency and articulation</rdfs:comment>
    </owl:Class>
    


    <!-- http://www.demcare.eu/ontologies/demlab.owl#DiagnosisAssessment -->

    <owl:Class rdf:about="&demlab;DiagnosisAssessment">
        <rdfs:subClassOf rdf:resource="&demlab;ClinicalAssessment"/>
        <rdfs:subClassOf>
            <owl:Restriction>
                <owl:onProperty rdf:resource="&demlab;hasClinicalDiagnosis"/>
                <owl:onClass rdf:resource="&demlab;DiagnosisType"/>
                <owl:qualifiedCardinality rdf:datatype="&xsd;nonNegativeInteger">1</owl:qualifiedCardinality>
            </owl:Restriction>
        </rdfs:subClassOf>
        <rdfs:comment xml:lang="en">Diagnosis established the day of the recording session. Participant is assigned to one of this 3 categories: Healthy Control participants, Alzheimer’s disease at pre-dementia stage, Alzheimer ’s disease at dementia stage</rdfs:comment>
        <rdfs:seeAlso rdf:resource="&demlab;DiagnosisType"/>
        <rdfs:seeAlso rdf:resource="&demlab;HealthyControlParticipant"/>
        <rdfs:seeAlso rdf:resource="&demlab;PersonWithDementia"/>
        <rdfs:seeAlso rdf:resource="&demlab;PersonWithPredementia"/>
        <rdfs:seeAlso rdf:resource="&demlab;hasClinicalDiagnosis"/>
    </owl:Class>
    


    <!-- http://www.demcare.eu/ontologies/demlab.owl#DiagnosisType -->

    <owl:Class rdf:about="&demlab;DiagnosisType">
        <owl:equivalentClass>
            <owl:Class>
                <owl:oneOf rdf:parseType="Collection">
                    <rdf:Description rdf:about="&demlab;healthy"/>
                    <rdf:Description rdf:about="&demlab;dementia"/>
                    <rdf:Description rdf:about="&demlab;predementia"/>
                </owl:oneOf>
            </owl:Class>
        </owl:equivalentClass>
    </owl:Class>
    


    <!-- http://www.demcare.eu/ontologies/demlab.owl#DirectedActivitiesStep -->

    <owl:Class rdf:about="&demlab;DirectedActivitiesStep">
        <rdfs:subClassOf rdf:resource="&demlab;ProtocolStep"/>
        <rdfs:subClassOf>
            <owl:Restriction>
                <owl:onProperty rdf:resource="&demlab;involvesTask"/>
                <owl:allValuesFrom>
                    <owl:Class>
                        <owl:unionOf rdf:parseType="Collection">
                            <rdf:Description rdf:about="&demlab;ArticulationControlTask"/>
                            <rdf:Description rdf:about="&demlab;CountingBackwardsTask"/>
                            <rdf:Description rdf:about="&demlab;SentenceRepeatingTask"/>
                            <rdf:Description rdf:about="&demlab;Task"/>
                            <rdf:Description rdf:about="&demlab;WalkingCountingBackwardsTask"/>
                            <rdf:Description rdf:about="&demlab;WalkingTask"/>
                        </owl:unionOf>
                    </owl:Class>
                </owl:allValuesFrom>
            </owl:Restriction>
        </rdfs:subClassOf>
        <rdfs:comment xml:lang="en">This ProtocolStep is conducted by a clinician, who details step by step the different activities to do by the participant. This step involves five Tasks. The tasks Walking, CountingBackwards and WalkingAndCountingBackwards are used for characterizing participants’ gait in mono and dual tasks, and the impact of cognitive activity on gait (e.g., walking speed, step length, stops during the walking exercise done in dual task). The tasks SentenceRepeating and ArticulationControl are vocally-directed tasks: one task consists of repeating a sentence after the clinician (this task is repeated with three sentences), and the other is an articulation control exercise done to evaluate the neuromuscular mechanism of speech production.</rdfs:comment>
    </owl:Class>
    


    <!-- http://www.demcare.eu/ontologies/demlab.owl#DirectedDiscussionTask -->

    <owl:Class rdf:about="&demlab;DirectedDiscussionTask">
        <rdfs:subClassOf rdf:resource="&demlab;DiscussionTask"/>
    </owl:Class>
    


    <!-- http://www.demcare.eu/ontologies/demlab.owl#DirectedExpressionTask -->

    <owl:Class rdf:about="&demlab;DirectedExpressionTask">
        <rdfs:subClassOf rdf:resource="&demlab;DirectedDiscussionTask"/>
        <rdfs:comment xml:lang="en">The clinician asks the same questions than the ones asked on the read article, e.g. What is the topic of the article?</rdfs:comment>
    </owl:Class>
    


    <!-- http://www.demcare.eu/ontologies/demlab.owl#DirectedTask -->

    <owl:Class rdf:about="&demlab;DirectedTask">
        <rdfs:subClassOf rdf:resource="&demlab;Task"/>
        <rdfs:comment xml:lang="en">Root concept for grouping the Tasks relevant to the DirectedActivitiesStep</rdfs:comment>
        <rdfs:seeAlso rdf:resource="&demlab;DirectedActivitiesStep"/>
        <rdfs:seeAlso rdf:resource="&demlab;Task"/>
    </owl:Class>
    


    <!-- http://www.demcare.eu/ontologies/demlab.owl#DiscussionInvolvementData -->

    <owl:Class rdf:about="&demlab;DiscussionInvolvementData">
        <rdfs:subClassOf rdf:resource="&demlab;MeasuredData"/>
        <rdfs:subClassOf>
            <owl:Restriction>
                <owl:onProperty rdf:resource="&demlab;verbalReactionSpontaneity"/>
                <owl:cardinality rdf:datatype="&xsd;nonNegativeInteger">1</owl:cardinality>
            </owl:Restriction>
        </rdfs:subClassOf>
        <rdfs:comment xml:lang="en">- Assessment of the impact of cognitive load imposed by the picture description task on speech fluency
- Memory and self-appraisal assessment
- Verbal fluency and mood (Apathy) assessment</rdfs:comment>
    </owl:Class>
    


    <!-- http://www.demcare.eu/ontologies/demlab.owl#DiscussionTask -->

    <owl:Class rdf:about="&demlab;DiscussionTask">
        <rdfs:subClassOf rdf:resource="&demlab;Task"/>
        <rdfs:subClassOf>
            <owl:Restriction>
                <owl:onProperty rdf:resource="&demlab;measuredData"/>
                <owl:allValuesFrom>
                    <owl:Class>
                        <owl:unionOf rdf:parseType="Collection">
                            <rdf:Description rdf:about="&demlab;StressData"/>
                            <rdf:Description rdf:about="&demlab;VoiceData"/>
                        </owl:unionOf>
                    </owl:Class>
                </owl:allValuesFrom>
            </owl:Restriction>
        </rdfs:subClassOf>
        <rdfs:comment xml:lang="en">Root concept for grouping the Tasks relevant to the DiscussionWithClinicianStep

The relevant tasks are used for assessing:
- Stress level
- Voice: e.g. speech rate, pause rate etc.</rdfs:comment>
    </owl:Class>
    


    <!-- http://www.demcare.eu/ontologies/demlab.owl#DiscussionWithClinicianStep -->

    <owl:Class rdf:about="&demlab;DiscussionWithClinicianStep">
        <rdfs:subClassOf rdf:resource="&demlab;ProtocolStep"/>
        <rdfs:subClassOf>
            <owl:Restriction>
                <owl:onProperty rdf:resource="&demlab;involvesTask"/>
                <owl:allValuesFrom>
                    <owl:Class>
                        <owl:unionOf rdf:parseType="Collection">
                            <rdf:Description rdf:about="&demlab;DirectedExpressionTask"/>
                            <rdf:Description rdf:about="&demlab;PictureDescriptionTask"/>
                            <rdf:Description rdf:about="&demlab;PictureDiscussionTask"/>
                        </owl:unionOf>
                    </owl:Class>
                </owl:allValuesFrom>
            </owl:Restriction>
        </rdfs:subClassOf>
        <rdfs:comment xml:lang="en">This ProtocolStep involves two Tasks. The first task (DirectedExpressionTask) is a directed discussion during which the clinician assesses the episodic memory of participant through questions related to events and activities of SemiDirectedActivitiesStep. The second task (PictureDescriptionTask) assesses the verbal fluency and mood of participant using a picture that the participant has to describe (with the picture in the eyes) and then to involve a discussion about their interests for the activity represented. This part is done with two different pictures.</rdfs:comment>
    </owl:Class>
    


    <!-- http://www.demcare.eu/ontologies/demlab.owl#EstablishAccountBalanceTask -->

    <owl:Class rdf:about="&demlab;EstablishAccountBalanceTask">
        <rdfs:subClassOf rdf:resource="&demlab;SemiDirectedTask"/>
        <rdfs:comment xml:lang="en">- Three bills (Electricity/Gaz/Phone) are proposed. The account balance is given. 
- The participant has to establish the amount balance after having taken into account the three bills.</rdfs:comment>
    </owl:Class>
    


    <!-- http://www.demcare.eu/ontologies/demlab.owl#FindBusLineOnMapTask -->

    <owl:Class rdf:about="&demlab;FindBusLineOnMapTask">
        <rdfs:subClassOf rdf:resource="&demlab;SemiDirectedTask"/>
        <rdfs:comment xml:lang="en">- A real bus map is showed to the participant with the indication of the current location of the participant. 
- The participant has to write on a sheet of paper located next to the bus map the bus lines to take for the itinerary (From Hospital to Station train). Two itineraries are accepted.</rdfs:comment>
    </owl:Class>
    


    <!-- http://www.demcare.eu/ontologies/demlab.owl#FreeDiscussionTask -->

    <owl:Class rdf:about="&demlab;FreeDiscussionTask">
        <rdfs:subClassOf rdf:resource="&demlab;DiscussionTask"/>
    </owl:Class>
    


    <!-- http://www.demcare.eu/ontologies/demlab.owl#FunctionalAbilitiesData -->

    <owl:Class rdf:about="&demlab;FunctionalAbilitiesData">
        <rdfs:subClassOf rdf:resource="&demlab;MeasuredData"/>
        <rdfs:subClassOf>
            <owl:Restriction>
                <owl:onProperty rdf:resource="&demlab;handTrajectory"/>
                <owl:onClass rdf:resource="&demlab;HandTrajectoryType"/>
                <owl:qualifiedCardinality rdf:datatype="&xsd;nonNegativeInteger">1</owl:qualifiedCardinality>
            </owl:Restriction>
        </rdfs:subClassOf>
        <rdfs:comment xml:lang="en">Explore functional abilities for the completion of specific activities</rdfs:comment>
    </owl:Class>
    


    <!-- http://www.demcare.eu/ontologies/demlab.owl#GaitData -->

    <owl:Class rdf:about="&demlab;GaitData">
        <rdfs:subClassOf rdf:resource="&demlab;MeasuredData"/>
        <rdfs:subClassOf>
            <owl:Restriction>
                <owl:onProperty rdf:resource="&demlab;stepLength"/>
                <owl:cardinality rdf:datatype="&xsd;nonNegativeInteger">1</owl:cardinality>
            </owl:Restriction>
        </rdfs:subClassOf>
        <rdfs:subClassOf>
            <owl:Restriction>
                <owl:onProperty rdf:resource="&demlab;dynamicBalance"/>
                <owl:cardinality rdf:datatype="&xsd;nonNegativeInteger">1</owl:cardinality>
            </owl:Restriction>
        </rdfs:subClassOf>
        <rdfs:subClassOf>
            <owl:Restriction>
                <owl:onProperty rdf:resource="&demlab;walkingSpeedInstantaneous"/>
                <owl:cardinality rdf:datatype="&xsd;nonNegativeInteger">1</owl:cardinality>
            </owl:Restriction>
        </rdfs:subClassOf>
        <rdfs:subClassOf>
            <owl:Restriction>
                <owl:onProperty rdf:resource="&demlab;walkingSpeed"/>
                <owl:cardinality rdf:datatype="&xsd;nonNegativeInteger">1</owl:cardinality>
            </owl:Restriction>
        </rdfs:subClassOf>
        <rdfs:subClassOf>
            <owl:Restriction>
                <owl:onProperty rdf:resource="&demlab;stoppingDisplacement"/>
                <owl:qualifiedCardinality rdf:datatype="&xsd;nonNegativeInteger">1</owl:qualifiedCardinality>
                <owl:onDataRange rdf:resource="&xsd;boolean"/>
            </owl:Restriction>
        </rdfs:subClassOf>
        <rdfs:comment xml:lang="en">Gait assessment and impact of a cognitive activity on gait performance</rdfs:comment>
    </owl:Class>
    


    <!-- http://www.demcare.eu/ontologies/demlab.owl#HandTrajectoryType -->

    <owl:Class rdf:about="&demlab;HandTrajectoryType"/>
    


    <!-- http://www.demcare.eu/ontologies/demlab.owl#HealthyControlParticipant -->

    <owl:Class rdf:about="&demlab;HealthyControlParticipant">
        <owl:equivalentClass>
            <owl:Restriction>
                <owl:onProperty rdf:resource="&demlab;hasClinicalRecord"/>
                <owl:someValuesFrom>
                    <owl:Class>
                        <owl:intersectionOf rdf:parseType="Collection">
                            <rdf:Description rdf:about="&demlab;ClinicalRecord"/>
                            <owl:Restriction>
                                <owl:onProperty rdf:resource="&demlab;containsAssessment"/>
                                <owl:someValuesFrom>
                                    <owl:Class>
                                        <owl:intersectionOf rdf:parseType="Collection">
                                            <rdf:Description rdf:about="&demlab;DiagnosisAssessment"/>
                                            <owl:Restriction>
                                                <owl:onProperty rdf:resource="&demlab;hasClinicalDiagnosis"/>
                                                <owl:someValuesFrom>
                                                    <owl:Class>
                                                        <owl:oneOf rdf:parseType="Collection">
                                                            <rdf:Description rdf:about="&demlab;healthy"/>
                                                        </owl:oneOf>
                                                    </owl:Class>
                                                </owl:someValuesFrom>
                                            </owl:Restriction>
                                        </owl:intersectionOf>
                                    </owl:Class>
                                </owl:someValuesFrom>
                            </owl:Restriction>
                        </owl:intersectionOf>
                    </owl:Class>
                </owl:someValuesFrom>
            </owl:Restriction>
        </owl:equivalentClass>
        <rdfs:subClassOf rdf:resource="&demlab;Participant"/>
        <rdfs:comment xml:lang="en">A Healthy Control Participant is defined as the participant whose clinical record contains a healthy clinical diagnosis</rdfs:comment>
        <rdfs:seeAlso rdf:resource="&demlab;ClinicalRecord"/>
        <rdfs:seeAlso rdf:resource="&demlab;DiagnosisAssessment"/>
        <rdfs:seeAlso rdf:resource="&demlab;DiagnosisType"/>
        <rdfs:seeAlso rdf:resource="&demlab;healthy"/>
    </owl:Class>
    


    <!-- http://www.demcare.eu/ontologies/demlab.owl#LatencyData -->

    <owl:Class rdf:about="&demlab;LatencyData">
        <rdfs:subClassOf rdf:resource="&demlab;MeasuredData"/>
        <rdfs:subClassOf>
            <owl:Restriction>
                <owl:onProperty rdf:resource="&demlab;latency"/>
                <owl:cardinality rdf:datatype="&xsd;nonNegativeInteger">1</owl:cardinality>
            </owl:Restriction>
        </rdfs:subClassOf>
        <rdfs:comment xml:lang="en">Explore the time of latency [stimulation, response] during the DirectedActivitiesTask (Explore sensitivity of this measure for assessing the apathy)</rdfs:comment>
    </owl:Class>
    


    <!-- http://www.demcare.eu/ontologies/demlab.owl#LeaveRoomTask -->

    <owl:Class rdf:about="&demlab;LeaveRoomTask">
        <rdfs:subClassOf rdf:resource="&demlab;SemiDirectedTask"/>
        <rdfs:comment xml:lang="en">The participant has to leave the room when he/she feels that all activities are performed and achieved</rdfs:comment>
    </owl:Class>
    


    <!-- http://www.demcare.eu/ontologies/demlab.owl#MeasuredData -->

    <owl:Class rdf:about="&demlab;MeasuredData">
        <rdfs:comment>MeasuredData is the root concept that groups the measurement types that are collected during the Tasks.</rdfs:comment>
    </owl:Class>
    


    <!-- http://www.demcare.eu/ontologies/demlab.owl#MotricityAbilitiesAssessment -->

    <owl:Class rdf:about="&demlab;MotricityAbilitiesAssessment">
        <rdfs:subClassOf rdf:resource="&demlab;ClinicalAssessment"/>
        <rdfs:subClassOf>
            <owl:Restriction>
                <owl:onProperty rdf:resource="&demlab;hasUPDRSScore"/>
                <owl:qualifiedCardinality rdf:datatype="&xsd;nonNegativeInteger">1</owl:qualifiedCardinality>
                <owl:onDataRange rdf:resource="&xsd;int"/>
            </owl:Restriction>
        </rdfs:subClassOf>
        <rdfs:comment xml:lang="en">Motricity abilities assessment:
- Part III of the Unified Parkinson’s Disease Rating Scale (UPDRS) .</rdfs:comment>
        <rdfs:seeAlso rdf:resource="&demlab;hasUPDRSScore"/>
    </owl:Class>
    


    <!-- http://www.demcare.eu/ontologies/demlab.owl#NeuropsychiatricAndMoodAssessment -->

    <owl:Class rdf:about="&demlab;NeuropsychiatricAndMoodAssessment">
        <rdfs:subClassOf rdf:resource="&demlab;ClinicalAssessment"/>
        <rdfs:subClassOf>
            <owl:Restriction>
                <owl:onProperty rdf:resource="&demlab;apathyInventory"/>
                <owl:cardinality rdf:datatype="&xsd;nonNegativeInteger">1</owl:cardinality>
            </owl:Restriction>
        </rdfs:subClassOf>
        <rdfs:subClassOf>
            <owl:Restriction>
                <owl:onProperty rdf:resource="&demlab;npi"/>
                <owl:cardinality rdf:datatype="&xsd;nonNegativeInteger">1</owl:cardinality>
            </owl:Restriction>
        </rdfs:subClassOf>
        <rdfs:subClassOf>
            <owl:Restriction>
                <owl:onProperty rdf:resource="&demlab;dsm_ivDepressionCriteria"/>
                <owl:cardinality rdf:datatype="&xsd;nonNegativeInteger">1</owl:cardinality>
            </owl:Restriction>
        </rdfs:subClassOf>
        <rdfs:comment xml:lang="en">Neuropsychiatric/Mood assessments:
- NPI 
- DSM-IV Criteria for depression 
- Apathy Inventory (AI) and diagnostic criteria for apathy.</rdfs:comment>
        <rdfs:seeAlso rdf:resource="&demlab;apathyInventory"/>
        <rdfs:seeAlso rdf:resource="&demlab;dsm_ivDepressionCriteria"/>
        <rdfs:seeAlso rdf:resource="&demlab;npi"/>
    </owl:Class>
    


    <!-- http://www.demcare.eu/ontologies/demlab.owl#OrganisationEfficiencyData -->

    <owl:Class rdf:about="&demlab;OrganisationEfficiencyData">
        <rdfs:subClassOf rdf:resource="&demlab;MeasuredData"/>
        <rdfs:subClassOf>
            <owl:Restriction>
                <owl:onProperty rdf:resource="&demlab;areasOfNoInterestExplored"/>
                <owl:someValuesFrom rdf:resource="&demlab;Zone"/>
            </owl:Restriction>
        </rdfs:subClassOf>
        <rdfs:subClassOf>
            <owl:Restriction>
                <owl:onProperty rdf:resource="&demlab;areasOfInterestExplored"/>
                <owl:someValuesFrom rdf:resource="&demlab;Zone"/>
            </owl:Restriction>
        </rdfs:subClassOf>
        <rdfs:subClassOf>
            <owl:Restriction>
                <owl:onProperty rdf:resource="&demlab;distanceWalked"/>
                <owl:cardinality rdf:datatype="&xsd;nonNegativeInteger">1</owl:cardinality>
            </owl:Restriction>
        </rdfs:subClassOf>
        <rdfs:comment xml:lang="en">Explore ability to organize with efficiency the different activities</rdfs:comment>
    </owl:Class>
    


    <!-- http://www.demcare.eu/ontologies/demlab.owl#Participant -->

    <owl:Class rdf:about="&demlab;Participant">
        <rdfs:subClassOf rdf:resource="http://xmlns.com/foaf/0.1/Person"/>
        <rdfs:subClassOf>
            <owl:Restriction>
                <owl:onProperty rdf:resource="&demlab;participates"/>
                <owl:someValuesFrom rdf:resource="&demlab;Protocol"/>
            </owl:Restriction>
        </rdfs:subClassOf>
        <rdfs:subClassOf>
            <owl:Restriction>
                <owl:onProperty rdf:resource="&demlab;hasClinicalRecord"/>
                <owl:onClass rdf:resource="&demlab;ClinicalRecord"/>
                <owl:qualifiedCardinality rdf:datatype="&xsd;nonNegativeInteger">1</owl:qualifiedCardinality>
            </owl:Restriction>
        </rdfs:subClassOf>
    </owl:Class>
    


    <!-- http://www.demcare.eu/ontologies/demlab.owl#PayBillTask -->

    <owl:Class rdf:about="&demlab;PayBillTask">
        <rdfs:subClassOf rdf:resource="&demlab;SemiDirectedTask"/>
        <rdfs:comment xml:lang="en">- Three bills (Electricity/Gaz/Phone) are proposed. The participant has to pay the phone bill by check. 
- The check is well completed if the amount, order (i.e. Phone Company), date and signature are right.</rdfs:comment>
    </owl:Class>
    


    <!-- http://www.demcare.eu/ontologies/demlab.owl#PersonWithDementia -->

    <owl:Class rdf:about="&demlab;PersonWithDementia">
        <owl:equivalentClass>
            <owl:Restriction>
                <owl:onProperty rdf:resource="&demlab;hasClinicalRecord"/>
                <owl:someValuesFrom>
                    <owl:Class>
                        <owl:intersectionOf rdf:parseType="Collection">
                            <rdf:Description rdf:about="&demlab;ClinicalRecord"/>
                            <owl:Restriction>
                                <owl:onProperty rdf:resource="&demlab;containsAssessment"/>
                                <owl:someValuesFrom>
                                    <owl:Class>
                                        <owl:intersectionOf rdf:parseType="Collection">
                                            <rdf:Description rdf:about="&demlab;DiagnosisAssessment"/>
                                            <owl:Restriction>
                                                <owl:onProperty rdf:resource="&demlab;hasClinicalDiagnosis"/>
                                                <owl:someValuesFrom>
                                                    <owl:Class>
                                                        <owl:oneOf rdf:parseType="Collection">
                                                            <rdf:Description rdf:about="&demlab;dementia"/>
                                                        </owl:oneOf>
                                                    </owl:Class>
                                                </owl:someValuesFrom>
                                            </owl:Restriction>
                                        </owl:intersectionOf>
                                    </owl:Class>
                                </owl:someValuesFrom>
                            </owl:Restriction>
                        </owl:intersectionOf>
                    </owl:Class>
                </owl:someValuesFrom>
            </owl:Restriction>
        </owl:equivalentClass>
        <rdfs:subClassOf rdf:resource="&demlab;Participant"/>
        <rdfs:comment xml:lang="en">A Person with Dementia is defined as the participant whose clinical record contains a dementia clinical diagnosis</rdfs:comment>
        <rdfs:seeAlso rdf:resource="&demlab;ClinicalRecord"/>
        <rdfs:seeAlso rdf:resource="&demlab;DiagnosisAssessment"/>
        <rdfs:seeAlso rdf:resource="&demlab;DiagnosisType"/>
        <rdfs:seeAlso rdf:resource="&demlab;dementia"/>
    </owl:Class>
    


    <!-- http://www.demcare.eu/ontologies/demlab.owl#PersonWithPredementia -->

    <owl:Class rdf:about="&demlab;PersonWithPredementia">
        <owl:equivalentClass>
            <owl:Restriction>
                <owl:onProperty rdf:resource="&demlab;hasClinicalRecord"/>
                <owl:someValuesFrom>
                    <owl:Class>
                        <owl:intersectionOf rdf:parseType="Collection">
                            <rdf:Description rdf:about="&demlab;ClinicalRecord"/>
                            <owl:Restriction>
                                <owl:onProperty rdf:resource="&demlab;containsAssessment"/>
                                <owl:someValuesFrom>
                                    <owl:Class>
                                        <owl:intersectionOf rdf:parseType="Collection">
                                            <rdf:Description rdf:about="&demlab;DiagnosisAssessment"/>
                                            <owl:Restriction>
                                                <owl:onProperty rdf:resource="&demlab;hasClinicalDiagnosis"/>
                                                <owl:someValuesFrom>
                                                    <owl:Class>
                                                        <owl:oneOf rdf:parseType="Collection">
                                                            <rdf:Description rdf:about="&demlab;predementia"/>
                                                        </owl:oneOf>
                                                    </owl:Class>
                                                </owl:someValuesFrom>
                                            </owl:Restriction>
                                        </owl:intersectionOf>
                                    </owl:Class>
                                </owl:someValuesFrom>
                            </owl:Restriction>
                        </owl:intersectionOf>
                    </owl:Class>
                </owl:someValuesFrom>
            </owl:Restriction>
        </owl:equivalentClass>
        <rdfs:subClassOf rdf:resource="&demlab;Participant"/>
        <rdfs:comment xml:lang="en">A Person with Predementia is defined as the participant whose clinical record contains a predementia clinical diagnosis</rdfs:comment>
        <rdfs:seeAlso rdf:resource="&demlab;ClinicalRecord"/>
        <rdfs:seeAlso rdf:resource="&demlab;DiagnosisAssessment"/>
        <rdfs:seeAlso rdf:resource="&demlab;DiagnosisType"/>
        <rdfs:seeAlso rdf:resource="&demlab;predementia"/>
    </owl:Class>
    


    <!-- http://www.demcare.eu/ontologies/demlab.owl#PictureDescriptionTask -->

    <owl:Class rdf:about="&demlab;PictureDescriptionTask">
        <rdfs:subClassOf rdf:resource="&demlab;FreeDiscussionTask"/>
        <rdfs:comment xml:lang="en">The clinician shows to the participant one picture representing daily activity and asks the participants to give a verbal description of the picture in a few sentences</rdfs:comment>
    </owl:Class>
    


    <!-- http://www.demcare.eu/ontologies/demlab.owl#PictureDiscussionTask -->

    <owl:Class rdf:about="&demlab;PictureDiscussionTask">
        <rdfs:subClassOf rdf:resource="&demlab;FreeDiscussionTask"/>
        <rdfs:comment xml:lang="en">The clinician asks if the participant likes doing this activity and why</rdfs:comment>
    </owl:Class>
    


    <!-- http://www.demcare.eu/ontologies/demlab.owl#PrepareDrugBoxTask -->

    <owl:Class rdf:about="&demlab;PrepareDrugBoxTask">
        <rdfs:subClassOf rdf:resource="&demlab;SemiDirectedTask"/>
        <rdfs:comment xml:lang="en">- 4 types of drugs are proposed to the participant. 
- The participant has to respect the posology prescribed (2 types of drugs at different moment of the day) and the date (day and moment of the day).</rdfs:comment>
    </owl:Class>
    


    <!-- http://www.demcare.eu/ontologies/demlab.owl#PrepareHotTeaTask -->

    <owl:Class rdf:about="&demlab;PrepareHotTeaTask">
        <rdfs:subClassOf rdf:resource="&demlab;SemiDirectedTask"/>
        <rdfs:comment xml:lang="en">- The participant has to switch on the electric kettle. 
- The participant has to pour the hot water on the glass containing the tea bag.</rdfs:comment>
    </owl:Class>
    


    <!-- http://www.demcare.eu/ontologies/demlab.owl#Protocol -->

    <owl:Class rdf:about="&demlab;Protocol">
        <rdfs:subClassOf>
            <owl:Restriction>
                <owl:onProperty rdf:resource="&demlab;hasProtocolStep"/>
                <owl:someValuesFrom rdf:resource="&demlab;ProtocolStep"/>
            </owl:Restriction>
        </rdfs:subClassOf>
        <rdfs:subClassOf>
            <owl:Restriction>
                <owl:onProperty rdf:resource="http://www.w3.org/2006/time#hasEnd"/>
                <owl:onClass rdf:resource="http://www.w3.org/2006/time#Instant"/>
                <owl:qualifiedCardinality rdf:datatype="&xsd;nonNegativeInteger">1</owl:qualifiedCardinality>
            </owl:Restriction>
        </rdfs:subClassOf>
        <rdfs:subClassOf>
            <owl:Restriction>
                <owl:onProperty rdf:resource="http://www.w3.org/2006/time#hasBeginning"/>
                <owl:onClass rdf:resource="http://www.w3.org/2006/time#Instant"/>
                <owl:qualifiedCardinality rdf:datatype="&xsd;nonNegativeInteger">1</owl:qualifiedCardinality>
            </owl:Restriction>
        </rdfs:subClassOf>
        <rdfs:subClassOf>
            <owl:Restriction>
                <owl:onProperty rdf:resource="&demlab;hasParticipant"/>
                <owl:onClass rdf:resource="http://xmlns.com/foaf/0.1/Person"/>
                <owl:qualifiedCardinality rdf:datatype="&xsd;nonNegativeInteger">1</owl:qualifiedCardinality>
            </owl:Restriction>
        </rdfs:subClassOf>
        <rdfs:comment xml:lang="en">A Protocol instance contains information regarding the participant and the duration of the protocol session. It can be also associated with one or more ProtocolSteps that define the Tasks and the corresponding MeasuredData.</rdfs:comment>
        <rdfs:seeAlso rdf:resource="&demlab;MeasuredData"/>
        <rdfs:seeAlso rdf:resource="&demlab;ProtocolStep"/>
        <rdfs:seeAlso rdf:resource="&demlab;Task"/>
    </owl:Class>
    


    <!-- http://www.demcare.eu/ontologies/demlab.owl#ProtocolStep -->

    <owl:Class rdf:about="&demlab;ProtocolStep">
        <rdfs:subClassOf>
            <owl:Restriction>
                <owl:onProperty rdf:resource="&demlab;involvesTask"/>
                <owl:someValuesFrom rdf:resource="&demlab;Task"/>
            </owl:Restriction>
        </rdfs:subClassOf>
        <rdfs:subClassOf>
            <owl:Restriction>
                <owl:onProperty rdf:resource="http://www.w3.org/2006/time#hasEnd"/>
                <owl:onClass rdf:resource="http://www.w3.org/2006/time#Instant"/>
                <owl:qualifiedCardinality rdf:datatype="&xsd;nonNegativeInteger">1</owl:qualifiedCardinality>
            </owl:Restriction>
        </rdfs:subClassOf>
        <rdfs:subClassOf>
            <owl:Restriction>
                <owl:onProperty rdf:resource="http://www.w3.org/2006/time#hasBeginning"/>
                <owl:onClass rdf:resource="http://www.w3.org/2006/time#Instant"/>
                <owl:qualifiedCardinality rdf:datatype="&xsd;nonNegativeInteger">1</owl:qualifiedCardinality>
            </owl:Restriction>
        </rdfs:subClassOf>
        <rdfs:comment xml:lang="en">A ProtocolStep defines the Tasks of interest. Three ProtocolStep types are currently defined in Dem@Care: DirectedActivities, SemiDirectedActivities and DiscussionWithTheClinician</rdfs:comment>
        <rdfs:seeAlso rdf:resource="&demlab;DirectedActivitiesStep"/>
        <rdfs:seeAlso rdf:resource="&demlab;DiscussionWithClinicianStep"/>
        <rdfs:seeAlso rdf:resource="&demlab;SemiDirectedActivitiesStep"/>
        <rdfs:seeAlso rdf:resource="&demlab;Task"/>
    </owl:Class>
    


    <!-- http://www.demcare.eu/ontologies/demlab.owl#ReadArticleTask -->

    <owl:Class rdf:about="&demlab;ReadArticleTask">
        <rdfs:subClassOf rdf:resource="&demlab;SemiDirectedTask"/>
        <rdfs:comment xml:lang="en">Three articles are proposed to the participant (Topics: Collection Cars; Cooking; Sightseeing). The three articles have the same words number and level of difficulty. Below each articles, the 3 following questions are asked
- Q1/ What is the topic of the article? 
- Q2/ What is the percentage of French interested in the … (Collection Car / Cooking / Sightseeing, text adapted to the article topic)? 
- Q3/ Who is interviewed?</rdfs:comment>
    </owl:Class>
    


    <!-- http://www.demcare.eu/ontologies/demlab.owl#SemiDirectedActivitiesStep -->

    <owl:Class rdf:about="&demlab;SemiDirectedActivitiesStep">
        <rdfs:subClassOf rdf:resource="&demlab;ProtocolStep"/>
        <rdfs:subClassOf>
            <owl:Restriction>
                <owl:onProperty rdf:resource="&demlab;involvesTask"/>
                <owl:allValuesFrom>
                    <owl:Class>
                        <owl:unionOf rdf:parseType="Collection">
                            <rdf:Description rdf:about="&demlab;AnswerPhoneTask"/>
                            <rdf:Description rdf:about="&demlab;CallPsychologistTask"/>
                            <rdf:Description rdf:about="&demlab;EstablishAccountBalanceTask"/>
                            <rdf:Description rdf:about="&demlab;FindBusLineOnMapTask"/>
                            <rdf:Description rdf:about="&demlab;LeaveRoomTask"/>
                            <rdf:Description rdf:about="&demlab;PayBillTask"/>
                            <rdf:Description rdf:about="&demlab;PrepareDrugBoxTask"/>
                            <rdf:Description rdf:about="&demlab;PrepareHotTeaTask"/>
                            <rdf:Description rdf:about="&demlab;Task"/>
                            <rdf:Description rdf:about="&demlab;TurnOnTVTask"/>
                            <rdf:Description rdf:about="&demlab;WaterPlantTask"/>
                        </owl:unionOf>
                    </owl:Class>
                </owl:allValuesFrom>
            </owl:Restriction>
        </rdfs:subClassOf>
        <rdfs:comment xml:lang="en">This ProtocolStep consists of assessing the autonomy of the participant. The participant has to organize himself/herself and correctly perform a list of Instrumental Activities of Daily Living (e.g., managing finance, using phone, preparing tea) within a timeframe of 15minutes. For this step, the participant is alone in the experimental setting and can refer to the instruction sheet of paper with the IADLs to perform at any time.</rdfs:comment>
    </owl:Class>
    


    <!-- http://www.demcare.eu/ontologies/demlab.owl#SemiDirectedTask -->

    <owl:Class rdf:about="&demlab;SemiDirectedTask">
        <rdfs:subClassOf rdf:resource="&demlab;Task"/>
        <rdfs:subClassOf>
            <owl:Restriction>
                <owl:onProperty rdf:resource="&demlab;measuredData"/>
                <owl:allValuesFrom>
                    <owl:Class>
                        <owl:unionOf rdf:parseType="Collection">
                            <rdf:Description rdf:about="&demlab;CognitiveAbilitiesData"/>
                            <rdf:Description rdf:about="&demlab;FunctionalAbilitiesData"/>
                            <rdf:Description rdf:about="&demlab;StressData"/>
                        </owl:unionOf>
                    </owl:Class>
                </owl:allValuesFrom>
            </owl:Restriction>
        </rdfs:subClassOf>
        <rdfs:comment xml:lang="en">In this Task the participant has to organize himself/herself and correctly perform a list of Instrumental Activities of Daily Living (e.g., managing finance, using phone, preparing tea) within a timeframe of 15minutes.

The relevant tasks are used for assessing:
- Cognitive abilities through activity repetitions, missed activities, order of activities
- Functional abilities for the completion of specific activities: e.g. hand trajectories
- Stress level</rdfs:comment>
    </owl:Class>
    


    <!-- http://www.demcare.eu/ontologies/demlab.owl#SentenceRepeatingTask -->

    <owl:Class rdf:about="&demlab;SentenceRepeatingTask">
        <rdfs:subClassOf rdf:resource="&demlab;DirectedTask"/>
        <rdfs:subClassOf>
            <owl:Restriction>
                <owl:onProperty rdf:resource="&demlab;measuredData"/>
                <owl:allValuesFrom>
                    <owl:Class>
                        <owl:unionOf rdf:parseType="Collection">
                            <rdf:Description rdf:about="&demlab;LatencyData"/>
                            <rdf:Description rdf:about="&demlab;StressData"/>
                            <rdf:Description rdf:about="&demlab;VoiceData"/>
                        </owl:unionOf>
                    </owl:Class>
                </owl:allValuesFrom>
            </owl:Restriction>
        </rdfs:subClassOf>
        <rdfs:comment xml:lang="en">- The participant is asked to repeat a short sentence after the assessor. 
- The assessor reads aloud a sentence. The participant repeats the sentence. The action is done once by sentence. Three sentences must be repeated.

This task is used for assessing:
- Latency: time of latency between the end of instructions (stimulation) and the beginning of the task
- Stress level
- Voice: e.g. verbal reaction time</rdfs:comment>
    </owl:Class>
    


    <!-- http://www.demcare.eu/ontologies/demlab.owl#StressData -->

    <owl:Class rdf:about="&demlab;StressData">
        <rdfs:subClassOf rdf:resource="&demlab;MeasuredData"/>
        <rdfs:subClassOf>
            <owl:Restriction>
                <owl:onProperty rdf:resource="&demlab;stressLevel"/>
                <owl:cardinality rdf:datatype="&xsd;nonNegativeInteger">1</owl:cardinality>
            </owl:Restriction>
        </rdfs:subClassOf>
        <rdfs:comment xml:lang="en">Explore stress level</rdfs:comment>
    </owl:Class>
    


    <!-- http://www.demcare.eu/ontologies/demlab.owl#Task -->

    <owl:Class rdf:about="&demlab;Task">
        <rdfs:subClassOf>
            <owl:Restriction>
                <owl:onProperty rdf:resource="http://www.w3.org/2006/time#hasBeginning"/>
                <owl:onClass rdf:resource="http://www.w3.org/2006/time#Instant"/>
                <owl:qualifiedCardinality rdf:datatype="&xsd;nonNegativeInteger">1</owl:qualifiedCardinality>
            </owl:Restriction>
        </rdfs:subClassOf>
        <rdfs:subClassOf>
            <owl:Restriction>
                <owl:onProperty rdf:resource="&demlab;measuredData"/>
                <owl:someValuesFrom rdf:resource="&demlab;MeasuredData"/>
            </owl:Restriction>
        </rdfs:subClassOf>
        <rdfs:subClassOf>
            <owl:Restriction>
                <owl:onProperty rdf:resource="http://www.w3.org/2006/time#hasEnd"/>
                <owl:onClass rdf:resource="http://www.w3.org/2006/time#Instant"/>
                <owl:qualifiedCardinality rdf:datatype="&xsd;nonNegativeInteger">1</owl:qualifiedCardinality>
            </owl:Restriction>
        </rdfs:subClassOf>
        <rdfs:comment></rdfs:comment>
        <rdfs:comment xml:lang="en">Each Task involves the collection of one or more measurements (MeasuredData instances).</rdfs:comment>
    </owl:Class>
    


    <!-- http://www.demcare.eu/ontologies/demlab.owl#TurnOnTVTask -->

    <owl:Class rdf:about="&demlab;TurnOnTVTask">
        <rdfs:subClassOf rdf:resource="&demlab;SemiDirectedTask"/>
        <rdfs:comment xml:lang="en">The TV is turn off. The participant has to take the remote control and turns on the TV</rdfs:comment>
    </owl:Class>
    


    <!-- http://www.demcare.eu/ontologies/demlab.owl#VoiceData -->

    <owl:Class rdf:about="&demlab;VoiceData">
        <rdfs:subClassOf rdf:resource="&demlab;MeasuredData"/>
        <rdfs:subClassOf>
            <owl:Restriction>
                <owl:onProperty rdf:resource="&demlab;articulation"/>
                <owl:cardinality rdf:datatype="&xsd;nonNegativeInteger">1</owl:cardinality>
            </owl:Restriction>
        </rdfs:subClassOf>
        <rdfs:subClassOf>
            <owl:Restriction>
                <owl:onProperty rdf:resource="&demlab;speechFluency"/>
                <owl:cardinality rdf:datatype="&xsd;nonNegativeInteger">1</owl:cardinality>
            </owl:Restriction>
        </rdfs:subClassOf>
        <rdfs:subClassOf>
            <owl:Restriction>
                <owl:onProperty rdf:resource="&demlab;vowelDuration"/>
                <owl:cardinality rdf:datatype="&xsd;nonNegativeInteger">1</owl:cardinality>
            </owl:Restriction>
        </rdfs:subClassOf>
        <rdfs:subClassOf>
            <owl:Restriction>
                <owl:onProperty rdf:resource="&demlab;verbalReactionTime"/>
                <owl:cardinality rdf:datatype="&xsd;nonNegativeInteger">1</owl:cardinality>
            </owl:Restriction>
        </rdfs:subClassOf>
        <rdfs:subClassOf>
            <owl:Restriction>
                <owl:onProperty rdf:resource="&demlab;pauseRate"/>
                <owl:cardinality rdf:datatype="&xsd;nonNegativeInteger">1</owl:cardinality>
            </owl:Restriction>
        </rdfs:subClassOf>
        <rdfs:subClassOf>
            <owl:Restriction>
                <owl:onProperty rdf:resource="&demlab;speechRate"/>
                <owl:cardinality rdf:datatype="&xsd;nonNegativeInteger">1</owl:cardinality>
            </owl:Restriction>
        </rdfs:subClassOf>
        <rdfs:comment xml:lang="en">- Vocal biomarkers extraction for cognitive load assessment
- Assessment of mutual influence of cognitive activities an motor activities
- Assessment of the verbal reaction time and the impact of cognitive load imposed by the sentence recall task on speech fluency
- Assessment of the level of the participants’ control over the neuromuscular mechanism of speech production</rdfs:comment>
    </owl:Class>
    


    <!-- http://www.demcare.eu/ontologies/demlab.owl#WalkingCountingBackwardsTask -->

    <owl:Class rdf:about="&demlab;WalkingCountingBackwardsTask">
        <rdfs:subClassOf rdf:resource="&demlab;DirectedTask"/>
        <rdfs:subClassOf>
            <owl:Restriction>
                <owl:onProperty rdf:resource="&demlab;measuredData"/>
                <owl:allValuesFrom>
                    <owl:Class>
                        <owl:unionOf rdf:parseType="Collection">
                            <rdf:Description rdf:about="&demlab;GaitData"/>
                            <rdf:Description rdf:about="&demlab;LatencyData"/>
                            <rdf:Description rdf:about="&demlab;StressData"/>
                            <rdf:Description rdf:about="&demlab;VoiceData"/>
                        </owl:unionOf>
                    </owl:Class>
                </owl:allValuesFrom>
            </owl:Restriction>
        </rdfs:subClassOf>
        <rdfs:comment xml:lang="en">(DualTask) The clinician asks the participant to walk and count aloud backwards simultaneously: 
- From 305 until the end of the walking tasks; or 
- From 20 to 0 for participants who don’t manage to count backwards from 305 to 285 during the CountingBackwardsTask

This task is used for assessing:
- Gait: walking speed, step length, etc.
- Latency: time of latency between the end of instructions (stimulation) and the beginning of the task
- Stress level
- Voice: e.g. speech fluency and articulation</rdfs:comment>
    </owl:Class>
    


    <!-- http://www.demcare.eu/ontologies/demlab.owl#WalkingTask -->

    <owl:Class rdf:about="&demlab;WalkingTask">
        <rdfs:subClassOf rdf:resource="&demlab;DirectedTask"/>
        <rdfs:subClassOf>
            <owl:Restriction>
                <owl:onProperty rdf:resource="&demlab;measuredData"/>
                <owl:someValuesFrom rdf:resource="&demlab;LatencyData"/>
            </owl:Restriction>
        </rdfs:subClassOf>
        <rdfs:subClassOf>
            <owl:Restriction>
                <owl:onProperty rdf:resource="&demlab;measuredData"/>
                <owl:someValuesFrom rdf:resource="&demlab;GaitData"/>
            </owl:Restriction>
        </rdfs:subClassOf>
        <rdfs:subClassOf>
            <owl:Restriction>
                <owl:onProperty rdf:resource="&demlab;measuredData"/>
                <owl:allValuesFrom>
                    <owl:Class>
                        <owl:unionOf rdf:parseType="Collection">
                            <rdf:Description rdf:about="&demlab;GaitData"/>
                            <rdf:Description rdf:about="&demlab;LatencyData"/>
                            <rdf:Description rdf:about="&demlab;StressData"/>
                        </owl:unionOf>
                    </owl:Class>
                </owl:allValuesFrom>
            </owl:Restriction>
        </rdfs:subClassOf>
        <rdfs:comment xml:lang="en">(MonoTask) The clinician asks the participant to walk 4 meters across the room, to turn and then to come back (total walking distance: 8m).

This task is used for assessing:
- Gait: walking speed, step length, etc.
- Latency: time of latency between the end of instructions (stimulation) and the beginning of the task
- Stress level</rdfs:comment>
    </owl:Class>
    


    <!-- http://www.demcare.eu/ontologies/demlab.owl#WaterPlantTask -->

    <owl:Class rdf:about="&demlab;WaterPlantTask">
        <rdfs:subClassOf rdf:resource="&demlab;SemiDirectedTask"/>
        <rdfs:comment xml:lang="en">The participant has to take the water can, and water the plant nearby.</rdfs:comment>
    </owl:Class>
    


    <!-- http://www.demcare.eu/ontologies/demlab.owl#Zone -->

    <owl:Class rdf:about="&demlab;Zone">
        <rdfs:comment xml:lang="en">Allows the definition of zones (areas) of interest, e.g. phone zone</rdfs:comment>
    </owl:Class>
    


    <!-- 
    ///////////////////////////////////////////////////////////////////////////////////////
    //
    // Individuals
    //
    ///////////////////////////////////////////////////////////////////////////////////////
     -->

    


    <!-- http://purl.org/dc/terms/Agent -->

    <owl:NamedIndividual rdf:about="&terms;Agent">
        <rdf:type rdf:resource="&terms;AgentClass"/>
    </owl:NamedIndividual>
    


    <!-- http://purl.org/dc/terms/DCMIType -->

    <owl:NamedIndividual rdf:about="&terms;DCMIType">
        <rdf:type rdf:resource="http://purl.org/dc/dcam/VocabularyEncodingScheme"/>
        <rdfs:label xml:lang="en">DCMI Type Vocabulary</rdfs:label>
        <terms:issued rdf:datatype="&xsd;date">2000-07-11</terms:issued>
        <terms:modified rdf:datatype="&xsd;date">2012-06-14</terms:modified>
        <rdfs:comment xml:lang="en">The set of classes specified by the DCMI Type Vocabulary, used to categorize the nature or genre of the resource.</rdfs:comment>
        <terms:hasVersion rdf:resource="http://dublincore.org/usage/terms/history/#DCMIType-005"/>
        <rdfs:seeAlso rdf:resource="http://purl.org/dc/dcmitype/"/>
        <rdfs:isDefinedBy rdf:resource="http://purl.org/dc/terms/"/>
    </owl:NamedIndividual>
    


    <!-- http://purl.org/dc/terms/DDC -->

    <owl:NamedIndividual rdf:about="&terms;DDC">
        <rdf:type rdf:resource="http://purl.org/dc/dcam/VocabularyEncodingScheme"/>
        <rdfs:label xml:lang="en">DDC</rdfs:label>
        <terms:issued rdf:datatype="&xsd;date">2000-07-11</terms:issued>
        <terms:modified rdf:datatype="&xsd;date">2008-01-14</terms:modified>
        <rdfs:comment xml:lang="en">The set of conceptual resources specified by the Dewey Decimal Classification.</rdfs:comment>
        <terms:hasVersion rdf:resource="http://dublincore.org/usage/terms/history/#DDC-003"/>
        <rdfs:isDefinedBy rdf:resource="http://purl.org/dc/terms/"/>
        <rdfs:seeAlso rdf:resource="http://www.oclc.org/dewey/"/>
    </owl:NamedIndividual>
    


    <!-- http://purl.org/dc/terms/IMT -->

    <owl:NamedIndividual rdf:about="&terms;IMT">
        <rdf:type rdf:resource="http://purl.org/dc/dcam/VocabularyEncodingScheme"/>
        <rdfs:label xml:lang="en">IMT</rdfs:label>
        <terms:issued rdf:datatype="&xsd;date">2000-07-11</terms:issued>
        <terms:modified rdf:datatype="&xsd;date">2008-01-14</terms:modified>
        <rdfs:comment xml:lang="en">The set of media types specified by the Internet Assigned Numbers Authority.</rdfs:comment>
        <terms:hasVersion rdf:resource="http://dublincore.org/usage/terms/history/#IMT-004"/>
        <rdfs:isDefinedBy rdf:resource="http://purl.org/dc/terms/"/>
        <rdfs:seeAlso rdf:resource="http://www.iana.org/assignments/media-types/"/>
    </owl:NamedIndividual>
    


    <!-- http://purl.org/dc/terms/LCC -->

    <owl:NamedIndividual rdf:about="&terms;LCC">
        <rdf:type rdf:resource="http://purl.org/dc/dcam/VocabularyEncodingScheme"/>
        <rdfs:label xml:lang="en">LCC</rdfs:label>
        <terms:issued rdf:datatype="&xsd;date">2000-07-11</terms:issued>
        <terms:modified rdf:datatype="&xsd;date">2008-01-14</terms:modified>
        <rdfs:comment xml:lang="en">The set of conceptual resources specified by the Library of Congress Classification.</rdfs:comment>
        <terms:hasVersion rdf:resource="http://dublincore.org/usage/terms/history/#LCC-003"/>
        <rdfs:seeAlso rdf:resource="http://lcweb.loc.gov/catdir/cpso/lcco/lcco.html"/>
        <rdfs:isDefinedBy rdf:resource="http://purl.org/dc/terms/"/>
    </owl:NamedIndividual>
    


    <!-- http://purl.org/dc/terms/LCSH -->

    <owl:NamedIndividual rdf:about="&terms;LCSH">
        <rdf:type rdf:resource="http://purl.org/dc/dcam/VocabularyEncodingScheme"/>
        <rdfs:label xml:lang="en">LCSH</rdfs:label>
        <terms:issued rdf:datatype="&xsd;date">2000-07-11</terms:issued>
        <terms:modified rdf:datatype="&xsd;date">2008-01-14</terms:modified>
        <rdfs:comment xml:lang="en">The set of labeled concepts specified by the Library of Congress Subject Headings.</rdfs:comment>
        <terms:hasVersion rdf:resource="http://dublincore.org/usage/terms/history/#LCSH-003"/>
        <rdfs:isDefinedBy rdf:resource="http://purl.org/dc/terms/"/>
    </owl:NamedIndividual>
    


    <!-- http://purl.org/dc/terms/MESH -->

    <owl:NamedIndividual rdf:about="&terms;MESH">
        <rdf:type rdf:resource="http://purl.org/dc/dcam/VocabularyEncodingScheme"/>
        <rdfs:label xml:lang="en">MeSH</rdfs:label>
        <terms:issued rdf:datatype="&xsd;date">2000-07-11</terms:issued>
        <terms:modified rdf:datatype="&xsd;date">2008-01-14</terms:modified>
        <rdfs:comment xml:lang="en">The set of labeled concepts specified by the Medical Subject Headings.</rdfs:comment>
        <terms:hasVersion rdf:resource="http://dublincore.org/usage/terms/history/#MESH-003"/>
        <rdfs:isDefinedBy rdf:resource="http://purl.org/dc/terms/"/>
        <rdfs:seeAlso rdf:resource="http://www.nlm.nih.gov/mesh/meshhome.html"/>
    </owl:NamedIndividual>
    


    <!-- http://purl.org/dc/terms/NLM -->

    <owl:NamedIndividual rdf:about="&terms;NLM">
        <rdf:type rdf:resource="http://purl.org/dc/dcam/VocabularyEncodingScheme"/>
        <rdfs:label xml:lang="en">NLM</rdfs:label>
        <terms:issued rdf:datatype="&xsd;date">2005-06-13</terms:issued>
        <terms:modified rdf:datatype="&xsd;date">2008-01-14</terms:modified>
        <rdfs:comment xml:lang="en">The set of conceptual resources specified by the National Library of Medicine Classification.</rdfs:comment>
        <terms:hasVersion rdf:resource="http://dublincore.org/usage/terms/history/#NLM-002"/>
        <rdfs:isDefinedBy rdf:resource="http://purl.org/dc/terms/"/>
        <rdfs:seeAlso rdf:resource="http://wwwcf.nlm.nih.gov/class/"/>
    </owl:NamedIndividual>
    


    <!-- http://purl.org/dc/terms/TGN -->

    <owl:NamedIndividual rdf:about="&terms;TGN">
        <rdf:type rdf:resource="http://purl.org/dc/dcam/VocabularyEncodingScheme"/>
        <rdfs:label xml:lang="en">TGN</rdfs:label>
        <terms:issued rdf:datatype="&xsd;date">2000-07-11</terms:issued>
        <terms:modified rdf:datatype="&xsd;date">2008-01-14</terms:modified>
        <rdfs:comment xml:lang="en">The set of places specified by the Getty Thesaurus of Geographic Names.</rdfs:comment>
        <terms:hasVersion rdf:resource="http://dublincore.org/usage/terms/history/#TGN-003"/>
        <rdfs:isDefinedBy rdf:resource="http://purl.org/dc/terms/"/>
        <rdfs:seeAlso rdf:resource="http://www.getty.edu/research/tools/vocabulary/tgn/index.html"/>
    </owl:NamedIndividual>
    


    <!-- http://purl.org/dc/terms/UDC -->

    <owl:NamedIndividual rdf:about="&terms;UDC">
        <rdf:type rdf:resource="http://purl.org/dc/dcam/VocabularyEncodingScheme"/>
        <rdfs:label xml:lang="en">UDC</rdfs:label>
        <terms:issued rdf:datatype="&xsd;date">2000-07-11</terms:issued>
        <terms:modified rdf:datatype="&xsd;date">2008-01-14</terms:modified>
        <rdfs:comment xml:lang="en">The set of conceptual resources specified by the Universal Decimal Classification.</rdfs:comment>
        <terms:hasVersion rdf:resource="http://dublincore.org/usage/terms/history/#UDC-003"/>
        <rdfs:isDefinedBy rdf:resource="http://purl.org/dc/terms/"/>
        <rdfs:seeAlso rdf:resource="http://www.udcc.org/"/>
    </owl:NamedIndividual>
    


    <!-- http://www.demcare.eu/ontologies/demlab.owl -->

    <owl:NamedIndividual rdf:about="http://www.demcare.eu/ontologies/demlab.owl"/>
    


    <!-- http://www.demcare.eu/ontologies/demlab.owl#completed -->

    <owl:NamedIndividual rdf:about="&demlab;completed">
        <rdf:type rdf:resource="&demlab;ActivityStatusType"/>
    </owl:NamedIndividual>
    


    <!-- http://www.demcare.eu/ontologies/demlab.owl#dementia -->

    <owl:NamedIndividual rdf:about="&demlab;dementia">
        <rdf:type rdf:resource="&demlab;DiagnosisType"/>
    </owl:NamedIndividual>
    


    <!-- http://www.demcare.eu/ontologies/demlab.owl#healthy -->

    <owl:NamedIndividual rdf:about="&demlab;healthy">
        <rdf:type rdf:resource="&demlab;DiagnosisType"/>
        <hasClinicalDiagnosis rdf:resource="&demlab;dementia"/>
    </owl:NamedIndividual>
    


    <!-- http://www.demcare.eu/ontologies/demlab.owl#incomplete -->

    <owl:NamedIndividual rdf:about="&demlab;incomplete">
        <rdf:type rdf:resource="&demlab;ActivityStatusType"/>
    </owl:NamedIndividual>
    


    <!-- http://www.demcare.eu/ontologies/demlab.owl#omitted -->

    <owl:NamedIndividual rdf:about="&demlab;omitted">
        <rdf:type rdf:resource="&demlab;ActivityStatusType"/>
    </owl:NamedIndividual>
    


    <!-- http://www.demcare.eu/ontologies/demlab.owl#predementia -->

    <owl:NamedIndividual rdf:about="&demlab;predementia">
        <rdf:type rdf:resource="&demlab;DiagnosisType"/>
    </owl:NamedIndividual>
    


    <!-- 
    ///////////////////////////////////////////////////////////////////////////////////////
    //
    // Annotations
    //
    ///////////////////////////////////////////////////////////////////////////////////////
     -->

    <rdf:Description rdf:about="http://purl.org/dc/terms/">
        <terms:modified rdf:datatype="&xsd;date">2012-06-14</terms:modified>
        <terms:title xml:lang="en">DCMI Metadata Terms - other</terms:title>
        <terms:publisher rdf:resource="http://purl.org/dc/aboutdcmi#DCMI"/>
    </rdf:Description>
</rdf:RDF>



<!-- Generated by the OWL API (version 3.4.2) http://owlapi.sourceforge.net -->

