<?xml version="1.0" encoding="utf-8"?>
<rdf:RDF xmlns:adms="http://www.w3.org/ns/adms#"
   xmlns:beverage="http://rdfs.co/bevon/beverage/"
   xmlns:bevon="http://rdfs.co/bevon/"
   xmlns:cc="http://creativecommons.org/ns#"
   xmlns:container="http://rdfs.co/bevon/container/"
   xmlns:dbpedia="http://dbpedia.org/ontology/"
   xmlns:dcam="http://purl.org/dc/dcam/"
   xmlns:dcterms="http://purl.org/dc/terms/"
   xmlns:foaf="http://xmlns.com/foaf/0.1/"
   xmlns:food="http://data.lirmm.fr/ontologies/food#"
   xmlns:fowl="http://www.w3.org/TR/2003/PR-owl-guide-20031209/food#"
   xmlns:gr="http://purl.org/goodrelations/v1#"
   xmlns:owl="http://www.w3.org/2002/07/owl#"
   xmlns:pto="http://www.productontology.org/id/"
   xmlns:rdf="http://www.w3.org/1999/02/22-rdf-syntax-ns#"
   xmlns:rdfs="http://www.w3.org/2000/01/rdf-schema#"
   xmlns:skos="http://www.w3.org/2004/02/skos/core#"
   xmlns:status="http://www.w3.org/2003/06/sw-vocab-status/ns#"
   xmlns:time="http://www.w3.org/2006/time#"
   xmlns:vann="http://purl.org/vocab/vann/"
   xmlns:voaf="http://purl.org/vocommons/voaf#"
   xmlns:whisky="http://purl.org/vocab/whisky/terms/"
   xmlns:wine="http://www.w3.org/TR/2003/PR-owl-guide-20031209/wine#"
   xmlns:xsd="http://www.w3.org/2001/XMLSchema#"
   xmlns:yago="http://dbpedia.org/class/yago/">
  <foaf:Person rdf:about="http://jayg.me/">
    <foaf:homepage rdf:resource="http://jayg.org/"/>
    <foaf:mbox_sha1sum>f03421e94730da58e8943d3a1d2c4c6b02898e14</foaf:mbox_sha1sum>
    <foaf:name xml:lang="en">James G. Kim</foaf:name>
    <foaf:name xml:lang="ko">김보람</foaf:name>
  </foaf:Person>
  <rdf:Description rdf:about="http://purl.org/vocab/whisky/terms/Distillery">
    <rdfs:subClassOf rdf:resource="http://rdfs.co/bevon/Distillery"/>
  </rdf:Description>
  <rdf:Description rdf:about="http://purl.org/vocab/whisky/terms/abv">
    <rdfs:subPropertyOf rdf:resource="http://rdfs.co/bevon/abv"/>
  </rdf:Description>
  <rdf:Description rdf:about="http://purl.org/vocab/whisky/terms/distillery">
    <rdfs:subPropertyOf rdf:resource="http://rdfs.co/bevon/distillery"/>
  </rdf:Description>
  <owl:Ontology rdf:about="http://rdfs.co/bevon/0.8">
    <cc:license rdf:resource="http://creativecommons.org/licenses/by/4.0/"/>
    <dcterms:creator rdf:resource="http://jayg.me/"/>
    <dcterms:description xml:lang="en">
    Beverage Ontology is a Web vocabulary for describing beverages, mainly
    alcoholic.
    </dcterms:description>
    <dcterms:hasFormat rdf:resource="http://rdfs.co/bevon/0.8/html"/>
    <dcterms:hasFormat rdf:resource="http://rdfs.co/bevon/0.8/rdf"/>
    <dcterms:hasFormat rdf:resource="http://rdfs.co/bevon/0.8/ttl"/>
    <dcterms:identifier>http://rdfs.co/bevon/0.8</dcterms:identifier>
    <dcterms:isVersionOf rdf:resource="http://rdfs.co/bevon/"/>
    <dcterms:issued rdf:datatype="http://www.w3.org/2001/XMLSchema#date">2013-07-04+09:00</dcterms:issued>
    <dcterms:modified rdf:datatype="http://www.w3.org/2001/XMLSchema#date">2015-10-07+09:00</dcterms:modified>
    <dcterms:publisher rdf:resource="http://jayg.me/"/>
    <dcterms:replaces rdf:resource="http://rdfs.co/bevon/0.7"/>
    <dcterms:rights>Copyright © 2013-2015 James G. Kim Some Rights Reserved.</dcterms:rights>
    <dcterms:title xml:lang="en">BEVON: Beverage Ontology</dcterms:title>
    <dcterms:type rdf:resource="http://purl.org/adms/assettype/Ontology"/>
    <vann:example>
      <rdf:Description>
        <rdfs:comment rdf:datatype="http://www.w3.org/1999/02/22-rdf-syntax-ns#HTML">
    &lt;pre&gt;&lt;code&gt;beverage:Glenfiddich12YearOld
  a owl:NamedIndividual, bevon:SpeysideSingleMalt , gr:ProductOrServiceModel ;
  bevon:name "Glenfiddich 12 Year Old"@en , "글렌피딕 12년"@ko ;
  bevon:description """
    Carefully matured in the finest American bourbon and Spanish sherry oak
    casks for at least 12 years. Married and mellowed in oak marrying tuns for
    complete harmony of aroma and flavor.

    A single malt Scotch whisky with distinctive fresh pear, creamy with subtle
    oak flavors and a long smooth and mellow finish.
    """@en ;
  bevon:origin &amp;lt;http://dbpedia.org/resource/Strathspey,_Scotland&amp;gt; ;
  bevon:launch "1887"^^xsd:gYear ;
  bevon:distillery [
    a bevon:Distillery ;
    owl:sameAs &amp;lt;http://dbpedia.org/resource/Glenfiddich_distillery&amp;gt; ;
    whisky:region &amp;lt;http://dbpedia.org/resource/Strathspey,_Scotland&amp;gt; ;
    whisky:owner &amp;lt;http://dbpedia.org/resource/William_Grant_%26_Sons&amp;gt; ;
    whisky:waterSource [
      a whisky:WaterSource ;
      dcterms:title "Robbie Dhu Springs"@en , "로비 듀 수원지"@ko
    ]
  ] ;
  bevon:manufacturer &amp;lt;http://dbpedia.org/resource/William_Grant_%26_Sons&amp;gt; ;
  bevon:fermentation_base &amp;lt;http://dbpedia.org/resource/Barley&amp;gt; ;
  bevon:aging [
    a bevon:Aging ;
    bevon:material &amp;lt;http://dbpedia.org/resource/Oak&amp;gt; ;
    bevon:previous_content
      &amp;lt;http://dbpedia.org/resource/Bourbon_whiskey&amp;gt; ,
      &amp;lt;http://dbpedia.org/resource/Sherry&amp;gt; ;
    bevon:duration [
      a time:DurationDescription ;
      time:years "12"^^xsd:decimal
    ]
  ] ;
  bevon:color [
    a dbpedia:Colour ;
    owl:sameAs &amp;lt;http://dbpedia.org/resource/Gold_(color)&amp;gt; ;
    owl:sameAs &amp;lt;http://purl.org/colors/rgb/FFD700&amp;gt; ;
    dcterms:title "Gold"@en
  ] ;
  bevon:abv "40"^^xsd:decimal ;
  bevon:container container:700mlGlassBottle .

container:700mlGlassBottle a owl:NamedIndividual, bevon:GlassBottle ;
  skos:prefLabel "700ml Glass Bottle"@en , "700ml 유리병"@ko ;
  skos:altLabel "70cl Glass Bottle"@en ;
  bevon:volume [
    a gr:QuantitativeValueInteger ;
    gr:hasUnitOfMeasurement "MLT" ;
    gr:hasValue "700"^^xsd:int
  ] .&lt;/code&gt;&lt;/pre&gt;
    </rdfs:comment>
        <rdfs:label xml:lang="en">Glenfiddich 12 Year Old</rdfs:label>
      </rdf:Description>
    </vann:example>
    <vann:example>
      <rdf:Description>
        <rdfs:comment rdf:datatype="http://www.w3.org/1999/02/22-rdf-syntax-ns#HTML">
    &lt;pre&gt;&lt;code&gt;beverage:WhiskyAndSoda
  a owl:NamedIndividual, bevon:Highball , gr:ProductOrServiceModel ;
  bevon:name "Whisky &amp;amp; Soda"@en , "위스키 소다"@ko ;
  bevon:description """
    Whisky &amp;amp; Soda is a kind of mixed drinks that are composed of whisky and
    carbonated water.
    """@en ;
  bevon:ingredient [
    a food:Ingredient ;
    bevon:food [
      a bevon:Whisky ;
      owl:sameAs &amp;lt;http://dbpedia.org/resource/Whisky&amp;gt; ;
      dcterms:title "Whisky"@en
    ] ;
    bevon:quantity [
      a gr:QuantitativeValueInteger ;
      gr:hasUnitOfMeasurement "OZA" ;
      gr:hasValue "2"^^xsd:int
    ]
  ] , [
    a food:Ingredient ;
    bevon:food [
      a bevon:CarbonatedWater ;
      owl:sameAs &amp;lt;http://dbpedia.org/resource/Carbonated_water&amp;gt; ;
      dcterms:title "Carbonated Water"@en
    ]
  ] .&lt;/code&gt;&lt;/pre&gt;
    </rdfs:comment>
        <rdfs:label xml:lang="en">Whisky &amp; Soda</rdfs:label>
      </rdf:Description>
    </vann:example>
    <vann:preferredNamespacePrefix>bevon</vann:preferredNamespacePrefix>
    <vann:preferredNamespaceUri>http://rdfs.co/bevon/</vann:preferredNamespaceUri>
    <vann:termGroup rdf:resource="http://rdfs.co/bevon/BeerGroup"/>
    <vann:termGroup rdf:resource="http://rdfs.co/bevon/CocktailGroup"/>
    <vann:termGroup rdf:resource="http://rdfs.co/bevon/ContainerGroup"/>
    <vann:termGroup rdf:resource="http://rdfs.co/bevon/CoreGroup"/>
    <vann:termGroup rdf:resource="http://rdfs.co/bevon/RelationGroup"/>
    <vann:termGroup rdf:resource="http://rdfs.co/bevon/WhiskyGroup"/>
    <vann:termGroup rdf:resource="http://rdfs.co/bevon/WineGroup"/>
    <rdf:type rdf:resource="http://creativecommons.org/ns#Work"/>
    <rdf:type rdf:resource="http://purl.org/vocommons/voaf#Vocabulary"/>
    <rdf:type rdf:resource="http://www.w3.org/ns/adms#SemanticAsset"/>
    <rdfs:comment rdf:datatype="http://www.w3.org/1999/02/22-rdf-syntax-ns#HTML">
    &lt;div&gt;
      The master version of this vocabulary is maintained in &lt;a
      href="https://github.com/jgkim/bevon"&gt;the GitHub repository&lt;/a&gt; so others
      can contribute edits and improvements.
    &lt;/div&gt;
    </rdfs:comment>
    <rdfs:comment xml:lang="en">
    Most of the descriptions given here are from Wikipedia or from the websites
    of the related products.
    </rdfs:comment>
    <rdfs:seeAlso rdf:resource="https://github.com/jgkim/bevon"/>
    <owl:versionInfo>0.8</owl:versionInfo>
    <skos:changeNote>
      <rdf:Description>
        <dcterms:creator rdf:resource="http://jayg.me/"/>
        <dcterms:date rdf:datatype="http://www.w3.org/2001/XMLSchema#date">2014-03-01+09:00</dcterms:date>
        <rdf:value xml:lang="en">
      Minor revisions for documentation
      </rdf:value>
      </rdf:Description>
    </skos:changeNote>
    <skos:changeNote>
      <rdf:Description>
        <dcterms:creator rdf:resource="http://jayg.me/"/>
        <dcterms:date rdf:datatype="http://www.w3.org/2001/XMLSchema#date">2014-03-03+09:00</dcterms:date>
        <rdf:value xml:lang="en">
      Added a link to the GitHub repository
      </rdf:value>
      </rdf:Description>
    </skos:changeNote>
    <skos:changeNote>
      <rdf:Description>
        <dcterms:creator rdf:resource="http://jayg.me/"/>
        <dcterms:date rdf:datatype="http://www.w3.org/2001/XMLSchema#date">2014-03-06+09:00</dcterms:date>
        <rdf:value xml:lang="en">
      Added term groups for core, relation, container, beer, whisky and
      cocktail terms
      </rdf:value>
      </rdf:Description>
    </skos:changeNote>
    <skos:changeNote>
      <rdf:Description>
        <dcterms:creator rdf:resource="http://jayg.me/"/>
        <dcterms:date rdf:datatype="http://www.w3.org/2001/XMLSchema#date">2015-07-27+09:00</dcterms:date>
        <rdf:value xml:lang="en">
      Made the vocabulary as a type of voaf:Vocabulary
      </rdf:value>
      </rdf:Description>
    </skos:changeNote>
    <skos:changeNote>
      <rdf:Description>
        <dcterms:creator rdf:resource="http://jayg.me/"/>
        <dcterms:date rdf:datatype="http://www.w3.org/2001/XMLSchema#date">2015-10-07+09:00</dcterms:date>
        <rdf:value xml:lang="en">
      Fixed the wrong use of rdf:XMLLiteral
      </rdf:value>
      </rdf:Description>
    </skos:changeNote>
    <skos:historyNote>
      <rdf:Description>
        <dcterms:creator rdf:resource="http://jayg.me/"/>
        <dcterms:date rdf:datatype="http://www.w3.org/2001/XMLSchema#date">2014-03-06+09:00</dcterms:date>
        <rdf:value xml:lang="en">
      Changed bevon:FermentedBeverages to bevon:FermentedBeverage for the
      consistency
      </rdf:value>
      </rdf:Description>
    </skos:historyNote>
    <skos:historyNote>
      <rdf:Description>
        <dcterms:creator rdf:resource="http://jayg.me/"/>
        <dcterms:date rdf:datatype="http://www.w3.org/2001/XMLSchema#date">2014-03-07+09:00</dcterms:date>
        <rdf:value xml:lang="en">
      Changed the semantics of bevon:Wine to be a superclass of wine:Wine
      </rdf:value>
      </rdf:Description>
    </skos:historyNote>
    <skos:historyNote>
      <rdf:Description>
        <dcterms:creator rdf:resource="http://jayg.me/"/>
        <dcterms:date rdf:datatype="http://www.w3.org/2001/XMLSchema#date">2014-03-07+09:00</dcterms:date>
        <rdf:value xml:lang="en">
      Added bevon:RedWine, bevon:WhiteWine and bevon:FruitWine
      </rdf:value>
      </rdf:Description>
    </skos:historyNote>
    <skos:historyNote>
      <rdf:Description>
        <dcterms:creator rdf:resource="http://jayg.me/"/>
        <dcterms:date rdf:datatype="http://www.w3.org/2001/XMLSchema#date">2015-07-23+09:00</dcterms:date>
        <rdf:value xml:lang="en">
      Fixed the sameAs relationship of bevon:Whisky
      </rdf:value>
      </rdf:Description>
    </skos:historyNote>
    <adms:status rdf:resource="http://purl.org/adms/status/UnderDevelopment"/>
  </owl:Ontology>
  <rdf:Description rdf:about="http://rdfs.co/bevon/0.8/html">
    <dcterms:format>
      <dcterms:MediaType>
        <dcam:memberOf rdf:resource="http://purl.org/dc/terms/IMT"/>
        <rdf:value>text/html</rdf:value>
        <rdfs:label xml:lang="en">HTML</rdfs:label>
        <rdfs:seeAlso rdf:resource="http://www.iana.org/assignments/media-types/text/html"/>
      </dcterms:MediaType>
    </dcterms:format>
  </rdf:Description>
  <rdf:Description rdf:about="http://rdfs.co/bevon/0.8/rdf">
    <dcterms:format>
      <dcterms:MediaType>
        <dcam:memberOf rdf:resource="http://purl.org/dc/terms/IMT"/>
        <rdf:value>application/rdf+xml</rdf:value>
        <rdfs:label xml:lang="en">RDF/XML</rdfs:label>
        <rdfs:seeAlso rdf:resource="http://www.iana.org/assignments/media-types/application/rdf+xml"/>
      </dcterms:MediaType>
    </dcterms:format>
  </rdf:Description>
  <rdf:Description rdf:about="http://rdfs.co/bevon/0.8/ttl">
    <dcterms:format>
      <dcterms:MediaType>
        <dcam:memberOf rdf:resource="http://purl.org/dc/terms/IMT"/>
        <rdf:value>text/turtle</rdf:value>
        <rdfs:label xml:lang="en">Turtle</rdfs:label>
        <rdfs:seeAlso rdf:resource="http://www.iana.org/assignments/media-types/text/turtle"/>
      </dcterms:MediaType>
    </dcterms:format>
  </rdf:Description>
  <owl:Class rdf:about="http://rdfs.co/bevon/Aging">
    <dcterms:issued rdf:datatype="http://www.w3.org/2001/XMLSchema#date">2013-07-04+09:00</dcterms:issued>
    <dcterms:modified rdf:datatype="http://www.w3.org/2001/XMLSchema#date">2014-03-01+09:00</dcterms:modified>
    <rdfs:isDefinedBy rdf:resource="http://rdfs.co/bevon/"/>
    <status:term_status xml:lang="en">unstable</status:term_status>
    <skos:definition xml:lang="en">
    Aging is the process of storing beverages in casks for a specific period of
    time to remove harsh flavors and add distinct characteristics found in the
    cask's wood.
    </skos:definition>
    <skos:prefLabel xml:lang="en">Aging</skos:prefLabel>
    <skos:prefLabel xml:lang="ko">숙성</skos:prefLabel>
  </owl:Class>
  <owl:Class rdf:about="http://rdfs.co/bevon/AlcoholicBeverage">
    <dcterms:issued rdf:datatype="http://www.w3.org/2001/XMLSchema#date">2013-07-04+09:00</dcterms:issued>
    <dcterms:modified rdf:datatype="http://www.w3.org/2001/XMLSchema#date">2014-03-01+09:00</dcterms:modified>
    <rdfs:isDefinedBy rdf:resource="http://rdfs.co/bevon/"/>
    <rdfs:seeAlso rdf:resource="http://en.wikipedia.org/wiki/Alcoholic_beverage"/>
    <rdfs:subClassOf rdf:resource="http://rdfs.co/bevon/Beverage"/>
    <rdfs:subClassOf rdf:resource="http://www.productontology.org/id/Alcoholic_beverage"/>
    <owl:disjointWith rdf:resource="http://rdfs.co/bevon/NonAlcoholicBeverage"/>
    <status:term_status xml:lang="en">testing</status:term_status>
    <skos:definition xml:lang="en">
     An alcoholic beverage is a drink and psychoactive drug containing
     ethyl alcohol which is commonly referred to as ethanol.
     </skos:definition>
    <skos:prefLabel xml:lang="en">Alcoholic Beverage</skos:prefLabel>
    <skos:prefLabel xml:lang="ko">알코올 음료</skos:prefLabel>
  </owl:Class>
  <owl:Class rdf:about="http://rdfs.co/bevon/Ale">
    <dcterms:issued rdf:datatype="http://www.w3.org/2001/XMLSchema#date">2013-07-04+09:00</dcterms:issued>
    <dcterms:modified rdf:datatype="http://www.w3.org/2001/XMLSchema#date">2014-03-01+09:00</dcterms:modified>
    <rdfs:comment xml:lang="en">
    The yeast will ferment the beer quickly, giving it a sweet, full bodied and
    fruity taste.
    </rdfs:comment>
    <rdfs:isDefinedBy rdf:resource="http://rdfs.co/bevon/"/>
    <rdfs:seeAlso rdf:resource="http://en.wikipedia.org/wiki/Ale"/>
    <rdfs:subClassOf rdf:resource="http://rdfs.co/bevon/Beer"/>
    <rdfs:subClassOf rdf:resource="http://www.productontology.org/id/Ale"/>
    <status:term_status xml:lang="en">unstable</status:term_status>
    <skos:definition xml:lang="en">
    Ale is a type of beer brewed from malted barley using a warm-fermentation
    with a strain of brewers' yeast.
    </skos:definition>
    <skos:prefLabel xml:lang="en">Ale</skos:prefLabel>
    <skos:prefLabel xml:lang="ko">에일</skos:prefLabel>
  </owl:Class>
  <owl:Class rdf:about="http://rdfs.co/bevon/AmericanWhiskey">
    <dcterms:issued rdf:datatype="http://www.w3.org/2001/XMLSchema#date">2013-07-04+09:00</dcterms:issued>
    <dcterms:modified rdf:datatype="http://www.w3.org/2001/XMLSchema#date">2014-03-01+09:00</dcterms:modified>
    <rdfs:comment xml:lang="en">
    The production and labeling of American whiskey are governed by Title 27 of
    the U.S. Code of Federal Regulations.
    </rdfs:comment>
    <rdfs:isDefinedBy rdf:resource="http://rdfs.co/bevon/"/>
    <rdfs:seeAlso rdf:resource="http://en.wikipedia.org/wiki/American_whiskey"/>
    <rdfs:subClassOf rdf:resource="http://rdfs.co/bevon/Whisky"/>
    <rdfs:subClassOf rdf:resource="http://www.productontology.org/id/American_whiskey"/>
    <status:term_status xml:lang="en">unstable</status:term_status>
    <skos:altLabel xml:lang="en">American Whisky</skos:altLabel>
    <skos:definition xml:lang="en">
    American whiskey is a distilled beverage produced in the United States from
    a fermented mash of cereal grain.
    </skos:definition>
    <skos:prefLabel xml:lang="en">American Whiskey</skos:prefLabel>
    <skos:prefLabel xml:lang="ko">아메리칸 위스키</skos:prefLabel>
  </owl:Class>
  <owl:Class rdf:about="http://rdfs.co/bevon/Beer">
    <dcterms:issued rdf:datatype="http://www.w3.org/2001/XMLSchema#date">2013-07-04+09:00</dcterms:issued>
    <dcterms:modified rdf:datatype="http://www.w3.org/2001/XMLSchema#date">2014-03-01+09:00</dcterms:modified>
    <rdfs:comment xml:lang="en">
    The starch and saccharification enzymes are often derived from malted
    cereal grains, most commonly malted barley and malted wheat.
    </rdfs:comment>
    <rdfs:isDefinedBy rdf:resource="http://rdfs.co/bevon/"/>
    <rdfs:seeAlso rdf:resource="http://en.wikipedia.org/wiki/Beer"/>
    <rdfs:subClassOf rdf:resource="http://rdfs.co/bevon/FermentedBeverage"/>
    <rdfs:subClassOf rdf:resource="http://www.productontology.org/id/Beer"/>
    <owl:disjointWith rdf:resource="http://rdfs.co/bevon/NonAlcoholicBeer"/>
    <status:term_status xml:lang="en">testing</status:term_status>
    <skos:definition xml:lang="en">
    Beer is an alcoholic beverage produced by the saccharification of starch
    and fermentation of the resulting sugar.
    </skos:definition>
    <skos:prefLabel xml:lang="en">Beer</skos:prefLabel>
    <skos:prefLabel xml:lang="ko">맥주</skos:prefLabel>
  </owl:Class>
  <owl:Class rdf:about="http://rdfs.co/bevon/BeerBottle">
    <dcterms:issued rdf:datatype="http://www.w3.org/2001/XMLSchema#date">2013-07-04+09:00</dcterms:issued>
    <dcterms:modified rdf:datatype="http://www.w3.org/2001/XMLSchema#date">2014-03-01+09:00</dcterms:modified>
    <rdfs:comment xml:lang="en">
    Dark amber or brown glass greatly reduces UV light from spoiling the beer.
    However, lighter colored bottles are often used for marketing reasons.
    </rdfs:comment>
    <rdfs:isDefinedBy rdf:resource="http://rdfs.co/bevon/"/>
    <rdfs:seeAlso rdf:resource="http://en.wikipedia.org/wiki/Beer_bottle"/>
    <rdfs:subClassOf rdf:resource="http://rdfs.co/bevon/GlassBottle"/>
    <status:term_status xml:lang="en">unstable</status:term_status>
    <skos:definition xml:lang="en">
    A beer bottle is a bottle made to contain beer, usually made of glass and
    come in various sizes, shapes and colors.
    </skos:definition>
    <skos:prefLabel xml:lang="en">Beer Bottle</skos:prefLabel>
    <skos:prefLabel xml:lang="ko">맥주병</skos:prefLabel>
  </owl:Class>
  <owl:Class rdf:about="http://rdfs.co/bevon/BeerCocktail">
    <dcterms:issued rdf:datatype="http://www.w3.org/2001/XMLSchema#date">2013-07-04+09:00</dcterms:issued>
    <dcterms:modified rdf:datatype="http://www.w3.org/2001/XMLSchema#date">2014-03-01+09:00</dcterms:modified>
    <rdfs:isDefinedBy rdf:resource="http://rdfs.co/bevon/"/>
    <rdfs:seeAlso rdf:resource="http://en.wikipedia.org/wiki/Beer_cocktail"/>
    <rdfs:subClassOf rdf:resource="http://rdfs.co/bevon/Cocktail"/>
    <rdfs:subClassOf rdf:resource="http://www.productontology.org/id/Beer_cocktail"/>
    <status:term_status xml:lang="en">unstable</status:term_status>
    <skos:definition xml:lang="en">
    A beer cocktail is a cocktail that is made by mixing beer with a distilled
    beverage. In this type of cocktail, the primary ingredient is beer.
    </skos:definition>
    <skos:prefLabel xml:lang="en">Beer Cocktail</skos:prefLabel>
    <skos:prefLabel xml:lang="ko">맥주 칵테일</skos:prefLabel>
  </owl:Class>
  <rdf:Bag rdf:about="http://rdfs.co/bevon/BeerGroup">
    <rdf:_1 rdf:resource="http://rdfs.co/bevon/Beer"/>
    <rdf:_10 rdf:resource="http://rdfs.co/bevon/PaleLager"/>
    <rdf:_11 rdf:resource="http://rdfs.co/bevon/Pilsner"/>
    <rdf:_12 rdf:resource="http://rdfs.co/bevon/NonAlcoholicBeer"/>
    <rdf:_13 rdf:resource="http://rdfs.co/bevon/Brewery"/>
    <rdf:_14 rdf:resource="http://rdfs.co/bevon/BeerBottle"/>
    <rdf:_15 rdf:resource="http://rdfs.co/bevon/Longneck"/>
    <rdf:_16 rdf:resource="http://rdfs.co/bevon/BeerKeg"/>
    <rdf:_17 rdf:resource="http://rdfs.co/bevon/ibu"/>
    <rdf:_18 rdf:resource="http://rdfs.co/bevon/srm"/>
    <rdf:_19 rdf:resource="http://rdfs.co/bevon/brewery"/>
    <rdf:_2 rdf:resource="http://rdfs.co/bevon/Ale"/>
    <rdf:_3 rdf:resource="http://rdfs.co/bevon/PaleAle"/>
    <rdf:_4 rdf:resource="http://rdfs.co/bevon/IrishRedAle"/>
    <rdf:_5 rdf:resource="http://rdfs.co/bevon/Porter"/>
    <rdf:_6 rdf:resource="http://rdfs.co/bevon/Stout"/>
    <rdf:_7 rdf:resource="http://rdfs.co/bevon/DryStout"/>
    <rdf:_8 rdf:resource="http://rdfs.co/bevon/Lager"/>
    <rdf:_9 rdf:resource="http://rdfs.co/bevon/Dunkel"/>
    <rdfs:comment xml:lang="en">
    In addition to the BEVON core terms, there are a number of terms for use
    when describing beverages categorized under Beer.
    </rdfs:comment>
    <rdfs:label xml:lang="en">Beer Terms</rdfs:label>
  </rdf:Bag>
  <owl:Class rdf:about="http://rdfs.co/bevon/BeerKeg">
    <dcterms:issued rdf:datatype="http://www.w3.org/2001/XMLSchema#date">2013-07-04+09:00</dcterms:issued>
    <dcterms:modified rdf:datatype="http://www.w3.org/2001/XMLSchema#date">2014-03-01+09:00</dcterms:modified>
    <rdfs:isDefinedBy rdf:resource="http://rdfs.co/bevon/"/>
    <rdfs:subClassOf rdf:resource="http://rdfs.co/bevon/Keg"/>
    <status:term_status xml:lang="en">unstable</status:term_status>
    <skos:definition xml:lang="en">
    Beer kegs are made of stainless steel, or less commonly, of aluminium.
    </skos:definition>
    <skos:prefLabel xml:lang="en">Beer Keg</skos:prefLabel>
    <skos:prefLabel xml:lang="ko">맥주 케그</skos:prefLabel>
  </owl:Class>
  <owl:Class rdf:about="http://rdfs.co/bevon/Beverage">
    <dcterms:issued rdf:datatype="http://www.w3.org/2001/XMLSchema#date">2013-07-04+09:00</dcterms:issued>
    <dcterms:modified rdf:datatype="http://www.w3.org/2001/XMLSchema#date">2014-03-01+09:00</dcterms:modified>
    <rdfs:isDefinedBy rdf:resource="http://rdfs.co/bevon/"/>
    <rdfs:seeAlso rdf:resource="http://en.wikipedia.org/wiki/Beverage"/>
    <rdfs:subClassOf rdf:resource="http://data.lirmm.fr/ontologies/food#Food"/>
    <rdfs:subClassOf rdf:resource="http://www.productontology.org/id/Drink"/>
    <rdfs:subClassOf rdf:resource="http://www.w3.org/TR/2003/PR-owl-guide-20031209/food#PotableLiquid"/>
    <status:term_status xml:lang="en">testing</status:term_status>
    <skos:altLabel xml:lang="en">Drink</skos:altLabel>
    <skos:definition xml:lang="en">
    A beverage, or drink, is a kind of liquid which is specifically prepared
    for human consumption.
    </skos:definition>
    <skos:prefLabel xml:lang="en">Beverage</skos:prefLabel>
    <skos:prefLabel xml:lang="ko">음료</skos:prefLabel>
  </owl:Class>
  <owl:Class rdf:about="http://rdfs.co/bevon/BeverageCan">
    <dcterms:issued rdf:datatype="http://www.w3.org/2001/XMLSchema#date">2013-07-04+09:00</dcterms:issued>
    <dcterms:modified rdf:datatype="http://www.w3.org/2001/XMLSchema#date">2014-03-01+09:00</dcterms:modified>
    <rdfs:comment xml:lang="en">
    Beverage cans are made of aluminium (75% of worldwide production) or
    tin-plated steel (25% worldwide production).
    </rdfs:comment>
    <rdfs:isDefinedBy rdf:resource="http://rdfs.co/bevon/"/>
    <rdfs:seeAlso rdf:resource="http://en.wikipedia.org/wiki/Beverage_can"/>
    <rdfs:subClassOf rdf:resource="http://rdfs.co/bevon/Container"/>
    <status:term_status xml:lang="en">unstable</status:term_status>
    <skos:definition xml:lang="en">
    A beverage can is a metal container designed to hold a fixed portion of
    liquid such as a carbonated soft drinks, alcoholic beverages, fruit juices,
    teas, tisanes, energy drinks, etc.
    </skos:definition>
    <skos:prefLabel xml:lang="en">Beverage Can</skos:prefLabel>
    <skos:prefLabel xml:lang="ko">음료 캔</skos:prefLabel>
  </owl:Class>
  <owl:Class rdf:about="http://rdfs.co/bevon/BourbonWhiskey">
    <dcterms:issued rdf:datatype="http://www.w3.org/2001/XMLSchema#date">2013-07-04+09:00</dcterms:issued>
    <dcterms:modified rdf:datatype="http://www.w3.org/2001/XMLSchema#date">2014-03-01+09:00</dcterms:modified>
    <rdfs:comment xml:lang="en">
    The name of the spirit derives from its historical association with an area
    known as Old Bourbon, around what is now Bourbon County, Kentucky (which,
    in turn, was named after the French House of Bourbon royal family). It has
    been produced since the 18th century. While it may be made anywhere in the
    United States, it is strongly associated with the American South in
    general, and Kentucky in particular.
    </rdfs:comment>
    <rdfs:isDefinedBy rdf:resource="http://rdfs.co/bevon/"/>
    <rdfs:seeAlso rdf:resource="http://en.wikipedia.org/wiki/Bourbon_whiskey"/>
    <rdfs:subClassOf rdf:resource="http://rdfs.co/bevon/AmericanWhisky"/>
    <rdfs:subClassOf rdf:resource="http://www.productontology.org/id/Bourbon_whiskey"/>
    <status:term_status xml:lang="en">unstable</status:term_status>
    <skos:altLabel xml:lang="en">Bourbon Whisky</skos:altLabel>
    <skos:definition xml:lang="en">
    Bourbon whiskey is a type of American whiskey – a barrel-aged distilled
    spirit made primarily from corn.
    </skos:definition>
    <skos:prefLabel xml:lang="en">Bourbon Whiskey</skos:prefLabel>
    <skos:prefLabel xml:lang="ko">버번 위스키</skos:prefLabel>
  </owl:Class>
  <owl:Class rdf:about="http://rdfs.co/bevon/Brandy">
    <dcterms:issued rdf:datatype="http://www.w3.org/2001/XMLSchema#date">2013-07-04+09:00</dcterms:issued>
    <dcterms:modified rdf:datatype="http://www.w3.org/2001/XMLSchema#date">2014-03-01+09:00</dcterms:modified>
    <rdfs:comment xml:lang="en">
    Brandy generally contains 35–60% alcohol by volume (70–120 US proof) and is
    typically taken as an after-dinner drink. Some brandies are aged in wooden
    casks, some are colored with caramel coloring to imitate the effect of
    aging, and some brandies are produced using a combination of both aging and
    coloring.
    </rdfs:comment>
    <rdfs:isDefinedBy rdf:resource="http://rdfs.co/bevon/"/>
    <rdfs:seeAlso rdf:resource="http://en.wikipedia.org/wiki/Brandy"/>
    <rdfs:subClassOf rdf:resource="http://rdfs.co/bevon/DistilledBeverage"/>
    <rdfs:subClassOf rdf:resource="http://www.productontology.org/id/Brandy"/>
    <status:term_status xml:lang="en">testing</status:term_status>
    <skos:definition xml:lang="en">
    Brandy (from brandywine, derived from Dutch brandewijn—"burnt wine") is a
    spirit produced by distilling wine.
    </skos:definition>
    <skos:prefLabel xml:lang="en">Brandy</skos:prefLabel>
    <skos:prefLabel xml:lang="ko">브랜디</skos:prefLabel>
  </owl:Class>
  <owl:Class rdf:about="http://rdfs.co/bevon/Brewery">
    <dcterms:issued rdf:datatype="http://www.w3.org/2001/XMLSchema#date">2013-07-04+09:00</dcterms:issued>
    <dcterms:modified rdf:datatype="http://www.w3.org/2001/XMLSchema#date">2014-03-01+09:00</dcterms:modified>
    <rdfs:comment xml:lang="en">
    A company that makes beer is called either a brewery or a brewing company.
    </rdfs:comment>
    <rdfs:isDefinedBy rdf:resource="http://rdfs.co/bevon/"/>
    <rdfs:seeAlso rdf:resource="http://en.wikipedia.org/wiki/Brewery"/>
    <status:term_status xml:lang="en">unstable</status:term_status>
    <skos:definition xml:lang="en">
    A brewery is a dedicated building for the making of beer, though beer can
    be made at home, and has been for much of beer's history.
    </skos:definition>
    <skos:prefLabel xml:lang="en">Brewery</skos:prefLabel>
    <skos:prefLabel xml:lang="ko">양조장</skos:prefLabel>
  </owl:Class>
  <owl:Class rdf:about="http://rdfs.co/bevon/CanadianWhisky">
    <dcterms:issued rdf:datatype="http://www.w3.org/2001/XMLSchema#date">2013-07-04+09:00</dcterms:issued>
    <dcterms:modified rdf:datatype="http://www.w3.org/2001/XMLSchema#date">2014-03-01+09:00</dcterms:modified>
    <rdfs:comment xml:lang="en">
    Most Canadian whiskies are blended multi-grain liquors containing a large
    percentage of corn spirits, and are typically lighter and smoother than
    other whisky styles.
    </rdfs:comment>
    <rdfs:isDefinedBy rdf:resource="http://rdfs.co/bevon/"/>
    <rdfs:seeAlso rdf:resource="http://en.wikipedia.org/wiki/Canadian_whisky"/>
    <rdfs:subClassOf rdf:resource="http://rdfs.co/bevon/Whisky"/>
    <rdfs:subClassOf rdf:resource="http://www.productontology.org/id/Canadian_whisky"/>
    <status:term_status xml:lang="en">unstable</status:term_status>
    <skos:altLabel xml:lang="en">Canadian Whiskey</skos:altLabel>
    <skos:definition xml:lang="en">
    Canadian whisky is a type of whisky produced in Canada.
    </skos:definition>
    <skos:prefLabel xml:lang="en">Canadian Whisky</skos:prefLabel>
    <skos:prefLabel xml:lang="ko">캐내디언 위스키</skos:prefLabel>
  </owl:Class>
  <owl:Class rdf:about="http://rdfs.co/bevon/CarbonatedWater">
    <dcterms:issued rdf:datatype="http://www.w3.org/2001/XMLSchema#date">2013-07-04+09:00</dcterms:issued>
    <dcterms:modified rdf:datatype="http://www.w3.org/2001/XMLSchema#date">2014-03-01+09:00</dcterms:modified>
    <rdfs:isDefinedBy rdf:resource="http://rdfs.co/bevon/"/>
    <rdfs:seeAlso rdf:resource="http://en.wikipedia.org/wiki/Carbonated_water"/>
    <rdfs:subClassOf rdf:resource="http://rdfs.co/bevon/Water"/>
    <rdfs:subClassOf rdf:resource="http://www.productontology.org/id/Carbonated_water"/>
    <status:term_status xml:lang="en">unstable</status:term_status>
    <skos:altLabel xml:lang="en">Club Soda</skos:altLabel>
    <skos:altLabel xml:lang="en">Fizzy Water</skos:altLabel>
    <skos:altLabel xml:lang="en">Seltzer Water</skos:altLabel>
    <skos:altLabel xml:lang="en">Soda Water</skos:altLabel>
    <skos:altLabel xml:lang="en">Sparkling Water</skos:altLabel>
    <skos:altLabel xml:lang="ko">소다수</skos:altLabel>
    <skos:altLabel xml:lang="ko">클럽소다</skos:altLabel>
    <skos:definition xml:lang="en">
    Carbonated water is water into which carbon dioxide gas under pressure has
    been dissolved.
    </skos:definition>
    <skos:prefLabel xml:lang="en">Carbonated Water</skos:prefLabel>
    <skos:prefLabel xml:lang="ko">탄산수</skos:prefLabel>
  </owl:Class>
  <owl:Class rdf:about="http://rdfs.co/bevon/Cocktail">
    <dcterms:issued rdf:datatype="http://www.w3.org/2001/XMLSchema#date">2013-07-04+09:00</dcterms:issued>
    <dcterms:modified rdf:datatype="http://www.w3.org/2001/XMLSchema#date">2014-03-01+09:00</dcterms:modified>
    <rdfs:comment xml:lang="en">
    Cocktails were originally a mixture of spirits, sugar, water, and bitters.
    It is now often used for almost any mixed drink that contains alcohol,
    including mixers, mixed shots, etc. A cocktail today usually contains one
    or more kinds of spirit and one or more mixers, such as soda or fruit
    juice. Additional ingredients may be sugar, honey, milk, cream, and various
    herbs.
    </rdfs:comment>
    <rdfs:isDefinedBy rdf:resource="http://rdfs.co/bevon/"/>
    <rdfs:seeAlso rdf:resource="http://en.wikipedia.org/wiki/Cocktail"/>
    <rdfs:subClassOf rdf:resource="http://rdfs.co/bevon/AlcoholicBeverage"/>
    <rdfs:subClassOf rdf:resource="http://rdfs.co/bevon/MixedDrink"/>
    <rdfs:subClassOf rdf:resource="http://www.productontology.org/id/Cocktail"/>
    <owl:disjointWith rdf:resource="http://rdfs.co/bevon/Mocktail"/>
    <status:term_status xml:lang="en">unstable</status:term_status>
    <skos:definition xml:lang="en">
    A cocktail is a mixed drink that contains alcohol, including mixers, mixed
    shots, etc.
    </skos:definition>
    <skos:prefLabel xml:lang="en">Cocktail</skos:prefLabel>
    <skos:prefLabel xml:lang="ko">칵테일</skos:prefLabel>
  </owl:Class>
  <rdf:Bag rdf:about="http://rdfs.co/bevon/CocktailGroup">
    <rdf:_1 rdf:resource="http://rdfs.co/bevon/Cocktail"/>
    <rdf:_2 rdf:resource="http://rdfs.co/bevon/Highball"/>
    <rdf:_3 rdf:resource="http://rdfs.co/bevon/BeerCocktail"/>
    <rdf:_4 rdf:resource="http://rdfs.co/bevon/Shandy"/>
    <rdf:_5 rdf:resource="http://rdfs.co/bevon/Mocktail"/>
    <rdfs:comment xml:lang="en">
    These classes and properties are for describing beverages categorized under
    Mixed Drink.
    </rdfs:comment>
    <rdfs:label xml:lang="en">Cocktail Terms</rdfs:label>
  </rdf:Bag>
  <owl:Class rdf:about="http://rdfs.co/bevon/Cognac">
    <dcterms:issued rdf:datatype="http://www.w3.org/2001/XMLSchema#date">2013-07-04+09:00</dcterms:issued>
    <dcterms:modified rdf:datatype="http://www.w3.org/2001/XMLSchema#date">2014-03-01+09:00</dcterms:modified>
    <rdfs:comment xml:lang="en">
    It is produced in the wine-growing region surrounding the town from which
    it takes its name, in the French Departements of Charente and
    Charente-Maritime.
    </rdfs:comment>
    <rdfs:isDefinedBy rdf:resource="http://rdfs.co/bevon/"/>
    <rdfs:seeAlso rdf:resource="http://en.wikipedia.org/wiki/Cognac"/>
    <rdfs:subClassOf rdf:resource="http://rdfs.co/bevon/Brandy"/>
    <rdfs:subClassOf rdf:resource="http://www.productontology.org/id/Cognac"/>
    <status:term_status xml:lang="en">testing</status:term_status>
    <skos:definition xml:lang="en">
    Cognac, named after the town of Cognac in France, is a variety of brandy.
    </skos:definition>
    <skos:prefLabel xml:lang="en">Cognac</skos:prefLabel>
    <skos:prefLabel xml:lang="ko">코냑</skos:prefLabel>
  </owl:Class>
  <owl:Class rdf:about="http://rdfs.co/bevon/Container">
    <dcterms:issued rdf:datatype="http://www.w3.org/2001/XMLSchema#date">2013-07-04+09:00</dcterms:issued>
    <dcterms:modified rdf:datatype="http://www.w3.org/2001/XMLSchema#date">2014-03-01+09:00</dcterms:modified>
    <rdfs:isDefinedBy rdf:resource="http://rdfs.co/bevon/"/>
    <rdfs:seeAlso rdf:resource="http://en.wikipedia.org/wiki/Container"/>
    <rdfs:subClassOf rdf:resource="http://dbpedia.org/class/yago/Containers"/>
    <status:term_status xml:lang="en">unstable</status:term_status>
    <skos:definition xml:lang="en">
    A container is an item used to contain, store, and transport a beverage.
    </skos:definition>
    <skos:prefLabel xml:lang="en">Container</skos:prefLabel>
    <skos:prefLabel xml:lang="ko">용기</skos:prefLabel>
  </owl:Class>
  <rdf:Bag rdf:about="http://rdfs.co/bevon/ContainerGroup">
    <rdf:_1 rdf:resource="http://rdfs.co/bevon/Container"/>
    <rdf:_2 rdf:resource="http://rdfs.co/bevon/BeverageCan"/>
    <rdf:_3 rdf:resource="http://rdfs.co/bevon/GlassBottle"/>
    <rdf:_4 rdf:resource="http://rdfs.co/bevon/PlasticBottle"/>
    <rdf:_5 rdf:resource="http://rdfs.co/bevon/Keg"/>
    <rdf:_6 rdf:resource="http://rdfs.co/bevon/volume"/>
    <rdfs:comment xml:lang="en">
    These classes and properties are used to describe beverage containers.
    </rdfs:comment>
    <rdfs:label xml:lang="en">Container Terms</rdfs:label>
  </rdf:Bag>
  <rdf:Bag rdf:about="http://rdfs.co/bevon/CoreGroup">
    <rdf:_1 rdf:resource="http://rdfs.co/bevon/Beverage"/>
    <rdf:_10 rdf:resource="http://rdfs.co/bevon/Distillery"/>
    <rdf:_11 rdf:resource="http://rdfs.co/bevon/name"/>
    <rdf:_12 rdf:resource="http://rdfs.co/bevon/description"/>
    <rdf:_13 rdf:resource="http://rdfs.co/bevon/origin"/>
    <rdf:_14 rdf:resource="http://rdfs.co/bevon/manufacturer"/>
    <rdf:_15 rdf:resource="http://rdfs.co/bevon/color"/>
    <rdf:_16 rdf:resource="http://rdfs.co/bevon/launch"/>
    <rdf:_17 rdf:resource="http://rdfs.co/bevon/abv"/>
    <rdf:_18 rdf:resource="http://rdfs.co/bevon/proof"/>
    <rdf:_19 rdf:resource="http://rdfs.co/bevon/container"/>
    <rdf:_2 rdf:resource="http://rdfs.co/bevon/AlcoholicBeverage"/>
    <rdf:_20 rdf:resource="http://rdfs.co/bevon/aging"/>
    <rdf:_21 rdf:resource="http://rdfs.co/bevon/fermentation_base"/>
    <rdf:_22 rdf:resource="http://rdfs.co/bevon/distillery"/>
    <rdf:_23 rdf:resource="http://rdfs.co/bevon/ingredient"/>
    <rdf:_3 rdf:resource="http://rdfs.co/bevon/FermentedBeverage"/>
    <rdf:_4 rdf:resource="http://rdfs.co/bevon/DistilledBeverage"/>
    <rdf:_5 rdf:resource="http://rdfs.co/bevon/NonAlcoholicBeverage"/>
    <rdf:_6 rdf:resource="http://rdfs.co/bevon/MixedDrink"/>
    <rdf:_7 rdf:resource="http://rdfs.co/bevon/Container"/>
    <rdf:_8 rdf:resource="http://rdfs.co/bevon/Aging"/>
    <rdf:_9 rdf:resource="http://rdfs.co/bevon/FermentationBase"/>
    <rdfs:comment xml:lang="en">
    These classes and properties form the core of BEVON. They describe
    characteristics of beverages in relatively broad terms.
    </rdfs:comment>
    <rdfs:label xml:lang="en">Core Terms</rdfs:label>
  </rdf:Bag>
  <owl:Class rdf:about="http://rdfs.co/bevon/DilutedSoju">
    <dcterms:issued rdf:datatype="http://www.w3.org/2001/XMLSchema#date">2013-07-04+09:00</dcterms:issued>
    <dcterms:modified rdf:datatype="http://www.w3.org/2001/XMLSchema#date">2014-03-01+09:00</dcterms:modified>
    <rdfs:isDefinedBy rdf:resource="http://rdfs.co/bevon/"/>
    <rdfs:subClassOf rdf:resource="http://rdfs.co/bevon/Soju"/>
    <owl:disjointWith rdf:resource="http://rdfs.co/bevon/DistilledSoju"/>
    <status:term_status xml:lang="en">unstable</status:term_status>
    <skos:definition xml:lang="en">
    Diluted Soju is made by mixing pure ethanol distilled from various grains,
    such as potatoes, wheat, barley, sweet potatoes, or tapioca, with water and
    flavoring.
    </skos:definition>
    <skos:prefLabel xml:lang="en">Diluted Soju</skos:prefLabel>
    <skos:prefLabel xml:lang="ko">희석식 소주</skos:prefLabel>
  </owl:Class>
  <owl:Class rdf:about="http://rdfs.co/bevon/DistilledBeverage">
    <dcterms:issued rdf:datatype="http://www.w3.org/2001/XMLSchema#date">2013-07-04+09:00</dcterms:issued>
    <dcterms:modified rdf:datatype="http://www.w3.org/2001/XMLSchema#date">2014-03-01+09:00</dcterms:modified>
    <rdfs:comment xml:lang="en">
     This excludes undistilled fermented beverages such as beer, wine, and
     cider.
     </rdfs:comment>
    <rdfs:isDefinedBy rdf:resource="http://rdfs.co/bevon/"/>
    <rdfs:seeAlso rdf:resource="http://en.wikipedia.org/wiki/Distilled_beverage"/>
    <rdfs:subClassOf rdf:resource="http://rdfs.co/bevon/AlcoholicBeverage"/>
    <rdfs:subClassOf rdf:resource="http://www.productontology.org/id/Distilled_beverage"/>
    <status:term_status xml:lang="en">testing</status:term_status>
    <skos:altLabel xml:lang="en">Liquor</skos:altLabel>
    <skos:altLabel xml:lang="en">Spirit</skos:altLabel>
    <skos:definition xml:lang="en">
     A distilled beverage, spirit, or liquor is an alcoholic beverage
     containing ethanol that is produced by distilling (i.e., concentrating
     by distillation) ethanol produced by means of fermenting grain, fruit,
     or vegetables.
     </skos:definition>
    <skos:prefLabel xml:lang="en">Distilled Beverage</skos:prefLabel>
    <skos:prefLabel xml:lang="ko">증류주</skos:prefLabel>
  </owl:Class>
  <owl:Class rdf:about="http://rdfs.co/bevon/DistilledSoju">
    <dcterms:issued rdf:datatype="http://www.w3.org/2001/XMLSchema#date">2013-07-04+09:00</dcterms:issued>
    <dcterms:modified rdf:datatype="http://www.w3.org/2001/XMLSchema#date">2014-03-01+09:00</dcterms:modified>
    <rdfs:isDefinedBy rdf:resource="http://rdfs.co/bevon/"/>
    <rdfs:subClassOf rdf:resource="http://rdfs.co/bevon/Soju"/>
    <owl:disjointWith rdf:resource="http://rdfs.co/bevon/DilutedSoju"/>
    <status:term_status xml:lang="en">unstable</status:term_status>
    <skos:definition xml:lang="en">
    Distilled Soju is manufactured traditionally by distillation from grains,
    mainly rice.
    </skos:definition>
    <skos:prefLabel xml:lang="en">Distilled Soju</skos:prefLabel>
    <skos:prefLabel xml:lang="ko">증류식 소주</skos:prefLabel>
  </owl:Class>
  <owl:Class rdf:about="http://rdfs.co/bevon/Distillery">
    <dcterms:issued rdf:datatype="http://www.w3.org/2001/XMLSchema#date">2013-07-04+09:00</dcterms:issued>
    <dcterms:modified rdf:datatype="http://www.w3.org/2001/XMLSchema#date">2014-03-01+09:00</dcterms:modified>
    <rdfs:isDefinedBy rdf:resource="http://rdfs.co/bevon/"/>
    <rdfs:seeAlso rdf:resource="http://en.wikipedia.org/wiki/Distillation"/>
    <status:term_status xml:lang="en">unstable</status:term_status>
    <skos:definition xml:lang="en">
    A distillery is a premise where distillation takes place, especially
    distillation of alcohol.
    </skos:definition>
    <skos:prefLabel xml:lang="en">Distillery</skos:prefLabel>
    <skos:prefLabel xml:lang="ko">증류소</skos:prefLabel>
  </owl:Class>
  <owl:Class rdf:about="http://rdfs.co/bevon/DryStout">
    <dcterms:issued rdf:datatype="http://www.w3.org/2001/XMLSchema#date">2013-07-04+09:00</dcterms:issued>
    <dcterms:modified rdf:datatype="http://www.w3.org/2001/XMLSchema#date">2014-03-01+09:00</dcterms:modified>
    <rdfs:isDefinedBy rdf:resource="http://rdfs.co/bevon/"/>
    <rdfs:subClassOf rdf:resource="http://rdfs.co/bevon/Stout"/>
    <status:term_status xml:lang="en">unstable</status:term_status>
    <skos:altLabel xml:lang="en">Irish Stout</skos:altLabel>
    <skos:definition xml:lang="en">
    Irish stout or dry stout is very dark or rich in color and it often has a
    "roasted" or coffee-like taste.
    </skos:definition>
    <skos:prefLabel xml:lang="en">Dry Stout</skos:prefLabel>
    <skos:prefLabel xml:lang="ko">드라이 스타우트</skos:prefLabel>
  </owl:Class>
  <owl:Class rdf:about="http://rdfs.co/bevon/Dunkel">
    <dcterms:issued rdf:datatype="http://www.w3.org/2001/XMLSchema#date">2013-07-04+09:00</dcterms:issued>
    <dcterms:modified rdf:datatype="http://www.w3.org/2001/XMLSchema#date">2014-03-01+09:00</dcterms:modified>
    <rdfs:comment xml:lang="en">
    Dunkel is the German word meaning dark, and dunkel beers typically range in
    color from amber to dark reddish brown. They are characterized by their
    smooth malty flavor.
    </rdfs:comment>
    <rdfs:isDefinedBy rdf:resource="http://rdfs.co/bevon/"/>
    <rdfs:seeAlso rdf:resource="https://en.wikipedia.org/wiki/Dunkel"/>
    <rdfs:subClassOf rdf:resource="http://rdfs.co/bevon/Lager"/>
    <rdfs:subClassOf rdf:resource="http://www.productontology.org/id/Dunkel"/>
    <status:term_status xml:lang="en">unstable</status:term_status>
    <skos:altLabel xml:lang="en">Dunkles</skos:altLabel>
    <skos:definition xml:lang="en">
    Dunkel, or Dunkles, is a word used for several types of dark German lager.
    </skos:definition>
    <skos:prefLabel xml:lang="en">Dunkel</skos:prefLabel>
    <skos:prefLabel xml:lang="ko">둔켈</skos:prefLabel>
  </owl:Class>
  <owl:Class rdf:about="http://rdfs.co/bevon/FermentationBase">
    <dcterms:issued rdf:datatype="http://www.w3.org/2001/XMLSchema#date">2013-07-04+09:00</dcterms:issued>
    <dcterms:modified rdf:datatype="http://www.w3.org/2001/XMLSchema#date">2014-03-01+09:00</dcterms:modified>
    <rdfs:isDefinedBy rdf:resource="http://rdfs.co/bevon/"/>
    <status:term_status xml:lang="en">unstable</status:term_status>
    <skos:definition xml:lang="en">
    A fruit or grain which provides the sugar for fermentation from which a
    alcoholic beverage is made.
    </skos:definition>
    <skos:prefLabel xml:lang="en">Fermentation Base</skos:prefLabel>
    <skos:prefLabel xml:lang="ko">발효 주재료</skos:prefLabel>
  </owl:Class>
  <owl:Class rdf:about="http://rdfs.co/bevon/FermentedBeverage">
    <dcterms:issued rdf:datatype="http://www.w3.org/2001/XMLSchema#date">2013-07-04+09:00</dcterms:issued>
    <dcterms:modified rdf:datatype="http://www.w3.org/2001/XMLSchema#date">2014-03-01+09:00</dcterms:modified>
    <rdfs:isDefinedBy rdf:resource="http://rdfs.co/bevon/"/>
    <rdfs:subClassOf rdf:resource="http://rdfs.co/bevon/AlcoholicBeverage"/>
    <status:term_status xml:lang="en">testing</status:term_status>
    <skos:altLabel xml:lang="ko">발효주</skos:altLabel>
    <skos:definition xml:lang="en">
    A fermented beverage is a drink produced by fermenting grain, fruit, or
    vegetables.
    </skos:definition>
    <skos:prefLabel xml:lang="en">Fermented Beverage</skos:prefLabel>
    <skos:prefLabel xml:lang="ko">양조주</skos:prefLabel>
  </owl:Class>
  <owl:Class rdf:about="http://rdfs.co/bevon/FruitWine">
    <dcterms:issued rdf:datatype="http://www.w3.org/2001/XMLSchema#date">2014-03-07+09:00</dcterms:issued>
    <dcterms:modified rdf:datatype="http://www.w3.org/2001/XMLSchema#date">2014-03-07+09:00</dcterms:modified>
    <rdfs:comment xml:lang="en">
    This definition is sometimes broadened to include any fermented alcoholic
    beverage except beer. For historical reasons, mead, cider, and perry are
    also excluded from the definition of fruit wine.
    </rdfs:comment>
    <rdfs:isDefinedBy rdf:resource="http://rdfs.co/bevon/"/>
    <rdfs:seeAlso rdf:resource="http://en.wikipedia.org/wiki/Fruit_wine"/>
    <rdfs:subClassOf rdf:resource="http://rdfs.co/bevon/Wine"/>
    <rdfs:subClassOf rdf:resource="http://www.productontology.org/id/Fruit_wine"/>
    <status:term_status xml:lang="en">testing</status:term_status>
    <skos:definition xml:lang="en">
    Fruit wines are fermented alcoholic beverages made from a variety of base
    ingredients (other than grapes); they may also have additional flavors
    taken from fruits, flowers, and herbs.
    </skos:definition>
    <skos:prefLabel xml:lang="en">Fruit Wine</skos:prefLabel>
    <skos:prefLabel xml:lang="fr">Vin de Sureau</skos:prefLabel>
    <skos:prefLabel xml:lang="ko">과실주</skos:prefLabel>
  </owl:Class>
  <owl:Class rdf:about="http://rdfs.co/bevon/Gin">
    <dcterms:issued rdf:datatype="http://www.w3.org/2001/XMLSchema#date">2013-07-04+09:00</dcterms:issued>
    <dcterms:modified rdf:datatype="http://www.w3.org/2001/XMLSchema#date">2014-03-01+09:00</dcterms:modified>
    <rdfs:isDefinedBy rdf:resource="http://rdfs.co/bevon/"/>
    <rdfs:seeAlso rdf:resource="http://en.wikipedia.org/wiki/Gin"/>
    <rdfs:subClassOf rdf:resource="http://rdfs.co/bevon/DistilledBeverage"/>
    <rdfs:subClassOf rdf:resource="http://www.productontology.org/id/Gin"/>
    <status:term_status xml:lang="en">testing</status:term_status>
    <skos:definition xml:lang="en">
    Gin is a spirit which derives its predominant flavor from juniper berries
    (Juniperus communis).
    </skos:definition>
    <skos:prefLabel xml:lang="en">Gin</skos:prefLabel>
    <skos:prefLabel xml:lang="ko">진</skos:prefLabel>
  </owl:Class>
  <owl:Class rdf:about="http://rdfs.co/bevon/GlassBottle">
    <dcterms:issued rdf:datatype="http://www.w3.org/2001/XMLSchema#date">2013-07-04+09:00</dcterms:issued>
    <dcterms:modified rdf:datatype="http://www.w3.org/2001/XMLSchema#date">2014-03-01+09:00</dcterms:modified>
    <rdfs:comment xml:lang="en">
    Glass bottles can vary in size considerably, but are most commonly found in
    sizes ranging between about 10ml and 5 litres.
    </rdfs:comment>
    <rdfs:isDefinedBy rdf:resource="http://rdfs.co/bevon/"/>
    <rdfs:seeAlso rdf:resource="http://en.wikipedia.org/wiki/Glass_bottle"/>
    <rdfs:subClassOf rdf:resource="http://rdfs.co/bevon/Container"/>
    <status:term_status xml:lang="en">unstable</status:term_status>
    <skos:definition xml:lang="en">
    A glass bottle is a bottle created from glass.
    </skos:definition>
    <skos:prefLabel xml:lang="en">Glass Bottle</skos:prefLabel>
    <skos:prefLabel xml:lang="ko">유리병</skos:prefLabel>
  </owl:Class>
  <owl:Class rdf:about="http://rdfs.co/bevon/Highball">
    <dcterms:issued rdf:datatype="http://www.w3.org/2001/XMLSchema#date">2013-07-04+09:00</dcterms:issued>
    <dcterms:modified rdf:datatype="http://www.w3.org/2001/XMLSchema#date">2014-03-01+09:00</dcterms:modified>
    <rdfs:isDefinedBy rdf:resource="http://rdfs.co/bevon/"/>
    <rdfs:seeAlso rdf:resource="http://en.wikipedia.org/wiki/Highball"/>
    <rdfs:subClassOf rdf:resource="http://rdfs.co/bevon/Cocktail"/>
    <rdfs:subClassOf rdf:resource="http://www.productontology.org/id/Highball"/>
    <status:term_status xml:lang="en">unstable</status:term_status>
    <skos:definition xml:lang="en">
    Highball is the name for a family of mixed drinks that are composed of an
    alcoholic base spirit and a larger proportion of a non-alcoholic mixer.
    </skos:definition>
    <skos:prefLabel xml:lang="en">Highball</skos:prefLabel>
    <skos:prefLabel xml:lang="ko">하이볼</skos:prefLabel>
  </owl:Class>
  <owl:Class rdf:about="http://rdfs.co/bevon/IrishRedAle">
    <dcterms:issued rdf:datatype="http://www.w3.org/2001/XMLSchema#date">2013-07-04+09:00</dcterms:issued>
    <dcterms:modified rdf:datatype="http://www.w3.org/2001/XMLSchema#date">2014-03-01+09:00</dcterms:modified>
    <rdfs:isDefinedBy rdf:resource="http://rdfs.co/bevon/"/>
    <rdfs:seeAlso rdf:resource="http://en.wikipedia.org/wiki/Irish_red_ale"/>
    <rdfs:subClassOf rdf:resource="http://rdfs.co/bevon/PaleAle"/>
    <status:term_status xml:lang="en">unstable</status:term_status>
    <skos:definition xml:lang="en">
    Irish red ale, red ale, or Irish ale is a name used by brewers in Ireland.
    </skos:definition>
    <skos:prefLabel xml:lang="en">Irish Red Ale</skos:prefLabel>
    <skos:prefLabel xml:lang="ko">아이리쉬 레드 에일</skos:prefLabel>
  </owl:Class>
  <owl:Class rdf:about="http://rdfs.co/bevon/IrishWhiskey">
    <dcterms:issued rdf:datatype="http://www.w3.org/2001/XMLSchema#date">2013-07-04+09:00</dcterms:issued>
    <dcterms:modified rdf:datatype="http://www.w3.org/2001/XMLSchema#date">2014-03-01+09:00</dcterms:modified>
    <rdfs:comment xml:lang="en">
    Key regulations defining Irish whiskey and its production are established
    by the Irish Whiskey Act of 1980.
    </rdfs:comment>
    <rdfs:isDefinedBy rdf:resource="http://rdfs.co/bevon/"/>
    <rdfs:seeAlso rdf:resource="http://en.wikipedia.org/wiki/Irish_whiskey"/>
    <rdfs:subClassOf rdf:resource="http://rdfs.co/bevon/Whisky"/>
    <rdfs:subClassOf rdf:resource="http://www.productontology.org/id/Irish_whiskey"/>
    <status:term_status xml:lang="en">unstable</status:term_status>
    <skos:altLabel xml:lang="en">Irish Whisky</skos:altLabel>
    <skos:definition xml:lang="en">
    Irish whiskey is whisky made in Ireland.
    </skos:definition>
    <skos:prefLabel xml:lang="ga">Fuisce</skos:prefLabel>
    <skos:prefLabel xml:lang="en">Irish Whiskey</skos:prefLabel>
    <skos:prefLabel xml:lang="ko">아이리쉬 위스키</skos:prefLabel>
  </owl:Class>
  <owl:Class rdf:about="http://rdfs.co/bevon/JapaneseWhisky">
    <dcterms:issued rdf:datatype="http://www.w3.org/2001/XMLSchema#date">2013-07-04+09:00</dcterms:issued>
    <dcterms:modified rdf:datatype="http://www.w3.org/2001/XMLSchema#date">2014-03-01+09:00</dcterms:modified>
    <rdfs:comment xml:lang="en">
    Whisky production in Japan began around 1870, but the first commercial
    production was in 1924 upon the opening of the country's first distillery,
    Yamazaki. Broadly speaking the style of Japanese whisky is more similar to
    that of Scotch whisky than Irish, American, or Canadian styles of whisky,
    and thus the spelling typically follows the Scottish convention (omitting
    the letter "e").
    </rdfs:comment>
    <rdfs:isDefinedBy rdf:resource="http://rdfs.co/bevon/"/>
    <rdfs:seeAlso rdf:resource="http://en.wikipedia.org/wiki/Japanese_whisky"/>
    <rdfs:subClassOf rdf:resource="http://rdfs.co/bevon/Whisky"/>
    <rdfs:subClassOf rdf:resource="http://www.productontology.org/id/Japanese_whisky"/>
    <status:term_status xml:lang="en">unstable</status:term_status>
    <skos:altLabel xml:lang="en">Japanese Whiskey</skos:altLabel>
    <skos:definition xml:lang="en">
    Japanese whisky is whisky made in Japan.
    </skos:definition>
    <skos:prefLabel xml:lang="en">Japanese Whisky</skos:prefLabel>
    <skos:prefLabel xml:lang="ko">재패니즈 위스키</skos:prefLabel>
  </owl:Class>
  <owl:Class rdf:about="http://rdfs.co/bevon/Keg">
    <dcterms:issued rdf:datatype="http://www.w3.org/2001/XMLSchema#date">2013-07-04+09:00</dcterms:issued>
    <dcterms:modified rdf:datatype="http://www.w3.org/2001/XMLSchema#date">2014-03-01+09:00</dcterms:modified>
    <rdfs:isDefinedBy rdf:resource="http://rdfs.co/bevon/"/>
    <rdfs:seeAlso rdf:resource="http://en.wikipedia.org/wiki/Keg"/>
    <rdfs:subClassOf rdf:resource="http://rdfs.co/bevon/Container"/>
    <status:term_status xml:lang="en">unstable</status:term_status>
    <skos:definition xml:lang="en">
    A keg is a small barrel.
    </skos:definition>
    <skos:prefLabel xml:lang="en">Keg</skos:prefLabel>
    <skos:prefLabel xml:lang="ko">케그</skos:prefLabel>
  </owl:Class>
  <owl:Class rdf:about="http://rdfs.co/bevon/Lager">
    <dcterms:issued rdf:datatype="http://www.w3.org/2001/XMLSchema#date">2013-07-04+09:00</dcterms:issued>
    <dcterms:modified rdf:datatype="http://www.w3.org/2001/XMLSchema#date">2014-03-01+09:00</dcterms:modified>
    <rdfs:isDefinedBy rdf:resource="http://rdfs.co/bevon/"/>
    <rdfs:seeAlso rdf:resource="http://en.wikipedia.org/wiki/Lager"/>
    <rdfs:subClassOf rdf:resource="http://rdfs.co/bevon/Beer"/>
    <rdfs:subClassOf rdf:resource="http://www.productontology.org/id/Lager"/>
    <status:term_status xml:lang="en">unstable</status:term_status>
    <skos:definition xml:lang="en">
    Lager is a type of beer that is fermented and conditioned at low
    temperatures.
    </skos:definition>
    <skos:prefLabel xml:lang="en">Lager</skos:prefLabel>
    <skos:prefLabel xml:lang="ko">라거</skos:prefLabel>
  </owl:Class>
  <owl:Class rdf:about="http://rdfs.co/bevon/Liqueur">
    <dcterms:issued rdf:datatype="http://www.w3.org/2001/XMLSchema#date">2013-07-04+09:00</dcterms:issued>
    <dcterms:modified rdf:datatype="http://www.w3.org/2001/XMLSchema#date">2014-03-01+09:00</dcterms:modified>
    <rdfs:comment xml:lang="en">
    Liqueurs are typically quite sweet; they are usually not aged for long
    after the ingredients are mixed, but may have resting periods during their
    production to allow flavors to marry.
    </rdfs:comment>
    <rdfs:isDefinedBy rdf:resource="http://rdfs.co/bevon/"/>
    <rdfs:seeAlso rdf:resource="http://en.wikipedia.org/wiki/Liqueur"/>
    <rdfs:subClassOf rdf:resource="http://rdfs.co/bevon/DistilledBeverage"/>
    <rdfs:subClassOf rdf:resource="http://www.productontology.org/id/Liqueur"/>
    <status:term_status xml:lang="en">testing</status:term_status>
    <skos:altLabel xml:lang="en">Cordials</skos:altLabel>
    <skos:altLabel xml:lang="en">Schnapps</skos:altLabel>
    <skos:definition xml:lang="en">
    A liqueur is an alcoholic beverage made from a distilled spirit that has
    been flavored with fruit, cream, herbs, spices, flowers or nuts and bottled
    with added sugar or other sweetener (such as high-fructose corn syrup).
    </skos:definition>
    <skos:prefLabel xml:lang="en">Liqueur</skos:prefLabel>
    <skos:prefLabel xml:lang="ko">리큐어</skos:prefLabel>
  </owl:Class>
  <owl:Class rdf:about="http://rdfs.co/bevon/Longneck">
    <dcterms:issued rdf:datatype="http://www.w3.org/2001/XMLSchema#date">2013-07-04+09:00</dcterms:issued>
    <dcterms:modified rdf:datatype="http://www.w3.org/2001/XMLSchema#date">2014-03-01+09:00</dcterms:modified>
    <rdfs:comment xml:lang="en">
    It is known as the standard longneck bottle or industry standard bottle
    (ISB). The ISB longnecks have a uniform capacity, height, weight and
    diameter and can be reused on average 16 times. The long neck offers a long
    cushion of air to absorb the pressure of carbonation to reduce the risk of
    exploding. The longneck also provides a handle for drinking directly from
    the bottle without transferring body heat to the beer from one's hand.
    </rdfs:comment>
    <rdfs:isDefinedBy rdf:resource="http://rdfs.co/bevon/"/>
    <rdfs:subClassOf rdf:resource="http://rdfs.co/bevon/BeerBottle"/>
    <status:term_status xml:lang="en">unstable</status:term_status>
    <skos:altLabel xml:lang="en">Industry Standard Bottle</skos:altLabel>
    <skos:altLabel xml:lang="en">North American Longneck</skos:altLabel>
    <skos:definition xml:lang="en">
    A longneck is a type of beer bottle with a long neck.
    </skos:definition>
    <skos:prefLabel xml:lang="en">Longneck</skos:prefLabel>
    <skos:prefLabel xml:lang="ko">긴목 맥주병</skos:prefLabel>
  </owl:Class>
  <owl:Class rdf:about="http://rdfs.co/bevon/MaltWhisky">
    <dcterms:issued rdf:datatype="http://www.w3.org/2001/XMLSchema#date">2013-07-04+09:00</dcterms:issued>
    <dcterms:modified rdf:datatype="http://www.w3.org/2001/XMLSchema#date">2014-03-01+09:00</dcterms:modified>
    <rdfs:isDefinedBy rdf:resource="http://rdfs.co/bevon/"/>
    <rdfs:seeAlso rdf:resource="http://en.wikipedia.org/wiki/Malt_whisky"/>
    <rdfs:subClassOf rdf:resource="http://rdfs.co/bevon/Whisky"/>
    <rdfs:subClassOf rdf:resource="http://www.productontology.org/id/Malt_whisky"/>
    <status:term_status xml:lang="en">unstable</status:term_status>
    <skos:altLabel xml:lang="en">Malt Whiskey</skos:altLabel>
    <skos:definition xml:lang="en">
    Malt whisky is whisky that is made from a fermented mash produced primarily
    from a malted grain.
    </skos:definition>
    <skos:prefLabel xml:lang="en">Malt Whisky</skos:prefLabel>
    <skos:prefLabel xml:lang="ko">몰트 위스키</skos:prefLabel>
  </owl:Class>
  <owl:Class rdf:about="http://rdfs.co/bevon/MineralWater">
    <dcterms:issued rdf:datatype="http://www.w3.org/2001/XMLSchema#date">2013-07-04+09:00</dcterms:issued>
    <dcterms:modified rdf:datatype="http://www.w3.org/2001/XMLSchema#date">2014-03-01+09:00</dcterms:modified>
    <rdfs:comment xml:lang="en">
    Mineral water may be sparkling due to contained gases.
    </rdfs:comment>
    <rdfs:isDefinedBy rdf:resource="http://rdfs.co/bevon/"/>
    <rdfs:seeAlso rdf:resource="http://en.wikipedia.org/wiki/Mineral_water"/>
    <rdfs:subClassOf rdf:resource="http://rdfs.co/bevon/Water"/>
    <rdfs:subClassOf rdf:resource="http://www.productontology.org/id/Mineral_water"/>
    <status:term_status xml:lang="en">unstable</status:term_status>
    <skos:definition xml:lang="en">
    Mineral water is water from a mineral spring containing various minerals
    such as salts and sulfur compounds.
    </skos:definition>
    <skos:prefLabel xml:lang="en">Mineral Water</skos:prefLabel>
    <skos:prefLabel xml:lang="ko">광천수</skos:prefLabel>
  </owl:Class>
  <owl:Class rdf:about="http://rdfs.co/bevon/MixedDrink">
    <dcterms:issued rdf:datatype="http://www.w3.org/2001/XMLSchema#date">2013-07-04+09:00</dcterms:issued>
    <dcterms:modified rdf:datatype="http://www.w3.org/2001/XMLSchema#date">2014-03-01+09:00</dcterms:modified>
    <rdfs:comment xml:lang="en">
    Some mixed drinks are alcoholic beverages that contain liquor; others are
    non-alcoholic.
    </rdfs:comment>
    <rdfs:isDefinedBy rdf:resource="http://rdfs.co/bevon/"/>
    <rdfs:seeAlso rdf:resource="http://en.wikipedia.org/wiki/Mixed_drink"/>
    <rdfs:subClassOf rdf:resource="http://rdfs.co/bevon/Beverage"/>
    <rdfs:subClassOf rdf:resource="http://www.productontology.org/id/Mixed_drink"/>
    <status:term_status xml:lang="en">testing</status:term_status>
    <skos:definition xml:lang="en">
    A mixed drink is a beverage in which two or more ingredients are mixed.
    </skos:definition>
    <skos:prefLabel xml:lang="en">Mixed Drink</skos:prefLabel>
    <skos:prefLabel xml:lang="ko">혼합 음료</skos:prefLabel>
  </owl:Class>
  <owl:Class rdf:about="http://rdfs.co/bevon/Mocktail">
    <dcterms:issued rdf:datatype="http://www.w3.org/2001/XMLSchema#date">2013-07-04+09:00</dcterms:issued>
    <dcterms:modified rdf:datatype="http://www.w3.org/2001/XMLSchema#date">2014-03-01+09:00</dcterms:modified>
    <rdfs:isDefinedBy rdf:resource="http://rdfs.co/bevon/"/>
    <rdfs:subClassOf rdf:resource="http://rdfs.co/bevon/MixedDrink"/>
    <rdfs:subClassOf rdf:resource="http://rdfs.co/bevon/NonAlcoholicBeverage"/>
    <owl:disjointWith rdf:resource="http://rdfs.co/bevon/Cocktail"/>
    <status:term_status xml:lang="en">unstable</status:term_status>
    <skos:definition xml:lang="en">
    Mocktails are mock cocktails, or those that do not contain any alcohol.
    </skos:definition>
    <skos:prefLabel xml:lang="en">Mocktail</skos:prefLabel>
    <skos:prefLabel xml:lang="ko">목테일</skos:prefLabel>
  </owl:Class>
  <owl:Class rdf:about="http://rdfs.co/bevon/NonAlcoholicBeer">
    <dcterms:issued rdf:datatype="http://www.w3.org/2001/XMLSchema#date">2013-07-04+09:00</dcterms:issued>
    <dcterms:modified rdf:datatype="http://www.w3.org/2001/XMLSchema#date">2014-03-01+09:00</dcterms:modified>
    <rdfs:isDefinedBy rdf:resource="http://rdfs.co/bevon/"/>
    <rdfs:seeAlso rdf:resource="http://en.wikipedia.org/wiki/Low-alcohol_beer"/>
    <rdfs:subClassOf rdf:resource="http://rdfs.co/bevon/NonAlcoholicBeverage"/>
    <rdfs:subClassOf rdf:resource="http://www.productontology.org/id/Low-alcohol_beer"/>
    <owl:disjointWith rdf:resource="http://rdfs.co/bevon/Beer"/>
    <status:term_status xml:lang="en">unstable</status:term_status>
    <skos:altLabel xml:lang="en">Low-alcoholic Beer</skos:altLabel>
    <skos:definition xml:lang="en">
    Non-alcohol beer (also called light beer, low-alcoholic beer, small beer,
    small ale, or near-beer) is beer with low alcohol content or no alcohol,
    which aim to reproduce the taste of beer without the inebriating effects of
    standard alcoholic brews.
    </skos:definition>
    <skos:prefLabel xml:lang="en">Non-alcoholic Beer</skos:prefLabel>
    <skos:prefLabel xml:lang="ko">비알코올 맥주</skos:prefLabel>
  </owl:Class>
  <owl:Class rdf:about="http://rdfs.co/bevon/NonAlcoholicBeverage">
    <dcterms:issued rdf:datatype="http://www.w3.org/2001/XMLSchema#date">2013-07-04+09:00</dcterms:issued>
    <dcterms:modified rdf:datatype="http://www.w3.org/2001/XMLSchema#date">2014-03-01+09:00</dcterms:modified>
    <rdfs:isDefinedBy rdf:resource="http://rdfs.co/bevon/"/>
    <rdfs:seeAlso rdf:resource="http://en.wikipedia.org/wiki/Non-alcoholic_beverage"/>
    <rdfs:subClassOf rdf:resource="http://rdfs.co/bevon/Beverage"/>
    <rdfs:subClassOf rdf:resource="http://www.productontology.org/id/Non-alcoholic_beverage"/>
    <owl:disjointWith rdf:resource="http://rdfs.co/bevon/AlcoholicBeverage"/>
    <status:term_status xml:lang="en">testing</status:term_status>
    <skos:definition xml:lang="en">
     A non-alcoholic beverage (also known as a virgin drink) is defined
     in the U.S. as a beverage that contains less than 0.5% alcohol by volume.
     </skos:definition>
    <skos:prefLabel xml:lang="en">Non-alcoholic Beverage</skos:prefLabel>
    <skos:prefLabel xml:lang="ko">비알코올 음료</skos:prefLabel>
  </owl:Class>
  <owl:Class rdf:about="http://rdfs.co/bevon/PaleAle">
    <dcterms:issued rdf:datatype="http://www.w3.org/2001/XMLSchema#date">2013-07-04+09:00</dcterms:issued>
    <dcterms:modified rdf:datatype="http://www.w3.org/2001/XMLSchema#date">2014-03-01+09:00</dcterms:modified>
    <rdfs:comment xml:lang="en">
    It is one of the world's major beer styles.
    </rdfs:comment>
    <rdfs:isDefinedBy rdf:resource="http://rdfs.co/bevon/"/>
    <rdfs:seeAlso rdf:resource="http://en.wikipedia.org/wiki/Pale_ale"/>
    <rdfs:subClassOf rdf:resource="http://rdfs.co/bevon/Ale"/>
    <rdfs:subClassOf rdf:resource="http://www.productontology.org/id/Pale_ale"/>
    <status:term_status xml:lang="en">unstable</status:term_status>
    <skos:definition xml:lang="en">
    Pale ale is a beer made by warm fermentation using predominantly pale malt.
    </skos:definition>
    <skos:prefLabel xml:lang="en">Pale Ale</skos:prefLabel>
    <skos:prefLabel xml:lang="ko">페일 에일</skos:prefLabel>
  </owl:Class>
  <owl:Class rdf:about="http://rdfs.co/bevon/PaleLager">
    <dcterms:issued rdf:datatype="http://www.w3.org/2001/XMLSchema#date">2013-07-04+09:00</dcterms:issued>
    <dcterms:modified rdf:datatype="http://www.w3.org/2001/XMLSchema#date">2014-03-01+09:00</dcterms:modified>
    <rdfs:isDefinedBy rdf:resource="http://rdfs.co/bevon/"/>
    <rdfs:seeAlso rdf:resource="http://en.wikipedia.org/wiki/Pale_lager"/>
    <rdfs:subClassOf rdf:resource="http://rdfs.co/bevon/Lager"/>
    <rdfs:subClassOf rdf:resource="http://www.productontology.org/id/Pale_lager"/>
    <status:term_status xml:lang="en">unstable</status:term_status>
    <skos:definition xml:lang="en">
    Pale lager is a very pale to golden-colored beer with a well attenuated
    body and a varying degree of noble hop bitterness.
    </skos:definition>
    <skos:prefLabel xml:lang="en">Pale Lager</skos:prefLabel>
    <skos:prefLabel xml:lang="ko">페일 라거</skos:prefLabel>
  </owl:Class>
  <owl:Class rdf:about="http://rdfs.co/bevon/Pilsner">
    <dcterms:issued rdf:datatype="http://www.w3.org/2001/XMLSchema#date">2013-07-04+09:00</dcterms:issued>
    <dcterms:modified rdf:datatype="http://www.w3.org/2001/XMLSchema#date">2014-03-01+09:00</dcterms:modified>
    <rdfs:comment xml:lang="en">
    It took its name from the city of Pilsen (Plzeň, Bohemia, Czech Republic,
    where it was first produced in 1842).
    </rdfs:comment>
    <rdfs:isDefinedBy rdf:resource="http://rdfs.co/bevon/"/>
    <rdfs:seeAlso rdf:resource="http://en.wikipedia.org/wiki/Pilsner"/>
    <rdfs:subClassOf rdf:resource="http://rdfs.co/bevon/PaleLager"/>
    <rdfs:subClassOf rdf:resource="http://www.productontology.org/id/Pilsner"/>
    <status:term_status xml:lang="en">unstable</status:term_status>
    <skos:altLabel xml:lang="en">Pils</skos:altLabel>
    <skos:altLabel xml:lang="en">Pilsener</skos:altLabel>
    <skos:definition xml:lang="en">
    Pilsner (also pilsener or simply pils) is a type of pale lager.
    </skos:definition>
    <skos:prefLabel xml:lang="en">Pilsner</skos:prefLabel>
    <skos:prefLabel xml:lang="ko">필스너</skos:prefLabel>
  </owl:Class>
  <owl:Class rdf:about="http://rdfs.co/bevon/Pisco">
    <dcterms:issued rdf:datatype="http://www.w3.org/2001/XMLSchema#date">2013-07-04+09:00</dcterms:issued>
    <dcterms:modified rdf:datatype="http://www.w3.org/2001/XMLSchema#date">2014-03-01+09:00</dcterms:modified>
    <rdfs:isDefinedBy rdf:resource="http://rdfs.co/bevon/"/>
    <rdfs:seeAlso rdf:resource="http://en.wikipedia.org/wiki/Pisco"/>
    <rdfs:subClassOf rdf:resource="http://rdfs.co/bevon/Brandy"/>
    <rdfs:subClassOf rdf:resource="http://www.productontology.org/id/Pisco"/>
    <status:term_status xml:lang="en">testing</status:term_status>
    <skos:definition xml:lang="en">
    Pisco is a colorless or yellowish-to-amber colored grape brandy produced
    in winemaking regions of Peru and Chile.
    </skos:definition>
    <skos:prefLabel xml:lang="en">Pisco</skos:prefLabel>
    <skos:prefLabel xml:lang="ko">피스코</skos:prefLabel>
  </owl:Class>
  <owl:Class rdf:about="http://rdfs.co/bevon/PlasticBottle">
    <dcterms:issued rdf:datatype="http://www.w3.org/2001/XMLSchema#date">2013-07-04+09:00</dcterms:issued>
    <dcterms:modified rdf:datatype="http://www.w3.org/2001/XMLSchema#date">2014-03-01+09:00</dcterms:modified>
    <rdfs:comment xml:lang="en">
    Plastic bottles are typically used to store liquids such as water, soft
    drinks, motor oil, cooking oil, medicine, shampoo, milk, and ink.
    </rdfs:comment>
    <rdfs:isDefinedBy rdf:resource="http://rdfs.co/bevon/"/>
    <rdfs:seeAlso rdf:resource="http://en.wikipedia.org/wiki/Plastic_bottle"/>
    <rdfs:subClassOf rdf:resource="http://rdfs.co/bevon/Container"/>
    <status:term_status xml:lang="en">unstable</status:term_status>
    <skos:definition xml:lang="en">
    A plastic bottle is a bottle constructed of plastic.
    </skos:definition>
    <skos:prefLabel xml:lang="en">Plastic Bottle</skos:prefLabel>
    <skos:prefLabel xml:lang="ko">플라스틱 병</skos:prefLabel>
  </owl:Class>
  <owl:Class rdf:about="http://rdfs.co/bevon/Porter">
    <dcterms:issued rdf:datatype="http://www.w3.org/2001/XMLSchema#date">2013-07-04+09:00</dcterms:issued>
    <dcterms:modified rdf:datatype="http://www.w3.org/2001/XMLSchema#date">2014-03-01+09:00</dcterms:modified>
    <rdfs:comment xml:lang="en">
    The name came about as a result of its popularity with street and river
    porters.
    </rdfs:comment>
    <rdfs:isDefinedBy rdf:resource="http://rdfs.co/bevon/"/>
    <rdfs:seeAlso rdf:resource="http://en.wikipedia.org/wiki/English_porter"/>
    <rdfs:subClassOf rdf:resource="http://rdfs.co/bevon/Ale"/>
    <rdfs:subClassOf rdf:resource="http://www.productontology.org/id/English_porter"/>
    <status:term_status xml:lang="en">unstable</status:term_status>
    <skos:altLabel xml:lang="en">English Porter</skos:altLabel>
    <skos:definition xml:lang="en">
    Porter is a dark style of beer originating in London in the 18th century,
    descended from brown beer, a well hopped beer made from brown malt.
    </skos:definition>
    <skos:prefLabel xml:lang="en">Porter</skos:prefLabel>
    <skos:prefLabel xml:lang="ko">포터</skos:prefLabel>
  </owl:Class>
  <owl:Class rdf:about="http://rdfs.co/bevon/RedWine">
    <dcterms:issued rdf:datatype="http://www.w3.org/2001/XMLSchema#date">2014-03-07+09:00</dcterms:issued>
    <dcterms:modified rdf:datatype="http://www.w3.org/2001/XMLSchema#date">2014-03-07+09:00</dcterms:modified>
    <rdfs:comment xml:lang="en">
    The actual colour of the wine can range from intense violet, typical of
    young wines, through to brick red for mature wines and brown for older red
    wines.
    </rdfs:comment>
    <rdfs:isDefinedBy rdf:resource="http://rdfs.co/bevon/"/>
    <rdfs:seeAlso rdf:resource="http://en.wikipedia.org/wiki/Red_wine"/>
    <rdfs:subClassOf rdf:resource="http://rdfs.co/bevon/Wine"/>
    <rdfs:subClassOf rdf:resource="http://www.productontology.org/id/Red_wine"/>
    <owl:sameAs rdf:resource="http://www.w3.org/TR/2003/PR-owl-guide-20031209/wine#RedWine"/>
    <status:term_status xml:lang="en">testing</status:term_status>
    <skos:definition xml:lang="en">
    Red wine is a type of wine made from dark-coloured (black) grape varieties.
    </skos:definition>
    <skos:prefLabel xml:lang="en">Red Wine</skos:prefLabel>
    <skos:prefLabel xml:lang="fr">Vin Rouge</skos:prefLabel>
    <skos:prefLabel xml:lang="ko">레드 와인</skos:prefLabel>
  </owl:Class>
  <rdf:Bag rdf:about="http://rdfs.co/bevon/RelationGroup">
    <rdf:_1 rdf:resource="http://rdfs.co/bevon/related"/>
    <rdf:_2 rdf:resource="http://rdfs.co/bevon/similar"/>
    <rdf:_3 rdf:resource="http://rdfs.co/bevon/variant"/>
    <rdf:_4 rdf:resource="http://rdfs.co/bevon/variantOf"/>
    <rdf:_5 rdf:resource="http://rdfs.co/bevon/non_alcoholic_version"/>
    <rdfs:comment xml:lang="en">
    These properties are used for describing relations between beverages.
    </rdfs:comment>
    <rdfs:label xml:lang="en">Relation Terms</rdfs:label>
  </rdf:Bag>
  <owl:Class rdf:about="http://rdfs.co/bevon/Rum">
    <dcterms:issued rdf:datatype="http://www.w3.org/2001/XMLSchema#date">2013-07-04+09:00</dcterms:issued>
    <dcterms:modified rdf:datatype="http://www.w3.org/2001/XMLSchema#date">2014-03-01+09:00</dcterms:modified>
    <rdfs:comment xml:lang="en">
    The distillate, a clear liquid, is then usually aged in
    oak barrels.
    </rdfs:comment>
    <rdfs:isDefinedBy rdf:resource="http://rdfs.co/bevon/"/>
    <rdfs:seeAlso rdf:resource="http://en.wikipedia.org/wiki/Rum"/>
    <rdfs:subClassOf rdf:resource="http://rdfs.co/bevon/DistilledBeverage"/>
    <rdfs:subClassOf rdf:resource="http://www.productontology.org/id/Rum"/>
    <status:term_status xml:lang="en">testing</status:term_status>
    <skos:definition xml:lang="en">
    Rum is a distilled alcoholic beverage made from sugarcane byproducts, such
    as molasses, or directly from sugarcane juice, by a process of fermentation
    and distillation.
    </skos:definition>
    <skos:prefLabel xml:lang="es">Ron</skos:prefLabel>
    <skos:prefLabel xml:lang="en">Rum</skos:prefLabel>
    <skos:prefLabel xml:lang="ko">럼</skos:prefLabel>
  </owl:Class>
  <owl:Class rdf:about="http://rdfs.co/bevon/Sake">
    <dcterms:issued rdf:datatype="http://www.w3.org/2001/XMLSchema#date">2013-07-04+09:00</dcterms:issued>
    <dcterms:modified rdf:datatype="http://www.w3.org/2001/XMLSchema#date">2014-03-01+09:00</dcterms:modified>
    <rdfs:isDefinedBy rdf:resource="http://rdfs.co/bevon/"/>
    <rdfs:seeAlso rdf:resource="http://en.wikipedia.org/wiki/Sake"/>
    <rdfs:subClassOf rdf:resource="http://rdfs.co/bevon/FermentedBeverage"/>
    <rdfs:subClassOf rdf:resource="http://www.productontology.org/id/Sake"/>
    <status:term_status xml:lang="en">testing</status:term_status>
    <skos:altLabel xml:lang="en">Rice Wine</skos:altLabel>
    <skos:definition xml:lang="en">
    Sake or saké is an alcoholic beverage of Japanese origin that is made from
    fermented rice.
    </skos:definition>
    <skos:prefLabel xml:lang="en">Sake</skos:prefLabel>
    <skos:prefLabel xml:lang="fr">Saké</skos:prefLabel>
    <skos:prefLabel xml:lang="ko">사케</skos:prefLabel>
  </owl:Class>
  <owl:Class rdf:about="http://rdfs.co/bevon/ScotchWhisky">
    <dcterms:issued rdf:datatype="http://www.w3.org/2001/XMLSchema#date">2013-07-04+09:00</dcterms:issued>
    <dcterms:modified rdf:datatype="http://www.w3.org/2001/XMLSchema#date">2014-03-01+09:00</dcterms:modified>
    <rdfs:comment xml:lang="en">
    All Scotch whisky was originally made from malt barley. Commercial
    distilleries began introducing whisky made from wheat and rye in the late
    eighteenth century.
    </rdfs:comment>
    <rdfs:isDefinedBy rdf:resource="http://rdfs.co/bevon/"/>
    <rdfs:seeAlso rdf:resource="http://en.wikipedia.org/wiki/Scotch_whisky"/>
    <rdfs:subClassOf rdf:resource="http://rdfs.co/bevon/Whisky"/>
    <rdfs:subClassOf rdf:resource="http://www.productontology.org/id/Scotch_whisky"/>
    <status:term_status xml:lang="en">unstable</status:term_status>
    <skos:altLabel xml:lang="en">Scotch Whiskey</skos:altLabel>
    <skos:definition xml:lang="en">
    Scotch whisky (often referred to simply as "Scotch") is malt whisky or grain
    whisky made in Scotland.
    </skos:definition>
    <skos:prefLabel xml:lang="en">Scotch Whisky</skos:prefLabel>
    <skos:prefLabel xml:lang="ko">스카치 위스키</skos:prefLabel>
  </owl:Class>
  <owl:Class rdf:about="http://rdfs.co/bevon/Shandy">
    <dcterms:issued rdf:datatype="http://www.w3.org/2001/XMLSchema#date">2013-07-04+09:00</dcterms:issued>
    <dcterms:modified rdf:datatype="http://www.w3.org/2001/XMLSchema#date">2014-03-01+09:00</dcterms:modified>
    <rdfs:comment xml:lang="en">
    The proportions of the two ingredients are adjusted to taste, usually
    half-and-half.
    </rdfs:comment>
    <rdfs:isDefinedBy rdf:resource="http://rdfs.co/bevon/"/>
    <rdfs:seeAlso rdf:resource="http://en.wikipedia.org/wiki/Shandy"/>
    <rdfs:subClassOf rdf:resource="http://rdfs.co/bevon/Cocktail"/>
    <rdfs:subClassOf rdf:resource="http://www.productontology.org/id/Shandy"/>
    <status:term_status xml:lang="en">unstable</status:term_status>
    <skos:definition xml:lang="en">
    A shandy, or shandygaff, is beer mixed with a soft drink, carbonated
    lemonade, ginger beer, ginger ale, or apple juice.
    </skos:definition>
    <skos:prefLabel xml:lang="en">Shandy</skos:prefLabel>
    <skos:prefLabel xml:lang="ko">섄디</skos:prefLabel>
  </owl:Class>
  <owl:Class rdf:about="http://rdfs.co/bevon/SingleMaltScotch">
    <dcterms:issued rdf:datatype="http://www.w3.org/2001/XMLSchema#date">2013-07-04+09:00</dcterms:issued>
    <dcterms:modified rdf:datatype="http://www.w3.org/2001/XMLSchema#date">2014-03-01+09:00</dcterms:modified>
    <rdfs:comment xml:lang="en">
    As with any Scotch whisky, a single malt Scotch must be distilled in
    Scotland and matured in oak casks in Scotland for at least three years
    (most single malts are matured longer).
    </rdfs:comment>
    <rdfs:isDefinedBy rdf:resource="http://rdfs.co/bevon/"/>
    <rdfs:seeAlso rdf:resource="http://en.wikipedia.org/wiki/Single_malt_Scotch"/>
    <rdfs:subClassOf rdf:resource="http://rdfs.co/bevon/ScotchWhisky"/>
    <rdfs:subClassOf rdf:resource="http://rdfs.co/bevon/SingleMaltWhisky"/>
    <rdfs:subClassOf rdf:resource="http://www.productontology.org/id/Single_malt_Scotch"/>
    <status:term_status xml:lang="en">unstable</status:term_status>
    <skos:definition xml:lang="en">
    Single Malt Scotch is single malt whisky made in Scotland using a pot still
    distillation process at a single distillery, with malted barley as the only
    grain ingredient.
    </skos:definition>
    <skos:prefLabel xml:lang="en">Single Malt Scotch</skos:prefLabel>
    <skos:prefLabel xml:lang="ko">싱글 몰트 스카치</skos:prefLabel>
  </owl:Class>
  <owl:Class rdf:about="http://rdfs.co/bevon/SingleMaltWhisky">
    <dcterms:issued rdf:datatype="http://www.w3.org/2001/XMLSchema#date">2013-07-04+09:00</dcterms:issued>
    <dcterms:modified rdf:datatype="http://www.w3.org/2001/XMLSchema#date">2014-03-01+09:00</dcterms:modified>
    <rdfs:isDefinedBy rdf:resource="http://rdfs.co/bevon/"/>
    <rdfs:seeAlso rdf:resource="http://en.wikipedia.org/wiki/Single_malt_whisky"/>
    <rdfs:subClassOf rdf:resource="http://rdfs.co/bevon/MaltWhisky"/>
    <rdfs:subClassOf rdf:resource="http://www.productontology.org/id/Single_malt_whisky"/>
    <status:term_status xml:lang="en">unstable</status:term_status>
    <skos:altLabel xml:lang="en">Single Malt Whiskey</skos:altLabel>
    <skos:definition xml:lang="en">
    Single malt whisky is a whisky made at one particular distillery from a
    mash that uses only malted grain, ordinarily barley.
    </skos:definition>
    <skos:prefLabel xml:lang="en">Single Malt Whisky</skos:prefLabel>
    <skos:prefLabel xml:lang="ko">싱글 몰트 위스키</skos:prefLabel>
  </owl:Class>
  <owl:Class rdf:about="http://rdfs.co/bevon/Soju">
    <dcterms:issued rdf:datatype="http://www.w3.org/2001/XMLSchema#date">2013-07-04+09:00</dcterms:issued>
    <dcterms:modified rdf:datatype="http://www.w3.org/2001/XMLSchema#date">2014-03-01+09:00</dcterms:modified>
    <rdfs:comment xml:lang="en">
    Its taste is comparable to vodka, though often slightly sweeter due to
    sugars added in the manufacturing process.
    </rdfs:comment>
    <rdfs:isDefinedBy rdf:resource="http://rdfs.co/bevon/"/>
    <rdfs:seeAlso rdf:resource="http://en.wikipedia.org/wiki/Soju"/>
    <rdfs:subClassOf rdf:resource="http://rdfs.co/bevon/DistilledBeverage"/>
    <rdfs:subClassOf rdf:resource="http://www.productontology.org/id/Soju"/>
    <status:term_status xml:lang="en">testing</status:term_status>
    <skos:definition xml:lang="en">
    Soju is a distilled beverage native to Korea.
    </skos:definition>
    <skos:prefLabel xml:lang="en">Soju</skos:prefLabel>
    <skos:prefLabel xml:lang="ko">소주</skos:prefLabel>
  </owl:Class>
  <owl:Class rdf:about="http://rdfs.co/bevon/SpeysideSingleMalt">
    <dcterms:issued rdf:datatype="http://www.w3.org/2001/XMLSchema#date">2013-07-04+09:00</dcterms:issued>
    <dcterms:modified rdf:datatype="http://www.w3.org/2001/XMLSchema#date">2014-03-01+09:00</dcterms:modified>
    <rdfs:isDefinedBy rdf:resource="http://rdfs.co/bevon/"/>
    <rdfs:seeAlso rdf:resource="http://en.wikipedia.org/wiki/Speyside_single_malts"/>
    <rdfs:subClassOf rdf:resource="http://rdfs.co/bevon/SingleMaltScotch"/>
    <rdfs:subClassOf rdf:resource="http://www.productontology.org/id/Speyside_single_malts"/>
    <status:term_status xml:lang="en">unstable</status:term_status>
    <skos:definition xml:lang="en">
    Speyside single malts are single malt Scotch whiskies, distilled in
    Strathspey, the area around the River Spey in Moray and Badenoch and
    Strathspey, in northeastern Scotland.
    </skos:definition>
    <skos:prefLabel xml:lang="en">Speyside Single Malt</skos:prefLabel>
    <skos:prefLabel xml:lang="ko">스페이사이드 싱글 몰트</skos:prefLabel>
  </owl:Class>
  <owl:Class rdf:about="http://rdfs.co/bevon/Stout">
    <dcterms:issued rdf:datatype="http://www.w3.org/2001/XMLSchema#date">2013-07-04+09:00</dcterms:issued>
    <dcterms:modified rdf:datatype="http://www.w3.org/2001/XMLSchema#date">2014-03-01+09:00</dcterms:modified>
    <rdfs:comment xml:lang="en">
    Stouts were traditionally the generic term for the strongest or stoutest
    porters, typically 7% or 8%, produced by a brewery.
    </rdfs:comment>
    <rdfs:isDefinedBy rdf:resource="http://rdfs.co/bevon/"/>
    <rdfs:seeAlso rdf:resource="http://en.wikipedia.org/wiki/Stout"/>
    <rdfs:subClassOf rdf:resource="http://rdfs.co/bevon/Porter"/>
    <rdfs:subClassOf rdf:resource="http://www.productontology.org/id/Stout"/>
    <status:term_status xml:lang="en">unstable</status:term_status>
    <skos:altLabel xml:lang="en">Strong Porter</skos:altLabel>
    <skos:definition xml:lang="en">
    Stout is a dark beer made using roasted malt or roasted barley, hops, water
    and yeast.
    </skos:definition>
    <skos:prefLabel xml:lang="en">Stout</skos:prefLabel>
    <skos:prefLabel xml:lang="ko">스타우트</skos:prefLabel>
  </owl:Class>
  <owl:Class rdf:about="http://rdfs.co/bevon/Tequila">
    <dcterms:issued rdf:datatype="http://www.w3.org/2001/XMLSchema#date">2013-07-04+09:00</dcterms:issued>
    <dcterms:modified rdf:datatype="http://www.w3.org/2001/XMLSchema#date">2014-03-01+09:00</dcterms:modified>
    <rdfs:isDefinedBy rdf:resource="http://rdfs.co/bevon/"/>
    <rdfs:seeAlso rdf:resource="http://en.wikipedia.org/wiki/Tequila"/>
    <rdfs:subClassOf rdf:resource="http://rdfs.co/bevon/DistilledBeverage"/>
    <rdfs:subClassOf rdf:resource="http://www.productontology.org/id/Tequila"/>
    <status:term_status xml:lang="en">testing</status:term_status>
    <skos:definition xml:lang="en">
    Tequila is a distilled beverage made from the blue agave plant, primarily
    in the area surrounding the city of Tequila, 65 kilometres (40 mi)
    northwest of Guadalajara, and in the highlands (Los Altos) of the western
    Mexican state of Jalisco.
    </skos:definition>
    <skos:prefLabel xml:lang="en">Tequila</skos:prefLabel>
    <skos:prefLabel xml:lang="ko">테킬라</skos:prefLabel>
  </owl:Class>
  <owl:Class rdf:about="http://rdfs.co/bevon/TequilaBlanco">
    <dcterms:issued rdf:datatype="http://www.w3.org/2001/XMLSchema#date">2013-07-04+09:00</dcterms:issued>
    <dcterms:modified rdf:datatype="http://www.w3.org/2001/XMLSchema#date">2014-03-01+09:00</dcterms:modified>
    <rdfs:isDefinedBy rdf:resource="http://rdfs.co/bevon/"/>
    <rdfs:subClassOf rdf:resource="http://rdfs.co/bevon/Tequila"/>
    <status:term_status xml:lang="en">unstable</status:term_status>
    <skos:altLabel xml:lang="en">Tequila Plata</skos:altLabel>
    <skos:definition xml:lang="en">
    Tequila Blanco ("white") or Plata ("silver") is a white spirit, un-aged and
    bottled or stored immediately after distillation, or aged less than two
    months in stainless steel or neutral oak barrels.
    </skos:definition>
    <skos:prefLabel xml:lang="en">Tequila Blanco</skos:prefLabel>
    <skos:prefLabel xml:lang="ko">테킬라 블랑코</skos:prefLabel>
  </owl:Class>
  <owl:Class rdf:about="http://rdfs.co/bevon/Vodka">
    <dcterms:issued rdf:datatype="http://www.w3.org/2001/XMLSchema#date">2013-07-04+09:00</dcterms:issued>
    <dcterms:modified rdf:datatype="http://www.w3.org/2001/XMLSchema#date">2014-03-01+09:00</dcterms:modified>
    <rdfs:comment xml:lang="en">
    Vodka is made by the distillation of fermented substances such as grains,
    potatoes, or sometimes fruits or sugar.
    </rdfs:comment>
    <rdfs:isDefinedBy rdf:resource="http://rdfs.co/bevon/"/>
    <rdfs:seeAlso rdf:resource="http://en.wikipedia.org/wiki/Vodka"/>
    <rdfs:subClassOf rdf:resource="http://rdfs.co/bevon/DistilledBeverage"/>
    <rdfs:subClassOf rdf:resource="http://www.productontology.org/id/Vodka"/>
    <status:term_status xml:lang="en">testing</status:term_status>
    <skos:definition xml:lang="en">
    Vodka is a distilled beverage composed primarily of water and ethanol,
    sometimes with traces of impurities and flavorings.
    </skos:definition>
    <skos:prefLabel xml:lang="en">Vodka</skos:prefLabel>
    <skos:prefLabel xml:lang="pl">Wódka</skos:prefLabel>
    <skos:prefLabel xml:lang="ru">водка</skos:prefLabel>
    <skos:prefLabel xml:lang="ko">보드카</skos:prefLabel>
  </owl:Class>
  <owl:Class rdf:about="http://rdfs.co/bevon/Water">
    <dcterms:issued rdf:datatype="http://www.w3.org/2001/XMLSchema#date">2013-07-04+09:00</dcterms:issued>
    <dcterms:modified rdf:datatype="http://www.w3.org/2001/XMLSchema#date">2014-03-01+09:00</dcterms:modified>
    <rdfs:isDefinedBy rdf:resource="http://rdfs.co/bevon/"/>
    <rdfs:seeAlso rdf:resource="http://en.wikipedia.org/wiki/Water"/>
    <rdfs:subClassOf rdf:resource="http://rdfs.co/bevon/NonAlcoholicBeverage"/>
    <rdfs:subClassOf rdf:resource="http://www.productontology.org/id/Water"/>
    <status:term_status xml:lang="en">testing</status:term_status>
    <skos:definition xml:lang="en">
    In the Beverage Ontology, Water means a drinking water.
    </skos:definition>
    <skos:prefLabel xml:lang="en">Water</skos:prefLabel>
    <skos:prefLabel xml:lang="ko">물</skos:prefLabel>
  </owl:Class>
  <owl:Class rdf:about="http://rdfs.co/bevon/Whisky">
    <dcterms:issued rdf:datatype="http://www.w3.org/2001/XMLSchema#date">2013-07-04+09:00</dcterms:issued>
    <dcterms:modified rdf:datatype="http://www.w3.org/2001/XMLSchema#date">2015-07-23+09:00</dcterms:modified>
    <rdfs:comment xml:lang="en">
    Different grains are used for different varieties, including barley, malted
    barley, rye, malted rye, wheat, and corn. Whisky is typically aged in
    wooden casks, made generally of charred white oak.
    </rdfs:comment>
    <rdfs:isDefinedBy rdf:resource="http://rdfs.co/bevon/"/>
    <rdfs:seeAlso rdf:resource="http://en.wikipedia.org/wiki/Whisky"/>
    <rdfs:subClassOf rdf:resource="http://rdfs.co/bevon/DistilledBeverage"/>
    <rdfs:subClassOf rdf:resource="http://www.productontology.org/id/Whisky"/>
    <owl:sameAs rdf:resource="http://purl.org/vocab/whisky/terms/Whisky"/>
    <status:term_status xml:lang="en">testing</status:term_status>
    <skos:altLabel xml:lang="en">Whiskey</skos:altLabel>
    <skos:definition xml:lang="en">
    Whisky or whiskey is a type of distilled alcoholic beverage made from
    fermented grain mash.
    </skos:definition>
    <skos:prefLabel xml:lang="en">Whisky</skos:prefLabel>
    <skos:prefLabel xml:lang="en">위스키</skos:prefLabel>
  </owl:Class>
  <rdf:Bag rdf:about="http://rdfs.co/bevon/WhiskyGroup">
    <rdf:_1 rdf:resource="http://rdfs.co/bevon/Whisky"/>
    <rdf:_10 rdf:resource="http://rdfs.co/bevon/SingleMaltScotch"/>
    <rdf:_11 rdf:resource="http://rdfs.co/bevon/SpeysideSingleMalt"/>
    <rdf:_2 rdf:resource="http://rdfs.co/bevon/AmericanWhiskey"/>
    <rdf:_3 rdf:resource="http://rdfs.co/bevon/BourbonWhiskey"/>
    <rdf:_4 rdf:resource="http://rdfs.co/bevon/CanadianWhisky"/>
    <rdf:_5 rdf:resource="http://rdfs.co/bevon/IrishWhiskey"/>
    <rdf:_6 rdf:resource="http://rdfs.co/bevon/JapaneseWhisky"/>
    <rdf:_7 rdf:resource="http://rdfs.co/bevon/ScotchWhisky"/>
    <rdf:_8 rdf:resource="http://rdfs.co/bevon/MaltWhisky"/>
    <rdf:_9 rdf:resource="http://rdfs.co/bevon/SingleMaltWhisky"/>
    <rdfs:comment xml:lang="en">
    These classes describe types of whiskies.
    </rdfs:comment>
    <rdfs:label xml:lang="en">Whisky Terms</rdfs:label>
  </rdf:Bag>
  <owl:Class rdf:about="http://rdfs.co/bevon/WhiteWine">
    <dcterms:issued rdf:datatype="http://www.w3.org/2001/XMLSchema#date">2014-03-07+09:00</dcterms:issued>
    <dcterms:modified rdf:datatype="http://www.w3.org/2001/XMLSchema#date">2014-03-07+09:00</dcterms:modified>
    <rdfs:comment xml:lang="en">
    It is produced by the alcoholic fermentation of the non-coloured pulp of
    grapes which may have a white or black skin. It is treated so as to
    maintain a yellow transparent colour in the final product.
    </rdfs:comment>
    <rdfs:isDefinedBy rdf:resource="http://rdfs.co/bevon/"/>
    <rdfs:seeAlso rdf:resource="http://en.wikipedia.org/wiki/White_wine"/>
    <rdfs:subClassOf rdf:resource="http://rdfs.co/bevon/Wine"/>
    <rdfs:subClassOf rdf:resource="http://www.productontology.org/id/White_wine"/>
    <owl:sameAs rdf:resource="http://www.w3.org/TR/2003/PR-owl-guide-20031209/wine#WhiteWine"/>
    <status:term_status xml:lang="en">testing</status:term_status>
    <skos:definition xml:lang="en">
    White wine is a wine whose colour can be straw-yellow, yellow-green, or
    yellow-gold coloured.
    </skos:definition>
    <skos:prefLabel xml:lang="fr">Vin Blanc</skos:prefLabel>
    <skos:prefLabel xml:lang="en">White Wine</skos:prefLabel>
    <skos:prefLabel xml:lang="ko">화이트 와인</skos:prefLabel>
  </owl:Class>
  <owl:Class rdf:about="http://rdfs.co/bevon/Wine">
    <dcterms:issued rdf:datatype="http://www.w3.org/2001/XMLSchema#date">2013-07-04+09:00</dcterms:issued>
    <dcterms:modified rdf:datatype="http://www.w3.org/2001/XMLSchema#date">2014-03-07+09:00</dcterms:modified>
    <rdfs:isDefinedBy rdf:resource="http://rdfs.co/bevon/"/>
    <rdfs:seeAlso rdf:resource="http://en.wikipedia.org/wiki/Wine"/>
    <rdfs:subClassOf rdf:resource="http://rdfs.co/bevon/FermentedBeverage"/>
    <rdfs:subClassOf rdf:resource="http://www.productontology.org/id/Wine"/>
    <status:term_status xml:lang="en">testing</status:term_status>
    <skos:definition xml:lang="en">
    Wine is an alcoholic beverage made from fermented grapes or other fruits.
    </skos:definition>
    <skos:historyNote>
      <rdf:Description>
        <dcterms:creator rdf:resource="http://jayg.me/"/>
        <dcterms:date rdf:datatype="http://www.w3.org/2001/XMLSchema#date">2014-03-07+09:00</dcterms:date>
        <rdf:value xml:lang="en">
      Changed the semantics of bevon:Wine not to be the same as wine:Wine
      </rdf:value>
      </rdf:Description>
    </skos:historyNote>
    <skos:prefLabel xml:lang="fr">Vin</skos:prefLabel>
    <skos:prefLabel xml:lang="en">Wine</skos:prefLabel>
    <skos:prefLabel xml:lang="ko">와인</skos:prefLabel>
  </owl:Class>
  <rdf:Bag rdf:about="http://rdfs.co/bevon/WineGroup">
    <rdf:_1 rdf:resource="http://rdfs.co/bevon/Wine"/>
    <rdf:_2 rdf:resource="http://rdfs.co/bevon/RedWine"/>
    <rdf:_3 rdf:resource="http://rdfs.co/bevon/WhiteWine"/>
    <rdf:_4 rdf:resource="http://rdfs.co/bevon/FruitWine"/>
    <rdfs:comment xml:lang="en">
    These classes describe types of wines.
    </rdfs:comment>
    <rdfs:label xml:lang="en">Wine Terms</rdfs:label>
  </rdf:Bag>
  <owl:DatatypeProperty rdf:about="http://rdfs.co/bevon/abv">
    <dcterms:issued rdf:datatype="http://www.w3.org/2001/XMLSchema#date">2013-07-04+09:00</dcterms:issued>
    <dcterms:modified rdf:datatype="http://www.w3.org/2001/XMLSchema#date">2014-03-01+09:00</dcterms:modified>
    <rdfs:domain rdf:resource="http://rdfs.co/bevon/Beverage"/>
    <rdfs:isDefinedBy rdf:resource="http://rdfs.co/bevon/"/>
    <rdfs:range rdf:resource="http://www.w3.org/2001/XMLSchema#decimal"/>
    <rdfs:seeAlso rdf:resource="http://en.wikipedia.org/wiki/Alcohol_by_volume"/>
    <status:term_status xml:lang="en">testing</status:term_status>
    <skos:altLabel xml:lang="en">alcohol by volume</skos:altLabel>
    <skos:definition xml:lang="en">
    ABV (Alcohol by Volume) is a standard measure of how much alcohol is
    contained in the drink.
    </skos:definition>
    <skos:prefLabel xml:lang="en">ABV</skos:prefLabel>
    <skos:prefLabel xml:lang="ko">알코올 도수</skos:prefLabel>
  </owl:DatatypeProperty>
  <owl:ObjectProperty rdf:about="http://rdfs.co/bevon/aging">
    <dcterms:issued rdf:datatype="http://www.w3.org/2001/XMLSchema#date">2013-07-04+09:00</dcterms:issued>
    <dcterms:modified rdf:datatype="http://www.w3.org/2001/XMLSchema#date">2014-03-01+09:00</dcterms:modified>
    <rdfs:domain rdf:resource="http://rdfs.co/bevon/AlcoholicBeverage"/>
    <rdfs:isDefinedBy rdf:resource="http://rdfs.co/bevon/"/>
    <rdfs:range rdf:resource="http://rdfs.co/bevon/Aging"/>
    <status:term_status xml:lang="en">unstable</status:term_status>
    <skos:definition xml:lang="en">
    This property specifies how the beverage has been aged.
    </skos:definition>
    <skos:prefLabel xml:lang="en">aging</skos:prefLabel>
    <skos:prefLabel xml:lang="ko">숙성</skos:prefLabel>
  </owl:ObjectProperty>
  <owl:NamedIndividual rdf:about="http://rdfs.co/bevon/beverage/Budweiser">
    <bevon:abv rdf:datatype="http://www.w3.org/2001/XMLSchema#decimal">5</bevon:abv>
    <bevon:container rdf:resource="http://rdfs.co/bevon/container/330mlLongneck"/>
    <bevon:container rdf:resource="http://rdfs.co/bevon/container/355mlBeverageCan"/>
    <bevon:container rdf:resource="http://rdfs.co/bevon/container/500mlBeverageCan"/>
    <bevon:description xml:lang="en">
    Budweiser is a pale lager produced by Anheuser–Busch InBev. Introduced in
    1876 by Adolphus Busch it has grown to become one of the highest selling
    beers in the United States, and is available in over 80 markets worldwide.
    </bevon:description>
    <bevon:fermentation_base rdf:resource="http://dbpedia.org/resource/Barley"/>
    <bevon:ibu rdf:datatype="http://www.w3.org/2001/XMLSchema#nonNegativeInteger">12</bevon:ibu>
    <bevon:launch rdf:datatype="http://www.w3.org/2001/XMLSchema#gYear">1876</bevon:launch>
    <bevon:manufacturer rdf:resource="http://dbpedia.org/resource/Anheuser–Busch_InBev"/>
    <bevon:name xml:lang="en">Budweiser</bevon:name>
    <bevon:name xml:lang="ko">버드와이저</bevon:name>
    <bevon:origin rdf:resource="http://dbpedia.org/resource/United_States"/>
    <bevon:srm rdf:datatype="http://www.w3.org/2001/XMLSchema#nonNegativeInteger">3</bevon:srm>
    <rdf:type rdf:resource="http://purl.org/goodrelations/v1#ProductOrServiceModel"/>
    <rdf:type rdf:resource="http://rdfs.co/bevon/PaleLager"/>
    <rdfs:seeAlso rdf:resource="https://en.wikipedia.org/wiki/Budweiser_(Anheuser-Busch)"/>
  </owl:NamedIndividual>
  <owl:NamedIndividual rdf:about="http://rdfs.co/bevon/beverage/Chamisul">
    <bevon:abv rdf:datatype="http://www.w3.org/2001/XMLSchema#decimal">19</bevon:abv>
    <bevon:color>
      <dbpedia:Colour>
        <dcterms:title xml:lang="en">Clear</dcterms:title>
        <owl:sameAs rdf:resource="http://dbpedia.org/resource/Clear_(color)"/>
      </dbpedia:Colour>
    </bevon:color>
    <bevon:container rdf:resource="http://rdfs.co/bevon/container/1_8lPlasticBottle"/>
    <bevon:container rdf:resource="http://rdfs.co/bevon/container/200mlPlasticBottle"/>
    <bevon:container rdf:resource="http://rdfs.co/bevon/container/360mlGlassBottle"/>
    <bevon:container rdf:resource="http://rdfs.co/bevon/container/640mlPlasticBottle"/>
    <bevon:description xml:lang="en">
    Chamisul is the diluted soju produced by HITEJiro.
    </bevon:description>
    <bevon:launch rdf:datatype="http://www.w3.org/2001/XMLSchema#gYear">1998</bevon:launch>
    <bevon:manufacturer rdf:resource="http://dbpedia.org/resource/Jinro"/>
    <bevon:name xml:lang="en">Chamisul</bevon:name>
    <bevon:name xml:lang="ko">참이슬</bevon:name>
    <bevon:origin rdf:resource="http://dbpedia.org/resource/South_Korea"/>
    <rdf:type rdf:resource="http://purl.org/goodrelations/v1#ProductOrServiceModel"/>
    <rdf:type rdf:resource="http://rdfs.co/bevon/DilutedSoju"/>
    <rdfs:seeAlso rdf:resource="http://ko.wikipedia.org/wiki/참이슬"/>
  </owl:NamedIndividual>
  <owl:NamedIndividual rdf:about="http://rdfs.co/bevon/beverage/Chum-Churum">
    <bevon:abv rdf:datatype="http://www.w3.org/2001/XMLSchema#decimal">19.5</bevon:abv>
    <bevon:color>
      <dbpedia:Colour>
        <dcterms:title xml:lang="en">Clear</dcterms:title>
        <owl:sameAs rdf:resource="http://dbpedia.org/resource/Clear_(color)"/>
      </dbpedia:Colour>
    </bevon:color>
    <bevon:container rdf:resource="http://rdfs.co/bevon/container/1_8lPlasticBottle"/>
    <bevon:container rdf:resource="http://rdfs.co/bevon/container/200mlPlasticBottle"/>
    <bevon:container rdf:resource="http://rdfs.co/bevon/container/360mlGlassBottle"/>
    <bevon:container rdf:resource="http://rdfs.co/bevon/container/360mlPlasticBottle"/>
    <bevon:container rdf:resource="http://rdfs.co/bevon/container/640mlPlasticBottle"/>
    <bevon:description xml:lang="en">
    Chum-Churum is the diluted soju produced by Lotte Liquor.
    </bevon:description>
    <bevon:launch rdf:datatype="http://www.w3.org/2001/XMLSchema#gYear">2006</bevon:launch>
    <bevon:manufacturer>
      <foaf:Organization>
        <rdfs:seeAlso rdf:resource="http://ko.wikipedia.org/wiki/롯데칠성음료"/>
        <foaf:homepage rdf:resource="http://www.lotteliquor.com"/>
        <foaf:name xml:lang="en">Lotte Liquor</foaf:name>
        <foaf:name xml:lang="ko">롯데주류</foaf:name>
      </foaf:Organization>
    </bevon:manufacturer>
    <bevon:name xml:lang="en">Chum-Churum</bevon:name>
    <bevon:name xml:lang="ko">처음처럼</bevon:name>
    <bevon:origin rdf:resource="http://dbpedia.org/resource/South_Korea"/>
    <rdf:type rdf:resource="http://purl.org/goodrelations/v1#ProductOrServiceModel"/>
    <rdf:type rdf:resource="http://rdfs.co/bevon/DilutedSoju"/>
    <rdfs:seeAlso rdf:resource="http://ko.wikipedia.org/wiki/처음처럼_(주류)"/>
    <owl:sameAs rdf:resource="http://dbpedia.org/resource/Chum-Churum"/>
  </owl:NamedIndividual>
  <owl:NamedIndividual rdf:about="http://rdfs.co/bevon/beverage/DonJulioBlanco">
    <bevon:abv rdf:datatype="http://www.w3.org/2001/XMLSchema#decimal">40</bevon:abv>
    <bevon:color>
      <dbpedia:Colour>
        <dcterms:title xml:lang="en">Clear</dcterms:title>
        <owl:sameAs rdf:resource="http://dbpedia.org/resource/Clear_(color)"/>
      </dbpedia:Colour>
    </bevon:color>
    <bevon:container rdf:resource="http://rdfs.co/bevon/container/750mlGlassBottle"/>
    <bevon:description xml:lang="en">
    Tequila Don Julio Blanco is the base from which all of our other variants
    are derived. Commonly referred to as "silver" tequila, its crisp agave
    flavor and hints of citrus make it an essential component to a variety of
    innovative drinks including margaritas. It can also be enjoyed neat or on
    the rocks.
    </bevon:description>
    <bevon:fermentation_base rdf:resource="http://dbpedia.org/resource/Agave"/>
    <bevon:launch rdf:datatype="http://www.w3.org/2001/XMLSchema#gYear">1942</bevon:launch>
    <bevon:manufacturer rdf:resource="http://dbpedia.org/resource/Diageo"/>
    <bevon:name xml:lang="en">Don Julio Blanco</bevon:name>
    <bevon:name xml:lang="ko">돈 훌리오 블랑코</bevon:name>
    <bevon:origin rdf:resource="http://dbpedia.org/resource/Mexico"/>
    <bevon:proof rdf:datatype="http://www.w3.org/2001/XMLSchema#decimal">80</bevon:proof>
    <rdf:type rdf:resource="http://purl.org/goodrelations/v1#ProductOrServiceModel"/>
    <rdf:type rdf:resource="http://rdfs.co/bevon/TequilaBlanco"/>
    <rdfs:seeAlso rdf:resource="http://www.donjulio.com/blanco.aspx"/>
  </owl:NamedIndividual>
  <owl:NamedIndividual rdf:about="http://rdfs.co/bevon/beverage/Glenfiddich12YearOld">
    <bevon:abv rdf:datatype="http://www.w3.org/2001/XMLSchema#decimal">40</bevon:abv>
    <bevon:aging>
      <bevon:Aging>
        <bevon:duration>
          <time:DurationDescription>
            <time:years rdf:datatype="http://www.w3.org/2001/XMLSchema#decimal">12</time:years>
          </time:DurationDescription>
        </bevon:duration>
        <bevon:material rdf:resource="http://dbpedia.org/resource/Oak"/>
        <bevon:previous_content rdf:resource="http://dbpedia.org/resource/Bourbon_whiskey"/>
        <bevon:previous_content rdf:resource="http://dbpedia.org/resource/Sherry"/>
      </bevon:Aging>
    </bevon:aging>
    <bevon:color>
      <dbpedia:Colour>
        <dcterms:title xml:lang="en">Gold</dcterms:title>
        <owl:sameAs rdf:resource="http://dbpedia.org/resource/Gold_(color)"/>
        <owl:sameAs rdf:resource="http://purl.org/colors/rgb/FFD700"/>
      </dbpedia:Colour>
    </bevon:color>
    <bevon:container rdf:resource="http://rdfs.co/bevon/container/700mlGlassBottle"/>
    <bevon:description xml:lang="en">
    Carefully matured in the finest American bourbon and Spanish sherry oak
    casks for at least 12 years. Married and mellowed in oak marrying tuns for
    complete harmony of aroma and flavor.

    A single malt Scotch whisky with distinctive fresh pear, creamy with subtle
    oak flavors and a long smooth and mellow finish.
    </bevon:description>
    <bevon:distillery>
      <bevon:Distillery>
        <whisky:owner rdf:resource="http://dbpedia.org/resource/William_Grant_%26_Sons"/>
        <whisky:region rdf:resource="http://dbpedia.org/resource/Strathspey,_Scotland"/>
        <whisky:waterSource>
          <whisky:WaterSource>
            <dcterms:title xml:lang="en">Robbie Dhu Springs</dcterms:title>
            <dcterms:title xml:lang="ko">로비 듀 수원지</dcterms:title>
          </whisky:WaterSource>
        </whisky:waterSource>
        <owl:sameAs rdf:resource="http://dbpedia.org/resource/Glenfiddich_distillery"/>
      </bevon:Distillery>
    </bevon:distillery>
    <bevon:fermentation_base rdf:resource="http://dbpedia.org/resource/Barley"/>
    <bevon:launch rdf:datatype="http://www.w3.org/2001/XMLSchema#gYear">1887</bevon:launch>
    <bevon:manufacturer rdf:resource="http://dbpedia.org/resource/William_Grant_%26_Sons"/>
    <bevon:name xml:lang="en">Glenfiddich 12 Year Old</bevon:name>
    <bevon:name xml:lang="ko">글렌피딕 12년</bevon:name>
    <bevon:origin rdf:resource="http://dbpedia.org/resource/Strathspey,_Scotland"/>
    <rdf:type rdf:resource="http://purl.org/goodrelations/v1#ProductOrServiceModel"/>
    <rdf:type rdf:resource="http://rdfs.co/bevon/SpeysideSingleMalt"/>
  </owl:NamedIndividual>
  <owl:NamedIndividual rdf:about="http://rdfs.co/bevon/beverage/Guinness">
    <bevon:abv rdf:datatype="http://www.w3.org/2001/XMLSchema#decimal">4.2</bevon:abv>
    <bevon:container rdf:resource="http://rdfs.co/bevon/container/15lBeerKeg"/>
    <bevon:container rdf:resource="http://rdfs.co/bevon/container/30lBeerKeg"/>
    <bevon:container rdf:resource="http://rdfs.co/bevon/container/330mlBeverageCan"/>
    <bevon:container rdf:resource="http://rdfs.co/bevon/container/330mlLongneck"/>
    <bevon:description xml:lang="en">
    Guinness is a popular Irish dry stout that originated in the brewery of
    Arthur Guinness (1725–1803) at St. James's Gate, Dublin. Guinness is one
    of the most successful beer brands worldwide.
    </bevon:description>
    <bevon:fermentation_base rdf:resource="http://dbpedia.org/resource/Barley"/>
    <bevon:ibu rdf:datatype="http://www.w3.org/2001/XMLSchema#nonNegativeInteger">37</bevon:ibu>
    <bevon:launch rdf:datatype="http://www.w3.org/2001/XMLSchema#gYear">1759</bevon:launch>
    <bevon:manufacturer rdf:resource="http://dbpedia.org/resource/Diageo"/>
    <bevon:name xml:lang="en">Guinness Draught</bevon:name>
    <bevon:name xml:lang="ko">기네스 드래프트</bevon:name>
    <bevon:origin rdf:resource="http://dbpedia.org/resource/Dublin"/>
    <bevon:srm rdf:datatype="http://www.w3.org/2001/XMLSchema#nonNegativeInteger">32</bevon:srm>
    <rdf:type rdf:resource="http://purl.org/goodrelations/v1#ProductOrServiceModel"/>
    <rdf:type rdf:resource="http://rdfs.co/bevon/DryStout"/>
    <rdfs:seeAlso rdf:resource="http://en.wikipedia.org/wiki/Guinness"/>
    <owl:sameAs rdf:resource="http://dbpedia.org/resource/Guinness"/>
  </owl:NamedIndividual>
  <owl:NamedIndividual rdf:about="http://rdfs.co/bevon/beverage/Kilkenny">
    <bevon:abv rdf:datatype="http://www.w3.org/2001/XMLSchema#decimal">4.3</bevon:abv>
    <bevon:container rdf:resource="http://rdfs.co/bevon/container/30lBeerKeg"/>
    <bevon:container rdf:resource="http://rdfs.co/bevon/container/440mlBeverageCan"/>
    <bevon:description xml:lang="en">
    Kilkenny is a nitrogenated Irish cream ale from the makers of Guinness,
    which originated in Kilkenny, Ireland. The brand is managed and produced
    by Diageo. It is available in draught and cans. It is brewed in Ireland
    and its heritage dates back to the 14th century.
    </bevon:description>
    <bevon:fermentation_base rdf:resource="http://dbpedia.org/resource/Barley"/>
    <bevon:ibu rdf:datatype="http://www.w3.org/2001/XMLSchema#nonNegativeInteger">23</bevon:ibu>
    <bevon:launch rdf:datatype="http://www.w3.org/2001/XMLSchema#gYear">1710</bevon:launch>
    <bevon:manufacturer rdf:resource="http://dbpedia.org/resource/Diageo"/>
    <bevon:name xml:lang="en">Kilkenny Irish Cream Ale</bevon:name>
    <bevon:name xml:lang="ko">킬케니 아이리쉬 크림 에일</bevon:name>
    <bevon:origin rdf:resource="http://dbpedia.org/resource/Kilkenny"/>
    <bevon:similar rdf:resource="http://rdfs.co/bevon/beverage/Smithwicks"/>
    <bevon:srm rdf:datatype="http://www.w3.org/2001/XMLSchema#nonNegativeInteger">14</bevon:srm>
    <rdf:type rdf:resource="http://purl.org/goodrelations/v1#ProductOrServiceModel"/>
    <rdf:type rdf:resource="http://rdfs.co/bevon/IrishRedAle"/>
    <rdfs:seeAlso rdf:resource="http://en.wikipedia.org/wiki/Kilkenny_(beer)"/>
    <owl:sameAs rdf:resource="http://dbpedia.org/resource/Kilkenny_(beer)"/>
  </owl:NamedIndividual>
  <owl:NamedIndividual rdf:about="http://rdfs.co/bevon/beverage/KozelDark">
    <bevon:abv rdf:datatype="http://www.w3.org/2001/XMLSchema#decimal">3.8</bevon:abv>
    <bevon:container rdf:resource="http://rdfs.co/bevon/container/500mlLongneck"/>
    <bevon:description xml:lang="en">
    Velkopopovický Kozel Dark beer is brewed to the original recipe using a
    special mix of dark malts, clean water from our own well close to the
    brewery, and a selection of the best hops. The caramelized malt gives this
    beer a unique ruby color and sweet flavor, thanks to which it is
    appreciated and respected all over the world.
    </bevon:description>
    <bevon:fermentation_base rdf:resource="http://dbpedia.org/resource/Barley"/>
    <bevon:launch rdf:datatype="http://www.w3.org/2001/XMLSchema#gYear">1874</bevon:launch>
    <bevon:manufacturer rdf:resource="http://dbpedia.org/resource/SABMiller"/>
    <bevon:name xml:lang="en">Velkopopovický Kozel Dark</bevon:name>
    <bevon:name xml:lang="cs">Velkopopovický Kozel Černý</bevon:name>
    <bevon:name xml:lang="ko">코젤 다크</bevon:name>
    <bevon:origin rdf:resource="http://dbpedia.org/resource/Velké_Popovice"/>
    <rdf:type rdf:resource="http://purl.org/goodrelations/v1#ProductOrServiceModel"/>
    <rdf:type rdf:resource="http://rdfs.co/bevon/Dunkel"/>
  </owl:NamedIndividual>
  <owl:NamedIndividual rdf:about="http://rdfs.co/bevon/beverage/Smithwicks">
    <bevon:abv rdf:datatype="http://www.w3.org/2001/XMLSchema#decimal">3.8</bevon:abv>
    <bevon:color>
      <dbpedia:Colour>
        <dcterms:title xml:lang="en">Ruby Red</dcterms:title>
        <owl:sameAs rdf:resource="http://dbpedia.org/resource/Ruby_(color)__Ruby_Red__1"/>
        <owl:sameAs rdf:resource="http://purl.org/colors/rgb/9B111E"/>
      </dbpedia:Colour>
    </bevon:color>
    <bevon:container rdf:resource="http://rdfs.co/bevon/container/30lBeerKeg"/>
    <bevon:container rdf:resource="http://rdfs.co/bevon/container/330mlLongneck"/>
    <bevon:container rdf:resource="http://rdfs.co/bevon/container/440mlBeverageCan"/>
    <bevon:description xml:lang="en">
    Smithwick's is an Irish red ale style beer from Kilkenny, Ireland. It is a
    clear beer with a rich ruby color and creamy head.
    </bevon:description>
    <bevon:fermentation_base rdf:resource="http://dbpedia.org/resource/Barley"/>
    <bevon:ibu rdf:datatype="http://www.w3.org/2001/XMLSchema#nonNegativeInteger">20</bevon:ibu>
    <bevon:launch rdf:datatype="http://www.w3.org/2001/XMLSchema#gYear">1710</bevon:launch>
    <bevon:manufacturer rdf:resource="http://dbpedia.org/resource/Diageo"/>
    <bevon:name xml:lang="en">Smithwick's Superior Irish Ale</bevon:name>
    <bevon:name xml:lang="ko">스미딕스 슈페리어 아이리쉬 에일</bevon:name>
    <bevon:origin rdf:resource="http://dbpedia.org/resource/Kilkenny"/>
    <bevon:similar rdf:resource="http://rdfs.co/bevon/beverage/Kilkenny"/>
    <bevon:srm rdf:datatype="http://www.w3.org/2001/XMLSchema#nonNegativeInteger">14</bevon:srm>
    <rdf:type rdf:resource="http://purl.org/goodrelations/v1#ProductOrServiceModel"/>
    <rdf:type rdf:resource="http://rdfs.co/bevon/IrishRedAle"/>
    <rdfs:seeAlso rdf:resource="http://en.wikipedia.org/wiki/Smithwick%27s"/>
    <owl:sameAs rdf:resource="http://dbpedia.org/resource/Smithwick%27s"/>
  </owl:NamedIndividual>
  <owl:NamedIndividual rdf:about="http://rdfs.co/bevon/beverage/Tsingtao">
    <bevon:abv rdf:datatype="http://www.w3.org/2001/XMLSchema#decimal">4.7</bevon:abv>
    <bevon:brewery rdf:resource="http://dbpedia.org/resource/Tsingtao_Brewery"/>
    <bevon:container rdf:resource="http://rdfs.co/bevon/container/330mlLongneck"/>
    <bevon:container rdf:resource="http://rdfs.co/bevon/container/355mlBeverageCan"/>
    <bevon:container rdf:resource="http://rdfs.co/bevon/container/500mlBeverageCan"/>
    <bevon:container rdf:resource="http://rdfs.co/bevon/container/640mlLongneck"/>
    <bevon:description xml:lang="en">
    Tsingtao Lager, a well-hopped standard pilsner of 4.7% alcohol, is the
    flagship brew, accounting for most of the brewery's production.
    </bevon:description>
    <bevon:fermentation_base rdf:resource="http://dbpedia.org/resource/Barley"/>
    <bevon:ibu rdf:datatype="http://www.w3.org/2001/XMLSchema#nonNegativeInteger">20</bevon:ibu>
    <bevon:launch rdf:datatype="http://www.w3.org/2001/XMLSchema#gYear">1904</bevon:launch>
    <bevon:manufacturer rdf:resource="http://dbpedia.org/resource/Tsingtao_Brewery"/>
    <bevon:name xml:lang="en">Tsingtao Lager</bevon:name>
    <bevon:name xml:lang="ko">칭타오 라거</bevon:name>
    <bevon:origin rdf:resource="http://dbpedia.org/resource/Qingdao"/>
    <bevon:srm rdf:datatype="http://www.w3.org/2001/XMLSchema#nonNegativeInteger">4</bevon:srm>
    <rdf:type rdf:resource="http://purl.org/goodrelations/v1#ProductOrServiceModel"/>
    <rdf:type rdf:resource="http://rdfs.co/bevon/Pilsner"/>
  </owl:NamedIndividual>
  <owl:NamedIndividual rdf:about="http://rdfs.co/bevon/beverage/WhiskyAndSoda">
    <bevon:description xml:lang="en">
    Whisky &amp; Soda is a kind of mixed drinks that are composed of whisky and
    carbonated water.
    </bevon:description>
    <bevon:ingredient>
      <food:Ingredient>
        <bevon:food>
          <bevon:Whisky>
            <dcterms:title xml:lang="en">Whisky</dcterms:title>
            <owl:sameAs rdf:resource="http://dbpedia.org/resource/Whisky"/>
          </bevon:Whisky>
        </bevon:food>
        <bevon:quantity>
          <gr:QuantitativeValueInteger>
            <gr:hasUnitOfMeasurement>OZA</gr:hasUnitOfMeasurement>
            <gr:hasValue rdf:datatype="http://www.w3.org/2001/XMLSchema#int">2</gr:hasValue>
          </gr:QuantitativeValueInteger>
        </bevon:quantity>
      </food:Ingredient>
    </bevon:ingredient>
    <bevon:ingredient>
      <food:Ingredient>
        <bevon:food>
          <bevon:CarbonatedWater>
            <dcterms:title xml:lang="en">Carbonated Water</dcterms:title>
            <owl:sameAs rdf:resource="http://dbpedia.org/resource/Carbonated_water"/>
          </bevon:CarbonatedWater>
        </bevon:food>
      </food:Ingredient>
    </bevon:ingredient>
    <bevon:name xml:lang="en">Whisky &amp; Soda</bevon:name>
    <bevon:name xml:lang="ko">위스키 소다</bevon:name>
    <rdf:type rdf:resource="http://purl.org/goodrelations/v1#ProductOrServiceModel"/>
    <rdf:type rdf:resource="http://rdfs.co/bevon/Highball"/>
  </owl:NamedIndividual>
  <owl:ObjectProperty rdf:about="http://rdfs.co/bevon/brewery">
    <dcterms:issued rdf:datatype="http://www.w3.org/2001/XMLSchema#date">2013-07-04+09:00</dcterms:issued>
    <dcterms:modified rdf:datatype="http://www.w3.org/2001/XMLSchema#date">2014-03-01+09:00</dcterms:modified>
    <rdfs:domain rdf:resource="http://rdfs.co/bevon/Beer"/>
    <rdfs:isDefinedBy rdf:resource="http://rdfs.co/bevon/"/>
    <rdfs:range rdf:resource="http://rdfs.co/bevon/Brewery"/>
    <rdfs:seeAlso rdf:resource="http://en.wikipedia.org/wiki/Brewery"/>
    <status:term_status xml:lang="en">unstable</status:term_status>
    <skos:definition xml:lang="en">
    This property relates a beer to its brewery.
    </skos:definition>
    <skos:prefLabel xml:lang="en">Brewery</skos:prefLabel>
    <skos:prefLabel xml:lang="ko">양조장</skos:prefLabel>
  </owl:ObjectProperty>
  <owl:DatatypeProperty rdf:about="http://rdfs.co/bevon/color">
    <dcterms:issued rdf:datatype="http://www.w3.org/2001/XMLSchema#date">2013-07-04+09:00</dcterms:issued>
    <dcterms:modified rdf:datatype="http://www.w3.org/2001/XMLSchema#date">2014-03-01+09:00</dcterms:modified>
    <rdfs:domain rdf:resource="http://rdfs.co/bevon/Beverage"/>
    <rdfs:isDefinedBy rdf:resource="http://rdfs.co/bevon/"/>
    <rdfs:range rdf:resource="http://dbpedia.org/ontology/Colour"/>
    <status:term_status xml:lang="en">unstable</status:term_status>
    <skos:definition xml:lang="en">
    This property specifies the color of the beverage.
    </skos:definition>
    <skos:prefLabel xml:lang="en">color</skos:prefLabel>
    <skos:prefLabel xml:lang="ko">색상</skos:prefLabel>
  </owl:DatatypeProperty>
  <owl:ObjectProperty rdf:about="http://rdfs.co/bevon/container">
    <dcterms:issued rdf:datatype="http://www.w3.org/2001/XMLSchema#date">2013-07-04+09:00</dcterms:issued>
    <dcterms:modified rdf:datatype="http://www.w3.org/2001/XMLSchema#date">2014-03-01+09:00</dcterms:modified>
    <rdfs:domain rdf:resource="http://rdfs.co/bevon/Beverage"/>
    <rdfs:isDefinedBy rdf:resource="http://rdfs.co/bevon/"/>
    <rdfs:range rdf:resource="http://rdfs.co/bevon/Container"/>
    <status:term_status xml:lang="en">unstable</status:term_status>
    <skos:definition xml:lang="en">
    This property can be used to indicate that the beverage is available in a
    type of container.
    </skos:definition>
    <skos:prefLabel xml:lang="en">container</skos:prefLabel>
    <skos:prefLabel xml:lang="ko">용기</skos:prefLabel>
  </owl:ObjectProperty>
  <owl:NamedIndividual rdf:about="http://rdfs.co/bevon/container/15lBeerKeg">
    <bevon:volume>
      <gr:QuantitativeValueInteger>
        <gr:hasUnitOfMeasurement>LTR</gr:hasUnitOfMeasurement>
        <gr:hasValue rdf:datatype="http://www.w3.org/2001/XMLSchema#int">15</gr:hasValue>
      </gr:QuantitativeValueInteger>
    </bevon:volume>
    <rdf:type rdf:resource="http://rdfs.co/bevon/BeerKeg"/>
    <skos:prefLabel xml:lang="en">15l Beer Keg</skos:prefLabel>
    <skos:prefLabel xml:lang="ko">15l 맥주 케그</skos:prefLabel>
  </owl:NamedIndividual>
  <owl:NamedIndividual rdf:about="http://rdfs.co/bevon/container/1_8lPlasticBottle">
    <bevon:volume>
      <gr:QuantitativeValueFloat>
        <gr:hasUnitOfMeasurement>LTR</gr:hasUnitOfMeasurement>
        <gr:hasValue rdf:datatype="http://www.w3.org/2001/XMLSchema#float">1.8</gr:hasValue>
      </gr:QuantitativeValueFloat>
    </bevon:volume>
    <rdf:type rdf:resource="http://rdfs.co/bevon/PlasticBottle"/>
    <skos:prefLabel xml:lang="en">1.8l Plastic Bottle</skos:prefLabel>
    <skos:prefLabel xml:lang="ko">1.8l 플라스틱 병</skos:prefLabel>
  </owl:NamedIndividual>
  <owl:NamedIndividual rdf:about="http://rdfs.co/bevon/container/200mlPlasticBottle">
    <bevon:volume>
      <gr:QuantitativeValueInteger>
        <gr:hasUnitOfMeasurement>MLT</gr:hasUnitOfMeasurement>
        <gr:hasValue rdf:datatype="http://www.w3.org/2001/XMLSchema#int">200</gr:hasValue>
      </gr:QuantitativeValueInteger>
    </bevon:volume>
    <rdf:type rdf:resource="http://rdfs.co/bevon/PlasticBottle"/>
    <skos:prefLabel xml:lang="en">200ml Plastic Bottle</skos:prefLabel>
    <skos:prefLabel xml:lang="ko">200ml 플라스틱 병</skos:prefLabel>
  </owl:NamedIndividual>
  <owl:NamedIndividual rdf:about="http://rdfs.co/bevon/container/25lBeerKeg">
    <bevon:volume>
      <gr:QuantitativeValueInteger>
        <gr:hasUnitOfMeasurement>LTR</gr:hasUnitOfMeasurement>
        <gr:hasValue rdf:datatype="http://www.w3.org/2001/XMLSchema#int">25</gr:hasValue>
      </gr:QuantitativeValueInteger>
    </bevon:volume>
    <rdf:type rdf:resource="http://rdfs.co/bevon/BeerKeg"/>
    <skos:prefLabel xml:lang="en">25l Beer Keg</skos:prefLabel>
    <skos:prefLabel xml:lang="ko">25l 맥주 케그</skos:prefLabel>
  </owl:NamedIndividual>
  <owl:NamedIndividual rdf:about="http://rdfs.co/bevon/container/30lBeerKeg">
    <bevon:volume>
      <gr:QuantitativeValueInteger>
        <gr:hasUnitOfMeasurement>LTR</gr:hasUnitOfMeasurement>
        <gr:hasValue rdf:datatype="http://www.w3.org/2001/XMLSchema#int">30</gr:hasValue>
      </gr:QuantitativeValueInteger>
    </bevon:volume>
    <rdf:type rdf:resource="http://rdfs.co/bevon/BeerKeg"/>
    <skos:prefLabel xml:lang="en">30l Beer Keg</skos:prefLabel>
    <skos:prefLabel xml:lang="ko">30l 맥주 케그</skos:prefLabel>
  </owl:NamedIndividual>
  <owl:NamedIndividual rdf:about="http://rdfs.co/bevon/container/330mlBeverageCan">
    <bevon:volume>
      <gr:QuantitativeValueInteger>
        <gr:hasUnitOfMeasurement>MLT</gr:hasUnitOfMeasurement>
        <gr:hasValue rdf:datatype="http://www.w3.org/2001/XMLSchema#int">330</gr:hasValue>
      </gr:QuantitativeValueInteger>
    </bevon:volume>
    <rdf:type rdf:resource="http://rdfs.co/bevon/BeverageCan"/>
    <skos:prefLabel xml:lang="en">330ml Beverage Can</skos:prefLabel>
    <skos:prefLabel xml:lang="ko">330ml 음료 캔</skos:prefLabel>
  </owl:NamedIndividual>
  <owl:NamedIndividual rdf:about="http://rdfs.co/bevon/container/330mlLongneck">
    <bevon:volume>
      <gr:QuantitativeValueInteger>
        <gr:hasUnitOfMeasurement>MLT</gr:hasUnitOfMeasurement>
        <gr:hasValue rdf:datatype="http://www.w3.org/2001/XMLSchema#int">330</gr:hasValue>
      </gr:QuantitativeValueInteger>
    </bevon:volume>
    <rdf:type rdf:resource="http://rdfs.co/bevon/Longneck"/>
    <skos:prefLabel xml:lang="en">330ml Longneck Bottle</skos:prefLabel>
    <skos:prefLabel xml:lang="ko">330ml 긴목 맥주병</skos:prefLabel>
  </owl:NamedIndividual>
  <owl:NamedIndividual rdf:about="http://rdfs.co/bevon/container/355mlBeverageCan">
    <bevon:volume>
      <gr:QuantitativeValueInteger>
        <gr:hasUnitOfMeasurement>MLT</gr:hasUnitOfMeasurement>
        <gr:hasValue rdf:datatype="http://www.w3.org/2001/XMLSchema#int">355</gr:hasValue>
      </gr:QuantitativeValueInteger>
    </bevon:volume>
    <rdf:type rdf:resource="http://rdfs.co/bevon/BeverageCan"/>
    <skos:prefLabel xml:lang="en">355ml Beverage Can</skos:prefLabel>
    <skos:prefLabel xml:lang="ko">355ml 음료 캔</skos:prefLabel>
  </owl:NamedIndividual>
  <owl:NamedIndividual rdf:about="http://rdfs.co/bevon/container/360mlGlassBottle">
    <bevon:volume>
      <gr:QuantitativeValueInteger>
        <gr:hasUnitOfMeasurement>MLT</gr:hasUnitOfMeasurement>
        <gr:hasValue rdf:datatype="http://www.w3.org/2001/XMLSchema#int">360</gr:hasValue>
      </gr:QuantitativeValueInteger>
    </bevon:volume>
    <rdf:type rdf:resource="http://rdfs.co/bevon/GlassBottle"/>
    <skos:prefLabel xml:lang="en">360ml Glass Bottle</skos:prefLabel>
    <skos:prefLabel xml:lang="ko">360ml 유리병</skos:prefLabel>
  </owl:NamedIndividual>
  <owl:NamedIndividual rdf:about="http://rdfs.co/bevon/container/360mlPlasticBottle">
    <bevon:volume>
      <gr:QuantitativeValueInteger>
        <gr:hasUnitOfMeasurement>MLT</gr:hasUnitOfMeasurement>
        <gr:hasValue rdf:datatype="http://www.w3.org/2001/XMLSchema#int">360</gr:hasValue>
      </gr:QuantitativeValueInteger>
    </bevon:volume>
    <rdf:type rdf:resource="http://rdfs.co/bevon/PlasticBottle"/>
    <skos:prefLabel xml:lang="en">360ml Plastic Bottle</skos:prefLabel>
    <skos:prefLabel xml:lang="ko">360ml 플라스틱 병</skos:prefLabel>
  </owl:NamedIndividual>
  <owl:NamedIndividual rdf:about="http://rdfs.co/bevon/container/440mlBeverageCan">
    <bevon:volume>
      <gr:QuantitativeValueInteger>
        <gr:hasUnitOfMeasurement>MLT</gr:hasUnitOfMeasurement>
        <gr:hasValue rdf:datatype="http://www.w3.org/2001/XMLSchema#int">440</gr:hasValue>
      </gr:QuantitativeValueInteger>
    </bevon:volume>
    <rdf:type rdf:resource="http://rdfs.co/bevon/BeverageCan"/>
    <skos:prefLabel xml:lang="en">440ml Beverage Can</skos:prefLabel>
    <skos:prefLabel xml:lang="ko">440ml 음료 캔</skos:prefLabel>
  </owl:NamedIndividual>
  <owl:NamedIndividual rdf:about="http://rdfs.co/bevon/container/500mlBeverageCan">
    <bevon:volume>
      <gr:QuantitativeValueInteger>
        <gr:hasUnitOfMeasurement>MLT</gr:hasUnitOfMeasurement>
        <gr:hasValue rdf:datatype="http://www.w3.org/2001/XMLSchema#int">500</gr:hasValue>
      </gr:QuantitativeValueInteger>
    </bevon:volume>
    <rdf:type rdf:resource="http://rdfs.co/bevon/BeverageCan"/>
    <skos:prefLabel xml:lang="en">500ml Beverage Can</skos:prefLabel>
    <skos:prefLabel xml:lang="ko">500ml 음료 캔</skos:prefLabel>
  </owl:NamedIndividual>
  <owl:NamedIndividual rdf:about="http://rdfs.co/bevon/container/500mlLongneck">
    <bevon:volume>
      <gr:QuantitativeValueInteger>
        <gr:hasUnitOfMeasurement>MLT</gr:hasUnitOfMeasurement>
        <gr:hasValue rdf:datatype="http://www.w3.org/2001/XMLSchema#int">500</gr:hasValue>
      </gr:QuantitativeValueInteger>
    </bevon:volume>
    <rdf:type rdf:resource="http://rdfs.co/bevon/Longneck"/>
    <skos:prefLabel xml:lang="en">500ml Longneck Bottle</skos:prefLabel>
    <skos:prefLabel xml:lang="ko">500ml 긴목 맥주병</skos:prefLabel>
  </owl:NamedIndividual>
  <owl:NamedIndividual rdf:about="http://rdfs.co/bevon/container/50lBeerKeg">
    <bevon:volume>
      <gr:QuantitativeValueInteger>
        <gr:hasUnitOfMeasurement>LTR</gr:hasUnitOfMeasurement>
        <gr:hasValue rdf:datatype="http://www.w3.org/2001/XMLSchema#int">50</gr:hasValue>
      </gr:QuantitativeValueInteger>
    </bevon:volume>
    <rdf:type rdf:resource="http://rdfs.co/bevon/BeerKeg"/>
    <skos:prefLabel xml:lang="en">50l Beer Keg</skos:prefLabel>
    <skos:prefLabel xml:lang="ko">50l 맥주 케그</skos:prefLabel>
  </owl:NamedIndividual>
  <owl:NamedIndividual rdf:about="http://rdfs.co/bevon/container/640mlLongneck">
    <bevon:volume>
      <gr:QuantitativeValueInteger>
        <gr:hasUnitOfMeasurement>MLT</gr:hasUnitOfMeasurement>
        <gr:hasValue rdf:datatype="http://www.w3.org/2001/XMLSchema#int">640</gr:hasValue>
      </gr:QuantitativeValueInteger>
    </bevon:volume>
    <rdf:type rdf:resource="http://rdfs.co/bevon/Longneck"/>
    <skos:prefLabel xml:lang="en">640ml Longneck Bottle</skos:prefLabel>
    <skos:prefLabel xml:lang="ko">640ml 긴목 맥주병</skos:prefLabel>
  </owl:NamedIndividual>
  <owl:NamedIndividual rdf:about="http://rdfs.co/bevon/container/640mlPlasticBottle">
    <bevon:volume>
      <gr:QuantitativeValueInteger>
        <gr:hasUnitOfMeasurement>MLT</gr:hasUnitOfMeasurement>
        <gr:hasValue rdf:datatype="http://www.w3.org/2001/XMLSchema#int">640</gr:hasValue>
      </gr:QuantitativeValueInteger>
    </bevon:volume>
    <rdf:type rdf:resource="http://rdfs.co/bevon/PlasticBottle"/>
    <skos:prefLabel xml:lang="en">640ml Plastic Bottle</skos:prefLabel>
    <skos:prefLabel xml:lang="ko">640ml 플라스틱 병</skos:prefLabel>
  </owl:NamedIndividual>
  <owl:NamedIndividual rdf:about="http://rdfs.co/bevon/container/700mlGlassBottle">
    <bevon:volume>
      <gr:QuantitativeValueInteger>
        <gr:hasUnitOfMeasurement>MLT</gr:hasUnitOfMeasurement>
        <gr:hasValue rdf:datatype="http://www.w3.org/2001/XMLSchema#int">700</gr:hasValue>
      </gr:QuantitativeValueInteger>
    </bevon:volume>
    <rdf:type rdf:resource="http://rdfs.co/bevon/GlassBottle"/>
    <skos:altLabel xml:lang="en">70cl Glass Bottle</skos:altLabel>
    <skos:prefLabel xml:lang="en">700ml Glass Bottle</skos:prefLabel>
    <skos:prefLabel xml:lang="ko">700ml 유리병</skos:prefLabel>
  </owl:NamedIndividual>
  <owl:NamedIndividual rdf:about="http://rdfs.co/bevon/container/750mlGlassBottle">
    <bevon:volume>
      <gr:QuantitativeValueInteger>
        <gr:hasUnitOfMeasurement>MLT</gr:hasUnitOfMeasurement>
        <gr:hasValue rdf:datatype="http://www.w3.org/2001/XMLSchema#int">750</gr:hasValue>
      </gr:QuantitativeValueInteger>
    </bevon:volume>
    <rdf:type rdf:resource="http://rdfs.co/bevon/GlassBottle"/>
    <skos:altLabel xml:lang="en">75cl Glass Bottle</skos:altLabel>
    <skos:prefLabel xml:lang="en">750ml Glass Bottle</skos:prefLabel>
    <skos:prefLabel xml:lang="ko">750ml 유리병</skos:prefLabel>
  </owl:NamedIndividual>
  <owl:DatatypeProperty rdf:about="http://rdfs.co/bevon/description">
    <dcterms:issued rdf:datatype="http://www.w3.org/2001/XMLSchema#date">2013-07-04+09:00</dcterms:issued>
    <dcterms:modified rdf:datatype="http://www.w3.org/2001/XMLSchema#date">2014-03-01+09:00</dcterms:modified>
    <rdfs:domain rdf:resource="http://rdfs.co/bevon/Beverage"/>
    <rdfs:isDefinedBy rdf:resource="http://rdfs.co/bevon/"/>
    <rdfs:range rdf:resource="http://www.w3.org/2001/XMLSchema#string"/>
    <rdfs:subPropertyOf rdf:resource="http://purl.org/dc/terms/description"/>
    <rdfs:subPropertyOf rdf:resource="http://purl.org/goodrelations/v1#description"/>
    <status:term_status xml:lang="en">testing</status:term_status>
    <skos:definition xml:lang="en">
    This property specifies the short text description of the beverage.
    </skos:definition>
    <skos:prefLabel xml:lang="en">description</skos:prefLabel>
    <skos:prefLabel xml:lang="ko">설명</skos:prefLabel>
  </owl:DatatypeProperty>
  <owl:ObjectProperty rdf:about="http://rdfs.co/bevon/distillery">
    <dcterms:issued rdf:datatype="http://www.w3.org/2001/XMLSchema#date">2013-07-04+09:00</dcterms:issued>
    <dcterms:modified rdf:datatype="http://www.w3.org/2001/XMLSchema#date">2014-03-01+09:00</dcterms:modified>
    <rdfs:domain rdf:resource="http://rdfs.co/bevon/DistilledBeverage"/>
    <rdfs:isDefinedBy rdf:resource="http://rdfs.co/bevon/"/>
    <rdfs:range rdf:resource="http://rdfs.co/bevon/Distillery"/>
    <rdfs:seeAlso rdf:resource="http://en.wikipedia.org/wiki/Distillation"/>
    <status:term_status xml:lang="en">unstable</status:term_status>
    <skos:definition xml:lang="en">
    This property relates a distilled beverage to its distillery.
    </skos:definition>
    <skos:prefLabel xml:lang="en">Distillery</skos:prefLabel>
    <skos:prefLabel xml:lang="ko">증류소</skos:prefLabel>
  </owl:ObjectProperty>
  <owl:ObjectProperty rdf:about="http://rdfs.co/bevon/duration">
    <dcterms:issued rdf:datatype="http://www.w3.org/2001/XMLSchema#date">2013-07-04+09:00</dcterms:issued>
    <dcterms:modified rdf:datatype="http://www.w3.org/2001/XMLSchema#date">2014-03-01+09:00</dcterms:modified>
    <rdfs:domain rdf:resource="http://rdfs.co/bevon/Aging"/>
    <rdfs:isDefinedBy rdf:resource="http://rdfs.co/bevon/"/>
    <rdfs:range rdf:resource="http://www.w3.org/2006/time#DurationDescription"/>
    <rdfs:subPropertyOf rdf:resource="http://www.w3.org/2006/time#hasDurationDescription"/>
    <status:term_status xml:lang="en">unstable</status:term_status>
    <skos:definition xml:lang="en">
    This property describes how long the beverage was aged in the cask.
    </skos:definition>
    <skos:prefLabel xml:lang="en">duration</skos:prefLabel>
    <skos:prefLabel xml:lang="ko">기간</skos:prefLabel>
  </owl:ObjectProperty>
  <owl:ObjectProperty rdf:about="http://rdfs.co/bevon/fermentation_base">
    <dcterms:issued rdf:datatype="http://www.w3.org/2001/XMLSchema#date">2013-07-04+09:00</dcterms:issued>
    <dcterms:modified rdf:datatype="http://www.w3.org/2001/XMLSchema#date">2014-03-01+09:00</dcterms:modified>
    <rdfs:domain rdf:resource="http://rdfs.co/bevon/AlcoholicBeverage"/>
    <rdfs:isDefinedBy rdf:resource="http://rdfs.co/bevon/"/>
    <rdfs:range rdf:resource="http://rdfs.co/bevon/FermentationBase"/>
    <status:term_status xml:lang="en">unstable</status:term_status>
    <skos:definition xml:lang="en">
    This property indicates which fermentation base is used to make the
    alcoholic beverage.
    </skos:definition>
    <skos:prefLabel xml:lang="en">fermentation base</skos:prefLabel>
    <skos:prefLabel xml:lang="ko">발효 주재료</skos:prefLabel>
  </owl:ObjectProperty>
  <owl:ObjectProperty rdf:about="http://rdfs.co/bevon/food">
    <dcterms:issued rdf:datatype="http://www.w3.org/2001/XMLSchema#date">2013-07-04+09:00</dcterms:issued>
    <dcterms:modified rdf:datatype="http://www.w3.org/2001/XMLSchema#date">2014-03-01+09:00</dcterms:modified>
    <rdfs:domain rdf:resource="http://data.lirmm.fr/ontologies/food#Ingredient"/>
    <rdfs:isDefinedBy rdf:resource="http://rdfs.co/bevon/"/>
    <rdfs:range rdf:resource="http://data.lirmm.fr/ontologies/food#Food"/>
    <rdfs:subPropertyOf rdf:resource="http://data.lirmm.fr/ontologies/food#food"/>
    <status:term_status xml:lang="en">unstable</status:term_status>
    <skos:definition xml:lang="en">
    This property describes food that is an ingredient of a mixed drink.
    </skos:definition>
    <skos:prefLabel xml:lang="en">food</skos:prefLabel>
    <skos:prefLabel xml:lang="ko">음식</skos:prefLabel>
  </owl:ObjectProperty>
  <owl:DatatypeProperty rdf:about="http://rdfs.co/bevon/ibu">
    <dcterms:issued rdf:datatype="http://www.w3.org/2001/XMLSchema#date">2013-07-04+09:00</dcterms:issued>
    <dcterms:modified rdf:datatype="http://www.w3.org/2001/XMLSchema#date">2014-03-01+09:00</dcterms:modified>
    <rdfs:domain rdf:resource="http://rdfs.co/bevon/Beer"/>
    <rdfs:isDefinedBy rdf:resource="http://rdfs.co/bevon/"/>
    <rdfs:range rdf:resource="http://www.w3.org/2001/XMLSchema#nonNegativeInteger"/>
    <rdfs:seeAlso rdf:resource="http://en.wikipedia.org/wiki/International_Bitterness_Units_scale"/>
    <status:term_status xml:lang="en">unstable</status:term_status>
    <skos:altLabel xml:lang="en">International Bitterness Unit scale</skos:altLabel>
    <skos:definition xml:lang="en">
    The International Bittering Units scale, or simply IBU scale, provides a
    measure of the bitterness of beer, which is provided by the hops used
    during brewing.
    </skos:definition>
    <skos:prefLabel xml:lang="en">IBU scale</skos:prefLabel>
    <skos:prefLabel xml:lang="ko">IBU 척도</skos:prefLabel>
  </owl:DatatypeProperty>
  <owl:ObjectProperty rdf:about="http://rdfs.co/bevon/ingredient">
    <dcterms:issued rdf:datatype="http://www.w3.org/2001/XMLSchema#date">2013-07-04+09:00</dcterms:issued>
    <dcterms:modified rdf:datatype="http://www.w3.org/2001/XMLSchema#date">2014-03-01+09:00</dcterms:modified>
    <rdfs:domain rdf:resource="http://rdfs.co/bevon/MixedDrink"/>
    <rdfs:isDefinedBy rdf:resource="http://rdfs.co/bevon/"/>
    <rdfs:range rdf:resource="http://data.lirmm.fr/ontologies/food#Ingredient"/>
    <rdfs:subPropertyOf rdf:resource="http://data.lirmm.fr/ontologies/food#containsIngredient"/>
    <status:term_status xml:lang="en">unstable</status:term_status>
    <skos:definition xml:lang="en">
    This property specifies an ingredient of the mixed drink.
    </skos:definition>
    <skos:prefLabel xml:lang="en">ingredient</skos:prefLabel>
    <skos:prefLabel xml:lang="ko">재료</skos:prefLabel>
  </owl:ObjectProperty>
  <owl:DatatypeProperty rdf:about="http://rdfs.co/bevon/launch">
    <dcterms:issued rdf:datatype="http://www.w3.org/2001/XMLSchema#date">2013-07-04+09:00</dcterms:issued>
    <dcterms:modified rdf:datatype="http://www.w3.org/2001/XMLSchema#date">2014-03-01+09:00</dcterms:modified>
    <rdfs:domain rdf:resource="http://rdfs.co/bevon/Beverage"/>
    <rdfs:isDefinedBy rdf:resource="http://rdfs.co/bevon/"/>
    <rdfs:range rdf:resource="http://www.w3.org/2001/XMLSchema#gYear"/>
    <status:term_status xml:lang="en">unstable</status:term_status>
    <skos:definition xml:lang="en">
    This property specifies the year when the beverage was first introduced to
    the market.
    </skos:definition>
    <skos:prefLabel xml:lang="en">launch</skos:prefLabel>
    <skos:prefLabel xml:lang="ko">출시년도</skos:prefLabel>
  </owl:DatatypeProperty>
  <owl:ObjectProperty rdf:about="http://rdfs.co/bevon/manufacturer">
    <dcterms:issued rdf:datatype="http://www.w3.org/2001/XMLSchema#date">2013-07-04+09:00</dcterms:issued>
    <dcterms:modified rdf:datatype="http://www.w3.org/2001/XMLSchema#date">2014-03-01+09:00</dcterms:modified>
    <rdfs:domain rdf:resource="http://rdfs.co/bevon/Beverage"/>
    <rdfs:isDefinedBy rdf:resource="http://rdfs.co/bevon/"/>
    <rdfs:range rdf:resource="http://xmlns.com/foaf/0.1/Agent"/>
    <rdfs:subPropertyOf rdf:resource="http://purl.org/goodrelations/v1#hasManufacturer"/>
    <status:term_status xml:lang="en">unstable</status:term_status>
    <skos:definition xml:lang="en">
    This property specifies the manufacturer of the beverage.
    </skos:definition>
    <skos:prefLabel xml:lang="en">manufacturer</skos:prefLabel>
    <skos:prefLabel xml:lang="ko">제조사</skos:prefLabel>
  </owl:ObjectProperty>
  <owl:ObjectProperty rdf:about="http://rdfs.co/bevon/material">
    <dcterms:issued rdf:datatype="http://www.w3.org/2001/XMLSchema#date">2013-07-04+09:00</dcterms:issued>
    <dcterms:modified rdf:datatype="http://www.w3.org/2001/XMLSchema#date">2014-03-01+09:00</dcterms:modified>
    <rdfs:domain rdf:resource="http://rdfs.co/bevon/Aging"/>
    <rdfs:isDefinedBy rdf:resource="http://rdfs.co/bevon/"/>
    <status:term_status xml:lang="en">unstable</status:term_status>
    <skos:definition xml:lang="en">
    This property specifies what the aging cask was made of.
    </skos:definition>
    <skos:prefLabel xml:lang="en">material</skos:prefLabel>
    <skos:prefLabel xml:lang="ko">소재</skos:prefLabel>
  </owl:ObjectProperty>
  <owl:DatatypeProperty rdf:about="http://rdfs.co/bevon/name">
    <dcterms:issued rdf:datatype="http://www.w3.org/2001/XMLSchema#date">2013-07-04+09:00</dcterms:issued>
    <dcterms:modified rdf:datatype="http://www.w3.org/2001/XMLSchema#date">2014-03-01+09:00</dcterms:modified>
    <rdfs:domain rdf:resource="http://rdfs.co/bevon/Beverage"/>
    <rdfs:isDefinedBy rdf:resource="http://rdfs.co/bevon/"/>
    <rdfs:range rdf:resource="http://www.w3.org/2001/XMLSchema#string"/>
    <rdfs:subPropertyOf rdf:resource="http://purl.org/dc/terms/title"/>
    <rdfs:subPropertyOf rdf:resource="http://purl.org/goodrelations/v1#name"/>
    <rdfs:subPropertyOf rdf:resource="http://xmlns.com/foaf/0.1/name"/>
    <status:term_status xml:lang="en">testing</status:term_status>
    <skos:definition xml:lang="en">
    This property indicates the name of the beverage.
    </skos:definition>
    <skos:prefLabel xml:lang="en">name</skos:prefLabel>
    <skos:prefLabel xml:lang="ko">이름</skos:prefLabel>
  </owl:DatatypeProperty>
  <owl:ObjectProperty rdf:about="http://rdfs.co/bevon/non_alcoholic_version">
    <dcterms:issued rdf:datatype="http://www.w3.org/2001/XMLSchema#date">2013-07-04+09:00</dcterms:issued>
    <dcterms:modified rdf:datatype="http://www.w3.org/2001/XMLSchema#date">2014-03-01+09:00</dcterms:modified>
    <rdfs:domain rdf:resource="http://rdfs.co/bevon/AlcoholicBeverage"/>
    <rdfs:isDefinedBy rdf:resource="http://rdfs.co/bevon/"/>
    <rdfs:range rdf:resource="http://rdfs.co/bevon/NonAlcoholicBeverage"/>
    <rdfs:subPropertyOf rdf:resource="http://rdfs.co/bevon/related"/>
    <status:term_status xml:lang="en">unstable</status:term_status>
    <skos:definition xml:lang="en">
    Some alcoholic beverages have non-alcoholic versions, such as non-alcoholic
    beer ("near beer") and cocktails ("mocktails").
    </skos:definition>
    <skos:prefLabel xml:lang="en">non-alcoholic version</skos:prefLabel>
    <skos:prefLabel xml:lang="ko">비알코올 버전</skos:prefLabel>
  </owl:ObjectProperty>
  <owl:ObjectProperty rdf:about="http://rdfs.co/bevon/origin">
    <dcterms:issued rdf:datatype="http://www.w3.org/2001/XMLSchema#date">2013-07-04+09:00</dcterms:issued>
    <dcterms:modified rdf:datatype="http://www.w3.org/2001/XMLSchema#date">2014-03-01+09:00</dcterms:modified>
    <rdfs:domain rdf:resource="http://rdfs.co/bevon/Beverage"/>
    <rdfs:isDefinedBy rdf:resource="http://rdfs.co/bevon/"/>
    <rdfs:range rdf:resource="http://dbpedia.org/ontology/Place"/>
    <status:term_status xml:lang="en">unstable</status:term_status>
    <skos:definition xml:lang="en">
    This property indicates the place where the beverage was first invented.
    </skos:definition>
    <skos:prefLabel xml:lang="en">origin</skos:prefLabel>
    <skos:prefLabel xml:lang="ko">원산지</skos:prefLabel>
  </owl:ObjectProperty>
  <owl:ObjectProperty rdf:about="http://rdfs.co/bevon/previous_content">
    <dcterms:issued rdf:datatype="http://www.w3.org/2001/XMLSchema#date">2013-07-04+09:00</dcterms:issued>
    <dcterms:modified rdf:datatype="http://www.w3.org/2001/XMLSchema#date">2014-03-01+09:00</dcterms:modified>
    <rdfs:domain rdf:resource="http://rdfs.co/bevon/Aging"/>
    <rdfs:isDefinedBy rdf:resource="http://rdfs.co/bevon/"/>
    <rdfs:range rdf:resource="http://www.w3.org/TR/2003/PR-owl-guide-20031209/food#PotableLiquid"/>
    <status:term_status xml:lang="en">unstable</status:term_status>
    <skos:definition xml:lang="en">
    This property specifies what as in the cask before the aging.
    </skos:definition>
    <skos:prefLabel xml:lang="en">previous content</skos:prefLabel>
    <skos:prefLabel xml:lang="ko">이전 내용물</skos:prefLabel>
  </owl:ObjectProperty>
  <owl:DatatypeProperty rdf:about="http://rdfs.co/bevon/proof">
    <dcterms:issued rdf:datatype="http://www.w3.org/2001/XMLSchema#date">2013-07-04+09:00</dcterms:issued>
    <dcterms:modified rdf:datatype="http://www.w3.org/2001/XMLSchema#date">2014-03-01+09:00</dcterms:modified>
    <rdfs:comment xml:lang="en">
    The term was originally used in the United Kingdom and was defined as 7/4
    times the alcohol by volume (ABV). The UK now uses the ABV standard instead
    of alcohol proof. In the United States, alcoholic proof is defined as twice
    the percentage of ABV.
    </rdfs:comment>
    <rdfs:domain rdf:resource="http://rdfs.co/bevon/Beverage"/>
    <rdfs:isDefinedBy rdf:resource="http://rdfs.co/bevon/"/>
    <rdfs:range rdf:resource="http://www.w3.org/2001/XMLSchema#decimal"/>
    <rdfs:seeAlso rdf:resource="http://en.wikipedia.org/wiki/Alcohol_proof"/>
    <status:term_status xml:lang="en">unstable</status:term_status>
    <skos:altLabel xml:lang="en">alcohol proof</skos:altLabel>
    <skos:definition xml:lang="en">
    Alcohol proof is a measure of how much alcohol (ethanol) is contained in an
    alcoholic beverage.
    </skos:definition>
    <skos:prefLabel xml:lang="en">proof</skos:prefLabel>
    <skos:prefLabel xml:lang="ko">프루프</skos:prefLabel>
  </owl:DatatypeProperty>
  <owl:ObjectProperty rdf:about="http://rdfs.co/bevon/quantity">
    <dcterms:issued rdf:datatype="http://www.w3.org/2001/XMLSchema#date">2013-07-04+09:00</dcterms:issued>
    <dcterms:modified rdf:datatype="http://www.w3.org/2001/XMLSchema#date">2014-03-01+09:00</dcterms:modified>
    <rdfs:domain rdf:resource="http://data.lirmm.fr/ontologies/food#Ingredient"/>
    <rdfs:isDefinedBy rdf:resource="http://rdfs.co/bevon/"/>
    <rdfs:range rdf:resource="http://purl.org/goodrelations/v1#QuantitativeValue"/>
    <status:term_status xml:lang="en">unstable</status:term_status>
    <skos:definition xml:lang="en">
    This property specifies the quantity of the ingredient with a type
    in the UN/CEFACT Common Code.
    </skos:definition>
    <skos:prefLabel xml:lang="en">quantity</skos:prefLabel>
    <skos:prefLabel xml:lang="ko">양</skos:prefLabel>
  </owl:ObjectProperty>
  <owl:ObjectProperty rdf:about="http://rdfs.co/bevon/related">
    <dcterms:issued rdf:datatype="http://www.w3.org/2001/XMLSchema#date">2013-07-04+09:00</dcterms:issued>
    <dcterms:modified rdf:datatype="http://www.w3.org/2001/XMLSchema#date">2014-03-01+09:00</dcterms:modified>
    <rdfs:domain rdf:resource="http://rdfs.co/bevon/Beverage"/>
    <rdfs:isDefinedBy rdf:resource="http://rdfs.co/bevon/"/>
    <rdfs:range rdf:resource="http://rdfs.co/bevon/Beverage"/>
    <status:term_status xml:lang="en">unstable</status:term_status>
    <skos:definition xml:lang="en">
    This property states that a beverage is related to another beverage.
    </skos:definition>
    <skos:prefLabel xml:lang="en">related</skos:prefLabel>
    <skos:prefLabel xml:lang="ko">연관</skos:prefLabel>
  </owl:ObjectProperty>
  <owl:SymmetricProperty rdf:about="http://rdfs.co/bevon/similar">
    <dcterms:issued rdf:datatype="http://www.w3.org/2001/XMLSchema#date">2013-07-04+09:00</dcterms:issued>
    <dcterms:modified rdf:datatype="http://www.w3.org/2001/XMLSchema#date">2014-03-01+09:00</dcterms:modified>
    <rdfs:domain rdf:resource="http://rdfs.co/bevon/Beverage"/>
    <rdfs:isDefinedBy rdf:resource="http://rdfs.co/bevon/"/>
    <rdfs:range rdf:resource="http://rdfs.co/bevon/Beverage"/>
    <rdfs:subPropertyOf rdf:resource="http://purl.org/goodrelations/v1#isSimilarTo"/>
    <rdfs:subPropertyOf rdf:resource="http://rdfs.co/bevon/related"/>
    <status:term_status xml:lang="en">unstable</status:term_status>
    <skos:definition xml:lang="en">
    This property states that a beverage is similar to another beverage.
    </skos:definition>
    <skos:prefLabel xml:lang="en">similar</skos:prefLabel>
    <skos:prefLabel xml:lang="ko">유사</skos:prefLabel>
  </owl:SymmetricProperty>
  <owl:DatatypeProperty rdf:about="http://rdfs.co/bevon/srm">
    <dcterms:issued rdf:datatype="http://www.w3.org/2001/XMLSchema#date">2013-07-04+09:00</dcterms:issued>
    <dcterms:modified rdf:datatype="http://www.w3.org/2001/XMLSchema#date">2014-03-01+09:00</dcterms:modified>
    <rdfs:domain rdf:resource="http://rdfs.co/bevon/Beer"/>
    <rdfs:isDefinedBy rdf:resource="http://rdfs.co/bevon/"/>
    <rdfs:range rdf:resource="http://www.w3.org/2001/XMLSchema#nonNegativeInteger"/>
    <rdfs:seeAlso rdf:resource="http://en.wikipedia.org/wiki/Standard_Reference_Method"/>
    <status:term_status xml:lang="en">unstable</status:term_status>
    <skos:altLabel xml:lang="en">Standard Reference Method</skos:altLabel>
    <skos:definition xml:lang="en">
    The Standard Reference Method or SRM is one of several systems modern
    brewers use to specify beer color.
    </skos:definition>
    <skos:prefLabel xml:lang="en">SRM</skos:prefLabel>
  </owl:DatatypeProperty>
  <owl:ObjectProperty rdf:about="http://rdfs.co/bevon/variant">
    <dcterms:issued rdf:datatype="http://www.w3.org/2001/XMLSchema#date">2013-07-04+09:00</dcterms:issued>
    <dcterms:modified rdf:datatype="http://www.w3.org/2001/XMLSchema#date">2014-03-01+09:00</dcterms:modified>
    <rdfs:domain rdf:resource="http://rdfs.co/bevon/Beverage"/>
    <rdfs:isDefinedBy rdf:resource="http://rdfs.co/bevon/"/>
    <rdfs:range rdf:resource="http://rdfs.co/bevon/Beverage"/>
    <rdfs:subPropertyOf rdf:resource="http://rdfs.co/bevon/related"/>
    <owl:inverseOf rdf:resource="http://rdfs.co/bevon/variantOf"/>
    <status:term_status xml:lang="en">unstable</status:term_status>
    <skos:definition xml:lang="en">
    This property states that a beverage has a variant.
    </skos:definition>
    <skos:prefLabel xml:lang="en">variant</skos:prefLabel>
    <skos:prefLabel xml:lang="ko">변형</skos:prefLabel>
  </owl:ObjectProperty>
  <owl:ObjectProperty rdf:about="http://rdfs.co/bevon/variantOf">
    <dcterms:issued rdf:datatype="http://www.w3.org/2001/XMLSchema#date">2013-07-04+09:00</dcterms:issued>
    <dcterms:modified rdf:datatype="http://www.w3.org/2001/XMLSchema#date">2014-03-01+09:00</dcterms:modified>
    <rdfs:domain rdf:resource="http://rdfs.co/bevon/Beverage"/>
    <rdfs:isDefinedBy rdf:resource="http://rdfs.co/bevon/"/>
    <rdfs:range rdf:resource="http://rdfs.co/bevon/Beverage"/>
    <rdfs:subPropertyOf rdf:resource="http://dbpedia.org/ontology/variantOf"/>
    <rdfs:subPropertyOf rdf:resource="http://purl.org/goodrelations/v1#isVariantOf"/>
    <rdfs:subPropertyOf rdf:resource="http://rdfs.co/bevon/related"/>
    <owl:inverseOf rdf:resource="http://rdfs.co/bevon/variant"/>
    <status:term_status xml:lang="en">unstable</status:term_status>
    <skos:definition xml:lang="en">
    This property states that a beverage is a variant of another beverage.
    </skos:definition>
    <skos:prefLabel xml:lang="en">variant of</skos:prefLabel>
    <skos:prefLabel xml:lang="ko">바탕</skos:prefLabel>
  </owl:ObjectProperty>
  <owl:ObjectProperty rdf:about="http://rdfs.co/bevon/volume">
    <dcterms:issued rdf:datatype="http://www.w3.org/2001/XMLSchema#date">2013-07-04+09:00</dcterms:issued>
    <dcterms:modified rdf:datatype="http://www.w3.org/2001/XMLSchema#date">2014-03-01+09:00</dcterms:modified>
    <rdfs:domain rdf:resource="http://rdfs.co/bevon/Container"/>
    <rdfs:isDefinedBy rdf:resource="http://rdfs.co/bevon/"/>
    <rdfs:range rdf:resource="http://purl.org/goodrelations/v1#QuantitativeValue"/>
    <status:term_status xml:lang="en">unstable</status:term_status>
    <skos:definition xml:lang="en">
    This property specifies the volume of the container.
    </skos:definition>
    <skos:prefLabel xml:lang="en">volume</skos:prefLabel>
    <skos:prefLabel xml:lang="ko">용량</skos:prefLabel>
  </owl:ObjectProperty>
  <rdf:Description rdf:about="http://www.w3.org/TR/2003/PR-owl-guide-20031209/wine#Wine">
    <rdfs:subClassOf rdf:resource="http://rdfs.co/bevon/Wine"/>
  </rdf:Description>
</rdf:RDF>
