<?xml version="1.0" encoding="utf-8" ?>
<rdf:RDF
	xmlns:rdf="http://www.w3.org/1999/02/22-rdf-syntax-ns#"
	xmlns:rdfs="http://www.w3.org/2000/01/rdf-schema#"
	xmlns:dct="http://purl.org/dc/terms/"
	xmlns:owl="http://www.w3.org/2002/07/owl#"
	xmlns:ns4="http://purl.org/vocab/vann/"
	xmlns:ns5="http://creativecommons.org/ns#" >
  <rdf:Description rdf:about="http://www.w3.org/2000/01/rdf-schema#label">
    <rdf:type rdf:resource="http://www.w3.org/2002/07/owl#DatatypeProperty" />
    <rdfs:domain rdf:resource="http://purl.org/net/dbm/ontology#Drug" />
    <rdfs:range rdf:resource="http://www.w3.org/2001/XMLSchema#string" />
    <rdfs:comment>This property holds the brand name of the drug, as a label.</rdfs:comment>
  </rdf:Description>
  <rdf:Description rdf:about="http://www.w3.org/2000/01/rdf-schema#seeAlso">
    <rdf:type rdf:resource="http://www.w3.org/2002/07/owl#ObjectProperty" />
    <rdfs:domain rdf:resource="http://purl.org/net/dbm/ontology#Drug" />
    <rdfs:range rdf:resource="http://wifo5-04.informatik.uni-mannheim.de/drugbank/resource/drugbank/drugs" />
    <rdfs:comment>This property links a drug from the Macedonian Drug Bureau with a drug from DrugBank, based on the ATC code.</rdfs:comment>
  </rdf:Description>
  <rdf:Description rdf:about="http://wifo5-04.informatik.uni-mannheim.de/drugbank/resource/drugbank/genericName">
    <rdf:type rdf:resource="http://www.w3.org/2002/07/owl#DatatypeProperty" />
    <rdfs:domain rdf:resource="http://purl.org/net/dbm/ontology#Drug" />
    <rdfs:range rdf:resource="http://www.w3.org/2001/XMLSchema#string" />
    <rdfs:comment>This property represents the generic name of the drug.</rdfs:comment>
  </rdf:Description>
  <rdf:Description rdf:about="http://wifo5-04.informatik.uni-mannheim.de/drugbank/resource/drugbank/brandName">
    <rdf:type rdf:resource="http://www.w3.org/2002/07/owl#DatatypeProperty" />
    <rdfs:domain rdf:resource="http://purl.org/net/dbm/ontology#Drug" />
    <rdfs:range rdf:resource="http://www.w3.org/2001/XMLSchema#string" />
    <rdfs:comment>This property represents the brand name of the drug.</rdfs:comment>
  </rdf:Description>
  <rdf:Description rdf:about="http://wifo5-04.informatik.uni-mannheim.de/drugbank/resource/drugbank/atcCode">
    <rdf:type rdf:resource="http://www.w3.org/2002/07/owl#DatatypeProperty" />
    <rdfs:domain rdf:resource="http://purl.org/net/dbm/ontology#Drug" />
    <rdfs:range rdf:resource="http://www.w3.org/2001/XMLSchema#string" />
    <rdfs:comment>This property represents the ATC code of the drug.</rdfs:comment>
  </rdf:Description>
  <rdf:Description rdf:about="http://wifo5-04.informatik.uni-mannheim.de/drugbank/resource/drugbank/drugs">
    <rdf:type rdf:resource="http://www.w3.org/2002/07/owl#Class" />
  </rdf:Description>
  <rdf:Description rdf:about="http://xmlns.com/foaf/0.1/page">
    <rdf:type rdf:resource="http://www.w3.org/2002/07/owl#DatatypeProperty" />
    <rdf:type rdf:resource="http://www.w3.org/2002/07/owl#FunctionalProperty" />
    <rdfs:domain rdf:resource="http://purl.org/net/dbm/ontology#Drug" />
    <rdfs:range rdf:resource="http://www.w3.org/2001/XMLSchema#string" />
    <rdfs:comment>This property holds the URL of the drug information page on the Macedonian Drug Bureau website.</rdfs:comment>
  </rdf:Description>
  <rdf:Description rdf:about="http://purl.org/net/dbm/ontology#atcCodeExtended">
    <rdf:type rdf:resource="http://www.w3.org/2002/07/owl#DatatypeProperty" />
    <rdfs:domain rdf:resource="http://purl.org/net/dbm/ontology#Drug" />
    <rdfs:range rdf:resource="http://www.w3.org/2001/XMLSchema#string" />
    <rdfs:comment>This property represents the extended ATC code for the drug, assigned by the Ministry of Health, of the Republic of Macedonia.</rdfs:comment>
  </rdf:Description>
  <rdf:Description rdf:about="http://purl.org/net/dbm/ontology#">
    <rdf:type rdf:resource="http://www.w3.org/2002/07/owl#Ontology" />
    <dct:modified>2016-08-28</dct:modified>
    <rdfs:label>DBM Ontology</rdfs:label>
    <rdfs:isDefinedBy rdf:resource="http://purl.org/net/dbm/ontology" />
    <rdfs:comment>An ontology for the Drug Bureau of Macedonia (DBM).</rdfs:comment>
    <owl:versionInfo>1.1</owl:versionInfo>
    <dct:description>An ontology for describing brand-name drugs.</dct:description>
    <dct:creator rdf:resource="https://plus.google.com/+MilosJovanovik" />
    <dct:issued>2014-09-01</dct:issued>
    <dct:publisher rdf:resource="http://finki.ukim.mk/" />
    <dct:title>DBM Ontology</dct:title>
    <ns4:preferredNamespacePrefix>dbm</ns4:preferredNamespacePrefix>
    <ns4:preferredNamespaceUri>http://purl.org/net/dbm/ontology#</ns4:preferredNamespaceUri>
    <ns5:license rdf:resource="https://creativecommons.org/licenses/by/3.0/" />
    <dct:rights>Copyright 2014, Milos Jovanovik</dct:rights>
  </rdf:Description>
  <rdf:Description rdf:about="http://purl.org/net/dbm/ontology#Drug">
    <rdf:type rdf:resource="http://www.w3.org/2002/07/owl#Class" />
    <rdfs:comment>This class represents a Drug entity from the Macedonian Drug Bureau.</rdfs:comment>
  </rdf:Description>
  <rdf:Description rdf:about="http://purl.org/net/dbm/ontology#approvalNumber">
    <rdf:type rdf:resource="http://www.w3.org/2002/07/owl#DatatypeProperty" />
    <rdfs:domain rdf:resource="http://purl.org/net/dbm/ontology#Drug" />
    <rdfs:range rdf:resource="http://www.w3.org/2001/XMLSchema#string" />
    <rdfs:comment>This property represents the approval number assigned by the Macedonian Drug Bureau, for the company.</rdfs:comment>
  </rdf:Description>
  <rdf:Description rdf:about="http://purl.org/net/dbm/ontology#approvedFor">
    <rdf:type rdf:resource="http://www.w3.org/2002/07/owl#DatatypeProperty" />
    <rdfs:domain rdf:resource="http://purl.org/net/dbm/ontology#Drug" />
    <rdfs:range rdf:resource="http://www.w3.org/2001/XMLSchema#string" />
    <rdfs:comment>This property represents the company which holds the approval by the Macedonian Drug Bureau for the drug.</rdfs:comment>
  </rdf:Description>
  <rdf:Description rdf:about="http://purl.org/net/dbm/ontology#approvedOn">
    <rdf:type rdf:resource="http://www.w3.org/2002/07/owl#DatatypeProperty" />
    <rdfs:domain rdf:resource="http://purl.org/net/dbm/ontology#Drug" />
    <rdfs:range rdf:resource="http://www.w3.org/2001/XMLSchema#dateTime" />
    <rdfs:comment>This property represents the date the company was given the approval by the Macedonian Drug Bureau for the drug.</rdfs:comment>
  </rdf:Description>
  <rdf:Description rdf:about="http://purl.org/net/dbm/ontology#approvedUntil">
    <rdf:type rdf:resource="http://www.w3.org/2002/07/owl#DatatypeProperty" />
    <rdfs:domain rdf:resource="http://purl.org/net/dbm/ontology#Drug" />
    <rdfs:range rdf:resource="http://www.w3.org/2001/XMLSchema#dateTime" />
    <rdfs:comment>This property represents the expiry date of the approval which the company was given by the Macedonian Drug Bureau for the drug.</rdfs:comment>
  </rdf:Description>
  <rdf:Description rdf:about="http://purl.org/net/dbm/ontology#brailleSupport">
    <rdf:type rdf:resource="http://www.w3.org/2002/07/owl#DatatypeProperty" />
    <rdfs:domain rdf:resource="http://purl.org/net/dbm/ontology#Drug" />
    <rdfs:range rdf:resource="http://www.w3.org/2001/XMLSchema#string" />
    <rdfs:comment>This property indicates wether the drug packaging has Braille support or not.</rdfs:comment>
  </rdf:Description>
  <rdf:Description rdf:about="http://purl.org/net/dbm/ontology#brandNameCyrillic">
    <rdf:type rdf:resource="http://www.w3.org/2002/07/owl#DatatypeProperty" />
    <rdfs:domain rdf:resource="http://purl.org/net/dbm/ontology#Drug" />
    <rdfs:range rdf:resource="http://www.w3.org/2001/XMLSchema#string" />
    <rdfs:comment>This property represents the brand name of the drug, in cyrillic alphabet.</rdfs:comment>
  </rdf:Description>
  <rdf:Description rdf:about="http://purl.org/net/dbm/ontology#dosage">
    <rdf:type rdf:resource="http://www.w3.org/2002/07/owl#DatatypeProperty" />
    <rdfs:domain rdf:resource="http://purl.org/net/dbm/ontology#Drug" />
    <rdfs:range rdf:resource="http://www.w3.org/2001/XMLSchema#string" />
    <rdfs:comment>This property represents the dosage information for the drug.</rdfs:comment>
  </rdf:Description>
  <rdf:Description rdf:about="http://purl.org/net/dbm/ontology#eanCode">
    <rdf:type rdf:resource="http://www.w3.org/2002/07/owl#FunctionalProperty" />
    <rdf:type rdf:resource="http://www.w3.org/2002/07/owl#DatatypeProperty" />
    <rdfs:domain rdf:resource="http://purl.org/net/dbm/ontology#Drug" />
    <rdfs:range rdf:resource="http://www.w3.org/2001/XMLSchema#string" />
    <rdfs:comment>This property represents the EAN code of the drug.</rdfs:comment>
  </rdf:Description>
  <rdf:Description rdf:about="http://purl.org/net/dbm/ontology#hifmCode">
    <rdf:type rdf:resource="http://www.w3.org/2002/07/owl#DatatypeProperty" />
    <rdf:type rdf:resource="http://www.w3.org/2002/07/owl#FunctionalProperty" />
    <rdfs:domain rdf:resource="http://purl.org/net/dbm/ontology#Drug" />
    <rdfs:range rdf:resource="http://www.w3.org/2001/XMLSchema#string" />
    <rdfs:comment>This is the code that the drug instance has in the local system of the Health Insurance Fund of Macedonia.</rdfs:comment>
  </rdf:Description>
  <rdf:Description rdf:about="http://purl.org/net/dbm/ontology#manufacturer">
    <rdf:type rdf:resource="http://www.w3.org/2002/07/owl#DatatypeProperty" />
    <rdfs:domain rdf:resource="http://purl.org/net/dbm/ontology#Drug" />
    <rdfs:range rdf:resource="http://www.w3.org/2001/XMLSchema#string" />
    <rdfs:comment>This property represents a manufacturer of a drug.</rdfs:comment>
  </rdf:Description>
  <rdf:Description rdf:about="http://purl.org/net/dbm/ontology#packaging">
    <rdf:type rdf:resource="http://www.w3.org/2002/07/owl#DatatypeProperty" />
    <rdfs:domain rdf:resource="http://purl.org/net/dbm/ontology#Drug" />
    <rdfs:range rdf:resource="http://www.w3.org/2001/XMLSchema#string" />
    <rdfs:comment>This property represents the packaging information of the drug.</rdfs:comment>
  </rdf:Description>
  <rdf:Description rdf:about="http://purl.org/net/dbm/ontology#positiveList">
    <rdf:type rdf:resource="http://www.w3.org/2002/07/owl#DatatypeProperty" />
    <rdfs:domain rdf:resource="http://purl.org/net/dbm/ontology#Drug" />
    <rdfs:range rdf:resource="http://www.w3.org/2001/XMLSchema#string" />
    <rdfs:comment>This property tells if the drug is featured on the positive list of drugs, or not.</rdfs:comment>
  </rdf:Description>
  <rdf:Description rdf:about="http://purl.org/net/dbm/ontology#priceWithVAT">
    <rdf:type rdf:resource="http://www.w3.org/2002/07/owl#DatatypeProperty" />
    <rdfs:domain rdf:resource="http://purl.org/net/dbm/ontology#Drug" />
    <rdfs:range rdf:resource="http://www.w3.org/2001/XMLSchema#float" />
    <rdfs:comment>This property represents the price of the drug in Macedonian Denars (MKD), with VAT calculated.</rdfs:comment>
  </rdf:Description>
  <rdf:Description rdf:about="http://purl.org/net/dbm/ontology#priceWithoutVAT">
    <rdf:type rdf:resource="http://www.w3.org/2002/07/owl#DatatypeProperty" />
    <rdfs:domain rdf:resource="http://purl.org/net/dbm/ontology#Drug" />
    <rdfs:range rdf:resource="http://www.w3.org/2001/XMLSchema#float" />
    <rdfs:comment>This property represents the price of the drug in Macedonian Denars (MKD), with no VAT calculated.</rdfs:comment>
  </rdf:Description>
  <rdf:Description rdf:about="http://purl.org/net/dbm/ontology#referencePrice">
    <rdf:type rdf:resource="http://www.w3.org/2002/07/owl#DatatypeProperty" />
    <rdfs:domain rdf:resource="http://purl.org/net/dbm/ontology#Drug" />
    <rdfs:range rdf:resource="http://www.w3.org/2001/XMLSchema#float" />
    <rdfs:comment>This property represents the reference price for the drug, as assigned by the Ministry of Health of the Republic of Macedonia.</rdfs:comment>
  </rdf:Description>
  <rdf:Description rdf:about="http://purl.org/net/dbm/ontology#similarTo">
    <rdf:type rdf:resource="http://www.w3.org/2002/07/owl#ObjectProperty" />
    <rdf:type rdf:resource="http://www.w3.org/2002/07/owl#TransitiveProperty" />
    <rdf:type rdf:resource="http://www.w3.org/2002/07/owl#SymmetricProperty" />
    <rdfs:domain rdf:resource="http://purl.org/net/dbm/ontology#Drug" />
    <rdfs:range rdf:resource="http://purl.org/net/dbm/ontology#Drug" />
    <rdfs:comment>This property is used to represent that the drugs in question are similar in their purpose, i.e. contain the same active substance.</rdfs:comment>
  </rdf:Description>
  <rdf:Description rdf:about="http://purl.org/net/dbm/ontology#strength">
    <rdf:type rdf:resource="http://www.w3.org/2002/07/owl#DatatypeProperty" />
    <rdfs:domain rdf:resource="http://purl.org/net/dbm/ontology#Drug" />
    <rdfs:range rdf:resource="http://www.w3.org/2001/XMLSchema#string" />
    <rdfs:comment>This property represents the strength of the drug.</rdfs:comment>
  </rdf:Description>
  <rdf:Description rdf:about="http://purl.org/net/dbm/ontology#summaryReport">
    <rdf:type rdf:resource="http://www.w3.org/2002/07/owl#FunctionalProperty" />
    <rdf:type rdf:resource="http://www.w3.org/2002/07/owl#DatatypeProperty" />
    <rdfs:domain rdf:resource="http://purl.org/net/dbm/ontology#Drug" />
    <rdfs:range rdf:resource="http://www.w3.org/2001/XMLSchema#string" />
    <rdfs:comment>This property holds the URL to the summary report for the drug, published by the Macedonian Drug Bureau.</rdfs:comment>
  </rdf:Description>
  <rdf:Description rdf:about="http://purl.org/net/dbm/ontology#updateDate">
    <rdf:type rdf:resource="http://www.w3.org/2002/07/owl#DatatypeProperty" />
    <rdfs:domain rdf:resource="http://purl.org/net/dbm/ontology#Drug" />
    <rdfs:range rdf:resource="http://www.w3.org/2001/XMLSchema#dateTime" />
    <rdfs:comment>This property represents the date the drug data has been updated.</rdfs:comment>
  </rdf:Description>
  <rdf:Description rdf:about="http://purl.org/net/dbm/ontology#usageGuidelines">
    <rdf:type rdf:resource="http://www.w3.org/2002/07/owl#FunctionalProperty" />
    <rdf:type rdf:resource="http://www.w3.org/2002/07/owl#DatatypeProperty" />
    <rdfs:domain rdf:resource="http://purl.org/net/dbm/ontology#Drug" />
    <rdfs:range rdf:resource="http://www.w3.org/2001/XMLSchema#string" />
    <rdfs:comment>This property holds the URL to the usage guidelines for the drug, published by the Macedonian Drug Bureau.</rdfs:comment>
  </rdf:Description>
</rdf:RDF>