<?xml version="1.0"?>


<!DOCTYPE rdf:RDF [
    <!ENTITY void "http://rdfs.org/ns/void#" >
    <!ENTITY ldp "http://www.w3.org/ns/ldp#" >
    <!ENTITY dct "http://purl.org/dc/terms/" >
    <!ENTITY prov "http://www.w3.org/ns/prov#" >
    <!ENTITY foaf "http://xmlns.com/foaf/0.1/" >
    <!ENTITY vann "http://purl.org/vocab/vann/" >
    <!ENTITY odrl "http://www.w3.org/ns/odrl/2/" >
    <!ENTITY mco-core "urn:mpeg:mpeg21:mco:core:2012#" >
    <!ENTITY cc "http://creativecommons.org/ns#" >
    <!ENTITY owl "http://www.w3.org/2002/07/owl#" >
    <!ENTITY acl "http://www.w3.org/ns/auth/acl#" >
    <!ENTITY voaf "http://purl.org/vocommons/voaf#" >
    <!ENTITY dc "http://purl.org/dc/elements/1.1/" >
    <!ENTITY frbr "http://purl.org/vocab/frbr/core#" >
    <!ENTITY xsd "http://www.w3.org/2001/XMLSchema#" >
    <!ENTITY skos "http://www.w3.org/2004/02/skos/core#" >
    <!ENTITY xml "http://www.w3.org/XML/1998/namespace" >
    <!ENTITY rdfs "http://www.w3.org/2000/01/rdf-schema#" >
    <!ENTITY rdf "http://www.w3.org/1999/02/22-rdf-syntax-ns#" >
    <!ENTITY lkif "http://www.estrellaproject.org/lkif-core/lkif-core.owl" >
    <!ENTITY cpannotationschema "http://www.ontologydesignpatterns.org/schemas/cpannotationschema.owl#" >
]>


<rdf:RDF xmlns="http://purl.oclc.org/NET/ldr/ns#"
     xml:base="http://purl.oclc.org/NET/ldr/ns"
     xmlns:lkif="http://www.estrellaproject.org/lkif-core/lkif-core.owl"
     xmlns:dc="http://purl.org/dc/elements/1.1/"
     xmlns:prov="http://www.w3.org/ns/prov#"
     xmlns:foaf="http://xmlns.com/foaf/0.1/"
     xmlns:mco-core="urn:mpeg:mpeg21:mco:core:2012#"
     xmlns:frbr="http://purl.org/vocab/frbr/core#"
     xmlns:acl="http://www.w3.org/ns/auth/acl#"
     xmlns:vann="http://purl.org/vocab/vann/"
     xmlns:void="http://rdfs.org/ns/void#"
     xmlns:xml="http://www.w3.org/XML/1998/namespace"
     xmlns:voaf="http://purl.org/vocommons/voaf#"
     xmlns:rdfs="http://www.w3.org/2000/01/rdf-schema#"
     xmlns:cpannotationschema="http://www.ontologydesignpatterns.org/schemas/cpannotationschema.owl#"
     xmlns:dct="http://purl.org/dc/terms/"
     xmlns:owl="http://www.w3.org/2002/07/owl#"
     xmlns:xsd="http://www.w3.org/2001/XMLSchema#"
     xmlns:rdf="http://www.w3.org/1999/02/22-rdf-syntax-ns#"
     xmlns:skos="http://www.w3.org/2004/02/skos/core#"
     xmlns:cc="http://creativecommons.org/ns#"
     xmlns:ldp="http://www.w3.org/ns/ldp#"
     xmlns:odrl="http://www.w3.org/ns/odrl/2/">
    <owl:Ontology rdf:about="http://purl.oclc.org/NET/ldr/ns#">
        <rdfs:label xml:lang="en">Linked Data Rights</rdfs:label>
        <voaf:propertyNumber rdf:datatype="&xsd;int">18</voaf:propertyNumber>
        <dct:issued rdf:datatype="&xsd;date">2013-09-20</dct:issued>
        <dct:issued rdf:datatype="&xsd;date">2014-08-30</dct:issued>
        <voaf:classNumber rdf:datatype="&xsd;int">31</voaf:classNumber>
        <cpannotationschema:scenarios xml:lang="en">Declaring rights on both Linked Open Data and Linked Closed Data</cpannotationschema:scenarios>
        <dct:title xml:lang="en">Linked Data Rights (LDR)</dct:title>
        <dct:contributor>Maria Poveda-Villalon</dct:contributor>
        <vann:preferredNamespacePrefix>ldr</vann:preferredNamespacePrefix>
        <dct:contributor>Asuncion Gomez-Perez</dct:contributor>
        <dct:contributor>Victor Rodriguez-Doncel</dct:contributor>
        <owl:versionInfo xml:lang="en">2.0</owl:versionInfo>
        <dct:creator>Ontology Engineering Group - Universidad Polit√©cnica de Madrid</dct:creator>
        <dct:contributor>Mari Carmen Suarez</dct:contributor>
        <dct:description xml:lang="en">The Linked Data Rights ontology provides the vocabulary for creating rights expressions for Linked Data resources by extending the ODRL ontology. 
								   Linked Data assets (RDF triples, graphs, datasets, mappings...) can be object of protection by the intellectual property law, the database law or its access or publication be restricted by other legal reasons (personal data pro- tection, security reasons, etc.). Publishing a rights expression along with the digital asset, allows the rightsholder waiving some or all of the IP and database rights (leaving the work in the public domain), permitting some operations if certain conditions are satisfied (like giving attribution to the author) or simply reminding the audience that some rights are reserved. Specific vocabulary is given for authorising specific uses of Linked Data.</dct:description>
        <vann:preferredNamespaceUri>http://purl.oclc.org/NET/ldr/ns#</vann:preferredNamespaceUri>
        <cpannotationschema:hasComponent xml:lang="en">http://www.w3.org/TR/swbp-n-aryRelations/</cpannotationschema:hasComponent>
        <cc:license rdf:resource="http://creativecommons.org/licenses/by/3.0/"/>
        <voaf:hasEquivalencesWith rdf:resource="&cc;null"/>
        <voaf:specializes rdf:resource="&cc;null"/>
        <voaf:reliesOn rdf:resource="&cc;null"/>
        <voaf:similar rdf:resource="http://data.opendataday.it/LiMo"/>
        <dc:creator rdf:resource="http://delicias.dia.fi.upm.es/~vrodriguez/"/>
        <voaf:similar rdf:resource="http://ns.inria.fr/l4lod/v2/l4lod_v2.rdf"/>
        <cpannotationschema:hasIntent rdf:resource="http://oeg-dev.dia.fi.upm.es/licensius/static/ldr/pattern.html#int"/>
        <cpannotationschema:coversRequirements rdf:resource="http://oeg-dev.dia.fi.upm.es/licensius/static/ldr/pattern.html#reqs"/>
        <prov:wasDerivedFrom rdf:resource="http://oeg-dev.dia.fi.upm.es/licensius/static/lldr/lldr-2013.07.18.owl"/>
        <voaf:similar rdf:resource="http://schema.theodi.org/odrs/"/>
        <voaf:reliesOn rdf:resource="http://www.w3.org/ns/odrl/2/"/>
        <voaf:similar rdf:resource="&odrl;null"/>
        <voaf:reliesOn rdf:resource="&odrl;null"/>
        <voaf:specializes rdf:resource="&odrl;null"/>
        <voaf:hasEquivalencesWith rdf:resource="&odrl;null"/>
        <voaf:hasEquivalencesWith rdf:resource="&foaf;null"/>
    </owl:Ontology>
    


    <!-- 
    ///////////////////////////////////////////////////////////////////////////////////////
    //
    // Annotation properties
    //
    ///////////////////////////////////////////////////////////////////////////////////////
     -->

    


    <!-- http://purl.oclc.org/NET/ldr/ns#issuedOn -->

    <owl:AnnotationProperty rdf:about="http://purl.oclc.org/NET/ldr/ns#issuedOn">
        <rdfs:comment xml:lang="en">Date on which the rights expression is issued, with legal consequences on the copyright or database right expiration.</rdfs:comment>
        <rdfs:domain rdf:resource="http://purl.oclc.org/NET/ldr/ns#Policy"/>
    </owl:AnnotationProperty>
    


    <!-- http://www.w3.org/2004/02/skos/core#closeMatch -->

    <owl:AnnotationProperty rdf:about="&skos;closeMatch"/>
    


    <!-- http://www.w3.org/2004/02/skos/core#exactMatch -->

    <owl:AnnotationProperty rdf:about="&skos;exactMatch"/>
    


    <!-- http://www.w3.org/2004/02/skos/core#example -->

    <owl:AnnotationProperty rdf:about="&skos;example"/>
    


    <!-- http://www.w3.org/2004/02/skos/core#narrowMatch -->

    <owl:AnnotationProperty rdf:about="&skos;narrowMatch"/>
    


    <!-- 
    ///////////////////////////////////////////////////////////////////////////////////////
    //
    // Object Properties
    //
    ///////////////////////////////////////////////////////////////////////////////////////
     -->

    


    <!-- http://purl.oclc.org/NET/ldr/ns#hasClaim -->

    <owl:ObjectProperty rdf:about="http://purl.oclc.org/NET/ldr/ns#hasClaim">
        <rdfs:comment xml:lang="en">Declares a claim asserted in the context of a rights expression</rdfs:comment>
        <rdfs:range rdf:resource="http://purl.oclc.org/NET/ldr/ns#Proposition"/>
    </owl:ObjectProperty>
    


    <!-- http://purl.oclc.org/NET/ldr/ns#hasExtendedRule -->

    <owl:ObjectProperty rdf:about="http://purl.oclc.org/NET/ldr/ns#hasExtendedRule">
        <rdfs:comment xml:lang="en">Links a Policy to an ExtendedRule it contains</rdfs:comment>
        <rdfs:range rdf:resource="http://purl.oclc.org/NET/ldr/ns#ExtendedRule"/>
        <rdfs:domain rdf:resource="&odrl;Policy"/>
    </owl:ObjectProperty>
    


    <!-- http://purl.oclc.org/NET/ldr/ns#hasLegalStatus -->

    <owl:ObjectProperty rdf:about="http://purl.oclc.org/NET/ldr/ns#hasLegalStatus">
        <rdfs:comment>Declares the legal status of a resource</rdfs:comment>
        <rdfs:domain rdf:resource="http://purl.oclc.org/NET/ldr/ns#LinkedDataResource"/>
        <rdfs:range rdf:resource="http://purl.oclc.org/NET/ldr/ns#ResourceLegalStatus"/>
    </owl:ObjectProperty>
    


    <!-- http://purl.oclc.org/NET/ldr/ns#hasRequirement -->

    <owl:ObjectProperty rdf:about="http://purl.oclc.org/NET/ldr/ns#hasRequirement">
        <rdfs:comment xml:lang="en">Declares which requirements have to be fulfilled for the Rule to be valid</rdfs:comment>
        <rdfs:range rdf:resource="http://purl.oclc.org/NET/ldr/ns#Proposition"/>
        <rdfs:domain rdf:resource="&odrl;Rule"/>
    </owl:ObjectProperty>
    


    <!-- 
    ///////////////////////////////////////////////////////////////////////////////////////
    //
    // Data properties
    //
    ///////////////////////////////////////////////////////////////////////////////////////
     -->

    


    <!-- http://purl.oclc.org/NET/ldr/ns#dataFormat -->

    <owl:DatatypeProperty rdf:about="http://purl.oclc.org/NET/ldr/ns#dataFormat">
        <rdfs:comment xml:lang="en">Format of the data (&quot;text/html&quot;, &quot;application/rdf+xml&quot;, etc.)</rdfs:comment>
        <rdfs:subPropertyOf rdf:resource="http://purl.oclc.org/NET/ldr/ns#hasclaim"/>
        <rdfs:subPropertyOf rdf:resource="&odrl;rightOperand"/>
    </owl:DatatypeProperty>
    


    <!-- http://purl.oclc.org/NET/ldr/ns#hasAttributionText -->

    <owl:DatatypeProperty rdf:about="http://purl.oclc.org/NET/ldr/ns#hasAttributionText">
        <rdfs:comment xml:lang="en">Text that has to be included as requested by a condition</rdfs:comment>
        <skos:closeMatch rdf:resource="&cc;attributionName"/>
        <skos:closeMatch rdf:resource="&cc;attributionURL"/>
        <rdfs:domain rdf:resource="http://purl.oclc.org/NET/ldr/ns#Proposition"/>
        <rdfs:subPropertyOf rdf:resource="http://purl.oclc.org/NET/ldr/ns#hasclaim"/>
        <rdfs:range rdf:resource="&rdfs;Literal"/>
        <rdfs:subPropertyOf rdf:resource="&odrl;rightOperand"/>
    </owl:DatatypeProperty>
    


    <!-- http://purl.oclc.org/NET/ldr/ns#hasCopyrightNotice -->

    <owl:DatatypeProperty rdf:about="http://purl.oclc.org/NET/ldr/ns#hasCopyrightNotice">
        <rdfs:comment xml:lang="en">Text that has to be attached imposed as a condition</rdfs:comment>
        <rdfs:subPropertyOf rdf:resource="http://purl.oclc.org/NET/ldr/ns#hasclaim"/>
        <rdfs:range rdf:resource="&rdfs;Literal"/>
        <rdfs:subPropertyOf rdf:resource="&odrl;rightOperand"/>
    </owl:DatatypeProperty>
    


    <!-- http://purl.oclc.org/NET/ldr/ns#hasDisclaimerText -->

    <owl:DatatypeProperty rdf:about="http://purl.oclc.org/NET/ldr/ns#hasDisclaimerText">
        <rdfs:comment xml:lang="en">Text discharging responsibilities on the use of the Linked Data resource</rdfs:comment>
        <rdfs:subPropertyOf rdf:resource="http://purl.oclc.org/NET/ldr/ns#hasclaim"/>
        <rdfs:domain rdf:resource="&odrl;Policy"/>
        <rdfs:subPropertyOf rdf:resource="&odrl;rightOperand"/>
    </owl:DatatypeProperty>
    


    <!-- http://purl.oclc.org/NET/ldr/ns#hasPersonalData -->

    <owl:DatatypeProperty rdf:about="http://purl.oclc.org/NET/ldr/ns#hasPersonalData">
        <rdfs:comment xml:lang="en">Declares that the referred resource has personal data</rdfs:comment>
        <rdfs:subPropertyOf rdf:resource="http://purl.oclc.org/NET/ldr/ns#hasclaim"/>
        <rdfs:subPropertyOf rdf:resource="&odrl;rightOperand"/>
    </owl:DatatypeProperty>
    


    <!-- http://purl.oclc.org/NET/ldr/ns#hasPrivacyLevel -->

    <owl:DatatypeProperty rdf:about="http://purl.oclc.org/NET/ldr/ns#hasPrivacyLevel">
        <rdfs:comment xml:lang="en">Declares the privacy level (e.g. personal data) for a Linked Data resource</rdfs:comment>
        <rdfs:domain rdf:resource="http://purl.oclc.org/NET/ldr/ns#LinkedDataResource"/>
        <rdfs:subPropertyOf rdf:resource="http://purl.oclc.org/NET/ldr/ns#hasclaim"/>
        <rdfs:subPropertyOf rdf:resource="&odrl;rightOperand"/>
    </owl:DatatypeProperty>
    


    <!-- http://purl.oclc.org/NET/ldr/ns#hasclaim -->

    <owl:DatatypeProperty rdf:about="http://purl.oclc.org/NET/ldr/ns#hasclaim"/>
    


    <!-- http://purl.oclc.org/NET/ldr/ns#issuedOn -->

    <owl:DatatypeProperty rdf:about="http://purl.oclc.org/NET/ldr/ns#issuedOn">
        <rdfs:comment xml:lang="en">Date on which the rights expression is issued, with legal consequences on the copyright or database right expiration.</rdfs:comment>
        <rdfs:range rdf:resource="&xsd;dateTime"/>
    </owl:DatatypeProperty>
    


    <!-- http://purl.oclc.org/NET/ldr/ns#operation -->

    <owl:DatatypeProperty rdf:about="http://purl.oclc.org/NET/ldr/ns#operation">
        <rdfs:comment xml:lang="en">May be set with one of the mathematical values AND, OR and XOR. (OR is the default if not specified.)</rdfs:comment>
        <rdfs:domain rdf:resource="http://purl.oclc.org/NET/ldr/ns#ExtendedRule"/>
        <rdfs:range rdf:resource="&xsd;string"/>
    </owl:DatatypeProperty>
    


    <!-- http://purl.oclc.org/NET/ldr/ns#protocol -->

    <owl:DatatypeProperty rdf:about="http://purl.oclc.org/NET/ldr/ns#protocol">
        <rdfs:comment xml:lang="en">Access protocol (e.g. &quot;SPARQL&quot;, &quot;HTTPS&quot;, etc.)</rdfs:comment>
        <rdfs:subPropertyOf rdf:resource="http://purl.oclc.org/NET/ldr/ns#hasclaim"/>
        <rdfs:subPropertyOf rdf:resource="&odrl;rightOperand"/>
    </owl:DatatypeProperty>
    


    <!-- http://purl.oclc.org/NET/ldr/ns#queriesPerDay -->

    <owl:DatatypeProperty rdf:about="http://purl.oclc.org/NET/ldr/ns#queriesPerDay">
        <rdfs:comment xml:lang="en">Number of queries per day</rdfs:comment>
        <rdfs:subPropertyOf rdf:resource="http://purl.oclc.org/NET/ldr/ns#hasclaim"/>
        <rdfs:subPropertyOf rdf:resource="&odrl;rightOperand"/>
    </owl:DatatypeProperty>
    


    <!-- http://purl.oclc.org/NET/ldr/ns#queriesPerMinute -->

    <owl:DatatypeProperty rdf:about="http://purl.oclc.org/NET/ldr/ns#queriesPerMinute">
        <rdfs:comment xml:lang="en">Number of queries per minute</rdfs:comment>
        <rdfs:subPropertyOf rdf:resource="http://purl.oclc.org/NET/ldr/ns#hasclaim"/>
        <rdfs:subPropertyOf rdf:resource="&odrl;rightOperand"/>
    </owl:DatatypeProperty>
    


    <!-- http://purl.oclc.org/NET/ldr/ns#truthValue -->

    <owl:DatatypeProperty rdf:about="http://purl.oclc.org/NET/ldr/ns#truthValue">
        <rdfs:comment xml:lang="en">Truth value</rdfs:comment>
        <rdfs:domain rdf:resource="http://purl.oclc.org/NET/ldr/ns#Proposition"/>
        <rdfs:range rdf:resource="&xsd;boolean"/>
    </owl:DatatypeProperty>
    


    <!-- http://www.w3.org/ns/odrl/2/rightOperand -->

    <owl:DatatypeProperty rdf:about="&odrl;rightOperand"/>
    


    <!-- 
    ///////////////////////////////////////////////////////////////////////////////////////
    //
    // Classes
    //
    ///////////////////////////////////////////////////////////////////////////////////////
     -->

    


    <!-- http://purl.oclc.org/NET/ldr/ns#Access -->

    <owl:Class rdf:about="http://purl.oclc.org/NET/ldr/ns#Access">
        <rdfs:subClassOf rdf:resource="http://purl.oclc.org/NET/ldr/ns#LinkedDataRight"/>
        <rdfs:comment xml:lang="en">Right of access, which can be legally granted (e.g. public sector information) or expressely restricted (e.g. secrets compromising national security)</rdfs:comment>
        <skos:exactMatch rdf:resource="&acl;Access"/>
    </owl:Class>
    


    <!-- http://purl.oclc.org/NET/ldr/ns#Action -->

    <owl:Class rdf:about="http://purl.oclc.org/NET/ldr/ns#Action"/>
    


    <!-- http://purl.oclc.org/NET/ldr/ns#CopyrightException -->

    <owl:Class rdf:about="http://purl.oclc.org/NET/ldr/ns#CopyrightException">
        <rdfs:subClassOf rdf:resource="http://purl.oclc.org/NET/ldr/ns#Proposition"/>
        <rdfs:comment xml:lang="en">Reason which can be invoked to make an exception to the intellectual property or database law </rdfs:comment>
    </owl:Class>
    


    <!-- http://purl.oclc.org/NET/ldr/ns#DatabaseRight -->

    <owl:Class rdf:about="http://purl.oclc.org/NET/ldr/ns#DatabaseRight">
        <rdfs:subClassOf rdf:resource="http://purl.oclc.org/NET/ldr/ns#LinkedDataRight"/>
        <rdfs:comment xml:lang="en">Sui generis right for databases, recognized in European countries and others</rdfs:comment>
    </owl:Class>
    


    <!-- http://purl.oclc.org/NET/ldr/ns#Derivation -->

    <owl:Class rdf:about="http://purl.oclc.org/NET/ldr/ns#Derivation">
        <rdfs:subClassOf rdf:resource="http://purl.oclc.org/NET/ldr/ns#IPRight"/>
        <rdfs:comment xml:lang="en">Transformation of the work, including translation adaptation or any other form modification</rdfs:comment>
        <skos:closeMatch rdf:resource="&cc;DerivativeWorks"/>
    </owl:Class>
    


    <!-- http://purl.oclc.org/NET/ldr/ns#Distribution -->

    <owl:Class rdf:about="http://purl.oclc.org/NET/ldr/ns#Distribution">
        <rdfs:subClassOf rdf:resource="http://purl.oclc.org/NET/ldr/ns#IPRight"/>
        <rdfs:comment xml:lang="en">Make available the original work or its copies, in a physical medium</rdfs:comment>
        <skos:exactMatch rdf:resource="&cc;Distribution"/>
    </owl:Class>
    


    <!-- http://purl.oclc.org/NET/ldr/ns#ExtendedRule -->

    <owl:Class rdf:about="http://purl.oclc.org/NET/ldr/ns#ExtendedRule">
        <rdfs:subClassOf rdf:resource="&odrl;Rule"/>
        <rdfs:comment>Extended Relations may tie Permission, Prohibition, Duty, and Constraint entities together with an AND, OR or XOR relationship. Only entities of the same type can be linked with this model. For example, a Permission and Prohibition cannot be linked together within this model. The Extended rule is composed of two or more rules</rdfs:comment>
    </owl:Class>
    


    <!-- http://purl.oclc.org/NET/ldr/ns#Extraction -->

    <owl:Class rdf:about="http://purl.oclc.org/NET/ldr/ns#Extraction">
        <rdfs:subClassOf rdf:resource="http://purl.oclc.org/NET/ldr/ns#DatabaseRight"/>
        <rdfs:comment xml:lang="en">Right to permanent or temporary transfer of all or a substantial part of the contents of a database to another medium by any means or in any form</rdfs:comment>
    </owl:Class>
    


    <!-- http://purl.oclc.org/NET/ldr/ns#FamousDataLicense -->

    <owl:Class rdf:about="http://purl.oclc.org/NET/ldr/ns#FamousDataLicense">
        <rdfs:subClassOf rdf:resource="http://purl.oclc.org/NET/ldr/ns#License"/>
        <rdfs:comment xml:lang="en">License publicly available and known to the public</rdfs:comment>
    </owl:Class>
    


    <!-- http://purl.oclc.org/NET/ldr/ns#IPRight -->

    <owl:Class rdf:about="http://purl.oclc.org/NET/ldr/ns#IPRight">
        <rdfs:subClassOf rdf:resource="http://purl.oclc.org/NET/ldr/ns#LinkedDataRight"/>
        <rdfs:comment xml:lang="en">Intellectual Property right</rdfs:comment>
    </owl:Class>
    


    <!-- http://purl.oclc.org/NET/ldr/ns#LDPAccess -->

    <owl:Class rdf:about="http://purl.oclc.org/NET/ldr/ns#LDPAccess">
        <rdfs:subClassOf rdf:resource="http://purl.oclc.org/NET/ldr/ns#Access"/>
    </owl:Class>
    


    <!-- http://purl.oclc.org/NET/ldr/ns#License -->

    <owl:Class rdf:about="http://purl.oclc.org/NET/ldr/ns#License">
        <rdfs:subClassOf rdf:resource="http://purl.oclc.org/NET/ldr/ns#LinkedDataPolicy"/>
        <rdfs:comment xml:lang="en">Set of rights expressions offered to the public, which grant one or more rights, possibly conditioned to the fulfillment of one or more conditions (propositions)</rdfs:comment>
    </owl:Class>
    


    <!-- http://purl.oclc.org/NET/ldr/ns#LinkedDataPolicy -->

    <owl:Class rdf:about="http://purl.oclc.org/NET/ldr/ns#LinkedDataPolicy">
        <rdfs:subClassOf rdf:resource="&odrl;Policy"/>
        <rdfs:comment xml:lang="en">A policy applied over a Linked Data resource</rdfs:comment>
    </owl:Class>
    


    <!-- http://purl.oclc.org/NET/ldr/ns#LinkedDataResource -->

    <owl:Class rdf:about="http://purl.oclc.org/NET/ldr/ns#LinkedDataResource">
        <rdfs:subClassOf rdf:resource="&odrl;Asset"/>
        <rdfs:comment xml:lang="en">A Linked Data resource, object of some rights</rdfs:comment>
    </owl:Class>
    


    <!-- http://purl.oclc.org/NET/ldr/ns#LinkedDataRight -->

    <owl:Class rdf:about="http://purl.oclc.org/NET/ldr/ns#LinkedDataRight">
        <rdfs:subClassOf rdf:resource="http://purl.oclc.org/NET/ldr/ns#Action"/>
        <rdfs:comment xml:lang="en">Action legally granted as allowable to be exercised on a Linked Data resource</rdfs:comment>
    </owl:Class>
    


    <!-- http://purl.oclc.org/NET/ldr/ns#Proposition -->

    <owl:Class rdf:about="http://purl.oclc.org/NET/ldr/ns#Proposition">
        <rdfs:comment xml:lang="en">A veritative statement</rdfs:comment>
    </owl:Class>
    


    <!-- http://purl.oclc.org/NET/ldr/ns#PublicCommunication -->

    <owl:Class rdf:about="http://purl.oclc.org/NET/ldr/ns#PublicCommunication">
        <rdfs:subClassOf rdf:resource="http://purl.oclc.org/NET/ldr/ns#IPRight"/>
        <rdfs:comment xml:lang="en">Granting a number of people access to the work without existing distribution</rdfs:comment>
    </owl:Class>
    


    <!-- http://purl.oclc.org/NET/ldr/ns#Reproduction -->

    <owl:Class rdf:about="http://purl.oclc.org/NET/ldr/ns#Reproduction">
        <rdfs:subClassOf rdf:resource="http://purl.oclc.org/NET/ldr/ns#IPRight"/>
        <rdfs:comment xml:lang="en">Direct or indirect fixation, allowing its communication and/or making copies of it</rdfs:comment>
        <skos:exactMatch rdf:resource="&cc;Reproduction"/>
    </owl:Class>
    


    <!-- http://purl.oclc.org/NET/ldr/ns#ResourceLegalStatus -->

    <owl:Class rdf:about="http://purl.oclc.org/NET/ldr/ns#ResourceLegalStatus">
        <rdfs:subClassOf rdf:resource="http://purl.oclc.org/NET/ldr/ns#Proposition"/>
        <rdfs:comment xml:lang="en">Attribute of a resource regarding its legal status</rdfs:comment>
    </owl:Class>
    


    <!-- http://purl.oclc.org/NET/ldr/ns#Reutilization -->

    <owl:Class rdf:about="http://purl.oclc.org/NET/ldr/ns#Reutilization">
        <rdfs:subClassOf rdf:resource="http://purl.oclc.org/NET/ldr/ns#DatabaseRight"/>
        <rdfs:comment xml:lang="en">Right to make available to the public all or a substantial part of the contents of a database by the distribution of copies, by renting, by on-line or other forms of transmission</rdfs:comment>
    </owl:Class>
    


    <!-- http://purl.oclc.org/NET/ldr/ns#SPARQLAccess -->

    <owl:Class rdf:about="http://purl.oclc.org/NET/ldr/ns#SPARQLAccess">
        <rdfs:subClassOf rdf:resource="http://purl.oclc.org/NET/ldr/ns#Access"/>
    </owl:Class>
    


    <!-- http://rdfs.org/ns/void#Dataset -->

    <owl:Class rdf:about="&void;Dataset">
        <rdfs:subClassOf rdf:resource="http://purl.oclc.org/NET/ldr/ns#LinkedDataResource"/>
    </owl:Class>
    


    <!-- http://rdfs.org/ns/void#Linkset -->

    <owl:Class rdf:about="&void;Linkset">
        <rdfs:subClassOf rdf:resource="http://purl.oclc.org/NET/ldr/ns#LinkedDataResource"/>
    </owl:Class>
    


    <!-- http://www.w3.org/1999/02/22-rdf-syntax-ns#Statement -->

    <owl:Class rdf:about="&rdf;Statement">
        <rdfs:subClassOf rdf:resource="http://purl.oclc.org/NET/ldr/ns#LinkedDataResource"/>
    </owl:Class>
    


    <!-- http://www.w3.org/2002/07/owl#Ontology -->

    <owl:Class rdf:about="&owl;Ontology">
        <rdfs:subClassOf rdf:resource="http://purl.oclc.org/NET/ldr/ns#LinkedDataResource"/>
    </owl:Class>
    


    <!-- http://www.w3.org/ns/ldp#Resource -->

    <owl:Class rdf:about="&ldp;Resource">
        <rdfs:subClassOf rdf:resource="http://purl.oclc.org/NET/ldr/ns#LinkedDataResource"/>
    </owl:Class>
    


    <!-- http://www.w3.org/ns/odrl/2/Asset -->

    <owl:Class rdf:about="&odrl;Asset"/>
    


    <!-- http://www.w3.org/ns/odrl/2/Constraint -->

    <owl:Class rdf:about="&odrl;Constraint">
        <rdfs:subClassOf rdf:resource="http://purl.oclc.org/NET/ldr/ns#Proposition"/>
    </owl:Class>
    


    <!-- http://www.w3.org/ns/odrl/2/Policy -->

    <owl:Class rdf:about="&odrl;Policy"/>
    


    <!-- http://www.w3.org/ns/odrl/2/Rule -->

    <owl:Class rdf:about="&odrl;Rule"/>
    


    <!-- urn:mpeg:mpeg21:mco:core:2012#Contract -->

    <owl:Class rdf:about="&mco-core;Contract">
        <rdfs:subClassOf rdf:resource="http://purl.oclc.org/NET/ldr/ns#LinkedDataPolicy"/>
    </owl:Class>
    


    <!-- 
    ///////////////////////////////////////////////////////////////////////////////////////
    //
    // Individuals
    //
    ///////////////////////////////////////////////////////////////////////////////////////
     -->

    


    <!-- http://purl.oclc.org/NET/ldr/ns#HTTPDELETE -->

    <owl:NamedIndividual rdf:about="http://purl.oclc.org/NET/ldr/ns#HTTPDELETE">
        <rdf:type rdf:resource="http://purl.oclc.org/NET/ldr/ns#LDPAccess"/>
        <rdfs:comment xml:lang="en">Accessing with the HTTP DELETE Method</rdfs:comment>
    </owl:NamedIndividual>
    


    <!-- http://purl.oclc.org/NET/ldr/ns#HTTPGET -->

    <owl:NamedIndividual rdf:about="http://purl.oclc.org/NET/ldr/ns#HTTPGET">
        <rdf:type rdf:resource="http://purl.oclc.org/NET/ldr/ns#LDPAccess"/>
        <rdfs:comment xml:lang="en">Accessing with the HTTP GET Method</rdfs:comment>
    </owl:NamedIndividual>
    


    <!-- http://purl.oclc.org/NET/ldr/ns#HTTPPATCH -->

    <owl:NamedIndividual rdf:about="http://purl.oclc.org/NET/ldr/ns#HTTPPATCH">
        <rdf:type rdf:resource="http://purl.oclc.org/NET/ldr/ns#LDPAccess"/>
        <rdfs:comment xml:lang="en">Accesing with the HTTP PATH Method</rdfs:comment>
    </owl:NamedIndividual>
    


    <!-- http://purl.oclc.org/NET/ldr/ns#HTTPPOST -->

    <owl:NamedIndividual rdf:about="http://purl.oclc.org/NET/ldr/ns#HTTPPOST">
        <rdf:type rdf:resource="http://purl.oclc.org/NET/ldr/ns#LDPAccess"/>
        <rdfs:comment xml:lang="en">Accessing with the HTTP POST Method</rdfs:comment>
    </owl:NamedIndividual>
    


    <!-- http://purl.oclc.org/NET/ldr/ns#HTTPPUT -->

    <owl:NamedIndividual rdf:about="http://purl.oclc.org/NET/ldr/ns#HTTPPUT">
        <rdf:type rdf:resource="http://purl.oclc.org/NET/ldr/ns#LDPAccess"/>
        <rdfs:comment xml:lang="en">Accessing with the HTTP PUT Method</rdfs:comment>
    </owl:NamedIndividual>
    


    <!-- http://purl.oclc.org/NET/ldr/ns#LinkedDataAccess -->

    <owl:NamedIndividual rdf:about="http://purl.oclc.org/NET/ldr/ns#LinkedDataAccess">
        <rdf:type rdf:resource="http://purl.oclc.org/NET/ldr/ns#Access"/>
        <rdfs:label xml:lang="en">Retrieval of Linked Data resources</rdfs:label>
    </owl:NamedIndividual>
    


    <!-- http://purl.oclc.org/NET/ldr/ns#SPARQLASK -->

    <owl:NamedIndividual rdf:about="http://purl.oclc.org/NET/ldr/ns#SPARQLASK">
        <rdf:type rdf:resource="http://purl.oclc.org/NET/ldr/ns#SPARQLAccess"/>
        <rdfs:comment xml:lang="en">Access through the SPARQL ASK query form</rdfs:comment>
    </owl:NamedIndividual>
    


    <!-- http://purl.oclc.org/NET/ldr/ns#SPARQLCONSTRUCT -->

    <owl:NamedIndividual rdf:about="http://purl.oclc.org/NET/ldr/ns#SPARQLCONSTRUCT">
        <rdf:type rdf:resource="http://purl.oclc.org/NET/ldr/ns#SPARQLAccess"/>
        <rdfs:comment xml:lang="en">Access through the SPARQL CONSTRUCT query form</rdfs:comment>
    </owl:NamedIndividual>
    


    <!-- http://purl.oclc.org/NET/ldr/ns#SPARQLDESCRIBE -->

    <owl:NamedIndividual rdf:about="http://purl.oclc.org/NET/ldr/ns#SPARQLDESCRIBE">
        <rdf:type rdf:resource="http://purl.oclc.org/NET/ldr/ns#SPARQLAccess"/>
        <rdfs:comment xml:lang="en">Access through the SPARQL DESCRIBE query form</rdfs:comment>
    </owl:NamedIndividual>
    


    <!-- http://purl.oclc.org/NET/ldr/ns#SPARQLSELECT -->

    <owl:NamedIndividual rdf:about="http://purl.oclc.org/NET/ldr/ns#SPARQLSELECT">
        <rdf:type rdf:resource="http://purl.oclc.org/NET/ldr/ns#SPARQLAccess"/>
        <rdfs:comment xml:lang="en">Access through the SPARQL SELECT query form</rdfs:comment>
    </owl:NamedIndividual>
    


    <!-- http://purl.oclc.org/NET/ldr/ns#access -->

    <owl:NamedIndividual rdf:about="http://purl.oclc.org/NET/ldr/ns#access">
        <rdf:type rdf:resource="http://purl.oclc.org/NET/ldr/ns#Access"/>
        <rdfs:comment>Access in any manner or form</rdfs:comment>
    </owl:NamedIndividual>
    


    <!-- http://purl.oclc.org/NET/ldr/ns#baseSoftwareUpon -->

    <owl:NamedIndividual rdf:about="http://purl.oclc.org/NET/ldr/ns#baseSoftwareUpon">
        <rdf:type rdf:resource="http://purl.oclc.org/NET/ldr/ns#Distribution"/>
        <rdfs:comment xml:lang="en">Distribute a pice of software whose well functioning depends on the related Linked Data resource</rdfs:comment>
    </owl:NamedIndividual>
    


    <!-- http://purl.oclc.org/NET/ldr/ns#copyDatabase -->

    <owl:NamedIndividual rdf:about="http://purl.oclc.org/NET/ldr/ns#copyDatabase">
        <rdf:type rdf:resource="http://purl.oclc.org/NET/ldr/ns#Extraction"/>
        <rdfs:comment xml:lang="en">Coyping a dataset, for other purposes than private use</rdfs:comment>
    </owl:NamedIndividual>
    


    <!-- http://purl.oclc.org/NET/ldr/ns#copyWork -->

    <owl:NamedIndividual rdf:about="http://purl.oclc.org/NET/ldr/ns#copyWork">
        <rdf:type rdf:resource="http://purl.oclc.org/NET/ldr/ns#Reproduction"/>
        <rdfs:comment xml:lang="en">copying the work for purposes other than private</rdfs:comment>
    </owl:NamedIndividual>
    


    <!-- http://purl.oclc.org/NET/ldr/ns#derivation -->

    <owl:NamedIndividual rdf:about="http://purl.oclc.org/NET/ldr/ns#derivation">
        <rdf:type rdf:resource="http://purl.oclc.org/NET/ldr/ns#Derivation"/>
        <rdfs:comment xml:lang="en">General transformation of the work</rdfs:comment>
    </owl:NamedIndividual>
    


    <!-- http://purl.oclc.org/NET/ldr/ns#deriveClasses -->

    <owl:NamedIndividual rdf:about="http://purl.oclc.org/NET/ldr/ns#deriveClasses">
        <rdf:type rdf:resource="http://purl.oclc.org/NET/ldr/ns#Derivation"/>
        <rdfs:comment xml:lang="en">Subclassing</rdfs:comment>
    </owl:NamedIndividual>
    


    <!-- http://purl.oclc.org/NET/ldr/ns#deriveProperties -->

    <owl:NamedIndividual rdf:about="http://purl.oclc.org/NET/ldr/ns#deriveProperties">
        <rdf:type rdf:resource="http://purl.oclc.org/NET/ldr/ns#Derivation"/>
        <rdfs:comment xml:lang="en">Subpropertying</rdfs:comment>
    </owl:NamedIndividual>
    


    <!-- http://purl.oclc.org/NET/ldr/ns#distribution -->

    <owl:NamedIndividual rdf:about="http://purl.oclc.org/NET/ldr/ns#distribution">
        <rdf:type rdf:resource="http://purl.oclc.org/NET/ldr/ns#Distribution"/>
        <rdfs:comment xml:lang="en">General act of making available the original work or its copies, in a physical medium</rdfs:comment>
    </owl:NamedIndividual>
    


    <!-- http://purl.oclc.org/NET/ldr/ns#downloadDatabase -->

    <owl:NamedIndividual rdf:about="http://purl.oclc.org/NET/ldr/ns#downloadDatabase">
        <rdf:type rdf:resource="http://purl.oclc.org/NET/ldr/ns#Extraction"/>
        <rdfs:comment xml:lang="en">Downloading a dataset, for other purposes than private use</rdfs:comment>
    </owl:NamedIndividual>
    


    <!-- http://purl.oclc.org/NET/ldr/ns#downloadWork -->

    <owl:NamedIndividual rdf:about="http://purl.oclc.org/NET/ldr/ns#downloadWork">
        <rdf:type rdf:resource="http://purl.oclc.org/NET/ldr/ns#Reproduction"/>
        <rdfs:comment xml:lang="en">downloading the work for purposes other than private</rdfs:comment>
    </owl:NamedIndividual>
    


    <!-- http://purl.oclc.org/NET/ldr/ns#extract -->

    <owl:NamedIndividual rdf:about="http://purl.oclc.org/NET/ldr/ns#extract">
        <rdf:type rdf:resource="http://purl.oclc.org/NET/ldr/ns#Extraction"/>
        <rdfs:comment xml:lang="en">General right of extraction</rdfs:comment>
    </owl:NamedIndividual>
    


    <!-- http://purl.oclc.org/NET/ldr/ns#hasAllRightsReserved -->

    <owl:NamedIndividual rdf:about="http://purl.oclc.org/NET/ldr/ns#hasAllRightsReserved">
        <rdf:type rdf:resource="http://purl.oclc.org/NET/ldr/ns#ResourceLegalStatus"/>
        <rdfs:comment xml:lang="en">Declares that the referred resource is protected under copyright or database rights, and none of them is waived</rdfs:comment>
    </owl:NamedIndividual>
    


    <!-- http://purl.oclc.org/NET/ldr/ns#hasCopyrightExpired -->

    <owl:NamedIndividual rdf:about="http://purl.oclc.org/NET/ldr/ns#hasCopyrightExpired">
        <rdf:type rdf:resource="http://purl.oclc.org/NET/ldr/ns#ResourceLegalStatus"/>
        <rdfs:comment xml:lang="en">Declares that the referred resource has its copyright expired</rdfs:comment>
    </owl:NamedIndividual>
    


    <!-- http://purl.oclc.org/NET/ldr/ns#hasDatabaseRightsExpired -->

    <owl:NamedIndividual rdf:about="http://purl.oclc.org/NET/ldr/ns#hasDatabaseRightsExpired">
        <rdf:type rdf:resource="http://purl.oclc.org/NET/ldr/ns#ResourceLegalStatus"/>
        <rdfs:comment xml:lang="en">Declares that the referred resource has the database rights expired</rdfs:comment>
    </owl:NamedIndividual>
    


    <!-- http://purl.oclc.org/NET/ldr/ns#hasIndustrialSecret -->

    <owl:NamedIndividual rdf:about="http://purl.oclc.org/NET/ldr/ns#hasIndustrialSecret">
        <rdf:type rdf:resource="http://purl.oclc.org/NET/ldr/ns#ResourceLegalStatus"/>
        <rdfs:comment xml:lang="en">The referred resource containts an Industrial Secret</rdfs:comment>
    </owl:NamedIndividual>
    


    <!-- http://purl.oclc.org/NET/ldr/ns#hasNationalSecurityInfo -->

    <owl:NamedIndividual rdf:about="http://purl.oclc.org/NET/ldr/ns#hasNationalSecurityInfo">
        <rdf:type rdf:resource="http://purl.oclc.org/NET/ldr/ns#ResourceLegalStatus"/>
        <rdfs:comment xml:lang="en">Declares that the referred resource has information whose disclosure might harm the national security</rdfs:comment>
    </owl:NamedIndividual>
    


    <!-- http://purl.oclc.org/NET/ldr/ns#hasPersonalData -->

    <owl:NamedIndividual rdf:about="http://purl.oclc.org/NET/ldr/ns#hasPersonalData">
        <rdf:type rdf:resource="http://purl.oclc.org/NET/ldr/ns#ResourceLegalStatus"/>
        <rdfs:comment xml:lang="en">Declares that the referred resource has personal data</rdfs:comment>
    </owl:NamedIndividual>
    


    <!-- http://purl.oclc.org/NET/ldr/ns#hasTopSecret -->

    <owl:NamedIndividual rdf:about="http://purl.oclc.org/NET/ldr/ns#hasTopSecret">
        <rdf:type rdf:resource="http://purl.oclc.org/NET/ldr/ns#ResourceLegalStatus"/>
        <rdfs:comment xml:lang="en">Declares that the referred resource contains top secret information of military nature or other</rdfs:comment>
    </owl:NamedIndividual>
    


    <!-- http://purl.oclc.org/NET/ldr/ns#isInPublicDomain -->

    <owl:NamedIndividual rdf:about="http://purl.oclc.org/NET/ldr/ns#isInPublicDomain">
        <rdf:type rdf:resource="http://purl.oclc.org/NET/ldr/ns#ResourceLegalStatus"/>
        <rdfs:comment xml:lang="en">Declares that the declared resource is in the public domain</rdfs:comment>
    </owl:NamedIndividual>
    


    <!-- http://purl.oclc.org/NET/ldr/ns#judicialProcess -->

    <owl:NamedIndividual rdf:about="http://purl.oclc.org/NET/ldr/ns#judicialProcess">
        <rdf:type rdf:resource="http://purl.oclc.org/NET/ldr/ns#CopyrightException"/>
        <rdfs:comment xml:lang="en">if the action is carried out for the purposes of an administrative or judicial procedure</rdfs:comment>
    </owl:NamedIndividual>
    


    <!-- http://purl.oclc.org/NET/ldr/ns#mirror -->

    <owl:NamedIndividual rdf:about="http://purl.oclc.org/NET/ldr/ns#mirror">
        <rdf:type rdf:resource="http://purl.oclc.org/NET/ldr/ns#Distribution"/>
        <rdfs:comment xml:lang="en">The action of mirroring any piece of Linked Data</rdfs:comment>
    </owl:NamedIndividual>
    


    <!-- http://purl.oclc.org/NET/ldr/ns#nationalSecurity -->

    <owl:NamedIndividual rdf:about="http://purl.oclc.org/NET/ldr/ns#nationalSecurity">
        <rdf:type rdf:resource="http://purl.oclc.org/NET/ldr/ns#CopyrightException"/>
        <rdfs:comment xml:lang="en">if the action is carried out in the interests of public security</rdfs:comment>
    </owl:NamedIndividual>
    


    <!-- http://purl.oclc.org/NET/ldr/ns#publicCommunication -->

    <owl:NamedIndividual rdf:about="http://purl.oclc.org/NET/ldr/ns#publicCommunication">
        <rdf:type rdf:resource="http://purl.oclc.org/NET/ldr/ns#PublicCommunication"/>
        <rdfs:comment xml:lang="en">General right of public communication</rdfs:comment>
    </owl:NamedIndividual>
    


    <!-- http://purl.oclc.org/NET/ldr/ns#publishDatabase -->

    <owl:NamedIndividual rdf:about="http://purl.oclc.org/NET/ldr/ns#publishDatabase">
        <rdf:type rdf:resource="http://purl.oclc.org/NET/ldr/ns#Reutilization"/>
        <rdfs:comment xml:lang="en">Make available a database in internet or by other means</rdfs:comment>
    </owl:NamedIndividual>
    


    <!-- http://purl.oclc.org/NET/ldr/ns#reasonWith -->

    <owl:NamedIndividual rdf:about="http://purl.oclc.org/NET/ldr/ns#reasonWith">
        <rdf:type rdf:resource="http://purl.oclc.org/NET/ldr/ns#Access"/>
        <rdfs:comment xml:lang="en">Accesing Linked Data with the purpose of reasoning, through an specialized protocol (e.g. OWLLink) or not</rdfs:comment>
    </owl:NamedIndividual>
    


    <!-- http://purl.oclc.org/NET/ldr/ns#rebaseURIs -->

    <owl:NamedIndividual rdf:about="http://purl.oclc.org/NET/ldr/ns#rebaseURIs">
        <rdf:type rdf:resource="http://purl.oclc.org/NET/ldr/ns#Derivation"/>
        <rdfs:comment xml:lang="en">Partially change the URI systematically rebasing the entities</rdfs:comment>
    </owl:NamedIndividual>
    


    <!-- http://purl.oclc.org/NET/ldr/ns#reificate -->

    <owl:NamedIndividual rdf:about="http://purl.oclc.org/NET/ldr/ns#reificate">
        <rdf:type rdf:resource="http://purl.oclc.org/NET/ldr/ns#Derivation"/>
        <rdfs:comment xml:lang="en">Reificate an RDF statement or a set thereof</rdfs:comment>
    </owl:NamedIndividual>
    


    <!-- http://purl.oclc.org/NET/ldr/ns#rent -->

    <owl:NamedIndividual rdf:about="http://purl.oclc.org/NET/ldr/ns#rent">
        <rdf:type rdf:resource="http://purl.oclc.org/NET/ldr/ns#Distribution"/>
        <rdfs:comment xml:lang="en">Renting a copy of the work</rdfs:comment>
    </owl:NamedIndividual>
    


    <!-- http://purl.oclc.org/NET/ldr/ns#reproduction -->

    <owl:NamedIndividual rdf:about="http://purl.oclc.org/NET/ldr/ns#reproduction">
        <rdf:type rdf:resource="http://purl.oclc.org/NET/ldr/ns#Reproduction"/>
        <rdfs:comment xml:lang="en">General right of public reproduction</rdfs:comment>
    </owl:NamedIndividual>
    


    <!-- http://purl.oclc.org/NET/ldr/ns#research -->

    <owl:NamedIndividual rdf:about="http://purl.oclc.org/NET/ldr/ns#research">
        <rdf:type rdf:resource="http://purl.oclc.org/NET/ldr/ns#CopyrightException"/>
        <rdfs:comment xml:lang="en">illustration for teaching or scientific research, provided the source, including the author&apos;s name, is acknowledged</rdfs:comment>
    </owl:NamedIndividual>
    


    <!-- http://purl.oclc.org/NET/ldr/ns#reutilization -->

    <owl:NamedIndividual rdf:about="http://purl.oclc.org/NET/ldr/ns#reutilization">
        <rdf:type rdf:resource="http://purl.oclc.org/NET/ldr/ns#Reutilization"/>
        <rdfs:comment xml:lang="en">General right of re-utilization</rdfs:comment>
    </owl:NamedIndividual>
    


    <!-- http://purl.oclc.org/NET/ldr/ns#sell -->

    <owl:NamedIndividual rdf:about="http://purl.oclc.org/NET/ldr/ns#sell">
        <rdf:type rdf:resource="http://purl.oclc.org/NET/ldr/ns#Distribution"/>
        <rdfs:comment xml:lang="en">Selling a copy of the work</rdfs:comment>
    </owl:NamedIndividual>
    


    <!-- http://purl.oclc.org/NET/ldr/ns#sellAccess -->

    <owl:NamedIndividual rdf:about="http://purl.oclc.org/NET/ldr/ns#sellAccess">
        <rdf:type rdf:resource="http://purl.oclc.org/NET/ldr/ns#Distribution"/>
        <rdfs:comment xml:lang="en">Offering for meny the access to a copy of the work</rdfs:comment>
    </owl:NamedIndividual>
    


    <!-- http://purl.oclc.org/NET/ldr/ns#transcodeWork -->

    <owl:NamedIndividual rdf:about="http://purl.oclc.org/NET/ldr/ns#transcodeWork">
        <rdf:type rdf:resource="http://purl.oclc.org/NET/ldr/ns#Derivation"/>
        <skos:example xml:lang="en">Having permission to publish a dataset as NTRIPLES, does not entitle the grantee the act of publishing the dataset as Turtle</skos:example>
        <rdfs:comment xml:lang="en">Transcoding the work</rdfs:comment>
    </owl:NamedIndividual>
    


    <!-- http://purl.oclc.org/NET/ldr/ns#translateWork -->

    <owl:NamedIndividual rdf:about="http://purl.oclc.org/NET/ldr/ns#translateWork">
        <rdf:type rdf:resource="http://purl.oclc.org/NET/ldr/ns#Derivation"/>
        <skos:example xml:lang="en">Having permission to publish a dataset, does not entitle the grantee the act of publishing a tanslated version of it</skos:example>
        <rdfs:comment xml:lang="en">Translating the work</rdfs:comment>
    </owl:NamedIndividual>
    


    <!-- http://purl.org/NET/rdflicense/cc-zero1.0 -->

    <owl:NamedIndividual rdf:about="http://purl.org/NET/rdflicense/cc-zero1.0">
        <rdf:type rdf:resource="http://purl.oclc.org/NET/ldr/ns#FamousDataLicense"/>
        <rdfs:label xml:lang="en">CC0</rdfs:label>
        <rdfs:comment xml:lang="en">Creative Commons public domain waiver</rdfs:comment>
    </owl:NamedIndividual>
    


    <!-- http://purl.org/NET/rdflicense/odbc-by1.0 -->

    <owl:NamedIndividual rdf:about="http://purl.org/NET/rdflicense/odbc-by1.0">
        <rdf:type rdf:resource="http://purl.oclc.org/NET/ldr/ns#FamousDataLicense"/>
        <rdfs:label xml:lang="en">Open Data Commons Attribution</rdfs:label>
        <rdfs:comment xml:lang="en">Attribution for data/databases</rdfs:comment>
    </owl:NamedIndividual>
    


    <!-- http://purl.org/NET/rdflicense/odbc-pddl1.0 -->

    <owl:NamedIndividual rdf:about="http://purl.org/NET/rdflicense/odbc-pddl1.0">
        <rdf:type rdf:resource="http://purl.oclc.org/NET/ldr/ns#FamousDataLicense"/>
        <rdfs:label xml:lang="en">ODC Public Domain Dedication and Licence (PDDL)</rdfs:label>
        <rdfs:comment xml:lang="en">Public Domain for data/databases</rdfs:comment>
    </owl:NamedIndividual>
    


    <!-- http://purl.org/NET/rdflicense/odbl1.0 -->

    <owl:NamedIndividual rdf:about="http://purl.org/NET/rdflicense/odbl1.0">
        <rdf:type rdf:resource="http://purl.oclc.org/NET/ldr/ns#FamousDataLicense"/>
        <rdfs:label xml:lang="en">ODC Open Database License</rdfs:label>
        <rdfs:comment xml:lang="en">Attribution Share-Alike for data/databases</rdfs:comment>
    </owl:NamedIndividual>
    


    <!-- http://www.nationalarchives.gov.uk/doc/open-government-licence/version/2/ -->

    <owl:NamedIndividual rdf:about="http://www.nationalarchives.gov.uk/doc/open-government-licence/version/2/">
        <rdf:type rdf:resource="http://purl.oclc.org/NET/ldr/ns#FamousDataLicense"/>
        <rdfs:label xml:lang="en">UK Open Government License</rdfs:label>
        <rdfs:label xml:lang="en">UK Open Government License for public sector information</rdfs:label>
    </owl:NamedIndividual>
    


    <!-- 
    ///////////////////////////////////////////////////////////////////////////////////////
    //
    // Annotations
    //
    ///////////////////////////////////////////////////////////////////////////////////////
     -->

    <rdf:Description rdf:about="&owl;topObjectProperty">
        <rdfs:comment xml:lang="en">hasIssuer</rdfs:comment>
    </rdf:Description>
    <rdf:Description rdf:about="http://purl.oclc.org/NET/ldr/ns#RightsObject">
        <owl:deprecated rdf:datatype="&xsd;boolean">true</owl:deprecated>
        <rdfs:comment xml:lang="en">Deprecated in favour of ODRL</rdfs:comment>
        <rdfs:comment xml:lang="en">Object over which a right is execised</rdfs:comment>
        <skos:exactMatch rdf:resource="&odrl;Asset"/>
    </rdf:Description>
    <rdf:Description rdf:about="http://purl.oclc.org/NET/ldr/ns#Agent">
        <owl:deprecated rdf:datatype="&xsd;boolean">true</owl:deprecated>
        <rdfs:comment>Agent related to a Linked Data resource</rdfs:comment>
        <rdfs:comment xml:lang="en">Deprecated in favour of the ODRL term</rdfs:comment>
        <skos:exactMatch rdf:resource="&odrl;Party"/>
        <skos:exactMatch rdf:resource="&foaf;Agent"/>
    </rdf:Description>
</rdf:RDF>



<!-- Generated by the OWL API (version 3.4.2) http://owlapi.sourceforge.net -->

