<?xml version="1.0"?>

<!DOCTYPE RDF [
   <!ENTITY rdf  "http://www.w3.org/1999/02/22-rdf-syntax-ns">
   <!ENTITY rdfs "http://www.w3.org/2000/01/rdf-schema">
   <!ENTITY xsd  "http://www.w3.org/2001/XMLSchema">
   <!ENTITY rdfg "http://www.w3.org/2004/03/trix/rdfg-1">
   <!ENTITY swp  "http://www.w3.org/2004/03/trix/swp-1">
]>

<rdf:RDF
  xml:base="&swp;/"
   xmlns:rdf="&rdf;#"
   xmlns:rdfs="&rdfs;#"
   xmlns:xsd="&xsd;#"
   xmlns:rdfg="&rdfg;/"
   xmlns:swp="&swp;/">

   <rdfs:Class rdf:about="&swp;/Authority">
      <rdfs:label>Authority</rdfs:label>
      <rdfs:comment>
An authority, or origin, of a graph; such as a person or company.
      </rdfs:comment>
   </rdfs:Class>

   <rdfs:Class rdf:about="&swp;/Warrant">
      <rdfs:label>Warrant</rdfs:label>
      <rdfs:comment>
A relationship between an authority and a graph, in which the authority is in
some way an origin of that graph. Warrants may include a digital signature of
the graph by the authority.
      </rdfs:comment>
   </rdfs:Class>

   <rdfs:Class rdf:about="&swp;/SignatureMethod">
      <rdfs:label>Signature Method</rdfs:label>
      <rdfs:comment>
A method used to construct a signature used to authenticate a graph.
      </rdfs:comment>
   </rdfs:Class>

   <!--
   <rdfs:Class rdf:about="&swp;/CertificationAuthority">
      <rdfs:label>Certification Authority</rdfs:label>
      <rdfs:comment>
An authority which issues certificates.
      </rdfs:comment>
   </rdfs:Class>
   -->

   <rdf:Property rdf:about="&swp;/assertedBy">
      <rdfs:label>asserted by</rdfs:label>
      <rdfs:comment>
The subject graph originates from and is asserted by the authority specified
for the object warrant. The statements expressed in the graph are taken to be
claims made by that authority. This property has performative semantics.
      </rdfs:comment>
      <rdfs:domain rdf:resource="&rdfg;/Graph"/>
      <rdfs:range rdf:resource="&swp;/Warrant"/>
   </rdf:Property>

   <rdf:Property rdf:about="&swp;/quotedBy">
      <rdfs:label>quoted by</rdfs:label>
      <rdfs:comment>
The subject graph originates from the authority specified for the object warrant.
The statements expressed in the graph are not taken to be claims made by that
authority, insofar as any statement using this property is concerned.
      </rdfs:comment>
      <rdfs:domain rdf:resource="&rdfg;/Graph"/>
      <rdfs:range rdf:resource="&swp;/Warrant"/>
   </rdf:Property>

   <rdf:Property rdf:about="&swp;/authority">
      <rdfs:label>authority</rdfs:label>
      <rdfs:comment>
The object authority is the origin of the graph with which the subject warrant
is associated.
      </rdfs:comment>
      <rdfs:domain rdf:resource="&swp;/Warrant"/>
      <rdfs:range rdf:resource="&swp;/Authority"/>
   </rdf:Property>

   <rdf:Property rdf:about="&swp;/signature">
      <rdfs:label>signature</rdfs:label>
      <rdfs:comment>
The object is the signature to be used to authenticate the graph with which the
subject warrant is associated.
      </rdfs:comment>
      <rdfs:domain rdf:resource="&swp;/Warrant"/>
      <rdfs:range rdf:resource="&xsd;#base64Binary"/>
   </rdf:Property>

   <rdf:Property rdf:about="&swp;/signatureMethod">
      <rdfs:label>signature method</rdfs:label>
      <rdfs:comment>
The object is the signature method by which  the signature specified for the
warrant subject was constructed.
      </rdfs:comment>
      <rdfs:domain rdf:resource="&swp;/Warrant"/>
      <rdfs:range rdf:resource="&swp;/SignatureMethod"/>
   </rdf:Property>

   <rdf:Property rdf:about="&swp;/certificate">
      <rdfs:label>certificate</rdfs:label>
      <rdfs:comment>
The object is a certificate by which the authority specified for the warrant
can be authenticated.
      </rdfs:comment>
      <rdfs:domain rdf:resource="&swp;/Warrant"/>
      <rdfs:range rdf:resource="&xsd;#base64Binary"/>
   </rdf:Property>

   <!--
   <rdf:Property rdf:about="&swp;/certificationAuthority">
      <rdfs:label>certification authority</rdfs:label>
      <rdfs:comment>
The object is the certification authority issuing the certificate specified
for the warrant.
      </rdfs:comment>
      <rdfs:domain rdf:resource="&swp;/Warrant"/>
      <rdfs:range rdf:resource="&swp;/CertificationAuthority"/>
   </rdf:Property>
   -->

   <!--
   <swp:SignatureMethod rdf:about="&swp;/X509">
      <rdfs:label>X509</rdfs:label>
      <rdfs:comment>X509 Signature Method</rdfs:comment>
   </swp:SignatureMethod>

   <swp:SignatureMethod rdf:about="&swp;/PGP">
      <rdfs:label>PGP</rdfs:label>
      <rdfs:comment>The PGP Signature Method</rdfs:comment>
   </swp:SignatureMethod>
   -->

</rdf:RDF>

