<?xml version="1.0" encoding="utf-8"?>
<rdf:RDF
   xmlns:dc="http://purl.org/dc/elements/1.1/"
   xmlns:foaf="http://xmlns.com/foaf/0.1/"
   xmlns:owl="http://www.w3.org/2002/07/owl#"
   xmlns:prv="http://purl.org/ontology/prv/core#"
   xmlns:rdf="http://www.w3.org/1999/02/22-rdf-syntax-ns#"
   xmlns:rdfs="http://www.w3.org/2000/01/rdf-schema#"
   xmlns:spin="http://spinrdf.org/spin#"
   xmlns:status="http://www.w3.org/2003/06/sw-vocab-status/ns#"
   xmlns:vann="http://purl.org/vocab/vann/"
   xmlns:xsd="http://www.w3.org/2001/XMLSchema#"
   xml:base="http://purl.org/ontology/prv/core#">
  <owl:Ontology rdf:about="http://purl.org/ontology/prv/core#">
    <dc:creator rdf:resource="http://foaf.me/zazi#me"/>
    <dc:creator rdf:resource="http://mud.cz/foaf.rdf#ojirio"/>
    <dc:creator rdf:resource="http://richard.cyganiak.de/foaf.rdf#cygri"/>
    <dc:creator rdf:resource="http://tobyinkster.co.uk/#i"/>
    <dc:date rdf:datatype="http://www.w3.org/2001/XMLSchema#dateTime">2011-02-19T14:38:53+01:00</dc:date>
    <dc:description xml:lang="en">A vocabulary for describing the ontology design pattern of property reification. That means the semantic relation of 
a "shortcut relation" (subject, predicate, object) with its detailed description of the relationship.</dc:description>
    <dc:title xml:lang="en">Property Reification Vocabulary</dc:title>
    <vann:preferredNamespacePrefix>prv</vann:preferredNamespacePrefix>
    <vann:preferredNamespaceUri>http://purl.org/ontology/prv/core#</vann:preferredNamespaceUri>
    <spin:imports rdf:resource="http://purl.org/ontology/prv/rules"/>
    <owl:imports rdf:resource="http://purl.org/dc/elements/1.1/"/>
    <owl:imports rdf:resource="http://purl.org/vocab/vann/"/>
    <owl:imports rdf:resource="http://www.w3.org/2003/06/sw-vocab-status/ns"/>
    <owl:imports rdf:resource="http://xmlns.com/foaf/0.1/"/>
    <owl:versionInfo rdf:datatype="http://www.w3.org/2001/XMLSchema#decimal">0.11</owl:versionInfo>
  </owl:Ontology>
  <rdfs:Class rdf:about="http://purl.org/ontology/prv/core#PropertyReification">
    <rdfs:comment xml:lang="en">The class, which describes the relations of a property reification. That means, its "shortcut relation", its 
reification class, and the properties that are relating to the subject and object of the "shortcut relation".</rdfs:comment>
    <rdfs:isDefinedBy rdf:resource="http://purl.org/ontology/prv/core#"/>
    <rdfs:label xml:lang="en">Property Reification</rdfs:label>
    <rdfs:subClassOf rdf:resource="http://www.w3.org/2000/01/rdf-schema#Class"/>
    <status:term_status xml:lang="en">testing</status:term_status>
  </rdfs:Class>
  <rdf:Property rdf:about="http://purl.org/ontology/prv/core#object_property">
    <rdfs:comment xml:lang="en">Relates to the property of the reification class, which relates to the object of the "shortcut relation".</rdfs:comment>
    <rdfs:domain rdf:resource="http://purl.org/ontology/prv/core#PropertyReification"/>
    <rdfs:isDefinedBy rdf:resource="http://purl.org/ontology/prv/core#"/>
    <rdfs:label xml:lang="en">has object property</rdfs:label>
    <rdfs:range rdf:resource="http://www.w3.org/1999/02/22-rdf-syntax-ns#Property"/>
    <status:term_status xml:lang="en">testing</status:term_status>
  </rdf:Property>
  <rdf:Property rdf:about="http://purl.org/ontology/prv/core#reification_class">
    <rdfs:comment xml:lang="en">Relates to the reification class, which can be related to the object and subject property to be able to associate the 
object and subject of the "shortcut relation". The reification class should provide detailed descriptions of the relationship that is 
described in a simple form by the "shortcut relation".</rdfs:comment>
    <rdfs:domain rdf:resource="http://purl.org/ontology/prv/core#PropertyReification"/>
    <rdfs:isDefinedBy rdf:resource="http://purl.org/ontology/prv/core#"/>
    <rdfs:label xml:lang="en">has reification class</rdfs:label>
    <rdfs:range rdf:resource="http://www.w3.org/2000/01/rdf-schema#Class"/>
    <status:term_status xml:lang="en">testing</status:term_status>
  </rdf:Property>
  <rdf:Property rdf:about="http://purl.org/ontology/prv/core#reified">
    <rdfs:comment xml:lang="en">This property relates an statement identifier of a shortcut relation with an instance of a reification class. Although, this is at the moment not really applicable, because it requires a notation for statement identifier as optional fourth element of a tuple; that means, triple + statement identifier.</rdfs:comment>
    <rdfs:domain rdf:resource="http://www.w3.org/2000/01/rdf-schema#Resource"/>
    <rdfs:isDefinedBy rdf:resource="http://purl.org/ontology/prv/core#"/>
    <rdfs:label xml:lang="en">reified</rdfs:label>
    <rdfs:range rdf:resource="http://www.w3.org/2002/07/owl#Thing"/>
    <status:term_status xml:lang="en">testing</status:term_status>
  </rdf:Property>
  <rdf:Property rdf:about="http://purl.org/ontology/prv/core#shortcut">
    <rdfs:comment xml:lang="en">Relates to the property of the "shortcut relation" (its predicate).</rdfs:comment>
    <rdfs:domain rdf:resource="http://purl.org/ontology/prv/core#PropertyReification"/>
    <rdfs:isDefinedBy rdf:resource="http://purl.org/ontology/prv/core#"/>
    <rdfs:label xml:lang="en">has shortcut</rdfs:label>
    <rdfs:range rdf:resource="http://www.w3.org/1999/02/22-rdf-syntax-ns#Property"/>
    <status:term_status xml:lang="en">testing</status:term_status>
  </rdf:Property>
  <rdf:Property rdf:about="http://purl.org/ontology/prv/core#shortcut_property">
    <rdfs:comment xml:lang="en">Relates to the property of the reification class,  which relates to the predicate of the "shortcut relation". So 
that the specific property reification can be "verified" (the property of the prv:shortcut relation and this one associated by the 
referred shortcut property should be equal).</rdfs:comment>
    <rdfs:domain rdf:resource="http://purl.org/ontology/prv/core#PropertyReification"/>
    <rdfs:isDefinedBy rdf:resource="http://purl.org/ontology/prv/core#"/>
    <rdfs:label xml:lang="en">has shortcut property</rdfs:label>
    <rdfs:range rdf:resource="http://www.w3.org/1999/02/22-rdf-syntax-ns#Property"/>
    <status:term_status xml:lang="en">testing</status:term_status>
  </rdf:Property>
  <rdf:Property rdf:about="http://purl.org/ontology/prv/core#subject_property">
    <rdfs:comment xml:lang="en">Relates to the property of the reification class, which relates to the subject of the "shortcut relation".</rdfs:comment>
    <rdfs:domain rdf:resource="http://purl.org/ontology/prv/core#PropertyReification"/>
    <rdfs:isDefinedBy rdf:resource="http://purl.org/ontology/prv/core#"/>
    <rdfs:label xml:lang="en">has subject property</rdfs:label>
    <rdfs:range rdf:resource="http://www.w3.org/1999/02/22-rdf-syntax-ns#Property"/>
    <status:term_status xml:lang="en">testing</status:term_status>
  </rdf:Property>
</rdf:RDF>
