<?xml version="1.0"?>
<rdf:RDF
    xmlns:rdf="http://www.w3.org/1999/02/22-rdf-syntax-ns#"
    xmlns:protege="http://protege.stanford.edu/plugins/owl/protege#"
    xmlns:xsp="http://www.owl-ontologies.com/2005/08/07/xsp.owl#"
    xmlns:owl="http://www.w3.org/2002/07/owl#"
    xmlns:dc="http://purl.org/dc/elements/1.1/"
    xmlns:dcterms="http://purl.org/dc/terms/"
    xmlns:owl2xml="http://www.w3.org/2006/12/owl2-xml#"
    xmlns:xsd="http://www.w3.org/2001/XMLSchema#"
    xmlns:swrl="http://www.w3.org/2003/11/swrl#"
    xmlns:swrlb="http://www.w3.org/2003/11/swrlb#"
    xmlns:dqm="http://purl.org/dqm-vocabulary/v1/dqm#"
    xmlns:rdfs="http://www.w3.org/2000/01/rdf-schema#"
  xml:base="http://purl.org/dqm-vocabulary/v1/dqm" > 
  <rdf:Description rdf:about="#taskDependent">
    <rdf:type rdf:resource="http://www.w3.org/2002/07/owl#FunctionalProperty"/>
    <rdf:type rdf:resource="http://www.w3.org/2002/07/owl#DatatypeProperty"/>
    <rdfs:domain rdf:resource="#DataRequirement"/>
    <rdfs:comment xml:lang="en">Specifies whether the data quality rule is task dependent.</rdfs:comment>
    <rdfs:range rdf:resource="http://www.w3.org/2001/XMLSchema#boolean"/>
    <rdfs:label xml:lang="en">Task Dependent</rdfs:label>
    <rdfs:subPropertyOf rdf:resource="#reqMetadata"/>
  </rdf:Description>
  <rdf:Description rdf:nodeID="A0">
    <rdf:rest rdf:resource="http://www.w3.org/1999/02/22-rdf-syntax-ns#nil"/>
    <rdf:first rdf:resource="#DataRequirement"/>
  </rdf:Description>
  <rdf:Description rdf:about="#subTaskOf">
    <rdf:type rdf:resource="http://www.w3.org/2002/07/owl#TransitiveProperty"/>
    <rdf:type rdf:resource="http://www.w3.org/2002/07/owl#ObjectProperty"/>
    <rdfs:domain rdf:resource="#Task"/>
    <rdfs:comment xml:lang="en">Property that can be used to represent hierachies of between tasks.</rdfs:comment>
    <rdfs:range rdf:resource="#Task"/>
    <rdfs:subPropertyOf rdf:resource="#dataRequirementsRelationship"/>
    <rdfs:label xml:lang="en">Sub Task Of</rdfs:label>
  </rdf:Description>
  <rdf:Description rdf:about="#reqName">
    <rdfs:subPropertyOf rdf:resource="#reqMetadata"/>
    <rdfs:comment xml:lang="en">Specifies the name of a data requirement in natural language.</rdfs:comment>
    <rdfs:label xml:lang="en">Requirement Name</rdfs:label>
    <rdfs:domain rdf:nodeID="A1"/>
    <rdf:type rdf:resource="http://www.w3.org/2002/07/owl#DatatypeProperty"/>
    <rdfs:range rdf:resource="http://www.w3.org/2001/XMLSchema#string"/>
  </rdf:Description>
  <rdf:Description rdf:about="#IllegalValue">
    <rdfs:label xml:lang="en">Illegal Value</rdfs:label>
    <rdf:type rdf:resource="http://www.w3.org/2002/07/owl#Class"/>
    <rdfs:comment xml:lang="en">An illegal value is a data value that must not be used for a property.</rdfs:comment>
    <rdfs:subClassOf rdf:resource="#DataRequirementViolation"/>
  </rdf:Description>
  <rdf:Description rdf:about="#reqDescription">
    <rdfs:subPropertyOf rdf:resource="#reqMetadata"/>
    <rdfs:range rdf:resource="http://www.w3.org/2001/XMLSchema#string"/>
    <rdfs:comment xml:lang="en">Describes a data requirement in natural language.</rdfs:comment>
    <rdfs:domain rdf:resource="#DataRequirement"/>
    <rdfs:label xml:lang="en">Requirement Description</rdfs:label>
    <rdf:type rdf:resource="http://www.w3.org/2002/07/owl#DatatypeProperty"/>
  </rdf:Description>
  <rdf:Description rdf:about="#requiredValue">
    <rdfs:comment xml:lang="en">Specifies whether a value for a property must exist.</rdfs:comment>
    <rdfs:domain rdf:nodeID="A2"/>
    <rdfs:range rdf:resource="http://www.w3.org/2001/XMLSchema#boolean"/>
    <rdfs:label xml:lang="en">Required Value</rdfs:label>
    <rdf:type rdf:resource="http://www.w3.org/2002/07/owl#FunctionalProperty"/>
    <rdf:type rdf:resource="http://www.w3.org/2002/07/owl#DatatypeProperty"/>
  </rdf:Description>
  <rdf:Description rdf:about="#blacklistProperty">
    <rdfs:subPropertyOf rdf:resource="#dataElementRelationship"/>
    <rdfs:domain rdf:resource="#IllegalValueRule"/>
    <rdfs:label xml:lang="en">Blacklist Property</rdfs:label>
    <rdfs:comment xml:lang="en">A blacklist property holds the values that are disallowed for a certain data set.</rdfs:comment>
    <rdfs:range rdf:resource="#BlacklistProperty"/>
    <rdf:type rdf:resource="http://www.w3.org/2002/07/owl#FunctionalProperty"/>
    <rdf:type rdf:resource="http://www.w3.org/2002/07/owl#ObjectProperty"/>
  </rdf:Description>
  <rdf:Description rdf:about="#AffectedProperty">
    <rdfs:label rdf:datatype="http://www.w3.org/2001/XMLSchema#string">Affected Property</rdfs:label>
    <rdfs:subClassOf rdf:resource="#DataElement"/>
    <rdfs:comment xml:lang="en">An affected property specifies the property of a data instance that contains one or more data quality problems.</rdfs:comment>
    <rdf:type rdf:resource="http://www.w3.org/2002/07/owl#Class"/>
  </rdf:Description>
  <rdf:Description rdf:nodeID="A3">
    <owl:unionOf rdf:nodeID="A4"/>
    <rdf:type rdf:resource="http://www.w3.org/2002/07/owl#Class"/>
  </rdf:Description>
  <rdf:Description rdf:nodeID="A1">
    <owl:unionOf rdf:nodeID="A5"/>
    <rdf:type rdf:resource="http://www.w3.org/2002/07/owl#Class"/>
  </rdf:Description>
  <rdf:Description rdf:about="#Completeness">
    <rdfs:comment xml:lang="en">Completeness is the extent to which data are of sufficient breadth, depth, and scope for the task at hand.</rdfs:comment>
    <rdfs:label xml:lang="en">Completeness</rdfs:label>
    <rdf:type rdf:resource="http://www.w3.org/2002/07/owl#Class"/>
    <rdfs:subClassOf rdf:resource="#DataQualityScore"/>
  </rdf:Description>
  <rdf:Description rdf:nodeID="A6">
    <rdf:first rdf:resource="#FuncDepValueRule"/>
    <rdf:rest rdf:resource="http://www.w3.org/1999/02/22-rdf-syntax-ns#nil"/>
  </rdf:Description>
  <rdf:Description rdf:about="#referenceProperty">
    <rdfs:label xml:lang="en">Reference Property</rdfs:label>
    <rdfs:range rdf:resource="#TrustedProperty"/>
    <rdf:type rdf:resource="http://www.w3.org/2002/07/owl#ObjectProperty"/>
    <rdfs:comment xml:lang="en">The reference property points to the URI of a property that holds trusted values, i.e. values of high quality</rdfs:comment>
    <rdfs:subPropertyOf rdf:resource="#dataElementRelationship"/>
  </rdf:Description>
  <rdf:Description rdf:about="http://purl.org/dc/terms/license">
    <rdf:type rdf:resource="http://www.w3.org/2002/07/owl#AnnotationProperty"/>
  </rdf:Description>
  <rdf:Description rdf:nodeID="A7">
    <rdf:first rdf:resource="#FuncDepReferenceRule"/>
    <rdf:rest rdf:nodeID="A8"/>
  </rdf:Description>
  <rdf:Description rdf:nodeID="A2">
    <owl:unionOf rdf:nodeID="A9"/>
    <rdf:type rdf:resource="http://www.w3.org/2002/07/owl#Class"/>
  </rdf:Description>
  <rdf:Description rdf:nodeID="A10">
    <rdf:type rdf:resource="http://www.w3.org/2002/07/owl#Class"/>
    <owl:unionOf rdf:nodeID="A11"/>
  </rdf:Description>
  <rdf:Description rdf:nodeID="A12">
    <rdf:first rdf:resource="#TestedProperty"/>
    <rdf:rest rdf:nodeID="A13"/>
  </rdf:Description>
  <rdf:Description rdf:about="#referenceClass">
    <rdfs:domain rdf:nodeID="A14"/>
    <rdfs:range rdf:resource="#TrustedClass"/>
    <rdfs:subPropertyOf rdf:resource="#dataElementRelationship"/>
    <rdfs:label xml:lang="en">Reference Class</rdfs:label>
    <rdfs:comment xml:lang="en">The reference class property points to the URI of a class that contains trusted instances, i.e. instances of high quality.</rdfs:comment>
    <rdf:type rdf:resource="http://www.w3.org/2002/07/owl#FunctionalProperty"/>
    <rdf:type rdf:resource="http://www.w3.org/2002/07/owl#ObjectProperty"/>
  </rdf:Description>
  <rdf:Description rdf:about="#SemanticAccuracy">
    <rdfs:subClassOf rdf:resource="#Accuracy"/>
    <rdfs:comment xml:lang="en">Semantic accuracy is the degree to which the data values of an instance represent the correct state of an entity’s property.</rdfs:comment>
    <rdf:type rdf:resource="http://www.w3.org/2002/07/owl#Class"/>
    <rdfs:label xml:lang="en">Semantic Accuracy</rdfs:label>
  </rdf:Description>
  <rdf:Description rdf:about="#officialName">
    <rdfs:label xml:lang="en">Official Name</rdfs:label>
    <rdfs:comment xml:lang="en">Official name of a value.</rdfs:comment>
    <rdf:type rdf:resource="http://www.w3.org/2002/07/owl#FunctionalProperty"/>
    <rdf:type rdf:resource="http://www.w3.org/2002/07/owl#DatatypeProperty"/>
    <rdfs:domain rdf:resource="#ScaleValue"/>
    <rdfs:range rdf:resource="http://www.w3.org/2001/XMLSchema#string"/>
  </rdf:Description>
  <rdf:Description rdf:about="#IllegalValueRule">
    <rdf:type rdf:resource="http://www.w3.org/2002/07/owl#Class"/>
    <rdfs:label xml:lang="en">Illegal Value Rule</rdfs:label>
    <rdfs:comment xml:lang="en">An illegal value rule is a property requirement that specifies the values that a certain property must not obtain. Illegal value rules, therefore, refer to reference properties that hold all disallowed values.</rdfs:comment>
    <rdfs:subClassOf rdf:resource="#PropertyRequirement"/>
  </rdf:Description>
  <rdf:Description rdf:nodeID="A15">
    <rdf:type rdf:resource="http://www.w3.org/2002/07/owl#Class"/>
    <owl:unionOf rdf:nodeID="A16"/>
  </rdf:Description>
  <rdf:Description rdf:about="#testedProperty">
    <rdf:type rdf:resource="http://www.w3.org/2002/07/owl#ObjectProperty"/>
    <rdfs:comment xml:lang="en">The property with the values that shall be tested for data quality problems.</rdfs:comment>
    <rdfs:label xml:lang="en">Tested Property</rdfs:label>
    <rdfs:range rdf:resource="#TestedProperty"/>
    <rdfs:subPropertyOf rdf:resource="#dataElementRelationship"/>
  </rdf:Description>
  <rdf:Description rdf:about="#BlacklistProperty">
    <rdfs:comment xml:lang="en">A blacklist property holds the values that are disallowed for a certain data set.</rdfs:comment>
    <rdfs:label xml:lang="en">Blacklist Property</rdfs:label>
    <rdfs:subClassOf rdf:resource="#DataElement"/>
    <rdf:type rdf:resource="http://www.w3.org/2002/07/owl#Class"/>
  </rdf:Description>
  <rdf:Description rdf:about="#UniqueValueRule">
    <rdfs:label xml:lang="en">Unique Value Rule</rdfs:label>
    <rdfs:comment xml:lang="en">A unique value rule is a property requirement that specifies that each value of a certain property must be unique in instances of a certain class.</rdfs:comment>
    <rdfs:subClassOf rdf:resource="#PropertyRequirement"/>
    <rdf:type rdf:resource="http://www.w3.org/2002/07/owl#Class"/>
  </rdf:Description>
  <rdf:Description rdf:about="#ruleViolation">
    <rdfs:comment xml:lang="en">Connects data requirements with data quality problems that have been identified using the requirement.</rdfs:comment>
    <rdfs:subPropertyOf rdf:resource="#dataRequirementsRelationship"/>
    <rdfs:range rdf:resource="#DataRequirementViolation"/>
    <owl:inverseOf rdf:resource="#ruleOfIdentification"/>
    <rdfs:domain rdf:resource="#DataRequirement"/>
    <rdf:type rdf:resource="http://www.w3.org/2002/07/owl#ObjectProperty"/>
    <rdfs:label xml:lang="en">Rule Violation</rdfs:label>
  </rdf:Description>
  <rdf:Description rdf:about="#testedClass">
    <rdfs:comment xml:lang="en">The tested class property specifies the class that holds the instances that shall be tested for data quality problems.</rdfs:comment>
    <rdfs:subPropertyOf rdf:resource="#dataElementRelationship"/>
    <rdfs:domain rdf:resource="#DataRequirement"/>
    <rdf:type rdf:resource="http://www.w3.org/2002/07/owl#FunctionalProperty"/>
    <rdf:type rdf:resource="http://www.w3.org/2002/07/owl#ObjectProperty"/>
    <rdfs:range rdf:resource="#TestedClass"/>
    <rdfs:label xml:lang="en">Tested Class</rdfs:label>
  </rdf:Description>
  <rdf:Description rdf:about="#timeOfIdentification">
    <rdf:type rdf:resource="http://www.w3.org/2002/07/owl#DatatypeProperty"/>
    <rdfs:domain rdf:resource="#DataRequirementViolation"/>
    <rdfs:label xml:lang="en">Time Of Identification</rdfs:label>
    <rdfs:comment xml:lang="en">The time of identification property specifies the date and time in which the data quality problem was detected</rdfs:comment>
    <rdfs:range rdf:resource="http://www.w3.org/2001/XMLSchema#dateTime"/>
  </rdf:Description>
  <rdf:Description rdf:about="#newValue">
    <rdfs:subPropertyOf rdf:resource="#cleansingProperty"/>
    <rdfs:label xml:lang="en">New Value</rdfs:label>
    <rdfs:range rdf:resource="http://www.w3.org/2001/XMLSchema#string"/>
    <rdfs:domain rdf:resource="#ValueSubstitution"/>
    <rdf:type rdf:resource="http://www.w3.org/2002/07/owl#FunctionalProperty"/>
    <rdf:type rdf:resource="http://www.w3.org/2002/07/owl#DatatypeProperty"/>
    <rdfs:comment xml:lang="en">The new value property specifies the new value which shall substitute the current value.</rdfs:comment>
  </rdf:Description>
  <rdf:Description rdf:about="#testedProperty5">
    <rdfs:label xml:lang="en">Tested Property 5</rdfs:label>
    <rdfs:domain rdf:resource="#MatchingValueRule"/>
    <rdf:type rdf:resource="http://www.w3.org/2002/07/owl#FunctionalProperty"/>
    <rdf:type rdf:resource="http://www.w3.org/2002/07/owl#ObjectProperty"/>
    <rdfs:comment xml:lang="en">The property with the values that shall be tested for data quality problems.</rdfs:comment>
    <rdfs:subPropertyOf rdf:resource="#testedProperty"/>
  </rdf:Description>
  <rdf:Description rdf:about="#PropertyUniqueness">
    <rdfs:subClassOf rdf:resource="#Uniqueness"/>
    <rdfs:comment xml:lang="en">Property uniqueness is the degree to which the values of a property (that must only contain unique values within instances of a certain class) are unique.</rdfs:comment>
    <rdfs:label xml:lang="en">Property Uniqueness</rdfs:label>
    <rdf:type rdf:resource="http://www.w3.org/2002/07/owl#Class"/>
  </rdf:Description>
  <rdf:Description rdf:about="#validFrom">
    <rdf:type rdf:resource="http://www.w3.org/2002/07/owl#FunctionalProperty"/>
    <rdf:type rdf:resource="http://www.w3.org/2002/07/owl#DatatypeProperty"/>
    <rdfs:subPropertyOf rdf:resource="#reqMetadata"/>
    <rdfs:comment xml:lang="en">Specifies the date and time from which a rule is valid.</rdfs:comment>
    <rdfs:label xml:lang="en">Valid From</rdfs:label>
    <rdfs:range rdf:resource="http://www.w3.org/2001/XMLSchema#dateTime"/>
    <rdfs:domain rdf:nodeID="A17"/>
  </rdf:Description>
  <rdf:Description rdf:nodeID="A18">
    <rdf:first rdf:resource="#DataCleansingRule"/>
    <rdf:rest rdf:nodeID="A0"/>
  </rdf:Description>
  <rdf:Description rdf:nodeID="A19">
    <rdf:first rdf:resource="#Task"/>
    <rdf:rest rdf:resource="http://www.w3.org/1999/02/22-rdf-syntax-ns#nil"/>
  </rdf:Description>
  <rdf:Description rdf:about="#notEqualTo">
    <rdfs:range rdf:resource="http://www.w3.org/2001/XMLSchema#string"/>
    <rdfs:label xml:lang="en">Not Equal To</rdfs:label>
    <rdfs:subPropertyOf rdf:resource="#operatedValue"/>
    <rdfs:domain rdf:nodeID="A20"/>
    <rdf:type rdf:resource="http://www.w3.org/2002/07/owl#FunctionalProperty"/>
    <rdf:type rdf:resource="http://www.w3.org/2002/07/owl#DatatypeProperty"/>
    <rdfs:comment xml:lang="en">Holds one or more consecutive characters that are used to identify values of another property that do not match with the value of this property.</rdfs:comment>
  </rdf:Description>
  <rdf:Description rdf:about="#basedOn">
    <rdfs:label xml:lang="en">Based On</rdfs:label>
    <rdfs:range rdf:resource="#DataRequirement"/>
    <rdfs:domain rdf:resource="#DataQualityScore"/>
    <rdf:type rdf:resource="http://www.w3.org/2002/07/owl#ObjectProperty"/>
    <owl:inverseOf rdf:resource="#hasScore"/>
    <rdfs:comment xml:lang="en">Connects a data quality score with the data requirements that were used to calculate the score.</rdfs:comment>
    <rdfs:subPropertyOf rdf:resource="#dataRequirementsRelationship"/>
  </rdf:Description>
  <rdf:Description rdf:nodeID="A21">
    <owl:unionOf rdf:nodeID="A18"/>
    <rdf:type rdf:resource="http://www.w3.org/2002/07/owl#Class"/>
  </rdf:Description>
  <rdf:Description rdf:about="#hasURI">
    <rdfs:comment xml:lang="en">The hasURI property is used to map properties to instances of a class.</rdfs:comment>
    <rdfs:label xml:lang="en">Has URI</rdfs:label>
    <rdfs:range rdf:resource="http://www.w3.org/2001/XMLSchema#anyURI"/>
    <rdfs:domain rdf:resource="#DataElement"/>
    <rdf:type rdf:resource="http://www.w3.org/2002/07/owl#FunctionalProperty"/>
    <rdf:type rdf:resource="http://www.w3.org/2002/07/owl#DatatypeProperty"/>
  </rdf:Description>
  <rdf:Description rdf:nodeID="A22">
    <rdf:rest rdf:nodeID="A23"/>
    <rdf:first rdf:resource="#DataElement"/>
  </rdf:Description>
  <rdf:Description rdf:about="#assessedProperty">
    <rdfs:label xml:lang="en">Assessed Property</rdfs:label>
    <rdf:type rdf:resource="http://www.w3.org/2002/07/owl#ObjectProperty"/>
    <rdfs:domain rdf:resource="#DataQualityScore"/>
    <rdfs:comment xml:lang="en">The assessed property represents all properties that have been tested for rule violations during the computation of the assessment score.</rdfs:comment>
    <rdfs:range rdf:resource="#TestedProperty"/>
    <rdfs:subPropertyOf rdf:resource="#dataElementRelationship"/>
  </rdf:Description>
  <rdf:Description rdf:about="#TrustedProperty">
    <rdfs:subClassOf rdf:resource="#DataElement"/>
    <rdfs:comment xml:lang="en">A trusted property holds the values that serve as a trusted reference in legal value rules / functional dependency reference rules, e.g. to define legal values for a tested property.</rdfs:comment>
    <rdfs:label xml:lang="en">Trusted Property</rdfs:label>
    <rdf:type rdf:resource="http://www.w3.org/2002/07/owl#Class"/>
  </rdf:Description>
  <rdf:Description rdf:about="#IllegalValueRangeRule">
    <rdfs:comment xml:lang="en">An illegal value range rule is a property requirement that specifies the upper and/or lower boundary of numeric values that a certain property must not obtain.</rdfs:comment>
    <rdfs:label xml:lang="en">Illegal Value Range Rule</rdfs:label>
    <rdf:type rdf:resource="http://www.w3.org/2002/07/owl#Class"/>
    <rdfs:subClassOf rdf:resource="#PropertyRequirement"/>
  </rdf:Description>
  <rdf:Description rdf:nodeID="A5">
    <rdf:rest rdf:nodeID="A24"/>
    <rdf:first rdf:resource="#DataCleansingRule"/>
  </rdf:Description>
  <rdf:Description rdf:about="#AffectedInstance">
    <rdfs:label xml:lang="en">Affected Instance</rdfs:label>
    <rdfs:comment xml:lang="en">An affected instance is a data instance that contains one or more data quality problems.</rdfs:comment>
    <rdf:type rdf:resource="http://www.w3.org/2002/07/owl#Class"/>
    <rdfs:subClassOf rdf:resource="#DataElement"/>
  </rdf:Description>
  <rdf:Description rdf:about="http://purl.org/dc/elements/1.1/title">
    <rdf:type rdf:resource="http://www.w3.org/2002/07/owl#AnnotationProperty"/>
  </rdf:Description>
  <rdf:Description rdf:nodeID="A25">
    <rdf:first rdf:resource="#Task"/>
    <rdf:rest rdf:resource="http://www.w3.org/1999/02/22-rdf-syntax-ns#nil"/>
  </rdf:Description>
  <rdf:Description rdf:about="#technicalName">
    <rdfs:domain rdf:resource="#ScaleValue"/>
    <rdf:type rdf:resource="http://www.w3.org/2002/07/owl#FunctionalProperty"/>
    <rdf:type rdf:resource="http://www.w3.org/2002/07/owl#DatatypeProperty"/>
    <rdfs:range rdf:resource="http://www.w3.org/2001/XMLSchema#string"/>
    <rdfs:label xml:lang="en">Technical Name</rdfs:label>
    <rdfs:comment xml:lang="en">Technical name of a value.</rdfs:comment>
  </rdf:Description>
  <rdf:Description rdf:nodeID="A26">
    <rdf:first rdf:resource="#MultiPropertyCleansingRule"/>
    <rdf:rest rdf:resource="http://www.w3.org/1999/02/22-rdf-syntax-ns#nil"/>
  </rdf:Description>
  <rdf:Description rdf:about="#requiredProperty">
    <rdf:type rdf:resource="http://www.w3.org/2002/07/owl#FunctionalProperty"/>
    <rdf:type rdf:resource="http://www.w3.org/2002/07/owl#DatatypeProperty"/>
    <rdfs:comment xml:lang="en">Specifies whether a property must exist.</rdfs:comment>
    <rdfs:range rdf:resource="http://www.w3.org/2001/XMLSchema#boolean"/>
    <rdfs:domain rdf:nodeID="A27"/>
    <rdfs:label xml:lang="en">Required Property</rdfs:label>
  </rdf:Description>
  <rdf:Description rdf:nodeID="A28">
    <rdf:first rdf:resource="#IllegalValueRangeRule"/>
    <rdf:rest rdf:nodeID="A29"/>
  </rdf:Description>
  <rdf:Description rdf:nodeID="A30">
    <rdf:type rdf:resource="http://www.w3.org/2002/07/owl#Class"/>
    <owl:unionOf rdf:nodeID="A31"/>
  </rdf:Description>
  <rdf:Description rdf:nodeID="A32">
    <rdf:first rdf:resource="#DataRequirement"/>
    <rdf:rest rdf:nodeID="A19"/>
  </rdf:Description>
  <rdf:Description rdf:about="#validUntil">
    <rdfs:domain rdf:nodeID="A33"/>
    <rdfs:label xml:lang="en">Valid Until</rdfs:label>
    <rdfs:subPropertyOf rdf:resource="#reqMetadata"/>
    <rdf:type rdf:resource="http://www.w3.org/2002/07/owl#FunctionalProperty"/>
    <rdf:type rdf:resource="http://www.w3.org/2002/07/owl#DatatypeProperty"/>
    <rdfs:comment xml:lang="en">Specifies the date and time until a rule stays valid.</rdfs:comment>
    <rdfs:range rdf:resource="http://www.w3.org/2001/XMLSchema#dateTime"/>
  </rdf:Description>
  <rdf:Description rdf:about="#ClassRequirement">
    <rdfs:subClassOf rdf:resource="#DataRequirement"/>
    <rdfs:label xml:lang="en">Class Requirement</rdfs:label>
    <rdf:type rdf:resource="http://www.w3.org/2002/07/owl#Class"/>
    <rdfs:comment xml:lang="en">A class requirement is a data requirement that refers to the instances of a class as a whole.</rdfs:comment>
  </rdf:Description>
  <rdf:Description rdf:about="#TestedProperty">
    <rdfs:subClassOf rdf:resource="#DataElement"/>
    <rdf:type rdf:resource="http://www.w3.org/2002/07/owl#Class"/>
    <rdfs:label xml:lang="en">Tested Property</rdfs:label>
    <rdfs:comment xml:lang="en">A tested property holds the values to be analyzed for data quality problems.</rdfs:comment>
  </rdf:Description>
  <rdf:Description rdf:about="#lastModified">
    <rdf:type rdf:resource="http://www.w3.org/2002/07/owl#FunctionalProperty"/>
    <rdf:type rdf:resource="http://www.w3.org/2002/07/owl#DatatypeProperty"/>
    <rdfs:label xml:lang="en">Last Modified</rdfs:label>
    <rdfs:comment xml:lang="en">The property lastModified indicates the date and time when the rule was last modified.</rdfs:comment>
    <rdfs:range rdf:resource="http://www.w3.org/2001/XMLSchema#dateTime"/>
    <rdfs:subPropertyOf rdf:resource="#reqMetadata"/>
    <rdfs:domain rdf:resource="#DataRequirement"/>
  </rdf:Description>
  <rdf:Description rdf:about="#blacklistClass">
    <rdfs:comment xml:lang="en">A blacklist class holds instances with values that are disallowed for a certain data set.</rdfs:comment>
    <rdfs:subPropertyOf rdf:resource="#dataElementRelationship"/>
    <rdfs:domain rdf:resource="#IllegalValueRule"/>
    <rdfs:range rdf:resource="#BlacklistClass"/>
    <rdf:type rdf:resource="http://www.w3.org/2002/07/owl#FunctionalProperty"/>
    <rdf:type rdf:resource="http://www.w3.org/2002/07/owl#ObjectProperty"/>
    <rdfs:label xml:lang="en">Blacklist Class</rdfs:label>
  </rdf:Description>
  <rdf:Description rdf:nodeID="A11">
    <rdf:rest rdf:nodeID="A34"/>
    <rdf:first rdf:resource="#Condition"/>
  </rdf:Description>
  <rdf:Description rdf:about="#dataCleansingRuleRelationship">
    <rdf:type rdf:resource="http://www.w3.org/2002/07/owl#ObjectProperty"/>
    <rdfs:label xml:lang="en">Data Cleansing Rule Relationship</rdfs:label>
    <rdfs:comment xml:lang="en">Data cleansing rule relationships are object properties of the data cleansing rules.</rdfs:comment>
  </rdf:Description>
  <rdf:Description rdf:about="#affectedInstance">
    <rdfs:comment xml:lang="de">An affected instance is the data instance that contains one or more data requirement violations.</rdfs:comment>
    <rdfs:domain rdf:resource="#DataRequirementViolation"/>
    <rdfs:range rdf:resource="#AffectedInstance"/>
    <rdfs:subPropertyOf rdf:resource="#dataElementRelationship"/>
    <rdf:type rdf:resource="http://www.w3.org/2002/07/owl#ObjectProperty"/>
    <rdfs:label xml:lang="de">Affected Instance</rdfs:label>
  </rdf:Description>
  <rdf:Description rdf:nodeID="A35">
    <rdf:rest rdf:resource="http://www.w3.org/1999/02/22-rdf-syntax-ns#nil"/>
    <rdf:first rdf:resource="#FuncDepValueRule"/>
  </rdf:Description>
  <rdf:Description rdf:about="#ExpiryRule">
    <rdfs:subClassOf rdf:resource="#OutdatedInstanceRule"/>
    <rdfs:comment xml:lang="en">An expiry rule is an outdated instance rule that specifies the expiration date of an instance that must not exceed the current date and time. Therefore, expiry rules require date information about the validity period of an instance.</rdfs:comment>
    <rdf:type rdf:resource="http://www.w3.org/2002/07/owl#Class"/>
    <rdfs:label xml:lang="en">Expiry Rule</rdfs:label>
  </rdf:Description>
  <rdf:Description rdf:nodeID="A36">
    <owl:unionOf rdf:nodeID="A28"/>
    <rdf:type rdf:resource="http://www.w3.org/2002/07/owl#Class"/>
  </rdf:Description>
  <rdf:Description rdf:about="#lessThan">
    <rdfs:label xml:lang="en">Less Than</rdfs:label>
    <rdfs:comment xml:lang="en">Holds a numeric value that is used to identify values of a property that are less than the value of this property.</rdfs:comment>
    <rdfs:subPropertyOf rdf:resource="#operatedValue"/>
    <rdfs:domain rdf:nodeID="A10"/>
    <rdfs:range rdf:resource="http://www.w3.org/2001/XMLSchema#float"/>
    <rdf:type rdf:resource="http://www.w3.org/2002/07/owl#FunctionalProperty"/>
    <rdf:type rdf:resource="http://www.w3.org/2002/07/owl#DatatypeProperty"/>
  </rdf:Description>
  <rdf:Description rdf:about="#contains">
    <rdfs:domain rdf:nodeID="A37"/>
    <rdfs:comment xml:lang="en">Holds one or more consecutive characters that are supposed to be found in strings of another property.</rdfs:comment>
    <rdfs:subPropertyOf rdf:resource="#operatedValue"/>
    <rdfs:label xml:lang="en">Contains</rdfs:label>
    <rdfs:range rdf:resource="http://www.w3.org/2001/XMLSchema#string"/>
    <rdf:type rdf:resource="http://www.w3.org/2002/07/owl#FunctionalProperty"/>
    <rdf:type rdf:resource="http://www.w3.org/2002/07/owl#DatatypeProperty"/>
  </rdf:Description>
  <rdf:Description rdf:nodeID="A38">
    <rdf:rest rdf:nodeID="A39"/>
    <rdf:first rdf:resource="#ConditionalRule"/>
  </rdf:Description>
  <rdf:Description rdf:about="#dataRequirementsRelationship">
    <rdfs:comment xml:lang="en">The data requirements relationship property is an abstract property that holds object properties that are used to define internal and external relationships of data requirements.</rdfs:comment>
    <rdfs:label xml:lang="en">Data Requirements Relationship</rdfs:label>
    <rdf:type rdf:resource="http://www.w3.org/2002/07/owl#ObjectProperty"/>
  </rdf:Description>
  <rdf:Description rdf:about="#ConditionalSyntaxRule">
    <rdfs:label xml:lang="en">Conditional Syntax Rule</rdfs:label>
    <rdfs:subClassOf rdf:resource="#ConditionalRule"/>
    <rdf:type rdf:resource="http://www.w3.org/2002/07/owl#Class"/>
    <rdfs:comment xml:lang="en">Conditional syntax rules define that the literal values of a tested property must follow a certain syntax when the value of another property obtains a certain state. E.g. the property foo:state must have a value with two capital letters when the property foo:country obtains the value "USA".</rdfs:comment>
  </rdf:Description>
  <rdf:Description rdf:about="#upperLimit">
    <rdfs:range rdf:resource="http://www.w3.org/2001/XMLSchema#float"/>
    <rdfs:comment xml:lang="en">Specifies the upper limit a numeric property value shall obtain.</rdfs:comment>
    <rdfs:domain rdf:nodeID="A40"/>
    <rdfs:label xml:lang="en">Upper Limit</rdfs:label>
    <rdf:type rdf:resource="http://www.w3.org/2002/07/owl#FunctionalProperty"/>
    <rdf:type rdf:resource="http://www.w3.org/2002/07/owl#DatatypeProperty"/>
  </rdf:Description>
  <rdf:Description rdf:about="http://purl.org/dc/elements/1.1/rights">
    <rdf:type rdf:resource="http://www.w3.org/2002/07/owl#AnnotationProperty"/>
  </rdf:Description>
  <rdf:Description rdf:about="#rank">
    <rdfs:label xml:lang="en">Rank</rdfs:label>
    <rdfs:range rdf:resource="http://www.w3.org/2001/XMLSchema#int"/>
    <rdfs:comment xml:lang="en">Position of a value in an ordinal scale.</rdfs:comment>
    <rdf:type rdf:resource="http://www.w3.org/2002/07/owl#FunctionalProperty"/>
    <rdf:type rdf:resource="http://www.w3.org/2002/07/owl#DatatypeProperty"/>
    <rdfs:domain rdf:resource="#ScaleValue"/>
  </rdf:Description>
  <rdf:Description rdf:nodeID="A41">
    <owl:unionOf rdf:nodeID="A42"/>
    <rdf:type rdf:resource="http://www.w3.org/2002/07/owl#Class"/>
  </rdf:Description>
  <rdf:Description rdf:about="#MultiPropertyRequirement">
    <rdfs:label xml:lang="en">Multi Property Requirement</rdfs:label>
    <rdfs:comment xml:lang="en">Multi property requirements are data requirements that consider values from two or more properties.</rdfs:comment>
    <rdf:type rdf:resource="http://www.w3.org/2002/07/owl#Class"/>
    <rdfs:subClassOf rdf:resource="#DataRequirement"/>
  </rdf:Description>
  <rdf:Description rdf:about="#affectedClass">
    <rdfs:subPropertyOf rdf:resource="#dataElementRelationship"/>
    <rdf:type rdf:resource="http://www.w3.org/2002/07/owl#ObjectProperty"/>
    <rdfs:comment xml:lang="en">An affected class holds one or more instances with one or more data requirement violations.</rdfs:comment>
    <rdfs:range rdf:resource="#AffectedClass"/>
    <rdfs:label xml:lang="en">Affected Class</rdfs:label>
    <rdfs:domain rdf:resource="#DataRequirementViolation"/>
  </rdf:Description>
  <rdf:Description rdf:about="#AffectedClass">
    <rdfs:comment xml:lang="en">An affected class holds one or more affected instances</rdfs:comment>
    <rdfs:label rdf:datatype="http://www.w3.org/2001/XMLSchema#string">Affected Class</rdfs:label>
    <rdfs:subClassOf rdf:resource="#DataElement"/>
    <rdf:type rdf:resource="http://www.w3.org/2002/07/owl#Class"/>
  </rdf:Description>
  <rdf:Description rdf:nodeID="A43">
    <rdf:first rdf:datatype="http://www.w3.org/2001/XMLSchema#string">ordinal</rdf:first>
    <rdf:rest rdf:nodeID="A44"/>
  </rdf:Description>
  <rdf:Description rdf:nodeID="A45">
    <rdf:rest rdf:nodeID="A46"/>
    <rdf:first rdf:resource="#Condition"/>
  </rdf:Description>
  <rdf:Description rdf:about="#cleansingProperty">
    <rdf:type rdf:resource="http://www.w3.org/2002/07/owl#DatatypeProperty"/>
    <rdfs:label xml:lang="en">Cleansing Property</rdfs:label>
    <rdfs:comment xml:lang="en">Cleansing properties are properties of data cleansing rules.</rdfs:comment>
  </rdf:Description>
  <rdf:Description rdf:about="#unitOfMeasurement">
    <rdfs:domain rdf:resource="#DataQualityScore"/>
    <rdfs:comment xml:lang="en">Indicates the unit of measurement, e.g. of data quality scores. It is recommended to use UN/CEFACT common codes to specify the unit of measurement, e.g. "P1" stands for percent.</rdfs:comment>
    <rdf:type rdf:resource="http://www.w3.org/2002/07/owl#FunctionalProperty"/>
    <rdf:type rdf:resource="http://www.w3.org/2002/07/owl#ObjectProperty"/>
    <rdfs:range rdf:resource="#Unit"/>
    <rdfs:label xml:lang="en">Unit of Measurement</rdfs:label>
  </rdf:Description>
  <rdf:Description rdf:about="#hasCondition1">
    <rdfs:label xml:lang="en">Has Condition 1</rdfs:label>
    <rdf:type rdf:resource="http://www.w3.org/2002/07/owl#FunctionalProperty"/>
    <rdf:type rdf:resource="http://www.w3.org/2002/07/owl#ObjectProperty"/>
    <rdfs:comment xml:lang="en">Connects a conditional rule with a certain condition.</rdfs:comment>
    <rdfs:subPropertyOf rdf:resource="#hasCondition"/>
    <rdfs:domain rdf:nodeID="A47"/>
  </rdf:Description>
  <rdf:Description rdf:about="#ConditionalRule">
    <rdf:type rdf:resource="http://www.w3.org/2002/07/owl#Class"/>
    <rdfs:label xml:lang="en">Conditional Rule</rdfs:label>
    <rdfs:comment xml:lang="en">A conditional rule is a multi property requirement that can be used to specify that values of a tested property A must always obtain a certain state under the condition that values of another property B obtain a certain state (condition).</rdfs:comment>
    <rdfs:subClassOf rdf:resource="#MultiPropertyRequirement"/>
  </rdf:Description>
  <rdf:Description rdf:about="#SyntacticAccuracy">
    <rdfs:subClassOf rdf:resource="#Accuracy"/>
    <rdfs:label xml:lang="en">Syntactic Accuracy</rdfs:label>
    <rdf:type rdf:resource="http://www.w3.org/2002/07/owl#Class"/>
    <rdfs:comment xml:lang="en">Syntactic accuracy is the degree to which data values of a property represent legal values and are free from syntax violations.</rdfs:comment>
  </rdf:Description>
  <rdf:Description rdf:nodeID="A34">
    <rdf:first rdf:resource="#FuncDepValueRule"/>
    <rdf:rest rdf:resource="http://www.w3.org/1999/02/22-rdf-syntax-ns#nil"/>
  </rdf:Description>
  <rdf:Description rdf:about="#expectedUpdateInterval">
    <rdfs:comment xml:lang="en">The expected update interval specifies the time interval in which instances of a specific class must be updated in order to be current.</rdfs:comment>
    <rdfs:range rdf:resource="http://www.w3.org/2001/XMLSchema#duration"/>
    <rdf:type rdf:resource="http://www.w3.org/2002/07/owl#FunctionalProperty"/>
    <rdf:type rdf:resource="http://www.w3.org/2002/07/owl#DatatypeProperty"/>
    <rdfs:domain rdf:resource="#UpdateRule"/>
    <rdfs:label xml:lang="en">Expected Update Interval</rdfs:label>
  </rdf:Description>
  <rdf:Description rdf:nodeID="A48">
    <owl:unionOf rdf:nodeID="A49"/>
    <rdf:type rdf:resource="http://www.w3.org/2002/07/owl#Class"/>
  </rdf:Description>
  <rdf:Description rdf:about="http://purl.org/dc/elements/1.1/subject">
    <rdf:type rdf:resource="http://www.w3.org/2002/07/owl#AnnotationProperty"/>
  </rdf:Description>
  <rdf:Description rdf:about="#FuncDepValueRule">
    <rdfs:subClassOf rdf:resource="#ConditionalRule"/>
    <rdfs:label xml:lang="en">Functionally Dependent Value Rule</rdfs:label>
    <rdfs:comment xml:lang="en">A functionally dependent value rule defines that the value of a tested property must have a certain value when the values of other properties obtain certain states (conditions). E.g. the property foo:inStock must have value "true" when the property foo:availableAmount is greater than zero.</rdfs:comment>
    <rdf:type rdf:resource="http://www.w3.org/2002/07/owl#Class"/>
  </rdf:Description>
  <rdf:Description rdf:about="#MatchingValueRule">
    <rdfs:label xml:lang="en">Matching Value Rule</rdfs:label>
    <rdfs:comment xml:lang="en">Matching value rules are multi property requirements in which the property values of other instances are used to identify data requirements violations in an instance.</rdfs:comment>
    <rdf:type rdf:resource="http://www.w3.org/2002/07/owl#Class"/>
    <rdfs:subClassOf rdf:resource="#MultiPropertyRequirement"/>
  </rdf:Description>
  <rdf:Description rdf:about="#BlacklistClass">
    <rdfs:comment xml:lang="en">A blacklist class holds instances with values that are disallowed for a certain data set. Thus, illegal value rules refer to such classes over the blacklist class property.</rdfs:comment>
    <rdfs:label xml:lang="en">Blacklist Class</rdfs:label>
    <rdfs:subClassOf rdf:resource="#DataElement"/>
    <rdf:type rdf:resource="http://www.w3.org/2002/07/owl#Class"/>
  </rdf:Description>
  <rdf:Description rdf:about="http://purl.org/dc/elements/1.1/creator">
    <rdf:type rdf:resource="http://www.w3.org/2002/07/owl#AnnotationProperty"/>
  </rdf:Description>
  <rdf:Description rdf:about="#SyntaxViolation">
    <rdfs:label xml:lang="en">Syntax Violation</rdfs:label>
    <rdf:type rdf:resource="http://www.w3.org/2002/07/owl#Class"/>
    <rdfs:comment xml:lang="en">A syntax violation is a data requirement violation that occurs when a data value contains disallowed characters or does not match a predefined pattern.</rdfs:comment>
    <rdfs:subClassOf rdf:resource="#DataRequirementViolation"/>
  </rdf:Description>
  <rdf:Description rdf:about="#OutOfRangeValue">
    <rdfs:subClassOf rdf:resource="#DataRequirementViolation"/>
    <rdf:type rdf:resource="http://www.w3.org/2002/07/owl#Class"/>
    <rdfs:label rdf:datatype="http://www.w3.org/2001/XMLSchema#string">Out of Range Value</rdfs:label>
    <rdfs:comment xml:lang="en">A value is out of range when it is not part of the legal value range or when it is part of the illegal value range.</rdfs:comment>
  </rdf:Description>
  <rdf:Description rdf:about="#hasCondition2">
    <rdf:type rdf:resource="http://www.w3.org/2002/07/owl#FunctionalProperty"/>
    <rdf:type rdf:resource="http://www.w3.org/2002/07/owl#ObjectProperty"/>
    <rdfs:comment xml:lang="en">Connects a conditional rule with a certain condition.</rdfs:comment>
    <rdfs:subPropertyOf rdf:resource="#hasCondition"/>
    <rdfs:domain rdf:nodeID="A3"/>
    <rdfs:label xml:lang="en">Has Condition 2</rdfs:label>
  </rdf:Description>
  <rdf:Description rdf:about="#greaterThan">
    <rdfs:domain rdf:nodeID="A50"/>
    <rdfs:subPropertyOf rdf:resource="#operatedValue"/>
    <rdfs:comment xml:lang="en">Holds a numeric value that is used to identify values of a property that are greater than the value of this property.</rdfs:comment>
    <rdfs:label xml:lang="en">Greater Than</rdfs:label>
    <rdfs:range rdf:resource="http://www.w3.org/2001/XMLSchema#float"/>
    <rdf:type rdf:resource="http://www.w3.org/2002/07/owl#FunctionalProperty"/>
    <rdf:type rdf:resource="http://www.w3.org/2002/07/owl#DatatypeProperty"/>
  </rdf:Description>
  <rdf:Description rdf:about="#timeOfAssessment">
    <rdfs:domain rdf:resource="#DataQualityScore"/>
    <rdfs:comment xml:lang="en">The time of assessment represents the data and time when the data quality score was computed.</rdfs:comment>
    <rdf:type rdf:resource="http://www.w3.org/2002/07/owl#DatatypeProperty"/>
    <rdfs:label xml:lang="en">Time Of Assessment</rdfs:label>
    <rdfs:range rdf:resource="http://www.w3.org/2001/XMLSchema#dateTime"/>
  </rdf:Description>
  <rdf:Description rdf:about="#currentValue">
    <rdfs:subPropertyOf rdf:resource="#cleansingProperty"/>
    <rdfs:label xml:lang="en">Current Value</rdfs:label>
    <rdfs:domain rdf:resource="#ValueSubstitution"/>
    <rdfs:range rdf:resource="http://www.w3.org/2001/XMLSchema#string"/>
    <rdf:type rdf:resource="http://www.w3.org/2002/07/owl#FunctionalProperty"/>
    <rdf:type rdf:resource="http://www.w3.org/2002/07/owl#DatatypeProperty"/>
    <rdfs:comment xml:lang="en">The current value propertiy specifies the value to be removed.</rdfs:comment>
  </rdf:Description>
  <rdf:Description rdf:nodeID="A51">
    <rdf:first rdf:resource="#LegalValueRangeRule"/>
    <rdf:rest rdf:nodeID="A52"/>
  </rdf:Description>
  <rdf:Description rdf:nodeID="A16">
    <rdf:first rdf:resource="#AffectedClass"/>
    <rdf:rest rdf:nodeID="A53"/>
  </rdf:Description>
  <rdf:Description rdf:about="#referenceProperty1">
    <rdfs:domain rdf:nodeID="A54"/>
    <rdfs:label xml:lang="en">Reference Property 1</rdfs:label>
    <rdf:type rdf:resource="http://www.w3.org/2002/07/owl#FunctionalProperty"/>
    <rdf:type rdf:resource="http://www.w3.org/2002/07/owl#ObjectProperty"/>
    <rdfs:subPropertyOf rdf:resource="#referenceProperty"/>
    <rdfs:comment xml:lang="en">The reference property points to the URI of a property that holds trusted values, i.e. values of high quality</rdfs:comment>
  </rdf:Description>
  <rdf:Description rdf:about="#PropertyCompletenessRule">
    <rdfs:subClassOf rdf:resource="#PropertyRequirement"/>
    <rdf:type rdf:resource="http://www.w3.org/2002/07/owl#Class"/>
    <rdfs:label xml:lang="en">Property Completeness Rule</rdfs:label>
    <rdfs:comment xml:lang="en">A property completeness rule is a data requirement that specifies that a certain property and/or its value must exist in all instances of a certain class.</rdfs:comment>
  </rdf:Description>
  <rdf:Description rdf:nodeID="A55">
    <rdf:rest rdf:resource="http://www.w3.org/1999/02/22-rdf-syntax-ns#nil"/>
    <rdf:first rdf:resource="#MultiPropertyCleansingRule"/>
  </rdf:Description>
  <rdf:Description rdf:nodeID="A13">
    <rdf:first rdf:resource="#TrustedProperty"/>
    <rdf:rest rdf:resource="http://www.w3.org/1999/02/22-rdf-syntax-ns#nil"/>
  </rdf:Description>
  <rdf:Description rdf:about="#DuplicateInstanceRule">
    <rdf:type rdf:resource="http://www.w3.org/2002/07/owl#Class"/>
    <rdfs:subClassOf rdf:resource="#MatchingValueRule"/>
    <rdfs:comment xml:lang="en">A duplicate instance rule is a multi property requirement which specifies the properties that (when seen together) uniquely identify an entity. I.e. if the properties of two or more different instances represent the same state, then the instances represent the same entity. Thus, the instances are considered to be duplicates.</rdfs:comment>
    <rdfs:label xml:lang="en">Duplicate Instance Rule</rdfs:label>
  </rdf:Description>
  <rdf:Description rdf:about="#MissingValue">
    <rdf:type rdf:resource="http://www.w3.org/2002/07/owl#Class"/>
    <rdfs:label xml:lang="en">Missing Value</rdfs:label>
    <rdfs:comment xml:lang="en">A missing value occurs when a property of an instance does not hold a value.</rdfs:comment>
    <rdfs:subClassOf rdf:resource="#MissingElement"/>
  </rdf:Description>
  <rdf:Description rdf:about="#hasCondition3">
    <rdfs:label xml:lang="en">Has Condition 3</rdfs:label>
    <rdfs:domain rdf:nodeID="A56"/>
    <rdf:type rdf:resource="http://www.w3.org/2002/07/owl#FunctionalProperty"/>
    <rdf:type rdf:resource="http://www.w3.org/2002/07/owl#ObjectProperty"/>
    <rdfs:comment xml:lang="en">Connects a conditional rule with a certain condition.</rdfs:comment>
    <rdfs:subPropertyOf rdf:resource="#hasCondition"/>
  </rdf:Description>
  <rdf:Description rdf:about="#TestedClass">
    <rdfs:label xml:lang="en">Tested Class</rdfs:label>
    <rdfs:comment xml:lang="en">A tested class is a class that holds the instances that shall be analyzed for data quality problems.</rdfs:comment>
    <rdf:type rdf:resource="http://www.w3.org/2002/07/owl#Class"/>
    <rdfs:subClassOf rdf:resource="#DataElement"/>
  </rdf:Description>
  <rdf:Description rdf:about="#ValueSubstitution">
    <rdfs:subClassOf rdf:resource="#LiteralCleansingRule"/>
    <rdfs:label xml:lang="en">Value Substitution Rule</rdfs:label>
    <rdfs:comment xml:lang="en">A value substitution rule specifies a value to be removed and a new value that shall substitute the removed value.</rdfs:comment>
    <rdf:type rdf:resource="http://www.w3.org/2002/07/owl#Class"/>
  </rdf:Description>
  <rdf:Description rdf:about="#unitName">
    <rdfs:domain rdf:resource="#Unit"/>
    <rdfs:label xml:lang="en">Unit Name</rdfs:label>
    <rdfs:comment xml:lang="en">Name of a unit of measurement.</rdfs:comment>
    <rdfs:range rdf:resource="http://www.w3.org/2001/XMLSchema#string"/>
    <rdf:type rdf:resource="http://www.w3.org/2002/07/owl#DatatypeProperty"/>
  </rdf:Description>
  <rdf:Description rdf:nodeID="A57">
    <rdf:rest rdf:resource="http://www.w3.org/1999/02/22-rdf-syntax-ns#nil"/>
    <rdf:first rdf:resource="#TrustedClass"/>
  </rdf:Description>
  <rdf:Description rdf:about="#hasProperties">
    <rdfs:subPropertyOf rdf:resource="#dataElementRelationship"/>
    <rdf:type rdf:resource="http://www.w3.org/2002/07/owl#ObjectProperty"/>
    <rdfs:range rdf:nodeID="A58"/>
    <rdfs:comment xml:lang="en">Reconnects mapped classes and properties with each other.</rdfs:comment>
    <rdfs:label xml:lang="en">Has Properties</rdfs:label>
    <rdfs:domain rdf:nodeID="A15"/>
  </rdf:Description>
  <rdf:Description rdf:about="#FunctionalDependencyViolation">
    <rdfs:comment xml:lang="en">A functional dependency violation is a combination of different property values within the same instance that must not occur together. E.g. an instance describing the man “Peter Miller” has the value “Mr.” as salutation property, but the value “female” as sex.</rdfs:comment>
    <rdfs:label xml:lang="en">Functional Dependency Violation</rdfs:label>
    <rdf:type rdf:resource="http://www.w3.org/2002/07/owl#Class"/>
    <rdfs:subClassOf rdf:resource="#DataRequirementViolation"/>
  </rdf:Description>
  <rdf:Description rdf:about="#next">
    <rdfs:domain rdf:resource="#ScaleValue"/>
    <rdfs:range rdf:resource="#ScaleValue"/>
    <rdf:type rdf:resource="http://www.w3.org/2002/07/owl#ObjectProperty"/>
    <rdfs:comment xml:lang="en">Links an instances to the next instance in an ordinal scale.</rdfs:comment>
  </rdf:Description>
  <rdf:Description rdf:about="#referenceProperty2">
    <rdfs:subPropertyOf rdf:resource="#referenceProperty"/>
    <rdfs:label xml:lang="en">Reference Property 2</rdfs:label>
    <rdfs:comment xml:lang="en">The reference property points to the URI of a property that holds trusted values, i.e. values of high quality</rdfs:comment>
    <rdfs:domain rdf:resource="#FuncDepReferenceRule"/>
    <rdf:type rdf:resource="http://www.w3.org/2002/07/owl#FunctionalProperty"/>
    <rdf:type rdf:resource="http://www.w3.org/2002/07/owl#ObjectProperty"/>
  </rdf:Description>
  <rdf:Description rdf:nodeID="A40">
    <rdf:type rdf:resource="http://www.w3.org/2002/07/owl#Class"/>
    <owl:unionOf rdf:nodeID="A59"/>
  </rdf:Description>
  <rdf:Description rdf:nodeID="A39">
    <rdf:rest rdf:resource="http://www.w3.org/1999/02/22-rdf-syntax-ns#nil"/>
    <rdf:first rdf:resource="#MultiPropertyCleansingRule"/>
  </rdf:Description>
  <rdf:Description rdf:about="#Accuracy">
    <rdfs:comment xml:lang="en">Accuracy is the degree to which a data value represents the desired state regarding its syntax and semantics.</rdfs:comment>
    <rdf:type rdf:resource="http://www.w3.org/2002/07/owl#Class"/>
    <rdfs:subClassOf rdf:resource="#DataQualityScore"/>
    <rdfs:label xml:lang="en">Accuracy</rdfs:label>
  </rdf:Description>
  <rdf:Description rdf:nodeID="A33">
    <rdf:type rdf:resource="http://www.w3.org/2002/07/owl#Class"/>
    <owl:unionOf rdf:nodeID="A60"/>
  </rdf:Description>
  <rdf:Description rdf:nodeID="A61">
    <rdf:first rdf:resource="#MultiPropertyCleansingRule"/>
    <rdf:rest rdf:resource="http://www.w3.org/1999/02/22-rdf-syntax-ns#nil"/>
  </rdf:Description>
  <rdf:Description rdf:nodeID="A62">
    <rdf:type rdf:resource="http://www.w3.org/2002/07/owl#Class"/>
    <owl:unionOf rdf:nodeID="A22"/>
  </rdf:Description>
  <rdf:Description rdf:about="#Task">
    <rdfs:comment xml:lang="en">Classifies the tasks for which the data quality rule shall apply for.</rdfs:comment>
    <rdfs:label xml:lang="en">Task</rdfs:label>
    <rdf:type rdf:resource="http://www.w3.org/2002/07/owl#Class"/>
  </rdf:Description>
  <rdf:Description rdf:nodeID="A63">
    <rdf:first rdf:resource="#FuncDepValueRule"/>
    <rdf:rest rdf:resource="http://www.w3.org/1999/02/22-rdf-syntax-ns#nil"/>
  </rdf:Description>
  <rdf:Description rdf:about="#cleansesClass">
    <rdf:type rdf:resource="http://www.w3.org/2002/07/owl#FunctionalProperty"/>
    <rdf:type rdf:resource="http://www.w3.org/2002/07/owl#ObjectProperty"/>
    <rdfs:label xml:lang="en">Cleanses Class</rdfs:label>
    <rdfs:subPropertyOf rdf:resource="#dataCleansingRuleRelationship"/>
    <rdfs:range rdf:resource="#TestedClass"/>
    <rdfs:comment xml:lang="en">This property identifies classes that contain instances that shall be cleansed via a data cleansing rule.</rdfs:comment>
    <rdfs:domain rdf:resource="#DataCleansingRule"/>
  </rdf:Description>
  <rdf:Description rdf:nodeID="A64">
    <rdf:rest rdf:nodeID="A26"/>
    <rdf:first rdf:resource="#ConditionalRule"/>
  </rdf:Description>
  <rdf:Description rdf:about="#plainScore">
    <rdfs:comment xml:lang="en">The plain score represents a data quality dimension score that was assessed by using a certain formula that accounts for the violations of data quality rules related to the size of the relevant data set.</rdfs:comment>
    <rdfs:range rdf:resource="http://www.w3.org/2000/01/rdf-schema#Literal"/>
    <rdfs:domain rdf:resource="#DataQualityScore"/>
    <rdfs:label xml:lang="en">Plain Score</rdfs:label>
    <rdf:type rdf:resource="http://www.w3.org/2002/07/owl#FunctionalProperty"/>
    <rdf:type rdf:resource="http://www.w3.org/2002/07/owl#DatatypeProperty"/>
  </rdf:Description>
  <rdf:Description rdf:about="#hasCondition4">
    <rdfs:domain rdf:nodeID="A65"/>
    <rdf:type rdf:resource="http://www.w3.org/2002/07/owl#FunctionalProperty"/>
    <rdf:type rdf:resource="http://www.w3.org/2002/07/owl#ObjectProperty"/>
    <rdfs:subPropertyOf rdf:resource="#hasCondition"/>
    <rdfs:comment xml:lang="en">Connects a conditional rule with a certain condition.</rdfs:comment>
    <rdfs:label xml:lang="en">Has Condition 4</rdfs:label>
  </rdf:Description>
  <rdf:Description rdf:nodeID="A20">
    <owl:unionOf rdf:nodeID="A45"/>
    <rdf:type rdf:resource="http://www.w3.org/2002/07/owl#Class"/>
  </rdf:Description>
  <rdf:Description rdf:nodeID="A37">
    <rdf:type rdf:resource="http://www.w3.org/2002/07/owl#Class"/>
    <owl:unionOf rdf:nodeID="A66"/>
  </rdf:Description>
  <rdf:Description rdf:nodeID="A67">
    <rdf:rest rdf:nodeID="A68"/>
    <rdf:first rdf:resource="#Condition"/>
  </rdf:Description>
  <rdf:Description rdf:about="#hasCondition">
    <rdfs:comment xml:lang="en">Connects a conditional rule with a certain condition</rdfs:comment>
    <rdfs:range rdf:resource="#Condition"/>
    <rdf:type rdf:resource="http://www.w3.org/2002/07/owl#ObjectProperty"/>
    <rdfs:label xml:lang="en">Condition</rdfs:label>
    <rdfs:subPropertyOf rdf:resource="#dataElementRelationship"/>
  </rdf:Description>
  <rdf:Description rdf:nodeID="A56">
    <owl:unionOf rdf:nodeID="A69"/>
    <rdf:type rdf:resource="http://www.w3.org/2002/07/owl#Class"/>
  </rdf:Description>
  <rdf:Description rdf:about="#DataElement">
    <rdf:type rdf:resource="http://www.w3.org/2002/07/owl#Class"/>
    <rdfs:label xml:lang="en">Data Element</rdfs:label>
    <rdfs:comment xml:lang="en">A data element is a class, a property, an instance, or a literal value.</rdfs:comment>
  </rdf:Description>
  <rdf:Description rdf:nodeID="A70">
    <rdf:first rdf:resource="#PropertyCompletenessRule"/>
    <rdf:rest rdf:resource="http://www.w3.org/1999/02/22-rdf-syntax-ns#nil"/>
  </rdf:Description>
  <rdf:Description rdf:nodeID="A50">
    <owl:unionOf rdf:nodeID="A71"/>
    <rdf:type rdf:resource="http://www.w3.org/2002/07/owl#Class"/>
  </rdf:Description>
  <rdf:Description rdf:about="#WhitespaceRemoval">
    <rdfs:comment xml:lang="en">A white space removal rule states that whitespaces at the beginning of a string and at the end of a string shall be removed for the specified property.</rdfs:comment>
    <rdf:type rdf:resource="http://www.w3.org/2002/07/owl#Class"/>
    <rdfs:label xml:lang="en">White Space Removal Rule</rdfs:label>
    <rdfs:subClassOf rdf:resource="#LiteralCleansingRule"/>
  </rdf:Description>
  <rdf:Description rdf:about="#Condition">
    <rdf:type rdf:resource="http://www.w3.org/2002/07/owl#Class"/>
    <rdfs:label xml:lang="en">Condition</rdfs:label>
    <rdfs:comment xml:lang="en">A condition constrains instances of a class to a certain subset for which certain data quality rules apply.</rdfs:comment>
  </rdf:Description>
  <rdf:Description rdf:about="#MissingProperty">
    <rdfs:label xml:lang="en">Missing Property</rdfs:label>
    <rdfs:subClassOf rdf:resource="#MissingElement"/>
    <rdfs:comment xml:lang="en">A property is missing when an instances does not contain a specific property that is required.</rdfs:comment>
    <rdf:type rdf:resource="http://www.w3.org/2002/07/owl#Class"/>
  </rdf:Description>
  <rdf:Description rdf:about="#referenceProperty3">
    <rdfs:comment xml:lang="en">The reference property points to the URI of a property that holds trusted values, i.e. values of high quality</rdfs:comment>
    <rdf:type rdf:resource="http://www.w3.org/2002/07/owl#FunctionalProperty"/>
    <rdf:type rdf:resource="http://www.w3.org/2002/07/owl#ObjectProperty"/>
    <rdfs:domain rdf:resource="#FuncDepReferenceRule"/>
    <rdfs:subPropertyOf rdf:resource="#referenceProperty"/>
    <rdfs:label xml:lang="en">Reference Property 3</rdfs:label>
  </rdf:Description>
  <rdf:Description rdf:about="">
    <rdfs:label xml:lang="en">The Data Quality Management Vocabulary - An Ontology for Data Requirements Management, Data Quality Monitoring, Data Quality Assessment, and Data Cleansing</rdfs:label>
    <owl:versionInfo rdf:datatype="http://www.w3.org/2001/XMLSchema#string">V 1.00, Release 09-10-2011</owl:versionInfo>
    <dc:creator rdf:datatype="http://www.w3.org/2001/XMLSchema#string">Christian Fürber and Martin Hepp</dc:creator>
    <dc:subject rdf:datatype="http://www.w3.org/2001/XMLSchema#string">Data Quality Management, Data Quality Assessment, Data Quality Monitoring, Data Profiling, Data Cleansing, Data Requirements Management</dc:subject>
    <dc:rights rdf:datatype="http://www.w3.org/2001/XMLSchema#string">The Data Quality Management Vocabulary is available under the Creative Commons Attribution - Non Commercial - Share Alike 3.0 Unported license; see http://creativecommons.org/licenses/by-nc-sa/3.0/. In a nutshell, you are free to copy, distribute and transmit the work and to remix/adapt the work (e.g. to import the ontology and create specializations of its elements) for non commercial purposes, as long as you attribute the work in the manner specified by the author or licensor (but not in any way that suggests that they endorse you or your use of the work). Proper Attribution: Simply include the statement "This work is based on the Data Quality Management Vocabulary, developed by Christian Fürber and Martin Hepp" and link back to http://purl.org/dqm-vocabulary .</dc:rights>
    <rdfs:comment xml:lang="en">The Data Quality Management Vocabulary provides an ontology for the structured representation of data requirements, data quality assessment results, data cleansing rules, and data requirement violations connected to their origin. It, therefore, supports data quality monitoring, data quality assessment, and data cleansing in Semantic Web architectures.</rdfs:comment>
    <dc:title rdf:datatype="http://www.w3.org/2001/XMLSchema#string">The Data Quality Management Vocabulary</dc:title>
    <dcterms:license rdf:datatype="http://www.w3.org/2001/XMLSchema#string">http://creativecommons.org/licenses/by-nc-sa/3.0/</dcterms:license>
    <rdf:type rdf:resource="http://www.w3.org/2002/07/owl#Ontology"/>
  </rdf:Description>
  <rdf:Description rdf:nodeID="A8">
    <rdf:first rdf:resource="#LegalValueRule"/>
    <rdf:rest rdf:resource="http://www.w3.org/1999/02/22-rdf-syntax-ns#nil"/>
  </rdf:Description>
  <rdf:Description rdf:about="#CustomRequirement">
    <rdf:type rdf:resource="http://www.w3.org/2002/07/owl#Class"/>
    <rdfs:comment xml:lang="en">A custom requirement is a data requirement that is expressed via a SPARQL query.</rdfs:comment>
    <rdfs:subClassOf rdf:resource="#DataRequirement"/>
    <rdfs:label xml:lang="en">Custom Requirement</rdfs:label>
  </rdf:Description>
  <rdf:Description rdf:about="#hasScore">
    <rdfs:label xml:lang="en">Has Score</rdfs:label>
    <rdf:type rdf:resource="http://www.w3.org/2002/07/owl#ObjectProperty"/>
    <rdfs:domain rdf:resource="#DataRequirement"/>
    <rdfs:subPropertyOf rdf:resource="#dataRequirementsRelationship"/>
    <rdfs:comment xml:lang="en">Connects data requirements with the data quality score which was calculated based on the requirement.</rdfs:comment>
    <rdfs:range rdf:resource="#DataQualityScore"/>
  </rdf:Description>
  <rdf:Description rdf:about="#UpdateRule">
    <rdfs:label xml:lang="en">Update Rule</rdfs:label>
    <rdfs:subClassOf rdf:resource="#OutdatedInstanceRule"/>
    <rdfs:comment xml:lang="en">An update rule is an outdated instance rule that specifies the maximum duration tolerated without any updates. Update rules require timestamps about the last update of an instance.</rdfs:comment>
    <rdf:type rdf:resource="http://www.w3.org/2002/07/owl#Class"/>
  </rdf:Description>
  <rdf:Description rdf:about="#pattern">
    <rdfs:domain rdf:nodeID="A30"/>
    <rdfs:range rdf:resource="http://www.w3.org/2001/XMLSchema#string"/>
    <rdfs:comment xml:lang="en">The pattern property can be used to express value patterns based on a simple syntax without the need for knowing regular expressions. E.g. the pattern "AaaaaNN" where "A" stands for capital letters, "a" for small letters, and "N" for numbers.</rdfs:comment>
    <rdfs:label xml:lang="en">Pattern</rdfs:label>
    <rdf:type rdf:resource="http://www.w3.org/2002/07/owl#FunctionalProperty"/>
    <rdf:type rdf:resource="http://www.w3.org/2002/07/owl#DatatypeProperty"/>
  </rdf:Description>
  <rdf:Description rdf:about="#appliesFor">
    <owl:inverseOf rdf:resource="#hasRequirement"/>
    <rdf:type rdf:resource="http://www.w3.org/2002/07/owl#ObjectProperty"/>
    <rdfs:subPropertyOf rdf:resource="#dataRequirementsRelationship"/>
    <rdfs:label xml:lang="en">Applies For</rdfs:label>
    <rdfs:domain rdf:resource="#DataRequirement"/>
    <rdfs:comment xml:lang="en">Connects data requirements with the tasks in which the requirement applies.</rdfs:comment>
    <rdfs:range rdf:resource="#Task"/>
  </rdf:Description>
  <rdf:Description rdf:about="#hasCondition5">
    <rdfs:subPropertyOf rdf:resource="#hasCondition"/>
    <rdfs:domain rdf:nodeID="A72"/>
    <rdfs:comment xml:lang="en">Connects a conditional rule with a certain condition.</rdfs:comment>
    <rdf:type rdf:resource="http://www.w3.org/2002/07/owl#FunctionalProperty"/>
    <rdf:type rdf:resource="http://www.w3.org/2002/07/owl#ObjectProperty"/>
    <rdfs:label xml:lang="en">Has Condition 5</rdfs:label>
  </rdf:Description>
  <rdf:Description rdf:about="#StrictValueCombination">
    <rdfs:label xml:lang="en">Strict Value Combination Rule</rdfs:label>
    <rdfs:subClassOf rdf:resource="#MultiPropertyCleansingRule"/>
    <rdfs:comment xml:lang="en">A strict value combination is a combination of two values of different properties that may only be assigned to each other, but not to other values.</rdfs:comment>
    <rdf:type rdf:resource="http://www.w3.org/2002/07/owl#Class"/>
  </rdf:Description>
  <rdf:Description rdf:nodeID="A27">
    <owl:unionOf rdf:nodeID="A73"/>
    <rdf:type rdf:resource="http://www.w3.org/2002/07/owl#Class"/>
  </rdf:Description>
  <rdf:Description rdf:about="#ConditionalPropertyCompletenessRule">
    <rdf:type rdf:resource="http://www.w3.org/2002/07/owl#Class"/>
    <rdfs:subClassOf rdf:resource="#ConditionalRule"/>
    <rdfs:label xml:lang="en">Conditional Data Competeness Rule</rdfs:label>
    <rdfs:comment xml:lang="en">Conditional property completeness rules specify that a tested property and/or its literal values must exist when the value of another property obtains a certain state. E.g. the property foo:state must exist and have a value when the property foo:country obtains the value "USA".</rdfs:comment>
  </rdf:Description>
  <rdf:Description rdf:about="#TrustedClass">
    <rdf:type rdf:resource="http://www.w3.org/2002/07/owl#Class"/>
    <rdfs:subClassOf rdf:resource="#DataElement"/>
    <rdfs:label xml:lang="en">Trusted Class</rdfs:label>
    <rdfs:comment xml:lang="en">Legal value rules and functional dependency reference rules require the specification of a trusted class as a reference that holds instances with legal values / legal value combinations.</rdfs:comment>
  </rdf:Description>
  <rdf:Description rdf:nodeID="A73">
    <rdf:rest rdf:nodeID="A70"/>
    <rdf:first rdf:resource="#ConditionalPropertyCompletenessRule"/>
  </rdf:Description>
  <rdf:Description rdf:nodeID="A53">
    <rdf:first rdf:resource="#BlacklistClass"/>
    <rdf:rest rdf:nodeID="A74"/>
  </rdf:Description>
  <rdf:Description rdf:about="#Unit">
    <rdfs:label xml:lang="en">Unit</rdfs:label>
    <rdf:type rdf:resource="http://www.w3.org/2002/07/owl#Class"/>
    <rdfs:comment xml:lang="en">Class for units of numerical values that are used to express certain property states.</rdfs:comment>
  </rdf:Description>
  <rdf:Description rdf:about="#DataCleansingRule">
    <rdfs:label xml:lang="en">Data Cleansing Rule</rdfs:label>
    <rdf:type rdf:resource="http://www.w3.org/2002/07/owl#Class"/>
    <rdfs:comment xml:lang="en">A data cleansing rule is an unambiguous rule that precisely specifies the required state of a data value.</rdfs:comment>
  </rdf:Description>
  <rdf:Description rdf:about="#referenceProperty4">
    <rdf:type rdf:resource="http://www.w3.org/2002/07/owl#FunctionalProperty"/>
    <rdf:type rdf:resource="http://www.w3.org/2002/07/owl#ObjectProperty"/>
    <rdfs:label xml:lang="en">Reference Property 4</rdfs:label>
    <rdfs:domain rdf:resource="#FuncDepReferenceRule"/>
    <rdfs:subPropertyOf rdf:resource="#referenceProperty"/>
    <rdfs:comment xml:lang="en">The reference property points to the URI of a property that holds trusted values, i.e. values of high quality</rdfs:comment>
  </rdf:Description>
  <rdf:Description rdf:nodeID="A9">
    <rdf:rest rdf:nodeID="A75"/>
    <rdf:first rdf:resource="#ConditionalPropertyCompletenessRule"/>
  </rdf:Description>
  <rdf:Description rdf:about="#sparqlrule">
    <rdf:type rdf:resource="http://www.w3.org/2002/07/owl#FunctionalProperty"/>
    <rdf:type rdf:resource="http://www.w3.org/2002/07/owl#DatatypeProperty"/>
    <rdfs:comment xml:lang="en">This property can store custom data requirements that are expressed via SPARQL queries.</rdfs:comment>
    <rdfs:range rdf:resource="http://www.w3.org/2001/XMLSchema#string"/>
    <rdfs:domain rdf:resource="#CustomRequirement"/>
    <rdfs:label xml:lang="en">SPARQL rule</rdfs:label>
  </rdf:Description>
  <rdf:Description rdf:nodeID="A74">
    <rdf:rest rdf:nodeID="A57"/>
    <rdf:first rdf:resource="#TestedClass"/>
  </rdf:Description>
  <rdf:Description rdf:nodeID="A76">
    <rdf:type rdf:resource="http://www.w3.org/2002/07/owl#DataRange"/>
    <owl:oneOf rdf:nodeID="A77"/>
  </rdf:Description>
  <rdf:Description rdf:nodeID="A44">
    <rdf:rest rdf:resource="http://www.w3.org/1999/02/22-rdf-syntax-ns#nil"/>
    <rdf:first rdf:datatype="http://www.w3.org/2001/XMLSchema#string">ratio</rdf:first>
  </rdf:Description>
  <rdf:Description rdf:nodeID="A78">
    <rdf:type rdf:resource="http://www.w3.org/2002/07/owl#Class"/>
    <owl:unionOf rdf:nodeID="A79"/>
  </rdf:Description>
  <rdf:Description rdf:nodeID="A79">
    <rdf:first rdf:resource="#DataElement"/>
    <rdf:rest rdf:nodeID="A32"/>
  </rdf:Description>
  <rdf:Description rdf:about="#confidence">
    <rdfs:subPropertyOf rdf:resource="#reqMetadata"/>
    <rdfs:domain rdf:resource="#DataRequirement"/>
    <rdfs:range rdf:resource="http://www.w3.org/2000/01/rdf-schema#Literal"/>
    <rdfs:label xml:lang="en">Confidence</rdfs:label>
    <rdfs:comment xml:lang="en">The confidence property indicates how confident a rule creators is regarding the correctness of the rule.</rdfs:comment>
    <rdf:type rdf:resource="http://www.w3.org/2002/07/owl#FunctionalProperty"/>
    <rdf:type rdf:resource="http://www.w3.org/2002/07/owl#DatatypeProperty"/>
  </rdf:Description>
  <rdf:Description rdf:about="#affectedProperty">
    <rdfs:label xml:lang="de">Affected Property</rdfs:label>
    <rdfs:subPropertyOf rdf:resource="#dataElementRelationship"/>
    <rdfs:domain rdf:resource="#DataRequirementViolation"/>
    <rdf:type rdf:resource="http://www.w3.org/2002/07/owl#ObjectProperty"/>
    <rdfs:comment xml:lang="de">An affected property specifies the property of a data instance that contains one or more data requirement violations. Some data requirement violations, such as functional dependency violations, have more than one affected property.</rdfs:comment>
    <rdfs:range rdf:resource="#AffectedProperty"/>
  </rdf:Description>
  <rdf:Description rdf:about="#addProperty">
    <rdfs:range rdf:resource="http://www.w3.org/2001/XMLSchema#anyURI"/>
    <rdf:type rdf:resource="http://www.w3.org/2002/07/owl#FunctionalProperty"/>
    <rdf:type rdf:resource="http://www.w3.org/2002/07/owl#DatatypeProperty"/>
    <rdfs:comment xml:lang="en">A property that shall be added to an instance.</rdfs:comment>
    <rdfs:label xml:lang="en">Add Property</rdfs:label>
    <rdfs:subPropertyOf rdf:resource="#cleansingProperty"/>
    <rdfs:domain rdf:resource="#PropertyCompletion"/>
  </rdf:Description>
  <rdf:Description rdf:nodeID="A71">
    <rdf:rest rdf:nodeID="A6"/>
    <rdf:first rdf:resource="#Condition"/>
  </rdf:Description>
  <rdf:Description rdf:nodeID="A80">
    <rdf:rest rdf:resource="http://www.w3.org/1999/02/22-rdf-syntax-ns#nil"/>
    <rdf:first rdf:resource="#FuncDepValueRule"/>
  </rdf:Description>
  <rdf:Description rdf:nodeID="A47">
    <owl:unionOf rdf:nodeID="A64"/>
    <rdf:type rdf:resource="http://www.w3.org/2002/07/owl#Class"/>
  </rdf:Description>
  <rdf:Description rdf:nodeID="A42">
    <rdf:first rdf:resource="#Condition"/>
    <rdf:rest rdf:nodeID="A63"/>
  </rdf:Description>
  <rdf:Description rdf:about="#ruleOfIdentification">
    <rdf:type rdf:resource="http://www.w3.org/2002/07/owl#ObjectProperty"/>
    <rdfs:label xml:lang="en">Rule Of Identification</rdfs:label>
    <rdfs:range rdf:resource="#DataRequirement"/>
    <rdfs:comment xml:lang="en">The rule of identification property connects the data quality problem instances with the instance of the data requirement that has detected the problem.</rdfs:comment>
    <rdfs:subPropertyOf rdf:resource="#dataRequirementsRelationship"/>
    <rdfs:domain rdf:resource="#DataRequirementViolation"/>
  </rdf:Description>
  <rdf:Description rdf:about="#referenceProperty5">
    <rdfs:subPropertyOf rdf:resource="#referenceProperty"/>
    <rdf:type rdf:resource="http://www.w3.org/2002/07/owl#FunctionalProperty"/>
    <rdf:type rdf:resource="http://www.w3.org/2002/07/owl#ObjectProperty"/>
    <rdfs:comment xml:lang="en">The reference property points to the URI of a property that holds trusted values, i.e. values of high quality</rdfs:comment>
    <rdfs:domain rdf:resource="#FuncDepReferenceRule"/>
    <rdfs:label xml:lang="en">Reference Property 5</rdfs:label>
  </rdf:Description>
  <rdf:Description rdf:about="#unitOfConfidence">
    <rdfs:label xml:lang="en">Unit of Confidence</rdfs:label>
    <rdf:type rdf:resource="http://www.w3.org/2002/07/owl#FunctionalProperty"/>
    <rdf:type rdf:resource="http://www.w3.org/2002/07/owl#ObjectProperty"/>
    <rdfs:domain rdf:resource="#DataRequirement"/>
    <rdfs:range rdf:resource="#Unit"/>
    <rdfs:comment xml:lang="en">The unit in which confidence is expressed.</rdfs:comment>
  </rdf:Description>
  <rdf:Description rdf:about="#endsWith">
    <rdf:type rdf:resource="http://www.w3.org/2002/07/owl#FunctionalProperty"/>
    <rdf:type rdf:resource="http://www.w3.org/2002/07/owl#DatatypeProperty"/>
    <rdfs:subPropertyOf rdf:resource="#operatedValue"/>
    <rdfs:comment xml:lang="en">Holds one or more consecutive characters that are supposed to be found at the end of strings of another property.</rdfs:comment>
    <rdfs:label xml:lang="en">Ends With</rdfs:label>
    <rdfs:domain rdf:nodeID="A81"/>
    <rdfs:range rdf:resource="http://www.w3.org/2001/XMLSchema#string"/>
  </rdf:Description>
  <rdf:Description rdf:about="#assessedClass">
    <rdfs:subPropertyOf rdf:resource="#dataElementRelationship"/>
    <rdfs:label xml:lang="en">Assessed Class</rdfs:label>
    <rdfs:comment xml:lang="en">The assessed class is the class that holds the instances that have been analyzed to compute the assessment score.</rdfs:comment>
    <rdf:type rdf:resource="http://www.w3.org/2002/07/owl#ObjectProperty"/>
    <rdfs:range rdf:resource="#TestedClass"/>
    <rdfs:domain rdf:resource="#DataQualityScore"/>
  </rdf:Description>
  <rdf:Description rdf:nodeID="A82">
    <rdf:first rdf:resource="#SyntaxRule"/>
    <rdf:rest rdf:resource="http://www.w3.org/1999/02/22-rdf-syntax-ns#nil"/>
  </rdf:Description>
  <rdf:Description rdf:about="#MissingPropertyAndValue">
    <rdfs:comment xml:lang="en">Class for instances that miss both a property and its value.</rdfs:comment>
    <rdfs:label xml:lang="en">Missing Property and Value</rdfs:label>
    <rdfs:subClassOf rdf:resource="#MissingElement"/>
    <rdf:type rdf:resource="http://www.w3.org/2002/07/owl#Class"/>
  </rdf:Description>
  <rdf:Description rdf:about="#weightedScore">
    <rdfs:label xml:lang="en">Weighted Score</rdfs:label>
    <rdfs:range rdf:resource="http://www.w3.org/2000/01/rdf-schema#Literal"/>
    <rdfs:comment xml:lang="en">A weighted score is a data quality dimension score that is computed by integration of importance values of data requirements, tasks, or data elements.</rdfs:comment>
    <rdf:type rdf:resource="http://www.w3.org/2002/07/owl#FunctionalProperty"/>
    <rdf:type rdf:resource="http://www.w3.org/2002/07/owl#DatatypeProperty"/>
    <rdfs:domain rdf:resource="#DataQualityScore"/>
  </rdf:Description>
  <rdf:Description rdf:nodeID="A24">
    <rdf:first rdf:resource="#DataRequirement"/>
    <rdf:rest rdf:resource="http://www.w3.org/1999/02/22-rdf-syntax-ns#nil"/>
  </rdf:Description>
  <rdf:Description rdf:about="#equals">
    <rdfs:domain rdf:nodeID="A83"/>
    <rdfs:label xml:lang="en">Equals</rdfs:label>
    <rdf:type rdf:resource="http://www.w3.org/2002/07/owl#FunctionalProperty"/>
    <rdf:type rdf:resource="http://www.w3.org/2002/07/owl#DatatypeProperty"/>
    <rdfs:range rdf:resource="http://www.w3.org/2001/XMLSchema#string"/>
    <rdfs:subPropertyOf rdf:resource="#operatedValue"/>
    <rdfs:comment xml:lang="en">Holds one or more consecutive characters that are supposed to be found in the same order in strings of another property.</rdfs:comment>
  </rdf:Description>
  <rdf:Description rdf:about="#Uniqueness">
    <rdfs:label xml:lang="en">Uniqueness</rdfs:label>
    <rdfs:subClassOf rdf:resource="#DataQualityScore"/>
    <rdfs:comment xml:lang="en">Uniqueness is the degree to which properties and classes are free of duplicate values and instances.</rdfs:comment>
    <rdf:type rdf:resource="http://www.w3.org/2002/07/owl#Class"/>
  </rdf:Description>
  <rdf:Description rdf:about="#valueMeaning">
    <rdfs:range rdf:resource="http://www.w3.org/2001/XMLSchema#string"/>
    <rdfs:label xml:lang="en">Value Meaning</rdfs:label>
    <rdf:type rdf:resource="http://www.w3.org/2002/07/owl#DatatypeProperty"/>
    <rdfs:domain rdf:resource="#ScaleValue"/>
    <rdfs:comment xml:lang="en">Meaning of a value.</rdfs:comment>
  </rdf:Description>
  <rdf:Description rdf:about="#Timeliness">
    <rdfs:label xml:lang="en">Timeliness</rdfs:label>
    <rdf:type rdf:resource="http://www.w3.org/2002/07/owl#Class"/>
    <rdfs:subClassOf rdf:resource="#DataQualityScore"/>
    <rdfs:comment xml:lang="en">Timeliness is the degree to which instances of a specific class (1) are updated within an expected time or (2) have not exceeded their expiration date.</rdfs:comment>
  </rdf:Description>
  <rdf:Description rdf:about="#conditionalProperty">
    <rdfs:range rdf:resource="#TestedProperty"/>
    <rdfs:subPropertyOf rdf:resource="#dataElementRelationship"/>
    <rdf:type rdf:resource="http://www.w3.org/2002/07/owl#FunctionalProperty"/>
    <rdf:type rdf:resource="http://www.w3.org/2002/07/owl#ObjectProperty"/>
    <rdfs:label xml:lang="en">Conditional Property</rdfs:label>
    <rdfs:domain rdf:resource="#Condition"/>
    <rdfs:comment xml:lang="en">The conditional property property indicates the URI of a property that holds values that can be used to filter the relevant subset of data for which a rule applies.</rdfs:comment>
  </rdf:Description>
  <rdf:Description rdf:about="#lowerLimit">
    <rdfs:comment xml:lang="en">Specifies the lower limit a numeric property value shall obtain.</rdfs:comment>
    <rdfs:range rdf:resource="http://www.w3.org/2001/XMLSchema#float"/>
    <rdfs:domain rdf:nodeID="A36"/>
    <rdf:type rdf:resource="http://www.w3.org/2002/07/owl#FunctionalProperty"/>
    <rdf:type rdf:resource="http://www.w3.org/2002/07/owl#DatatypeProperty"/>
    <rdfs:label xml:lang="en">Lower Limit</rdfs:label>
  </rdf:Description>
  <rdf:Description rdf:nodeID="A84">
    <rdf:rest rdf:nodeID="A61"/>
    <rdf:first rdf:resource="#ConditionalRule"/>
  </rdf:Description>
  <rdf:Description rdf:nodeID="A85">
    <rdf:first rdf:resource="#SyntaxRule"/>
    <rdf:rest rdf:resource="http://www.w3.org/1999/02/22-rdf-syntax-ns#nil"/>
  </rdf:Description>
  <rdf:Description rdf:about="#LegalValueRule">
    <rdfs:comment xml:lang="en">A legal value rule is a property requirement that specifies all values that a certain property is allowed to obtain. Legal value rules, therefore, refer to reference properties of classes that hold instances with all allowed values.</rdfs:comment>
    <rdf:type rdf:resource="http://www.w3.org/2002/07/owl#Class"/>
    <rdfs:subClassOf rdf:resource="#PropertyRequirement"/>
    <rdfs:label xml:lang="en">Legal Value Rule</rdfs:label>
  </rdf:Description>
  <rdf:Description rdf:nodeID="A86">
    <rdf:first rdf:datatype="http://www.w3.org/2001/XMLSchema#string">nominal</rdf:first>
    <rdf:rest rdf:nodeID="A43"/>
  </rdf:Description>
  <rdf:Description rdf:nodeID="A87">
    <rdf:rest rdf:nodeID="A80"/>
    <rdf:first rdf:resource="#Condition"/>
  </rdf:Description>
  <rdf:Description rdf:nodeID="A65">
    <owl:unionOf rdf:nodeID="A38"/>
    <rdf:type rdf:resource="http://www.w3.org/2002/07/owl#Class"/>
  </rdf:Description>
  <rdf:Description rdf:nodeID="A75">
    <rdf:rest rdf:resource="http://www.w3.org/1999/02/22-rdf-syntax-ns#nil"/>
    <rdf:first rdf:resource="#PropertyCompletenessRule"/>
  </rdf:Description>
  <rdf:Description rdf:about="#LiteralCleansingRule">
    <rdfs:comment xml:lang="en">Literal cleansing rules can be used to cleanse the literal values of a certain property.</rdfs:comment>
    <rdf:type rdf:resource="http://www.w3.org/2002/07/owl#Class"/>
    <rdfs:subClassOf rdf:resource="#DataCleansingRule"/>
    <rdfs:label xml:lang="en">Literal Cleansing Rule</rdfs:label>
  </rdf:Description>
  <rdf:Description rdf:about="#ScaleValue">
    <rdf:type rdf:resource="http://www.w3.org/2002/07/owl#Class"/>
    <rdfs:comment xml:lang="en">A scale value is a value of a nominal or ordinal scale.</rdfs:comment>
    <rdfs:label xml:lang="en">Scale Value</rdfs:label>
  </rdf:Description>
  <rdf:Description rdf:about="#hasRequirement">
    <rdfs:comment xml:lang="en">Specifies the data requirements that have to be fulfilled to perform the task.</rdfs:comment>
    <rdfs:domain rdf:resource="#Task"/>
    <rdfs:subPropertyOf rdf:resource="#dataRequirementsRelationship"/>
    <rdf:type rdf:resource="http://www.w3.org/2002/07/owl#ObjectProperty"/>
    <rdfs:label xml:lang="en">Has Requirement</rdfs:label>
    <rdfs:range rdf:resource="#DataRequirement"/>
  </rdf:Description>
  <rdf:Description rdf:about="#testedProperty2">
    <rdfs:label xml:lang="en">Tested Property 2</rdfs:label>
    <rdfs:domain rdf:resource="#MatchingValueRule"/>
    <rdfs:comment xml:lang="en">The property with the values that shall be tested for data quality problems.</rdfs:comment>
    <rdfs:subPropertyOf rdf:resource="#testedProperty"/>
    <rdf:type rdf:resource="http://www.w3.org/2002/07/owl#FunctionalProperty"/>
    <rdf:type rdf:resource="http://www.w3.org/2002/07/owl#ObjectProperty"/>
  </rdf:Description>
  <rdf:Description rdf:nodeID="A88">
    <rdf:first rdf:resource="#DataCleansingRule"/>
    <rdf:rest rdf:nodeID="A89"/>
  </rdf:Description>
  <rdf:Description rdf:about="#PopulationUniqueness">
    <rdf:type rdf:resource="http://www.w3.org/2002/07/owl#Class"/>
    <rdfs:subClassOf rdf:resource="#Uniqueness"/>
    <rdfs:comment xml:lang="en">Entity uniqueness is the degree to which entities (that must be uniquely represented within a certain class) are unique.</rdfs:comment>
    <rdfs:label xml:lang="en">Population Uniqueness</rdfs:label>
  </rdf:Description>
  <rdf:Description rdf:nodeID="A90">
    <rdf:rest rdf:nodeID="A91"/>
    <rdf:first rdf:resource="#AffectedProperty"/>
  </rdf:Description>
  <rdf:Description rdf:about="#PropertyCompletion">
    <rdfs:subClassOf rdf:resource="#MultiPropertyCleansingRule"/>
    <rdf:type rdf:resource="http://www.w3.org/2002/07/owl#Class"/>
    <rdfs:label xml:lang="en">Property Completion Rule</rdfs:label>
    <rdfs:comment xml:lang="en">A property completion rule specifies a property and value that shall be added to certain instances.</rdfs:comment>
  </rdf:Description>
  <rdf:Description rdf:about="#DataRequirementViolation">
    <rdfs:label xml:lang="en">Data Requirement Violation</rdfs:label>
    <rdfs:comment xml:lang="en">A data requirement violation occurs when a data value or a data instance does not meet its requirements.</rdfs:comment>
    <rdf:type rdf:resource="http://www.w3.org/2002/07/owl#Class"/>
  </rdf:Description>
  <rdf:Description rdf:nodeID="A91">
    <rdf:first rdf:resource="#BlacklistProperty"/>
    <rdf:rest rdf:nodeID="A12"/>
  </rdf:Description>
  <rdf:Description rdf:about="#DataRequirement">
    <rdf:type rdf:resource="http://www.w3.org/2002/07/owl#Class"/>
    <rdfs:comment xml:lang="en">A data requirement is a prescribed directive or consensual agreement that defines the content and/or structure that constitute high quality data instances and values.</rdfs:comment>
    <rdfs:label xml:lang="en">Data Requirement</rdfs:label>
  </rdf:Description>
  <rdf:Description rdf:nodeID="A49">
    <rdf:first rdf:resource="#ConditionalSyntaxRule"/>
    <rdf:rest rdf:nodeID="A82"/>
  </rdf:Description>
  <rdf:Description rdf:nodeID="A4">
    <rdf:rest rdf:nodeID="A92"/>
    <rdf:first rdf:resource="#ConditionalRule"/>
  </rdf:Description>
  <rdf:Description rdf:about="#reqSource">
    <rdfs:comment xml:lang="en">Specifies the source of a data requirement.</rdfs:comment>
    <rdfs:domain rdf:nodeID="A21"/>
    <rdf:type rdf:resource="http://www.w3.org/2002/07/owl#DatatypeProperty"/>
    <rdfs:range rdf:resource="http://www.w3.org/2001/XMLSchema#string"/>
    <rdfs:subPropertyOf rdf:resource="#reqMetadata"/>
    <rdfs:label xml:lang="en">Requirement Source</rdfs:label>
  </rdf:Description>
  <rdf:Description rdf:about="#validation">
    <rdfs:range rdf:resource="http://www.w3.org/2001/XMLSchema#boolean"/>
    <rdfs:domain rdf:resource="#DataRequirement"/>
    <rdf:type rdf:resource="http://www.w3.org/2002/07/owl#FunctionalProperty"/>
    <rdf:type rdf:resource="http://www.w3.org/2002/07/owl#DatatypeProperty"/>
    <rdfs:label xml:lang="en">Validation</rdfs:label>
    <rdfs:comment xml:lang="en">Validation indicates whether a data quality rule shall be used for validation during data entry.</rdfs:comment>
  </rdf:Description>
  <rdf:Description rdf:nodeID="A59">
    <rdf:first rdf:resource="#IllegalValueRangeRule"/>
    <rdf:rest rdf:nodeID="A51"/>
  </rdf:Description>
  <rdf:Description rdf:about="#DataQualityScore">
    <rdfs:comment xml:lang="en">Data quality score is an abstract class that can be used to structure data quality dimension scores that indicate the quality state of classes and/or properties.</rdfs:comment>
    <rdf:type rdf:resource="http://www.w3.org/2002/07/owl#Class"/>
    <rdfs:label xml:lang="en">Data Quality Assessment</rdfs:label>
  </rdf:Description>
  <rdf:Description rdf:nodeID="A52">
    <rdf:rest rdf:resource="http://www.w3.org/1999/02/22-rdf-syntax-ns#nil"/>
    <rdf:first rdf:resource="#Unit"/>
  </rdf:Description>
  <rdf:Description rdf:about="#UniquenessViolation">
    <rdfs:subClassOf rdf:resource="#DataRequirementViolation"/>
    <rdfs:label xml:lang="en">Uniqueness Violation</rdfs:label>
    <rdf:type rdf:resource="http://www.w3.org/2002/07/owl#Class"/>
    <rdfs:comment xml:lang="en">A uniqueness violation occurs when two or more identical values are assigned to a property that requires unique values.</rdfs:comment>
  </rdf:Description>
  <rdf:Description rdf:about="#LegalValueRangeRule">
    <rdf:type rdf:resource="http://www.w3.org/2002/07/owl#Class"/>
    <rdfs:label xml:lang="en">Legal Value Range Rule</rdfs:label>
    <rdfs:comment xml:lang="en">A legal value range rule is a property requirement that specifies the upper and/or lower boundary of numeric values that a certain property is allowed to obtain.</rdfs:comment>
    <rdfs:subClassOf rdf:resource="#PropertyRequirement"/>
  </rdf:Description>
  <rdf:Description rdf:about="#unitDescription">
    <rdfs:domain rdf:resource="#Unit"/>
    <rdf:type rdf:resource="http://www.w3.org/2002/07/owl#DatatypeProperty"/>
    <rdfs:range rdf:resource="http://www.w3.org/2001/XMLSchema#string"/>
    <rdfs:label xml:lang="en">Unit Description</rdfs:label>
    <rdfs:comment xml:lang="en">Description of a unit of measurement.</rdfs:comment>
  </rdf:Description>
  <rdf:Description rdf:about="#OutdatedInstance">
    <rdfs:subClassOf rdf:resource="#DataRequirementViolation"/>
    <rdfs:comment xml:lang="en">An instance is outdated when it represents an outdated state of its corresponding real-world entity.</rdfs:comment>
    <rdf:type rdf:resource="http://www.w3.org/2002/07/owl#Class"/>
    <rdfs:label xml:lang="en">Outdated Instance</rdfs:label>
  </rdf:Description>
  <rdf:Description rdf:about="#PopulationCompleteness">
    <rdfs:comment xml:lang="en">Population completeness is the degree to which all objects of a certain reference are represented in a specific class.</rdfs:comment>
    <rdf:type rdf:resource="http://www.w3.org/2002/07/owl#Class"/>
    <rdfs:label xml:lang="en">Population Completeness</rdfs:label>
    <rdfs:subClassOf rdf:resource="#Completeness"/>
  </rdf:Description>
  <rdf:Description rdf:nodeID="A31">
    <rdf:rest rdf:nodeID="A85"/>
    <rdf:first rdf:resource="#ConditionalSyntaxRule"/>
  </rdf:Description>
  <rdf:Description rdf:nodeID="A66">
    <rdf:first rdf:resource="#Condition"/>
    <rdf:rest rdf:nodeID="A35"/>
  </rdf:Description>
  <rdf:Description rdf:nodeID="A29">
    <rdf:first rdf:resource="#LegalValueRangeRule"/>
    <rdf:rest rdf:nodeID="A93"/>
  </rdf:Description>
  <rdf:Description rdf:nodeID="A58">
    <owl:unionOf rdf:nodeID="A90"/>
    <rdf:type rdf:resource="http://www.w3.org/2002/07/owl#Class"/>
  </rdf:Description>
  <rdf:Description rdf:nodeID="A54">
    <rdf:type rdf:resource="http://www.w3.org/2002/07/owl#Class"/>
    <owl:unionOf rdf:nodeID="A7"/>
  </rdf:Description>
  <rdf:Description rdf:nodeID="A69">
    <rdf:first rdf:resource="#ConditionalRule"/>
    <rdf:rest rdf:nodeID="A55"/>
  </rdf:Description>
  <rdf:Description rdf:nodeID="A17">
    <rdf:type rdf:resource="http://www.w3.org/2002/07/owl#Class"/>
    <owl:unionOf rdf:nodeID="A88"/>
  </rdf:Description>
  <rdf:Description rdf:about="#OutdatedInstanceRule">
    <rdfs:subClassOf rdf:resource="#ClassRequirement"/>
    <rdf:type rdf:resource="http://www.w3.org/2002/07/owl#Class"/>
    <rdfs:comment xml:lang="en">An outdated instance rule is a data requirement that specifies the point in time when an instance is not current anymore.</rdfs:comment>
    <rdfs:label xml:lang="en">Outdated Instance Rule</rdfs:label>
  </rdf:Description>
  <rdf:Description rdf:about="#testedProperty1">
    <rdfs:label xml:lang="en">Tested Property 1</rdfs:label>
    <rdf:type rdf:resource="http://www.w3.org/2002/07/owl#FunctionalProperty"/>
    <rdf:type rdf:resource="http://www.w3.org/2002/07/owl#ObjectProperty"/>
    <rdfs:subPropertyOf rdf:resource="#testedProperty"/>
    <rdfs:comment xml:lang="en">The property with the values that shall be tested for data quality problems.</rdfs:comment>
    <rdfs:domain rdf:resource="#DataRequirement"/>
  </rdf:Description>
  <rdf:Description rdf:about="#scaleValues">
    <rdfs:comment xml:lang="en">Links to values of a certain ordinal or nominal scale.</rdfs:comment>
    <rdfs:domain rdf:resource="#Unit"/>
    <rdfs:range rdf:resource="#ScaleValue"/>
    <rdf:type rdf:resource="http://www.w3.org/2002/07/owl#ObjectProperty"/>
    <rdfs:label xml:lang="en">Scale Values</rdfs:label>
  </rdf:Description>
  <rdf:Description rdf:about="#assessment">
    <rdfs:comment xml:lang="en">The assessment property indicates whether the rule shall be used for data quality assessment.</rdfs:comment>
    <rdf:type rdf:resource="http://www.w3.org/2002/07/owl#FunctionalProperty"/>
    <rdf:type rdf:resource="http://www.w3.org/2002/07/owl#DatatypeProperty"/>
    <rdfs:subPropertyOf rdf:resource="#reqMetadata"/>
    <rdfs:domain rdf:resource="#DataRequirement"/>
    <rdfs:label xml:lang="en">Assessment</rdfs:label>
    <rdfs:range rdf:resource="http://www.w3.org/2001/XMLSchema#boolean"/>
  </rdf:Description>
  <rdf:Description rdf:about="#taskDescription">
    <rdfs:range rdf:resource="http://www.w3.org/2001/XMLSchema#string"/>
    <rdfs:comment xml:lang="en">Describes the task in natural language.</rdfs:comment>
    <rdfs:domain rdf:resource="#Task"/>
    <rdf:type rdf:resource="http://www.w3.org/2002/07/owl#DatatypeProperty"/>
    <rdfs:label xml:lang="en">Task Description</rdfs:label>
  </rdf:Description>
  <rdf:Description rdf:about="#dataElementRelationship">
    <rdf:type rdf:resource="http://www.w3.org/2002/07/owl#ObjectProperty"/>
    <rdfs:comment xml:lang="en">The data element relationship property is an abstract property that holds object properties that are used to define internal and external relationships of data elements.</rdfs:comment>
    <rdfs:label xml:lang="en">Data Element Relationship</rdfs:label>
  </rdf:Description>
  <rdf:Description rdf:about="#PropertyCompleteness">
    <rdfs:subClassOf rdf:resource="#Completeness"/>
    <rdfs:comment xml:lang="en">Property completeness is the degree to which values for a specific property are missing in entities of a specific class.</rdfs:comment>
    <rdf:type rdf:resource="http://www.w3.org/2002/07/owl#Class"/>
    <rdfs:label xml:lang="en">Property Completeness</rdfs:label>
  </rdf:Description>
  <rdf:Description rdf:about="#filtering">
    <rdfs:label xml:lang="en">Filtering</rdfs:label>
    <rdfs:subPropertyOf rdf:resource="#reqMetadata"/>
    <rdfs:domain rdf:resource="#DataRequirement"/>
    <rdfs:comment xml:lang="en">The filtering property indicates whether the rule shall be used for information filtering, i.e. only high quality data is retrieved.</rdfs:comment>
    <rdf:type rdf:resource="http://www.w3.org/2002/07/owl#FunctionalProperty"/>
    <rdf:type rdf:resource="http://www.w3.org/2002/07/owl#DatatypeProperty"/>
    <rdfs:range rdf:resource="http://www.w3.org/2001/XMLSchema#boolean"/>
  </rdf:Description>
  <rdf:Description rdf:about="#startsWith">
    <rdfs:domain rdf:nodeID="A41"/>
    <rdf:type rdf:resource="http://www.w3.org/2002/07/owl#FunctionalProperty"/>
    <rdf:type rdf:resource="http://www.w3.org/2002/07/owl#DatatypeProperty"/>
    <rdfs:range rdf:resource="http://www.w3.org/2001/XMLSchema#string"/>
    <rdfs:comment xml:lang="en">Holds one or more consecutive characters that are supposed to be found at the beginning of strings of another property.</rdfs:comment>
    <rdfs:label xml:lang="en">Starts With</rdfs:label>
    <rdfs:subPropertyOf rdf:resource="#operatedValue"/>
  </rdf:Description>
  <rdf:Description rdf:nodeID="A92">
    <rdf:rest rdf:resource="http://www.w3.org/1999/02/22-rdf-syntax-ns#nil"/>
    <rdf:first rdf:resource="#MultiPropertyCleansingRule"/>
  </rdf:Description>
  <rdf:Description rdf:about="#DuplicateInstance">
    <rdf:type rdf:resource="http://www.w3.org/2002/07/owl#Class"/>
    <rdfs:label xml:lang="en">Duplicate Instance</rdfs:label>
    <rdfs:subClassOf rdf:resource="#DataRequirementViolation"/>
    <rdfs:comment xml:lang="en">Two or more instances are duplicates when they represent the same real world entity.</rdfs:comment>
  </rdf:Description>
  <rdf:Description rdf:nodeID="A14">
    <rdf:type rdf:resource="http://www.w3.org/2002/07/owl#Class"/>
    <owl:unionOf rdf:nodeID="A94"/>
  </rdf:Description>
  <rdf:Description rdf:about="#cleansing">
    <rdfs:label xml:lang="en">Cleansing</rdfs:label>
    <rdfs:domain rdf:resource="#DataRequirement"/>
    <rdfs:range rdf:resource="http://www.w3.org/2001/XMLSchema#boolean"/>
    <rdf:type rdf:resource="http://www.w3.org/2002/07/owl#FunctionalProperty"/>
    <rdf:type rdf:resource="http://www.w3.org/2002/07/owl#DatatypeProperty"/>
    <rdfs:subPropertyOf rdf:resource="#reqMetadata"/>
    <rdfs:comment xml:lang="en">The data cleansing property specifies whether the rule shall be applied to cleanse the data in a data source.</rdfs:comment>
  </rdf:Description>
  <rdf:Description rdf:nodeID="A94">
    <rdf:first rdf:resource="#FuncDepReferenceRule"/>
    <rdf:rest rdf:nodeID="A95"/>
  </rdf:Description>
  <rdf:Description rdf:about="#testedProperty4">
    <rdfs:comment xml:lang="en">The property with the values that shall be tested for data quality problems.</rdfs:comment>
    <rdfs:subPropertyOf rdf:resource="#testedProperty"/>
    <rdf:type rdf:resource="http://www.w3.org/2002/07/owl#FunctionalProperty"/>
    <rdf:type rdf:resource="http://www.w3.org/2002/07/owl#ObjectProperty"/>
    <rdfs:domain rdf:resource="#MatchingValueRule"/>
    <rdfs:label xml:lang="en">Tested Property 4</rdfs:label>
  </rdf:Description>
  <rdf:Description rdf:about="#FuncDepReferenceRule">
    <rdfs:label xml:lang="en">Functional Dependency Reference Rule</rdfs:label>
    <rdfs:subClassOf rdf:resource="#MatchingValueRule"/>
    <rdf:type rdf:resource="http://www.w3.org/2002/07/owl#Class"/>
    <rdfs:comment xml:lang="en">A functional dependency reference rule is a multi property requirement that specifies legal value combinations for two or more properties that are allowed to occur within the same instance. Functional dependency reference rules refer to reference properties of classes that hold instances with all allowed value combinations.</rdfs:comment>
  </rdf:Description>
  <rdf:Description rdf:about="http://purl.org/dc/elements/1.1/contributor">
    <rdf:type rdf:resource="http://www.w3.org/2002/07/owl#AnnotationProperty"/>
  </rdf:Description>
  <rdf:Description rdf:about="#reqMetadata">
    <rdf:type rdf:resource="http://www.w3.org/2002/07/owl#DatatypeProperty"/>
    <rdfs:label xml:lang="en">Requirement Metadata</rdfs:label>
    <rdfs:comment xml:lang="en">An abstract property that holds generic datatype properties that describe a data requirement.</rdfs:comment>
  </rdf:Description>
  <rdf:Description rdf:nodeID="A77">
    <rdf:first rdf:datatype="http://www.w3.org/2001/XMLSchema#string">interval</rdf:first>
    <rdf:rest rdf:nodeID="A86"/>
  </rdf:Description>
  <rdf:Description rdf:about="#addValue">
    <rdfs:comment xml:lang="en">A value that shall be added to a property of an instance.</rdfs:comment>
    <rdfs:label xml:lang="en">Add Value</rdfs:label>
    <rdfs:subPropertyOf rdf:resource="#cleansingProperty"/>
    <rdfs:domain rdf:resource="#PropertyCompletion"/>
    <rdf:type rdf:resource="http://www.w3.org/2002/07/owl#FunctionalProperty"/>
    <rdf:type rdf:resource="http://www.w3.org/2002/07/owl#DatatypeProperty"/>
    <rdfs:range rdf:resource="http://www.w3.org/2001/XMLSchema#string"/>
  </rdf:Description>
  <rdf:Description rdf:nodeID="A46">
    <rdf:rest rdf:resource="http://www.w3.org/1999/02/22-rdf-syntax-ns#nil"/>
    <rdf:first rdf:resource="#FuncDepValueRule"/>
  </rdf:Description>
  <rdf:Description rdf:nodeID="A83">
    <owl:unionOf rdf:nodeID="A87"/>
    <rdf:type rdf:resource="http://www.w3.org/2002/07/owl#Class"/>
  </rdf:Description>
  <rdf:Description rdf:about="#importance">
    <rdfs:subPropertyOf rdf:resource="#reqMetadata"/>
    <rdfs:label xml:lang="en">Importance</rdfs:label>
    <rdfs:domain rdf:nodeID="A78"/>
    <rdfs:comment xml:lang="en">Specifies the importance of a task, a data quality rule, or a data element.</rdfs:comment>
    <rdf:type rdf:resource="http://www.w3.org/2002/07/owl#FunctionalProperty"/>
    <rdf:type rdf:resource="http://www.w3.org/2002/07/owl#DatatypeProperty"/>
    <rdfs:range rdf:resource="http://www.w3.org/2000/01/rdf-schema#Literal"/>
  </rdf:Description>
  <rdf:Description rdf:about="#MultiPropertyCleansingRule">
    <rdfs:comment xml:lang="en">Multi property cleansing rules can be used to cleanse the literal values of two or more dependent properties.</rdfs:comment>
    <rdfs:label xml:lang="en">Multi Property Cleansing Rule</rdfs:label>
    <rdf:type rdf:resource="http://www.w3.org/2002/07/owl#Class"/>
    <rdfs:subClassOf rdf:resource="#DataCleansingRule"/>
  </rdf:Description>
  <rdf:Description rdf:about="#taskName">
    <rdfs:domain rdf:resource="#Task"/>
    <rdfs:comment xml:lang="en">Specifies the name of the task.</rdfs:comment>
    <rdf:type rdf:resource="http://www.w3.org/2002/07/owl#DatatypeProperty"/>
    <rdfs:label xml:lang="en">Task Name</rdfs:label>
    <rdfs:range rdf:resource="http://www.w3.org/2001/XMLSchema#string"/>
  </rdf:Description>
  <rdf:Description rdf:nodeID="A81">
    <rdf:type rdf:resource="http://www.w3.org/2002/07/owl#Class"/>
    <owl:unionOf rdf:nodeID="A67"/>
  </rdf:Description>
  <rdf:Description rdf:nodeID="A68">
    <rdf:rest rdf:resource="http://www.w3.org/1999/02/22-rdf-syntax-ns#nil"/>
    <rdf:first rdf:resource="#FuncDepValueRule"/>
  </rdf:Description>
  <rdf:Description rdf:nodeID="A72">
    <rdf:type rdf:resource="http://www.w3.org/2002/07/owl#Class"/>
    <owl:unionOf rdf:nodeID="A84"/>
  </rdf:Description>
  <rdf:Description rdf:about="#operatedValue">
    <rdf:type rdf:resource="http://www.w3.org/2002/07/owl#DatatypeProperty"/>
    <rdfs:comment xml:lang="en">The operated value property is an abstract property for datatype properties that are used to express string filtering criteria.</rdfs:comment>
    <rdfs:label xml:lang="en">Operated Value</rdfs:label>
  </rdf:Description>
  <rdf:Description rdf:about="#cleansesProperty1">
    <rdf:type rdf:resource="http://www.w3.org/2002/07/owl#FunctionalProperty"/>
    <rdf:type rdf:resource="http://www.w3.org/2002/07/owl#ObjectProperty"/>
    <rdfs:subPropertyOf rdf:resource="#dataCleansingRuleRelationship"/>
    <rdfs:label xml:lang="en">Cleanses Property 1</rdfs:label>
    <rdfs:domain rdf:resource="#DataCleansingRule"/>
    <rdfs:range rdf:resource="#TestedProperty"/>
    <rdfs:comment xml:lang="en">This property identifies a property that holds values that shall be cleansed.</rdfs:comment>
  </rdf:Description>
  <rdf:Description rdf:about="#testedProperty3">
    <rdfs:domain rdf:resource="#MatchingValueRule"/>
    <rdfs:label xml:lang="en">Tested Property 3</rdfs:label>
    <rdf:type rdf:resource="http://www.w3.org/2002/07/owl#FunctionalProperty"/>
    <rdf:type rdf:resource="http://www.w3.org/2002/07/owl#ObjectProperty"/>
    <rdfs:comment xml:lang="en">The property with the values that shall be tested for data quality problems.</rdfs:comment>
    <rdfs:subPropertyOf rdf:resource="#testedProperty"/>
  </rdf:Description>
  <rdf:Description rdf:nodeID="A89">
    <rdf:rest rdf:resource="http://www.w3.org/1999/02/22-rdf-syntax-ns#nil"/>
    <rdf:first rdf:resource="#DataRequirement"/>
  </rdf:Description>
  <rdf:Description rdf:about="#PropertyRequirement">
    <rdfs:comment xml:lang="en">Property requirements are data requirements that are related to values of a single property.</rdfs:comment>
    <rdf:type rdf:resource="http://www.w3.org/2002/07/owl#Class"/>
    <rdfs:label xml:lang="en">Property Requirement</rdfs:label>
    <rdfs:subClassOf rdf:resource="#DataRequirement"/>
  </rdf:Description>
  <rdf:Description rdf:about="#SyntaxRule">
    <rdf:type rdf:resource="http://www.w3.org/2002/07/owl#Class"/>
    <rdfs:comment xml:lang="en">A syntax rule is a property requirement that specifies the allowed characters and/or character pattern to be used in values for a certain property in instances of a certain class.</rdfs:comment>
    <rdfs:subClassOf rdf:resource="#PropertyRequirement"/>
    <rdfs:label xml:lang="en">Syntax Rule</rdfs:label>
  </rdf:Description>
  <rdf:Description rdf:nodeID="A96">
    <rdf:rest rdf:resource="http://www.w3.org/1999/02/22-rdf-syntax-ns#nil"/>
    <rdf:first rdf:resource="#DataRequirement"/>
  </rdf:Description>
  <rdf:Description rdf:nodeID="A23">
    <rdf:rest rdf:nodeID="A25"/>
    <rdf:first rdf:resource="#DataRequirement"/>
  </rdf:Description>
  <rdf:Description rdf:nodeID="A95">
    <rdf:rest rdf:resource="http://www.w3.org/1999/02/22-rdf-syntax-ns#nil"/>
    <rdf:first rdf:resource="#LegalValueRule"/>
  </rdf:Description>
  <rdf:Description rdf:nodeID="A60">
    <rdf:rest rdf:nodeID="A96"/>
    <rdf:first rdf:resource="#DataCleansingRule"/>
  </rdf:Description>
  <rdf:Description rdf:about="#unitOfImportance">
    <rdf:type rdf:resource="http://www.w3.org/2002/07/owl#FunctionalProperty"/>
    <rdf:type rdf:resource="http://www.w3.org/2002/07/owl#ObjectProperty"/>
    <rdfs:comment xml:lang="en">The unit in which importance is expressed.</rdfs:comment>
    <rdfs:domain rdf:nodeID="A62"/>
    <rdfs:range rdf:resource="#Unit"/>
    <rdfs:label xml:lang="en">Unit of Importance</rdfs:label>
  </rdf:Description>
  <rdf:Description rdf:about="#commonCode">
    <rdfs:comment xml:lang="en">UN/CEFACT common code of a unit of measurement.</rdfs:comment>
    <rdf:type rdf:resource="http://www.w3.org/2002/07/owl#FunctionalProperty"/>
    <rdf:type rdf:resource="http://www.w3.org/2002/07/owl#DatatypeProperty"/>
    <rdfs:label xml:lang="en">UN/CEFACT common code</rdfs:label>
    <rdfs:domain rdf:resource="#Unit"/>
    <rdfs:range rdf:resource="http://www.w3.org/2001/XMLSchema#string"/>
  </rdf:Description>
  <rdf:Description rdf:about="#scaleType">
    <rdf:type rdf:resource="http://www.w3.org/2002/07/owl#FunctionalProperty"/>
    <rdf:type rdf:resource="http://www.w3.org/2002/07/owl#DatatypeProperty"/>
    <rdfs:range rdf:nodeID="A76"/>
    <rdfs:domain rdf:resource="#Unit"/>
    <rdfs:label xml:lang="en">Scale Type</rdfs:label>
    <rdfs:comment xml:lang="en">Type of statistical scale.</rdfs:comment>
  </rdf:Description>
  <rdf:Description rdf:about="#regex">
    <rdfs:label xml:lang="en">Regular Expression</rdfs:label>
    <rdf:type rdf:resource="http://www.w3.org/2002/07/owl#FunctionalProperty"/>
    <rdf:type rdf:resource="http://www.w3.org/2002/07/owl#DatatypeProperty"/>
    <rdfs:comment xml:lang="en">The regular expressions property can be used to express legal character ranges and data patterns for values of a certain property via regular expressions.</rdfs:comment>
    <rdfs:domain rdf:nodeID="A48"/>
    <rdfs:range rdf:resource="http://www.w3.org/2001/XMLSchema#string"/>
  </rdf:Description>
  <rdf:Description rdf:about="#MissingElement">
    <rdfs:label xml:lang="en">Missing Element</rdfs:label>
    <rdfs:comment xml:lang="en">A missing element is a data requirement violation that occurs when schema elements, instances, or data values are missing, but required.</rdfs:comment>
    <rdfs:subClassOf rdf:resource="#DataRequirementViolation"/>
    <rdf:type rdf:resource="http://www.w3.org/2002/07/owl#Class"/>
  </rdf:Description>
  <rdf:Description rdf:nodeID="A93">
    <rdf:rest rdf:resource="http://www.w3.org/1999/02/22-rdf-syntax-ns#nil"/>
    <rdf:first rdf:resource="#Unit"/>
  </rdf:Description>
</rdf:RDF>

<!-- Created with Protege (with OWL Plugin 3.4.4, Build 579)  http://protege.stanford.edu -->
