<?xml version="1.0"?>

<rdf:RDF xmlns="http://zbw.eu/namespaces/zbw-extensions/"
     xml:base="http://zbw.eu/namespaces/zbw-extensions/"
     xmlns:rdfs="http://www.w3.org/2000/01/rdf-schema#"
     xmlns:owl2xml="http://www.w3.org/2006/12/owl2-xml#"
     xmlns:owl="http://www.w3.org/2002/07/owl#"
     xmlns:xsd="http://www.w3.org/2001/XMLSchema#"
     xmlns:rdf="http://www.w3.org/1999/02/22-rdf-syntax-ns#"
     xmlns:dc="http://purl.org/dc/elements/1.1/"
     xmlns:dcterms="http://purl.org/dc/terms/"
     xmlns:skos="http://www.w3.org/2004/02/skos/core#">

  <rdf:Description rdf:about="">
    <dc:title xml:lang="en">Extensions to SKOS and other standard vocabularies used by the German National Library of Economics (ZBW)</dc:title>
    <dc:creator>Joachim Neubert</dc:creator>
    <dc:publisher xml:lang="en">German National Library of Economics (ZBW)</dc:publisher>
    <dcterms:created>2010-04-28</dcterms:created>
    <dcterms:modified>2017-04-12</dcterms:modified>
  </rdf:Description>

  <rdf:Description rdf:about="Descriptor">
    <rdf:type rdf:resource="http://www.w3.org/2002/07/owl#Class"/>
    <rdfs:label xml:lang="en">Descriptor</rdfs:label>
    <rdfs:isDefinedBy rdf:resource="http://zbw.eu/namespaces/zbw-extensions/zbw-extensions.rdf"/>
    <rdfs:subClassOf rdf:resource="http://www.w3.org/2004/02/skos/core#Concept"/>
    <skos:definition xml:lang="en">The descriptors part of the STW - concepts used for indexing.</skos:definition>
    <rdfs:comment xml:lang="en">Among themselves, the Descriptor entries are 
    linked in multiple skos:broader/skos:narrower hierarchies and skos:related 
    connections. To Thsys entries, only skos:broader connections are
    allowed.</rdfs:comment> 
  </rdf:Description>

  <rdf:Description rdf:about="Thsys">
    <rdf:type rdf:resource="http://www.w3.org/2002/07/owl#Class"/>
    <rdfs:label xml:lang="en">Thsys</rdfs:label>
    <rdfs:isDefinedBy rdf:resource="http://zbw.eu/namespaces/zbw-extensions/zbw-extensions.rdf"/>
    <rdfs:subClassOf rdf:resource="http://www.w3.org/2004/02/skos/core#Concept"/>
    <skos:definition xml:lang="en">The systematic part of the STW - concepts used for
    organizing descriptors in broader subject categories.</skos:definition>
    <rdfs:comment xml:lang="en">Each entry has a rdfs:label property for each 
    supported language and one skos:notation property. skos:prefLabel 
    properties are generated by concatenation of these properties. 
    Among themselves, the thsys entries are linked in several
    skos:broader/skos:narrower mono-hierarchies under a top-level 
    "Subthesaurus" Thsys concept. To Descriptor entities, only skos:narrower 
    connections are allowed.</rdfs:comment> 
  </rdf:Description>

  <rdf:Description rdf:about="Found">
    <rdf:type rdf:resource="http://www.w3.org/2002/07/owl#Class"/>
    <rdfs:label xml:lang="en">Found</rdfs:label>
    <rdfs:isDefinedBy rdf:resource="http://zbw.eu/namespaces/zbw-extensions/zbw-extensions.rdf"/>
    <rdfs:subClassOf rdf:resource="http://www.w3.org/2004/02/skos/core#Concept"/>
    <skos:definition xml:lang="en">A skos:Concept (or another object), found
    by a search operation.</skos:definition>
    <rdfs:comment xml:lang="en">Class to mark concepts which were
    matched by a search query, as opposed to other (e.g., skos:narrower or
    skos:related) concepts returned in the same result set. (Experimental)
    </rdfs:comment>
  </rdf:Description>

  <rdf:Description rdf:about="useInsteadNote">
    <rdf:type rdf:resource="http://www.w3.org/2002/07/owl#AnnotationProperty"/>
    <rdfs:label xml:lang="en">useInsteadNote</rdfs:label>
    <rdfs:isDefinedBy rdf:resource="http://zbw.eu/namespaces/zbw-extensions/zbw-extensions.rdf"/>
    <rdfs:subPropertyOf rdf:resource="http://www.w3.org/2004/02/skos/core#note"/>
    <skos:definition xml:lang="en">For an aspect of the current concept use the 
    concept to which the note points instead of the current.</skos:definition>
    <rdfs:comment xml:lang="en">The note consists of a blank node. It contains 
    a rdfs:value literal which designates the aspect and a rdfs:seeAlso link to 
    the concept which should be used instead.</rdfs:comment> 
  </rdf:Description>

  <rdf:Description rdf:about="indexedItem">
    <rdf:type rdf:resource="http://www.w3.org/2002/07/owl#ObjectProperty"/>
    <rdfs:label xml:lang="en">indexedItem</rdfs:label>
    <rdfs:isDefinedBy rdf:resource="http://zbw.eu/namespaces/zbw-extensions/zbw-extensions.rdf"/>
    <rdfs:subPropertyOf rdf:resource="http://www.w3.org/2000/01/rdf-schema#seeAlso"/>
    <skos:definition xml:lang="en">The concept is used as an index term or subject 
    for the resource.</skos:definition>
    <rdfs:comment xml:lang="en">A substitute for the vanished skos:isSubjectOf. 
    May be used with collections of resources also.</rdfs:comment> 
  </rdf:Description>

  <rdf:Description rdf:about="econbizCount">
    <rdf:type rdf:resource="http://www.w3.org/2002/07/owl#FunctionalProperty"/>
    <rdfs:label xml:lang="en">econbizCount</rdfs:label>
    <rdfs:isDefinedBy rdf:resource="http://zbw.eu/namespaces/zbw-extensions/zbw-extensions.rdf"/>
    <rdfs:subPropertyOf rdf:resource="http://rdf.myexperiment.org/ontologies/base/count"/>
    <skos:definition xml:lang="en">Count of matching items in EconBiz (virtual library 
    for economics and business studies, http://econbiz.eu).</skos:definition>
  </rdf:Description>

  <rdf:Description rdf:about="altLabelNarrower">
    <rdf:type rdf:resource="http://www.w3.org/2002/07/owl#AnnotationProperty"/>
    <rdfs:label xml:lang="en">altLabelNarrower</rdfs:label>
    <rdfs:isDefinedBy rdf:resource="http://zbw.eu/namespaces/zbw-extensions/zbw-extensions.rdf"/>
    <skos:definition xml:lang="en">Lexical label for a narrower term which is
    not defined as a separate concept (according to ISO 25964, 8.4), sometimes
    referred to as 'upward posting'. Intended for use with
    skos:Concept, instead of using skos:altLabel.</skos:definition>
  </rdf:Description>

</rdf:RDF>

