<?xml version="1.0" encoding="utf-8"?>
<rdf:RDF
   xmlns:owl="http://www.w3.org/2002/07/owl#"
   xmlns:rdf="http://www.w3.org/1999/02/22-rdf-syntax-ns#"
   xmlns:rdfs="http://www.w3.org/2000/01/rdf-schema#"
   xmlns:skos="http://www.w3.org/2004/02/skos/core#"
   xmlns:vs="http://www.w3.org/2003/06/sw-vocab-status/ns#"
   xmlns:xsd="http://www.w3.org/2001/XMLSchema#"
   xmlns="http://geovocab.org/spatial#">
  <owl:Ontology rdf:about="http://geovocab.org/spatial">
    <rdfs:comment>A vocabulary for describing topological relations between features. $Id: spatial# 81 2012-02-05 11:06:49Z non88sense@gmail.com $</rdfs:comment>
    <rdfs:label>NeoGeo Spatial Ontology</rdfs:label>
    <owl:imports rdf:resource="http://geovocab.org/mappings/spatial"/>
  </owl:Ontology>
  <owl:ObjectProperty rdf:about="http://geovocab.org/spatial#C">
    <rdf:type rdf:resource="http://www.w3.org/2002/07/owl#SymmetricProperty"/>
    <rdfs:comment>Relation C(x,y), read as 'x is connected with y'. This relation holds when two regions share a common point. It is the primitive relation
				in the RCC theory.</rdfs:comment>
    <rdfs:domain rdf:resource="http://geovocab.org/spatial#Feature"/>
    <rdfs:label>connects with</rdfs:label>
    <rdfs:range rdf:resource="http://geovocab.org/spatial#Feature"/>
    <vs:term_status>testing</vs:term_status>
  </owl:ObjectProperty>
  <owl:ObjectProperty rdf:about="http://geovocab.org/spatial#DC">
    <rdf:type rdf:resource="http://www.w3.org/2002/07/owl#SymmetricProperty"/>
    <rdfs:comment>Relation DC(x,y), read as 'x is disconnected from y'. In order to prevent an exponential growth of triples when handling large
				  amounts of data, a closed world assumption may also be possible. More precisely, by considering not explicitely connected regions as discrete
				  regions. Moreover, discrete regions, which are not explicitely labeled as externally connected, would be considered disconnected from
				  eachother.</rdfs:comment>
    <rdfs:domain rdf:resource="http://geovocab.org/spatial#Feature"/>
    <rdfs:label>disconnected from</rdfs:label>
    <rdfs:range rdf:resource="http://geovocab.org/spatial#Feature"/>
    <rdfs:subPropertyOf rdf:resource="http://geovocab.org/spatial#DR"/>
    <vs:term_status>testing</vs:term_status>
  </owl:ObjectProperty>
  <owl:ObjectProperty rdf:about="http://geovocab.org/spatial#DR">
    <rdf:type rdf:resource="http://www.w3.org/2002/07/owl#SymmetricProperty"/>
    <rdfs:comment>Relation DR(x,y), read as 'x is discrete from y'. In order to prevent an exponential growth of triples when handling large
				  amounts of data, a closed world assumption may also be possible. More precisely, by considering not explicitely connected regions as discrete
				  regions. Moreover, discrete regions, which are not explicitely labeled as externally connected, would be considered disconnected from
				  eachother.</rdfs:comment>
    <rdfs:domain rdf:resource="http://geovocab.org/spatial#Feature"/>
    <rdfs:label>discrete from</rdfs:label>
    <rdfs:range rdf:resource="http://geovocab.org/spatial#Feature"/>
    <vs:term_status>testing</vs:term_status>
  </owl:ObjectProperty>
  <owl:ObjectProperty rdf:about="http://geovocab.org/spatial#EC">
    <rdf:type rdf:resource="http://www.w3.org/2002/07/owl#SymmetricProperty"/>
    <rdfs:comment>Relation EC(x,y), read as 'x is externally connected with y'. This relation holds, when the two regions share at least
						 one common point of their borders, but share no points of their interiors, i.e. they do not overlap.</rdfs:comment>
    <rdfs:domain rdf:resource="http://geovocab.org/spatial#Feature"/>
    <rdfs:label>externally connected with</rdfs:label>
    <rdfs:range rdf:resource="http://geovocab.org/spatial#Feature"/>
    <rdfs:subPropertyOf rdf:resource="http://geovocab.org/spatial#C"/>
    <rdfs:subPropertyOf rdf:resource="http://geovocab.org/spatial#DR"/>
    <vs:term_status>testing</vs:term_status>
  </owl:ObjectProperty>
  <owl:ObjectProperty rdf:about="http://geovocab.org/spatial#EQ">
    <rdf:type rdf:resource="http://www.w3.org/2002/07/owl#SymmetricProperty"/>
    <rdf:type rdf:resource="http://www.w3.org/2002/07/owl#TransitiveProperty"/>
    <rdfs:comment>Relation x=y, read as 'x is identical with y'. This relation holds when two regions are spatially co-located.</rdfs:comment>
    <rdfs:domain rdf:resource="http://geovocab.org/spatial#Feature"/>
    <rdfs:label>equals</rdfs:label>
    <rdfs:range rdf:resource="http://geovocab.org/spatial#Feature"/>
    <rdfs:subPropertyOf rdf:resource="http://geovocab.org/spatial#P"/>
    <rdfs:subPropertyOf rdf:resource="http://geovocab.org/spatial#Pi"/>
    <vs:term_status>testing</vs:term_status>
  </owl:ObjectProperty>
  <owl:Class rdf:about="http://geovocab.org/spatial#Feature">
    <rdfs:comment>A geographical feature, capable of holding spatial relations.</rdfs:comment>
    <rdfs:label>Feature</rdfs:label>
    <vs:term_status>testing</vs:term_status>
  </owl:Class>
  <owl:ObjectProperty rdf:about="http://geovocab.org/spatial#NTPP">
    <rdf:type rdf:resource="http://www.w3.org/2002/07/owl#TransitiveProperty"/>
    <rdfs:comment>Relation NTPP(x,y), read as 'x is a non-tangential proper part of y'. This relation holds, whenever a region x is 
							 labeled as a proper part of a region y, and they do not share common point in their borders.</rdfs:comment>
    <rdfs:domain rdf:resource="http://geovocab.org/spatial#Feature"/>
    <rdfs:label>is non-tangential proper part of</rdfs:label>
    <rdfs:range rdf:resource="http://geovocab.org/spatial#Feature"/>
    <rdfs:subPropertyOf rdf:resource="http://geovocab.org/spatial#PP"/>
    <vs:term_status>testing</vs:term_status>
  </owl:ObjectProperty>
  <owl:ObjectProperty rdf:about="http://geovocab.org/spatial#NTPPi">
    <rdf:type rdf:resource="http://www.w3.org/2002/07/owl#TransitiveProperty"/>
    <rdfs:comment>Relation NTPPi(x,y), read as 'x non-tangentially properly contains y'. Inverse of the NTPP(x,y) relation.</rdfs:comment>
    <rdfs:domain rdf:resource="http://geovocab.org/spatial#Feature"/>
    <rdfs:label>non tangentially properly contains</rdfs:label>
    <rdfs:range rdf:resource="http://geovocab.org/spatial#Feature"/>
    <rdfs:subPropertyOf rdf:resource="http://geovocab.org/spatial#PPi"/>
    <owl:inverseOf rdf:resource="http://geovocab.org/spatial#NTPP"/>
    <vs:term_status>testing</vs:term_status>
  </owl:ObjectProperty>
  <owl:ObjectProperty rdf:about="http://geovocab.org/spatial#O">
    <rdf:type rdf:resource="http://www.w3.org/2002/07/owl#SymmetricProperty"/>
    <rdfs:comment>Relation O(x,y), read as 'x overlaps y'. A region x overlaps a region y, if they share at least one common point of their interiors.</rdfs:comment>
    <rdfs:domain rdf:resource="http://geovocab.org/spatial#Feature"/>
    <rdfs:label>overlaps</rdfs:label>
    <rdfs:range rdf:resource="http://geovocab.org/spatial#Feature"/>
    <rdfs:subPropertyOf rdf:resource="http://geovocab.org/spatial#C"/>
    <vs:term_status>testing</vs:term_status>
  </owl:ObjectProperty>
  <owl:ObjectProperty rdf:about="http://geovocab.org/spatial#P">
    <rdf:type rdf:resource="http://www.w3.org/2002/07/owl#TransitiveProperty"/>
    <rdfs:comment>Relation P(x,y), read as 'x is a part of y', holds whenever the region x is contained within the borders of the region y.</rdfs:comment>
    <rdfs:domain rdf:resource="http://geovocab.org/spatial#Feature"/>
    <rdfs:label>is part of</rdfs:label>
    <rdfs:range rdf:resource="http://geovocab.org/spatial#Feature"/>
    <rdfs:subPropertyOf rdf:resource="http://geovocab.org/spatial#O"/>
    <owl:inverseOf rdf:resource="http://geovocab.org/spatial#Pi"/>
    <vs:term_status>testing</vs:term_status>
  </owl:ObjectProperty>
  <owl:ObjectProperty rdf:about="http://geovocab.org/spatial#PO">
    <rdf:type rdf:resource="http://www.w3.org/2002/07/owl#SymmetricProperty"/>
    <rdfs:comment>Relation PO(x,y), read as 'x partially overlaps y'. A region x overlaps a region y, if they share at least one common point of their 
				   interiors, and one does not contain the other within its borders.</rdfs:comment>
    <rdfs:domain rdf:resource="http://geovocab.org/spatial#Feature"/>
    <rdfs:label>partially overlaps</rdfs:label>
    <rdfs:range rdf:resource="http://geovocab.org/spatial#Feature"/>
    <rdfs:subPropertyOf rdf:resource="http://geovocab.org/spatial#O"/>
    <vs:term_status>testing</vs:term_status>
  </owl:ObjectProperty>
  <owl:ObjectProperty rdf:about="http://geovocab.org/spatial#PP">
    <rdf:type rdf:resource="http://www.w3.org/2002/07/owl#TransitiveProperty"/>
    <rdfs:comment>Relation PP(x,y), read as 'x is a proper part of y', means that the region x is contained within the borders of the 
				region y, and region y is not contained within the borders of the region y, which means they are not equals.</rdfs:comment>
    <rdfs:domain rdf:resource="http://geovocab.org/spatial#Feature"/>
    <rdfs:label>is proper part of</rdfs:label>
    <rdfs:range rdf:resource="http://geovocab.org/spatial#Feature"/>
    <rdfs:subPropertyOf rdf:resource="http://geovocab.org/spatial#P"/>
    <owl:inverseOf rdf:resource="http://geovocab.org/spatial#PPi"/>
    <vs:term_status>testing</vs:term_status>
  </owl:ObjectProperty>
  <owl:ObjectProperty rdf:about="http://geovocab.org/spatial#PPi">
    <rdf:type rdf:resource="http://www.w3.org/2002/07/owl#TransitiveProperty"/>
    <rdfs:comment>Relation PPi(x,y), read as 'x properly contains y'. Inverse of the PP(x,y) relation.</rdfs:comment>
    <rdfs:domain rdf:resource="http://geovocab.org/spatial#Feature"/>
    <rdfs:label>properly contains</rdfs:label>
    <rdfs:range rdf:resource="http://geovocab.org/spatial#Feature"/>
    <rdfs:subPropertyOf rdf:resource="http://geovocab.org/spatial#Pi"/>
    <vs:term_status>testing</vs:term_status>
  </owl:ObjectProperty>
  <owl:ObjectProperty rdf:about="http://geovocab.org/spatial#Pi">
    <rdf:type rdf:resource="http://www.w3.org/2002/07/owl#TransitiveProperty"/>
    <rdfs:comment>Relation Pi(x,y), read as 'x contains y'. Inverse of the P(x,y) relation.</rdfs:comment>
    <rdfs:domain rdf:resource="http://geovocab.org/spatial#Feature"/>
    <rdfs:label>contains</rdfs:label>
    <rdfs:range rdf:resource="http://geovocab.org/spatial#Feature"/>
    <rdfs:subPropertyOf rdf:resource="http://geovocab.org/spatial#O"/>
    <vs:term_status>testing</vs:term_status>
  </owl:ObjectProperty>
  <owl:ObjectProperty rdf:about="http://geovocab.org/spatial#TPP">
    <rdf:type rdf:resource="http://www.w3.org/2002/07/owl#TransitiveProperty"/>
    <rdfs:comment>Relation TPP(x,y), read as 'x is a tangential proper part of y'. This relation holds, whenever a region x is 
						  labeled as a proper part of a region y, and they share at least one common point in their borders, which means that they are
						  externally connected.</rdfs:comment>
    <rdfs:domain rdf:resource="http://geovocab.org/spatial#Feature"/>
    <rdfs:label>is tangential proper part of</rdfs:label>
    <rdfs:range rdf:resource="http://geovocab.org/spatial#Feature"/>
    <rdfs:subPropertyOf rdf:resource="http://geovocab.org/spatial#PP"/>
    <vs:term_status>testing</vs:term_status>
  </owl:ObjectProperty>
  <owl:ObjectProperty rdf:about="http://geovocab.org/spatial#TPPi">
    <rdf:type rdf:resource="http://www.w3.org/2002/07/owl#TransitiveProperty"/>
    <rdfs:comment>Relation TPPi(x,y), read as 'x tangentially properly contains y'. Inverse of the TPP(x,y) relation.</rdfs:comment>
    <rdfs:domain rdf:resource="http://geovocab.org/spatial#Feature"/>
    <rdfs:label>tangentially properly contains</rdfs:label>
    <rdfs:range rdf:resource="http://geovocab.org/spatial#Feature"/>
    <rdfs:subPropertyOf rdf:resource="http://geovocab.org/spatial#PPi"/>
    <owl:inverseOf rdf:resource="http://geovocab.org/spatial#TPP"/>
    <vs:term_status>testing</vs:term_status>
  </owl:ObjectProperty>
  <owl:ObjectProperty rdf:about="http://geovocab.org/spatial#inconsistentWith">
    <rdf:type rdf:resource="http://www.w3.org/2002/07/owl#SymmetricProperty"/>
    <rdfs:comment>Although this relation is not a part of the RCC theory, it has been introduced in order to detect relations between regions
								which are inconsistent with the RCC axioms.</rdfs:comment>
    <rdfs:label>inconsistent with</rdfs:label>
    <vs:term_status>unstable</vs:term_status>
  </owl:ObjectProperty>
</rdf:RDF>
