<?xml version="1.0"?>
<rdf:RDF xmlns="http://linked.earth/ontology#"
     xml:base="http://linked.earth/ontology"
     xmlns:vaem="http://www.linkedmodel.org/schema/vaem#"
     xmlns:rdf="http://www.w3.org/1999/02/22-rdf-syntax-ns#"
     xmlns:owl="http://www.w3.org/2002/07/owl#"
     xmlns:xml="http://www.w3.org/XML/1998/namespace"
     xmlns:xsd="http://www.w3.org/2001/XMLSchema#"
     xmlns:dcterms="http://purl.org/dc/terms/"
     xmlns:rdfs="http://www.w3.org/2000/01/rdf-schema#"
     xmlns:vann="http://purl.org/vocab/vann/">
    <owl:Ontology rdf:about="http://linked.earth/ontology#">
        <rdfs:comment xml:lang="en">The Linked Earth Ontology aims to provide a common vocabulary for annotating paleoclimatology data</rdfs:comment>
        <vann:preferredNamespacePrefix>le</vann:preferredNamespacePrefix>
        <owl:versionInfo xml:lang="en">1.2.0</owl:versionInfo>
        <dcterms:description xml:lang="en">The Linked Earth Ontology aims to provide a common vocabulary for annotating paleoclimatology data</dcterms:description>
        <vann:preferredNamespaceUri>http://linked.earth/ontology#</vann:preferredNamespaceUri>
        <dcterms:license rdf:resource="http://creativecommons.org/licenses/by/2.0/"/>
    </owl:Ontology>
    


    <!-- 
    ///////////////////////////////////////////////////////////////////////////////////////
    //
    // Annotation properties
    //
    ///////////////////////////////////////////////////////////////////////////////////////
     -->

    


    <!-- http://purl.org/vocab/vann/example -->

    <owl:AnnotationProperty rdf:about="http://purl.org/vocab/vann/example"/>
    


    <!-- http://www.linkedmodel.org/schema/vaem#rationale -->

    <owl:AnnotationProperty rdf:about="http://www.linkedmodel.org/schema/vaem#rationale"/>
    


    <!-- 
    ///////////////////////////////////////////////////////////////////////////////////////
    //
    // Datatypes
    //
    ///////////////////////////////////////////////////////////////////////////////////////
     -->

    


    <!-- http://www.w3.org/2000/01/rdf-schema#Literal -->

    <rdf:Description rdf:about="http://www.w3.org/2000/01/rdf-schema#Literal">
        <owl:equivalentClass rdf:resource="http://www.w3.org/2001/XMLSchema#string"/>
    </rdf:Description>
    


    <!-- 
    ///////////////////////////////////////////////////////////////////////////////////////
    //
    // Object Properties
    //
    ///////////////////////////////////////////////////////////////////////////////////////
     -->

    


    <!-- http://linked.earth/ontology#author -->

    <owl:ObjectProperty rdf:about="http://linked.earth/ontology#author">
        <rdfs:subPropertyOf rdf:resource="http://purl.org/dc/terms/creator"/>
        <rdfs:subPropertyOf rdf:resource="http://schema.org/author"/>
        <rdfs:domain>
            <owl:Class>
                <owl:unionOf rdf:parseType="Collection">
                    <rdf:Description rdf:about="http://linked.earth/ontology#Compilation"/>
                    <rdf:Description rdf:about="http://linked.earth/ontology#Dataset"/>
                    <rdf:Description rdf:about="http://linked.earth/ontology#Publication"/>
                </owl:unionOf>
            </owl:Class>
        </rdfs:domain>
        <rdfs:range rdf:resource="http://linked.earth/ontology#Person"/>
        <vann:example rdf:resource="http://wiki.linked.earth/Publication.10.1002/2013PA002534"/>
        <vaem:rationale xml:lang="en">Give credit to the original author of the resource</vaem:rationale>
        <rdfs:comment xml:lang="en">Answers the question: Who wrote (i.e., created) the resource, such as a Publication?</rdfs:comment>
        <rdfs:label xml:lang="en">author</rdfs:label>
    </owl:ObjectProperty>
    


    <!-- http://linked.earth/ontology#calibratedVia -->

    <owl:ObjectProperty rdf:about="http://linked.earth/ontology#calibratedVia">
        <rdfs:domain rdf:resource="http://linked.earth/ontology#InferredVariable"/>
        <rdfs:range rdf:resource="http://linked.earth/ontology#CalibrationModel"/>
        <vann:example rdf:resource="http://wiki.linked.earth/MD982181.Khider.2014.paleo1measurement2.sst"/>
        <vaem:rationale xml:lang="en">Provides calibration information, especially useful for legacy datasets where the raw measurements may not be available and for comparison of datasets.</vaem:rationale>
        <rdfs:comment xml:lang="en">Answers the question: What calibration process was used to relate the InferredVariable to the MeasuredVariable?</rdfs:comment>
        <rdfs:label xml:lang="en">calibrated via</rdfs:label>
    </owl:ObjectProperty>
    


    <!-- http://linked.earth/ontology#calibrationReferences -->

    <owl:ObjectProperty rdf:about="http://linked.earth/ontology#calibrationReferences">
        <rdfs:subPropertyOf rdf:resource="http://purl.org/dc/terms/references"/>
        <rdfs:domain rdf:resource="http://linked.earth/ontology#CalibrationModel"/>
        <rdfs:range rdf:resource="http://linked.earth/ontology#Publication"/>
        <vann:example rdf:resource="http://wiki.linked.earth/MD982181.Khider.2014.paleo1measurement1.mgcarub.Calibration"/>
        <vaem:rationale xml:lang="en">Relationship needed to link to a Publication desribing the calibration being applied to the dataset</vaem:rationale>
        <rdfs:comment xml:lang="en">Answers the question: In what Reference(s) is the Calibration described/justified?</rdfs:comment>
        <rdfs:label xml:lang="en">calibration references</rdfs:label>
    </owl:ObjectProperty>
    


    <!-- http://linked.earth/ontology#chronModeledBy -->

    <owl:ObjectProperty rdf:about="http://linked.earth/ontology#chronModeledBy">
        <rdfs:subPropertyOf rdf:resource="http://linked.earth/ontology#modeledBy"/>
        <rdfs:domain>
            <owl:Class>
                <owl:unionOf rdf:parseType="Collection">
                    <rdf:Description rdf:about="http://linked.earth/ontology#ChronData"/>
                    <rdf:Description rdf:about="http://linked.earth/ontology#ChronProxySystem"/>
                </owl:unionOf>
            </owl:Class>
        </rdfs:domain>
        <rdfs:range rdf:resource="http://linked.earth/ontology#ChronModel"/>
        <vaem:rationale xml:lang="en">Subproperty of modeledBy. The subdivision between chronological and paleoenvironmental information reflects the fact that Datasets are fundamentally characterized by two distinct components</vaem:rationale>
        <rdfs:comment xml:lang="en">Answers the question: What is the ChronModel for the ChronData or ProxySystem under consideration?</rdfs:comment>
        <rdfs:label xml:lang="en">chron modeled by</rdfs:label>
    </owl:ObjectProperty>
    


    <!-- http://linked.earth/ontology#collectedFrom -->

    <owl:ObjectProperty rdf:about="http://linked.earth/ontology#collectedFrom">
        <rdfs:subPropertyOf rdf:resource="http://schema.org/contentLocation"/>
        <rdfs:domain rdf:resource="http://linked.earth/ontology#Dataset"/>
        <rdfs:range rdf:resource="http://linked.earth/ontology#Location"/>
        <vann:example rdf:resource="http://wiki.linked.earth/MD982181.Khider.2014"/>
        <vaem:rationale xml:lang="en">Describe the geographical coordinates for the provenance of the ProxyArchive where the dataset was collected from</vaem:rationale>
        <rdfs:comment xml:lang="en">Answers the question: Where (in the world) was the data in the Dataset collected? Refers to the location of the ProxyArchive</rdfs:comment>
        <rdfs:label xml:lang="en">collected from</rdfs:label>
    </owl:ObjectProperty>
    


    <!-- http://linked.earth/ontology#contributor -->

    <owl:ObjectProperty rdf:about="http://linked.earth/ontology#contributor">
        <rdfs:subPropertyOf rdf:resource="http://purl.org/dc/terms/contributor"/>
        <rdfs:subPropertyOf rdf:resource="http://schema.org/contributor"/>
        <rdfs:domain rdf:resource="http://linked.earth/ontology#Dataset"/>
        <rdfs:range rdf:resource="http://linked.earth/ontology#Person"/>
        <vann:example rdf:resource="http://wiki.linked.earth/MD982181.Khider.2014"/>
        <vaem:rationale xml:lang="en">Allows distinction between contributor to a resource and the author</vaem:rationale>
        <rdfs:comment xml:lang="en">Answers the question: Who contributed the resource? A contributor may be the same as the authors of the resource or different. For instance, in the case of a legacy dataset, a Linked Earth member may contribute a previously-published dataset that he/she may not have authored</rdfs:comment>
        <rdfs:label xml:lang="en">contributor</rdfs:label>
    </owl:ObjectProperty>
    


    <!-- http://linked.earth/ontology#distributionTableGeneratedByModel -->

    <owl:ObjectProperty rdf:about="http://linked.earth/ontology#distributionTableGeneratedByModel">
        <rdfs:subPropertyOf rdf:resource="http://linked.earth/ontology#generatedByModel"/>
        <rdf:type rdf:resource="http://www.w3.org/2002/07/owl#FunctionalProperty"/>
        <rdfs:domain rdf:resource="http://linked.earth/ontology#DistributionTable"/>
        <rdfs:range>
            <owl:Class>
                <owl:unionOf rdf:parseType="Collection">
                    <rdf:Description rdf:about="http://linked.earth/ontology#ChronModel"/>
                    <rdf:Description rdf:about="http://linked.earth/ontology#PaleoModel"/>
                </owl:unionOf>
            </owl:Class>
        </rdfs:range>
        <vann:example rdf:resource="http://wiki.linked.earth/ODP1098B1_2.ChronData1.Model1"/>
        <vaem:rationale xml:lang="en">&quot;Subproperty of foundinTable to Link the Model to its outputs&quot;</vaem:rationale>
        <rdfs:comment xml:lang="en">Answers the question: In which DistributionTable is the Model output found?</rdfs:comment>
        <rdfs:label xml:lang="en">distribution table generated by Model</rdfs:label>
    </owl:ObjectProperty>
    


    <!-- http://linked.earth/ontology#ensembleTableGeneratedByModel -->

    <owl:ObjectProperty rdf:about="http://linked.earth/ontology#ensembleTableGeneratedByModel">
        <rdfs:subPropertyOf rdf:resource="http://linked.earth/ontology#generatedByModel"/>
        <rdf:type rdf:resource="http://www.w3.org/2002/07/owl#FunctionalProperty"/>
        <rdfs:domain rdf:resource="http://linked.earth/ontology#EnsembleTable"/>
        <rdfs:range>
            <owl:Class>
                <owl:unionOf rdf:parseType="Collection">
                    <rdf:Description rdf:about="http://linked.earth/ontology#ChronModel"/>
                    <rdf:Description rdf:about="http://linked.earth/ontology#PaleoModel"/>
                </owl:unionOf>
            </owl:Class>
        </rdfs:range>
        <vaem:rationale rdf:resource="http://wiki.linked.earth/ODP1098B1_2.ChronData1.Model1"/>
        <vaem:rationale xml:lang="en">&quot;Subproperty of foundinTable to link the Model to its outputs&quot;</vaem:rationale>
        <rdfs:comment xml:lang="en">Answers the question: In which EnsembleTable is the Model output found?</rdfs:comment>
        <rdfs:label xml:lang="en">ensemble table generated by model</rdfs:label>
    </owl:ObjectProperty>
    


    <!-- http://linked.earth/ontology#foundInMeasurementTable -->

    <owl:ObjectProperty rdf:about="http://linked.earth/ontology#foundInMeasurementTable">
        <rdfs:subPropertyOf rdf:resource="http://linked.earth/ontology#foundInTable"/>
        <rdfs:domain rdf:resource="http://linked.earth/ontology#Data"/>
        <rdfs:range rdf:resource="http://linked.earth/ontology#MeasurementTable"/>
        <vann:example rdf:resource="http://wiki.linked.earth/MD982181.Khider.2014.PaleoData1"/>
        <vaem:rationale xml:lang="en">Subproperty of foundinTable to link the Data to the Variables</vaem:rationale>
        <rdfs:comment xml:lang="en">Answers the question: In which MeasurementTable are the Variables found?</rdfs:comment>
        <rdfs:label xml:lang="en">found in measurement table</rdfs:label>
    </owl:ObjectProperty>
    


    <!-- http://linked.earth/ontology#foundInTable -->

    <owl:ObjectProperty rdf:about="http://linked.earth/ontology#foundInTable">
        <rdfs:domain>
            <owl:Class>
                <owl:unionOf rdf:parseType="Collection">
                    <rdf:Description rdf:about="http://linked.earth/ontology#Data"/>
                    <rdf:Description rdf:about="http://linked.earth/ontology#Variable"/>
                </owl:unionOf>
            </owl:Class>
        </rdfs:domain>
        <rdfs:range rdf:resource="http://linked.earth/ontology#DataTable"/>
        <vaem:rationale xml:lang="en">Allows to link the data to the csv table and the models to its output</vaem:rationale>
        <rdfs:comment xml:lang="en">Answers the question: In which DataTable can the information/data be found?</rdfs:comment>
        <rdfs:label xml:lang="en">found in table</rdfs:label>
    </owl:ObjectProperty>
    


    <!-- http://linked.earth/ontology#fundedBy -->

    <owl:ObjectProperty rdf:about="http://linked.earth/ontology#fundedBy">
        <rdfs:subPropertyOf rdf:resource="http://schema.org/funder"/>
        <rdfs:domain>
            <owl:Class>
                <owl:unionOf rdf:parseType="Collection">
                    <rdf:Description rdf:about="http://linked.earth/ontology#Compilation"/>
                    <rdf:Description rdf:about="http://linked.earth/ontology#Dataset"/>
                </owl:unionOf>
            </owl:Class>
        </rdfs:domain>
        <rdfs:range rdf:resource="http://linked.earth/ontology#Funding"/>
        <vann:example rdf:resource="http://wiki.linked.earth/MD982181.Khider.2014"/>
        <vaem:rationale xml:lang="en">Links a dataset to its source of funding</vaem:rationale>
        <rdfs:comment xml:lang="en">Answers the question: What was the Funding source for the Dataset?</rdfs:comment>
        <rdfs:label xml:lang="en">funded by</rdfs:label>
    </owl:ObjectProperty>
    


    <!-- http://linked.earth/ontology#generatedByModel -->

    <owl:ObjectProperty rdf:about="http://linked.earth/ontology#generatedByModel">
        <rdfs:subPropertyOf rdf:resource="http://www.w3.org/ns/prov#wasDerivedFrom"/>
        <rdfs:domain rdf:resource="http://linked.earth/ontology#DataTable"/>
        <rdfs:range rdf:resource="http://linked.earth/ontology#Model"/>
        <vaem:rationale xml:lang="en">Needed to link the model to the data tables it generates</vaem:rationale>
        <rdfs:comment xml:lang="en">Answers the question: which model was used to generated this data table?</rdfs:comment>
        <rdfs:label xml:lang="en">generated by model</rdfs:label>
    </owl:ObjectProperty>
    


    <!-- http://linked.earth/ontology#hasCode -->

    <owl:ObjectProperty rdf:about="http://linked.earth/ontology#hasCode">
        <rdf:type rdf:resource="http://www.w3.org/2002/07/owl#FunctionalProperty"/>
        <rdfs:domain rdf:resource="http://linked.earth/ontology#Model"/>
        <rdfs:range rdf:resource="http://linked.earth/ontology#SoftwareCode"/>
        <vaem:rationale xml:lang="en">Links a Model to its SoftwareCode.</vaem:rationale>
        <rdfs:comment xml:lang="en">Answers the question: What SoftwareCode was used to generate the Model output?</rdfs:comment>
        <rdfs:label xml:lang="en">has code</rdfs:label>
    </owl:ObjectProperty>
    


    <!-- http://linked.earth/ontology#hasIntegrationTime -->

    <owl:ObjectProperty rdf:about="http://linked.earth/ontology#hasIntegrationTime">
        <rdfs:domain rdf:resource="http://linked.earth/ontology#ProxySensor"/>
        <rdfs:range rdf:resource="http://linked.earth/ontology#IntegrationTime"/>
        <vaem:rationale xml:lang="en">Property added to link the proxySystem to the IntegrationTime class</vaem:rationale>
        <rdfs:comment xml:lang="en">Answers the question: What is the integration time needed for a ProxySensor to imprint environmental information on the ProxyArchive? Both are included as part of a ProxySystem</rdfs:comment>
        <rdfs:label xml:lang="en">has integration time</rdfs:label>
    </owl:ObjectProperty>
    


    <!-- http://linked.earth/ontology#hasProxySystem -->

    <owl:ObjectProperty rdf:about="http://linked.earth/ontology#hasProxySystem">
        <rdfs:domain rdf:resource="http://linked.earth/ontology#MeasuredVariable"/>
        <rdfs:range rdf:resource="http://linked.earth/ontology#ProxySystem"/>
        <vann:example rdf:resource="http://wiki.linked.earth/MD982181.Khider.2014.paleo1measurement1.mgcarub"/>
        <vaem:rationale xml:lang="en">Links the MeasuredVariable to its ProxySystem. For instance, Mg/Ca measurements on foraminiferal shells have ProxySystem: MarineSediment.Foraminifera.Mg/Ca</vaem:rationale>
        <rdfs:comment xml:lang="en">Answers the question: What is the ProxySystem associated with this MeasuredVariable?</rdfs:comment>
        <rdfs:label xml:lang="en">has proxy system</rdfs:label>
    </owl:ObjectProperty>
    


    <!-- http://linked.earth/ontology#hasResolution -->

    <owl:ObjectProperty rdf:about="http://linked.earth/ontology#hasResolution">
        <rdfs:domain rdf:resource="http://linked.earth/ontology#Variable"/>
        <rdfs:range rdf:resource="http://linked.earth/ontology#Resolution"/>
        <vann:example xml:lang="en">http://wiki.linked.earth/MD982181.Khider.2014.paleo1measurement1.mgcarub.ICPAES</vann:example>
        <vaem:rationale xml:lang="en">Needed to link a Variable to Resolution</vaem:rationale>
        <rdfs:comment>Answers the question: What is the Resolution of the Variable?</rdfs:comment>
        <rdfs:label xml:lang="en">has resolution</rdfs:label>
    </owl:ObjectProperty>
    


    <!-- http://linked.earth/ontology#hasUncertainty -->

    <owl:ObjectProperty rdf:about="http://linked.earth/ontology#hasUncertainty">
        <rdfs:domain>
            <owl:Class>
                <owl:unionOf rdf:parseType="Collection">
                    <rdf:Description rdf:about="http://linked.earth/ontology#Instrument"/>
                    <rdf:Description rdf:about="http://linked.earth/ontology#Model"/>
                    <rdf:Description rdf:about="http://linked.earth/ontology#Variable"/>
                </owl:unionOf>
            </owl:Class>
        </rdfs:domain>
        <rdfs:range rdf:resource="http://linked.earth/ontology#Uncertainty"/>
        <vann:example rdf:resource="http://wiki.linked.earth/MD982181.Khider.2014.paleo1measurement1.mgcarub"/>
        <vaem:rationale xml:lang="en">Links to the Uncertainty class</vaem:rationale>
        <rdfs:comment xml:lang="en">Answers the question: What is the Uncertainty associated with the Variable, Model, or Instrument?</rdfs:comment>
        <rdfs:label xml:lang="en">has uncertainty</rdfs:label>
    </owl:ObjectProperty>
    


    <!-- http://linked.earth/ontology#includesChronData -->

    <owl:ObjectProperty rdf:about="http://linked.earth/ontology#includesChronData">
        <rdfs:subPropertyOf rdf:resource="http://linked.earth/ontology#includesData"/>
        <rdfs:domain rdf:resource="http://linked.earth/ontology#Dataset"/>
        <rdfs:range rdf:resource="http://linked.earth/ontology#ChronData"/>
        <vann:example rdf:resource="http://wiki.linked.earth/MD982181.Khider.2014"/>
        <vaem:rationale xml:lang="en">Subproperty of includesData. The subdivision between chronological and paleoenvironmental information reflects the fact that Datasets are fundamentally characterized by two distinct components</vaem:rationale>
        <rdfs:comment xml:lang="en">Answers the question: Which ChronData are included in the Dataset?</rdfs:comment>
        <rdfs:label xml:lang="en">includes chron data</rdfs:label>
    </owl:ObjectProperty>
    


    <!-- http://linked.earth/ontology#includesData -->

    <owl:ObjectProperty rdf:about="http://linked.earth/ontology#includesData">
        <rdfs:domain rdf:resource="http://linked.earth/ontology#Dataset"/>
        <rdfs:range rdf:resource="http://linked.earth/ontology#Data"/>
        <vaem:rationale xml:lang="en">Links Dataset to Data</vaem:rationale>
        <rdfs:comment xml:lang="en">Answers the question: Which Data are included in the Dataset?</rdfs:comment>
        <rdfs:label xml:lang="en">includes data</rdfs:label>
    </owl:ObjectProperty>
    


    <!-- http://linked.earth/ontology#includesPaleoData -->

    <owl:ObjectProperty rdf:about="http://linked.earth/ontology#includesPaleoData">
        <rdfs:subPropertyOf rdf:resource="http://linked.earth/ontology#includesData"/>
        <rdfs:domain rdf:resource="http://linked.earth/ontology#Dataset"/>
        <rdfs:range rdf:resource="http://linked.earth/ontology#PaleoData"/>
        <vann:example rdf:resource="http://wiki.linked.earth/MD982181.Khider.2014"/>
        <vaem:rationale xml:lang="en">Subproperty of includesData. The subdivision between chronological and paleoenvironmental information reflects the fact that Datasets are fundamentally characterized by two distinct components</vaem:rationale>
        <rdfs:comment xml:lang="en">Answers the question: Which PaleoData are included in the Dataset?</rdfs:comment>
        <rdfs:label xml:lang="en">includes paleo data</rdfs:label>
    </owl:ObjectProperty>
    


    <!-- http://linked.earth/ontology#includesVariable -->

    <owl:ObjectProperty rdf:about="http://linked.earth/ontology#includesVariable">
        <rdfs:domain rdf:resource="http://linked.earth/ontology#DataTable"/>
        <rdfs:range rdf:resource="http://linked.earth/ontology#Variable"/>
        <vann:example rdf:resource="http://wiki.linked.earth/MD982181.Khider.2014.paleo1measurement2"/>
        <vaem:rationale xml:lang="en">Links DataTable to Variable</vaem:rationale>
        <rdfs:comment xml:lang="en">Answers the question: Which Variables are included in the DataTable?</rdfs:comment>
        <rdfs:label xml:lang="en">includes variable</rdfs:label>
    </owl:ObjectProperty>
    


    <!-- http://linked.earth/ontology#inferredFrom -->

    <owl:ObjectProperty rdf:about="http://linked.earth/ontology#inferredFrom">
        <rdfs:domain rdf:resource="http://linked.earth/ontology#InferredVariable"/>
        <rdfs:range rdf:resource="http://linked.earth/ontology#MeasuredVariable"/>
        <vann:example rdf:resource="http://wiki.linked.earth/MD982181.Khider.2014.paleo1measurement2.sst"/>
        <vaem:rationale xml:lang="en">Provides a link between the Measured and Inferred Variables. For instance, SST is inferred from Mg/Ca measurements</vaem:rationale>
        <rdfs:comment xml:lang="en">Answers the question: From which MeasuredVariable(s) is (are) the InferredVariable inferred from?</rdfs:comment>
        <rdfs:label xml:lang="en">inferred from</rdfs:label>
    </owl:ObjectProperty>
    


    <!-- http://linked.earth/ontology#inferredVariableType -->

    <owl:ObjectProperty rdf:about="http://linked.earth/ontology#inferredVariableType">
        <rdfs:domain rdf:resource="http://linked.earth/ontology#InferredVariable"/>
        <rdfs:range rdf:resource="http://linked.earth/ontology#InferredVariable"/>
        <vann:example rdf:resource="http://wiki.linked.earth/MD982181.Khider.2014.paleo1measurement2.sst"/>
        <vaem:rationale xml:lang="en">Links the InferredVariable values to their type. For instance, the value of 29.1 degC is of type SST. This is important to normalize the variations in VariableNames (e.g. SST, sst, sea-surface temp)</vaem:rationale>
        <rdfs:comment xml:lang="en">Answers the question: What type of InferredVariable does the InferredVariable belongs to?</rdfs:comment>
        <rdfs:label xml:lang="en">inferred variable type</rdfs:label>
    </owl:ObjectProperty>
    


    <!-- http://linked.earth/ontology#interpretationReferences -->

    <owl:ObjectProperty rdf:about="http://linked.earth/ontology#interpretationReferences">
        <rdfs:subPropertyOf rdf:resource="http://purl.org/dc/terms/references"/>
        <rdfs:domain rdf:resource="http://linked.earth/ontology#Interpretation"/>
        <rdfs:range rdf:resource="http://linked.earth/ontology#Publication"/>
        <vann:example rdf:resource="http://wiki.linked.earth/MD982181.Khider.2014.paleo1measurement1.mgcarub.Calibration"/>
        <vaem:rationale xml:lang="en">Links an interpretation to a reference citation (can be the same as the calibrationReferences for a Dataset)</vaem:rationale>
        <rdfs:comment xml:lang="en">Answers the question: In which Publication(s) is the Interpretation substantiated?</rdfs:comment>
        <rdfs:label xml:lang="en">interpretation references</rdfs:label>
    </owl:ObjectProperty>
    


    <!-- http://linked.earth/ontology#interpretedAs -->

    <owl:ObjectProperty rdf:about="http://linked.earth/ontology#interpretedAs">
        <rdfs:domain rdf:resource="http://linked.earth/ontology#Variable"/>
        <rdfs:range rdf:resource="http://linked.earth/ontology#Interpretation"/>
        <vann:example rdf:resource="http://wiki.linked.earth/MD982181.Khider.2014.paleo1measurement2.sst"/>
        <vaem:rationale xml:lang="en">Links the Variable to its Interpretation</vaem:rationale>
        <rdfs:comment xml:lang="en">Answers the question: What is the Variable&apos;s Interpretation?</rdfs:comment>
        <rdfs:label xml:lang="en">interpreted as</rdfs:label>
    </owl:ObjectProperty>
    


    <!-- http://linked.earth/ontology#measuredBy -->

    <owl:ObjectProperty rdf:about="http://linked.earth/ontology#measuredBy">
        <rdfs:subPropertyOf rdf:resource="http://purl.oclc.org/NET/ssnx/ssn#observedBy"/>
        <rdfs:domain rdf:resource="http://linked.earth/ontology#MeasuredVariable"/>
        <rdfs:range rdf:resource="http://linked.earth/ontology#Instrument"/>
        <vann:example rdf:resource="http://wiki.linked.earth/MD982181.Khider.2014.paleo1measurement2.mgcarub"/>
        <vaem:rationale xml:lang="en">Links the MeasuredVariable to the Instrument responsible for its creation</vaem:rationale>
        <rdfs:comment xml:lang="en">Answers the question: Which Instrument was used to produce the MeasuredVariable?</rdfs:comment>
        <rdfs:label xml:lang="en">measured by</rdfs:label>
    </owl:ObjectProperty>
    


    <!-- http://linked.earth/ontology#measuredOn -->

    <owl:ObjectProperty rdf:about="http://linked.earth/ontology#measuredOn">
        <rdfs:subPropertyOf rdf:resource="http://www.w3.org/2002/07/owl#topObjectProperty"/>
        <rdfs:domain rdf:resource="http://linked.earth/ontology#MeasuredVariable"/>
        <rdfs:range rdf:resource="http://linked.earth/ontology#PhysicalSample"/>
        <vann:example rdf:resource="http://wiki.linked.earth/MD982181.Khider.2014.paleo1measurement1.d18omund"/>
        <vann:example rdf:resource="http://wiki.linked.earth/MD982181.Khider.2014.paleo1measurement2.mgcarub"/>
        <vaem:rationale xml:lang="en">Links the MeasuredVariable to the ProxyArchive. Refers to the specific archive (i.e. the specific coral head, lake sediment...) and a specific Variable since ProxyArchive provides a link to the ProxySensor. In some instances, two MeasuredVariables on the same PhysicalSample may have different ProxyArchive page. This would be the case for measurements on various species of foraminifera in a MarineSediment</vaem:rationale>
        <rdfs:comment xml:lang="en">Answers the question: On which PhysicalSample was the MeasuredVariable measured?</rdfs:comment>
        <rdfs:label xml:lang="en">measured on</rdfs:label>
    </owl:ObjectProperty>
    


    <!-- http://linked.earth/ontology#modelReferences -->

    <owl:ObjectProperty rdf:about="http://linked.earth/ontology#modelReferences">
        <rdfs:subPropertyOf rdf:resource="http://purl.org/dc/terms/references"/>
        <rdfs:domain rdf:resource="http://linked.earth/ontology#Model"/>
        <rdfs:range rdf:resource="http://linked.earth/ontology#Publication"/>
        <vann:example rdf:resource="http://wiki.linked.earth/MD982181.Khider.2014.paleo1measurement1.mgcarub.Calibration"/>
        <vaem:rationale xml:lang="en">Links a Model to its Publication. 
Note: calibrationReferences and modelReferences in the Calibration may not need to be the same. For instance, the calibration data and one mathematical formulation can be provided in one Publication (answering the calibrationReferences) but a different mathematical Model may be applied in another Publication (answering the modelReferences)</vaem:rationale>
        <rdfs:comment xml:lang="en">Answers the question: In which Publication is the model described/applied?</rdfs:comment>
        <rdfs:label xml:lang="en">model references</rdfs:label>
    </owl:ObjectProperty>
    


    <!-- http://linked.earth/ontology#modeledBy -->

    <owl:ObjectProperty rdf:about="http://linked.earth/ontology#modeledBy">
        <rdfs:domain>
            <owl:Class>
                <owl:unionOf rdf:parseType="Collection">
                    <rdf:Description rdf:about="http://linked.earth/ontology#Compilation"/>
                    <rdf:Description rdf:about="http://linked.earth/ontology#Data"/>
                    <rdf:Description rdf:about="http://linked.earth/ontology#ProxySystem"/>
                </owl:unionOf>
            </owl:Class>
        </rdfs:domain>
        <rdfs:range rdf:resource="http://linked.earth/ontology#Model"/>
        <vaem:rationale xml:lang="en">Links Data, Compilation or ProxySystem to Model</vaem:rationale>
        <rdfs:comment xml:lang="en">Answers the question: What is the Model for the Data, Compilation or ProxySystem under consideration?</rdfs:comment>
        <rdfs:label xml:lang="en">modeled by</rdfs:label>
    </owl:ObjectProperty>
    


    <!-- http://linked.earth/ontology#paleoModeledBy -->

    <owl:ObjectProperty rdf:about="http://linked.earth/ontology#paleoModeledBy">
        <rdfs:subPropertyOf rdf:resource="http://linked.earth/ontology#modeledBy"/>
        <rdfs:domain>
            <owl:Class>
                <owl:unionOf rdf:parseType="Collection">
                    <rdf:Description rdf:about="http://linked.earth/ontology#PaleoData"/>
                    <rdf:Description rdf:about="http://linked.earth/ontology#ProxySystem"/>
                </owl:unionOf>
            </owl:Class>
        </rdfs:domain>
        <rdfs:range rdf:resource="http://linked.earth/ontology#PaleoModel"/>
        <vaem:rationale xml:lang="en">Subclass of modeledBy, pertaining to paleoenvironmental information</vaem:rationale>
        <rdfs:comment xml:lang="en">Answers the question: What is the PaleoModel for the PaleoData or ProxySytem under consideration?</rdfs:comment>
        <rdfs:label xml:lang="en">paleo modeled by</rdfs:label>
    </owl:ObjectProperty>
    


    <!-- http://linked.earth/ontology#partOfCompilation -->

    <owl:ObjectProperty rdf:about="http://linked.earth/ontology#partOfCompilation">
        <rdfs:subPropertyOf rdf:resource="http://purl.org/dc/terms/isPartOf"/>
        <rdfs:subPropertyOf rdf:resource="http://schema.org/includedInDataCatalog"/>
        <rdfs:domain rdf:resource="http://linked.earth/ontology#Dataset"/>
        <rdfs:range rdf:resource="http://linked.earth/ontology#Compilation"/>
        <vaem:rationale xml:lang="en">Links the dataset to the compilation</vaem:rationale>
        <rdfs:comment xml:lang="en">Answer the question: Which compilation does a dataset belong to?</rdfs:comment>
        <rdfs:label xml:lang="en">part of compilation</rdfs:label>
    </owl:ObjectProperty>
    


    <!-- http://linked.earth/ontology#principalInvestigator -->

    <owl:ObjectProperty rdf:about="http://linked.earth/ontology#principalInvestigator">
        <rdfs:domain rdf:resource="http://linked.earth/ontology#Funding"/>
        <rdfs:range rdf:resource="http://linked.earth/ontology#Person"/>
        <vann:example rdf:resource="http://wiki.linked.earth/MD982181.Khider.2014.Funding1"/>
        <vaem:rationale xml:lang="en">Links the source of Funding to the PI (a Person)</vaem:rationale>
        <rdfs:comment xml:lang="en">Answers the question: Who was the lead on the source of Funding for the Dataset?</rdfs:comment>
        <rdfs:label xml:lang="en">principal investigator</rdfs:label>
    </owl:ObjectProperty>
    


    <!-- http://linked.earth/ontology#proxyArchiveModel -->

    <owl:ObjectProperty rdf:about="http://linked.earth/ontology#proxyArchiveModel">
        <rdfs:domain rdf:resource="http://linked.earth/ontology#ProxySystemModel"/>
        <rdfs:range rdf:resource="http://linked.earth/ontology#ProxyArchiveModel"/>
        <vaem:rationale xml:lang="en">Links ProxySystemModel to ProxyArchiveModel</vaem:rationale>
        <rdfs:comment xml:lang="en">Answers the question: Which ProxyArchiveModel is used in the ProxySystemModel?</rdfs:comment>
        <rdfs:label xml:lang="en">proxy archive model</rdfs:label>
    </owl:ObjectProperty>
    


    <!-- http://linked.earth/ontology#proxyArchiveType -->

    <owl:ObjectProperty rdf:about="http://linked.earth/ontology#proxyArchiveType">
        <rdfs:domain rdf:resource="http://linked.earth/ontology#ProxySystem"/>
        <rdfs:range rdf:resource="http://linked.earth/ontology#ProxyArchive"/>
        <vann:example rdf:resource="http://wiki.linked.earth/MD982181.Khider.2014.paleo1measurement1.mgcarub.MarineSediment.Globigerinoides_ruber.Mg/Ca"/>
        <vaem:rationale xml:lang="en">Links ProxySystem to ProxyArchive</vaem:rationale>
        <rdfs:comment xml:lang="en">Answers the question: Which ProxyArchive underlies this ProxySystem?</rdfs:comment>
        <rdfs:label xml:lang="en">proxy archive type</rdfs:label>
    </owl:ObjectProperty>
    


    <!-- http://linked.earth/ontology#proxyObservationModel -->

    <owl:ObjectProperty rdf:about="http://linked.earth/ontology#proxyObservationModel">
        <rdfs:domain rdf:resource="http://linked.earth/ontology#ProxySystemModel"/>
        <rdfs:range rdf:resource="http://linked.earth/ontology#ProxyObservationModel"/>
        <vaem:rationale xml:lang="en">Links ProxySystemModel to ProxyObservationModel</vaem:rationale>
        <rdfs:comment xml:lang="en">Answers the question: Which ProxyObservationModel is used in the ProxySystemModel?</rdfs:comment>
        <rdfs:label xml:lang="en">proxy observation model</rdfs:label>
    </owl:ObjectProperty>
    


    <!-- http://linked.earth/ontology#proxyObservationType -->

    <owl:ObjectProperty rdf:about="http://linked.earth/ontology#proxyObservationType">
        <rdfs:domain>
            <owl:Class>
                <owl:unionOf rdf:parseType="Collection">
                    <rdf:Description rdf:about="http://linked.earth/ontology#MeasuredVariable"/>
                    <rdf:Description rdf:about="http://linked.earth/ontology#ProxySystem"/>
                </owl:unionOf>
            </owl:Class>
        </rdfs:domain>
        <rdfs:range rdf:resource="http://linked.earth/ontology#ProxyObservation"/>
        <vann:example rdf:resource="http://wiki.linked.earth/MD982181.Khider.2014.paleo1measurement1.mgcarub"/>
        <vann:example rdf:resource="http://wiki.linked.earth/MD982181.Khider.2014.paleo1measurement1.mgcarub.MarineSediment.Globigerinoides_ruber.Mg/Ca"/>
        <vaem:rationale xml:lang="en">The need to link a measured variable or a proxy system to the proxy observation type being measured.</vaem:rationale>
        <rdfs:comment xml:lang="en">Answers the question: What type of ProxyObservation does the MeasuredVariable or Proxy System belong to?
For example, the measured value of 5.63 mmol/mol is of type Mg/Ca, or the proxy observation of the current prpoxy system is Mg/Ca</rdfs:comment>
        <rdfs:label xml:lang="en">proxy observation type</rdfs:label>
    </owl:ObjectProperty>
    


    <!-- http://linked.earth/ontology#proxySensorModel -->

    <owl:ObjectProperty rdf:about="http://linked.earth/ontology#proxySensorModel">
        <rdfs:domain rdf:resource="http://linked.earth/ontology#ProxySystemModel"/>
        <rdfs:range rdf:resource="http://linked.earth/ontology#ProxySensorModel"/>
        <vaem:rationale xml:lang="en">Links ProxySystemModel to ProxySensorModel</vaem:rationale>
        <rdfs:comment xml:lang="en">Answers the question: Which ProxySensorModel is used in the ProxySystemModel?</rdfs:comment>
        <rdfs:label xml:lang="en">proxy sensor model</rdfs:label>
    </owl:ObjectProperty>
    


    <!-- http://linked.earth/ontology#proxySensorType -->

    <owl:ObjectProperty rdf:about="http://linked.earth/ontology#proxySensorType">
        <rdfs:domain rdf:resource="http://linked.earth/ontology#ProxySystem"/>
        <rdfs:range rdf:resource="http://linked.earth/ontology#ProxySensor"/>
        <vann:example rdf:resource="http://wiki.linked.earth/MD982181.Khider.2014.paleo1measurement1.mgcarub.MarineSediment.Globigerinoides_ruber.Mg/Ca"/>
        <vaem:rationale xml:lang="en">Links ProxySensor to ProxyArchive</vaem:rationale>
        <rdfs:comment xml:lang="en">Answers the question: Which ProxySensor underlies this ProxySystem?</rdfs:comment>
        <rdfs:label xml:lang="en">proxy sensor type</rdfs:label>
    </owl:ObjectProperty>
    


    <!-- http://linked.earth/ontology#publishedIn -->

    <owl:ObjectProperty rdf:about="http://linked.earth/ontology#publishedIn">
        <rdfs:domain rdf:resource="http://linked.earth/ontology#Dataset"/>
        <rdfs:range rdf:resource="http://linked.earth/ontology#Publication"/>
        <vann:example rdf:resource="http://wiki.linked.earth/MD982181.Khider.2014"/>
        <vaem:rationale xml:lang="en">Links the resource to its Publication</vaem:rationale>
        <rdfs:comment xml:lang="en">Answers the question: In which Publication was the Dataset or Compilation issued?</rdfs:comment>
        <rdfs:label xml:lang="en">published in</rdfs:label>
    </owl:ObjectProperty>
    


    <!-- http://linked.earth/ontology#reportedIn -->

    <owl:ObjectProperty rdf:about="http://linked.earth/ontology#reportedIn">
        <rdfs:domain rdf:resource="http://linked.earth/ontology#Uncertainty"/>
        <rdfs:range>
            <owl:Class>
                <owl:unionOf rdf:parseType="Collection">
                    <rdf:Description rdf:about="http://linked.earth/ontology#DataTable"/>
                    <rdf:Description rdf:about="http://linked.earth/ontology#Variable"/>
                </owl:unionOf>
            </owl:Class>
        </rdfs:range>
        <vann:example rdf:resource="http://wiki.linked.earth/MD982181.Khider.2014.paleo1measurement2.sst.Uncertainty"/>
        <vaem:rationale xml:lang="en">Links the uncertainty to the model output</vaem:rationale>
        <rdfs:comment xml:lang="en">Answers the question: In which EnsembleTable, DistributionTable, and/or SummaryTable is the Uncertainty reported?</rdfs:comment>
        <rdfs:label xml:lang="en">reported in</rdfs:label>
    </owl:ObjectProperty>
    


    <!-- http://linked.earth/ontology#summaryTableGeneratedByModel -->

    <owl:ObjectProperty rdf:about="http://linked.earth/ontology#summaryTableGeneratedByModel">
        <rdfs:subPropertyOf rdf:resource="http://linked.earth/ontology#generatedByModel"/>
        <rdf:type rdf:resource="http://www.w3.org/2002/07/owl#FunctionalProperty"/>
        <rdfs:domain rdf:resource="http://linked.earth/ontology#SummaryTable"/>
        <rdfs:range>
            <owl:Class>
                <owl:unionOf rdf:parseType="Collection">
                    <rdf:Description rdf:about="http://linked.earth/ontology#ChronModel"/>
                    <rdf:Description rdf:about="http://linked.earth/ontology#PaleoModel"/>
                </owl:unionOf>
            </owl:Class>
        </rdfs:range>
        <vann:example rdf:resource="http://wiki.linked.earth/MD982181.Khider.2014.PaleoData1.Model1"/>
        <vaem:rationale xml:lang="en">Subproperty of foundinTable to link the Model to its outputs</vaem:rationale>
        <rdfs:comment xml:lang="en">Answers the question: In which SummaryTable can the statistics on the Model Output be found?</rdfs:comment>
        <rdfs:label xml:lang="en">summary table generated by model</rdfs:label>
    </owl:ObjectProperty>
    


    <!-- http://linked.earth/ontology#takenAtDepth -->

    <owl:ObjectProperty rdf:about="http://linked.earth/ontology#takenAtDepth">
        <rdfs:domain rdf:resource="http://linked.earth/ontology#Variable"/>
        <rdfs:range rdf:resource="http://linked.earth/ontology#Variable"/>
        <vann:example rdf:resource="http://wiki.linked.earth/MD982181.Khider.2014.paleo1measurement2.mgcarub"/>
        <vaem:rationale xml:lang="en">Provides depth information. Can link to the depth Variable in the DataTable</vaem:rationale>
        <rdfs:comment xml:lang="en">Answers the question: At which depth in the ProxyArchive is the Variable measured or inferred?</rdfs:comment>
        <rdfs:label xml:lang="en">taken at depth</rdfs:label>
    </owl:ObjectProperty>
    


    <!-- http://purl.oclc.org/NET/ssnx/ssn#observedBy -->

    <owl:ObjectProperty rdf:about="http://purl.oclc.org/NET/ssnx/ssn#observedBy">
        <rdfs:isDefinedBy rdf:resource="http://purl.oclc.org/NET/ssnx/ssn#"/>
    </owl:ObjectProperty>
    


    <!-- http://purl.org/dc/terms/contributor -->

    <owl:ObjectProperty rdf:about="http://purl.org/dc/terms/contributor">
        <rdfs:isDefinedBy rdf:resource="http://purl.org/dc/terms/"/>
    </owl:ObjectProperty>
    


    <!-- http://purl.org/dc/terms/creator -->

    <owl:ObjectProperty rdf:about="http://purl.org/dc/terms/creator">
        <rdfs:isDefinedBy rdf:resource="http://purl.org/dc/terms/"/>
    </owl:ObjectProperty>
    


    <!-- http://purl.org/dc/terms/isPartOf -->

    <owl:ObjectProperty rdf:about="http://purl.org/dc/terms/isPartOf">
        <rdfs:isDefinedBy rdf:resource="http://purl.org/dc/terms/"/>
    </owl:ObjectProperty>
    


    <!-- http://purl.org/dc/terms/references -->

    <owl:ObjectProperty rdf:about="http://purl.org/dc/terms/references">
        <rdfs:isDefinedBy rdf:resource="http://purl.org/dc/terms/"/>
    </owl:ObjectProperty>
    


    <!-- http://schema.org/author -->

    <owl:ObjectProperty rdf:about="http://schema.org/author">
        <rdfs:isDefinedBy rdf:resource="http://schema.org/author"/>
    </owl:ObjectProperty>
    


    <!-- http://schema.org/contentLocation -->

    <owl:ObjectProperty rdf:about="http://schema.org/contentLocation">
        <rdfs:isDefinedBy rdf:resource="http://schema.org/"/>
    </owl:ObjectProperty>
    


    <!-- http://schema.org/contributor -->

    <owl:ObjectProperty rdf:about="http://schema.org/contributor">
        <rdfs:isDefinedBy rdf:resource="http://schema.org/"/>
    </owl:ObjectProperty>
    


    <!-- http://schema.org/funder -->

    <owl:ObjectProperty rdf:about="http://schema.org/funder">
        <rdfs:isDefinedBy rdf:resource="http://schema.org/"/>
    </owl:ObjectProperty>
    


    <!-- http://schema.org/includedInDataCatalog -->

    <owl:ObjectProperty rdf:about="http://schema.org/includedInDataCatalog">
        <rdfs:isDefinedBy rdf:resource="http://schema.org/"/>
    </owl:ObjectProperty>
    


    <!-- http://www.opengis.net/ont/geosparql#hasGeometry -->

    <owl:ObjectProperty rdf:about="http://www.opengis.net/ont/geosparql#hasGeometry">
        <rdfs:domain rdf:resource="http://www.opengis.net/ont/geosparql#Feature"/>
        <rdfs:range rdf:resource="http://www.opengis.net/ont/geosparql#Geometry"/>
        <rdfs:isDefinedBy rdf:resource="http://www.opengis.net/spec/geosparql/1.0"/>
    </owl:ObjectProperty>
    


    <!-- http://www.w3.org/ns/prov#wasDerivedFrom -->

    <owl:ObjectProperty rdf:about="http://www.w3.org/ns/prov#wasDerivedFrom">
        <rdfs:isDefinedBy rdf:resource="http://www.w3.org/ns/prov#"/>
    </owl:ObjectProperty>
    


    <!-- 
    ///////////////////////////////////////////////////////////////////////////////////////
    //
    // Data properties
    //
    ///////////////////////////////////////////////////////////////////////////////////////
     -->

    


    <!-- http://linked.earth/ontology#book -->

    <owl:DatatypeProperty rdf:about="http://linked.earth/ontology#book">
        <rdfs:domain rdf:resource="http://linked.earth/ontology#Publication"/>
        <rdfs:range rdf:resource="http://www.w3.org/2001/XMLSchema#string"/>
        <vaem:rationale xml:lang="en">Separate between journal and book publication</vaem:rationale>
        <rdfs:comment xml:lang="en">Answers the question: In which book was the resource published?</rdfs:comment>
        <rdfs:label xml:lang="en">book</rdfs:label>
    </owl:DatatypeProperty>
    


    <!-- http://linked.earth/ontology#compilationCitation -->

    <owl:DatatypeProperty rdf:about="http://linked.earth/ontology#compilationCitation">
        <rdfs:subPropertyOf rdf:resource="http://purl.org/dc/terms/bibliographicCitation"/>
        <rdfs:subPropertyOf rdf:resource="http://schema.org/citation"/>
        <rdfs:domain rdf:resource="http://linked.earth/ontology#Compilation"/>
        <rdfs:range rdf:resource="http://www.w3.org/2001/XMLSchema#string"/>
        <vaem:rationale xml:lang="en">Data property needed to specify how to cite compilations, in order to provide appropriate credit to all contributors</vaem:rationale>
        <rdfs:comment xml:lang="en">Answers the question: How should someone cite the compilation?</rdfs:comment>
        <rdfs:label xml:lang="en">compilation citation</rdfs:label>
    </owl:DatatypeProperty>
    


    <!-- http://linked.earth/ontology#compilationDate -->

    <owl:DatatypeProperty rdf:about="http://linked.earth/ontology#compilationDate">
        <rdfs:subPropertyOf rdf:resource="http://purl.org/dc/terms/created"/>
        <rdfs:subPropertyOf rdf:resource="http://schema.org/dateCreated"/>
        <rdfs:domain rdf:resource="http://linked.earth/ontology#Compilation"/>
        <rdfs:range rdf:resource="http://www.w3.org/2001/XMLSchema#dateTime"/>
        <vaem:rationale xml:lang="en">Separate compilation date from the publication year. An example is LR04 (datsetdate in 2004) but published in 2005</vaem:rationale>
        <rdfs:comment xml:lang="en">Answers the question: At what date was the Compilation created?</rdfs:comment>
        <rdfs:label xml:lang="en">compilation date</rdfs:label>
    </owl:DatatypeProperty>
    


    <!-- http://linked.earth/ontology#compilationVersion -->

    <owl:DatatypeProperty rdf:about="http://linked.earth/ontology#compilationVersion">
        <rdfs:subPropertyOf rdf:resource="http://schema.org/version"/>
        <rdfs:domain rdf:resource="http://linked.earth/ontology#Compilation"/>
        <rdfs:range rdf:resource="http://www.w3.org/2001/XMLSchema#string"/>
        <vaem:rationale xml:lang="en">Needed to state the version associated to a compilation, which may not be the same as the datasets it contains</vaem:rationale>
        <rdfs:comment xml:lang="en">Answers the question: What is the version of the Compilation?</rdfs:comment>
        <rdfs:label xml:lang="en">compilation version</rdfs:label>
    </owl:DatatypeProperty>
    


    <!-- http://linked.earth/ontology#datasetCitation -->

    <owl:DatatypeProperty rdf:about="http://linked.earth/ontology#datasetCitation">
        <rdfs:subPropertyOf rdf:resource="http://purl.org/dc/terms/bibliographicCitation"/>
        <rdfs:subPropertyOf rdf:resource="http://schema.org/citation"/>
        <rdfs:domain rdf:resource="http://linked.earth/ontology#Dataset"/>
        <rdfs:range rdf:resource="http://www.w3.org/2000/01/rdf-schema#Literal"/>
        <vaem:rationale xml:lang="en">The need for providing appropriate credit to the datasets</vaem:rationale>
        <rdfs:comment xml:lang="en">Sentence indicating how a dataset should be cited</rdfs:comment>
        <rdfs:label xml:lang="en">dataset citation</rdfs:label>
    </owl:DatatypeProperty>
    


    <!-- http://linked.earth/ontology#datasetDate -->

    <owl:DatatypeProperty rdf:about="http://linked.earth/ontology#datasetDate">
        <rdfs:subPropertyOf rdf:resource="http://purl.org/dc/terms/created"/>
        <rdfs:subPropertyOf rdf:resource="http://schema.org/dateCreated"/>
        <rdf:type rdf:resource="http://www.w3.org/2002/07/owl#FunctionalProperty"/>
        <rdfs:domain rdf:resource="http://linked.earth/ontology#Dataset"/>
        <rdfs:range rdf:resource="http://www.w3.org/2001/XMLSchema#dateTime"/>
        <vann:example xml:lang="en">http://wiki.linked.earth/MD982181.Khider.2014</vann:example>
        <vaem:rationale xml:lang="en">Separate dataset date from the publication year. An example is LR04 (datsetdate in 2004) but published in 2005</vaem:rationale>
        <rdfs:comment xml:lang="en">Answers the question: At what date was the Dataset created?</rdfs:comment>
        <rdfs:label xml:lang="en">dataset date</rdfs:label>
    </owl:DatatypeProperty>
    


    <!-- http://linked.earth/ontology#datasetLicense -->

    <owl:DatatypeProperty rdf:about="http://linked.earth/ontology#datasetLicense">
        <rdfs:subPropertyOf rdf:resource="http://purl.org/dc/terms/license"/>
        <rdfs:subPropertyOf rdf:resource="http://schema.org/license"/>
        <rdfs:domain rdf:resource="http://linked.earth/ontology#Dataset"/>
        <rdfs:range rdf:resource="http://www.w3.org/2001/XMLSchema#anyURI"/>
        <vaem:rationale xml:lang="en">Property needed to let other scientists know about the usage and attribution terms of the uploaded dataset</vaem:rationale>
        <rdfs:comment xml:lang="en">License associated to a dataset</rdfs:comment>
        <rdfs:label xml:lang="en">dataset license</rdfs:label>
    </owl:DatatypeProperty>
    


    <!-- http://linked.earth/ontology#datasetVersion -->

    <owl:DatatypeProperty rdf:about="http://linked.earth/ontology#datasetVersion">
        <rdfs:subPropertyOf rdf:resource="http://schema.org/version"/>
        <rdf:type rdf:resource="http://www.w3.org/2002/07/owl#FunctionalProperty"/>
        <rdfs:domain rdf:resource="http://linked.earth/ontology#Dataset"/>
        <rdfs:range rdf:resource="http://www.w3.org/2001/XMLSchema#string"/>
        <vann:example rdf:resource="http://wiki.linked.earth/MD982181.Khider.2014"/>
        <vaem:rationale xml:lang="en">Allows to update a dataset if Data/Models are added and keep track of the various versions</vaem:rationale>
        <rdfs:comment xml:lang="en">Answers the question: What is the version of the Dataset?

It should follow the x.y.z notation where x refers to changes in metadata and data following a publication (for instance, the creation of a new age model using a different code), y refers to changes to the data following a publication (for instance, adding data further back in time without changing the model underlying the interpretation), and z refers to changes not associated with a publication (for instance, typos).</rdfs:comment>
        <rdfs:label xml:lang="en">dataset version</rdfs:label>
    </owl:DatatypeProperty>
    


    <!-- http://linked.earth/ontology#description -->

    <owl:DatatypeProperty rdf:about="http://linked.earth/ontology#description">
        <rdfs:domain rdf:resource="http://www.w3.org/2002/07/owl#Thing"/>
        <rdfs:range rdf:resource="http://www.w3.org/2001/XMLSchema#string"/>
        <vann:example rdf:resource="http://wiki.linked.earth/MD982181.Khider.2014.paleo1measurement1.mgcarub"/>
        <vaem:rationale xml:lang="en">This property may be used to provide further details on instrument descriptions, uncertainty description,etc.</vaem:rationale>
        <rdfs:comment xml:lang="en">Answers the question: What additional details would you give about the resource?</rdfs:comment>
        <rdfs:label xml:lang="en">description</rdfs:label>
    </owl:DatatypeProperty>
    


    <!-- http://linked.earth/ontology#detail -->

    <owl:DatatypeProperty rdf:about="http://linked.earth/ontology#detail">
        <rdfs:domain rdf:resource="http://linked.earth/ontology#Interpretation"/>
        <rdfs:range rdf:resource="http://www.w3.org/2001/XMLSchema#string"/>
        <vann:example rdf:resource="http://wiki.linked.earth/MD982181.Khider.2014.paleo1measurement1.mgcarub.Interpretation"/>
        <rdfs:comment xml:lang="en">Answers the  &quot;of what&quot; question for an Interpretation. For intance, sea surface in sea surface temperature.</rdfs:comment>
        <rdfs:label xml:lang="en">detail</rdfs:label>
    </owl:DatatypeProperty>
    


    <!-- http://linked.earth/ontology#email -->

    <owl:DatatypeProperty rdf:about="http://linked.earth/ontology#email">
        <rdfs:domain rdf:resource="http://linked.earth/ontology#Person"/>
        <rdfs:range rdf:resource="http://www.w3.org/2001/XMLSchema#string"/>
        <vann:example rdf:resource="http://wiki.linked.earth/D._Khider"/>
        <vaem:rationale xml:lang="en">Allow to store contact information</vaem:rationale>
        <rdfs:comment xml:lang="en">Answers the question: What is the email address of the Person?</rdfs:comment>
        <rdfs:label xml:lang="en">email</rdfs:label>
    </owl:DatatypeProperty>
    


    <!-- http://linked.earth/ontology#equation -->

    <owl:DatatypeProperty rdf:about="http://linked.earth/ontology#equation">
        <rdfs:domain rdf:resource="http://linked.earth/ontology#Model"/>
        <rdfs:range rdf:resource="http://www.w3.org/2001/XMLSchema#string"/>
        <vann:example rdf:resource="http://wiki.linked.earth/MD982176.Stott.2004.paleo1measurement1.Mg/Ca-g.rub.Calibration"/>
        <vaem:rationale xml:lang="en">Allows to provide the equation as part of the metadata</vaem:rationale>
        <rdfs:comment xml:lang="en">Answers the question: What is the mathematical formulation of the Model?</rdfs:comment>
        <rdfs:label xml:lang="en">equation</rdfs:label>
    </owl:DatatypeProperty>
    


    <!-- http://linked.earth/ontology#fundingAgency -->

    <owl:DatatypeProperty rdf:about="http://linked.earth/ontology#fundingAgency">
        <rdf:type rdf:resource="http://www.w3.org/2002/07/owl#FunctionalProperty"/>
        <rdfs:domain rdf:resource="http://linked.earth/ontology#Funding"/>
        <rdfs:range rdf:resource="http://www.w3.org/2001/XMLSchema#string"/>
        <vann:example rdf:resource="http://wiki.linked.earth/MD982181.Khider.2014.Funding1"/>
        <vaem:rationale xml:lang="en">Provides information about the Agency funding the study</vaem:rationale>
        <rdfs:comment xml:lang="en">Answers the question: Which entity was the Dataset fundedBy?</rdfs:comment>
        <rdfs:label xml:lang="en">funding agency</rdfs:label>
    </owl:DatatypeProperty>
    


    <!-- http://linked.earth/ontology#fundingCountry -->

    <owl:DatatypeProperty rdf:about="http://linked.earth/ontology#fundingCountry">
        <rdf:type rdf:resource="http://www.w3.org/2002/07/owl#FunctionalProperty"/>
        <rdfs:domain rdf:resource="http://linked.earth/ontology#Funding"/>
        <rdfs:range rdf:resource="http://www.w3.org/2001/XMLSchema#string"/>
        <vaem:rationale rdf:resource="http://wiki.linked.earth/MD982181.Khider.2014.Funding1"/>
        <vaem:rationale xml:lang="en">Provides information about the country the agency is from</vaem:rationale>
        <rdfs:comment xml:lang="en">Answers the question: Which nation funded the Dataset?</rdfs:comment>
        <rdfs:label xml:lang="en">funding country</rdfs:label>
    </owl:DatatypeProperty>
    


    <!-- http://linked.earth/ontology#grantNumber -->

    <owl:DatatypeProperty rdf:about="http://linked.earth/ontology#grantNumber">
        <rdfs:domain rdf:resource="http://linked.earth/ontology#Funding"/>
        <rdfs:range rdf:resource="http://www.w3.org/2001/XMLSchema#string"/>
        <vann:example rdf:resource="http://wiki.linked.earth/MD982181.Khider.2014.Funding1"/>
        <vaem:rationale xml:lang="en">Provides information about the grant number</vaem:rationale>
        <rdfs:comment xml:lang="en">Answers the question: What is the unique identifier associated with the Funding for the Dataset?</rdfs:comment>
        <rdfs:label xml:lang="en">grant number</rdfs:label>
    </owl:DatatypeProperty>
    


    <!-- http://linked.earth/ontology#hasColumnNumber -->

    <owl:DatatypeProperty rdf:about="http://linked.earth/ontology#hasColumnNumber">
        <rdfs:domain rdf:resource="http://linked.earth/ontology#Variable"/>
        <rdfs:range rdf:resource="http://www.w3.org/2001/XMLSchema#integer"/>
        <vann:example rdf:resource="http://wiki.linked.earth/MD982181.Khider.2014.paleo1measurement1.mgcarub"/>
        <vaem:rationale xml:lang="en">Links the Variable metadata to the values stored in the csv file</vaem:rationale>
        <rdfs:comment xml:lang="en">Answers the question: In which column of the csv file can the Variable be found?</rdfs:comment>
        <rdfs:label xml:lang="en">has column number</rdfs:label>
    </owl:DatatypeProperty>
    


    <!-- http://linked.earth/ontology#hasDOI -->

    <owl:DatatypeProperty rdf:about="http://linked.earth/ontology#hasDOI">
        <rdfs:subPropertyOf rdf:resource="http://purl.org/dc/terms/identifier"/>
        <rdf:type rdf:resource="http://www.w3.org/2002/07/owl#FunctionalProperty"/>
        <rdfs:domain>
            <owl:Class>
                <owl:unionOf rdf:parseType="Collection">
                    <rdf:Description rdf:about="http://linked.earth/ontology#Dataset"/>
                    <rdf:Description rdf:about="http://linked.earth/ontology#Publication"/>
                    <rdf:Description rdf:about="http://linked.earth/ontology#SoftwareCode"/>
                </owl:unionOf>
            </owl:Class>
        </rdfs:domain>
        <rdfs:range rdf:resource="http://www.w3.org/2001/XMLSchema#string"/>
        <vann:example rdf:resource="http://wiki.linked.earth/Publication.10.1002/2013PA002534"/>
        <vaem:rationale xml:lang="en">Allows to link to a resource using a digital object identifier</vaem:rationale>
        <rdfs:comment xml:lang="en">Answers the question: What is the digital object identifier associated with the resource?</rdfs:comment>
        <rdfs:label xml:lang="en">has DOI</rdfs:label>
    </owl:DatatypeProperty>
    


    <!-- http://linked.earth/ontology#hasExecutionCommand -->

    <owl:DatatypeProperty rdf:about="http://linked.earth/ontology#hasExecutionCommand">
        <rdfs:domain rdf:resource="http://linked.earth/ontology#SoftwareCode"/>
        <rdfs:range rdf:resource="http://www.w3.org/2001/XMLSchema#string"/>
        <vaem:rationale xml:lang="en">Allows to store the execution command of a script</vaem:rationale>
        <rdfs:comment xml:lang="en">Answers the question: What is the command to run the script or the code?</rdfs:comment>
        <rdfs:label xml:lang="en">has execution command</rdfs:label>
    </owl:DatatypeProperty>
    


    <!-- http://linked.earth/ontology#hasExecutionEnvironment -->

    <owl:DatatypeProperty rdf:about="http://linked.earth/ontology#hasExecutionEnvironment">
        <rdfs:domain rdf:resource="http://linked.earth/ontology#SoftwareCode"/>
        <rdfs:range rdf:resource="http://www.w3.org/2001/XMLSchema#string"/>
        <vaem:rationale xml:lang="en">Provides information about the operating system version in which the software code was exceuted?</vaem:rationale>
        <rdfs:comment xml:lang="en">Answers the question: In which environment is the script meant to be run in?</rdfs:comment>
        <rdfs:label xml:lang="en">has execution environment</rdfs:label>
    </owl:DatatypeProperty>
    


    <!-- http://linked.earth/ontology#hasFileName -->

    <owl:DatatypeProperty rdf:about="http://linked.earth/ontology#hasFileName">
        <rdf:type rdf:resource="http://www.w3.org/2002/07/owl#FunctionalProperty"/>
        <rdfs:domain rdf:resource="http://linked.earth/ontology#DataTable"/>
        <rdfs:range rdf:resource="http://www.w3.org/2001/XMLSchema#string"/>
        <vann:example rdf:resource="http://wiki.linked.earth/MD982181.Khider.2014.paleo1measurement2"/>
        <vaem:rationale xml:lang="en">Links a DataTable with its appropriate csv file</vaem:rationale>
        <rdfs:comment xml:lang="en">Answers the question: What is the name of the csv file in which the Variable values are stored?</rdfs:comment>
        <rdfs:label xml:lang="en">has file name</rdfs:label>
    </owl:DatatypeProperty>
    


    <!-- http://linked.earth/ontology#hasIGSN -->

    <owl:DatatypeProperty rdf:about="http://linked.earth/ontology#hasIGSN">
        <rdfs:subPropertyOf rdf:resource="http://purl.org/dc/terms/identifier"/>
        <rdfs:domain rdf:resource="http://linked.earth/ontology#PhysicalSample"/>
        <rdfs:range rdf:resource="http://www.w3.org/2001/XMLSchema#string"/>
        <vaem:rationale xml:lang="en">Needed to properly described physical samples</vaem:rationale>
        <rdfs:comment xml:lang="en">IGSN identifier associated to a physical sample</rdfs:comment>
        <rdfs:label xml:lang="en">has IGSN</rdfs:label>
    </owl:DatatypeProperty>
    


    <!-- http://linked.earth/ontology#hasISBN -->

    <owl:DatatypeProperty rdf:about="http://linked.earth/ontology#hasISBN">
        <rdfs:subPropertyOf rdf:resource="http://purl.org/dc/terms/identifier"/>
        <rdfs:domain rdf:resource="http://linked.earth/ontology#Publication"/>
        <rdfs:range rdf:resource="http://www.w3.org/2001/XMLSchema#string"/>
        <vaem:rationale xml:lang="en">Link to the ISBN: Identifier used commonly to refer to publications</vaem:rationale>
        <rdfs:comment xml:lang="en">Answers the question: What is the international book number of the Publication?</rdfs:comment>
        <rdfs:label xml:lang="en">has ISBN</rdfs:label>
    </owl:DatatypeProperty>
    


    <!-- http://linked.earth/ontology#hasISSN -->

    <owl:DatatypeProperty rdf:about="http://linked.earth/ontology#hasISSN">
        <rdfs:subPropertyOf rdf:resource="http://purl.org/dc/terms/identifier"/>
        <rdfs:domain rdf:resource="http://linked.earth/ontology#Publication"/>
        <rdfs:range rdf:resource="http://www.w3.org/2001/XMLSchema#string"/>
        <vaem:rationale xml:lang="en">8-digit code used to identify publications</vaem:rationale>
        <rdfs:comment xml:lang="en">Answers the question: What is the International Standard Serial Number of the Publication?</rdfs:comment>
        <rdfs:label xml:lang="en">has ISSN</rdfs:label>
    </owl:DatatypeProperty>
    


    <!-- http://linked.earth/ontology#hasLink -->

    <owl:DatatypeProperty rdf:about="http://linked.earth/ontology#hasLink">
        <rdfs:domain rdf:resource="http://www.w3.org/2002/07/owl#Thing"/>
        <rdfs:range rdf:resource="http://www.w3.org/2001/XMLSchema#anyURI"/>
        <vann:example rdf:resource="http://wiki.linked.earth/Publication.10.1002/2013PA002534"/>
        <vaem:rationale xml:lang="en">Allows to point to the original source of a resource</vaem:rationale>
        <rdfs:comment xml:lang="en">Answers the question: What is the universal resource locator to a resource?</rdfs:comment>
        <rdfs:label xml:lang="en">has link</rdfs:label>
    </owl:DatatypeProperty>
    


    <!-- http://linked.earth/ontology#hasMaxValue -->

    <owl:DatatypeProperty rdf:about="http://linked.earth/ontology#hasMaxValue">
        <rdfs:domain rdf:resource="http://linked.earth/ontology#Variable"/>
        <rdfs:range rdf:resource="http://www.w3.org/2001/XMLSchema#float"/>
        <vann:example rdf:resource="http://wiki.linked.earth/MD982181.Khider.2014.paleo1measurement2.sst"/>
        <vaem:rationale xml:lang="en">property relevant to facilitate queries, as in most cases the contents of a csv file are not directly represented</vaem:rationale>
        <rdfs:comment xml:lang="en">Answers the question: What is the maximum value of the Variable?</rdfs:comment>
        <rdfs:label xml:lang="en">has max value</rdfs:label>
    </owl:DatatypeProperty>
    


    <!-- http://linked.earth/ontology#hasMeanValue -->

    <owl:DatatypeProperty rdf:about="http://linked.earth/ontology#hasMeanValue">
        <rdfs:domain rdf:resource="http://linked.earth/ontology#Variable"/>
        <rdfs:range rdf:resource="http://www.w3.org/2001/XMLSchema#float"/>
        <vann:example rdf:resource="http://wiki.linked.earth/MD982181.Khider.2014.paleo1measurement2.sst"/>
        <vaem:rationale xml:lang="en">property relevant to facilitate queries, as in most cases the contents of a csv file are not directly represented</vaem:rationale>
        <rdfs:comment xml:lang="en">Answers the question: What is the mean value of the Variable?</rdfs:comment>
        <rdfs:label xml:lang="en">has mean value</rdfs:label>
    </owl:DatatypeProperty>
    


    <!-- http://linked.earth/ontology#hasMedianValue -->

    <owl:DatatypeProperty rdf:about="http://linked.earth/ontology#hasMedianValue">
        <rdfs:domain rdf:resource="http://linked.earth/ontology#Variable"/>
        <rdfs:range rdf:resource="http://www.w3.org/2001/XMLSchema#float"/>
        <vann:example rdf:resource="http://wiki.linked.earth/MD982181.Khider.2014.paleo1measurement1.mgcarub.ICPAES"/>
        <vaem:rationale xml:lang="en">property relevant to facilitate queries, as in most cases the contents of a csv file are not directly represented</vaem:rationale>
        <rdfs:comment xml:lang="en">Answers the question: What is the median value of the Variable?</rdfs:comment>
        <rdfs:label xml:lang="en">has median value</rdfs:label>
    </owl:DatatypeProperty>
    


    <!-- http://linked.earth/ontology#hasMinValue -->

    <owl:DatatypeProperty rdf:about="http://linked.earth/ontology#hasMinValue">
        <rdfs:domain rdf:resource="http://linked.earth/ontology#Variable"/>
        <rdfs:range rdf:resource="http://www.w3.org/2001/XMLSchema#float"/>
        <vann:example rdf:resource="http://wiki.linked.earth/MD982181.Khider.2014.paleo1measurement2.sst"/>
        <vaem:rationale xml:lang="en">property relevant to facilitate queries, as in most cases the contents of a csv file are not directly represented</vaem:rationale>
        <rdfs:comment xml:lang="en">Answers the question: What is the minimum value of the Variable?</rdfs:comment>
        <rdfs:label xml:lang="en">has min value</rdfs:label>
    </owl:DatatypeProperty>
    


    <!-- http://linked.earth/ontology#hasMissingValue -->

    <owl:DatatypeProperty rdf:about="http://linked.earth/ontology#hasMissingValue">
        <rdf:type rdf:resource="http://www.w3.org/2002/07/owl#FunctionalProperty"/>
        <rdfs:domain>
            <owl:Class>
                <owl:unionOf rdf:parseType="Collection">
                    <rdf:Description rdf:about="http://linked.earth/ontology#Uncertainty"/>
                    <rdf:Description rdf:about="http://linked.earth/ontology#Variable"/>
                </owl:unionOf>
            </owl:Class>
        </rdfs:domain>
        <rdfs:range rdf:resource="http://www.w3.org/2001/XMLSchema#string"/>
        <owl:propertyDisjointWith rdf:resource="http://linked.earth/ontology#hasValue"/>
        <vann:example rdf:resource="http://wiki.linked.earth/MD982181.Khider.2014.paleo1measurement1.mgcarub"/>
        <vaem:rationale xml:lang="en">Useful for coding around the missing values</vaem:rationale>
        <rdfs:comment xml:lang="en">Answers the question: How are the missing values of the Variable identified in the DataTable?</rdfs:comment>
        <rdfs:label xml:lang="en">has missing value</rdfs:label>
    </owl:DatatypeProperty>
    


    <!-- http://linked.earth/ontology#hasRank -->

    <owl:DatatypeProperty rdf:about="http://linked.earth/ontology#hasRank">
        <rdf:type rdf:resource="http://www.w3.org/2002/07/owl#FunctionalProperty"/>
        <rdfs:domain rdf:resource="http://linked.earth/ontology#Interpretation"/>
        <rdfs:range rdf:resource="http://www.w3.org/2001/XMLSchema#int"/>
        <vann:example rdf:resource="http://wiki.linked.earth/MD982181.Khider.2014.paleo1measurement1.d18orub.Interpretation1"/>
        <vaem:rationale xml:lang="en">Allows to rank the environmental variable controlling the interpretation. For instance, the d18O of coral aragonite responds to both temperature and the d18O of seawater (closely linked to salinity). Depending on the locale and/or timescale, one variable may dominate over the other.</vaem:rationale>
        <rdfs:comment xml:lang="en">Answers the question: What is the importance of the Interpretation?</rdfs:comment>
        <rdfs:label xml:lang="en">has rank</rdfs:label>
    </owl:DatatypeProperty>
    


    <!-- http://linked.earth/ontology#hasUnits -->

    <owl:DatatypeProperty rdf:about="http://linked.earth/ontology#hasUnits">
        <rdf:type rdf:resource="http://www.w3.org/2002/07/owl#FunctionalProperty"/>
        <rdfs:domain>
            <owl:Class>
                <owl:unionOf rdf:parseType="Collection">
                    <rdf:Description rdf:about="http://linked.earth/ontology#MeasuredVariable"/>
                    <rdf:Description rdf:about="http://linked.earth/ontology#Resolution"/>
                    <rdf:Description rdf:about="http://linked.earth/ontology#Uncertainty"/>
                    <rdf:Description rdf:about="http://linked.earth/ontology#Variable"/>
                </owl:unionOf>
            </owl:Class>
        </rdfs:domain>
        <rdfs:range rdf:resource="http://www.w3.org/2001/XMLSchema#string"/>
        <vann:example rdf:resource="http://wiki.linked.earth/MD982181.Khider.2014.paleo1measurement1.d18orub"/>
        <vaem:rationale xml:lang="en">Links the units and the values of the Variable</vaem:rationale>
        <rdfs:comment xml:lang="en">Answers the question: In what unit of measure is (are) the Variable(s) expressed?</rdfs:comment>
        <rdfs:label xml:lang="en">has units</rdfs:label>
    </owl:DatatypeProperty>
    


    <!-- http://linked.earth/ontology#hasValue -->

    <owl:DatatypeProperty rdf:about="http://linked.earth/ontology#hasValue">
        <rdfs:domain>
            <owl:Class>
                <owl:unionOf rdf:parseType="Collection">
                    <rdf:Description rdf:about="http://linked.earth/ontology#Model"/>
                    <rdf:Description rdf:about="http://linked.earth/ontology#Uncertainty"/>
                    <rdf:Description rdf:about="http://linked.earth/ontology#Variable"/>
                </owl:unionOf>
            </owl:Class>
        </rdfs:domain>
        <rdfs:range rdf:resource="http://www.w3.org/2001/XMLSchema#string"/>
        <vann:example rdf:resource="http://wiki.linked.earth/MD982181.Khider.2014.paleo1measurement1.d18orub.Uncertainty"/>
        <vaem:rationale xml:lang="en">Useful if there is only a single value rather than a vector of numbers. Often the case for analytical uncertainty or uncertainty reported as a RMSE</vaem:rationale>
        <rdfs:comment xml:lang="en">Answers the question: What are the numerical values of the Variable, Uncertainty, and Model outputs?</rdfs:comment>
        <rdfs:label xml:lang="en">has value</rdfs:label>
    </owl:DatatypeProperty>
    


    <!-- http://linked.earth/ontology#hasVariableID -->

    <owl:DatatypeProperty rdf:about="http://linked.earth/ontology#hasVariableID">
        <rdfs:subPropertyOf rdf:resource="http://purl.org/dc/terms/identifier"/>
        <rdfs:domain rdf:resource="http://linked.earth/ontology#Variable"/>
        <rdfs:range rdf:resource="http://www.w3.org/2001/XMLSchema#string"/>
        <vaem:rationale xml:lang="en">LiPD assigns a unique identifier (TSid) to each table column described in a LiPD file.

Allows to assign a unique identifier to each series, facilitating data citation and recognition

This allows someone to change every piece of metadata about column or dataset, including its names (both dataset and variable) and still get back to the right spot. Its fundamental to working with LiPD data.</vaem:rationale>
        <rdfs:comment xml:lang="en">Answers the question: What is the unique identifier for the Variable?</rdfs:comment>
        <rdfs:label xml:lang="en">has variable ID</rdfs:label>
    </owl:DatatypeProperty>
    


    <!-- http://linked.earth/ontology#housedAt -->

    <owl:DatatypeProperty rdf:about="http://linked.earth/ontology#housedAt">
        <rdfs:domain>
            <owl:Class>
                <owl:unionOf rdf:parseType="Collection">
                    <rdf:Description rdf:about="http://linked.earth/ontology#Instrument"/>
                    <rdf:Description rdf:about="http://linked.earth/ontology#PhysicalSample"/>
                </owl:unionOf>
            </owl:Class>
        </rdfs:domain>
        <rdfs:range rdf:resource="http://www.w3.org/2001/XMLSchema#string"/>
        <vann:example rdf:resource="http://wiki.linked.earth/MD982181.Khider.2014.paleo1measurement2.mgcarub"/>
        <vaem:rationale xml:lang="en">Link to a particular laboratory. Provides circumstantial information about the measurement technique and how it was applied. Allows to give some information about the actual location of the sample</vaem:rationale>
        <rdfs:comment xml:lang="en">Answers the question: In which laboratory/repository is the Instrument/PhysicalSample located?</rdfs:comment>
        <rdfs:label xml:lang="en">housed at</rdfs:label>
    </owl:DatatypeProperty>
    


    <!-- http://linked.earth/ontology#interpretationDirection -->

    <owl:DatatypeProperty rdf:about="http://linked.earth/ontology#interpretationDirection">
        <rdf:type rdf:resource="http://www.w3.org/2002/07/owl#FunctionalProperty"/>
        <rdfs:domain rdf:resource="http://linked.earth/ontology#Interpretation"/>
        <rdfs:range rdf:resource="http://www.w3.org/2001/XMLSchema#string"/>
        <vann:example rdf:resource="http://wiki.linked.earth/MD982181.Khider.2014.paleo1measurement1.d18orub.Interpretation1"/>
        <vaem:rationale xml:lang="en">Answer is only positive or negative. Useful metadata when the calibration equation is not readily available.
Also applies to InferredVariable to faciliate the search in database</vaem:rationale>
        <rdfs:comment xml:lang="en">Answers the question: Is the InferredVariable value increasing or decreasing as the value of the MeasuredVariable is increasing?</rdfs:comment>
        <rdfs:label xml:lang="en">interpretation direction</rdfs:label>
    </owl:DatatypeProperty>
    


    <!-- http://linked.earth/ontology#isLocal -->

    <owl:DatatypeProperty rdf:about="http://linked.earth/ontology#isLocal">
        <rdf:type rdf:resource="http://www.w3.org/2002/07/owl#FunctionalProperty"/>
        <rdfs:domain rdf:resource="http://linked.earth/ontology#Interpretation"/>
        <rdfs:range rdf:resource="http://www.w3.org/2001/XMLSchema#string"/>
        <vaem:rationale xml:lang="en">Added to allow data analysis. Is the interpretation relevant to these coordinates? Does putting a colored dot on the map here make sense?</vaem:rationale>
        <rdfs:comment>Answers the question: Does the Interpretation describe local variability, or far-field variability that may not reflect local conditions?</rdfs:comment>
        <rdfs:label xml:lang="en">is local</rdfs:label>
    </owl:DatatypeProperty>
    


    <!-- http://linked.earth/ontology#issue -->

    <owl:DatatypeProperty rdf:about="http://linked.earth/ontology#issue">
        <rdf:type rdf:resource="http://www.w3.org/2002/07/owl#FunctionalProperty"/>
        <rdfs:domain rdf:resource="http://linked.earth/ontology#Publication"/>
        <rdfs:range rdf:resource="http://www.w3.org/2001/XMLSchema#int"/>
        <vann:example rdf:resource="http://wiki.linked.earth/Publication.10.1002/2013PA002534"/>
        <vaem:rationale xml:lang="en">Part of standard metadata for Publications</vaem:rationale>
        <rdfs:comment xml:lang="en">Answers the question: In what issue of the journal can the resource be found?</rdfs:comment>
        <rdfs:label xml:lang="en">issue</rdfs:label>
    </owl:DatatypeProperty>
    


    <!-- http://linked.earth/ontology#journal -->

    <owl:DatatypeProperty rdf:about="http://linked.earth/ontology#journal">
        <rdfs:domain rdf:resource="http://linked.earth/ontology#Publication"/>
        <rdfs:range rdf:resource="http://www.w3.org/2001/XMLSchema#string"/>
        <vann:example rdf:resource="http://wiki.linked.earth/Publication.10.1002/2013PA002534"/>
        <vaem:rationale xml:lang="en">Part of standard metadata for Publications</vaem:rationale>
        <rdfs:comment xml:lang="en">Answers the question: What is the name of the journal in which the resource can be found?</rdfs:comment>
        <rdfs:label xml:lang="en">journal</rdfs:label>
    </owl:DatatypeProperty>
    


    <!-- http://linked.earth/ontology#method -->

    <owl:DatatypeProperty rdf:about="http://linked.earth/ontology#method">
        <rdfs:domain>
            <owl:Class>
                <owl:unionOf rdf:parseType="Collection">
                    <rdf:Description rdf:about="http://linked.earth/ontology#MeasuredVariable"/>
                    <rdf:Description rdf:about="http://linked.earth/ontology#Model"/>
                    <rdf:Description rdf:about="http://linked.earth/ontology#PhysicalSample"/>
                </owl:unionOf>
            </owl:Class>
        </rdfs:domain>
        <rdfs:range rdf:resource="http://www.w3.org/2001/XMLSchema#string"/>
        <vann:example rdf:resource="http://wiki.linked.earth/A7.Sun.2005.paleo1measurement1.d18og"/>
        <vaem:rationale xml:lang="en">Allows to describe methods.</vaem:rationale>
        <rdfs:comment xml:lang="en">Answers the question: How is the information obtained from the resource?</rdfs:comment>
        <rdfs:label xml:lang="en">method</rdfs:label>
    </owl:DatatypeProperty>
    


    <!-- http://linked.earth/ontology#name -->

    <owl:DatatypeProperty rdf:about="http://linked.earth/ontology#name">
        <rdfs:subPropertyOf rdf:resource="http://schema.org/name"/>
        <rdfs:domain rdf:resource="http://www.w3.org/2002/07/owl#Thing"/>
        <rdfs:range rdf:resource="http://www.w3.org/2001/XMLSchema#string"/>
        <vann:example rdf:resource="http://wiki.linked.earth/MD982176.Stott.2004.paleo1measurement1.Mg/Ca-g.rub"/>
        <rdfs:comment xml:lang="en">Answers the question: How is the resource called?</rdfs:comment>
        <rdfs:label xml:lang="en">name</rdfs:label>
    </owl:DatatypeProperty>
    


    <!-- http://linked.earth/ontology#notes -->

    <owl:DatatypeProperty rdf:about="http://linked.earth/ontology#notes">
        <rdfs:domain>
            <owl:Class>
                <owl:unionOf rdf:parseType="Collection">
                    <rdf:Description rdf:about="http://linked.earth/ontology#DataTable"/>
                    <rdf:Description rdf:about="http://linked.earth/ontology#Dataset"/>
                    <rdf:Description rdf:about="http://linked.earth/ontology#Model"/>
                    <rdf:Description rdf:about="http://linked.earth/ontology#Variable"/>
                </owl:unionOf>
            </owl:Class>
        </rdfs:domain>
        <rdfs:range rdf:resource="http://www.w3.org/2001/XMLSchema#string"/>
        <vann:example rdf:resource="http://wiki.linked.earth/A7.Sun.2005.chron1measurement1"/>
        <vaem:rationale xml:lang="en">Allows to add notes to specific cells in the DataTable</vaem:rationale>
        <rdfs:comment xml:lang="en">Answers the question: What additional information would you give about the Variable or DataTable ?</rdfs:comment>
        <rdfs:label xml:lang="en">notes</rdfs:label>
    </owl:DatatypeProperty>
    


    <!-- http://linked.earth/ontology#orcidNumber -->

    <owl:DatatypeProperty rdf:about="http://linked.earth/ontology#orcidNumber">
        <rdfs:subPropertyOf rdf:resource="http://purl.org/dc/terms/identifier"/>
        <rdf:type rdf:resource="http://www.w3.org/2002/07/owl#FunctionalProperty"/>
        <rdfs:domain rdf:resource="http://linked.earth/ontology#Person"/>
        <rdfs:range rdf:resource="http://www.w3.org/2001/XMLSchema#string"/>
        <vann:example rdf:resource="http://wiki.linked.earth/D._Khider"/>
        <vaem:rationale xml:lang="en">LinkedEarth uses ORCID number for membership</vaem:rationale>
        <rdfs:comment>Answers the question: What is the persistent digital identifier of the Person?</rdfs:comment>
        <rdfs:label xml:lang="en">orcid number</rdfs:label>
    </owl:DatatypeProperty>
    


    <!-- http://linked.earth/ontology#pages -->

    <owl:DatatypeProperty rdf:about="http://linked.earth/ontology#pages">
        <rdf:type rdf:resource="http://www.w3.org/2002/07/owl#FunctionalProperty"/>
        <rdfs:domain rdf:resource="http://linked.earth/ontology#Publication"/>
        <rdfs:range rdf:resource="http://www.w3.org/2001/XMLSchema#string"/>
        <vann:example rdf:resource="http://wiki.linked.earth/Publication.10.1002/2013PA002534"/>
        <vaem:rationale xml:lang="en">Part of standard metadata for Publications</vaem:rationale>
        <rdfs:comment xml:lang="en">Answers the question: In what pages of the Publication can the reference to the resource be found?</rdfs:comment>
        <rdfs:label xml:lang="en">pages</rdfs:label>
    </owl:DatatypeProperty>
    


    <!-- http://linked.earth/ontology#programmedIn -->

    <owl:DatatypeProperty rdf:about="http://linked.earth/ontology#programmedIn">
        <rdfs:subPropertyOf rdf:resource="http://ontosoft.org/software#hasImplementationLanguage"/>
        <rdfs:domain rdf:resource="http://linked.earth/ontology#SoftwareCode"/>
        <rdfs:range rdf:resource="http://www.w3.org/2001/XMLSchema#string"/>
        <vann:example rdf:resource="http://wiki.linked.earth/Pyleoclim"/>
        <vaem:rationale xml:lang="en">Provides the user with information about the software</vaem:rationale>
        <rdfs:comment xml:lang="en">Answers the question: In which language was the software code written in?</rdfs:comment>
        <rdfs:label xml:lang="en">programmed in</rdfs:label>
    </owl:DatatypeProperty>
    


    <!-- http://linked.earth/ontology#publicationYear -->

    <owl:DatatypeProperty rdf:about="http://linked.earth/ontology#publicationYear">
        <rdfs:subPropertyOf rdf:resource="http://purl.org/dc/terms/created"/>
        <rdfs:subPropertyOf rdf:resource="http://schema.org/dateCreated"/>
        <rdf:type rdf:resource="http://www.w3.org/2002/07/owl#FunctionalProperty"/>
        <rdfs:domain rdf:resource="http://linked.earth/ontology#Publication"/>
        <rdfs:range rdf:resource="http://www.w3.org/2001/XMLSchema#int"/>
        <vann:example rdf:resource="http://wiki.linked.earth/Publication.10.1002/2013PA002534"/>
        <vaem:rationale xml:lang="en">Part of standard metadata for Publications</vaem:rationale>
        <rdfs:comment xml:lang="en">Answers the question: What year was the Publication issued?</rdfs:comment>
        <rdfs:label xml:lang="en">publication year</rdfs:label>
    </owl:DatatypeProperty>
    


    <!-- http://linked.earth/ontology#relevantQuote -->

    <owl:DatatypeProperty rdf:about="http://linked.earth/ontology#relevantQuote">
        <rdfs:subPropertyOf rdf:resource="http://linked.earth/ontology#description"/>
        <rdfs:range rdf:resource="http://www.w3.org/2001/XMLSchema#string"/>
        <vann:example rdf:resource="http://wiki.linked.earth/Ocean2kHR_119.d18O.ClimateInterpretation"/>
        <vaem:rationale xml:lang="en">Often it&apos;s useful to put a quote from the paper that describes the interpretation</vaem:rationale>
        <rdfs:comment>Answers the question: Which part of the publication describes the Calibration or Interpretation?</rdfs:comment>
        <rdfs:label xml:lang="en">relevant quote</rdfs:label>
    </owl:DatatypeProperty>
    


    <!-- http://linked.earth/ontology#scope -->

    <owl:DatatypeProperty rdf:about="http://linked.earth/ontology#scope">
        <rdfs:domain rdf:resource="http://linked.earth/ontology#Interpretation"/>
        <rdfs:range rdf:resource="http://www.w3.org/2001/XMLSchema#string"/>
        <vaem:rationale xml:lang="en">Allows to separate the various types of interpretation</vaem:rationale>
        <rdfs:comment xml:lang="en">Answers the question: how would you classify the Interpretation? Examples include Isotope, Climate</rdfs:comment>
        <rdfs:label xml:lang="en">scope</rdfs:label>
    </owl:DatatypeProperty>
    


    <!-- http://linked.earth/ontology#seasonality -->

    <owl:DatatypeProperty rdf:about="http://linked.earth/ontology#seasonality">
        <rdfs:domain>
            <owl:Class>
                <owl:unionOf rdf:parseType="Collection">
                    <rdf:Description rdf:about="http://linked.earth/ontology#Interpretation"/>
                    <rdf:Description rdf:about="http://linked.earth/ontology#ProxySensor"/>
                </owl:unionOf>
            </owl:Class>
        </rdfs:domain>
        <rdfs:range rdf:resource="http://www.w3.org/2001/XMLSchema#string"/>
        <vann:example rdf:resource="http://wiki.linked.earth/Ocean2kHR_119.d18O.ClimateInterpretation"/>
        <vaem:rationale xml:lang="en">Seasonality is critical to properly related measuredVariable and innferredVariable, as the former only senses part of the range of the latter.</vaem:rationale>
        <rdfs:comment xml:lang="en">Answers the question: To which part of the year is the Interpretation or ProxySensor restricted to? Acceptable answers may be &quot;MJJA&quot;, &quot;growing season&quot;,or [5,6,7,8]</rdfs:comment>
        <rdfs:label xml:lang="en">seasonality</rdfs:label>
    </owl:DatatypeProperty>
    


    <!-- http://linked.earth/ontology#sensorGenus -->

    <owl:DatatypeProperty rdf:about="http://linked.earth/ontology#sensorGenus">
        <rdfs:domain rdf:resource="http://linked.earth/ontology#OrganicProxySensor"/>
        <rdfs:range rdf:resource="http://www.w3.org/2001/XMLSchema#string"/>
        <vann:example rdf:resource="http://wiki.linked.earth/Globigerinoides_ruber"/>
        <vaem:rationale xml:lang="en">Scientific Name of the organic ProxySensor</vaem:rationale>
        <rdfs:comment>Answers the question: What is the Genus of the Organic ProxySensor?</rdfs:comment>
        <rdfs:label xml:lang="en">sensor genus</rdfs:label>
    </owl:DatatypeProperty>
    


    <!-- http://linked.earth/ontology#sensorSpecies -->

    <owl:DatatypeProperty rdf:about="http://linked.earth/ontology#sensorSpecies">
        <rdfs:domain rdf:resource="http://linked.earth/ontology#OrganicProxySensor"/>
        <rdfs:range rdf:resource="http://www.w3.org/2001/XMLSchema#string"/>
        <vann:example rdf:resource="http://wiki.linked.earth/Globigerinoides_ruber"/>
        <vaem:rationale xml:lang="en">Scientific Name of the organic ProxySensor</vaem:rationale>
        <rdfs:comment xml:lang="en">Answers the question: What is the species of the Organic ProxySensor?</rdfs:comment>
        <rdfs:label xml:lang="en">sensor species</rdfs:label>
    </owl:DatatypeProperty>
    


    <!-- http://linked.earth/ontology#standard -->

    <owl:DatatypeProperty rdf:about="http://linked.earth/ontology#standard">
        <rdfs:domain rdf:resource="http://linked.earth/ontology#MeasuredVariable"/>
        <rdfs:range rdf:resource="http://www.w3.org/2001/XMLSchema#string"/>
        <vann:example rdf:resource="http://wiki.linked.earth/MD982181.Khider.2014.paleo1measurement1.d18Og.rub-w.v"/>
        <vaem:rationale xml:lang="en">Crucial for isotopic measurements (for instance, d18O measurements (VSMOW vs VPDB))</vaem:rationale>
        <rdfs:comment xml:lang="en">Answers the question: Reference material against which the MeasuredVariable is reported?</rdfs:comment>
        <rdfs:label xml:lang="en">standard</rdfs:label>
    </owl:DatatypeProperty>
    


    <!-- http://linked.earth/ontology#title -->

    <owl:DatatypeProperty rdf:about="http://linked.earth/ontology#title">
        <rdfs:subPropertyOf rdf:resource="http://purl.org/dc/terms/title"/>
        <rdfs:domain rdf:resource="http://linked.earth/ontology#Publication"/>
        <rdfs:range rdf:resource="http://www.w3.org/2001/XMLSchema#string"/>
        <vann:example rdf:resource="http://wiki.linked.earth/Publication.10.1029/98PA00070"/>
        <vaem:rationale xml:lang="en">Part of standard metadata for Publications</vaem:rationale>
        <rdfs:comment xml:lang="en">Answers the question: What is the title of the Publication?</rdfs:comment>
        <rdfs:label xml:lang="en">title</rdfs:label>
    </owl:DatatypeProperty>
    


    <!-- http://linked.earth/ontology#uncertaintyLevel -->

    <owl:DatatypeProperty rdf:about="http://linked.earth/ontology#uncertaintyLevel">
        <rdfs:domain rdf:resource="http://linked.earth/ontology#Uncertainty"/>
        <rdfs:range rdf:resource="http://www.w3.org/2001/XMLSchema#string"/>
        <vann:example rdf:resource="http://wiki.linked.earth/MD982181.Khider.2014.paleo1measurement1.d18orub.Uncertainty"/>
        <vaem:rationale xml:lang="en">Allows to properly make use of the reported Uncertainty values</vaem:rationale>
        <rdfs:comment xml:lang="en">Answers the question: What parameter of the error distribution is the Uncertainty value referring to?

Examples include 1-sigma, 2-sigma, 95% confidence bounds</rdfs:comment>
        <rdfs:label xml:lang="en">uncertainty level</rdfs:label>
    </owl:DatatypeProperty>
    


    <!-- http://linked.earth/ontology#volume -->

    <owl:DatatypeProperty rdf:about="http://linked.earth/ontology#volume">
        <rdf:type rdf:resource="http://www.w3.org/2002/07/owl#FunctionalProperty"/>
        <rdfs:domain rdf:resource="http://linked.earth/ontology#Publication"/>
        <rdfs:range rdf:resource="http://www.w3.org/2001/XMLSchema#string"/>
        <vann:example rdf:resource="http://wiki.linked.earth/Publication.10.1029/98PA00070"/>
        <vaem:rationale xml:lang="en">Part of standard metadata for Publications</vaem:rationale>
        <rdfs:comment xml:lang="en">Answers the question: In which volume of the Publication does the reference to the Datatset appear?</rdfs:comment>
        <rdfs:label xml:lang="en">volume</rdfs:label>
    </owl:DatatypeProperty>
    


    <!-- http://ontosoft.org/software#hasImplementationLanguage -->

    <owl:DatatypeProperty rdf:about="http://ontosoft.org/software#hasImplementationLanguage">
        <rdfs:isDefinedBy rdf:resource="http://ontosoft.org/software#"/>
    </owl:DatatypeProperty>
    


    <!-- http://purl.org/dc/terms/bibliographicCitation -->

    <owl:DatatypeProperty rdf:about="http://purl.org/dc/terms/bibliographicCitation">
        <rdfs:isDefinedBy rdf:resource="http://purl.org/dc/terms/"/>
    </owl:DatatypeProperty>
    


    <!-- http://purl.org/dc/terms/created -->

    <owl:DatatypeProperty rdf:about="http://purl.org/dc/terms/created">
        <rdfs:isDefinedBy rdf:resource="http://purl.org/dc/terms/"/>
    </owl:DatatypeProperty>
    


    <!-- http://purl.org/dc/terms/identifier -->

    <owl:DatatypeProperty rdf:about="http://purl.org/dc/terms/identifier">
        <rdfs:isDefinedBy rdf:resource="http://purl.org/dc/terms/"/>
    </owl:DatatypeProperty>
    


    <!-- http://purl.org/dc/terms/license -->

    <owl:DatatypeProperty rdf:about="http://purl.org/dc/terms/license"/>
    


    <!-- http://purl.org/dc/terms/title -->

    <owl:DatatypeProperty rdf:about="http://purl.org/dc/terms/title">
        <rdfs:isDefinedBy rdf:resource="http://purl.org/dc/terms/"/>
    </owl:DatatypeProperty>
    


    <!-- http://schema.org/citation -->

    <owl:DatatypeProperty rdf:about="http://schema.org/citation">
        <rdfs:isDefinedBy rdf:resource="http://schema.org/"/>
    </owl:DatatypeProperty>
    


    <!-- http://schema.org/dateCreated -->

    <owl:DatatypeProperty rdf:about="http://schema.org/dateCreated">
        <rdfs:isDefinedBy rdf:resource="http://schema.org/"/>
    </owl:DatatypeProperty>
    


    <!-- http://schema.org/license -->

    <owl:DatatypeProperty rdf:about="http://schema.org/license">
        <rdfs:isDefinedBy rdf:resource="http://schema.org/"/>
    </owl:DatatypeProperty>
    


    <!-- http://schema.org/name -->

    <owl:DatatypeProperty rdf:about="http://schema.org/name">
        <rdfs:domain rdf:resource="http://www.w3.org/2002/07/owl#Thing"/>
        <rdfs:range rdf:resource="http://www.w3.org/2001/XMLSchema#string"/>
        <rdfs:isDefinedBy rdf:resource="http://schema.org/"/>
    </owl:DatatypeProperty>
    


    <!-- http://schema.org/version -->

    <owl:DatatypeProperty rdf:about="http://schema.org/version">
        <rdfs:isDefinedBy rdf:resource="http://schema.org/"/>
    </owl:DatatypeProperty>
    


    <!-- http://www.opengis.net/ont/geosparql#asWKT -->

    <owl:DatatypeProperty rdf:about="http://www.opengis.net/ont/geosparql#asWKT">
        <rdfs:domain rdf:resource="http://www.opengis.net/ont/geosparql#Geometry"/>
        <rdfs:range rdf:resource="http://www.w3.org/2000/01/rdf-schema#Literal"/>
        <rdfs:isDefinedBy rdf:resource="http://www.opengis.net/ont/geosparql#"/>
    </owl:DatatypeProperty>
    


    <!-- http://www.w3.org/2003/01/geo/wgs84_pos#alt -->

    <owl:DatatypeProperty rdf:about="http://www.w3.org/2003/01/geo/wgs84_pos#alt">
        <rdfs:subPropertyOf rdf:resource="http://www.w3.org/2002/07/owl#topDataProperty"/>
        <rdfs:domain rdf:resource="http://www.w3.org/2003/01/geo/wgs84_pos#SpatialThing"/>
        <rdfs:range rdf:resource="http://www.w3.org/2001/XMLSchema#string"/>
        <rdfs:isDefinedBy rdf:resource="http://www.w3.org/2003/01/geo/wgs84_pos#"/>
    </owl:DatatypeProperty>
    


    <!-- http://www.w3.org/2003/01/geo/wgs84_pos#lat -->

    <owl:DatatypeProperty rdf:about="http://www.w3.org/2003/01/geo/wgs84_pos#lat">
        <rdfs:domain rdf:resource="http://www.w3.org/2003/01/geo/wgs84_pos#SpatialThing"/>
        <rdfs:range rdf:resource="http://www.w3.org/2001/XMLSchema#string"/>
        <rdfs:isDefinedBy rdf:resource="http://www.w3.org/2003/01/geo/wgs84_pos#"/>
    </owl:DatatypeProperty>
    


    <!-- http://www.w3.org/2003/01/geo/wgs84_pos#long -->

    <owl:DatatypeProperty rdf:about="http://www.w3.org/2003/01/geo/wgs84_pos#long">
        <rdfs:domain rdf:resource="http://www.w3.org/2003/01/geo/wgs84_pos#SpatialThing"/>
        <rdfs:range rdf:resource="http://www.w3.org/2001/XMLSchema#string"/>
        <rdfs:isDefinedBy rdf:resource="http://www.w3.org/2003/01/geo/wgs84_pos#"/>
    </owl:DatatypeProperty>
    


    <!-- 
    ///////////////////////////////////////////////////////////////////////////////////////
    //
    // Classes
    //
    ///////////////////////////////////////////////////////////////////////////////////////
     -->

    


    <!-- http://linked.earth/ontology#AcceleratorMassSpectrometer -->

    <owl:Class rdf:about="http://linked.earth/ontology#AcceleratorMassSpectrometer">
        <rdfs:subClassOf rdf:resource="http://linked.earth/ontology#MassSpectrometer"/>
        <rdfs:label xml:lang="en">Accelerator mass spectrometer</rdfs:label>
    </owl:Class>
    


    <!-- http://linked.earth/ontology#AcceleratorMassSpectrometerInstrument -->

    <owl:Class rdf:about="http://linked.earth/ontology#AcceleratorMassSpectrometerInstrument">
        <rdfs:subClassOf rdf:resource="http://linked.earth/ontology#AcceleratorMassSpectrometer"/>
        <rdfs:label xml:lang="en">Accelerator mass spectrometer</rdfs:label>
    </owl:Class>
    


    <!-- http://linked.earth/ontology#Archea -->

    <owl:Class rdf:about="http://linked.earth/ontology#Archea">
        <rdfs:subClassOf rdf:resource="http://linked.earth/ontology#OrganicProxySensor"/>
        <rdfs:label xml:lang="en">Archea</rdfs:label>
    </owl:Class>
    


    <!-- http://linked.earth/ontology#Assemblage -->

    <owl:Class rdf:about="http://linked.earth/ontology#Assemblage">
        <rdfs:subClassOf rdf:resource="http://linked.earth/ontology#ProxyObservation"/>
        <rdfs:label xml:lang="en">Assemblage</rdfs:label>
    </owl:Class>
    


    <!-- http://linked.earth/ontology#AtmosphericChemistry -->

    <owl:Class rdf:about="http://linked.earth/ontology#AtmosphericChemistry">
        <rdfs:subClassOf rdf:resource="http://linked.earth/ontology#InferredVariable"/>
        <rdfs:label xml:lang="en">Atmospheric chemistry</rdfs:label>
    </owl:Class>
    


    <!-- http://linked.earth/ontology#BinocularMicroscope -->

    <owl:Class rdf:about="http://linked.earth/ontology#BinocularMicroscope">
        <rdfs:subClassOf rdf:resource="http://linked.earth/ontology#Microscope"/>
        <rdfs:label xml:lang="en">Binocular microscope</rdfs:label>
    </owl:Class>
    


    <!-- http://linked.earth/ontology#Bivalves -->

    <owl:Class rdf:about="http://linked.earth/ontology#Bivalves">
        <rdfs:subClassOf rdf:resource="http://linked.earth/ontology#Mollusk"/>
        <rdfs:label xml:lang="en">Bivalves</rdfs:label>
    </owl:Class>
    


    <!-- http://linked.earth/ontology#CFAMS -->

    <owl:Class rdf:about="http://linked.earth/ontology#CFAMS">
        <rdfs:subClassOf rdf:resource="http://linked.earth/ontology#AcceleratorMassSpectrometer"/>
        <rdfs:label xml:lang="en">Continuous-flow AMS system</rdfs:label>
    </owl:Class>
    


    <!-- http://linked.earth/ontology#CRDS -->

    <owl:Class rdf:about="http://linked.earth/ontology#CRDS">
        <rdfs:subClassOf rdf:resource="http://linked.earth/ontology#Spectroscope"/>
        <rdfs:label xml:lang="en">Cavity Ring-Down Spectroscopy</rdfs:label>
    </owl:Class>
    


    <!-- http://linked.earth/ontology#CalibrationModel -->

    <owl:Class rdf:about="http://linked.earth/ontology#CalibrationModel">
        <rdfs:subClassOf rdf:resource="http://linked.earth/ontology#Model"/>
        <vann:example rdf:resource="http://wiki.linked.earth/MD982181.Khider.2014.paleo1measurement1.mgcarub.Calibration"/>
        <vaem:rationale xml:lang="en">Make the model behind the calibration explicit</vaem:rationale>
        <rdfs:comment xml:lang="en">Metadata about how the variable was calibrated to reflect an environmental variable</rdfs:comment>
        <rdfs:label xml:lang="en">Calibration model</rdfs:label>
    </owl:Class>
    


    <!-- http://linked.earth/ontology#Chemical -->

    <owl:Class rdf:about="http://linked.earth/ontology#Chemical">
        <rdfs:subClassOf rdf:resource="http://linked.earth/ontology#ProxyObservation"/>
        <rdfs:label xml:lang="en">Chemical</rdfs:label>
    </owl:Class>
    


    <!-- http://linked.earth/ontology#Chironomids -->

    <owl:Class rdf:about="http://linked.earth/ontology#Chironomids">
        <rdfs:subClassOf rdf:resource="http://linked.earth/ontology#OrganicProxySensor"/>
        <rdfs:label xml:lang="en">Chironomids</rdfs:label>
    </owl:Class>
    


    <!-- http://linked.earth/ontology#ChronData -->

    <owl:Class rdf:about="http://linked.earth/ontology#ChronData">
        <rdfs:subClassOf rdf:resource="http://linked.earth/ontology#Data"/>
        <vann:example rdf:resource="http://wiki.linked.earth/MD982181.Khider.2014.ChronData1"/>
        <vaem:rationale xml:lang="en">Subdivision between chronological and paleoenvironmental information reflects the fact that Datasets are fundamentally characterized by two distinct components</vaem:rationale>
        <rdfs:comment xml:lang="en">The data, metadata, and Model that describe the set of Variables used to relate depth/position to time (chronological information)</rdfs:comment>
        <rdfs:label xml:lang="en">Chron data</rdfs:label>
    </owl:Class>
    


    <!-- http://linked.earth/ontology#ChronDataTable -->

    <owl:Class rdf:about="http://linked.earth/ontology#ChronDataTable">
        <rdfs:subClassOf rdf:resource="http://linked.earth/ontology#DataTable"/>
        <owl:disjointWith rdf:resource="http://linked.earth/ontology#PaleoDataTable"/>
        <vann:example rdf:resource="http://wiki.linked.earth/MD982181.Khider.2014.chron1measurement1"/>
        <vaem:rationale xml:lang="en">Subdivision between chronological and paleoenvironmental information reflects the fact that Datasets are fundamentally characterized by two distinct components</vaem:rationale>
        <rdfs:comment xml:lang="en">DataTable containing Variables pertaining to chronological information</rdfs:comment>
        <rdfs:label xml:lang="en">Chron data table</rdfs:label>
    </owl:Class>
    


    <!-- http://linked.earth/ontology#ChronModel -->

    <owl:Class rdf:about="http://linked.earth/ontology#ChronModel">
        <rdfs:subClassOf rdf:resource="http://linked.earth/ontology#Model"/>
        <vann:example rdf:resource="http://wiki.linked.earth/MD982181.Khider.2014.ChronData1.Model1"/>
        <vaem:rationale xml:lang="en">Subdivision between chronological and paleoenvironmental information reflects the fact that Datasets are fundamentally characterized by two distinct components</vaem:rationale>
        <rdfs:comment xml:lang="en">Model used to derive a time (or age) axis from the ChronDataModel</rdfs:comment>
        <rdfs:label xml:lang="en">Chron model</rdfs:label>
    </owl:Class>
    


    <!-- http://linked.earth/ontology#ChronProxySystem -->

    <owl:Class rdf:about="http://linked.earth/ontology#ChronProxySystem">
        <rdfs:subClassOf rdf:resource="http://linked.earth/ontology#ProxySystem"/>
        <vaem:rationale xml:lang="en">Subdivision between chronological and paleoenvironmental information reflects the fact that Datasets are fundamentally characterized by two distinct components.

Agreed that the ProxySystem concept applies to both Chron and PaleoData</vaem:rationale>
        <rdfs:comment xml:lang="en">The combination of ProxyArchive, ProxySensor, and ProxyObservations pertaining to chronological information. For instance, measurements of radiocarbon on foraminiferal shells would have a ChronProxySystem consisting of ProxyArchive: marine sediment, ProxySensor: Foraminifera, ProxyObservations: Radiocarbon. (ref: Evans et al. [2013])</rdfs:comment>
        <rdfs:label xml:lang="en">Chron proxy system</rdfs:label>
    </owl:Class>
    


    <!-- http://linked.earth/ontology#ClimateIndex -->

    <owl:Class rdf:about="http://linked.earth/ontology#ClimateIndex">
        <rdfs:subClassOf rdf:resource="http://linked.earth/ontology#InferredVariable"/>
        <rdfs:label xml:lang="en">Climate index</rdfs:label>
    </owl:Class>
    


    <!-- http://linked.earth/ontology#Coccolithophores -->

    <owl:Class rdf:about="http://linked.earth/ontology#Coccolithophores">
        <rdfs:subClassOf rdf:resource="http://linked.earth/ontology#OrganicProxySensor"/>
        <rdfs:label xml:lang="en">Coccolithophores</rdfs:label>
    </owl:Class>
    


    <!-- http://linked.earth/ontology#Compilation -->

    <owl:Class rdf:about="http://linked.earth/ontology#Compilation">
        <rdfs:subClassOf rdf:resource="http://schema.org/DataCatalog"/>
        <vaem:rationale xml:lang="en">Encodes what Data/Metadata gathering effort/scientific project led to the curation of the Datasets. Examples: PAGES2k, Iso2k, LR04, OC3, MARGO</vaem:rationale>
        <rdfs:comment xml:lang="en">A curated aggregation of datasets</rdfs:comment>
        <rdfs:label xml:lang="en">Compilation</rdfs:label>
    </owl:Class>
    


    <!-- http://linked.earth/ontology#Composition -->

    <owl:Class rdf:about="http://linked.earth/ontology#Composition">
        <rdfs:subClassOf rdf:resource="http://linked.earth/ontology#Physical"/>
        <rdfs:label xml:lang="en">Composition</rdfs:label>
    </owl:Class>
    


    <!-- http://linked.earth/ontology#Coral -->

    <owl:Class rdf:about="http://linked.earth/ontology#Coral">
        <rdfs:subClassOf rdf:resource="http://linked.earth/ontology#ProxyArchive"/>
        <rdfs:comment xml:lang="en">&lt;p&gt;The geochemical tracers contain in the skeletons of &lt;a rel=&quot;nofollow&quot; class=&quot;external text&quot; href=&quot;https://en.wikipedia.org/wiki/Coral&quot;&gt;corals&lt;/a&gt; provide an unaltered record of the chemical and physical conditions that existed in the surrounding seawater at the time of accretion of its calcium carbonate skeleton &lt;sup id=&quot;cite_ref-druffel1997_1-0&quot; class=&quot;reference&quot;&gt;&lt;a href=&quot;#cite_note-druffel1997-1&quot;&gt;[1]&lt;/a&gt;&lt;/sup&gt;. Corals are useful oceanic recorders because they are widely distributed, can be accurately dated, provide an  enhanced time resolution (monthly) available from the high growth rate, and are nor subjected to the mixing processes that are present in all toxic sediments (i.e., bioturbation) &lt;sup id=&quot;cite_ref-druffel1997_1-1&quot; class=&quot;reference&quot;&gt;&lt;a href=&quot;#cite_note-druffel1997-1&quot;&gt;[1]&lt;/a&gt;&lt;/sup&gt; &lt;sup id=&quot;cite_ref-2&quot; class=&quot;reference&quot;&gt;&lt;a href=&quot;#cite_note-2&quot;&gt;[2]&lt;/a&gt;&lt;/sup&gt;.
&lt;/p&gt;&lt;p&gt;Corals are from the order Scleractinian, a group in the subclass Zoantharia. Scleractinians include solitary and colonial species of corals. may of which secrete external skeletons of &lt;a rel=&quot;nofollow&quot; class=&quot;external text&quot; href=&quot;https://en.wikipedia.org/wiki/Aragonite&quot;&gt;aragonite&lt;/a&gt; &lt;sup id=&quot;cite_ref-druffel1997_1-2&quot; class=&quot;reference&quot;&gt;&lt;a href=&quot;#cite_note-druffel1997-1&quot;&gt;[1]&lt;/a&gt;&lt;/sup&gt;. The oldest known scleractinians are shallow water corals from the Middle Triassic &lt;sup id=&quot;cite_ref-3&quot; class=&quot;reference&quot;&gt;&lt;a href=&quot;#cite_note-3&quot;&gt;[3]&lt;/a&gt;&lt;/sup&gt;.
&lt;/p&gt;
The polyp portion of the coral secretes calcium carbonate (CaCO&lt;sub&gt;3&lt;/sub&gt;) as the mineral aragonite &lt;sup id=&quot;cite_ref-druffel1997_1-3&quot; class=&quot;reference&quot;&gt;&lt;a href=&quot;#cite_note-druffel1997-1&quot;&gt;[1]&lt;/a&gt;&lt;/sup&gt;. Massive &lt;a rel=&quot;nofollow&quot; class=&quot;external text&quot; href=&quot;https://en.wikipedia.org/wiki/Hermatypic_coral&quot;&gt;hermatypic corals&lt;/a&gt; (i.e., reef-building corals) are more desirable than the branching varieties for paleoreconstructions. First, massive corals form round, wave-resistant structures that can include hundreds of years of uninterrupted growth. Second, the accretion rate of calcium carbonate is much higher for hermatypic corals  that contain symbiotic &lt;a rel=&quot;nofollow&quot; class=&quot;external text&quot; href=&quot;https://en.wikipedia.org/wiki/Zooxanthellae&quot;&gt;zooxanthellae&lt;/a&gt; than for deep species &lt;sup id=&quot;cite_ref-druffel1997_1-4&quot; class=&quot;reference&quot;&gt;&lt;a href=&quot;#cite_note-druffel1997-1&quot;&gt;[1]&lt;/a&gt;&lt;/sup&gt;. Most massive reef corals live at water depths of &amp;lt;40m and grow continuously at rated of 6-20 mm yr&lt;sup&gt;-1&lt;/sup&gt; &lt;sup id=&quot;cite_ref-4&quot; class=&quot;reference&quot;&gt;&lt;a href=&quot;#cite_note-4&quot;&gt;[4]&lt;/a&gt;&lt;/sup&gt;&lt;ol class=&quot;references&quot;&gt;
&lt;li id=&quot;cite_note-druffel1997-1&quot;&gt;&lt;span class=&quot;mw-cite-backlink&quot;&gt;? &lt;sup&gt;&lt;a href=&quot;#cite_ref-druffel1997_1-0&quot;&gt;1.0&lt;/a&gt;&lt;/sup&gt; &lt;sup&gt;&lt;a href=&quot;#cite_ref-druffel1997_1-1&quot;&gt;1.1&lt;/a&gt;&lt;/sup&gt; &lt;sup&gt;&lt;a href=&quot;#cite_ref-druffel1997_1-2&quot;&gt;1.2&lt;/a&gt;&lt;/sup&gt; &lt;sup&gt;&lt;a href=&quot;#cite_ref-druffel1997_1-3&quot;&gt;1.3&lt;/a&gt;&lt;/sup&gt; &lt;sup&gt;&lt;a href=&quot;#cite_ref-druffel1997_1-4&quot;&gt;1.4&lt;/a&gt;&lt;/sup&gt;&lt;/span&gt; &lt;span class=&quot;reference-text&quot;&gt;Druffel, E. R. M. (1997). Geochemistry of corals: Proxies of past ocean chemistry, ocean circulation, and climate. Proceeding of the National Academy of Sciences, 94, 8354-8361. &lt;/span&gt;
&lt;/li&gt;
&lt;li id=&quot;cite_note-2&quot;&gt;&lt;span class=&quot;mw-cite-backlink&quot;&gt;&lt;a href=&quot;#cite_ref-2&quot;&gt;?&lt;/a&gt;&lt;/span&gt; &lt;span class=&quot;reference-text&quot;&gt; Gagan, M. K., Ayliffe, L. K., Beck, J. W., Cole, J. E., Druffel, E. R. M., Dunbar, R. B., &amp;amp; Schrag, D. P. (2000). New views of tropical paleoclimates from corals. Quaternary Science Reviews, 19(1-5), 45-64. doi:10.1016/S0277-3791(99)00054-2&lt;/span&gt;
&lt;/li&gt;
&lt;li id=&quot;cite_note-3&quot;&gt;&lt;span class=&quot;mw-cite-backlink&quot;&gt;&lt;a href=&quot;#cite_ref-3&quot;&gt;?&lt;/a&gt;&lt;/span&gt; &lt;span class=&quot;reference-text&quot;&gt; Stanley, G. (1981). Early history of scleractinian corals and its geological consequences. Geology, 9, 507-511. &lt;/span&gt;
&lt;/li&gt;
&lt;li id=&quot;cite_note-4&quot;&gt;&lt;span class=&quot;mw-cite-backlink&quot;&gt;&lt;a href=&quot;#cite_ref-4&quot;&gt;?&lt;/a&gt;&lt;/span&gt; &lt;span class=&quot;reference-text&quot;&gt;Knutson, D. W., Buddemeier, R. W., &amp;amp; Smith, S. V. (1972). Coal chronologies: seasonal growth bands in reef corals. Science, 177, 270-272. &lt;/span&gt;
&lt;/li&gt;
&lt;/ol&gt;</rdfs:comment>
        <rdfs:label xml:lang="en">Coral</rdfs:label>
    </owl:Class>
    


    <!-- http://linked.earth/ontology#Data -->

    <owl:Class rdf:about="http://linked.earth/ontology#Data">
        <vaem:rationale xml:lang="en">Needed to describe the paleoenvironmental and/or chronological data comprising the dataset as opposed to the Publication, Funding and Location information</vaem:rationale>
        <rdfs:comment xml:lang="en">An aggregation of DataTables and Models with their supporting paleoenvironmental and/or chronological information</rdfs:comment>
        <rdfs:label xml:lang="en">Data</rdfs:label>
    </owl:Class>
    


    <!-- http://linked.earth/ontology#DataTable -->

    <owl:Class rdf:about="http://linked.earth/ontology#DataTable">
        <vaem:rationale xml:lang="en">Connects to the csv file where the data values are stored</vaem:rationale>
        <rdfs:comment xml:lang="en">A set of Variables organized in columns</rdfs:comment>
        <rdfs:label xml:lang="en">Data table</rdfs:label>
    </owl:Class>
    


    <!-- http://linked.earth/ontology#Dataset -->

    <owl:Class rdf:about="http://linked.earth/ontology#Dataset">
        <rdfs:subClassOf rdf:resource="http://schema.org/Dataset"/>
        <vaem:rationale xml:lang="en">Fundamental unit at which we think about paleoclimate data. Also tends to correspond to the scope of the study</vaem:rationale>
        <rdfs:comment xml:lang="en">A structured collection of related information, including -but not limited to -measured and/or modelled geograhical, chronological, and environmental data</rdfs:comment>
        <rdfs:label xml:lang="en">Dataset</rdfs:label>
    </owl:Class>
    


    <!-- http://linked.earth/ontology#Diffraction -->

    <owl:Class rdf:about="http://linked.earth/ontology#Diffraction">
        <rdfs:subClassOf rdf:resource="http://linked.earth/ontology#Spectral"/>
        <rdfs:label xml:lang="en">Diffraction</rdfs:label>
    </owl:Class>
    


    <!-- http://linked.earth/ontology#DistributionTable -->

    <owl:Class rdf:about="http://linked.earth/ontology#DistributionTable">
        <rdfs:subClassOf rdf:resource="http://linked.earth/ontology#DataTable"/>
        <vann:example rdf:resource="http://wiki.linked.earth/ODP1098B12.Chron1.Model1.distributionTable.1"/>
        <vaem:rationale xml:lang="en">Added to allow outputs from Bayesian model (especially Bchron) to be saved as part of a dataset. Required to encode irregular probability distributions</vaem:rationale>
        <rdfs:comment xml:lang="en">DataTable containing the probability distribution of a single value of a Variable. Output of a Model</rdfs:comment>
        <rdfs:label xml:lang="en">Distribution table</rdfs:label>
    </owl:Class>
    


    <!-- http://linked.earth/ontology#Document -->

    <owl:Class rdf:about="http://linked.earth/ontology#Document">
        <rdfs:subClassOf rdf:resource="http://linked.earth/ontology#ProxyArchive"/>
        <rdfs:label xml:lang="en">Document</rdfs:label>
    </owl:Class>
    


    <!-- http://linked.earth/ontology#ElNinoIndex -->

    <owl:Class rdf:about="http://linked.earth/ontology#ElNinoIndex">
        <rdfs:subClassOf rdf:resource="http://linked.earth/ontology#ClimateIndex"/>
    </owl:Class>
    


    <!-- http://linked.earth/ontology#EnergyDispersiveSpectrometer -->

    <owl:Class rdf:about="http://linked.earth/ontology#EnergyDispersiveSpectrometer">
        <rdfs:subClassOf rdf:resource="http://linked.earth/ontology#Spectrometer"/>
        <rdfs:label xml:lang="en">Energy dispersive spectrometer</rdfs:label>
    </owl:Class>
    


    <!-- http://linked.earth/ontology#EnsembleTable -->

    <owl:Class rdf:about="http://linked.earth/ontology#EnsembleTable">
        <rdfs:subClassOf rdf:resource="http://linked.earth/ontology#DataTable"/>
        <vann:example rdf:resource="http://wiki.linked.earth/ODP1098B12.Chron1.Model1.EnsembleTable"/>
        <vaem:rationale xml:lang="en">Added to allow outputs from Bayesian model to be saved as part of a dataset</vaem:rationale>
        <rdfs:comment xml:lang="en">DataTable constaining many possible series of how the Variable is modeled. Output of a Model</rdfs:comment>
        <rdfs:label xml:lang="en">Ensemble table</rdfs:label>
    </owl:Class>
    


    <!-- http://linked.earth/ontology#Fluorescence -->

    <owl:Class rdf:about="http://linked.earth/ontology#Fluorescence">
        <rdfs:subClassOf rdf:resource="http://linked.earth/ontology#Spectral"/>
        <rdfs:label xml:lang="en">Fluorescence</rdfs:label>
    </owl:Class>
    


    <!-- http://linked.earth/ontology#Foraminifera -->

    <owl:Class rdf:about="http://linked.earth/ontology#Foraminifera">
        <rdfs:subClassOf rdf:resource="http://linked.earth/ontology#OrganicProxySensor"/>
        <rdfs:comment xml:lang="en">Because of their population size, foraminifera produce a significant amount of oceanic carbonate, making them a valuable source of paleoceanographic information.

The following parameters are used in paleoceanographic applications:

* Faunal Assemblage
* Geochemical measurements:
 *  Isotopes
 * Stable oxygen isotopes
 * Stable carbon isotopes
 * Radiocarbon
* Trace Elements</rdfs:comment>
        <rdfs:isDefinedBy rdf:resource="http://wiki.linked.earth/Foraminifera"/>
        <rdfs:label xml:lang="en">Foraminifera</rdfs:label>
    </owl:Class>
    


    <!-- http://linked.earth/ontology#Funding -->

    <owl:Class rdf:about="http://linked.earth/ontology#Funding">
        <vann:example xml:lang="en">http://wiki.linked.earth/MD982181.Khider.2014.Funding1</vann:example>
        <vaem:rationale xml:lang="en">Allows to associate a grant number following U.S. federal regulation</vaem:rationale>
        <rdfs:comment xml:lang="en">Source of monetary support underlying the collection/creation/analysis/curation of the Dataset</rdfs:comment>
        <rdfs:label xml:lang="en">Funding</rdfs:label>
    </owl:Class>
    


    <!-- http://linked.earth/ontology#GC-IR-MS -->

    <owl:Class rdf:about="http://linked.earth/ontology#GC-IR-MS">
        <rdfs:subClassOf rdf:resource="http://linked.earth/ontology#GasChromatographyMassSpectrometer"/>
        <rdfs:label xml:lang="en">Gas Chromatography - Isotope ratio -Mass Spectrometer</rdfs:label>
    </owl:Class>
    


    <!-- http://linked.earth/ontology#GCMS -->

    <owl:Class rdf:about="http://linked.earth/ontology#GCMS">
        <rdfs:subClassOf rdf:resource="http://linked.earth/ontology#GasChromatographyMassSpectrometer"/>
        <rdfs:label xml:lang="en">Gas chromatography mass spectrometer</rdfs:label>
    </owl:Class>
    


    <!-- http://linked.earth/ontology#GasChromatograph -->

    <owl:Class rdf:about="http://linked.earth/ontology#GasChromatograph">
        <rdfs:subClassOf rdf:resource="http://linked.earth/ontology#Instrument"/>
        <rdfs:label xml:lang="en">Gas chromatograph</rdfs:label>
    </owl:Class>
    


    <!-- http://linked.earth/ontology#GasChromatographyMassSpectrometer -->

    <owl:Class rdf:about="http://linked.earth/ontology#GasChromatographyMassSpectrometer">
        <rdfs:subClassOf rdf:resource="http://linked.earth/ontology#MassSpectrometer"/>
        <rdfs:label xml:lang="en">Gas chromatography - mass spectrometer</rdfs:label>
    </owl:Class>
    


    <!-- http://linked.earth/ontology#Gastropods -->

    <owl:Class rdf:about="http://linked.earth/ontology#Gastropods">
        <rdfs:subClassOf rdf:resource="http://linked.earth/ontology#Mollusk"/>
        <rdfs:label xml:lang="en">Gastropods</rdfs:label>
    </owl:Class>
    


    <!-- http://linked.earth/ontology#GlacierIce -->

    <owl:Class rdf:about="http://linked.earth/ontology#GlacierIce">
        <rdfs:subClassOf rdf:resource="http://linked.earth/ontology#ProxyArchive"/>
        <rdfs:label xml:lang="en">Glacier ice</rdfs:label>
    </owl:Class>
    


    <!-- http://linked.earth/ontology#Hybrid -->

    <owl:Class rdf:about="http://linked.earth/ontology#Hybrid">
        <rdfs:subClassOf rdf:resource="http://linked.earth/ontology#ProxyArchive"/>
        <rdfs:label xml:lang="en">Hybrid</rdfs:label>
    </owl:Class>
    


    <!-- http://linked.earth/ontology#Hydrology -->

    <owl:Class rdf:about="http://linked.earth/ontology#Hydrology">
        <rdfs:subClassOf rdf:resource="http://linked.earth/ontology#InferredVariable"/>
        <rdfs:label xml:lang="en">Hydrology</rdfs:label>
    </owl:Class>
    


    <!-- http://linked.earth/ontology#ICP-AES -->

    <owl:Class rdf:about="http://linked.earth/ontology#ICP-AES">
        <owl:equivalentClass rdf:resource="http://linked.earth/ontology#ICP-OES"/>
        <rdfs:subClassOf rdf:resource="http://linked.earth/ontology#Spectroscope"/>
        <rdfs:comment xml:lang="en">Inductively coupled plasma atomic emission spectroscopy (ICP-AES), also referred to as inductively coupled plasma optical emission spectrometry (ICP-OES), is an analytical technique used for the detection of trace metals.</rdfs:comment>
        <rdfs:label xml:lang="en">Inductively coupled plasma atomic emission spectroscope</rdfs:label>
    </owl:Class>
    


    <!-- http://linked.earth/ontology#ICP-MS -->

    <owl:Class rdf:about="http://linked.earth/ontology#ICP-MS">
        <rdfs:subClassOf rdf:resource="http://linked.earth/ontology#IsotopeRatioMassSpectrometer"/>
        <rdfs:label xml:lang="en">Inductively coupled plasma mass spectrometer</rdfs:label>
    </owl:Class>
    


    <!-- http://linked.earth/ontology#ICP-OES -->

    <owl:Class rdf:about="http://linked.earth/ontology#ICP-OES">
        <rdfs:subClassOf rdf:resource="http://linked.earth/ontology#Spectroscope"/>
        <rdfs:label xml:lang="en">Inductively coupled plasma optical emission spectrometry</rdfs:label>
    </owl:Class>
    


    <!-- http://linked.earth/ontology#IRMS -->

    <owl:Class rdf:about="http://linked.earth/ontology#IRMS">
        <rdfs:subClassOf rdf:resource="http://linked.earth/ontology#IsotopeRatioMassSpectrometer"/>
        <rdfs:comment xml:lang="en">An &lt;b&gt;isotope-ration mass spectrometer&lt;/b&gt; measures the relative abundance of isotopes in a given sample.</rdfs:comment>
        <rdfs:label xml:lang="en">Isotope ratio mass spectrometer</rdfs:label>
    </owl:Class>
    


    <!-- http://linked.earth/ontology#IceSheet -->

    <owl:Class rdf:about="http://linked.earth/ontology#IceSheet">
        <rdfs:subClassOf rdf:resource="http://linked.earth/ontology#InorganicProxySensor"/>
        <rdfs:label xml:lang="en">Ice sheet</rdfs:label>
    </owl:Class>
    


    <!-- http://linked.earth/ontology#InferredVariable -->

    <owl:Class rdf:about="http://linked.earth/ontology#InferredVariable">
        <rdfs:subClassOf rdf:resource="http://linked.earth/ontology#Variable"/>
        <owl:disjointWith rdf:resource="http://linked.earth/ontology#MeasuredVariable"/>
        <vann:example rdf:resource="http://wiki.linked.earth/MD982181.Khider.2014.paleo1measurement2.sst"/>
        <vaem:rationale xml:lang="en">See InferredVariable Ontology for concept description.</vaem:rationale>
        <rdfs:comment xml:lang="en">A Variable that is inferred from one or more MeasuredVariable (s)</rdfs:comment>
        <rdfs:isDefinedBy rdf:resource="http://linked.earth/ontology/core/1.2.0"/>
        <rdfs:label xml:lang="en">Inferred variable</rdfs:label>
    </owl:Class>
    


    <!-- http://linked.earth/ontology#InorganicProxySensor -->

    <owl:Class rdf:about="http://linked.earth/ontology#InorganicProxySensor">
        <rdfs:subClassOf rdf:resource="http://linked.earth/ontology#ProxySensor"/>
        <owl:disjointWith rdf:resource="http://linked.earth/ontology#OrganicProxySensor"/>
        <vaem:rationale xml:lang="en">Encode the Genus and Species metadata</vaem:rationale>
        <rdfs:comment xml:lang="en">An inorganic substrate sensing enviromental changes. Examples: karst, snow, watershed, ice sheet, rock, etc.</rdfs:comment>
        <rdfs:isDefinedBy rdf:resource="http://linked.earth/ontology/core/"/>
        <rdfs:label xml:lang="en">Inorganic proxy sensor</rdfs:label>
    </owl:Class>
    


    <!-- http://linked.earth/ontology#Instrument -->

    <owl:Class rdf:about="http://linked.earth/ontology#Instrument">
        <vann:example rdf:resource="http://wiki.linked.earth/MD982181.Khider.2014.paleo1measurement1.mgcarub.ICPAES"/>
        <vaem:rationale xml:lang="en">Needed to categorize types of instruments used for taking the different measurements. See Instrument Ontology for concept description.</vaem:rationale>
        <rdfs:comment xml:lang="en">A tool  used to produce MeasuredVariables</rdfs:comment>
        <rdfs:isDefinedBy rdf:resource="http://linked.earth/ontology/core/1.2.0"/>
        <rdfs:label xml:lang="en">Instrument</rdfs:label>
    </owl:Class>
    


    <!-- http://linked.earth/ontology#IntegrationTime -->

    <owl:Class rdf:about="http://linked.earth/ontology#IntegrationTime">
        <vaem:rationale xml:lang="en">Soilwater mixing above speleothems: Although the sample might only represent 5 years of calcification, it can record 30 years of water mixing.</vaem:rationale>
        <rdfs:comment>The time it takes for the ProxySensor to imprint environmental information on the ProxyArchive. It may be further qualified with time periods and units</rdfs:comment>
        <rdfs:label xml:lang="en">Integration time</rdfs:label>
    </owl:Class>
    


    <!-- http://linked.earth/ontology#Interpretation -->

    <owl:Class rdf:about="http://linked.earth/ontology#Interpretation">
        <vann:example rdf:resource="http://wiki.linked.earth/MD982181.Khider.2014.paleo1measurement1.mgcarub.Interpretation"/>
        <vaem:rationale xml:lang="en">Used to describe the interpretation of the Variable. For instance, radiocarbon is interpreted to represent age</vaem:rationale>
        <rdfs:comment xml:lang="en">A suite of metadata that describes which phenomena drove variability in this Variable (e.g. environmental drivers).</rdfs:comment>
        <rdfs:label xml:lang="en">Interpretation</rdfs:label>
    </owl:Class>
    


    <!-- http://linked.earth/ontology#Isotope -->

    <owl:Class rdf:about="http://linked.earth/ontology#Isotope">
        <rdfs:subClassOf rdf:resource="http://linked.earth/ontology#Chemical"/>
        <rdfs:comment xml:lang="en">&lt;p&gt;Atoms can be simply described as consisting of &lt;a rel=&quot;nofollow&quot; class=&quot;external text&quot; href=&quot;https://en.wikipedia.org/wiki/Proton&quot;&gt;protons&lt;/a&gt;, &lt;a rel=&quot;nofollow&quot; class=&quot;external text&quot; href=&quot;https://en.wikipedia.org/wiki/Electron&quot;&gt;electrons&lt;/a&gt;, and &lt;a rel=&quot;nofollow&quot; class=&quot;external text&quot; href=&quot;https://en.wikipedia.org/wiki/Neutron&quot;&gt;neutrons&lt;/a&gt;. Isotopes of the same element differ by the number of neutrons in the nucleus, resulting in different mass.
&lt;/p&gt;</rdfs:comment>
        <rdfs:label xml:lang="en">Isotope</rdfs:label>
    </owl:Class>
    


    <!-- http://linked.earth/ontology#IsotopeRatioMassSpectrometer -->

    <owl:Class rdf:about="http://linked.earth/ontology#IsotopeRatioMassSpectrometer">
        <rdfs:subClassOf rdf:resource="http://linked.earth/ontology#MassSpectrometer"/>
        <rdfs:label xml:lang="en">Isotope ratio mass spectrometer</rdfs:label>
    </owl:Class>
    


    <!-- http://linked.earth/ontology#IsotopicComposition -->

    <owl:Class rdf:about="http://linked.earth/ontology#IsotopicComposition">
        <rdfs:subClassOf>
            <owl:Class>
                <owl:unionOf rdf:parseType="Collection">
                    <rdf:Description rdf:about="http://linked.earth/ontology#Hydrology"/>
                    <rdf:Description rdf:about="http://linked.earth/ontology#OceanChemistry"/>
                </owl:unionOf>
            </owl:Class>
        </rdfs:subClassOf>
        <rdfs:label xml:lang="en">Isotopic composition</rdfs:label>
    </owl:Class>
    


    <!-- http://linked.earth/ontology#Karst -->

    <owl:Class rdf:about="http://linked.earth/ontology#Karst">
        <rdfs:subClassOf rdf:resource="http://linked.earth/ontology#InorganicProxySensor"/>
        <rdfs:label xml:lang="en">Karst</rdfs:label>
    </owl:Class>
    


    <!-- http://linked.earth/ontology#LA-ICP-MS -->

    <owl:Class rdf:about="http://linked.earth/ontology#LA-ICP-MS">
        <rdfs:subClassOf rdf:resource="http://linked.earth/ontology#IsotopeRatioMassSpectrometer"/>
        <rdfs:label xml:lang="en">Laser-ablation (LA) Inductively coupled plasma mass spectrometry (ICP-MS)</rdfs:label>
    </owl:Class>
    


    <!-- http://linked.earth/ontology#LakeSediment -->

    <owl:Class rdf:about="http://linked.earth/ontology#LakeSediment">
        <rdfs:subClassOf rdf:resource="http://linked.earth/ontology#ProxyArchive"/>
        <rdfs:comment xml:lang="en">&lt;p&gt;&lt;a rel=&quot;nofollow&quot; class=&quot;external text&quot; href=&quot;https://en.wikipedia.org/wiki/Lake&quot;&gt;Lake&lt;/a&gt; &lt;a rel=&quot;nofollow&quot; class=&quot;external text&quot; href=&quot;https://en.wikipedia.org/wiki/Sediment&quot;&gt;sediment&lt;/a&gt; proxies provide widespread, continuous records of terrestrial environment variability. A variety of sensors are used to indicate past water temperature, physical properties, biology, and chemistry within the &lt;a rel=&quot;nofollow&quot; class=&quot;external text&quot; href=&quot;https://en.wikipedia.org/wiki/Lake&quot;&gt;lake&lt;/a&gt; environment as well as changes in vegetation and precipitation in the &lt;a rel=&quot;nofollow&quot; class=&quot;external text&quot; href=&quot;https://en.wikipedia.org/wiki/Drainage_basin&quot;&gt;catchment&lt;/a&gt; area.
&lt;/p&gt;</rdfs:comment>
        <rdfs:label xml:lang="en">Lake sediment</rdfs:label>
    </owl:Class>
    


    <!-- http://linked.earth/ontology#Location -->

    <owl:Class rdf:about="http://linked.earth/ontology#Location">
        <rdfs:subClassOf rdf:resource="http://schema.org/Place"/>
        <rdfs:subClassOf rdf:resource="http://www.opengis.net/ont/geosparql#Feature"/>
        <rdfs:subClassOf rdf:resource="http://www.w3.org/2003/01/geo/wgs84_pos#SpatialThing"/>
        <vann:example rdf:resource="http://wiki.linked.earth/MD982181.Khider.2014.Location"/>
        <vaem:rationale xml:lang="en">Gives information about where the ProxyArchive comes from.</vaem:rationale>
        <rdfs:comment xml:lang="en">The geographic data and metadata for the dataset</rdfs:comment>
        <rdfs:label xml:lang="en">Location</rdfs:label>
    </owl:Class>
    


    <!-- http://linked.earth/ontology#MC-ICP-MS -->

    <owl:Class rdf:about="http://linked.earth/ontology#MC-ICP-MS">
        <rdfs:subClassOf rdf:resource="http://linked.earth/ontology#IsotopeRatioMassSpectrometer"/>
        <rdfs:label xml:lang="en">Multi-collector (MC) Inductively coupled plasma mass spectrometry (ICPMS)</rdfs:label>
    </owl:Class>
    


    <!-- http://linked.earth/ontology#MajorElement -->

    <owl:Class rdf:about="http://linked.earth/ontology#MajorElement">
        <rdfs:subClassOf rdf:resource="http://linked.earth/ontology#Chemical"/>
        <rdfs:label xml:lang="en">Major element</rdfs:label>
    </owl:Class>
    


    <!-- http://linked.earth/ontology#MarineSediment -->

    <owl:Class rdf:about="http://linked.earth/ontology#MarineSediment">
        <rdfs:subClassOf rdf:resource="http://linked.earth/ontology#ProxyArchive"/>
        <rdfs:comment xml:lang="en">&lt;p&gt;&lt;a rel=&quot;nofollow&quot; class=&quot;external text&quot; href=&quot;https://en.wikipedia.org/w/index.php?title=Pelagic_sediment&amp;amp;redirect=no&quot;&gt;Marine sediments&lt;/a&gt; are a type of &lt;a href=&quot;#ProxyArchive&quot; title=&quot;Category:ProxyArchive&quot;&gt; proxy archives&amp;rlm;&amp;lrm;&lt;/a&gt; that provide long, continuous records of past &lt;a rel=&quot;nofollow&quot; class=&quot;external text&quot; href=&quot;https://en.wikipedia.org/wiki/Ocean&quot;&gt;ocean&lt;/a&gt; variability. The timescales associated with this &lt;a href=&quot;#ProxyArchive&quot; title=&quot;Category:ProxyArchive&quot;&gt;archive&amp;rlm;&amp;lrm;&lt;/a&gt; are usually in the order of several tens to millions of years. The resolution of the sedimentary archive varies from annual to multi-century. &lt;a rel=&quot;nofollow&quot; class=&quot;external text&quot; href=&quot;https://en.wikipedia.org/wiki/Paleoceanography&quot;&gt;Paleoceanographic&lt;/a&gt; data are derived from many sensors found in deep-sea sediments including trace metal and isotopic composition of foraminifera, alkenones, and TEX86.
&lt;/p&gt;</rdfs:comment>
        <rdfs:label xml:lang="en">Marine sediment</rdfs:label>
    </owl:Class>
    


    <!-- http://linked.earth/ontology#MassSpectrometer -->

    <owl:Class rdf:about="http://linked.earth/ontology#MassSpectrometer">
        <rdfs:subClassOf rdf:resource="http://linked.earth/ontology#Spectrometer"/>
        <rdfs:label xml:lang="en">Mass spectrometer</rdfs:label>
    </owl:Class>
    


    <!-- http://linked.earth/ontology#MassSpectrometerInstrument -->

    <owl:Class rdf:about="http://linked.earth/ontology#MassSpectrometerInstrument">
        <rdfs:subClassOf rdf:resource="http://linked.earth/ontology#MassSpectrometer"/>
        <rdfs:label xml:lang="en">Mass spectrometer</rdfs:label>
    </owl:Class>
    


    <!-- http://linked.earth/ontology#MeasuredVariable -->

    <owl:Class rdf:about="http://linked.earth/ontology#MeasuredVariable">
        <rdfs:subClassOf>
            <owl:Class>
                <owl:intersectionOf rdf:parseType="Collection">
                    <rdf:Description rdf:about="http://linked.earth/ontology#Variable"/>
                    <rdf:Description rdf:about="http://purl.oclc.org/NET/ssnx/ssn#Observation"/>
                </owl:intersectionOf>
            </owl:Class>
        </rdfs:subClassOf>
        <vann:example rdf:resource="http://wiki.linked.earth/MD982181.Khider.2014.paleo1measurement1.mgcarub"/>
        <vaem:rationale xml:lang="en">Subclass of Variables. Allows to make the disctinction between raw measurements (e.g., tree ring width, oxygen isotopes, trace elements) and the variables being reconstructed (e.g., moisture, temperature)</vaem:rationale>
        <rdfs:comment xml:lang="en">Variables that are measured by an Instrument. MeasuredVariables are ssn: Observations. They represent the values of a certain type of ProxyObservations</rdfs:comment>
        <rdfs:label xml:lang="en">Measured variable</rdfs:label>
    </owl:Class>
    


    <!-- http://linked.earth/ontology#MeasurementTable -->

    <owl:Class rdf:about="http://linked.earth/ontology#MeasurementTable">
        <rdfs:subClassOf rdf:resource="http://linked.earth/ontology#DataTable"/>
        <vann:example rdf:resource="http://wiki.linked.earth/MD982181.Khider.2014.paleo1measurement1"/>
        <vaem:rationale xml:lang="en">Subclass of DataTable. Allows InferredVariables (despite the name) for practical purposes</vaem:rationale>
        <rdfs:comment xml:lang="en">DataTable that contains the Variables (both measured and inferred)</rdfs:comment>
        <rdfs:label xml:lang="en">Measurement table</rdfs:label>
    </owl:Class>
    


    <!-- http://linked.earth/ontology#Microscope -->

    <owl:Class rdf:about="http://linked.earth/ontology#Microscope">
        <rdfs:subClassOf rdf:resource="http://linked.earth/ontology#Instrument"/>
        <rdfs:label xml:lang="en">Microscope</rdfs:label>
    </owl:Class>
    


    <!-- http://linked.earth/ontology#Model -->

    <owl:Class rdf:about="http://linked.earth/ontology#Model">
        <vann:example rdf:resource="http://wiki.linked.earth/MD982181.Khider.2014.PaleoData1.Model1"/>
        <vaem:rationale xml:lang="en">Allows to describe models whose outputs are stored in the Dataset. One example of is Bchron for age modeling</vaem:rationale>
        <rdfs:comment xml:lang="en">A mathematical construct that is at least partially isomorphic to the target system, and is used to derive information about the structure and/or dynamics of the target system</rdfs:comment>
        <rdfs:label xml:lang="en">Model</rdfs:label>
    </owl:Class>
    


    <!-- http://linked.earth/ontology#Mollusk -->

    <owl:Class rdf:about="http://linked.earth/ontology#Mollusk">
        <rdfs:subClassOf rdf:resource="http://linked.earth/ontology#OrganicProxySensor"/>
        <rdfs:label xml:lang="en">Mollusk</rdfs:label>
    </owl:Class>
    


    <!-- http://linked.earth/ontology#MolluskShells -->

    <owl:Class rdf:about="http://linked.earth/ontology#MolluskShells">
        <rdfs:subClassOf rdf:resource="http://linked.earth/ontology#ProxyArchive"/>
        <rdfs:label xml:lang="en">Mollusk shells</rdfs:label>
    </owl:Class>
    


    <!-- http://linked.earth/ontology#NOSAMSTandetron -->

    <owl:Class rdf:about="http://linked.earth/ontology#NOSAMSTandetron">
        <rdfs:subClassOf rdf:resource="http://linked.earth/ontology#AcceleratorMassSpectrometer"/>
        <rdfs:label xml:lang="en">NOSAMS tandetron</rdfs:label>
    </owl:Class>
    


    <!-- http://linked.earth/ontology#NonPeerReviewedPublication -->

    <owl:Class rdf:about="http://linked.earth/ontology#NonPeerReviewedPublication">
        <rdfs:subClassOf rdf:resource="http://linked.earth/ontology#Publication"/>
        <owl:disjointWith rdf:resource="http://linked.earth/ontology#PeerReviewedPublication"/>
        <vaem:rationale xml:lang="en">Subclass of Publication.Allows to clearly mark datasets not generated as part of a peer-reviewed publication.</vaem:rationale>
        <rdfs:comment xml:lang="en">A publication that has not undergone a formal review process; for instance, a Dataset attached to a dissertation.</rdfs:comment>
        <rdfs:label xml:lang="en">Non peer reviewed publication</rdfs:label>
    </owl:Class>
    


    <!-- http://linked.earth/ontology#OceanChemistry -->

    <owl:Class rdf:about="http://linked.earth/ontology#OceanChemistry">
        <rdfs:subClassOf rdf:resource="http://linked.earth/ontology#InferredVariable"/>
        <rdfs:label xml:lang="en">Ocean chemistry</rdfs:label>
    </owl:Class>
    


    <!-- http://linked.earth/ontology#OrganicIndex -->

    <owl:Class rdf:about="http://linked.earth/ontology#OrganicIndex">
        <rdfs:subClassOf rdf:resource="http://linked.earth/ontology#Chemical"/>
        <rdfs:comment xml:lang="en">&lt;p&gt;Paleoceanographers use the term &lt;b&gt;biomarker&lt;/b&gt; to describe organic molecules found in &lt;a href=&quot;/Category:MarineSediment&quot; title=&quot;Category:MarineSediment&quot;&gt; marine sediments&lt;/a&gt;, initially produced by a variety of organisms either on land or in the marine environment &lt;sup id=&quot;cite_ref-rosell2007_1-0&quot; class=&quot;reference&quot;&gt;&lt;a href=&quot;#cite_note-rosell2007-1&quot;&gt;[1]&lt;/a&gt;&lt;/sup&gt;. A key characteristic of biomarkers is their ability to survive deposition in the &lt;a href=&quot;/Category:ProxyArchive_%C2%A9&quot; title=&quot;Category:ProxyArchive &quot;&gt; archive&lt;/a&gt; in terms of their original structure and steroidal configuration (i.e., spatial distribution of the atoms) &lt;sup id=&quot;cite_ref-rosell2007_1-1&quot; class=&quot;reference&quot;&gt;&lt;a href=&quot;#cite_note-rosell2007-1&quot;&gt;[1]&lt;/a&gt;&lt;/sup&gt;. Their usefulness for paleoceanographic reconstructions largely depends on their &lt;a href=&quot;/wiki/index.php?title=Degradation&amp;amp;action=edit&amp;amp;redlink=1&quot; class=&quot;new&quot; title=&quot;Degradation (page does not exist)&quot;&gt;degradation&lt;/a&gt; within the &lt;a href=&quot;/Category:ProxyArchive_%C2%A9&quot; title=&quot;Category:ProxyArchive &quot;&gt; archive&lt;/a&gt; &lt;sup id=&quot;cite_ref-rosell2007_1-2&quot; class=&quot;reference&quot;&gt;&lt;a href=&quot;#cite_note-rosell2007-1&quot;&gt;[1]&lt;/a&gt;&lt;/sup&gt;.&lt;ol class=&quot;references&quot;&gt;
&lt;li id=&quot;cite_note-rosell2007-1&quot;&gt;&lt;span class=&quot;mw-cite-backlink&quot;&gt;? &lt;sup&gt;&lt;a href=&quot;#cite_ref-rosell2007_1-0&quot;&gt;1.0&lt;/a&gt;&lt;/sup&gt; &lt;sup&gt;&lt;a href=&quot;#cite_ref-rosell2007_1-1&quot;&gt;1.1&lt;/a&gt;&lt;/sup&gt; &lt;sup&gt;&lt;a href=&quot;#cite_ref-rosell2007_1-2&quot;&gt;1.2&lt;/a&gt;&lt;/sup&gt;&lt;/span&gt; &lt;span class=&quot;reference-text&quot;&gt;Rosell-Mel, A., &amp;amp; McClymont, E. L. (2007). Biomarkers as Paleoceanographic proxies. Developments in Marine Geology, 1, 441-490. doi:10.1016/S1572-5480(07)01016-0 &lt;/span&gt;
&lt;/li&gt;
&lt;/ol&gt;</rdfs:comment>
        <rdfs:label xml:lang="en">Organic index</rdfs:label>
    </owl:Class>
    


    <!-- http://linked.earth/ontology#OrganicProxySensor -->

    <owl:Class rdf:about="http://linked.earth/ontology#OrganicProxySensor">
        <rdfs:subClassOf rdf:resource="http://linked.earth/ontology#ProxySensor"/>
        <vann:example rdf:resource="http://wiki.linked.earth/Globigerinoides_ruber"/>
        <vaem:rationale xml:lang="en">Subclass of ProxySensor. Makes the distinction between organic and inorganic. See the ProxySensor ontology for concepts</vaem:rationale>
        <rdfs:comment xml:lang="en">Biologically-mediated ProxySensor. Examples include: foraminifera, trees, mollusks, polyps</rdfs:comment>
        <rdfs:isDefinedBy rdf:resource="http://linked.earth/ontology/core/"/>
        <rdfs:label xml:lang="en">Organic proxy sensor</rdfs:label>
    </owl:Class>
    


    <!-- http://linked.earth/ontology#Ostracods -->

    <owl:Class rdf:about="http://linked.earth/ontology#Ostracods">
        <rdfs:subClassOf rdf:resource="http://linked.earth/ontology#Mollusk"/>
        <rdfs:label xml:lang="en">Ostracods</rdfs:label>
    </owl:Class>
    


    <!-- http://linked.earth/ontology#PaleoData -->

    <owl:Class rdf:about="http://linked.earth/ontology#PaleoData">
        <rdfs:subClassOf rdf:resource="http://linked.earth/ontology#Data"/>
        <vann:example rdf:resource="http://wiki.linked.earth/MD982181.Khider.2014.PaleoData1"/>
        <vaem:rationale xml:lang="en">Subdivision between chronological and paleoenvironmental information reflects the fact that Datasets are fundamentally characterized by two distinct components</vaem:rationale>
        <rdfs:comment xml:lang="en">The Data pertaining to past environmental variability</rdfs:comment>
        <rdfs:label xml:lang="en">Paleo data</rdfs:label>
    </owl:Class>
    


    <!-- http://linked.earth/ontology#PaleoDataTable -->

    <owl:Class rdf:about="http://linked.earth/ontology#PaleoDataTable">
        <rdfs:subClassOf rdf:resource="http://linked.earth/ontology#DataTable"/>
        <vann:example rdf:resource="http://wiki.linked.earth/MD982181.Khider.2014.paleo1measurement1"/>
        <vaem:rationale xml:lang="en">Subdivision between chronological and paleoenvironmental information reflects the fact that Datasets are fundamentally characterized by two distinct components</vaem:rationale>
        <rdfs:comment xml:lang="en">DataTable containing PaleoData Variables</rdfs:comment>
        <rdfs:label xml:lang="en">PaleoData table</rdfs:label>
    </owl:Class>
    


    <!-- http://linked.earth/ontology#PaleoModel -->

    <owl:Class rdf:about="http://linked.earth/ontology#PaleoModel">
        <rdfs:subClassOf rdf:resource="http://linked.earth/ontology#Model"/>
        <vann:example rdf:resource="http://wiki.linked.earth/MD982181.Khider.2014.PaleoData1.Model1"/>
        <vaem:rationale xml:lang="en">Subdivision between chronological and paleoenvironmental information reflects the fact that Datasets are fundamentally characterized by two distinct components</vaem:rationale>
        <rdfs:comment xml:lang="en">Model used to derive an environmental axis from the PaleoDataModel</rdfs:comment>
        <rdfs:label xml:lang="en">Paleo model</rdfs:label>
    </owl:Class>
    


    <!-- http://linked.earth/ontology#PaleoProxySystem -->

    <owl:Class rdf:about="http://linked.earth/ontology#PaleoProxySystem">
        <rdfs:subClassOf rdf:resource="http://linked.earth/ontology#ProxySystem"/>
        <vaem:rationale xml:lang="en">Gives a formal definition of climate proxy following the Evans et al. (2013) framework.
Subclass of ProxySystem, pertaining to climate information</vaem:rationale>
        <rdfs:comment xml:lang="en">Climate observations prior to the instrumental era are necessarily indirect. These observations are made on climate proxies in various geological (e.g. lake or marine sediments, living or fossil coral reefs, cave deposits), glaciological (ice cores or snow pits) or biological (trees) archives. Many types of measurements can be made on each archives, each sensing a different aspect of the environment (sometimes, several aspects at once). A paleoclimate dataset is a set of observations made on an archive.</rdfs:comment>
        <rdfs:label xml:lang="en">Paleo proxy system</rdfs:label>
    </owl:Class>
    


    <!-- http://linked.earth/ontology#Peat -->

    <owl:Class rdf:about="http://linked.earth/ontology#Peat">
        <rdfs:subClassOf rdf:resource="http://linked.earth/ontology#ProxyArchive"/>
        <rdfs:label xml:lang="en">Peat </rdfs:label>
    </owl:Class>
    


    <!-- http://linked.earth/ontology#PeerReviewedPublication -->

    <owl:Class rdf:about="http://linked.earth/ontology#PeerReviewedPublication">
        <rdfs:subClassOf rdf:resource="http://linked.earth/ontology#Publication"/>
        <vann:example rdf:resource="http://wiki.linked.earth/Publication.10.1002/2013PA002534"/>
        <vaem:rationale xml:lang="en">Subclass of Publication.Allows to clearly mark datasets generated as part of a peer-reviewed publication.</vaem:rationale>
        <rdfs:comment xml:lang="en">A Publication that has undergone a formal peer-review process</rdfs:comment>
        <rdfs:label xml:lang="en">Peer reviewed publication</rdfs:label>
    </owl:Class>
    


    <!-- http://linked.earth/ontology#Person -->

    <owl:Class rdf:about="http://linked.earth/ontology#Person">
        <owl:equivalentClass rdf:resource="http://schema.org/Person"/>
        <owl:equivalentClass rdf:resource="http://xmlns.com/foaf/0.1/Person"/>
        <vann:example rdf:resource="http://wiki.linked.earth/D._Khider"/>
        <vaem:rationale xml:lang="en">The researcher, author on a publication.</vaem:rationale>
        <rdfs:comment xml:lang="en">An individual who has participated directly or indirectly in the authoring of any resources on the LinkedEarth wiki</rdfs:comment>
        <rdfs:label xml:lang="en">Person</rdfs:label>
    </owl:Class>
    


    <!-- http://linked.earth/ontology#Physical -->

    <owl:Class rdf:about="http://linked.earth/ontology#Physical">
        <rdfs:subClassOf rdf:resource="http://linked.earth/ontology#ProxyObservation"/>
        <rdfs:label xml:lang="en">Physical observation</rdfs:label>
    </owl:Class>
    


    <!-- http://linked.earth/ontology#PhysicalSample -->

    <owl:Class rdf:about="http://linked.earth/ontology#PhysicalSample">
        <vann:example rdf:resource="http://wiki.linked.earth/MD98-2181"/>
        <vaem:rationale xml:lang="en">Used to differentiate between the concept of a ProxyArchive and its physical (real) manifestation</vaem:rationale>
        <rdfs:comment xml:lang="en">The actual sample on which the measurements are made. For instance, the lake core analyzed in the lab is the physical sample.</rdfs:comment>
        <rdfs:label xml:lang="en">Physical sample</rdfs:label>
    </owl:Class>
    


    <!-- http://linked.earth/ontology#Polyp -->

    <owl:Class rdf:about="http://linked.earth/ontology#Polyp">
        <rdfs:subClassOf rdf:resource="http://linked.earth/ontology#OrganicProxySensor"/>
        <rdfs:label xml:lang="en">Polyp</rdfs:label>
    </owl:Class>
    


    <!-- http://linked.earth/ontology#Precipitation -->

    <owl:Class rdf:about="http://linked.earth/ontology#Precipitation">
        <rdfs:subClassOf rdf:resource="http://linked.earth/ontology#Hydrology"/>
        <rdfs:label xml:lang="en">Precipitation</rdfs:label>
    </owl:Class>
    


    <!-- http://linked.earth/ontology#ProxyArchive -->

    <owl:Class rdf:about="http://linked.earth/ontology#ProxyArchive">
        <vann:example rdf:resource="http://wiki.linked.earth/MD982181.Khider.2014.paleo1measurement1.d18omund.MarineSediment"/>
        <vaem:rationale xml:lang="en">&quot;See ProxyArchive ontology for details about the concept. 

We adopted the Evans et al. (2013) framework since this is the only published definition of what is most commonly referred to as &quot;&quot;proxy&quot;&quot; in the paleoclimate community&quot;</vaem:rationale>
        <rdfs:comment xml:lang="en">According to the Evans et al. (2013), the medium in which the response of a ProxySensor to environmental forcing is recorded. Example of archives include: marine sediments, corals, wood, lake sediments, speleothems, glacier ice</rdfs:comment>
        <rdfs:comment xml:lang="en">The medium in which the response of a sensor to environmental forcing is recorded. Sensu Evans et al. (2013).

Examples of archives include: marine sediments, corals, wood, lake sediments, speleothems, glacier ice, etc.</rdfs:comment>
        <rdfs:isDefinedBy rdf:resource="http://www.sciencedirect.com/science/article/pii/S0277379113002011"/>
        <rdfs:label xml:lang="en">Proxy archive</rdfs:label>
    </owl:Class>
    


    <!-- http://linked.earth/ontology#ProxyArchiveModel -->

    <owl:Class rdf:about="http://linked.earth/ontology#ProxyArchiveModel">
        <rdfs:subClassOf rdf:resource="http://linked.earth/ontology#Model"/>
        <vaem:rationale xml:lang="en">We adopted the Evans et al. (2013) framework since this is the only published definition of what is most commonly referred to as &quot;&quot;proxy&quot;&quot; in the paleoclimate community&quot;</vaem:rationale>
        <rdfs:comment xml:lang="en">A Model of how the ProxySensor either creates or emplaces the signal into the ProxyArchive. Sensu Evans et al. (2013)</rdfs:comment>
        <rdfs:isDefinedBy rdf:resource="http://www.sciencedirect.com/science/article/pii/S0277379113002011"/>
        <rdfs:label xml:lang="en">Proxy archive model</rdfs:label>
    </owl:Class>
    


    <!-- http://linked.earth/ontology#ProxyObservation -->

    <owl:Class rdf:about="http://linked.earth/ontology#ProxyObservation">
        <vann:example rdf:resource="http://wiki.linked.earth/D18O"/>
        <vaem:rationale xml:lang="en">See ProxyObservation ontology for details about the concept. 

We adopted the Evans et al. (2013) framework since this is the only published definition of what is most commonly referred to as &quot;&quot;proxy&quot;&quot; in the paleoclimate community</vaem:rationale>
        <rdfs:comment xml:lang="en">The type of MeasuredVariables measured on the ProxyArchive, whether chemical (e.g. Mg/Ca, D18O, Sr/Ca), physical (e.g. density, layer thickness), or biological (e.g. Species abundance)</rdfs:comment>
        <rdfs:isDefinedBy rdf:resource="http://linked.earth/ontology/core/1.2.0/"/>
        <rdfs:isDefinedBy rdf:resource="http://www.sciencedirect.com/science/article/pii/S0277379113002011"/>
        <rdfs:label xml:lang="en">Proxy observation</rdfs:label>
    </owl:Class>
    


    <!-- http://linked.earth/ontology#ProxyObservationModel -->

    <owl:Class rdf:about="http://linked.earth/ontology#ProxyObservationModel">
        <rdfs:subClassOf rdf:resource="http://linked.earth/ontology#Model"/>
        <vaem:rationale xml:lang="en">We adopted the Evans et al. (2013) framework since this is the only published definition of what is most commonly referred to as &quot;&quot;proxy&quot;&quot; in the paleoclimate community</vaem:rationale>
        <rdfs:comment xml:lang="en">The Model of how ProxyObservations are made on the archive. Sensu Evans et al. (2013)</rdfs:comment>
        <rdfs:isDefinedBy rdf:resource="http://www.sciencedirect.com/science/article/pii/S0277379113002011"/>
        <rdfs:label xml:lang="en">Proxy observation model</rdfs:label>
    </owl:Class>
    


    <!-- http://linked.earth/ontology#ProxySensor -->

    <owl:Class rdf:about="http://linked.earth/ontology#ProxySensor">
        <vann:example rdf:resource="http://wiki.linked.earth/Cibicidoides_mundulus"/>
        <vaem:rationale xml:lang="en">See ProxySensor ontology for details about the concept. 

We adopted the Evans et al. (2013) framework since this is the only published definition of what is most commonly referred to as &quot;&quot;proxy&quot;&quot; in the paleoclimate community</vaem:rationale>
        <rdfs:comment xml:lang="en">The sensor comprises physical, chemical, and/or biological components that react to environmental conditions. Sensors often respond to more than one environmental variable, and may have complex responses to the environment they sense, including thresholds (record only part of the range of environmental conditions), seasonal biases (record environmental conditions over a few months of the year), and/or nonlinear responses (Evans et al. (2013))</rdfs:comment>
        <rdfs:comment xml:lang="en">The sensor comprises physical, chemical, and/or biological components that react to environmental conditions. Sensors often respond to more than one environmental variable, and may have complex responses to the environment they sense, including thresholds (record only part of the range of environmental conditions), seasonal biases (record environmental conditions over a few months of the year), and/or nonlinear responses (Evans et al. (2013)). Signals recorded by the ProxySensor are imprinted onto the ProxyArchive.</rdfs:comment>
        <rdfs:isDefinedBy rdf:resource="http://www.sciencedirect.com/science/article/pii/S0277379113002011"/>
        <rdfs:label xml:lang="en">Proxy sensor</rdfs:label>
    </owl:Class>
    


    <!-- http://linked.earth/ontology#ProxySensorModel -->

    <owl:Class rdf:about="http://linked.earth/ontology#ProxySensorModel">
        <rdfs:subClassOf rdf:resource="http://linked.earth/ontology#Model"/>
        <vaem:rationale xml:lang="en">One component of the ProxySystemModel</vaem:rationale>
        <rdfs:comment xml:lang="en">A Model of the ProxySensor. Sensu Evans et al. (2013)</rdfs:comment>
        <rdfs:isDefinedBy rdf:resource="http://www.sciencedirect.com/science/article/pii/S0277379113002011"/>
        <rdfs:label xml:lang="en">Proxy sensor model</rdfs:label>
    </owl:Class>
    


    <!-- http://linked.earth/ontology#ProxySystem -->

    <owl:Class rdf:about="http://linked.earth/ontology#ProxySystem">
        <vann:example rdf:resource="http://wiki.linked.earth/MD982181.Khider.2014.paleo1measurement1.mgcarub.MarineSediment.Globigerinoides_ruber.Mg/Ca"/>
        <vaem:rationale xml:lang="en">We adopted the Evans et al. (2013) framework since this is the only published definition of what is most commonly referred to as &quot;proxy&quot; in the paleoclimate community</vaem:rationale>
        <rdfs:comment xml:lang="en">&lt;p&gt;Climate observations prior to the instrumental era are necessarily indirect. These observations are made on climate &lt;b&gt;proxies&lt;/b&gt; in various geological (e.g. lake or marine sediments, living or fossil coral reefs, cave deposits), glaciological (ice cores or snow pits) or biological (trees) archives. Many types of data can often be collected from each archives, each &lt;b&gt;sensing&lt;/b&gt; a different aspect of the environment (sometimes, several aspects at once).  A paleoclimate dataset is almost always a &lt;a rel=&quot;nofollow&quot; class=&quot;external text&quot; href=&quot;https://en.wikipedia.org/wiki/Time_series&quot;&gt;time series&lt;/a&gt; of observations made on an archive.&lt;/p&gt;
&lt;p&gt;
Evans et al. (2013) &lt;sup id=&quot;cite_ref-evans2013_1-0&quot; class=&quot;reference&quot;&gt;&lt;a href=&quot;#cite_note-evans2013-1&quot;&gt;[1]&lt;/a&gt;&lt;/sup&gt; define a proxy system as comprised of three components (Fig 1).:
&lt;/p&gt;
&lt;ul&gt;&lt;li&gt; The &lt;a href=&quot;#ProxySensor&quot; title=&quot;Category:ProxySensor&quot;&gt; sensor&lt;/a&gt; comprises physical, chemical, and/or biological components that react to environmental conditions. Sensors often respond to more than one environmental &lt;a href=&quot;#InferredVariable&quot; title=&quot;Category:InferredVariable&quot;&gt; variable&lt;/a&gt;, and may have complex responses to the environment they sense, including thresholds  (record only part of the range of environmental conditions), seasonal biases (record environmental conditions over a few months of the year), and/or  nonlinear responses. For instance, &lt;a href=&quot;#Foraminifera&quot; title=&quot;Category:Foraminifera&quot;&gt; foraminifera&lt;/a&gt; are an often used sensor for oceanic conditions. Multiple observations can be made on this sensor, recording different environmental &lt;a href=&quot;#InferredVariable&quot; title=&quot;Category:InferredVariable&quot;&gt; variables&lt;/a&gt;. Similarly, picking foraminifera of a given species to conduct the measurements is part of the observation process, though it does affect the sensor definition&amp;nbsp;: the habitat of these forams determines with environmental &lt;a href=&quot;#InferredVariable&quot; title=&quot;Category:InferredVariable&quot;&gt; variable&lt;/a&gt; (e.g. surface, sub-surface, or thermocline temperature) they are most sensitive to.  &lt;/li&gt;&lt;/ul&gt;
&lt;ul&gt;&lt;li&gt; The &lt;a href=&quot;#ProxyArchive&quot; title=&quot;Category:ProxyArchive &quot;&gt; archive&lt;/a&gt; is the medium in which the response of a sensor to environmental forcing is recorded.  Marine sediments are a type of archive, on which many sensors and observations may be recorded (e.g. Foraminifera Mg/Ca, &lt;sup&gt;18&lt;/sup&gt;O, TEX86)&lt;/li&gt;&lt;/ul&gt;
&lt;ul&gt;&lt;li&gt; &lt;a href=&quot;#ProxyObservation&quot; title=&quot;Category:ProxyObservation&quot;&gt; Observations&lt;/a&gt; are made on archives and are  generally referred to as &quot;proxies&quot;. The term &quot;proxy&quot; used ubiquitously, and often ambiguously, throughout the paleoclimate literature, is most commonly equivalent to &quot;sensor + observation&quot;. &quot;Observation&quot; is the more explicit, and thus, preferred term, however &quot;proxy&quot; can be treated as a synonym of &quot;observation&quot;. For instance, Foraminifera Mg/Ca is often used to investigate past changes in sea-surface temperature but depends also on sea-surface salinity and deep-ocean carbonate saturation &lt;sup id=&quot;cite_ref-2&quot; class=&quot;reference&quot;&gt;&lt;a href=&quot;#cite_note-2&quot;&gt;[2]&lt;/a&gt;&lt;/sup&gt;.  Furthermore, its temperature and salinity dependence is exponential &lt;sup id=&quot;cite_ref-3&quot; class=&quot;reference&quot;&gt;&lt;a href=&quot;#cite_note-3&quot;&gt;[3]&lt;/a&gt;&lt;/sup&gt; &lt;sup id=&quot;cite_ref-4&quot; class=&quot;reference&quot;&gt;&lt;a href=&quot;#cite_note-4&quot;&gt;[4]&lt;/a&gt;&lt;/sup&gt; &lt;sup id=&quot;cite_ref-5&quot; class=&quot;reference&quot;&gt;&lt;a href=&quot;#cite_note-5&quot;&gt;[5]&lt;/a&gt;&lt;/sup&gt; while its response to carbonate saturation is thresholded &lt;sup id=&quot;cite_ref-6&quot; class=&quot;reference&quot;&gt;&lt;a href=&quot;#cite_note-6&quot;&gt;[6]&lt;/a&gt;&lt;/sup&gt;.  &lt;/li&gt;&lt;/ul&gt;

&lt;p&gt;These three major components may be individually modeled, and linked together within a &lt;a href=&quot;/Category:ProxySystemModel_%C2%A9&quot; title=&quot;Category:ProxySystemModel &quot;&gt;Proxy System Model&lt;/a&gt; &lt;sup id=&quot;cite_ref-evans2013_1-2&quot; class=&quot;reference&quot;&gt;&lt;a href=&quot;#cite_note-evans2013-1&quot;&gt;[1]&lt;/a&gt;&lt;/sup&gt; &lt;sup id=&quot;cite_ref-7&quot; class=&quot;reference&quot;&gt;&lt;a href=&quot;#cite_note-7&quot;&gt;[7]&lt;/a&gt;&lt;/sup&gt;. Some sensors are common to multiple archives (e.g. &lt;sup&gt;18&lt;/sup&gt;O), and all archives support more than one possible sensor. 
&lt;/p&gt;

&lt;h2&gt;&lt;span class=&quot;mw-headline&quot; id=&quot;References&quot;&gt;References&lt;/span&gt;&lt;/h2&gt;

&lt;ol class=&quot;references&quot;&gt;
&lt;li id=&quot;cite_note-evans2013-1&quot;&gt;&lt;span class=&quot;mw-cite-backlink&quot;&gt; &lt;sup&gt;&lt;a href=&quot;#cite_ref-evans2013_1-0&quot;&gt;&lt;span class=&quot;cite-accessibility-label&quot;&gt;Jump up to: &lt;/span&gt;1.0&lt;/a&gt;&lt;/sup&gt; &lt;sup&gt;&lt;a href=&quot;#cite_ref-evans2013_1-1&quot;&gt;1.1&lt;/a&gt;&lt;/sup&gt; &lt;sup&gt;&lt;a href=&quot;#cite_ref-evans2013_1-2&quot;&gt;1.2&lt;/a&gt;&lt;/sup&gt;&lt;/span&gt; &lt;span class=&quot;reference-text&quot;&gt; Evans, M. N., Tolwinski-Ward, S. E., Thompson, D. M., &amp;amp; Anchukaitis, K. J. (2013). Applications of proxy system modeling in high resolution paleoclimatology. Quaternary Science Reviews, 76, 16-28. doi:10.1016/j.quascirev.2013.05.024 &lt;/span&gt;
&lt;/li&gt;
&lt;li id=&quot;cite_note-2&quot;&gt;&lt;span class=&quot;mw-cite-backlink&quot;&gt;&lt;a href=&quot;#cite_ref-2&quot;&gt;&lt;span class=&quot;cite-accessibility-label&quot;&gt;Jump up &lt;/span&gt;&lt;/a&gt;&lt;/span&gt; &lt;span class=&quot;reference-text&quot;&gt; Khider, D., Huerta, G., Jackson, C., Stott, L. D., &amp;amp; Emile-Geay, J. (2015). A Bayesian, multivariate calibration for Globigerinoides ruber Mg/Ca. Geochemistry Geophysics Geosystems, 16(9), 2916-2932. doi:10.1002/2015GC005844 &lt;/span&gt;
&lt;/li&gt;
&lt;li id=&quot;cite_note-3&quot;&gt;&lt;span class=&quot;mw-cite-backlink&quot;&gt;&lt;a href=&quot;#cite_ref-3&quot;&gt;&lt;span class=&quot;cite-accessibility-label&quot;&gt;Jump up &lt;/span&gt;&lt;/a&gt;&lt;/span&gt; &lt;span class=&quot;reference-text&quot;&gt; Anand, P., Elderfield, H., &amp;amp; Conte, M. H. (2003). Calibration of Mg/Ca thermometry in planktonic foraminifera from a sediment trap time series. Paleoceanography, 18(2), 1050. doi:10.1029/2002PA000846 &lt;/span&gt;
&lt;/li&gt;
&lt;li id=&quot;cite_note-4&quot;&gt;&lt;span class=&quot;mw-cite-backlink&quot;&gt;&lt;a href=&quot;#cite_ref-4&quot;&gt;&lt;span class=&quot;cite-accessibility-label&quot;&gt;Jump up &lt;/span&gt;&lt;/a&gt;&lt;/span&gt; &lt;span class=&quot;reference-text&quot;&gt; Lea, D. W., Mashiotta, T. A., &amp;amp; Spero, H. J. (1999). Controls on magnesium and strontium uptake in planktonic foraminifera determined by live culturing. Geochimica et cosmochimica acta, 63(16), 2369-2379. &lt;/span&gt;
&lt;/li&gt;
&lt;li id=&quot;cite_note-5&quot;&gt;&lt;span class=&quot;mw-cite-backlink&quot;&gt;&lt;a href=&quot;#cite_ref-5&quot;&gt;&lt;span class=&quot;cite-accessibility-label&quot;&gt;Jump up &lt;/span&gt;&lt;/a&gt;&lt;/span&gt; &lt;span class=&quot;reference-text&quot;&gt; Kisakrek, B., Eisenhauer, A., Bhm, F., Garbe-Schnberg, D., &amp;amp; Erez, J. (2008). Controls on shell Mg/Ca and Sr/Ca in cultured planktonic foraminiferan, Globigeriniodes ruber (white). Earth and Planetary Science Letters, 273, 260-269. doi:10.1016/j.epsl.2008.06.026 &lt;/span&gt;
&lt;/li&gt;
&lt;li id=&quot;cite_note-6&quot;&gt;&lt;span class=&quot;mw-cite-backlink&quot;&gt;&lt;a href=&quot;#cite_ref-6&quot;&gt;&lt;span class=&quot;cite-accessibility-label&quot;&gt;Jump up &lt;/span&gt;&lt;/a&gt;&lt;/span&gt; &lt;span class=&quot;reference-text&quot;&gt; Regenberg, M., Regenberg, A., Garbe-Schonberg, D., &amp;amp; Lea, D. W. (2014). Global dissolution effects on planktonic foraminiferal Mg/Ca ratios controlled by the calcite-saturation state of bottom waters. Paleoceanography, 29, 127-142. doi:10.1002/2013PA002492 &lt;/span&gt;
&lt;/li&gt;
&lt;li id=&quot;cite_note-7&quot;&gt;&lt;span class=&quot;mw-cite-backlink&quot;&gt;&lt;a href=&quot;#cite_ref-7&quot;&gt;&lt;span class=&quot;cite-accessibility-label&quot;&gt;Jump up &lt;/span&gt;&lt;/a&gt;&lt;/span&gt; &lt;span class=&quot;reference-text&quot;&gt; Dee, S., Emile-Geay, J., Evans, M. N., Allam, A., Steig, E. J., &amp;amp; Thompson, D. M. (2015). PRYSM: An open-source framework  for PRoxy System Modeling, with applications to oxygen-isotope systems. Journal of Advances in Modeling Earth Systems, 7, 1220-1247. doi:10.1002/2015MS000447&lt;/span&gt;
&lt;/li&gt;
&lt;/ol&gt;</rdfs:comment>
        <rdfs:isDefinedBy rdf:resource="http://www.sciencedirect.com/science/article/pii/S0277379113002011"/>
        <rdfs:label xml:lang="en">Proxy system</rdfs:label>
    </owl:Class>
    


    <!-- http://linked.earth/ontology#ProxySystemModel -->

    <owl:Class rdf:about="http://linked.earth/ontology#ProxySystemModel">
        <rdfs:subClassOf rdf:resource="http://linked.earth/ontology#Model"/>
        <vaem:rationale xml:lang="en">We adopted the Evans et al. (2013) framework since this is the only published definition of what is most commonly referred to as &quot;proxy&quot; in the paleoclimate community</vaem:rationale>
        <rdfs:comment xml:lang="en">In the Evans et al. (2013) framework, this is the combination of sensor, archive and observation models . &quot;A generalized proxy system model encapuslates a simplified representation of prior physical, chemical, biological, and/or geological understanding of the ways in which environmental variation ultimately results in the observations used to retrieve paleoclimatic information.&quot;</rdfs:comment>
        <rdfs:isDefinedBy rdf:resource="http://www.sciencedirect.com/science/article/pii/S0277379113002011"/>
        <rdfs:label xml:lang="en">Proxy system model</rdfs:label>
    </owl:Class>
    


    <!-- http://linked.earth/ontology#Publication -->

    <owl:Class rdf:about="http://linked.earth/ontology#Publication">
        <vann:example rdf:resource="http://wiki.linked.earth/Publication.10.1029/2012GC004293"/>
        <vaem:rationale xml:lang="en">Can be used to credit the contributor of the dataset as well as linking toward the conclusions of the study and relevant methods</vaem:rationale>
        <rdfs:comment xml:lang="en">A document that serves as reference for a Dataset or its components</rdfs:comment>
        <rdfs:label xml:lang="en">Publication</rdfs:label>
    </owl:Class>
    


    <!-- http://linked.earth/ontology#Radioisotope -->

    <owl:Class rdf:about="http://linked.earth/ontology#Radioisotope">
        <rdfs:subClassOf rdf:resource="http://linked.earth/ontology#Isotope"/>
        <rdfs:label xml:lang="en">Radioisotope</rdfs:label>
    </owl:Class>
    


    <!-- http://linked.earth/ontology#Reflectance -->

    <owl:Class rdf:about="http://linked.earth/ontology#Reflectance">
        <rdfs:subClassOf rdf:resource="http://linked.earth/ontology#Spectral"/>
        <rdfs:label xml:lang="en">Reflectance</rdfs:label>
    </owl:Class>
    


    <!-- http://linked.earth/ontology#Resolution -->

    <owl:Class rdf:about="http://linked.earth/ontology#Resolution">
        <vaem:rationale xml:lang="en">Class added to describe the annual resolution of the archives</vaem:rationale>
        <rdfs:comment xml:lang="en">Refers to the time difference between two adjacent values of a Variable.</rdfs:comment>
        <rdfs:label xml:lang="en">Resolution</rdfs:label>
    </owl:Class>
    


    <!-- http://linked.earth/ontology#Rock -->

    <owl:Class rdf:about="http://linked.earth/ontology#Rock">
        <rdfs:subClassOf rdf:resource="http://linked.earth/ontology#InorganicProxySensor"/>
        <rdfs:subClassOf rdf:resource="http://linked.earth/ontology#ProxyArchive"/>
        <rdfs:label xml:lang="en">Rock</rdfs:label>
    </owl:Class>
    


    <!-- http://linked.earth/ontology#RockHammer -->

    <owl:Class rdf:about="http://linked.earth/ontology#RockHammer">
        <rdfs:subClassOf rdf:resource="http://linked.earth/ontology#Instrument"/>
        <rdfs:label xml:lang="en">Rock hammer</rdfs:label>
    </owl:Class>
    


    <!-- http://linked.earth/ontology#SHRIMP -->

    <owl:Class rdf:about="http://linked.earth/ontology#SHRIMP">
        <rdfs:subClassOf rdf:resource="http://linked.earth/ontology#SecondaryIonMassSpectrometer"/>
        <rdfs:label xml:lang="en">Sensitive high-resolution ion microprobe</rdfs:label>
    </owl:Class>
    


    <!-- http://linked.earth/ontology#SIMS -->

    <owl:Class rdf:about="http://linked.earth/ontology#SIMS">
        <rdfs:subClassOf rdf:resource="http://linked.earth/ontology#SecondaryIonMassSpectrometer"/>
        <rdfs:label xml:lang="en">Secondary ion mass spectrometer</rdfs:label>
    </owl:Class>
    


    <!-- http://linked.earth/ontology#Sclerosponge -->

    <owl:Class rdf:about="http://linked.earth/ontology#Sclerosponge">
        <rdfs:subClassOf rdf:resource="http://linked.earth/ontology#ProxyArchive"/>
        <rdfs:label xml:lang="en">Sclerosponge</rdfs:label>
    </owl:Class>
    


    <!-- http://linked.earth/ontology#SecondaryIonMassSpectrometer -->

    <owl:Class rdf:about="http://linked.earth/ontology#SecondaryIonMassSpectrometer">
        <rdfs:subClassOf rdf:resource="http://linked.earth/ontology#MassSpectrometer"/>
        <rdfs:label xml:lang="en">Secondary ion mass spectrometer</rdfs:label>
    </owl:Class>
    


    <!-- http://linked.earth/ontology#Snow -->

    <owl:Class rdf:about="http://linked.earth/ontology#Snow">
        <rdfs:subClassOf rdf:resource="http://linked.earth/ontology#InorganicProxySensor"/>
        <rdfs:label xml:lang="en">Snow</rdfs:label>
    </owl:Class>
    


    <!-- http://linked.earth/ontology#SoftwareCode -->

    <owl:Class rdf:about="http://linked.earth/ontology#SoftwareCode">
        <rdfs:subClassOf rdf:resource="http://ontosoft.org/software#Software"/>
        <vann:example rdf:resource="http://wiki.linked.earth/Pyleoclim"/>
        <vaem:rationale xml:lang="en">Added to allow for a link towards the code if on a public repository like GitHub</vaem:rationale>
        <rdfs:comment xml:lang="en">A script that describes the model, in any programming language (e.g., Excel, Matlab, Python, R)</rdfs:comment>
        <rdfs:label xml:lang="en">Software code</rdfs:label>
    </owl:Class>
    


    <!-- http://linked.earth/ontology#Spectral -->

    <owl:Class rdf:about="http://linked.earth/ontology#Spectral">
        <rdfs:subClassOf rdf:resource="http://linked.earth/ontology#ProxyObservation"/>
        <rdfs:label xml:lang="en">Spectral observation</rdfs:label>
    </owl:Class>
    


    <!-- http://linked.earth/ontology#Spectrometer -->

    <owl:Class rdf:about="http://linked.earth/ontology#Spectrometer">
        <rdfs:subClassOf rdf:resource="http://linked.earth/ontology#Instrument"/>
        <rdfs:label xml:lang="en">Spectrometer</rdfs:label>
    </owl:Class>
    


    <!-- http://linked.earth/ontology#Spectroscope -->

    <owl:Class rdf:about="http://linked.earth/ontology#Spectroscope">
        <rdfs:subClassOf rdf:resource="http://linked.earth/ontology#Instrument"/>
        <rdfs:label xml:lang="en">Spectroscope</rdfs:label>
    </owl:Class>
    


    <!-- http://linked.earth/ontology#Speleothem -->

    <owl:Class rdf:about="http://linked.earth/ontology#Speleothem">
        <rdfs:subClassOf rdf:resource="http://linked.earth/ontology#ProxyArchive"/>
        <rdfs:label xml:lang="en">Speleothem</rdfs:label>
    </owl:Class>
    


    <!-- http://linked.earth/ontology#StableCarbonIsotope -->

    <owl:Class rdf:about="http://linked.earth/ontology#StableCarbonIsotope">
        <rdfs:subClassOf rdf:resource="http://linked.earth/ontology#StableIsotope"/>
        <rdfs:comment xml:lang="en">&lt;p&gt;&lt;a rel=&quot;nofollow&quot; class=&quot;external text&quot; href=&quot;https://en.wikipedia.org/wiki/Carbon&quot;&gt;Carbon&lt;/a&gt; in nature exists in oxidized (i.e., &lt;a rel=&quot;nofollow&quot; class=&quot;external text&quot; href=&quot;https://en.wikipedia.org/wiki/Carbon_dioxide&quot;&gt;CO&lt;sub&gt;2&lt;/sub&gt;&lt;/a&gt; and &lt;a rel=&quot;nofollow&quot; class=&quot;external text&quot; href=&quot;https://en.wikipedia.org/wiki/Carbonate&quot;&gt;carbonates&lt;/a&gt;), elemental (i.e., &lt;a rel=&quot;nofollow&quot; class=&quot;external text&quot; href=&quot;https://en.wikipedia.org/wiki/Graphite&quot;&gt;graphite&lt;/a&gt; and &lt;a rel=&quot;nofollow&quot; class=&quot;external text&quot; href=&quot;https://en.wikipedia.org/wiki/Diamond&quot;&gt;diamond&lt;/a&gt;), and reduced (i.e., &lt;a rel=&quot;nofollow&quot; class=&quot;external text&quot; href=&quot;https://en.wikipedia.org/wiki/Methane&quot;&gt;methane&lt;/a&gt; and organic matter]) forms. Carbon has two &lt;a href=&quot;/Category:StableIsotope&quot; title=&quot;Category:StableIsotope&quot;&gt; stable isotopes&lt;/a&gt;: the light isotope &lt;sup&gt;12&lt;/sup&gt;C (abundance: 98.9%, mass: 12.000000 amu) and the heavy isotope &lt;sup&gt;13&lt;/sup&gt;C (abundance: 1.1%, mass: 13.003355 amu). Since the mass of &lt;sup&gt;13&lt;/sup&gt;C is higher than the mass of &lt;sup&gt;12&lt;/sup&gt;C, the carbon isotopes are fractionated by chemical and biological processes. In general, &lt;sup&gt;12&lt;/sup&gt;C is strongly partitioned into organic matter (reduced form) while the heavy isotope is concentrated in the oxidized forms of carbon.
&lt;/p&gt;</rdfs:comment>
        <rdfs:label xml:lang="en">Stable Carbon isotope</rdfs:label>
    </owl:Class>
    


    <!-- http://linked.earth/ontology#StableHydrogenIsotope -->

    <owl:Class rdf:about="http://linked.earth/ontology#StableHydrogenIsotope">
        <rdfs:subClassOf rdf:resource="http://linked.earth/ontology#StableIsotope"/>
        <rdfs:label xml:lang="en">Stable Hydrogen isotope</rdfs:label>
    </owl:Class>
    


    <!-- http://linked.earth/ontology#StableIsotope -->

    <owl:Class rdf:about="http://linked.earth/ontology#StableIsotope">
        <rdfs:subClassOf rdf:resource="http://linked.earth/ontology#Isotope"/>
        <rdfs:label xml:lang="en">Stable isotope</rdfs:label>
    </owl:Class>
    


    <!-- http://linked.earth/ontology#StableNitrogenIsotope -->

    <owl:Class rdf:about="http://linked.earth/ontology#StableNitrogenIsotope">
        <rdfs:subClassOf rdf:resource="http://linked.earth/ontology#StableIsotope"/>
        <rdfs:label xml:lang="en">Stable Nitrogen isotope</rdfs:label>
    </owl:Class>
    


    <!-- http://linked.earth/ontology#StableOxygenIsotope -->

    <owl:Class rdf:about="http://linked.earth/ontology#StableOxygenIsotope">
        <rdfs:subClassOf rdf:resource="http://linked.earth/ontology#StableIsotope"/>
        <rdfs:label xml:lang="en">Stable Oxygen isotope</rdfs:label>
    </owl:Class>
    


    <!-- http://linked.earth/ontology#StableSulfurIsotope -->

    <owl:Class rdf:about="http://linked.earth/ontology#StableSulfurIsotope">
        <rdfs:subClassOf rdf:resource="http://linked.earth/ontology#StableIsotope"/>
        <rdfs:label xml:lang="en">Stable sulfur isotope</rdfs:label>
    </owl:Class>
    


    <!-- http://linked.earth/ontology#SummaryTable -->

    <owl:Class rdf:about="http://linked.earth/ontology#SummaryTable">
        <rdfs:subClassOf rdf:resource="http://linked.earth/ontology#DataTable"/>
        <vann:example rdf:resource="http://wiki.linked.earth/MD982181.Khider.2014.paleo1model1summary1"/>
        <vaem:rationale xml:lang="en">Allows to represent a summary of basic statistics such as median, mean, standard deviation, and various quantiles from the output of the Model</vaem:rationale>
        <rdfs:comment xml:lang="en">A DataTable that contains summary information for the Variable and is output from a Model.</rdfs:comment>
        <rdfs:label xml:lang="en">Summary table</rdfs:label>
    </owl:Class>
    


    <!-- http://linked.earth/ontology#Temperature -->

    <owl:Class rdf:about="http://linked.earth/ontology#Temperature">
        <rdfs:subClassOf rdf:resource="http://linked.earth/ontology#InferredVariable"/>
        <rdfs:comment xml:lang="en">Thermodynamic property allowing to quantitatively measure how warm or cold a material, fluid is.</rdfs:comment>
        <rdfs:label xml:lang="en">Temperature</rdfs:label>
    </owl:Class>
    


    <!-- http://linked.earth/ontology#Time -->

    <owl:Class rdf:about="http://linked.earth/ontology#Time">
        <rdfs:subClassOf rdf:resource="http://linked.earth/ontology#InferredVariable"/>
        <rdfs:label xml:lang="en">Time</rdfs:label>
    </owl:Class>
    


    <!-- http://linked.earth/ontology#TraceElement -->

    <owl:Class rdf:about="http://linked.earth/ontology#TraceElement">
        <rdfs:subClassOf rdf:resource="http://linked.earth/ontology#Chemical"/>
        <rdfs:label xml:lang="en">Trace element</rdfs:label>
    </owl:Class>
    


    <!-- http://linked.earth/ontology#Tree -->

    <owl:Class rdf:about="http://linked.earth/ontology#Tree">
        <rdfs:subClassOf rdf:resource="http://linked.earth/ontology#OrganicProxySensor"/>
        <rdfs:isDefinedBy rdf:resource="http://wiki.linked.earth/Tree"/>
        <rdfs:label xml:lang="en">Tree</rdfs:label>
    </owl:Class>
    


    <!-- http://linked.earth/ontology#Uncertainty -->

    <owl:Class rdf:about="http://linked.earth/ontology#Uncertainty">
        <vann:example rdf:resource="http://wiki.linked.earth/MD982181.Khider.2014.paleo1measurement1.mgcarub.Uncertainty"/>
        <vann:example rdf:resource="http://wiki.linked.earth/MD982181.Khider.2014.paleo1measurement2.sst.Uncertainty"/>
        <vaem:rationale xml:lang="en">To allow to describe the uncertainty on a Variable or a Model, would it be a single number (e.g., the uncertainty on the measurements are 0.1 per mil, one sigma confidence level, or reportedIn an EnsembleTable and/or SummaryTable)</vaem:rationale>
        <rdfs:comment xml:lang="en">A state of incomplete knowledge that results from a lack of information or from different modeling choices. Uncertainty may come from many sources, from imprecision in the data to ambigously defined concepts or terminology. Uncertainty can be represented by quantitative measures (e.g., probability density function) or by qualitative statements (e.g., reflecting the judgement of a team of experts). Sensu IPCC AR5</rdfs:comment>
        <rdfs:isDefinedBy rdf:resource="https://www.ipcc.ch/pdf/assessment-report/ar5/wg1/WG1AR5_AnnexIII_FINAL.pdf"/>
        <rdfs:label xml:lang="en">Uncertainty</rdfs:label>
    </owl:Class>
    


    <!-- http://linked.earth/ontology#UncertaintyModel -->

    <owl:Class rdf:about="http://linked.earth/ontology#UncertaintyModel">
        <rdfs:subClassOf rdf:resource="http://linked.earth/ontology#Model"/>
        <vaem:rationale xml:lang="en">Allows description of how uncertainty was calculated</vaem:rationale>
        <rdfs:comment xml:lang="en">A Model quantifiying the Uncertainty</rdfs:comment>
        <rdfs:label xml:lang="en">Uncertainty model</rdfs:label>
    </owl:Class>
    


    <!-- http://linked.earth/ontology#Variable -->

    <owl:Class rdf:about="http://linked.earth/ontology#Variable">
        <vaem:rationale rdf:resource="http://wiki.linked.earth/MD982181.Khider.2014.paleo1measurement2.sst"/>
        <vaem:rationale xml:lang="en">Basic definition of the values in the columns of the csv file</vaem:rationale>
        <rdfs:comment xml:lang="en">Quantities that may change from value to value. They are usually represented as column of values in a data table</rdfs:comment>
        <rdfs:label xml:lang="en">Variable</rdfs:label>
    </owl:Class>
    


    <!-- http://linked.earth/ontology#Vegetation -->

    <owl:Class rdf:about="http://linked.earth/ontology#Vegetation">
        <rdfs:subClassOf rdf:resource="http://linked.earth/ontology#OrganicProxySensor"/>
        <rdfs:label xml:lang="en">Vegetation</rdfs:label>
    </owl:Class>
    


    <!-- http://linked.earth/ontology#Watershed -->

    <owl:Class rdf:about="http://linked.earth/ontology#Watershed">
        <rdfs:subClassOf rdf:resource="http://linked.earth/ontology#InorganicProxySensor"/>
        <rdfs:label xml:lang="en">Watershed</rdfs:label>
    </owl:Class>
    


    <!-- http://linked.earth/ontology#WavelengthDispersiveSpectrometer -->

    <owl:Class rdf:about="http://linked.earth/ontology#WavelengthDispersiveSpectrometer">
        <rdfs:subClassOf rdf:resource="http://linked.earth/ontology#Spectrometer"/>
        <rdfs:label xml:lang="en">Wavelength dispersive spectrometry</rdfs:label>
    </owl:Class>
    


    <!-- http://linked.earth/ontology#Wood -->

    <owl:Class rdf:about="http://linked.earth/ontology#Wood">
        <rdfs:subClassOf rdf:resource="http://linked.earth/ontology#ProxyArchive"/>
        <rdfs:comment xml:lang="en">&lt;p&gt;The field of &lt;a rel=&quot;nofollow&quot; class=&quot;external text&quot; href=&quot;https://en.wikipedia.org/wiki/Dendroclimatology&quot;&gt;dendroclimatology&lt;/a&gt; and, to some extent, the field of &lt;a href=&quot;/Dendrochronology&quot; title=&quot;Dendrochronology&quot;&gt; dendrochronology&lt;/a&gt; have played an important role in generating climate reconstructions of the past millennium &lt;sup id=&quot;cite_ref-1&quot; class=&quot;reference&quot;&gt;&lt;a href=&quot;#cite_note-1&quot;&gt;[1]&lt;/a&gt;&lt;/sup&gt; &lt;sup id=&quot;cite_ref-2&quot; class=&quot;reference&quot;&gt;&lt;a href=&quot;#cite_note-2&quot;&gt;[2]&lt;/a&gt;&lt;/sup&gt; &lt;sup id=&quot;cite_ref-3&quot; class=&quot;reference&quot;&gt;&lt;a href=&quot;#cite_note-3&quot;&gt;[3]&lt;/a&gt;&lt;/sup&gt; &lt;sup id=&quot;cite_ref-4&quot; class=&quot;reference&quot;&gt;&lt;a href=&quot;#cite_note-4&quot;&gt;[4]&lt;/a&gt;&lt;/sup&gt;. In regions with large seasonal variations, trees produce rings of varying color depending on the species. In most cases, the rings shift from a lighter, low density early wood of spring and early summer to a darker, denser band of late wood at the end of the growing season. The growing season generally occurs during the summer month and its length depends on the species, latitude, and altitude. Therefore, trees  hold perhaps the greatest potential for reconstructing past terrestrial climates at annual or even sub-annual resolution. 
&lt;/p&gt;&lt;p&gt;The following observations can be made on the wood archive:
&lt;/p&gt;
&lt;ul&gt;&lt;li&gt; Tree ring width&lt;/li&gt;
&lt;li&gt; Wood density&lt;/li&gt;
&lt;li&gt; Stables isotopes&lt;ol class=&quot;references&quot;&gt;&lt;/li&gt;&lt;/ul&gt;&lt;ol&gt;
&lt;li id=&quot;cite_note-1&quot;&gt;&lt;span class=&quot;mw-cite-backlink&quot;&gt;&lt;a href=&quot;#cite_ref-1&quot;&gt;?&lt;/a&gt;&lt;/span&gt; &lt;span class=&quot;reference-text&quot;&gt; Mann, M. E., Bradley, R. S., &amp;amp; Hughes, M. K. (1998). Global-scale temperature patterns and climate forcing over the past six centuries. Nature, 392(6678), 779-787. doi:10.1038/33859 &lt;/span&gt;
&lt;/li&gt;
&lt;li id=&quot;cite_note-2&quot;&gt;&lt;span class=&quot;mw-cite-backlink&quot;&gt;&lt;a href=&quot;#cite_ref-2&quot;&gt;?&lt;/a&gt;&lt;/span&gt; &lt;span class=&quot;reference-text&quot;&gt;Mann, M. E., Bradley, R. S., &amp;amp; Hughes, M. K. (1999). Northern Hemipshere temperatures during the past millennium: Inferences, Uncertainties, and Limitations. Geophysical Research Letters, 26(6), 759. &lt;/span&gt;
&lt;/li&gt;
&lt;li id=&quot;cite_note-3&quot;&gt;&lt;span class=&quot;mw-cite-backlink&quot;&gt;&lt;a href=&quot;#cite_ref-3&quot;&gt;?&lt;/a&gt;&lt;/span&gt; &lt;span class=&quot;reference-text&quot;&gt;Moberg, A., Sonechkin, D. M., Holmgren, K., Datsenko, N. M., &amp;amp; Karlen, W. (2005). Highly variable Northern Hemisphere temperatures reconstructed from low- and high-resolution proxy data. Nature, 433(7026), 613-617. doi:10.1038/nature03265&lt;/span&gt;
&lt;/li&gt;
&lt;li id=&quot;cite_note-4&quot;&gt;&lt;span class=&quot;mw-cite-backlink&quot;&gt;&lt;a href=&quot;#cite_ref-4&quot;&gt;?&lt;/a&gt;&lt;/span&gt; &lt;span class=&quot;reference-text&quot;&gt;Mann, M. E., Zhang, Z., Rutherford, S., Bradley, R., Hughes, M. K., Shindell, D. T., . . . Ni, F. (2009). Global signatures and dynamical origins of the Little Ice Age and Medieval Climate Anomaly. Science, 326, 1256-1260. dos: 10.1126/science.1177303&lt;/span&gt;
&lt;/li&gt;
&lt;/ol&gt;</rdfs:comment>
        <rdfs:label xml:lang="en">Wood</rdfs:label>
    </owl:Class>
    


    <!-- http://linked.earth/ontology#ZeissPetrographicMicroscope -->

    <owl:Class rdf:about="http://linked.earth/ontology#ZeissPetrographicMicroscope">
        <rdfs:subClassOf rdf:resource="http://linked.earth/ontology#Microscope"/>
        <rdfs:label xml:lang="en">Zeiss petrographic microscope</rdfs:label>
    </owl:Class>
    


    <!-- http://ontosoft.org/software#Software -->

    <owl:Class rdf:about="http://ontosoft.org/software#Software">
        <rdfs:isDefinedBy rdf:resource="http://ontosoft.org/software#"/>
    </owl:Class>
    


    <!-- http://purl.oclc.org/NET/ssnx/ssn#Observation -->

    <owl:Class rdf:about="http://purl.oclc.org/NET/ssnx/ssn#Observation">
        <rdfs:comment xml:lang="en">The class ssn:Observation provides the structure to represent a single observation. An observation is a situation that describes an observed feature, an observed property, a sensor and method of sensing used and a value observed for the property: that is, an observation describes a single value attributed to a single property by a particular sensor. Observations of multiple features or multiple properties of the one feature should be represented as either compound properties, features and values or as multiple observations, grouped in some appropriate structure.</rdfs:comment>
        <rdfs:isDefinedBy rdf:resource="http://purl.oclc.org/NET/ssnx/ssn"/>
    </owl:Class>
    


    <!-- http://schema.org/DataCatalog -->

    <owl:Class rdf:about="http://schema.org/DataCatalog">
        <rdfs:isDefinedBy rdf:resource="http://schema.org/"/>
    </owl:Class>
    


    <!-- http://schema.org/Dataset -->

    <owl:Class rdf:about="http://schema.org/Dataset">
        <rdfs:isDefinedBy rdf:resource="http://schema.org/"/>
    </owl:Class>
    


    <!-- http://schema.org/Person -->

    <owl:Class rdf:about="http://schema.org/Person">
        <rdfs:isDefinedBy rdf:resource="http://schema.org/"/>
    </owl:Class>
    


    <!-- http://schema.org/Place -->

    <owl:Class rdf:about="http://schema.org/Place">
        <rdfs:isDefinedBy rdf:resource="http://schema.org/"/>
    </owl:Class>
    


    <!-- http://www.opengis.net/ont/geosparql#Feature -->

    <owl:Class rdf:about="http://www.opengis.net/ont/geosparql#Feature">
        <rdfs:isDefinedBy rdf:resource="http://www.opengis.net/ont/geosparql"/>
    </owl:Class>
    


    <!-- http://www.opengis.net/ont/geosparql#Geometry -->

    <owl:Class rdf:about="http://www.opengis.net/ont/geosparql#Geometry">
        <rdfs:isDefinedBy rdf:resource="http://www.opengis.net/spec/geosparql/1.0"/>
    </owl:Class>
    


    <!-- http://www.w3.org/2003/01/geo/wgs84_pos#SpatialThing -->

    <owl:Class rdf:about="http://www.w3.org/2003/01/geo/wgs84_pos#SpatialThing">
        <rdfs:isDefinedBy rdf:resource="http://www.w3.org/2003/01/geo/wgs84_pos#"/>
    </owl:Class>
    


    <!-- http://xmlns.com/foaf/0.1/Person -->

    <owl:Class rdf:about="http://xmlns.com/foaf/0.1/Person">
        <rdfs:isDefinedBy rdf:resource="http://xmlns.com/foaf/0.1/"/>
    </owl:Class>
    


    <!-- 
    ///////////////////////////////////////////////////////////////////////////////////////
    //
    // Individuals
    //
    ///////////////////////////////////////////////////////////////////////////////////////
     -->

    


    <!-- http://earth.usc.edu/~khider/ -->

    <owl:NamedIndividual rdf:about="http://earth.usc.edu/~khider/"/>
    


    <!-- http://linked.earth/ontology# -->

    <owl:NamedIndividual rdf:about="http://linked.earth/ontology#">
        <dcterms:contributor rdf:resource="http://w3id.org/people/dgarijo"/>
        <dcterms:contributor rdf:resource="http://www.isi.edu/~gil/"/>
        <dcterms:creator rdf:resource="http://earth.usc.edu/~khider/"/>
        <dcterms:creator rdf:resource="http://orcid.org/0000-0001-5920-4751"/>
        <dcterms:creator rdf:resource="http://www.cefns.nau.edu/~npm4/"/>
        <dcterms:license>http://creativecommons.org/licenses/by/2.0/</dcterms:license>
        <dcterms:title xml:lang="en">The Linked Earth Ontology</dcterms:title>
    </owl:NamedIndividual>
    


    <!-- http://linked.earth/ontology#Ar-Ar -->

    <owl:NamedIndividual rdf:about="http://linked.earth/ontology#Ar-Ar">
        <rdf:type rdf:resource="http://linked.earth/ontology#Radioisotope"/>
        <rdfs:label xml:lang="en">Ar-Ar</rdfs:label>
    </owl:NamedIndividual>
    


    <!-- http://linked.earth/ontology#C -->

    <owl:NamedIndividual rdf:about="http://linked.earth/ontology#C">
        <rdf:type rdf:resource="http://linked.earth/ontology#MajorElement"/>
        <rdfs:label xml:lang="en">C</rdfs:label>
    </owl:NamedIndividual>
    


    <!-- http://linked.earth/ontology#CarbonateIonConcentration -->

    <owl:NamedIndividual rdf:about="http://linked.earth/ontology#CarbonateIonConcentration">
        <rdf:type rdf:resource="http://linked.earth/ontology#OceanChemistry"/>
        <rdfs:label xml:lang="en">Carbonate ion concentration</rdfs:label>
    </owl:NamedIndividual>
    


    <!-- http://linked.earth/ontology#ClayFraction -->

    <owl:NamedIndividual rdf:about="http://linked.earth/ontology#ClayFraction">
        <rdf:type rdf:resource="http://linked.earth/ontology#Composition"/>
        <rdfs:label xml:lang="en">Clay fraction</rdfs:label>
    </owl:NamedIndividual>
    


    <!-- http://linked.earth/ontology#Color -->

    <owl:NamedIndividual rdf:about="http://linked.earth/ontology#Color">
        <rdf:type rdf:resource="http://linked.earth/ontology#Physical"/>
        <rdfs:label xml:lang="en">Color</rdfs:label>
    </owl:NamedIndividual>
    


    <!-- http://linked.earth/ontology#Density -->

    <owl:NamedIndividual rdf:about="http://linked.earth/ontology#Density">
        <rdf:type rdf:resource="http://linked.earth/ontology#Physical"/>
        <rdfs:label xml:lang="en">Density</rdfs:label>
    </owl:NamedIndividual>
    


    <!-- http://linked.earth/ontology#DiffuseSpectralReflectance -->

    <owl:NamedIndividual rdf:about="http://linked.earth/ontology#DiffuseSpectralReflectance">
        <rdf:type rdf:resource="http://linked.earth/ontology#Reflectance"/>
        <rdfs:label xml:lang="en">Diffuse spectral reflectance</rdfs:label>
    </owl:NamedIndividual>
    


    <!-- http://linked.earth/ontology#Faunal -->

    <owl:NamedIndividual rdf:about="http://linked.earth/ontology#Faunal">
        <rdf:type rdf:resource="http://linked.earth/ontology#Assemblage"/>
        <rdfs:label xml:lang="en">Faunal</rdfs:label>
    </owl:NamedIndividual>
    


    <!-- http://linked.earth/ontology#Floral -->

    <owl:NamedIndividual rdf:about="http://linked.earth/ontology#Floral">
        <rdf:type rdf:resource="http://linked.earth/ontology#Assemblage"/>
        <rdfs:label xml:lang="en">Floral</rdfs:label>
    </owl:NamedIndividual>
    


    <!-- http://linked.earth/ontology#GrainSize -->

    <owl:NamedIndividual rdf:about="http://linked.earth/ontology#GrainSize">
        <rdf:type rdf:resource="http://linked.earth/ontology#Physical"/>
        <rdfs:label xml:lang="en">Grain size</rdfs:label>
    </owl:NamedIndividual>
    


    <!-- http://linked.earth/ontology#Historic -->

    <owl:NamedIndividual rdf:about="http://linked.earth/ontology#Historic">
        <rdf:type rdf:resource="http://linked.earth/ontology#ProxyObservation"/>
        <rdfs:label xml:lang="en">Historic</rdfs:label>
    </owl:NamedIndividual>
    


    <!-- http://linked.earth/ontology#LayerThickness -->

    <owl:NamedIndividual rdf:about="http://linked.earth/ontology#LayerThickness">
        <rdf:type rdf:resource="http://linked.earth/ontology#Physical"/>
        <rdfs:label xml:lang="en">Layer thickness</rdfs:label>
    </owl:NamedIndividual>
    


    <!-- http://linked.earth/ontology#LeadIsotope -->

    <owl:NamedIndividual rdf:about="http://linked.earth/ontology#LeadIsotope">
        <rdf:type rdf:resource="http://linked.earth/ontology#Radioisotope"/>
        <rdfs:label xml:lang="en">Lead Isotope</rdfs:label>
    </owl:NamedIndividual>
    


    <!-- http://linked.earth/ontology#Lithics -->

    <owl:NamedIndividual rdf:about="http://linked.earth/ontology#Lithics">
        <rdf:type rdf:resource="http://linked.earth/ontology#Physical"/>
        <rdfs:label xml:lang="en">Lithics</rdfs:label>
    </owl:NamedIndividual>
    


    <!-- http://linked.earth/ontology#Luminescence -->

    <owl:NamedIndividual rdf:about="http://linked.earth/ontology#Luminescence">
        <rdf:type rdf:resource="http://linked.earth/ontology#Spectral"/>
        <rdfs:label xml:lang="en">Luminescence</rdfs:label>
    </owl:NamedIndividual>
    


    <!-- http://linked.earth/ontology#MagneticSusceptibility -->

    <owl:NamedIndividual rdf:about="http://linked.earth/ontology#MagneticSusceptibility">
        <rdf:type rdf:resource="http://linked.earth/ontology#Physical"/>
        <rdfs:label xml:lang="en">Magnetic susceptibility
</rdfs:label>
    </owl:NamedIndividual>
    


    <!-- http://linked.earth/ontology#MineralMatter -->

    <owl:NamedIndividual rdf:about="http://linked.earth/ontology#MineralMatter">
        <rdf:type rdf:resource="http://linked.earth/ontology#Chemical"/>
        <rdfs:label xml:lang="en">Mineral matter</rdfs:label>
    </owl:NamedIndividual>
    


    <!-- http://linked.earth/ontology#MoistureContent -->

    <owl:NamedIndividual rdf:about="http://linked.earth/ontology#MoistureContent">
        <rdf:type rdf:resource="http://linked.earth/ontology#Physical"/>
        <rdfs:label xml:lang="en">Moisture Content</rdfs:label>
    </owl:NamedIndividual>
    


    <!-- http://linked.earth/ontology#N -->

    <owl:NamedIndividual rdf:about="http://linked.earth/ontology#N">
        <rdf:type rdf:resource="http://linked.earth/ontology#MajorElement"/>
        <rdfs:label xml:lang="en">N</rdfs:label>
    </owl:NamedIndividual>
    


    <!-- http://linked.earth/ontology#Neodymium -->

    <owl:NamedIndividual rdf:about="http://linked.earth/ontology#Neodymium">
        <rdf:type rdf:resource="http://linked.earth/ontology#Radioisotope"/>
        <rdfs:label xml:lang="en">Neodymium</rdfs:label>
    </owl:NamedIndividual>
    


    <!-- http://linked.earth/ontology#Nino1Plus2 -->

    <owl:NamedIndividual rdf:about="http://linked.earth/ontology#Nino1Plus2">
        <rdf:type rdf:resource="http://linked.earth/ontology#ElNinoIndex"/>
        <rdfs:label xml:lang="en">Nino 1+2</rdfs:label>
    </owl:NamedIndividual>
    


    <!-- http://linked.earth/ontology#OrganicMatter -->

    <owl:NamedIndividual rdf:about="http://linked.earth/ontology#OrganicMatter">
        <rdf:type rdf:resource="http://linked.earth/ontology#Chemical"/>
        <rdfs:label xml:lang="en">Organic matter</rdfs:label>
    </owl:NamedIndividual>
    


    <!-- http://linked.earth/ontology#P -->

    <owl:NamedIndividual rdf:about="http://linked.earth/ontology#P">
        <rdf:type rdf:resource="http://linked.earth/ontology#MajorElement"/>
        <rdfs:label xml:lang="en">P</rdfs:label>
    </owl:NamedIndividual>
    


    <!-- http://linked.earth/ontology#Permeability -->

    <owl:NamedIndividual rdf:about="http://linked.earth/ontology#Permeability">
        <rdf:type rdf:resource="http://linked.earth/ontology#Physical"/>
        <rdfs:label xml:lang="en">Permeability</rdfs:label>
    </owl:NamedIndividual>
    


    <!-- http://linked.earth/ontology#Porosity -->

    <owl:NamedIndividual rdf:about="http://linked.earth/ontology#Porosity">
        <rdf:type rdf:resource="http://linked.earth/ontology#Physical"/>
        <rdfs:label xml:lang="en">Porosity</rdfs:label>
    </owl:NamedIndividual>
    


    <!-- http://linked.earth/ontology#Radiocarbon -->

    <owl:NamedIndividual rdf:about="http://linked.earth/ontology#Radiocarbon">
        <rdf:type rdf:resource="http://linked.earth/ontology#Radioisotope"/>
        <rdfs:label xml:lang="en">Radiocarbon</rdfs:label>
    </owl:NamedIndividual>
    


    <!-- http://linked.earth/ontology#Resistivity -->

    <owl:NamedIndividual rdf:about="http://linked.earth/ontology#Resistivity">
        <rdf:type rdf:resource="http://linked.earth/ontology#Physical"/>
        <rdfs:label xml:lang="en">Resistivity</rdfs:label>
    </owl:NamedIndividual>
    


    <!-- http://linked.earth/ontology#SandFraction -->

    <owl:NamedIndividual rdf:about="http://linked.earth/ontology#SandFraction">
        <rdf:type rdf:resource="http://linked.earth/ontology#Composition"/>
        <rdfs:label xml:lang="en">Sand fraction
</rdfs:label>
    </owl:NamedIndividual>
    


    <!-- http://linked.earth/ontology#Si -->

    <owl:NamedIndividual rdf:about="http://linked.earth/ontology#Si">
        <rdf:type rdf:resource="http://linked.earth/ontology#MajorElement"/>
        <rdfs:label xml:lang="en">Si</rdfs:label>
    </owl:NamedIndividual>
    


    <!-- http://linked.earth/ontology#SiltFraction -->

    <owl:NamedIndividual rdf:about="http://linked.earth/ontology#SiltFraction">
        <rdf:type rdf:resource="http://linked.earth/ontology#Composition"/>
        <rdfs:label xml:lang="en">Silt fraction</rdfs:label>
    </owl:NamedIndividual>
    


    <!-- http://linked.earth/ontology#TEX86 -->

    <owl:NamedIndividual rdf:about="http://linked.earth/ontology#TEX86">
        <rdf:type rdf:resource="http://linked.earth/ontology#OrganicIndex"/>
        <rdfs:comment xml:lang="en">The use of TEX86 (TetraEther indeX of 86 carbons) as a tool to reconstruct past sea surface temperature variability is based on the relative cyclization of isoprenoidal glycerol dialkyl glycerol tetra ethers (GDGTs) produced by marine archaea. TEX86 is defined as [1]:

TEX_{86}=\frac{GDGT-2+GDGT-3+Cren&apos;}{GDGT-1+GDGT-2+GDGT-3+Cren&apos;}

where GDGTs 1-3 indicate compounds containing 1-3 cyclopentyl moieties, respectively, and Cren&apos; denotes the regioisomer of crenarchaeol, a diagnostic biomarker for the Thaumarchaeota, the primary producers of GDGTs in the marine realm. By definition, values of the TEX86 index are comprised between 0 and 1.

Experimental evidence suggests that archaea produce GDGTs with more rings warmer waters, a response observed in cultures of hyperthermophile archaea [2] [3] and mesocosm experiments with natural seawater containing heterogenous archaeal population [4] [5].
References

[1] Schouten, S., Hopmans, E. C., Schefu, E., &amp; Sinninghe Damst, J. S. (2002). Distributional variations in marine crenarchaeotal membrane lipids: a new organic proxy for reconstructing ancient sea water temperatures? . Earth and Planetary Science Letters, 204, 265-274.

[2] de Rosa, M., Esposito, E., Gambacorta, A., Nicolaus, B., &amp; Bu&apos;Lock, J. (1980). Effects of temperature on ether lipid composition of Caldariella acidophilia. Phytochemistry, 19, 827-831.

[3] Uda, I., Sugai, A., Itoh, Y., &amp; Itoh, T. (2001). Variation in molecular species of polar liipds from Thermoplasma acidophilum depends on growth temperature. Lipids, 36, 103-105.

[4] Wuchter, C., Schouten, S., Coolen, M. J. L., &amp; Sinninghe Damst, J. S. (2004). Temperature-dependent variation in the distribution of tetraether membrane lipids of marine Crenarchaeota: implications for TEX86 paleothermometry. Paleoceanography, 19, PA4028. doi:10.1029/2004PA001041

[5]Schouten, S., Forster, A., Panato, E., &amp; Sinninghe Damst, J. S. (2007). Towards the calibration of the TEX86 paleothermometer on ancient greenhouse worlds. Organic Geochemistry. doi:10.1016/j.orggeochem.2007.05.014</rdfs:comment>
        <rdfs:label xml:lang="en">TEX86</rdfs:label>
    </owl:NamedIndividual>
    


    <!-- http://linked.earth/ontology#U-Th -->

    <owl:NamedIndividual rdf:about="http://linked.earth/ontology#U-Th">
        <rdf:type rdf:resource="http://linked.earth/ontology#Radioisotope"/>
        <rdfs:label xml:lang="en">U-Th</rdfs:label>
    </owl:NamedIndividual>
    


    <!-- http://linked.earth/ontology#Uk37 -->

    <owl:NamedIndividual rdf:about="http://linked.earth/ontology#Uk37">
        <rdf:type rdf:resource="http://linked.earth/ontology#OrganicIndex"/>
        <rdfs:comment xml:lang="en">The C37 alkenone unsaturation index ( U_{37}^{k&apos;} ) is a firmly established tool for past sea surface temperatures reconstruction and is based on the relative abundance of di- (C37:2) and tri- (C37:3) unsaturated ketones with 37 carbon atoms. The index varies between 0 and 1, thus it may saturate in the temperature extremes as it becomes more challenging to determine since C37:3 and C37:2 alkenones approach their detection limits. Since alkenones come exclusively from a few species of haptophyte algae which require sunlight, alkenone thermometry offers the advantage of direct estimate of near-surface ocean temperatures. The ubiquitous presence of alkenone-synthesizing organisms (most commonly the coccolithophorids Emiliania huxleyi and Gephyrocapsa oceanic through the world&apos;s ocean and the rapidity and high-precision of the alkenone analyses had made U_{37}^{k&apos;} a valuable proxy for paleoceanographic reconstructions.

However, the U_{37}^{k&apos;} proxy is subject to non-temperature effects, such as lateral transport through oceanic currents (Ohkouchi et al. (2002)) and preferential post-depositional oxidation of C37:3 compared to C37:2 [1] [2]. Furthermore, changes in the seasonality of the proxy (i.e., which part of the seasonal cycle the proxy is recording) may bias the inferred temperatures toward winter or summer conditions [3]. Finally in oceanic regions where the photic zone extends below the surface mixed layer, the sedimentary signal may not strictly represent sea surface temperatures but rather a composite temperature of the mixed layer and the thermocline [4][5].
References

[1] Hoefs, M. J. L., Versteegh, G. J. M., Rijpstra, W. I. C., de Leeuw, J. W., &amp; Damst, J. S. S. (1998). Postdepositional oxic degradation of alkenones: Implications for the measurement of palaeo sea surface temperatures. Paleoceanography, 13(1), 42-49. doi:10.1029/97pa02893

[2] Ohkouchi, N., Eglinton, T. I., Keigwin, L. D., &amp; Hayes, J. M. (2002). Spatial and temporal offsets between proxy records in a sediment drift. Science, 298(5596), 1224-1227. doi:10.1126/science.1075287

[3] Herfort, L., Schouten, S., Boon, J. P., &amp; Sinninghe Damst, J. S. (2006). Application of the TEX86 temperature proxy in the southern North Sea. Organic Geochemistry, 37, 1715-1726.

[4] Mller, P. J., Kirst, G., Ruhland, G., von Storch, I., &amp; Rosell-Mel, A. (1998). Calibration of the alkenone paleotemperature index U_{37}^{k&apos;} based on core-tops from the eastern South Atlantic and the global ocean (60N-60S). Geochimica et cosmochimica acta, 62, 1757-1772.

[5] Prahl, F. G., Mix, A. C., &amp; Sparrow, M. A. (2006). Alkenone paleothermometry: biological lessons from amrine sediment records off Western South America. Geochimica and Cosmochimica Acta, 70, 101-117.</rdfs:comment>
        <rdfs:label xml:lang="en">Uk37</rdfs:label>
    </owl:NamedIndividual>
    


    <!-- http://linked.earth/ontology#Uk37Prime -->

    <owl:NamedIndividual rdf:about="http://linked.earth/ontology#Uk37Prime">
        <rdf:type rdf:resource="http://linked.earth/ontology#OrganicIndex"/>
        <rdfs:comment xml:lang="en">The currently accepted U37kprime (Prahl and Wakeman, 1987) varies positively with temperature, and is defines as C(37:2)/(C(37:2)+C(37:3), where C(37:2) represents the quantity of the di-unsaturated ketone and C(37:3) the quantity of the tri-unsaturated form.

Herbet, T.D., 2003, Alkenone paleotemperature determinations in Treatise on Geochemistry, Volume 6, pp 391-432</rdfs:comment>
        <rdfs:label xml:lang="en">Uk 37&apos;</rdfs:label>
    </owl:NamedIndividual>
    


    <!-- http://linked.earth/ontology#X-RayDiffraction -->

    <owl:NamedIndividual rdf:about="http://linked.earth/ontology#X-RayDiffraction">
        <rdf:type rdf:resource="http://linked.earth/ontology#Diffraction"/>
        <rdfs:label xml:lang="en">X-Ray diffraction</rdfs:label>
    </owl:NamedIndividual>
    


    <!-- http://linked.earth/ontology#X-rayFluorescence -->

    <owl:NamedIndividual rdf:about="http://linked.earth/ontology#X-rayFluorescence">
        <rdf:type rdf:resource="http://linked.earth/ontology#Fluorescence"/>
        <rdfs:label xml:lang="en">X-ray fluorescence</rdfs:label>
    </owl:NamedIndividual>
    


    <!-- http://linked.earth/ontology#age -->

    <owl:NamedIndividual rdf:about="http://linked.earth/ontology#age">
        <rdf:type rdf:resource="http://linked.earth/ontology#Time"/>
        <rdfs:comment xml:lang="en">The age of a sample</rdfs:comment>
        <rdfs:label xml:lang="en">Age</rdfs:label>
    </owl:NamedIndividual>
    


    <!-- http://linked.earth/ontology#arcticOscillation -->

    <owl:NamedIndividual rdf:about="http://linked.earth/ontology#arcticOscillation">
        <rdf:type rdf:resource="http://linked.earth/ontology#ClimateIndex"/>
        <rdfs:label xml:lang="en">Arctic Oscillation (AO, AAO)</rdfs:label>
    </owl:NamedIndividual>
    


    <!-- http://linked.earth/ontology#atlanticMultiDecadalOscillation -->

    <owl:NamedIndividual rdf:about="http://linked.earth/ontology#atlanticMultiDecadalOscillation">
        <rdf:type rdf:resource="http://linked.earth/ontology#ClimateIndex"/>
        <rdfs:label xml:lang="en">Atlantic Multi-decadal Oscillation (AMO)</rdfs:label>
    </owl:NamedIndividual>
    


    <!-- http://linked.earth/ontology#bottomWaterTemperature -->

    <owl:NamedIndividual rdf:about="http://linked.earth/ontology#bottomWaterTemperature">
        <rdf:type rdf:resource="http://linked.earth/ontology#Temperature"/>
        <rdfs:label xml:lang="en">Bottom water temperature</rdfs:label>
    </owl:NamedIndividual>
    


    <!-- http://linked.earth/ontology#carbonDioxideConcentration -->

    <owl:NamedIndividual rdf:about="http://linked.earth/ontology#carbonDioxideConcentration">
        <rdf:type rdf:resource="http://linked.earth/ontology#AtmosphericChemistry"/>
        <rdfs:label xml:lang="en">Carbon dioxide concentration</rdfs:label>
    </owl:NamedIndividual>
    


    <!-- http://linked.earth/ontology#carbonateSaturation -->

    <owl:NamedIndividual rdf:about="http://linked.earth/ontology#carbonateSaturation">
        <rdf:type rdf:resource="http://linked.earth/ontology#OceanChemistry"/>
        <rdfs:label xml:lang="en">Carbonate saturation</rdfs:label>
    </owl:NamedIndividual>
    


    <!-- http://linked.earth/ontology#coral -->

    <owl:NamedIndividual rdf:about="http://linked.earth/ontology#coral">
        <rdf:type rdf:resource="http://linked.earth/ontology#Coral"/>
        <rdfs:label xml:lang="en">Coral</rdfs:label>
    </owl:NamedIndividual>
    


    <!-- http://linked.earth/ontology#d13C -->

    <owl:NamedIndividual rdf:about="http://linked.earth/ontology#d13C">
        <rdf:type rdf:resource="http://linked.earth/ontology#StableCarbonIsotope"/>
        <rdfs:label xml:lang="en">d13C</rdfs:label>
    </owl:NamedIndividual>
    


    <!-- http://linked.earth/ontology#d15N -->

    <owl:NamedIndividual rdf:about="http://linked.earth/ontology#d15N">
        <rdf:type rdf:resource="http://linked.earth/ontology#StableNitrogenIsotope"/>
        <rdfs:label xml:lang="en">d15N</rdfs:label>
    </owl:NamedIndividual>
    


    <!-- http://linked.earth/ontology#d170 -->

    <owl:NamedIndividual rdf:about="http://linked.earth/ontology#d170">
        <rdf:type rdf:resource="http://linked.earth/ontology#StableOxygenIsotope"/>
        <rdfs:label xml:lang="en">d170</rdfs:label>
    </owl:NamedIndividual>
    


    <!-- http://linked.earth/ontology#d180 -->

    <owl:NamedIndividual rdf:about="http://linked.earth/ontology#d180">
        <rdf:type rdf:resource="http://linked.earth/ontology#IsotopicComposition"/>
        <rdf:type rdf:resource="http://linked.earth/ontology#StableOxygenIsotope"/>
        <rdfs:comment xml:lang="en">Oxygen has three naturally-occuring stable isotopes: 16O, 17O, 18O, with 16O being the most abundant (99.762%).

Two international reference standards are used to report variations in oxygen isotope standards: PDB and SMOW. The use of the PDB standard in reporting oxygen isotope composition is restricted to carbonates of low-temperature origins (e.g., oceanic, lacustrine ). The conversion between SMOW and PDB scales is given by:
\delta^{18}O_{SMOW} = 1.03091 (\delta^{18}O_{PDB}) +30.91

18O may be measured on the shells of foraminifera</rdfs:comment>
        <rdfs:label xml:lang="en">d180</rdfs:label>
    </owl:NamedIndividual>
    


    <!-- http://linked.earth/ontology#d34S -->

    <owl:NamedIndividual rdf:about="http://linked.earth/ontology#d34S">
        <rdf:type rdf:resource="http://linked.earth/ontology#StableSulfurIsotope"/>
        <rdfs:label xml:lang="en">d34S</rdfs:label>
    </owl:NamedIndividual>
    


    <!-- http://linked.earth/ontology#dD -->

    <owl:NamedIndividual rdf:about="http://linked.earth/ontology#dD">
        <rdf:type rdf:resource="http://linked.earth/ontology#IsotopicComposition"/>
        <rdf:type rdf:resource="http://linked.earth/ontology#StableHydrogenIsotope"/>
        <rdfs:label xml:lang="en">DD</rdfs:label>
        <rdfs:label xml:lang="en">dD</rdfs:label>
    </owl:NamedIndividual>
    


    <!-- http://linked.earth/ontology#deuteriumExcess -->

    <owl:NamedIndividual rdf:about="http://linked.earth/ontology#deuteriumExcess">
        <rdf:type rdf:resource="http://linked.earth/ontology#IsotopicComposition"/>
        <rdfs:label xml:lang="en">Deuterium excess (excessD)</rdfs:label>
    </owl:NamedIndividual>
    


    <!-- http://linked.earth/ontology#document -->

    <owl:NamedIndividual rdf:about="http://linked.earth/ontology#document">
        <rdf:type rdf:resource="http://linked.earth/ontology#Document"/>
        <rdfs:label xml:lang="en">Document</rdfs:label>
    </owl:NamedIndividual>
    


    <!-- http://linked.earth/ontology#freeOxygenLevels -->

    <owl:NamedIndividual rdf:about="http://linked.earth/ontology#freeOxygenLevels">
        <rdf:type rdf:resource="http://linked.earth/ontology#AtmosphericChemistry"/>
        <rdfs:label xml:lang="en">Free oxygen levels</rdfs:label>
    </owl:NamedIndividual>
    


    <!-- http://linked.earth/ontology#glacierIce -->

    <owl:NamedIndividual rdf:about="http://linked.earth/ontology#glacierIce">
        <rdf:type rdf:resource="http://linked.earth/ontology#GlacierIce"/>
        <rdfs:label xml:lang="en">Glacier ice</rdfs:label>
    </owl:NamedIndividual>
    


    <!-- http://linked.earth/ontology#hybrid -->

    <owl:NamedIndividual rdf:about="http://linked.earth/ontology#hybrid">
        <rdf:type rdf:resource="http://linked.earth/ontology#Hybrid"/>
        <rdfs:label xml:lang="en">Hybrid</rdfs:label>
    </owl:NamedIndividual>
    


    <!-- http://linked.earth/ontology#julianDay -->

    <owl:NamedIndividual rdf:about="http://linked.earth/ontology#julianDay">
        <rdf:type rdf:resource="http://linked.earth/ontology#Time"/>
        <rdfs:label xml:lang="en">Julian day</rdfs:label>
    </owl:NamedIndividual>
    


    <!-- http://linked.earth/ontology#lakeSediment -->

    <owl:NamedIndividual rdf:about="http://linked.earth/ontology#lakeSediment">
        <rdf:type rdf:resource="http://linked.earth/ontology#LakeSediment"/>
        <rdfs:label xml:lang="en">Lake sediment</rdfs:label>
    </owl:NamedIndividual>
    


    <!-- http://linked.earth/ontology#marineSediment -->

    <owl:NamedIndividual rdf:about="http://linked.earth/ontology#marineSediment">
        <rdf:type rdf:resource="http://linked.earth/ontology#MarineSediment"/>
        <rdfs:label xml:lang="en">Marine sediment</rdfs:label>
    </owl:NamedIndividual>
    


    <!-- http://linked.earth/ontology#methaneConcentration -->

    <owl:NamedIndividual rdf:about="http://linked.earth/ontology#methaneConcentration">
        <rdf:type rdf:resource="http://linked.earth/ontology#AtmosphericChemistry"/>
        <rdfs:label xml:lang="en">Methane concentration</rdfs:label>
    </owl:NamedIndividual>
    


    <!-- http://linked.earth/ontology#moistureContent -->

    <owl:NamedIndividual rdf:about="http://linked.earth/ontology#moistureContent">
        <rdf:type rdf:resource="http://linked.earth/ontology#Hydrology"/>
        <rdfs:label xml:lang="en">Moisture content</rdfs:label>
    </owl:NamedIndividual>
    


    <!-- http://linked.earth/ontology#molluskShells -->

    <owl:NamedIndividual rdf:about="http://linked.earth/ontology#molluskShells">
        <rdf:type rdf:resource="http://linked.earth/ontology#MolluskShells"/>
        <rdfs:label xml:lang="en">Mollusk shells</rdfs:label>
    </owl:NamedIndividual>
    


    <!-- http://linked.earth/ontology#nino1 -->

    <owl:NamedIndividual rdf:about="http://linked.earth/ontology#nino1">
        <rdf:type rdf:resource="http://linked.earth/ontology#ElNinoIndex"/>
        <rdfs:label xml:lang="en">Nino 1</rdfs:label>
    </owl:NamedIndividual>
    


    <!-- http://linked.earth/ontology#nino2 -->

    <owl:NamedIndividual rdf:about="http://linked.earth/ontology#nino2">
        <rdf:type rdf:resource="http://linked.earth/ontology#ElNinoIndex"/>
        <rdfs:label xml:lang="en">Nino 2</rdfs:label>
    </owl:NamedIndividual>
    


    <!-- http://linked.earth/ontology#nino3 -->

    <owl:NamedIndividual rdf:about="http://linked.earth/ontology#nino3">
        <rdf:type rdf:resource="http://linked.earth/ontology#ElNinoIndex"/>
        <rdfs:label xml:lang="en">Nino 3</rdfs:label>
    </owl:NamedIndividual>
    


    <!-- http://linked.earth/ontology#nino3_4 -->

    <owl:NamedIndividual rdf:about="http://linked.earth/ontology#nino3_4">
        <rdf:type rdf:resource="http://linked.earth/ontology#ElNinoIndex"/>
        <rdfs:label xml:lang="en">Nino 3.4</rdfs:label>
    </owl:NamedIndividual>
    


    <!-- http://linked.earth/ontology#nino4 -->

    <owl:NamedIndividual rdf:about="http://linked.earth/ontology#nino4">
        <rdf:type rdf:resource="http://linked.earth/ontology#ElNinoIndex"/>
        <rdfs:label xml:lang="en">Nino 4</rdfs:label>
    </owl:NamedIndividual>
    


    <!-- http://linked.earth/ontology#nitrousOxideConcentration -->

    <owl:NamedIndividual rdf:about="http://linked.earth/ontology#nitrousOxideConcentration">
        <rdf:type rdf:resource="http://linked.earth/ontology#AtmosphericChemistry"/>
        <rdfs:label xml:lang="en">Nitrous oxide concentration</rdfs:label>
    </owl:NamedIndividual>
    


    <!-- http://linked.earth/ontology#northAtlanticOscillation -->

    <owl:NamedIndividual rdf:about="http://linked.earth/ontology#northAtlanticOscillation">
        <rdf:type rdf:resource="http://linked.earth/ontology#ClimateIndex"/>
        <rdfs:label xml:lang="en">North Atlantic Oscillation (NAO)</rdfs:label>
    </owl:NamedIndividual>
    


    <!-- http://linked.earth/ontology#oceanMixedLayerTemperature -->

    <owl:NamedIndividual rdf:about="http://linked.earth/ontology#oceanMixedLayerTemperature">
        <rdf:type rdf:resource="http://linked.earth/ontology#Temperature"/>
        <rdfs:label xml:lang="en">Ocean mixed layer temperature</rdfs:label>
    </owl:NamedIndividual>
    


    <!-- http://linked.earth/ontology#pH -->

    <owl:NamedIndividual rdf:about="http://linked.earth/ontology#pH">
        <rdf:type rdf:resource="http://linked.earth/ontology#OceanChemistry"/>
        <rdfs:label xml:lang="en">PH</rdfs:label>
    </owl:NamedIndividual>
    


    <!-- http://linked.earth/ontology#palmerDroughtIndex -->

    <owl:NamedIndividual rdf:about="http://linked.earth/ontology#palmerDroughtIndex">
        <rdf:type rdf:resource="http://linked.earth/ontology#ClimateIndex"/>
        <owl:sameAs rdf:resource="http://linked.earth/ontology#palmerDroughtSeverityIndex"/>
        <rdfs:label xml:lang="en">Palmer Drought Index</rdfs:label>
    </owl:NamedIndividual>
    


    <!-- http://linked.earth/ontology#palmerDroughtSeverityIndex -->

    <owl:NamedIndividual rdf:about="http://linked.earth/ontology#palmerDroughtSeverityIndex">
        <rdf:type rdf:resource="http://linked.earth/ontology#ClimateIndex"/>
        <rdf:type rdf:resource="http://linked.earth/ontology#Hydrology"/>
        <rdfs:label xml:lang="en">Palmer Drought Severity Index (PDSI)</rdfs:label>
    </owl:NamedIndividual>
    


    <!-- http://linked.earth/ontology#peat -->

    <owl:NamedIndividual rdf:about="http://linked.earth/ontology#peat">
        <rdf:type rdf:resource="http://linked.earth/ontology#Peat"/>
        <rdfs:label xml:lang="en">Peat</rdfs:label>
    </owl:NamedIndividual>
    


    <!-- http://linked.earth/ontology#precipitationAmount -->

    <owl:NamedIndividual rdf:about="http://linked.earth/ontology#precipitationAmount">
        <rdf:type rdf:resource="http://linked.earth/ontology#Precipitation"/>
        <rdfs:label xml:lang="en">Precipitation amount</rdfs:label>
    </owl:NamedIndividual>
    


    <!-- http://linked.earth/ontology#radiocarbonAge -->

    <owl:NamedIndividual rdf:about="http://linked.earth/ontology#radiocarbonAge">
        <rdf:type rdf:resource="http://linked.earth/ontology#Time"/>
        <rdfs:label xml:lang="en">Radiocarbon age</rdfs:label>
    </owl:NamedIndividual>
    


    <!-- http://linked.earth/ontology#rock -->

    <owl:NamedIndividual rdf:about="http://linked.earth/ontology#rock">
        <rdf:type rdf:resource="http://linked.earth/ontology#Rock"/>
        <rdfs:label xml:lang="en">Rock</rdfs:label>
    </owl:NamedIndividual>
    


    <!-- http://linked.earth/ontology#salinity -->

    <owl:NamedIndividual rdf:about="http://linked.earth/ontology#salinity">
        <rdf:type rdf:resource="http://linked.earth/ontology#OceanChemistry"/>
        <rdfs:label xml:lang="en">Salinity</rdfs:label>
    </owl:NamedIndividual>
    


    <!-- http://linked.earth/ontology#sclerosponge -->

    <owl:NamedIndividual rdf:about="http://linked.earth/ontology#sclerosponge">
        <rdf:type rdf:resource="http://linked.earth/ontology#Sclerosponge"/>
        <rdfs:label xml:lang="en">Sclerosponge</rdfs:label>
    </owl:NamedIndividual>
    


    <!-- http://linked.earth/ontology#seaSurfaceTemperature -->

    <owl:NamedIndividual rdf:about="http://linked.earth/ontology#seaSurfaceTemperature">
        <rdf:type rdf:resource="http://linked.earth/ontology#Temperature"/>
        <rdfs:comment xml:lang="en">The temperature close to the ocean&apos;s surface</rdfs:comment>
        <rdfs:label xml:lang="en">Sea surface temperature</rdfs:label>
    </owl:NamedIndividual>
    


    <!-- http://linked.earth/ontology#southernAnnularMode -->

    <owl:NamedIndividual rdf:about="http://linked.earth/ontology#southernAnnularMode">
        <rdf:type rdf:resource="http://linked.earth/ontology#ClimateIndex"/>
        <rdfs:label xml:lang="en">Southern Annular Mode (SAM)</rdfs:label>
    </owl:NamedIndividual>
    


    <!-- http://linked.earth/ontology#southernOscillationIndex -->

    <owl:NamedIndividual rdf:about="http://linked.earth/ontology#southernOscillationIndex">
        <rdf:type rdf:resource="http://linked.earth/ontology#ElNinoIndex"/>
        <rdfs:label xml:lang="en">Southern oscillation index (SOI)</rdfs:label>
    </owl:NamedIndividual>
    


    <!-- http://linked.earth/ontology#speleothem -->

    <owl:NamedIndividual rdf:about="http://linked.earth/ontology#speleothem">
        <rdf:type rdf:resource="http://linked.earth/ontology#Speleothem"/>
        <rdfs:label xml:lang="en">Speleothem</rdfs:label>
    </owl:NamedIndividual>
    


    <!-- http://linked.earth/ontology#surfaceAirTemperature -->

    <owl:NamedIndividual rdf:about="http://linked.earth/ontology#surfaceAirTemperature">
        <rdf:type rdf:resource="http://linked.earth/ontology#Temperature"/>
        <rdfs:label xml:lang="en">Surface air temperature</rdfs:label>
    </owl:NamedIndividual>
    


    <!-- http://linked.earth/ontology#temperature -->

    <owl:NamedIndividual rdf:about="http://linked.earth/ontology#temperature">
        <rdf:type rdf:resource="http://linked.earth/ontology#Temperature"/>
        <rdfs:comment xml:lang="en">Thermodynamic property which quantifies how cold or warm an object, a fluid, or a substance is.</rdfs:comment>
        <rdfs:label xml:lang="en">Temperature</rdfs:label>
    </owl:NamedIndividual>
    


    <!-- http://linked.earth/ontology#wood -->

    <owl:NamedIndividual rdf:about="http://linked.earth/ontology#wood">
        <rdf:type rdf:resource="http://linked.earth/ontology#Wood"/>
        <rdfs:label xml:lang="en">Wood</rdfs:label>
    </owl:NamedIndividual>
    


    <!-- http://linked.earth/ontology#year -->

    <owl:NamedIndividual rdf:about="http://linked.earth/ontology#year">
        <rdf:type rdf:resource="http://linked.earth/ontology#Time"/>
        <rdfs:label xml:lang="en">Year</rdfs:label>
    </owl:NamedIndividual>
    


    <!-- http://linked.earth/ontology#Al/Ca -->

    <owl:NamedIndividual rdf:about="http://linked.earth/ontology#Al/Ca">
        <rdf:type rdf:resource="http://linked.earth/ontology#TraceElement"/>
        <rdfs:label xml:lang="en">Al/Ca</rdfs:label>
    </owl:NamedIndividual>
    


    <!-- http://linked.earth/ontology#B/Ca -->

    <owl:NamedIndividual rdf:about="http://linked.earth/ontology#B/Ca">
        <rdf:type rdf:resource="http://linked.earth/ontology#TraceElement"/>
        <rdfs:label xml:lang="en">B/Ca</rdfs:label>
    </owl:NamedIndividual>
    


    <!-- http://linked.earth/ontology#Ba/Ca -->

    <owl:NamedIndividual rdf:about="http://linked.earth/ontology#Ba/Ca">
        <rdf:type rdf:resource="http://linked.earth/ontology#TraceElement"/>
        <rdfs:label xml:lang="en">Ba/Ca</rdfs:label>
    </owl:NamedIndividual>
    


    <!-- http://linked.earth/ontology#Fe/Ca -->

    <owl:NamedIndividual rdf:about="http://linked.earth/ontology#Fe/Ca">
        <rdf:type rdf:resource="http://linked.earth/ontology#TraceElement"/>
        <rdfs:label xml:lang="en">Fe/Ca</rdfs:label>
    </owl:NamedIndividual>
    


    <!-- http://linked.earth/ontology#Li/Ca -->

    <owl:NamedIndividual rdf:about="http://linked.earth/ontology#Li/Ca">
        <rdf:type rdf:resource="http://linked.earth/ontology#TraceElement"/>
        <rdfs:label xml:lang="en">Li/Ca</rdfs:label>
    </owl:NamedIndividual>
    


    <!-- http://linked.earth/ontology#Mg/Ca -->

    <owl:NamedIndividual rdf:about="http://linked.earth/ontology#Mg/Ca">
        <rdf:type rdf:resource="http://linked.earth/ontology#TraceElement"/>
        <rdfs:label xml:lang="en">Mg/Ca</rdfs:label>
    </owl:NamedIndividual>
    


    <!-- http://linked.earth/ontology#Mn/Ca -->

    <owl:NamedIndividual rdf:about="http://linked.earth/ontology#Mn/Ca">
        <rdf:type rdf:resource="http://linked.earth/ontology#TraceElement"/>
        <rdfs:label xml:lang="en">Mn/Ca</rdfs:label>
    </owl:NamedIndividual>
    


    <!-- http://linked.earth/ontology#Sr/Ca -->

    <owl:NamedIndividual rdf:about="http://linked.earth/ontology#Sr/Ca">
        <rdf:type rdf:resource="http://linked.earth/ontology#TraceElement"/>
        <rdfs:label xml:lang="en">Sr/Ca</rdfs:label>
    </owl:NamedIndividual>
    


    <!-- http://linked.earth/ontology#Zn/Ca -->

    <owl:NamedIndividual rdf:about="http://linked.earth/ontology#Zn/Ca">
        <rdf:type rdf:resource="http://linked.earth/ontology#TraceElement"/>
        <rdfs:label xml:lang="en">Zn/Ca</rdfs:label>
    </owl:NamedIndividual>
    


    <!-- http://orcid.org/0000-0001-5920-4751 -->

    <owl:NamedIndividual rdf:about="http://orcid.org/0000-0001-5920-4751"/>
    


    <!-- http://w3id.org/people/dgarijo -->

    <owl:NamedIndividual rdf:about="http://w3id.org/people/dgarijo"/>
    


    <!-- http://www.cefns.nau.edu/~npm4/ -->

    <owl:NamedIndividual rdf:about="http://www.cefns.nau.edu/~npm4/"/>
    


    <!-- http://www.isi.edu/~gil/ -->

    <owl:NamedIndividual rdf:about="http://www.isi.edu/~gil/"/>
    


    <!-- 
    ///////////////////////////////////////////////////////////////////////////////////////
    //
    // Annotations
    //
    ///////////////////////////////////////////////////////////////////////////////////////
     -->

    <rdf:Description rdf:about="http://purl.org/dc/terms/license">
        <rdfs:isDefinedBy rdf:resource="http://purl.org/dc/terms/"/>
    </rdf:Description>
</rdf:RDF>



<!-- Generated by the OWL API (version 4.2.5.20160517-0735) https://github.com/owlcs/owlapi -->

